# baseURI: http://anzsoil.org/def/au/scma/
# imports: http://purl.org/dc/elements/1.1/

@prefix dc: <http://purl.org/dc/elements/1.1/> .
@prefix dcat: <http://www.w3.org/ns/dcat#> .
@prefix dct: <http://purl.org/dc/terms/> .
@prefix euvoc: <http://publications.europa.eu/ontology/euvoc#> .
@prefix foaf: <http://xmlns.com/foaf/0.1/> .
@prefix org: <http://www.w3.org/ns/org#> .
@prefix owl: <http://www.w3.org/2002/07/owl#> .
@prefix prov: <http://www.w3.org/ns/prov#> .
@prefix qb: <http://purl.org/linked-data/cube#> .
@prefix rdf: <http://www.w3.org/1999/02/22-rdf-syntax-ns#> .
@prefix rdfs: <http://www.w3.org/2000/01/rdf-schema#> .
@prefix s: <http://anzsoil.org/def/au/scma/> .
@prefix schema: <http://schema.org/> .
@prefix sdo: <https://schema.org/> .
@prefix sh: <http://www.w3.org/ns/shacl#> .
@prefix skos: <http://www.w3.org/2004/02/skos/core#> .
@prefix skosthes: <http://purl.org/iso25964/skos-thes#> .
@prefix skosxl: <http://www.w3.org/2008/05/skos-xl#> .
@prefix sosa: <http://www.w3.org/ns/sosa/> .
@prefix xsd: <http://www.w3.org/2001/XMLSchema#> .

s:scma-2011 a skos:ConceptScheme , owl:Ontology ;
  owl:imports dc: ;
  dct:accrualPeriodicity <http://purl.org/cld/freq/irregular>;
  dct:contributor <https://orcid.org/0000-0002-2991-2308>, <https://orcid.org/0000-0002-3884-3420>;
  dct:created "2021-01-01"^^xsd:date;
  dct:description "<p>This Concept Scheme is a machine-readable representation of the classifiers described in <a href='https://catalogue.nla.gov.au/Record/4854518'>Soil Chemical Methods Australasia</a> 1. (2011), by George E Rayment and David J Lyons. These comprise the laboratory and field chemical tests relevant to Australasia and beyond. </p> <p>Supersedes <a href='https://catalogue.nla.gov.au/Record/685915'>Australian Laboratory Handbook of Soil and Water Chemical Methods</a> (Rayment and Higginson 1992) while retaining method codes and other strengths of that Handbook. This register includes the method codes from Rayment and Higginson (1992) that were made redundant or superseded by new codes in George E Rayment and David J Lyons (2011).</p>"^^rdf:HTML;
  dct:identifier "http://anzsoil.org/def/au/scma/scma-2011"^^xsd:anyURI;
  dct:license <https://creativecommons.org/publicdomain/zero/1.0/>;
  dct:modified "2022-03-04"^^xsd:date;
  dct:replaces s:swcm-1992;
  dct:source <https://catalogue.nla.gov.au/Record/4854518>;
  dct:title "Soil chemical methods - Australasia";
  skos:hasTopConcept s:02A1, s:02B1, s:02C1, s:02D1, s:03A1, s:03B1, s:03C1, s:03D1,
    s:04A1, s:04A2, s:04A3, s:04B1, s:04B2, s:04B3, s:04B4, s:04B5, s:04C1, s:04C2, s:04C3,
    s:04C4, s:04D1, s:04E1, s:04F1, s:04G1, s:05A1, s:05A2, s:05A3a, s:05A3b, s:05A4,
    s:06A1, s:06B1, s:06B2, s:06B3, s:06B4, s:06C1, s:06D1, s:06E1, s:06F1, s:06G1, s:07A1,
    s:07A2, s:07A3, s:07A4, s:07A5, s:07A6, s:07B, s:07C1, s:07C2, s:07D, s:08A1, s:08B1,
    s:09A, s:09B, s:09C, s:09D1, s:09E, s:09F1, s:09F2, s:09G1, s:09G2, s:09H1, s:09I,
    s:09J, s:09K, s:10A1, s:10A2, s:10B, s:10C1, s:10D1, s:11A1, s:11A2, s:12A1, s:12B1,
    s:12C1, s:12C2, s:12D1, s:12E1, s:13A1, s:13B1, s:13C1, s:13D, s:14A1, s:14A2, s:14A3,
    s:14A4, s:14B1, s:14C1, s:14D1, s:14D2, s:14E1, s:14E2, s:14E3, s:14F1, s:14F2, s:14F3,
    s:14F4, s:14F5, s:14G1, s:14G2, s:14H1, s:15A1, s:15A2, s:15A3, s:15B1, s:15B2, s:15B3,
    s:15C1, s:15C2, s:15D1, s:15D2, s:15D3, s:15E1, s:15E2, s:15E3, s:15F1, s:15F2, s:15F3,
    s:15G1, s:15H1, s:15I1, s:15I2, s:15I3, s:15I4, s:15J1, s:15K1, s:15L1, s:15M1, s:15N1,
    s:15O1, s:16A1, s:16B1, s:16C1, s:16D1, s:17A1, s:17A2, s:17B1, s:17B2, s:17C1, s:18A1,
    s:18B1, s:18C1, s:18D1, s:18E1, s:18F, s:18G1, s:19A1, s:19B, s:19C1, s:19D1, s:20A1,
    s:20B1, s:20C1, s:20D1, s:20E1, s:20F1, s:20F2, s:20G1, s:20H1, s:20I1, s:20J1, s:20K1;
  sdo:codeRepository <https://github.com/ANZSoilData/def-au-scma> .

s:02 a skos:Collection;
  dct:identifier "http://anzsoil.org/def/au/scma/02"^^xsd:anyURI;
  dct:source "URN:ISBN:978-0-643-10218-7";
  skos:definition <https://raw.githack.com/ANZSoilData/def-au-scma/master/html/02/02.html>;
  skos:inScheme s:scma-2011;
  skos:member s:02A1, s:02B1, s:02C1, s:02D1;
  skos:notation "02";
  skos:prefLabel "Sampling, preparation and moisture content" .

s:02A1 a skos:Concept, sosa:Procedure;
  dct:identifier "http://anzsoil.org/def/au/scma/02A1"^^xsd:anyURI;
  dct:source "URN:ISBN:978-0-643-10218-7";
  skos:definition <https://raw.githack.com/ANZSoilData/def-au-scma/master/html/02/02A1.html>;
  skos:inScheme s:scma-2011;
  skos:notation "02A1";
  skos:prefLabel "Air-dry moisture content";
  skos:topConceptOf s:scma-2011 .

s:02B1 a skos:Concept, sosa:Procedure;
  dct:identifier "http://anzsoil.org/def/au/scma/02B1"^^xsd:anyURI;
  dct:source "URN:ISBN:978-0-643-10218-7";
  skos:definition <https://raw.githack.com/ANZSoilData/def-au-scma/master/html/02/02B1.html>;
  skos:inScheme s:scma-2011;
  skos:notation "02B1";
  skos:prefLabel "As received moisture content";
  skos:topConceptOf s:scma-2011 .

s:02C1 a skos:Concept, sosa:Procedure;
  dct:identifier "http://anzsoil.org/def/au/scma/02C1"^^xsd:anyURI;
  dct:source "URN:ISBN:978-0-643-10218-7";
  skos:definition <https://raw.githack.com/ANZSoilData/def-au-scma/master/html/02/02C1.html>;
  skos:inScheme s:scma-2011;
  skos:notation "02C1";
  skos:prefLabel "Moisture content - 10 mm tension";
  skos:topConceptOf s:scma-2011 .

s:02D1 a skos:Concept, sosa:Procedure;
  dct:identifier "http://anzsoil.org/def/au/scma/02D1"^^xsd:anyURI;
  dct:source "URN:ISBN:978-0-643-10218-7";
  skos:definition <https://raw.githack.com/ANZSoilData/def-au-scma/master/html/02/02D1.html>;
  skos:inScheme s:scma-2011;
  skos:notation "02D1";
  skos:prefLabel "Moisture content - approximate saturation paste";
  skos:topConceptOf s:scma-2011 .

s:03 a skos:Collection;
  dct:identifier "http://anzsoil.org/def/au/scma/03"^^xsd:anyURI;
  dct:source "URN:ISBN:978-0-643-10218-7";
  skos:definition <https://raw.githack.com/ANZSoilData/def-au-scma/master/html/03/03.html>;
  skos:inScheme s:scma-2011;
  skos:member s:03A1, s:03B1, s:03C1, s:03D1;
  skos:notation "03";
  skos:prefLabel "Electrical conductivity, related attributes and redox potential" .

s:03A1 a skos:Concept, sosa:Procedure;
  dct:identifier "http://anzsoil.org/def/au/scma/03A1"^^xsd:anyURI;
  dct:source "URN:ISBN:978-0-643-10218-7";
  skos:definition <https://raw.githack.com/ANZSoilData/def-au-scma/master/html/03/03A1.html>;
  skos:inScheme s:scma-2011;
  skos:notation "03A1";
  skos:prefLabel "Electrical conductivity (EC) of 1:5 soil/water extract";
  skos:topConceptOf s:scma-2011 .

s:03B1 a skos:Concept, sosa:Procedure;
  dct:identifier "http://anzsoil.org/def/au/scma/03B1"^^xsd:anyURI;
  dct:source "URN:ISBN:978-0-643-10218-7";
  skos:definition <https://raw.githack.com/ANZSoilData/def-au-scma/master/html/03/03B1.html>;
  skos:inScheme s:scma-2011;
  skos:notation "03B1";
  skos:prefLabel "Estimated soluble salt concentration";
  skos:topConceptOf s:scma-2011 .

s:03C1 a skos:Concept, sosa:Procedure;
  dct:identifier "http://anzsoil.org/def/au/scma/03C1"^^xsd:anyURI;
  dct:source "URN:ISBN:978-0-643-10218-7";
  skos:definition <https://raw.githack.com/ANZSoilData/def-au-scma/master/html/03/03C1.html>;
  skos:inScheme s:scma-2011;
  skos:notation "03C1";
  skos:prefLabel "Estimated soil ionic strength";
  skos:topConceptOf s:scma-2011 .

s:03D1 a skos:Concept, sosa:Procedure;
  dct:identifier "http://anzsoil.org/def/au/scma/03D1"^^xsd:anyURI;
  dct:source "URN:ISBN:978-0-643-10218-7";
  skos:definition <https://raw.githack.com/ANZSoilData/def-au-scma/master/html/03/03D1.html>;
  skos:inScheme s:scma-2011;
  skos:notation "03D1";
  skos:prefLabel "Redox potential (Eh; field)";
  skos:topConceptOf s:scma-2011 .

s:04 a skos:Collection;
  dct:identifier "http://anzsoil.org/def/au/scma/04"^^xsd:anyURI;
  dct:source "URN:ISBN:978-0-643-10218-7";
  skos:definition <https://raw.githack.com/ANZSoilData/def-au-scma/master/html/04-pH/04.html>;
  skos:inScheme s:scma-2011;
  skos:member s:04A1, s:04A2, s:04A3, s:04B1, s:04B2, s:04B3, s:04B4, s:04B5, s:04C1,
    s:04C2, s:04C3, s:04C4, s:04D1, s:04E1, s:04F1, s:04G1;
  skos:notation "04";
  skos:prefLabel "Soil pH" .

s:04A1 a skos:Concept, sosa:Procedure;
  dct:identifier "http://anzsoil.org/def/au/scma/04A1"^^xsd:anyURI;
  dct:source "URN:ISBN:978-0-643-10218-7";
  skos:definition <https://raw.githack.com/ANZSoilData/def-au-scma/master/html/04-pH/04A1.html>;
  skos:inScheme s:scma-2011;
  skos:notation "04A1";
  skos:prefLabel "pH of a 1:5 soil/water suspension";
  skos:topConceptOf s:scma-2011 .

s:04A2 a skos:Concept, sosa:Procedure;
  dct:identifier "http://anzsoil.org/def/au/scma/04A2"^^xsd:anyURI;
  dct:source "URN:ISBN:978-0-643-10218-7";
  skos:definition <https://raw.githack.com/ANZSoilData/def-au-scma/master/html/04-pH/04A2.html>;
  skos:inScheme s:scma-2011;
  skos:notation "04A2";
  skos:prefLabel "pH of a 1:1 soil/water suspension";
  skos:topConceptOf s:scma-2011 .

s:04A3 a skos:Concept, sosa:Procedure;
  dct:identifier "http://anzsoil.org/def/au/scma/04A3"^^xsd:anyURI;
  dct:source "URN:ISBN:978-0-643-10218-7";
  skos:definition <https://raw.githack.com/ANZSoilData/def-au-scma/master/html/04-pH/04A3.html>;
  skos:inScheme s:scma-2011;
  skos:notation "04A3";
  skos:prefLabel "pH of a 1:2.5 soil/water suspension";
  skos:topConceptOf s:scma-2011 .

s:04B1 a skos:Concept, sosa:Procedure;
  dct:identifier "http://anzsoil.org/def/au/scma/04B1"^^xsd:anyURI;
  dct:source "URN:ISBN:978-0-643-10218-7";
  skos:definition <https://raw.githack.com/ANZSoilData/def-au-scma/master/html/04-pH/04B1.html>;
  skos:inScheme s:scma-2011;
  skos:notation "04B1";
  skos:prefLabel "pH of 1:5 soil/0.01 M calcium chloride extract - direct (without stirring during measurement)";
  skos:topConceptOf s:scma-2011 .

s:04B2 a skos:Concept, sosa:Procedure;
  dct:identifier "http://anzsoil.org/def/au/scma/04B2"^^xsd:anyURI;
  dct:source "URN:ISBN:978-0-643-10218-7";
  skos:definition <https://raw.githack.com/ANZSoilData/def-au-scma/master/html/04-pH/04B2.html>;
  skos:inScheme s:scma-2011;
  skos:notation "04B2";
  skos:prefLabel "pH of 1:5 soil/0.01 M calcium chloride extract - following method 4A1 (without stirring during measurement)";
  skos:topConceptOf s:scma-2011 .

s:04B3 a skos:Concept, sosa:Procedure;
  dct:identifier "http://anzsoil.org/def/au/scma/04B3"^^xsd:anyURI;
  dct:source "URN:ISBN:978-0-643-10218-7";
  skos:definition <https://raw.githack.com/ANZSoilData/def-au-scma/master/html/04-pH/04B3.html>;
  skos:inScheme s:scma-2011;
  skos:notation "04B3";
  skos:prefLabel "pH of 1:5 soil/0.01 M calcium chloride extract -direct (without stirring during measurement)";
  skos:topConceptOf s:scma-2011 .

s:04B4 a skos:Concept, sosa:Procedure;
  dct:identifier "http://anzsoil.org/def/au/scma/04B4"^^xsd:anyURI;
  dct:source "URN:ISBN:978-0-643-10218-7";
  skos:definition <https://raw.githack.com/ANZSoilData/def-au-scma/master/html/04-pH/04B4.html>;
  skos:inScheme s:scma-2011;
  skos:notation "04B4";
  skos:prefLabel "pH of 1:5 soil/0.01 M calcium chloride extract - following method 4A1 (with stirring during measurement)";
  skos:topConceptOf s:scma-2011 .

s:04B5 a skos:Concept, sosa:Procedure;
  dct:identifier "http://anzsoil.org/def/au/scma/04B5"^^xsd:anyURI;
  dct:source "URN:ISBN:978-0-643-10218-7";
  skos:definition <https://raw.githack.com/ANZSoilData/def-au-scma/master/html/04-pH/04B5.html>;
  skos:inScheme s:scma-2011;
  skos:notation "04B5";
  skos:prefLabel "pH of 1:5 soil/0.01 M calcium chloride extract equivalent, by MIR reflectance spectroscopy";
  skos:topConceptOf s:scma-2011 .

s:04C1 a skos:Concept, sosa:Procedure;
  dct:identifier "http://anzsoil.org/def/au/scma/04C1"^^xsd:anyURI;
  dct:source "URN:ISBN:978-0-643-10218-7";
  skos:definition <https://raw.githack.com/ANZSoilData/def-au-scma/master/html/04-pH/04C1.html>;
  skos:inScheme s:scma-2011;
  skos:notation "04C1";
  skos:prefLabel "pH of 1:5 soil/1M potassium chloride extract - direct (without stirring during measurement)";
  skos:topConceptOf s:scma-2011 .

s:04C2 a skos:Concept, sosa:Procedure;
  dct:identifier "http://anzsoil.org/def/au/scma/04C2"^^xsd:anyURI;
  dct:source "URN:ISBN:978-0-643-10218-7";
  skos:definition <https://raw.githack.com/ANZSoilData/def-au-scma/master/html/04-pH/04C2.html>;
  skos:inScheme s:scma-2011;
  skos:notation "04C2";
  skos:prefLabel "pH of 1:5 soil/1M potassium chloride extract following method 4A1 (without stirring during measurement)";
  skos:topConceptOf s:scma-2011 .

s:04C3 a skos:Concept, sosa:Procedure;
  dct:identifier "http://anzsoil.org/def/au/scma/04C3"^^xsd:anyURI;
  dct:source "URN:ISBN:978-0-643-10218-7";
  skos:definition <https://raw.githack.com/ANZSoilData/def-au-scma/master/html/04-pH/04C3.html>;
  skos:inScheme s:scma-2011;
  skos:notation "04C3";
  skos:prefLabel "pH of 1:5 soil/1M potassium chloride extract - direct (with stirring during measurement)";
  skos:topConceptOf s:scma-2011 .

s:04C4 a skos:Concept, sosa:Procedure;
  dct:identifier "http://anzsoil.org/def/au/scma/04C4"^^xsd:anyURI;
  dct:source "URN:ISBN:978-0-643-10218-7";
  skos:definition <https://raw.githack.com/ANZSoilData/def-au-scma/master/html/04-pH/04C4.html>;
  skos:inScheme s:scma-2011;
  skos:notation "04C4";
  skos:prefLabel "pH of 1:5 soil 1M potassium chloride extract - following method 4A1 (with stirring during measurement)";
  skos:topConceptOf s:scma-2011 .

s:04D1 a skos:Concept, sosa:Procedure;
  dct:identifier "http://anzsoil.org/def/au/scma/04D1"^^xsd:anyURI;
  dct:source "URN:ISBN:978-0-643-10218-7";
  skos:definition <https://raw.githack.com/ANZSoilData/def-au-scma/master/html/04-pH/04D1.html>;
  skos:inScheme s:scma-2011;
  skos:notation "04D1";
  skos:prefLabel "pH of sodium fluoride potential suspension and \\'reactivity class\\'";
  skos:topConceptOf s:scma-2011 .

s:04E1 a skos:Concept, sosa:Procedure;
  dct:identifier "http://anzsoil.org/def/au/scma/04E1"^^xsd:anyURI;
  dct:source "URN:ISBN:978-0-643-10218-7";
  skos:definition <https://raw.githack.com/ANZSoilData/def-au-scma/master/html/04-pH/04E1.html>;
  skos:inScheme s:scma-2011;
  skos:notation "04E1";
  skos:prefLabel "pH of hydrogen peroxide extract";
  skos:topConceptOf s:scma-2011 .

s:04F1 a skos:Concept, sosa:Procedure;
  dct:identifier "http://anzsoil.org/def/au/scma/04F1"^^xsd:anyURI;
  dct:source "URN:ISBN:978-0-643-10218-7";
  skos:definition <https://raw.githack.com/ANZSoilData/def-au-scma/master/html/04-pH/04F1.html>;
  skos:inScheme s:scma-2011;
  skos:notation "04F1";
  skos:prefLabel "pH change";
  skos:topConceptOf s:scma-2011 .

s:04G1 a skos:Concept, sosa:Procedure;
  dct:identifier "http://anzsoil.org/def/au/scma/04G1"^^xsd:anyURI;
  dct:source "URN:ISBN:978-0-643-10218-7";
  skos:definition <https://raw.githack.com/ANZSoilData/def-au-scma/master/html/04-pH/04G1.html>;
  skos:inScheme s:scma-2011;
  skos:notation "04G1";
  skos:prefLabel "Field determination of pH";
  skos:topConceptOf s:scma-2011 .

s:05 a skos:Collection;
  dct:identifier "http://anzsoil.org/def/au/scma/05"^^xsd:anyURI;
  dct:source "URN:ISBN:978-0-643-10218-7";
  skos:definition <https://raw.githack.com/ANZSoilData/def-au-scma/master/html/05-soluble-Cl/05.html>;
  skos:inScheme s:scma-2011;
  skos:member s:05A1, s:05A2, s:05A2a, s:05A2b, s:05A3a, s:05A3b, s:05A4;
  skos:notation "05";
  skos:prefLabel "Soluble chloride" .

s:05A1 a skos:Concept, sosa:Procedure;
  dct:identifier "http://anzsoil.org/def/au/scma/05A1"^^xsd:anyURI;
  dct:source "URN:ISBN:978-0-643-10218-7";
  skos:definition <https://raw.githack.com/ANZSoilData/def-au-scma/master/html/05-soluble-Cl/05A1.html>;
  skos:inScheme s:scma-2011;
  skos:notation "05A1";
  skos:prefLabel "Chloride - 1:5 soil/water extract, potentiometric titration";
  skos:topConceptOf s:scma-2011 .

s:05A2 a skos:Concept, sosa:Procedure;
  dct:identifier "http://anzsoil.org/def/au/scma/05A2"^^xsd:anyURI;
  dct:isReplacedBy s:05A2a, s:05A2b;
  dct:source "URN:ISBN:978-0-909605-68-1";
  skos:inScheme s:scma-2011;
  skos:narrower s:05A2a, s:05A2b;
  skos:notation "05A2";
  skos:prefLabel "Chloride - 1:5 soil/water extract, automated colour";
  skos:topConceptOf s:scma-2011 .

s:05A2a a skos:Concept, sosa:Procedure;
  dct:identifier "http://anzsoil.org/def/au/scma/05A2a"^^xsd:anyURI;
  dct:source "URN:ISBN:978-0-643-10218-7";
  skos:broader s:05A2;
  skos:definition <https://raw.githack.com/ANZSoilData/def-au-scma/master/html/05-soluble-Cl/05A2a.html>;
  skos:inScheme s:scma-2011;
  skos:notation "05A2a";
  skos:prefLabel "Chloride - 1:5 soil/water extract, automated colour" .

s:05A2b a skos:Concept, sosa:Procedure;
  dct:identifier "http://anzsoil.org/def/au/scma/05A2b"^^xsd:anyURI;
  dct:source "URN:ISBN:978-0-643-10218-7";
  skos:broader s:05A2;
  skos:definition <https://raw.githack.com/ANZSoilData/def-au-scma/master/html/05-soluble-Cl/05A2b.html>;
  skos:inScheme s:scma-2011;
  skos:notation "05A2b";
  skos:prefLabel "Chloride - 1:5 soil/water extract, FIA" .

s:05A3a a skos:Concept, sosa:Procedure;
  dct:identifier "http://anzsoil.org/def/au/scma/05A3a"^^xsd:anyURI;
  dct:source "URN:ISBN:978-0-643-10218-7";
  skos:definition <https://raw.githack.com/ANZSoilData/def-au-scma/master/html/05-soluble-Cl/05A3a.html>;
  skos:inScheme s:scma-2011;
  skos:notation "05A3a";
  skos:prefLabel "Chloride - 1:5 soil/water extract, ion chromatography (chemical suppression of eluent conductivity)";
  skos:topConceptOf s:scma-2011 .

s:05A3b a skos:Concept, sosa:Procedure;
  dct:identifier "http://anzsoil.org/def/au/scma/05A3b"^^xsd:anyURI;
  dct:source "URN:ISBN:978-0-643-10218-7";
  skos:definition <https://raw.githack.com/ANZSoilData/def-au-scma/master/html/05-soluble-Cl/05A3b.html>;
  skos:inScheme s:scma-2011;
  skos:notation "05A3b";
  skos:prefLabel "Chloride - 1:5 soil/water extract, ion chromatography (single-column with electronic suppression of eluent conductivity)";
  skos:topConceptOf s:scma-2011 .

s:05A4 a skos:Concept, sosa:Procedure;
  dct:identifier "http://anzsoil.org/def/au/scma/05A4"^^xsd:anyURI;
  dct:source "URN:ISBN:978-0-643-10218-7";
  skos:definition <https://raw.githack.com/ANZSoilData/def-au-scma/master/html/05-soluble-Cl/05A4.html>;
  skos:inScheme s:scma-2011;
  skos:notation "05A4";
  skos:prefLabel "Chloride - 1:5 soil/water extract ICPAES";
  skos:topConceptOf s:scma-2011 .

s:06 a skos:Collection;
  dct:identifier "http://anzsoil.org/def/au/scma/06"^^xsd:anyURI;
  dct:source "URN:ISBN:978-0-643-10218-7";
  skos:definition <https://raw.githack.com/ANZSoilData/def-au-scma/master/html/06-C/06.html>;
  skos:inScheme s:scma-2011;
  skos:member s:06A1, s:06B1, s:06B2, s:06B2a, s:06B2b, s:06B3, s:06B4, s:06B4a, s:06B4b,
    s:06C1, s:06D1, s:06E1, s:06F1, s:06G1;
  skos:notation "06";
  skos:prefLabel "Carbon" .

s:06A1 a skos:Concept, sosa:Procedure;
  dct:identifier "http://anzsoil.org/def/au/scma/06A1"^^xsd:anyURI;
  dct:source "URN:ISBN:978-0-643-10218-7";
  skos:definition <https://raw.githack.com/ANZSoilData/def-au-scma/master/html/06-C/06A1.html>;
  skos:inScheme s:scma-2011;
  skos:notation "06A1";
  skos:prefLabel "Organic C - W&B";
  skos:topConceptOf s:scma-2011 .

s:06B1 a skos:Concept, sosa:Procedure;
  dct:identifier "http://anzsoil.org/def/au/scma/06B1"^^xsd:anyURI;
  dct:source "URN:ISBN:978-0-643-10218-7";
  skos:definition <https://raw.githack.com/ANZSoilData/def-au-scma/master/html/06-C/06B1.html>;
  skos:inScheme s:scma-2011;
  skos:notation "06B1";
  skos:prefLabel "Total organic C - Heanes wet oxidisation";
  skos:topConceptOf s:scma-2011 .

s:06B2 a skos:Concept, sosa:Procedure;
  dct:identifier "http://anzsoil.org/def/au/scma/06B2"^^xsd:anyURI;
  dct:source "URN:ISBN:978-0-643-10218-7";
  skos:definition <https://raw.githack.com/ANZSoilData/def-au-scma/master/html/06-C/06B2.html>;
  skos:inScheme s:scma-2011;
  skos:narrower s:06B2a, s:06B2b;
  skos:notation "06B2";
  skos:prefLabel "Total organic C - Dumas high-temperature combustion";
  skos:topConceptOf s:scma-2011 .

s:06B2a a skos:Concept, sosa:Procedure;
  dct:identifier "http://anzsoil.org/def/au/scma/06B2a"^^xsd:anyURI;
  dct:source "URN:ISBN:978-0-643-10218-7";
  skos:broader s:06B2;
  skos:definition <https://raw.githack.com/ANZSoilData/def-au-scma/master/html/06-C/06B2a.html>;
  skos:inScheme s:scma-2011;
  skos:notation "06B2a";
  skos:prefLabel "Total organic C - Dumas high-temperature combustion, volumetric (no soil pretreatment)" .

s:06B2b a skos:Concept, sosa:Procedure;
  dct:identifier "http://anzsoil.org/def/au/scma/06B2b"^^xsd:anyURI;
  dct:source "URN:ISBN:978-0-643-10218-7";
  skos:broader s:06B2;
  skos:definition <https://raw.githack.com/ANZSoilData/def-au-scma/master/html/06-C/06B2b.html>;
  skos:inScheme s:scma-2011;
  skos:notation "06B2b";
  skos:prefLabel "Total organic C - Dumas high-temperature combustion, infrared/thermal conductivity detection (no soil pretreatment)" .

s:06B3 a skos:Concept, sosa:Procedure;
  dct:identifier "http://anzsoil.org/def/au/scma/06B3"^^xsd:anyURI;
  dct:source "URN:ISBN:978-0-643-10218-7";
  skos:definition <https://raw.githack.com/ANZSoilData/def-au-scma/master/html/06-C/06B3.html>;
  skos:inScheme s:scma-2011;
  skos:notation "06B3";
  skos:prefLabel "Total organic C - Dumas high-temperature combustion, infrared/thermal conductivity detection (with prior physical removal of charcoal and chemical removal of carbonates)";
  skos:topConceptOf s:scma-2011 .

s:06B4 a skos:Concept, sosa:Procedure;
  dct:identifier "http://anzsoil.org/def/au/scma/06B4"^^xsd:anyURI;
  dct:source "URN:ISBN:978-0-643-10218-7";
  skos:definition <https://raw.githack.com/ANZSoilData/def-au-scma/master/html/06-C/06B4.html>;
  skos:inScheme s:scma-2011;
  skos:narrower s:06B4a, s:06B4b;
  skos:notation "06B4";
  skos:prefLabel "Total organic C - infrared diffuse reflectance spectroscopy";
  skos:topConceptOf s:scma-2011 .

s:06B4a a skos:Concept, sosa:Procedure;
  dct:identifier "http://anzsoil.org/def/au/scma/06B4a"^^xsd:anyURI;
  dct:source "URN:ISBN:978-0-643-10218-7";
  skos:broader s:06B4;
  skos:definition <https://raw.githack.com/ANZSoilData/def-au-scma/master/html/06-C/06B4a.html>;
  skos:inScheme s:scma-2011;
  skos:notation "06B4a";
  skos:prefLabel "Total organic C - NIR reflectance spectroscopy" .

s:06B4b a skos:Concept, sosa:Procedure;
  dct:identifier "http://anzsoil.org/def/au/scma/06B4b"^^xsd:anyURI;
  dct:source "URN:ISBN:978-0-643-10218-7";
  skos:broader s:06B4;
  skos:definition <https://raw.githack.com/ANZSoilData/def-au-scma/master/html/06-C/06B4b.html>;
  skos:inScheme s:scma-2011;
  skos:notation "06B4b";
  skos:prefLabel "Total organic C - MIR reflectance spectroscopy" .

s:06C1 a skos:Concept, sosa:Procedure;
  dct:identifier "http://anzsoil.org/def/au/scma/06C1"^^xsd:anyURI;
  dct:source "URN:ISBN:978-0-643-10218-7";
  skos:definition <https://raw.githack.com/ANZSoilData/def-au-scma/master/html/06-C/06C1.html>;
  skos:inScheme s:scma-2011;
  skos:notation "06C1";
  skos:prefLabel "Particulate organic C (POC)";
  skos:topConceptOf s:scma-2011 .

s:06D1 a skos:Concept, sosa:Procedure;
  dct:identifier "http://anzsoil.org/def/au/scma/06D1"^^xsd:anyURI;
  dct:source "URN:ISBN:978-0-643-10218-7";
  skos:definition <https://raw.githack.com/ANZSoilData/def-au-scma/master/html/06-C/06D1.html>;
  skos:inScheme s:scma-2011;
  skos:notation "06D1";
  skos:prefLabel "Pyrophosphate-extractable C";
  skos:topConceptOf s:scma-2011 .

s:06E1 a skos:Concept, sosa:Procedure;
  dct:identifier "http://anzsoil.org/def/au/scma/06E1"^^xsd:anyURI;
  dct:source "URN:ISBN:978-0-643-10218-7";
  skos:definition <https://raw.githack.com/ANZSoilData/def-au-scma/master/html/06-C/06E1.html>;
  skos:inScheme s:scma-2011;
  skos:notation "06E1";
  skos:prefLabel "Potassium permanganate oxidisable C (PPOC)";
  skos:topConceptOf s:scma-2011 .

s:06F1 a skos:Concept, sosa:Procedure;
  dct:identifier "http://anzsoil.org/def/au/scma/06F1"^^xsd:anyURI;
  dct:source "URN:ISBN:978-0-643-10218-7";
  skos:definition <https://raw.githack.com/ANZSoilData/def-au-scma/master/html/06-C/06F1.html>;
  skos:inScheme s:scma-2011;
  skos:notation "06F1";
  skos:prefLabel "Charcoal-C";
  skos:topConceptOf s:scma-2011 .

s:06G1 a skos:Concept, sosa:Procedure;
  dct:identifier "http://anzsoil.org/def/au/scma/06G1"^^xsd:anyURI;
  dct:source "URN:ISBN:978-0-643-10218-7";
  skos:definition <https://raw.githack.com/ANZSoilData/def-au-scma/master/html/06-C/06G1.html>;
  skos:inScheme s:scma-2011;
  skos:notation "06G1";
  skos:prefLabel "Total organic matter, organic C, and carbonate by loss-on-ignition";
  skos:topConceptOf s:scma-2011 .

s:07 a skos:Collection;
  dct:identifier "http://anzsoil.org/def/au/scma/07"^^xsd:anyURI;
  dct:source "URN:ISBN:978-0-643-10218-7";
  skos:definition <https://raw.githack.com/ANZSoilData/def-au-scma/master/html/07-N/07.html>;
  skos:inScheme s:scma-2011;
  skos:member s:07A1, s:07A2, s:07A2a, s:07A2b, s:07A3, s:07A4, s:07A5, s:07A6, s:07A6a,
    s:07A6b, s:07B, s:07B1, s:07B1a, s:07B1b, s:07B2, s:07C1, s:07C1a, s:07C1b, s:07C1c,
    s:07C1d, s:07C1e, s:07C1f, s:07C1g, s:07C1h, s:07C2, s:07C2a, s:07C2b, s:07D, s:07D1a,
    s:07D1b, s:07D1c, s:07D2a, s:07D2b;
  skos:notation "07";
  skos:prefLabel "Nitrogen" .

s:07A1 a skos:Concept, sosa:Procedure;
  dct:identifier "http://anzsoil.org/def/au/scma/07A1"^^xsd:anyURI;
  dct:source "URN:ISBN:978-0-643-10218-7";
  skos:definition <https://raw.githack.com/ANZSoilData/def-au-scma/master/html/07-N/07A1.html>;
  skos:inScheme s:scma-2011;
  skos:notation "07A1";
  skos:prefLabel "Total soil-N, semi micro Kjeldahl - steam distillation";
  skos:topConceptOf s:scma-2011 .

s:07A2 a skos:Concept, sosa:Procedure;
  dct:identifier "http://anzsoil.org/def/au/scma/07A2"^^xsd:anyURI;
  dct:isReplacedBy s:07A2a, s:07A2b;
  dct:source "URN:ISBN:978-0-909605-68-1";
  skos:inScheme s:scma-2011;
  skos:narrower s:07A2a, s:07A2b;
  skos:notation "07A2";
  skos:prefLabel "Total soil-N, semi micro Kjeldahl - automated colour|Total nitrogen - semimicro Kjeldahl, automated colour";
  skos:topConceptOf s:scma-2011 .

s:07A2a a skos:Concept, sosa:Procedure;
  dct:identifier "http://anzsoil.org/def/au/scma/07A2a"^^xsd:anyURI;
  dct:source "URN:ISBN:978-0-643-10218-7";
  skos:broader s:07A2;
  skos:definition <https://raw.githack.com/ANZSoilData/def-au-scma/master/html/07-N/07A2a.html>;
  skos:inScheme s:scma-2011;
  skos:notation "07A2a";
  skos:prefLabel "Total soil-N, semi micro Kjeldahl - automated colour, continuous segmented flow" .

s:07A2b a skos:Concept, sosa:Procedure;
  dct:identifier "http://anzsoil.org/def/au/scma/07A2b"^^xsd:anyURI;
  dct:source "URN:ISBN:978-0-643-10218-7";
  skos:broader s:07A2;
  skos:definition <https://raw.githack.com/ANZSoilData/def-au-scma/master/html/07-N/07A2b.html>;
  skos:inScheme s:scma-2011;
  skos:notation "07A2b";
  skos:prefLabel "Total soil-N, semi micro Kjeldahl - automated colour - FIA" .

s:07A3 a skos:Concept, sosa:Procedure;
  dct:identifier "http://anzsoil.org/def/au/scma/07A3"^^xsd:anyURI;
  dct:source "URN:ISBN:978-0-643-10218-7";
  skos:definition <https://raw.githack.com/ANZSoilData/def-au-scma/master/html/07-N/07A3.html>;
  skos:inScheme s:scma-2011;
  skos:notation "07A3";
  skos:prefLabel "Total soil-N (where nitrate >20 mg N/kg) - steam distillation";
  skos:topConceptOf s:scma-2011 .

s:07A4 a skos:Concept, sosa:Procedure;
  dct:identifier "http://anzsoil.org/def/au/scma/07A4"^^xsd:anyURI;
  dct:source "URN:ISBN:978-0-643-10218-7";
  skos:definition <https://raw.githack.com/ANZSoilData/def-au-scma/master/html/07-N/07A4.html>;
  skos:inScheme s:scma-2011;
  skos:notation "07A4";
  skos:prefLabel "Total-N (where nitrate >20 mg N/kg) - automated colour, continuous segmented flow/FIA";
  skos:topConceptOf s:scma-2011 .

s:07A5 a skos:Concept, sosa:Procedure;
  dct:identifier "http://anzsoil.org/def/au/scma/07A5"^^xsd:anyURI;
  dct:source "URN:ISBN:978-0-643-10218-7";
  skos:definition <https://raw.githack.com/ANZSoilData/def-au-scma/master/html/07-N/07A5.html>;
  skos:inScheme s:scma-2011;
  skos:notation "07A5";
  skos:prefLabel "Total soil-N - Dumas high-temperature combustion";
  skos:topConceptOf s:scma-2011 .

s:07A6 a skos:Concept, sosa:Procedure;
  dct:identifier "http://anzsoil.org/def/au/scma/07A6"^^xsd:anyURI;
  dct:source "URN:ISBN:978-0-643-10218-7";
  skos:definition <https://raw.githack.com/ANZSoilData/def-au-scma/master/html/07-N/07A6.html>;
  skos:inScheme s:scma-2011;
  skos:narrower s:07A6a, s:07A6b;
  skos:notation "07A6";
  skos:prefLabel "Total soil-N - infrared diffuse reflectance spectroscopy";
  skos:topConceptOf s:scma-2011 .

s:07A6a a skos:Concept, sosa:Procedure;
  dct:identifier "http://anzsoil.org/def/au/scma/07A6a"^^xsd:anyURI;
  dct:source "URN:ISBN:978-0-643-10218-7";
  skos:broader s:07A6;
  skos:definition <https://raw.githack.com/ANZSoilData/def-au-scma/master/html/07-N/07A6a.html>;
  skos:inScheme s:scma-2011;
  skos:notation "07A6a";
  skos:prefLabel "Total Soil-N - NIR diffuse reflectance spectroscopy" .

s:07A6b a skos:Concept, sosa:Procedure;
  dct:identifier "http://anzsoil.org/def/au/scma/07A6b"^^xsd:anyURI;
  dct:source "URN:ISBN:978-0-643-10218-7";
  skos:broader s:07A6;
  skos:definition <https://raw.githack.com/ANZSoilData/def-au-scma/master/html/07-N/07A6b.html>;
  skos:inScheme s:scma-2011;
  skos:notation "07A6b";
  skos:prefLabel "Total soil-N - MIR diffuse reflectance spectroscopy" .

s:07B a skos:Concept, sosa:Procedure;
  dct:identifier "http://anzsoil.org/def/au/scma/07B"^^xsd:anyURI;
  dct:source "URN:ISBN:978-0-643-10218-7";
  skos:definition <https://raw.githack.com/ANZSoilData/def-au-scma/master/html/07-N/07B.html>;
  skos:inScheme s:scma-2011;
  skos:narrower s:07B1, s:07B2;
  skos:notation "07B";
  skos:prefLabel "Water-soluble nitrate-N";
  skos:topConceptOf s:scma-2011 .

s:07B1 a skos:Concept, sosa:Procedure;
  dct:identifier "http://anzsoil.org/def/au/scma/07B1"^^xsd:anyURI;
  dct:isReplacedBy s:07B1a, s:07B1b;
  dct:source "URN:ISBN:978-0-909605-68-1";
  skos:broader s:07B;
  skos:inScheme s:scma-2011;
  skos:narrower s:07B1a, s:07B1b;
  skos:notation "07B1";
  skos:prefLabel "Water-soluble nitrate-N - automated colour|Water soluble nitrate - automated colour" .

s:07B1a a skos:Concept, sosa:Procedure;
  dct:identifier "http://anzsoil.org/def/au/scma/07B1a"^^xsd:anyURI;
  dct:source "URN:ISBN:978-0-643-10218-7";
  skos:broader s:07B1;
  skos:definition <https://raw.githack.com/ANZSoilData/def-au-scma/master/html/07-N/07B1a.html>;
  skos:inScheme s:scma-2011;
  skos:notation "07B1a";
  skos:prefLabel "Water-soluble nitrate-N - automated colour, continuous segmented flow" .

s:07B1b a skos:Concept, sosa:Procedure;
  dct:identifier "http://anzsoil.org/def/au/scma/07B1b"^^xsd:anyURI;
  dct:source "URN:ISBN:978-0-643-10218-7";
  skos:broader s:07B1;
  skos:definition <https://raw.githack.com/ANZSoilData/def-au-scma/master/html/07-N/07B1b.html>;
  skos:inScheme s:scma-2011;
  skos:notation "07B1b";
  skos:prefLabel "Water-soluble nitrate-N - automated colour, FIA" .

s:07B2 a skos:Concept, sosa:Procedure;
  dct:identifier "http://anzsoil.org/def/au/scma/07B2"^^xsd:anyURI;
  dct:source "URN:ISBN:978-0-643-10218-7";
  skos:broader s:07B;
  skos:definition <https://raw.githack.com/ANZSoilData/def-au-scma/master/html/07-N/07B2.html>;
  skos:inScheme s:scma-2011;
  skos:notation "07B2";
  skos:prefLabel "Water-soluble nitrate-N - ion chromatography" .

s:07C1 a skos:Concept, sosa:Procedure;
  dct:identifier "http://anzsoil.org/def/au/scma/07C1"^^xsd:anyURI;
  dct:source "URN:ISBN:978-0-643-10218-7";
  skos:definition <https://raw.githack.com/ANZSoilData/def-au-scma/master/html/07-N/07C1.html>;
  skos:inScheme s:scma-2011;
  skos:narrower s:07C1a, s:07C1b, s:07C1c, s:07C1d, s:07C1e, s:07C1f, s:07C1g, s:07C1h;
  skos:notation "07C1";
  skos:prefLabel "Mineral-N 2 M KCl, steam distillation";
  skos:topConceptOf s:scma-2011 .

s:07C1a a skos:Concept, sosa:Procedure;
  dct:identifier "http://anzsoil.org/def/au/scma/07C1a"^^xsd:anyURI;
  dct:source "URN:ISBN:978-0-643-10218-7";
  skos:broader s:07C1;
  skos:definition <https://raw.githack.com/ANZSoilData/def-au-scma/master/html/07-N/07C1a.html>;
  skos:inScheme s:scma-2011;
  skos:notation "07C1a";
  skos:prefLabel "Ammonium-N (in presence or absence of nitrite) - steam distillation" .

s:07C1b a skos:Concept, sosa:Procedure;
  dct:identifier "http://anzsoil.org/def/au/scma/07C1b"^^xsd:anyURI;
  dct:source "URN:ISBN:978-0-643-10218-7";
  skos:broader s:07C1;
  skos:definition <https://raw.githack.com/ANZSoilData/def-au-scma/master/html/07-N/07C1b.html>;
  skos:inScheme s:scma-2011;
  skos:notation "07C1b";
  skos:prefLabel "(Nitrate + Nitrite)-N - steam distillation" .

s:07C1c a skos:Concept, sosa:Procedure;
  dct:identifier "http://anzsoil.org/def/au/scma/07C1c"^^xsd:anyURI;
  dct:source "URN:ISBN:978-0-643-10218-7";
  skos:broader s:07C1;
  skos:definition <https://raw.githack.com/ANZSoilData/def-au-scma/master/html/07-N/07C1c.html>;
  skos:inScheme s:scma-2011;
  skos:notation "07C1c";
  skos:prefLabel "(Ammonium + Nitrate + Nitrite)-N - steam distillation" .

s:07C1d a skos:Concept, sosa:Procedure;
  dct:identifier "http://anzsoil.org/def/au/scma/07C1d"^^xsd:anyURI;
  dct:source "URN:ISBN:978-0-643-10218-7";
  skos:broader s:07C1;
  skos:definition <https://raw.githack.com/ANZSoilData/def-au-scma/master/html/07-N/07C1d.html>;
  skos:inScheme s:scma-2011;
  skos:notation "07C1d";
  skos:prefLabel "(Ammonium + Nitrate)-N, in presence of nitrite - steam distillation" .

s:07C1e a skos:Concept, sosa:Procedure;
  dct:identifier "http://anzsoil.org/def/au/scma/07C1e"^^xsd:anyURI;
  dct:source "URN:ISBN:978-0-643-10218-7";
  skos:broader s:07C1;
  skos:definition <https://raw.githack.com/ANZSoilData/def-au-scma/master/html/07-N/07C1e.html>;
  skos:inScheme s:scma-2011;
  skos:notation "07C1e";
  skos:prefLabel "Nitrate-N, in presence of nitrite - steam distillation" .

s:07C1f a skos:Concept, sosa:Procedure;
  dct:identifier "http://anzsoil.org/def/au/scma/07C1f"^^xsd:anyURI;
  dct:source "URN:ISBN:978-0-643-10218-7";
  skos:broader s:07C1;
  skos:definition <https://raw.githack.com/ANZSoilData/def-au-scma/master/html/07-N/07C1f.html>;
  skos:inScheme s:scma-2011;
  skos:notation "07C1f";
  skos:prefLabel "Nitrate-N, in absence of nitrite - steam distillation" .

s:07C1g a skos:Concept, sosa:Procedure;
  dct:identifier "http://anzsoil.org/def/au/scma/07C1g"^^xsd:anyURI;
  dct:source "URN:ISBN:978-0-643-10218-7";
  skos:broader s:07C1;
  skos:definition <https://raw.githack.com/ANZSoilData/def-au-scma/master/html/07-N/07C1g.html>;
  skos:inScheme s:scma-2011;
  skos:notation "07C1g";
  skos:prefLabel "(Ammonium + Nitrate)-N, in absence of nitrite - steam distillation" .

s:07C1h a skos:Concept, sosa:Procedure;
  dct:identifier "http://anzsoil.org/def/au/scma/07C1h"^^xsd:anyURI;
  dct:source "URN:ISBN:978-0-643-10218-7";
  skos:broader s:07C1;
  skos:definition <https://raw.githack.com/ANZSoilData/def-au-scma/master/html/07-N/07C1h.html>;
  skos:inScheme s:scma-2011;
  skos:notation "07C1h";
  skos:prefLabel "Nitrite-N - steam distillation" .

s:07C2 a skos:Concept, sosa:Procedure;
  dct:identifier "http://anzsoil.org/def/au/scma/07C2"^^xsd:anyURI;
  dct:isReplacedBy s:07C2a, s:07C2b;
  dct:source "URN:ISBN:978-0-909605-68-1";
  skos:inScheme s:scma-2011;
  skos:narrower s:07C2a, s:07C2b;
  skos:notation "07C2";
  skos:prefLabel "Mineral-N 2 M KCl, automated colour|mineral nitrogen with 2M KCl - automated colour";
  skos:topConceptOf s:scma-2011 .

s:07C2a a skos:Concept, sosa:Procedure;
  dct:identifier "http://anzsoil.org/def/au/scma/07C2a"^^xsd:anyURI;
  dct:source "URN:ISBN:978-0-643-10218-7";
  skos:broader s:07C2;
  skos:definition <https://raw.githack.com/ANZSoilData/def-au-scma/master/html/07-N/07C2a.html>;
  skos:inScheme s:scma-2011;
  skos:notation "07C2a";
  skos:prefLabel "Mineral-N 2 M KCl, automated colour, continuous segmented flow" .

s:07C2b a skos:Concept, sosa:Procedure;
  dct:identifier "http://anzsoil.org/def/au/scma/07C2b"^^xsd:anyURI;
  dct:source "URN:ISBN:978-0-643-10218-7";
  skos:broader s:07C2;
  skos:definition <https://raw.githack.com/ANZSoilData/def-au-scma/master/html/07-N/07C2b.html>;
  skos:inScheme s:scma-2011;
  skos:notation "07C2b";
  skos:prefLabel "Mineral-N - 2 M KCl, automated colour, FIA" .

s:07D a skos:Concept, sosa:Procedure;
  dct:identifier "http://anzsoil.org/def/au/scma/07D"^^xsd:anyURI;
  dct:source "URN:ISBN:978-0-643-10218-7";
  skos:definition <https://raw.githack.com/ANZSoilData/def-au-scma/master/html/07-N/07D.html>;
  skos:inScheme s:scma-2011;
  skos:narrower s:07D1a, s:07D1b, s:07D1c, s:07D2a, s:07D2b;
  skos:notation "07D";
  skos:prefLabel "Potentially mineralisable N (PMN)";
  skos:topConceptOf s:scma-2011 .

s:07D1a a skos:Concept, sosa:Procedure;
  dct:identifier "http://anzsoil.org/def/au/scma/07D1a"^^xsd:anyURI;
  dct:source "URN:ISBN:978-0-643-10218-7";
  skos:broader s:07D;
  skos:definition <https://raw.githack.com/ANZSoilData/def-au-scma/master/html/07-N/07D1a.html>;
  skos:inScheme s:scma-2011;
  skos:notation "07D1a";
  skos:prefLabel "Potentially mineralisable N, hot-KCl extraction (PMN KCl) - automated colour, continuous segmented flow" .

s:07D1b a skos:Concept, sosa:Procedure;
  dct:identifier "http://anzsoil.org/def/au/scma/07D1b"^^xsd:anyURI;
  dct:source "URN:ISBN:978-0-643-10218-7";
  skos:broader s:07D;
  skos:definition <https://raw.githack.com/ANZSoilData/def-au-scma/master/html/07-N/07D1b.html>;
  skos:inScheme s:scma-2011;
  skos:notation "07D1b";
  skos:prefLabel "Potentially mineralisable N, hot-KCl extraction (PMN KCl) - automated colour, FIA" .

s:07D1c a skos:Concept, sosa:Procedure;
  dct:identifier "http://anzsoil.org/def/au/scma/07D1c"^^xsd:anyURI;
  dct:source "URN:ISBN:978-0-643-10218-7";
  skos:broader s:07D;
  skos:definition <https://raw.githack.com/ANZSoilData/def-au-scma/master/html/07-N/07D1c.html>;
  skos:inScheme s:scma-2011;
  skos:notation "07D1c";
  skos:prefLabel "Potentially mineralisable N, hot-KCl extraction (PMN KCl) - NIR diffuse reflectance spectroscopy" .

s:07D2a a skos:Concept, sosa:Procedure;
  dct:identifier "http://anzsoil.org/def/au/scma/07D2a"^^xsd:anyURI;
  dct:source "URN:ISBN:978-0-643-10218-7";
  skos:broader s:07D;
  skos:definition <https://raw.githack.com/ANZSoilData/def-au-scma/master/html/07-N/07D2a.html>;
  skos:inScheme s:scma-2011;
  skos:notation "07D2a";
  skos:prefLabel "Potentially mineralisable N, anaerobic incubation - automated colour, continuous segmented flow" .

s:07D2b a skos:Concept, sosa:Procedure;
  dct:identifier "http://anzsoil.org/def/au/scma/07D2b"^^xsd:anyURI;
  dct:source "URN:ISBN:978-0-643-10218-7";
  skos:broader s:07D;
  skos:definition <https://raw.githack.com/ANZSoilData/def-au-scma/master/html/07-N/07D2b.html>;
  skos:inScheme s:scma-2011;
  skos:notation "07D2b";
  skos:prefLabel "Potentially mineralisable N, anaerobic incubation - automated colour, FIA" .

s:08 a skos:Collection;
  dct:identifier "http://anzsoil.org/def/au/scma/08"^^xsd:anyURI;
  dct:source "URN:ISBN:978-0-643-10218-7";
  skos:definition <https://raw.githack.com/ANZSoilData/def-au-scma/master/html/08-CN-ratio/08.html>;
  skos:inScheme s:scma-2011;
  skos:member s:08A1, s:08B1;
  skos:notation "08";
  skos:prefLabel "Carbon/nitrogen ratio" .

s:08A1 a skos:Concept, sosa:Procedure;
  dct:identifier "http://anzsoil.org/def/au/scma/08A1"^^xsd:anyURI;
  dct:source "URN:ISBN:978-0-643-10218-7";
  skos:definition <https://raw.githack.com/ANZSoilData/def-au-scma/master/html/08-CN-ratio/08A1.html>;
  skos:inScheme s:scma-2011;
  skos:notation "08A1";
  skos:prefLabel "Total organic carbon/total nitrogen ratio";
  skos:topConceptOf s:scma-2011 .

s:08B1 a skos:Concept, sosa:Procedure;
  dct:identifier "http://anzsoil.org/def/au/scma/08B1"^^xsd:anyURI;
  dct:source "URN:ISBN:978-0-643-10218-7";
  skos:definition <https://raw.githack.com/ANZSoilData/def-au-scma/master/html/08-CN-ratio/08B1.html>;
  skos:inScheme s:scma-2011;
  skos:notation "08B1";
  skos:prefLabel "Organic carbon - W&B/total nitrogen ratio";
  skos:topConceptOf s:scma-2011 .

s:09 a skos:Collection;
  dct:identifier "http://anzsoil.org/def/au/scma/09"^^xsd:anyURI;
  dct:source "URN:ISBN:978-0-643-10218-7";
  skos:definition <https://raw.githack.com/ANZSoilData/def-au-scma/master/html/09-P/09.html>;
  skos:inScheme s:scma-2011;
  skos:member s:09A, s:09A1, s:09A2, s:09A3a, s:09A3b, s:09B, s:09B1, s:09B2, s:09C,
    s:09C1, s:09C2, s:09C2a, s:09C2b, s:09D1, s:09E, s:09E1, s:09E2, s:09F1, s:09F2, s:09G1,
    s:09G2, s:09H1, s:09I, s:09I1, s:09I2a, s:09I2b, s:09I2c, s:09I3a, s:09I3b, s:09I3c,
    s:09I4a, s:09I4b, s:09I4c, s:09J, s:09J1, s:09J2, s:09K, s:09K1a, s:09K1b, s:09K2;
  skos:notation "09";
  skos:prefLabel "Phosphorus" .

s:09A a skos:Concept, sosa:Procedure;
  dct:identifier "http://anzsoil.org/def/au/scma/09A"^^xsd:anyURI;
  dct:source "URN:ISBN:978-0-643-10218-7";
  skos:definition <https://raw.githack.com/ANZSoilData/def-au-scma/master/html/09-P/09A.html>;
  skos:inScheme s:scma-2011;
  skos:narrower s:09A1, s:09A2, s:09A3a, s:09A3b;
  skos:notation "09A";
  skos:prefLabel "Total P";
  skos:topConceptOf s:scma-2011 .

s:09A1 a skos:Concept, sosa:Procedure;
  dct:identifier "http://anzsoil.org/def/au/scma/09A1"^^xsd:anyURI;
  dct:source "URN:ISBN:978-0-643-10218-7";
  skos:broader s:09A;
  skos:definition <https://raw.githack.com/ANZSoilData/def-au-scma/master/html/09-P/09A1.html>;
  skos:inScheme s:scma-2011;
  skos:notation "09A1";
  skos:prefLabel "Total P - X-ray fluorescence" .

s:09A2 a skos:Concept, sosa:Procedure;
  dct:identifier "http://anzsoil.org/def/au/scma/09A2"^^xsd:anyURI;
  dct:source "URN:ISBN:978-0-643-10218-7";
  skos:broader s:09A;
  skos:definition <https://raw.githack.com/ANZSoilData/def-au-scma/master/html/09-P/09A2.html>;
  skos:inScheme s:scma-2011;
  skos:notation "09A2";
  skos:prefLabel "Total P - sodium carbonate fusion" .

s:09A3a a skos:Concept, sosa:Procedure;
  dct:identifier "http://anzsoil.org/def/au/scma/09A3a"^^xsd:anyURI;
  dct:source "URN:ISBN:978-0-643-10218-7";
  skos:broader s:09A;
  skos:definition <https://raw.githack.com/ANZSoilData/def-au-scma/master/html/09-P/09A3a.html>;
  skos:inScheme s:scma-2011;
  skos:notation "09A3a";
  skos:prefLabel "Kjeldahl P (KP) - automated colour, FIA/continuous segmented flow" .

s:09A3b a skos:Concept, sosa:Procedure;
  dct:identifier "http://anzsoil.org/def/au/scma/09A3b"^^xsd:anyURI;
  dct:source "URN:ISBN:978-0-643-10218-7";
  skos:broader s:09A;
  skos:definition <https://raw.githack.com/ANZSoilData/def-au-scma/master/html/09-P/09A3b.html>;
  skos:inScheme s:scma-2011;
  skos:notation "09A3b";
  skos:prefLabel "Kjeldahl P (KP) - ICPAES" .

s:09B a skos:Concept, sosa:Procedure;
  dct:identifier "http://anzsoil.org/def/au/scma/09B"^^xsd:anyURI;
  dct:source "URN:ISBN:978-0-643-10218-7";
  skos:definition <https://raw.githack.com/ANZSoilData/def-au-scma/master/html/09-P/09B.html>;
  skos:inScheme s:scma-2011;
  skos:narrower s:09B1, s:09B2;
  skos:notation "09B";
  skos:prefLabel "Bicarbonate-extractable P (Colwell-P)";
  skos:topConceptOf s:scma-2011 .

s:09B1 a skos:Concept, sosa:Procedure;
  dct:identifier "http://anzsoil.org/def/au/scma/09B1"^^xsd:anyURI;
  dct:source "URN:ISBN:978-0-643-10218-7";
  skos:broader s:09B;
  skos:definition <https://raw.githack.com/ANZSoilData/def-au-scma/master/html/09-P/09B1.html>;
  skos:inScheme s:scma-2011;
  skos:notation "09B1";
  skos:prefLabel "Bicarbonate-extractable P (Colwell-P) - manual colour" .

s:09B2 a skos:Concept, sosa:Procedure;
  dct:identifier "http://anzsoil.org/def/au/scma/09B2"^^xsd:anyURI;
  dct:source "URN:ISBN:978-0-643-10218-7";
  skos:broader s:09B;
  skos:definition <https://raw.githack.com/ANZSoilData/def-au-scma/master/html/09-P/09B2.html>;
  skos:inScheme s:scma-2011;
  skos:notation "09B2";
  skos:prefLabel "Bicarbonate-extractable P (Colwell-P) - automated colour, continuous segmented flow/FIA" .

s:09C a skos:Concept, sosa:Procedure;
  dct:identifier "http://anzsoil.org/def/au/scma/09C"^^xsd:anyURI;
  dct:source "URN:ISBN:978-0-643-10218-7";
  skos:definition <https://raw.githack.com/ANZSoilData/def-au-scma/master/html/09-P/09C.html>;
  skos:inScheme s:scma-2011;
  skos:narrower s:09C1, s:09C2;
  skos:notation "09C";
  skos:prefLabel "Olsen-extractable P (Olsen-P)";
  skos:topConceptOf s:scma-2011 .

s:09C1 a skos:Concept, sosa:Procedure;
  dct:identifier "http://anzsoil.org/def/au/scma/09C1"^^xsd:anyURI;
  dct:source "URN:ISBN:978-0-643-10218-7";
  skos:broader s:09C;
  skos:definition <https://raw.githack.com/ANZSoilData/def-au-scma/master/html/09-P/09C1.html>;
  skos:inScheme s:scma-2011;
  skos:notation "09C1";
  skos:prefLabel "Olsen-extractable P (Olsen-P) - manual colour" .

s:09C2 a skos:Concept, sosa:Procedure;
  dct:identifier "http://anzsoil.org/def/au/scma/09C2"^^xsd:anyURI;
  dct:isReplacedBy s:09C2a, s:09C2b;
  dct:source "URN:ISBN:978-0-909605-68-1";
  skos:broader s:09C;
  skos:inScheme s:scma-2011;
  skos:narrower s:09C2a, s:09C2b;
  skos:notation "09C2";
  skos:prefLabel "Olsen-extractable phosphorus - automated colour|Olsen-extractable P (Olsen-P) - automated colour" .

s:09C2a a skos:Concept, sosa:Procedure;
  dct:identifier "http://anzsoil.org/def/au/scma/09C2a"^^xsd:anyURI;
  dct:source "URN:ISBN:978-0-643-10218-7";
  skos:broader s:09C2;
  skos:definition <https://raw.githack.com/ANZSoilData/def-au-scma/master/html/09-P/09C2a.html>;
  skos:inScheme s:scma-2011;
  skos:notation "09C2a";
  skos:prefLabel "Olsen-extractable P (Olsen-P) - automated colour, continuous segmented flow" .

s:09C2b a skos:Concept, sosa:Procedure;
  dct:identifier "http://anzsoil.org/def/au/scma/09C2b"^^xsd:anyURI;
  dct:source "URN:ISBN:978-0-643-10218-7";
  skos:broader s:09C2;
  skos:definition <https://raw.githack.com/ANZSoilData/def-au-scma/master/html/09-P/09C2b.html>;
  skos:inScheme s:scma-2011;
  skos:notation "09C2b";
  skos:prefLabel "Olsen-extractable P (Olsen-P) - automated colour/FIA" .

s:09D1 a skos:Concept, sosa:Procedure;
  dct:identifier "http://anzsoil.org/def/au/scma/09D1"^^xsd:anyURI;
  dct:source "URN:ISBN:978-0-643-10218-7";
  skos:definition <https://raw.githack.com/ANZSoilData/def-au-scma/master/html/09-P/09D1.html>;
  skos:inScheme s:scma-2011;
  skos:notation "09D1";
  skos:prefLabel "Lactate-extractable P (Lactate-P) - manual colour";
  skos:topConceptOf s:scma-2011 .

s:09E a skos:Concept, sosa:Procedure;
  dct:identifier "http://anzsoil.org/def/au/scma/09E"^^xsd:anyURI;
  dct:source "URN:ISBN:978-0-643-10218-7";
  skos:definition <https://raw.githack.com/ANZSoilData/def-au-scma/master/html/09-P/09E.html>;
  skos:inScheme s:scma-2011;
  skos:narrower s:09E1, s:09E2;
  skos:notation "09E";
  skos:prefLabel "Fluoride-extractable P (Bray-1 P)";
  skos:topConceptOf s:scma-2011 .

s:09E1 a skos:Concept, sosa:Procedure;
  dct:identifier "http://anzsoil.org/def/au/scma/09E1"^^xsd:anyURI;
  dct:source "URN:ISBN:978-0-643-10218-7";
  skos:broader s:09E;
  skos:definition <https://raw.githack.com/ANZSoilData/def-au-scma/master/html/09-P/09E1.html>;
  skos:inScheme s:scma-2011;
  skos:notation "09E1";
  skos:prefLabel "Fluoride-extractable P (Bray-1 P) - manual colour" .

s:09E2 a skos:Concept, sosa:Procedure;
  dct:identifier "http://anzsoil.org/def/au/scma/09E2"^^xsd:anyURI;
  dct:source "URN:ISBN:978-0-643-10218-7";
  skos:broader s:09E;
  skos:definition <https://raw.githack.com/ANZSoilData/def-au-scma/master/html/09-P/09E2.html>;
  skos:inScheme s:scma-2011;
  skos:notation "09E2";
  skos:prefLabel "Fluoride-extractable P (Bray-1 P) - continuous segmented flow/FIA automated colour" .

s:09F1 a skos:Concept, sosa:Procedure;
  dct:identifier "http://anzsoil.org/def/au/scma/09F1"^^xsd:anyURI;
  dct:source "URN:ISBN:978-0-643-10218-7";
  skos:definition <https://raw.githack.com/ANZSoilData/def-au-scma/master/html/09-P/09F1.html>;
  skos:inScheme s:scma-2011;
  skos:notation "09F1";
  skos:prefLabel "Calcium chloride-extractable P - manual colour";
  skos:topConceptOf s:scma-2011 .

s:09F2 a skos:Concept, sosa:Procedure;
  dct:identifier "http://anzsoil.org/def/au/scma/09F2"^^xsd:anyURI;
  dct:source "URN:ISBN:978-0-643-10218-7";
  skos:definition <https://raw.githack.com/ANZSoilData/def-au-scma/master/html/09-P/09F2.html>;
  skos:inScheme s:scma-2011;
  skos:notation "09F2";
  skos:prefLabel "Calcium chloride-extractable P - continuous segmented flow/FIA automated colour";
  skos:topConceptOf s:scma-2011 .

s:09G1 a skos:Concept, sosa:Procedure;
  dct:identifier "http://anzsoil.org/def/au/scma/09G1"^^xsd:anyURI;
  dct:source "URN:ISBN:978-0-643-10218-7";
  skos:definition <https://raw.githack.com/ANZSoilData/def-au-scma/master/html/09-P/09G1.html>;
  skos:inScheme s:scma-2011;
  skos:notation "09G1";
  skos:prefLabel "Acid-extractable P (BSES-P) - manual colour";
  skos:topConceptOf s:scma-2011 .

s:09G2 a skos:Concept, sosa:Procedure;
  dct:identifier "http://anzsoil.org/def/au/scma/09G2"^^xsd:anyURI;
  dct:source "URN:ISBN:978-0-643-10218-7";
  skos:definition <https://raw.githack.com/ANZSoilData/def-au-scma/master/html/09-P/09G2.html>;
  skos:inScheme s:scma-2011;
  skos:notation "09G2";
  skos:prefLabel "Acid-extractable P (BSES-P) - continuous segmented flow/FIA automated colour";
  skos:topConceptOf s:scma-2011 .

s:09H1 a skos:Concept, sosa:Procedure;
  dct:identifier "http://anzsoil.org/def/au/scma/09H1"^^xsd:anyURI;
  dct:source "URN:ISBN:978-0-643-10218-7";
  skos:definition <https://raw.githack.com/ANZSoilData/def-au-scma/master/html/09-P/09H1.html>;
  skos:inScheme s:scma-2011;
  skos:notation "09H1";
  skos:prefLabel "Anion Storage Capacity (previously P Retention)";
  skos:topConceptOf s:scma-2011 .

s:09I a skos:Concept, sosa:Procedure;
  dct:identifier "http://anzsoil.org/def/au/scma/09I"^^xsd:anyURI;
  dct:source "URN:ISBN:978-0-643-10218-7";
  skos:definition <https://raw.githack.com/ANZSoilData/def-au-scma/master/html/09-P/09I.html>;
  skos:inScheme s:scma-2011;
  skos:narrower s:09I1, s:09I2a, s:09I2b, s:09I2c, s:09I3a, s:09I3b, s:09I3c, s:09I4a,
    s:09I4b, s:09I4c;
  skos:notation "09I";
  skos:prefLabel "Phosphate Indices";
  skos:topConceptOf s:scma-2011 .

s:09I1 a skos:Concept, sosa:Procedure;
  dct:identifier "http://anzsoil.org/def/au/scma/09I1"^^xsd:anyURI;
  dct:source "URN:ISBN:978-0-643-10218-7";
  skos:broader s:09I;
  skos:definition <https://raw.githack.com/ANZSoilData/def-au-scma/master/html/09-P/09I1.html>;
  skos:inScheme s:scma-2011;
  skos:notation "09I1";
  skos:prefLabel "Phosphate Sorption Index" .

s:09I2a a skos:Concept, sosa:Procedure;
  dct:identifier "http://anzsoil.org/def/au/scma/09I2a"^^xsd:anyURI;
  dct:source "URN:ISBN:978-0-643-10218-7";
  skos:broader s:09I;
  skos:definition <https://raw.githack.com/ANZSoilData/def-au-scma/master/html/09-P/09I2a.html>;
  skos:inScheme s:scma-2011;
  skos:notation "09I2a";
  skos:prefLabel "P buffer index - PBI (ColP) - Murphy and Riley|P buffer index - PBI (ColP)" .

s:09I2b a skos:Concept, sosa:Procedure;
  dct:identifier "http://anzsoil.org/def/au/scma/09I2b"^^xsd:anyURI;
  dct:source "URN:ISBN:978-0-643-10218-7";
  skos:broader s:09I;
  skos:definition <https://raw.githack.com/ANZSoilData/def-au-scma/master/html/09-P/09I2b.html>;
  skos:inScheme s:scma-2011;
  skos:notation "09I2b";
  skos:prefLabel "P buffer index - PBI (ColP)|P buffer index - PBI (ColP) - ICPAES" .

s:09I2c a skos:Concept, sosa:Procedure;
  dct:identifier "http://anzsoil.org/def/au/scma/09I2c"^^xsd:anyURI;
  dct:source "URN:ISBN:978-0-643-10218-7";
  skos:broader s:09I;
  skos:definition <https://raw.githack.com/ANZSoilData/def-au-scma/master/html/09-P/09I2c.html>;
  skos:inScheme s:scma-2011;
  skos:notation "09I2c";
  skos:prefLabel "P buffer index - PBI (ColP)|P buffer index - PBI (ColP) - Vanadate" .

s:09I3a a skos:Concept, sosa:Procedure;
  dct:identifier "http://anzsoil.org/def/au/scma/09I3a"^^xsd:anyURI;
  dct:source "URN:ISBN:978-0-643-10218-7";
  skos:broader s:09I;
  skos:definition <https://raw.githack.com/ANZSoilData/def-au-scma/master/html/09-P/09I3a.html>;
  skos:inScheme s:scma-2011;
  skos:notation "09I3a";
  skos:prefLabel "P buffer index - PBI (OlsenP)|P buffer index - PBI (OlsenP) - Murphy and Riley" .

s:09I3b a skos:Concept, sosa:Procedure;
  dct:identifier "http://anzsoil.org/def/au/scma/09I3b"^^xsd:anyURI;
  dct:source "URN:ISBN:978-0-643-10218-7";
  skos:broader s:09I;
  skos:definition <https://raw.githack.com/ANZSoilData/def-au-scma/master/html/09-P/09I3b.html>;
  skos:inScheme s:scma-2011;
  skos:notation "09I3b";
  skos:prefLabel "P buffer index - PBI (OlsenP)|P buffer index - PBI (OlsenP) - ICPAES" .

s:09I3c a skos:Concept, sosa:Procedure;
  dct:identifier "http://anzsoil.org/def/au/scma/09I3c"^^xsd:anyURI;
  dct:source "URN:ISBN:978-0-643-10218-7";
  skos:broader s:09I;
  skos:definition <https://raw.githack.com/ANZSoilData/def-au-scma/master/html/09-P/09I3c.html>;
  skos:inScheme s:scma-2011;
  skos:notation "09I3c";
  skos:prefLabel "P buffer index - PBI (OlsenP)|P buffer index - PBI (OlsenP) - Vanadate" .

s:09I4a a skos:Concept, sosa:Procedure;
  dct:identifier "http://anzsoil.org/def/au/scma/09I4a"^^xsd:anyURI;
  dct:source "URN:ISBN:978-0-643-10218-7";
  skos:broader s:09I;
  skos:definition <https://raw.githack.com/ANZSoilData/def-au-scma/master/html/09-P/09I4a.html>;
  skos:inScheme s:scma-2011;
  skos:notation "09I4a";
  skos:prefLabel "P buffer index - PBI (unadj) - Murphy and Riley|P buffer index - PBI (unadj)" .

s:09I4b a skos:Concept, sosa:Procedure;
  dct:identifier "http://anzsoil.org/def/au/scma/09I4b"^^xsd:anyURI;
  dct:source "URN:ISBN:978-0-643-10218-7";
  skos:broader s:09I;
  skos:definition <https://raw.githack.com/ANZSoilData/def-au-scma/master/html/09-P/09I4b.html>;
  skos:inScheme s:scma-2011;
  skos:notation "09I4b";
  skos:prefLabel "P buffer index - PBI (unadj) - ICPAES|P buffer index - PBI (unadj)" .

s:09I4c a skos:Concept, sosa:Procedure;
  dct:identifier "http://anzsoil.org/def/au/scma/09I4c"^^xsd:anyURI;
  dct:source "URN:ISBN:978-0-643-10218-7";
  skos:broader s:09I;
  skos:definition <https://raw.githack.com/ANZSoilData/def-au-scma/master/html/09-P/09I4c.html>;
  skos:inScheme s:scma-2011;
  skos:notation "09I4c";
  skos:prefLabel "P buffer index - PBI (unadj)|P buffer index - PBI (unadj) - Vanadate" .

s:09J a skos:Concept, sosa:Procedure;
  dct:identifier "http://anzsoil.org/def/au/scma/09J"^^xsd:anyURI;
  dct:source "URN:ISBN:978-0-643-10218-7";
  skos:definition <https://raw.githack.com/ANZSoilData/def-au-scma/master/html/09-P/09J.html>;
  skos:inScheme s:scma-2011;
  skos:narrower s:09J1, s:09J2;
  skos:notation "09J";
  skos:prefLabel "Phosphate sorption curve";
  skos:topConceptOf s:scma-2011 .

s:09J1 a skos:Concept, sosa:Procedure;
  dct:identifier "http://anzsoil.org/def/au/scma/09J1"^^xsd:anyURI;
  dct:source "URN:ISBN:978-0-643-10218-7";
  skos:broader s:09J;
  skos:definition <https://raw.githack.com/ANZSoilData/def-au-scma/master/html/09-P/09J1.html>;
  skos:inScheme s:scma-2011;
  skos:notation "09J1";
  skos:prefLabel "Phosphate sorption curve - manual colour" .

s:09J2 a skos:Concept, sosa:Procedure;
  dct:identifier "http://anzsoil.org/def/au/scma/09J2"^^xsd:anyURI;
  dct:source "URN:ISBN:978-0-643-10218-7";
  skos:broader s:09J;
  skos:definition <https://raw.githack.com/ANZSoilData/def-au-scma/master/html/09-P/09J2.html>;
  skos:inScheme s:scma-2011;
  skos:notation "09J2";
  skos:prefLabel "Phosphate sorption curve - continuous segmented flow/FIA automated colour" .

s:09K a skos:Concept, sosa:Procedure;
  dct:identifier "http://anzsoil.org/def/au/scma/09K"^^xsd:anyURI;
  dct:source "URN:ISBN:978-0-643-10218-7";
  skos:definition <https://raw.githack.com/ANZSoilData/def-au-scma/master/html/09-P/09K.html>;
  skos:inScheme s:scma-2011;
  skos:narrower s:09K1a, s:09K1b, s:09K2;
  skos:notation "09K";
  skos:prefLabel "Environmental soil P tests";
  skos:topConceptOf s:scma-2011 .

s:09K1a a skos:Concept, sosa:Procedure;
  dct:identifier "http://anzsoil.org/def/au/scma/09K1a"^^xsd:anyURI;
  dct:source "URN:ISBN:978-0-643-10218-7";
  skos:broader s:09K;
  skos:definition <https://raw.githack.com/ANZSoilData/def-au-scma/master/html/09-P/09K1a.html>;
  skos:inScheme s:scma-2011;
  skos:notation "09K1a";
  skos:prefLabel "Mehlich 3-P saturation ratio (M3PSR colour) [colormetric estimate of P]" .

s:09K1b a skos:Concept, sosa:Procedure;
  dct:identifier "http://anzsoil.org/def/au/scma/09K1b"^^xsd:anyURI;
  dct:source "URN:ISBN:978-0-643-10218-7";
  skos:broader s:09K;
  skos:definition <https://raw.githack.com/ANZSoilData/def-au-scma/master/html/09-P/09K1b.html>;
  skos:inScheme s:scma-2011;
  skos:notation "09K1b";
  skos:prefLabel "Mehlich 3-P saturation ratio (M3PSR ICPAES) [ICPAES estimate of P]" .

s:09K2 a skos:Concept, sosa:Procedure;
  dct:identifier "http://anzsoil.org/def/au/scma/09K2"^^xsd:anyURI;
  dct:source "URN:ISBN:978-0-643-10218-7";
  skos:broader s:09K;
  skos:definition <https://raw.githack.com/ANZSoilData/def-au-scma/master/html/09-P/09K2.html>;
  skos:inScheme s:scma-2011;
  skos:notation "09K2";
  skos:prefLabel "Colwell-P/PBI (ColP) ratio" .

s:10 a skos:Collection;
  dct:identifier "http://anzsoil.org/def/au/scma/10"^^xsd:anyURI;
  dct:source "URN:ISBN:978-0-643-10218-7";
  skos:definition <https://raw.githack.com/ANZSoilData/def-au-scma/master/html/10-S/10.html>;
  skos:inScheme s:scma-2011;
  skos:member s:10A1, s:10A2, s:10B, s:10B1, s:10B2, s:10B3, s:10B4, s:10C1, s:10D1;
  skos:notation "10";
  skos:prefLabel "Sulfur" .

s:10A1 a skos:Concept, sosa:Procedure;
  dct:identifier "http://anzsoil.org/def/au/scma/10A1"^^xsd:anyURI;
  dct:source "URN:ISBN:978-0-643-10218-7";
  skos:definition <https://raw.githack.com/ANZSoilData/def-au-scma/master/html/10-S/10A1.html>;
  skos:inScheme s:scma-2011;
  skos:notation "10A1";
  skos:prefLabel "Total S - X-ray fluorescence";
  skos:topConceptOf s:scma-2011 .

s:10A2 a skos:Concept, sosa:Procedure;
  dct:identifier "http://anzsoil.org/def/au/scma/10A2"^^xsd:anyURI;
  dct:source "URN:ISBN:978-0-643-10218-7";
  skos:definition <https://raw.githack.com/ANZSoilData/def-au-scma/master/html/10-S/10A2.html>;
  skos:inScheme s:scma-2011;
  skos:notation "10A2";
  skos:prefLabel "Total soil S - high-temperature combustion";
  skos:topConceptOf s:scma-2011 .

s:10B a skos:Concept, sosa:Procedure;
  dct:identifier "http://anzsoil.org/def/au/scma/10B"^^xsd:anyURI;
  dct:source "URN:ISBN:978-0-643-10218-7";
  skos:definition <https://raw.githack.com/ANZSoilData/def-au-scma/master/html/10-S/10B.html>;
  skos:inScheme s:scma-2011;
  skos:narrower s:10B1, s:10B2, s:10B3, s:10B4;
  skos:notation "10B";
  skos:prefLabel "Calcium phosphate-extractable S";
  skos:topConceptOf s:scma-2011 .

s:10B1 a skos:Concept, sosa:Procedure;
  dct:identifier "http://anzsoil.org/def/au/scma/10B1"^^xsd:anyURI;
  dct:source "URN:ISBN:978-0-643-10218-7";
  skos:broader s:10B;
  skos:definition <https://raw.githack.com/ANZSoilData/def-au-scma/master/html/10-S/10B1.html>;
  skos:inScheme s:scma-2011;
  skos:notation "10B1";
  skos:prefLabel "Calcium phosphate-extractable S - manual distillation" .

s:10B2 a skos:Concept, sosa:Procedure;
  dct:identifier "http://anzsoil.org/def/au/scma/10B2"^^xsd:anyURI;
  dct:source "URN:ISBN:978-0-643-10218-7";
  skos:broader s:10B;
  skos:definition <https://raw.githack.com/ANZSoilData/def-au-scma/master/html/10-S/10B2.html>;
  skos:inScheme s:scma-2011;
  skos:notation "10B2";
  skos:prefLabel "Calcium phosphate-extractable S - automated distillation" .

s:10B3 a skos:Concept, sosa:Procedure;
  dct:identifier "http://anzsoil.org/def/au/scma/10B3"^^xsd:anyURI;
  dct:source "URN:ISBN:978-0-643-10218-7";
  skos:broader s:10B;
  skos:definition <https://raw.githack.com/ANZSoilData/def-au-scma/master/html/10-S/10B3.html>;
  skos:inScheme s:scma-2011;
  skos:notation "10B3";
  skos:prefLabel "Calcium phosphate-extractable S - ICPAES" .

s:10B4 a skos:Concept, sosa:Procedure;
  dct:identifier "http://anzsoil.org/def/au/scma/10B4"^^xsd:anyURI;
  dct:source "URN:ISBN:978-0-643-10218-7";
  skos:broader s:10B;
  skos:definition <https://raw.githack.com/ANZSoilData/def-au-scma/master/html/10-S/10B4.html>;
  skos:inScheme s:scma-2011;
  skos:notation "10B4";
  skos:prefLabel "Calcium phosphate-extractable S - ion chromatography" .

s:10C1 a skos:Concept, sosa:Procedure;
  dct:identifier "http://anzsoil.org/def/au/scma/10C1"^^xsd:anyURI;
  dct:source "URN:ISBN:978-0-643-10218-7";
  skos:definition <https://raw.githack.com/ANZSoilData/def-au-scma/master/html/10-S/10C1.html>;
  skos:inScheme s:scma-2011;
  skos:notation "10C1";
  skos:prefLabel "Calcium phosphate-extractable S - ICPAES, + charcoal (CPC-S)";
  skos:topConceptOf s:scma-2011 .

s:10D1 a skos:Concept, sosa:Procedure;
  dct:identifier "http://anzsoil.org/def/au/scma/10D1"^^xsd:anyURI;
  dct:source "URN:ISBN:978-0-643-10218-7";
  skos:definition <https://raw.githack.com/ANZSoilData/def-au-scma/master/html/10-S/10D1.html>;
  skos:inScheme s:scma-2011;
  skos:notation "10D1";
  skos:prefLabel "Potassium Chloride - 40 Sulfur (KCl-40)-S";
  skos:topConceptOf s:scma-2011 .

s:11 a skos:Collection;
  dct:identifier "http://anzsoil.org/def/au/scma/11"^^xsd:anyURI;
  dct:source "URN:ISBN:978-0-643-10218-7";
  skos:definition <https://raw.githack.com/ANZSoilData/def-au-scma/master/html/11-gypsum/11.html>;
  skos:inScheme s:scma-2011;
  skos:member s:11A1, s:11A2;
  skos:notation "11";
  skos:prefLabel "Gypsum" .

s:11A1 a skos:Concept, sosa:Procedure;
  dct:identifier "http://anzsoil.org/def/au/scma/11A1"^^xsd:anyURI;
  dct:source "URN:ISBN:978-0-643-10218-7";
  skos:definition <https://raw.githack.com/ANZSoilData/def-au-scma/master/html/11-gypsum/11A1.html>;
  skos:inScheme s:scma-2011;
  skos:notation "11A1";
  skos:prefLabel "Total gypsum";
  skos:topConceptOf s:scma-2011 .

s:11A2 a skos:Concept, sosa:Procedure;
  dct:identifier "http://anzsoil.org/def/au/scma/11A2"^^xsd:anyURI;
  dct:source "URN:ISBN:978-0-643-10218-7";
  skos:definition <https://raw.githack.com/ANZSoilData/def-au-scma/master/html/11-gypsum/11A2.html>;
  skos:inScheme s:scma-2011;
  skos:notation "11A2";
  skos:prefLabel "Total gypsum by MIR reflectance spectroscopy";
  skos:topConceptOf s:scma-2011 .

s:12 a skos:Collection;
  dct:identifier "http://anzsoil.org/def/au/scma/12"^^xsd:anyURI;
  dct:source "URN:ISBN:978-0-643-10218-7";
  skos:definition <https://raw.githack.com/ANZSoilData/def-au-scma/master/html/12-micronutrients/12.html>;
  skos:inScheme s:scma-2011;
  skos:member s:12A1, s:12B1, s:12C1, s:12C2, s:12D1, s:12E1;
  skos:notation "12";
  skos:prefLabel "Micronutrients" .

s:12A1 a skos:Concept, sosa:Procedure;
  dct:identifier "http://anzsoil.org/def/au/scma/12A1"^^xsd:anyURI;
  dct:source "URN:ISBN:978-0-643-10218-7";
  skos:definition <https://raw.githack.com/ANZSoilData/def-au-scma/master/html/12-micronutrients/12A1.html>;
  skos:inScheme s:scma-2011;
  skos:notation "12A1";
  skos:prefLabel "DTPA-extractable Cu, Zn, Mn and Fe";
  skos:topConceptOf s:scma-2011 .

s:12B1 a skos:Concept, sosa:Procedure;
  dct:identifier "http://anzsoil.org/def/au/scma/12B1"^^xsd:anyURI;
  dct:source "URN:ISBN:978-0-643-10218-7";
  skos:definition <https://raw.githack.com/ANZSoilData/def-au-scma/master/html/12-micronutrients/12B1.html>;
  skos:inScheme s:scma-2011;
  skos:notation "12B1";
  skos:prefLabel "Ammonium bicarbonate/EDTA-extractable Cu and Zn";
  skos:topConceptOf s:scma-2011 .

s:12C1 a skos:Concept, sosa:Procedure;
  dct:identifier "http://anzsoil.org/def/au/scma/12C1"^^xsd:anyURI;
  dct:source "URN:ISBN:978-0-643-10218-7";
  skos:definition <https://raw.githack.com/ANZSoilData/def-au-scma/master/html/12-micronutrients/12C1.html>;
  skos:inScheme s:scma-2011;
  skos:notation "12C1";
  skos:prefLabel "Calcium chloride-extractable B - manual colour";
  skos:topConceptOf s:scma-2011 .

s:12C2 a skos:Concept, sosa:Procedure;
  dct:identifier "http://anzsoil.org/def/au/scma/12C2"^^xsd:anyURI;
  dct:source "URN:ISBN:978-0-643-10218-7";
  skos:definition <https://raw.githack.com/ANZSoilData/def-au-scma/master/html/12-micronutrients/12C2.html>;
  skos:inScheme s:scma-2011;
  skos:notation "12C2";
  skos:prefLabel "Calcium chloride-extractable B - ICPAES";
  skos:topConceptOf s:scma-2011 .

s:12D1 a skos:Concept, sosa:Procedure;
  dct:identifier "http://anzsoil.org/def/au/scma/12D1"^^xsd:anyURI;
  dct:source "URN:ISBN:978-0-643-10218-7";
  skos:definition <https://raw.githack.com/ANZSoilData/def-au-scma/master/html/12-micronutrients/12D1.html>;
  skos:inScheme s:scma-2011;
  skos:notation "12D1";
  skos:prefLabel "0.1 M HCl-extractable Cu, Zn, Mn and Fe";
  skos:topConceptOf s:scma-2011 .

s:12E1 a skos:Concept, sosa:Procedure;
  dct:identifier "http://anzsoil.org/def/au/scma/12E1"^^xsd:anyURI;
  dct:source "URN:ISBN:978-0-643-10218-7";
  skos:definition <https://raw.githack.com/ANZSoilData/def-au-scma/master/html/12-micronutrients/12E1.html>;
  skos:inScheme s:scma-2011;
  skos:notation "12E1";
  skos:prefLabel "Calcium chloride-extractable Mo";
  skos:topConceptOf s:scma-2011 .

s:13 a skos:Collection;
  dct:identifier "http://anzsoil.org/def/au/scma/13"^^xsd:anyURI;
  dct:source "URN:ISBN:978-0-643-10218-7";
  skos:definition <https://raw.githack.com/ANZSoilData/def-au-scma/master/html/13-extractable-Fe-Al-Si/13.html>;
  skos:inScheme s:scma-2011;
  skos:member s:13A1, s:13B1, s:13C1, s:13D, s:13D1, s:13D2;
  skos:notation "13";
  skos:prefLabel "Extractable iron, aluminium and silicon" .

s:13A1 a skos:Concept, sosa:Procedure;
  dct:identifier "http://anzsoil.org/def/au/scma/13A1"^^xsd:anyURI;
  dct:source "URN:ISBN:978-0-643-10218-7";
  skos:definition <https://raw.githack.com/ANZSoilData/def-au-scma/master/html/13-extractable-Fe-Al-Si/13A1.html>;
  skos:inScheme s:scma-2011;
  skos:notation "13A1";
  skos:prefLabel "Oxalate-extractable iron, aluminium and silicon";
  skos:topConceptOf s:scma-2011 .

s:13B1 a skos:Concept, sosa:Procedure;
  dct:identifier "http://anzsoil.org/def/au/scma/13B1"^^xsd:anyURI;
  dct:source "URN:ISBN:978-0-643-10218-7";
  skos:definition <https://raw.githack.com/ANZSoilData/def-au-scma/master/html/13-extractable-Fe-Al-Si/13B1.html>;
  skos:inScheme s:scma-2011;
  skos:notation "13B1";
  skos:prefLabel "Pyrophosphate-extractable Fe and Al";
  skos:topConceptOf s:scma-2011 .

s:13C1 a skos:Concept, sosa:Procedure;
  dct:identifier "http://anzsoil.org/def/au/scma/13C1"^^xsd:anyURI;
  dct:source "URN:ISBN:978-0-643-10218-7";
  skos:definition <https://raw.githack.com/ANZSoilData/def-au-scma/master/html/13-extractable-Fe-Al-Si/13C1.html>;
  skos:inScheme s:scma-2011;
  skos:notation "13C1";
  skos:prefLabel "Citrate/dihionite-extractable iron and aluminium";
  skos:topConceptOf s:scma-2011 .

s:13D a skos:Concept, sosa:Procedure;
  dct:identifier "http://anzsoil.org/def/au/scma/13D"^^xsd:anyURI;
  dct:source "URN:ISBN:978-0-643-10218-7";
  skos:definition <https://raw.githack.com/ANZSoilData/def-au-scma/master/html/13-extractable-Fe-Al-Si/13D.html>;
  skos:inScheme s:scma-2011;
  skos:narrower s:13D1, s:13D2;
  skos:notation "13D";
  skos:prefLabel "Acid-extractable soil silicon";
  skos:topConceptOf s:scma-2011 .

s:13D1 a skos:Concept, sosa:Procedure;
  dct:identifier "http://anzsoil.org/def/au/scma/13D1"^^xsd:anyURI;
  dct:source "URN:ISBN:978-0-643-10218-7";
  skos:broader s:13D;
  skos:definition <https://raw.githack.com/ANZSoilData/def-au-scma/master/html/13-extractable-Fe-Al-Si/13D1.html>;
  skos:inScheme s:scma-2011;
  skos:notation "13D1";
  skos:prefLabel "Acid-extractable soil silicon - automated colour" .

s:13D2 a skos:Concept, sosa:Procedure;
  dct:identifier "http://anzsoil.org/def/au/scma/13D2"^^xsd:anyURI;
  dct:source "URN:ISBN:978-0-643-10218-7";
  skos:broader s:13D;
  skos:definition <https://raw.githack.com/ANZSoilData/def-au-scma/master/html/13-extractable-Fe-Al-Si/13D2.html>;
  skos:inScheme s:scma-2011;
  skos:notation "13D2";
  skos:prefLabel "Acid-extractable soil silicon - ICPAES" .

s:14 a skos:Collection;
  dct:identifier "http://anzsoil.org/def/au/scma/14"^^xsd:anyURI;
  dct:source "URN:ISBN:978-0-643-10218-7";
  skos:definition <https://raw.githack.com/ANZSoilData/def-au-scma/master/html/14-saturation-extracts/14.html>;
  skos:inScheme s:scma-2011;
  skos:member s:14A1, s:14A2, s:14A3, s:14A4, s:14B1, s:14C1, s:14D1, s:14D2, s:14E1,
    s:14E2, s:14E2a, s:14E2b, s:14E3, s:14F1, s:14F2, s:14F3, s:14F4, s:14F5, s:14F5a,
    s:14F5b, s:14G1, s:14G2, s:14G2a, s:14G2b, s:14H1;
  skos:notation "14";
  skos:prefLabel "Saturation extracts" .

s:14A1 a skos:Concept, sosa:Procedure;
  dct:identifier "http://anzsoil.org/def/au/scma/14A1"^^xsd:anyURI;
  dct:source "URN:ISBN:978-0-643-10218-7";
  skos:definition <https://raw.githack.com/ANZSoilData/def-au-scma/master/html/14-saturation-extracts/14A1.html>;
  skos:inScheme s:scma-2011;
  skos:notation "14A1";
  skos:prefLabel "Saturation extract - filter suction";
  skos:topConceptOf s:scma-2011 .

s:14A2 a skos:Concept, sosa:Procedure;
  dct:identifier "http://anzsoil.org/def/au/scma/14A2"^^xsd:anyURI;
  dct:source "URN:ISBN:978-0-643-10218-7";
  skos:definition <https://raw.githack.com/ANZSoilData/def-au-scma/master/html/14-saturation-extracts/14A2.html>;
  skos:inScheme s:scma-2011;
  skos:notation "14A2";
  skos:prefLabel "Saturation extract -automatic extractor";
  skos:topConceptOf s:scma-2011 .

s:14A3 a skos:Concept, sosa:Procedure;
  dct:identifier "http://anzsoil.org/def/au/scma/14A3"^^xsd:anyURI;
  dct:source "URN:ISBN:978-0-643-10218-7";
  skos:definition <https://raw.githack.com/ANZSoilData/def-au-scma/master/html/14-saturation-extracts/14A3.html>;
  skos:inScheme s:scma-2011;
  skos:notation "14A3";
  skos:prefLabel "Saturation extract - centrifuge, closed system";
  skos:topConceptOf s:scma-2011 .

s:14A4 a skos:Concept, sosa:Procedure;
  dct:identifier "http://anzsoil.org/def/au/scma/14A4"^^xsd:anyURI;
  dct:source "URN:ISBN:978-0-643-10218-7";
  skos:definition <https://raw.githack.com/ANZSoilData/def-au-scma/master/html/14-saturation-extracts/14A4.html>;
  skos:inScheme s:scma-2011;
  skos:notation "14A4";
  skos:prefLabel "Saturation extract - centrifuge, Gillman";
  skos:topConceptOf s:scma-2011 .

s:14B1 a skos:Concept, sosa:Procedure;
  dct:identifier "http://anzsoil.org/def/au/scma/14B1"^^xsd:anyURI;
  dct:source "URN:ISBN:978-0-643-10218-7";
  skos:definition <https://raw.githack.com/ANZSoilData/def-au-scma/master/html/14-saturation-extracts/14B1.html>;
  skos:inScheme s:scma-2011;
  skos:notation "14B1";
  skos:prefLabel "Electrical conductivity of SE (EC of SE)";
  skos:topConceptOf s:scma-2011 .

s:14C1 a skos:Concept, sosa:Procedure;
  dct:identifier "http://anzsoil.org/def/au/scma/14C1"^^xsd:anyURI;
  dct:source "URN:ISBN:978-0-643-10218-7";
  skos:definition <https://raw.githack.com/ANZSoilData/def-au-scma/master/html/14-saturation-extracts/14C1.html>;
  skos:inScheme s:scma-2011;
  skos:notation "14C1";
  skos:prefLabel "pH of SE";
  skos:topConceptOf s:scma-2011 .

s:14D1 a skos:Concept, sosa:Procedure;
  dct:identifier "http://anzsoil.org/def/au/scma/14D1"^^xsd:anyURI;
  dct:source "URN:ISBN:978-0-643-10218-7";
  skos:definition <https://raw.githack.com/ANZSoilData/def-au-scma/master/html/14-saturation-extracts/14D1.html>;
  skos:inScheme s:scma-2011;
  skos:notation "14D1";
  skos:prefLabel "Bicarbonate of SE and carbonate of SE - potentiometric titration";
  skos:topConceptOf s:scma-2011 .

s:14D2 a skos:Concept, sosa:Procedure;
  dct:identifier "http://anzsoil.org/def/au/scma/14D2"^^xsd:anyURI;
  dct:source "URN:ISBN:978-0-643-10218-7";
  skos:definition <https://raw.githack.com/ANZSoilData/def-au-scma/master/html/14-saturation-extracts/14D2.html>;
  skos:inScheme s:scma-2011;
  skos:notation "14D2";
  skos:prefLabel "Bicarbonate of SE and carbonate of SE - indicator method";
  skos:topConceptOf s:scma-2011 .

s:14E1 a skos:Concept, sosa:Procedure;
  dct:identifier "http://anzsoil.org/def/au/scma/14E1"^^xsd:anyURI;
  dct:source "URN:ISBN:978-0-643-10218-7";
  skos:definition <https://raw.githack.com/ANZSoilData/def-au-scma/master/html/14-saturation-extracts/14E1.html>;
  skos:inScheme s:scma-2011;
  skos:notation "14E1";
  skos:prefLabel "Chloride of SE - potentiometric titration";
  skos:topConceptOf s:scma-2011 .

s:14E2 a skos:Concept, sosa:Procedure;
  dct:identifier "http://anzsoil.org/def/au/scma/14E2"^^xsd:anyURI;
  dct:isReplacedBy s:14E2a, s:14E2b;
  dct:source "URN:ISBN:978-0-909605-68-1";
  skos:inScheme s:scma-2011;
  skos:narrower s:14E2a, s:14E2b;
  skos:notation "14E2";
  skos:prefLabel "Chloride (saturation extract) - ion chromotography|Chloride of SE - IC";
  skos:topConceptOf s:scma-2011 .

s:14E2a a skos:Concept, sosa:Procedure;
  dct:identifier "http://anzsoil.org/def/au/scma/14E2a"^^xsd:anyURI;
  dct:source "URN:ISBN:978-0-643-10218-7";
  skos:broader s:14E2;
  skos:definition <https://raw.githack.com/ANZSoilData/def-au-scma/master/html/14-saturation-extracts/14E2a.html>;
  skos:inScheme s:scma-2011;
  skos:notation "14E2a";
  skos:prefLabel "Chloride of SE - IC (chemical suppression of eluent conductivity)" .

s:14E2b a skos:Concept, sosa:Procedure;
  dct:identifier "http://anzsoil.org/def/au/scma/14E2b"^^xsd:anyURI;
  dct:source "URN:ISBN:978-0-643-10218-7";
  skos:broader s:14E2;
  skos:definition <https://raw.githack.com/ANZSoilData/def-au-scma/master/html/14-saturation-extracts/14E2b.html>;
  skos:inScheme s:scma-2011;
  skos:notation "14E2b";
  skos:prefLabel "Chloride of SE - IC (single-column with electronic suppression of eluent conductivity)" .

s:14E3 a skos:Concept, sosa:Procedure;
  dct:identifier "http://anzsoil.org/def/au/scma/14E3"^^xsd:anyURI;
  dct:source "URN:ISBN:978-0-643-10218-7";
  skos:definition <https://raw.githack.com/ANZSoilData/def-au-scma/master/html/14-saturation-extracts/14E3.html>;
  skos:inScheme s:scma-2011;
  skos:notation "14E3";
  skos:prefLabel "Chloride of SE - ICPAES";
  skos:topConceptOf s:scma-2011 .

s:14F1 a skos:Concept, sosa:Procedure;
  dct:identifier "http://anzsoil.org/def/au/scma/14F1"^^xsd:anyURI;
  dct:source "URN:ISBN:978-0-643-10218-7";
  skos:definition <https://raw.githack.com/ANZSoilData/def-au-scma/master/html/14-saturation-extracts/14F1.html>;
  skos:inScheme s:scma-2011;
  skos:notation "14F1";
  skos:prefLabel "Sulfate-S of SE - ICPAES (plus P and soluble cations)";
  skos:topConceptOf s:scma-2011 .

s:14F2 a skos:Concept, sosa:Procedure;
  dct:identifier "http://anzsoil.org/def/au/scma/14F2"^^xsd:anyURI;
  dct:source "URN:ISBN:978-0-643-10218-7";
  skos:definition <https://raw.githack.com/ANZSoilData/def-au-scma/master/html/14-saturation-extracts/14F2.html>;
  skos:inScheme s:scma-2011;
  skos:notation "14F2";
  skos:prefLabel "Sulfate-S of SE - turbidimetric";
  skos:topConceptOf s:scma-2011 .

s:14F3 a skos:Concept, sosa:Procedure;
  dct:identifier "http://anzsoil.org/def/au/scma/14F3"^^xsd:anyURI;
  dct:source "URN:ISBN:978-0-643-10218-7";
  skos:definition <https://raw.githack.com/ANZSoilData/def-au-scma/master/html/14-saturation-extracts/14F3.html>;
  skos:inScheme s:scma-2011;
  skos:notation "14F3";
  skos:prefLabel "Sulfate-S of SE - gravimetric";
  skos:topConceptOf s:scma-2011 .

s:14F4 a skos:Concept, sosa:Procedure;
  dct:identifier "http://anzsoil.org/def/au/scma/14F4"^^xsd:anyURI;
  dct:source "URN:ISBN:978-0-643-10218-7";
  skos:definition <https://raw.githack.com/ANZSoilData/def-au-scma/master/html/14-saturation-extracts/14F4.html>;
  skos:inScheme s:scma-2011;
  skos:notation "14F4";
  skos:prefLabel "Sulfate-S of SE - automated colour";
  skos:topConceptOf s:scma-2011 .

s:14F5 a skos:Concept, sosa:Procedure;
  dct:identifier "http://anzsoil.org/def/au/scma/14F5"^^xsd:anyURI;
  dct:isReplacedBy s:14F5a, s:14F5b;
  dct:source "URN:ISBN:978-0-909605-68-1";
  skos:inScheme s:scma-2011;
  skos:narrower s:14F5a, s:14F5b;
  skos:notation "14F5";
  skos:prefLabel "Sulfate-S (saturation extract) - ion chromotography|Sulfate-S of SE - IC";
  skos:topConceptOf s:scma-2011 .

s:14F5a a skos:Concept, sosa:Procedure;
  dct:identifier "http://anzsoil.org/def/au/scma/14F5a"^^xsd:anyURI;
  dct:source "URN:ISBN:978-0-643-10218-7";
  skos:broader s:14F5;
  skos:definition <https://raw.githack.com/ANZSoilData/def-au-scma/master/html/14-saturation-extracts/14F5a.html>;
  skos:inScheme s:scma-2011;
  skos:notation "14F5a";
  skos:prefLabel "Sulfate-S of SE - IC (chemical suppression of eluent conductivity)" .

s:14F5b a skos:Concept, sosa:Procedure;
  dct:identifier "http://anzsoil.org/def/au/scma/14F5b"^^xsd:anyURI;
  dct:source "URN:ISBN:978-0-643-10218-7";
  skos:broader s:14F5;
  skos:definition <https://raw.githack.com/ANZSoilData/def-au-scma/master/html/14-saturation-extracts/14F5b.html>;
  skos:inScheme s:scma-2011;
  skos:notation "14F5b";
  skos:prefLabel "Sulfate-S of SE - IC (single-column with electronic suppression of eluent conductivity)" .

s:14G1 a skos:Concept, sosa:Procedure;
  dct:identifier "http://anzsoil.org/def/au/scma/14G1"^^xsd:anyURI;
  dct:source "URN:ISBN:978-0-643-10218-7";
  skos:definition <https://raw.githack.com/ANZSoilData/def-au-scma/master/html/14-saturation-extracts/14G1.html>;
  skos:inScheme s:scma-2011;
  skos:notation "14G1";
  skos:prefLabel "Fluoride of SE - specific ion electrode";
  skos:topConceptOf s:scma-2011 .

s:14G2 a skos:Concept, sosa:Procedure;
  dct:identifier "http://anzsoil.org/def/au/scma/14G2"^^xsd:anyURI;
  dct:isReplacedBy s:14G2a, s:14G2b;
  dct:source "URN:ISBN:978-0-909605-68-1";
  skos:inScheme s:scma-2011;
  skos:narrower s:14G2a, s:14G2b;
  skos:notation "14G2";
  skos:prefLabel "Fluoride (saturation extract) - ion chromotography|Fluoride of SE - IC";
  skos:topConceptOf s:scma-2011 .

s:14G2a a skos:Concept, sosa:Procedure;
  dct:identifier "http://anzsoil.org/def/au/scma/14G2a"^^xsd:anyURI;
  dct:source "URN:ISBN:978-0-643-10218-7";
  skos:broader s:14G2;
  skos:definition <https://raw.githack.com/ANZSoilData/def-au-scma/master/html/14-saturation-extracts/14G2a.html>;
  skos:inScheme s:scma-2011;
  skos:notation "14G2a";
  skos:prefLabel "Fluoride of SE - IC (chemical suppression of eluent conductivity)" .

s:14G2b a skos:Concept, sosa:Procedure;
  dct:identifier "http://anzsoil.org/def/au/scma/14G2b"^^xsd:anyURI;
  dct:source "URN:ISBN:978-0-643-10218-7";
  skos:broader s:14G2;
  skos:definition <https://raw.githack.com/ANZSoilData/def-au-scma/master/html/14-saturation-extracts/14G2b.html>;
  skos:inScheme s:scma-2011;
  skos:notation "14G2b";
  skos:prefLabel "Fluoride of SE - IC (single-column with electronic suppression of eluent conductivity)" .

s:14H1 a skos:Concept, sosa:Procedure;
  dct:identifier "http://anzsoil.org/def/au/scma/14H1"^^xsd:anyURI;
  dct:source "URN:ISBN:978-0-643-10218-7";
  skos:definition <https://raw.githack.com/ANZSoilData/def-au-scma/master/html/14-saturation-extracts/14H1.html>;
  skos:inScheme s:scma-2011;
  skos:notation "14H1";
  skos:prefLabel "Soluble bases of SE (Ca, Mg, K, Na)";
  skos:topConceptOf s:scma-2011 .

s:15 a skos:Collection;
  dct:identifier "http://anzsoil.org/def/au/scma/15"^^xsd:anyURI;
  dct:source "URN:ISBN:978-0-643-10218-7";
  skos:definition <https://raw.githack.com/ANZSoilData/def-au-scma/master/html/15-ion-exchange-properties/15.html>;
  skos:inScheme s:scma-2011;
  skos:member s:15A1, s:15A2, s:15A3, s:15B1, s:15B2, s:15B3, s:15C1, s:15C2, s:15D1,
    s:15D2, s:15D3, s:15E1, s:15E2, s:15E3, s:15F1, s:15F2, s:15F3, s:15G1, s:15H1, s:15I1,
    s:15I2, s:15I3, s:15I4, s:15J1, s:15K1, s:15L1, s:15M1, s:15N1, s:15O1;
  skos:notation "15";
  skos:prefLabel "Ion-exchange properties" .

s:15A1 a skos:Concept, sosa:Procedure;
  dct:identifier "http://anzsoil.org/def/au/scma/15A1"^^xsd:anyURI;
  dct:source "URN:ISBN:978-0-643-10218-7";
  skos:definition <https://raw.githack.com/ANZSoilData/def-au-scma/master/html/15-ion-exchange-properties/15A1.html>;
  skos:inScheme s:scma-2011;
  skos:notation "15A1";
  skos:prefLabel "Exchangeable bases (Ca2+, Mg2+, Na+, K+) - 1 M ammonium chloride at pH 7.0, no pre-treatment for soluble salts";
  skos:topConceptOf s:scma-2011 .

s:15A2 a skos:Concept, sosa:Procedure;
  dct:identifier "http://anzsoil.org/def/au/scma/15A2"^^xsd:anyURI;
  dct:source "URN:ISBN:978-0-643-10218-7";
  skos:definition <https://raw.githack.com/ANZSoilData/def-au-scma/master/html/15-ion-exchange-properties/15A2.html>;
  skos:inScheme s:scma-2011;
  skos:notation "15A2";
  skos:prefLabel "Exchangeable bases by 1 M ammonium chloride at pH 7.0, pre-treatment for soluble salts";
  skos:topConceptOf s:scma-2011 .

s:15A3 a skos:Concept, sosa:Procedure;
  dct:identifier "http://anzsoil.org/def/au/scma/15A3"^^xsd:anyURI;
  dct:source "URN:ISBN:978-0-643-10218-7";
  skos:definition <https://raw.githack.com/ANZSoilData/def-au-scma/master/html/15-ion-exchange-properties/15A3.html>;
  skos:inScheme s:scma-2011;
  skos:notation "15A3";
  skos:prefLabel "Exchangeable bases - 1 M ammonium chloride at pH 7.0, adjusted for soluble Na+";
  skos:topConceptOf s:scma-2011 .

s:15B1 a skos:Concept, sosa:Procedure;
  dct:identifier "http://anzsoil.org/def/au/scma/15B1"^^xsd:anyURI;
  dct:source "URN:ISBN:978-0-643-10218-7";
  skos:definition <https://raw.githack.com/ANZSoilData/def-au-scma/master/html/15-ion-exchange-properties/15B1.html>;
  skos:inScheme s:scma-2011;
  skos:notation "15B1";
  skos:prefLabel "Exchangeable bases and cation exchange capacity - 1 M ammonium chloride at pH 7.0, no pre-treatment for soluble salts";
  skos:topConceptOf s:scma-2011 .

s:15B2 a skos:Concept, sosa:Procedure;
  dct:identifier "http://anzsoil.org/def/au/scma/15B2"^^xsd:anyURI;
  dct:source "URN:ISBN:978-0-643-10218-7";
  skos:definition <https://raw.githack.com/ANZSoilData/def-au-scma/master/html/15-ion-exchange-properties/15B2.html>;
  skos:inScheme s:scma-2011;
  skos:notation "15B2";
  skos:prefLabel "Exchangeable bases and CEC - 1 M ammonium chloride at pH 7.0, pre-treatment for soluble salts";
  skos:topConceptOf s:scma-2011 .

s:15B3 a skos:Concept, sosa:Procedure;
  dct:identifier "http://anzsoil.org/def/au/scma/15B3"^^xsd:anyURI;
  dct:source "URN:ISBN:978-0-643-10218-7";
  skos:definition <https://raw.githack.com/ANZSoilData/def-au-scma/master/html/15-ion-exchange-properties/15B3.html>;
  skos:inScheme s:scma-2011;
  skos:notation "15B3";
  skos:prefLabel "Exchangeable bases and CEC - 1 M ammonium chloride at pH 7.0, adjusted for soluble Na+";
  skos:topConceptOf s:scma-2011 .

s:15C1 a skos:Concept, sosa:Procedure;
  dct:identifier "http://anzsoil.org/def/au/scma/15C1"^^xsd:anyURI;
  dct:source "URN:ISBN:978-0-643-10218-7";
  skos:definition <https://raw.githack.com/ANZSoilData/def-au-scma/master/html/15-ion-exchange-properties/15C1.html>;
  skos:inScheme s:scma-2011;
  skos:notation "15C1";
  skos:prefLabel "Exchangeable bases and CEC - alcoholic 1 M ammonium chloride at pH 8.5, pre-treatment for soluble salts";
  skos:topConceptOf s:scma-2011 .

s:15C2 a skos:Concept, sosa:Procedure;
  dct:identifier "http://anzsoil.org/def/au/scma/15C2"^^xsd:anyURI;
  dct:source "URN:ISBN:978-0-643-10218-7";
  skos:definition <https://raw.githack.com/ANZSoilData/def-au-scma/master/html/15-ion-exchange-properties/15C2.html>;
  skos:inScheme s:scma-2011;
  skos:notation "15C2";
  skos:prefLabel "Exchangeable divalent cations and CEC - by MIR diffuse reflectance spectroscopy";
  skos:topConceptOf s:scma-2011 .

s:15D1 a skos:Concept, sosa:Procedure;
  dct:identifier "http://anzsoil.org/def/au/scma/15D1"^^xsd:anyURI;
  dct:source "URN:ISBN:978-0-643-10218-7";
  skos:definition <https://raw.githack.com/ANZSoilData/def-au-scma/master/html/15-ion-exchange-properties/15D1.html>;
  skos:inScheme s:scma-2011;
  skos:notation "15D1";
  skos:prefLabel "Exchangeable bases and CEC - 1 M ammonium acetate at pH 7.0, pre-treatment for soluble salts, manual leach";
  skos:topConceptOf s:scma-2011 .

s:15D2 a skos:Concept, sosa:Procedure;
  dct:identifier "http://anzsoil.org/def/au/scma/15D2"^^xsd:anyURI;
  dct:source "URN:ISBN:978-0-643-10218-7";
  skos:definition <https://raw.githack.com/ANZSoilData/def-au-scma/master/html/15-ion-exchange-properties/15D2.html>;
  skos:inScheme s:scma-2011;
  skos:notation "15D2";
  skos:prefLabel "Exchangeable bases and CEC - 1 M ammonium acetate at pH 7.0, pre-treatment for soluble salts, automatic extractor";
  skos:topConceptOf s:scma-2011 .

s:15D3 a skos:Concept, sosa:Procedure;
  dct:identifier "http://anzsoil.org/def/au/scma/15D3"^^xsd:anyURI;
  dct:source "URN:ISBN:978-0-643-10218-7";
  skos:definition <https://raw.githack.com/ANZSoilData/def-au-scma/master/html/15-ion-exchange-properties/15D3.html>;
  skos:inScheme s:scma-2011;
  skos:notation "15D3";
  skos:prefLabel "Exchangeable bases and CEC - 1 M ammonium acetate at pH 7.0, rapid method with no pre-treatment for soluble salts";
  skos:topConceptOf s:scma-2011 .

s:15E1 a skos:Concept, sosa:Procedure;
  dct:identifier "http://anzsoil.org/def/au/scma/15E1"^^xsd:anyURI;
  dct:source "URN:ISBN:978-0-643-10218-7";
  skos:definition <https://raw.githack.com/ANZSoilData/def-au-scma/master/html/15-ion-exchange-properties/15E1.html>;
  skos:inScheme s:scma-2011;
  skos:notation "15E1";
  skos:prefLabel "Exchangeable bases, CEC and anion exchange capacity by compulsive exchange, no pre-treatment for soluble salts";
  skos:topConceptOf s:scma-2011 .

s:15E2 a skos:Concept, sosa:Procedure;
  dct:identifier "http://anzsoil.org/def/au/scma/15E2"^^xsd:anyURI;
  dct:source "URN:ISBN:978-0-643-10218-7";
  skos:definition <https://raw.githack.com/ANZSoilData/def-au-scma/master/html/15-ion-exchange-properties/15E2.html>;
  skos:inScheme s:scma-2011;
  skos:notation "15E2";
  skos:prefLabel "Exchangeable bases, CEC and AEC by compulsive exchange, pre-treatment for soluble salts";
  skos:topConceptOf s:scma-2011 .

s:15E3 a skos:Concept, sosa:Procedure;
  dct:identifier "http://anzsoil.org/def/au/scma/15E3"^^xsd:anyURI;
  dct:source "URN:ISBN:978-0-643-10218-7";
  skos:definition <https://raw.githack.com/ANZSoilData/def-au-scma/master/html/15-ion-exchange-properties/15E3.html>;
  skos:inScheme s:scma-2011;
  skos:notation "15E3";
  skos:prefLabel "Exchangeable bases, CEC and AEC by compulsive exchange, adjusted for soluble Na+";
  skos:topConceptOf s:scma-2011 .

s:15F1 a skos:Concept, sosa:Procedure;
  dct:identifier "http://anzsoil.org/def/au/scma/15F1"^^xsd:anyURI;
  dct:source "URN:ISBN:978-0-643-10218-7";
  skos:definition <https://raw.githack.com/ANZSoilData/def-au-scma/master/html/15-ion-exchange-properties/15F1.html>;
  skos:inScheme s:scma-2011;
  skos:notation "15F1";
  skos:prefLabel "Exchangeable bases by 0.01 M silver-thiourea (AgTU+) - no pre-treatment for soluble salts";
  skos:topConceptOf s:scma-2011 .

s:15F2 a skos:Concept, sosa:Procedure;
  dct:identifier "http://anzsoil.org/def/au/scma/15F2"^^xsd:anyURI;
  dct:source "URN:ISBN:978-0-643-10218-7";
  skos:definition <https://raw.githack.com/ANZSoilData/def-au-scma/master/html/15-ion-exchange-properties/15F2.html>;
  skos:inScheme s:scma-2011;
  skos:notation "15F2";
  skos:prefLabel "Exchangeable aluminium by 0.01 M AgTU+";
  skos:topConceptOf s:scma-2011 .

s:15F3 a skos:Concept, sosa:Procedure;
  dct:identifier "http://anzsoil.org/def/au/scma/15F3"^^xsd:anyURI;
  dct:source "URN:ISBN:978-0-643-10218-7";
  skos:definition <https://raw.githack.com/ANZSoilData/def-au-scma/master/html/15-ion-exchange-properties/15F3.html>;
  skos:inScheme s:scma-2011;
  skos:notation "15F3";
  skos:prefLabel "Cation exchange capacity by 0.01 M AgTU+ [CEC AgTU]";
  skos:topConceptOf s:scma-2011 .

s:15G1 a skos:Concept, sosa:Procedure;
  dct:identifier "http://anzsoil.org/def/au/scma/15G1"^^xsd:anyURI;
  dct:source "URN:ISBN:978-0-643-10218-7";
  skos:definition <https://raw.githack.com/ANZSoilData/def-au-scma/master/html/15-ion-exchange-properties/15G1.html>;
  skos:inScheme s:scma-2011;
  skos:notation "15G1";
  skos:prefLabel "Exchange acidity (H+ + Al3+) by 1 M potassium chloride";
  skos:topConceptOf s:scma-2011 .

s:15H1 a skos:Concept, sosa:Procedure;
  dct:identifier "http://anzsoil.org/def/au/scma/15H1"^^xsd:anyURI;
  dct:source "URN:ISBN:978-0-643-10218-7";
  skos:definition <https://raw.githack.com/ANZSoilData/def-au-scma/master/html/15-ion-exchange-properties/15H1.html>;
  skos:inScheme s:scma-2011;
  skos:notation "15H1";
  skos:prefLabel "Exchange acidity by triethanolamine (TEA)";
  skos:topConceptOf s:scma-2011 .

s:15I1 a skos:Concept, sosa:Procedure;
  dct:identifier "http://anzsoil.org/def/au/scma/15I1"^^xsd:anyURI;
  dct:source "URN:ISBN:978-0-643-10218-7";
  skos:definition <https://raw.githack.com/ANZSoilData/def-au-scma/master/html/15-ion-exchange-properties/15I1.html>;
  skos:inScheme s:scma-2011;
  skos:notation "15I1";
  skos:prefLabel "Cation exchange capacity measurement - distillation of NH+4";
  skos:topConceptOf s:scma-2011 .

s:15I2 a skos:Concept, sosa:Procedure;
  dct:identifier "http://anzsoil.org/def/au/scma/15I2"^^xsd:anyURI;
  dct:source "URN:ISBN:978-0-643-10218-7";
  skos:definition <https://raw.githack.com/ANZSoilData/def-au-scma/master/html/15-ion-exchange-properties/15I2.html>;
  skos:inScheme s:scma-2011;
  skos:notation "15I2";
  skos:prefLabel "Cation exchange capacity measurement - automated determination of NH+4";
  skos:topConceptOf s:scma-2011 .

s:15I3 a skos:Concept, sosa:Procedure;
  dct:identifier "http://anzsoil.org/def/au/scma/15I3"^^xsd:anyURI;
  dct:source "URN:ISBN:978-0-643-10218-7";
  skos:definition <https://raw.githack.com/ANZSoilData/def-au-scma/master/html/15-ion-exchange-properties/15I3.html>;
  skos:inScheme s:scma-2011;
  skos:notation "15I3";
  skos:prefLabel "Cation exchange capacity measurement - automated determination of NH+4 and Cl+";
  skos:topConceptOf s:scma-2011 .

s:15I4 a skos:Concept, sosa:Procedure;
  dct:identifier "http://anzsoil.org/def/au/scma/15I4"^^xsd:anyURI;
  dct:source "URN:ISBN:978-0-643-10218-7";
  skos:definition <https://raw.githack.com/ANZSoilData/def-au-scma/master/html/15-ion-exchange-properties/15I4.html>;
  skos:inScheme s:scma-2011;
  skos:notation "15I4";
  skos:prefLabel "Cation exchange capacity measurement - titration of NH+4 and Cl-";
  skos:topConceptOf s:scma-2011 .

s:15J1 a skos:Concept, sosa:Procedure;
  dct:identifier "http://anzsoil.org/def/au/scma/15J1"^^xsd:anyURI;
  dct:source "URN:ISBN:978-0-643-10218-7";
  skos:definition <https://raw.githack.com/ANZSoilData/def-au-scma/master/html/15-ion-exchange-properties/15J1.html>;
  skos:inScheme s:scma-2011;
  skos:notation "15J1";
  skos:prefLabel "Effective cation exchange capacity (ECEC)";
  skos:topConceptOf s:scma-2011 .

s:15K1 a skos:Concept, sosa:Procedure;
  dct:identifier "http://anzsoil.org/def/au/scma/15K1"^^xsd:anyURI;
  dct:source "URN:ISBN:978-0-643-10218-7";
  skos:definition <https://raw.githack.com/ANZSoilData/def-au-scma/master/html/15-ion-exchange-properties/15K1.html>;
  skos:inScheme s:scma-2011;
  skos:notation "15K1";
  skos:prefLabel "Cation exchange capacity - pH 8.2 (CEC pH 8.2)";
  skos:topConceptOf s:scma-2011 .

s:15L1 a skos:Concept, sosa:Procedure;
  dct:identifier "http://anzsoil.org/def/au/scma/15L1"^^xsd:anyURI;
  dct:source "URN:ISBN:978-0-643-10218-7";
  skos:definition <https://raw.githack.com/ANZSoilData/def-au-scma/master/html/15-ion-exchange-properties/15L1.html>;
  skos:inScheme s:scma-2011;
  skos:notation "15L1";
  skos:prefLabel "Base saturation percentage (ESP)";
  skos:topConceptOf s:scma-2011 .

s:15M1 a skos:Concept, sosa:Procedure;
  dct:identifier "http://anzsoil.org/def/au/scma/15M1"^^xsd:anyURI;
  dct:source "URN:ISBN:978-0-643-10218-7";
  skos:definition <https://raw.githack.com/ANZSoilData/def-au-scma/master/html/15-ion-exchange-properties/15M1.html>;
  skos:inScheme s:scma-2011;
  skos:notation "15M1";
  skos:prefLabel "Basic cation saturation ratios";
  skos:topConceptOf s:scma-2011 .

s:15N1 a skos:Concept, sosa:Procedure;
  dct:identifier "http://anzsoil.org/def/au/scma/15N1"^^xsd:anyURI;
  dct:source "URN:ISBN:978-0-643-10218-7";
  skos:definition <https://raw.githack.com/ANZSoilData/def-au-scma/master/html/15-ion-exchange-properties/15N1.html>;
  skos:inScheme s:scma-2011;
  skos:notation "15N1";
  skos:prefLabel "Exchangeable Na+ percentage (ESP)";
  skos:topConceptOf s:scma-2011 .

s:15O1 a skos:Concept, sosa:Procedure;
  dct:identifier "http://anzsoil.org/def/au/scma/15O1"^^xsd:anyURI;
  dct:source "URN:ISBN:978-0-643-10218-7";
  skos:definition <https://raw.githack.com/ANZSoilData/def-au-scma/master/html/15-ion-exchange-properties/15O1.html>;
  skos:inScheme s:scma-2011;
  skos:notation "15O1";
  skos:prefLabel "Percent Al saturation";
  skos:topConceptOf s:scma-2011 .

s:16 a skos:Collection;
  dct:identifier "http://anzsoil.org/def/au/scma/16"^^xsd:anyURI;
  dct:source "URN:ISBN:978-0-643-10218-7";
  skos:definition <https://raw.githack.com/ANZSoilData/def-au-scma/master/html/16-lime-requirement/16.html>;
  skos:inScheme s:scma-2011;
  skos:member s:16A1, s:16B1, s:16C1, s:16D1;
  skos:notation "16";
  skos:prefLabel "Lime requirement" .

s:16A1 a skos:Concept, sosa:Procedure;
  dct:identifier "http://anzsoil.org/def/au/scma/16A1"^^xsd:anyURI;
  dct:source "URN:ISBN:978-0-643-10218-7";
  skos:definition <https://raw.githack.com/ANZSoilData/def-au-scma/master/html/16-lime-requirement/16A.html>;
  skos:inScheme s:scma-2011;
  skos:notation "16A1";
  skos:prefLabel "Calculated lime rate - from exchangeable Al3+";
  skos:topConceptOf s:scma-2011 .

s:16B1 a skos:Concept, sosa:Procedure;
  dct:identifier "http://anzsoil.org/def/au/scma/16B1"^^xsd:anyURI;
  dct:source "URN:ISBN:978-0-643-10218-7";
  skos:definition <https://raw.githack.com/ANZSoilData/def-au-scma/master/html/16-lime-requirement/16B1.html>;
  skos:inScheme s:scma-2011;
  skos:notation "16B1";
  skos:prefLabel "Calculated lime rate - Cregan";
  skos:topConceptOf s:scma-2011 .

s:16C1 a skos:Concept, sosa:Procedure;
  dct:identifier "http://anzsoil.org/def/au/scma/16C1"^^xsd:anyURI;
  dct:source "URN:ISBN:978-0-643-10218-7";
  skos:definition <https://raw.githack.com/ANZSoilData/def-au-scma/master/html/16-lime-requirement/16C1.html>;
  skos:inScheme s:scma-2011;
  skos:notation "16C1";
  skos:prefLabel "Lime requirement - Mehlich single buffer";
  skos:topConceptOf s:scma-2011 .

s:16D1 a skos:Concept, sosa:Procedure;
  dct:identifier "http://anzsoil.org/def/au/scma/16D1"^^xsd:anyURI;
  dct:source "URN:ISBN:978-0-643-10218-7";
  skos:definition <https://raw.githack.com/ANZSoilData/def-au-scma/master/html/16-lime-requirement/16D1.html>;
  skos:inScheme s:scma-2011;
  skos:notation "16D1";
  skos:prefLabel "Lime requirement - Dunn titration curves";
  skos:topConceptOf s:scma-2011 .

s:17 a skos:Collection;
  dct:identifier "http://anzsoil.org/def/au/scma/17"^^xsd:anyURI;
  dct:source "URN:ISBN:978-0-643-10218-7";
  skos:definition <https://raw.githack.com/ANZSoilData/def-au-scma/master/html/17-total-miscellaneous-elements/17.html>;
  skos:inScheme s:scma-2011;
  skos:member s:17A1, s:17A2, s:17B1, s:17B2, s:17C1;
  skos:notation "17";
  skos:prefLabel "Total miscellaneous elements" .

s:17A1 a skos:Concept, sosa:Procedure;
  dct:identifier "http://anzsoil.org/def/au/scma/17A1"^^xsd:anyURI;
  dct:source "URN:ISBN:978-0-643-10218-7";
  skos:definition <https://raw.githack.com/ANZSoilData/def-au-scma/master/html/17-total-miscellaneous-elements/17A1.html>;
  skos:inScheme s:scma-2011;
  skos:notation "17A1";
  skos:prefLabel "Total elemental analysis of soils and sediments -X-ray fluorescence spectroscopy";
  skos:topConceptOf s:scma-2011 .

s:17A2 a skos:Concept, sosa:Procedure;
  dct:identifier "http://anzsoil.org/def/au/scma/17A2"^^xsd:anyURI;
  dct:source "URN:ISBN:978-0-643-10218-7";
  skos:definition <https://raw.githack.com/ANZSoilData/def-au-scma/master/html/17-total-miscellaneous-elements/17A2.html>;
  skos:inScheme s:scma-2011;
  skos:notation "17A2";
  skos:prefLabel "Total elemental analysis of soils and sediments - microwave assisted digestion, with determination by atomic spectroscopy";
  skos:topConceptOf s:scma-2011 .

s:17B1 a skos:Concept, sosa:Procedure;
  dct:identifier "http://anzsoil.org/def/au/scma/17B1"^^xsd:anyURI;
  dct:source "URN:ISBN:978-0-643-10218-7";
  skos:definition <https://raw.githack.com/ANZSoilData/def-au-scma/master/html/17-total-miscellaneous-elements/17B1.html>;
  skos:inScheme s:scma-2011;
  skos:notation "17B1";
  skos:prefLabel "Pseudo-total elemental analysis of soils and sediments - reverse aqua regia block digestion with determination by atomic spectroscopy";
  skos:topConceptOf s:scma-2011 .

s:17B2 a skos:Concept, sosa:Procedure;
  dct:identifier "http://anzsoil.org/def/au/scma/17B2"^^xsd:anyURI;
  dct:source "URN:ISBN:978-0-643-10218-7";
  skos:definition <https://raw.githack.com/ANZSoilData/def-au-scma/master/html/17-total-miscellaneous-elements/17B2.html>;
  skos:inScheme s:scma-2011;
  skos:notation "17B2";
  skos:prefLabel "Pseudo-total elements of soils and sediments - reverse aqua regia microwave assisted digestion of sludges, soils and sediments, with determination by atomic spectroscopy";
  skos:topConceptOf s:scma-2011 .

s:17C1 a skos:Concept, sosa:Procedure;
  dct:identifier "http://anzsoil.org/def/au/scma/17C1"^^xsd:anyURI;
  dct:source "URN:ISBN:978-0-643-10218-7";
  skos:definition <https://raw.githack.com/ANZSoilData/def-au-scma/master/html/17-total-miscellaneous-elements/17C1.html>;
  skos:inScheme s:scma-2011;
  skos:notation "17C1";
  skos:prefLabel "Pseudo-total elements of soils and sediments - conventional aqua regia block digestion and determination by atomic spectroscopy";
  skos:topConceptOf s:scma-2011 .

s:18 a skos:Collection;
  dct:identifier "http://anzsoil.org/def/au/scma/18"^^xsd:anyURI;
  dct:source "URN:ISBN:978-0-643-10218-7";
  skos:definition <https://raw.githack.com/ANZSoilData/def-au-scma/master/html/18-miscellaneous-extractable-elements/18.html>;
  skos:inScheme s:scma-2011;
  skos:member s:18A1, s:18B1, s:18C1, s:18D1, s:18E1, s:18F, s:18F1, s:18F2, s:18G1;
  skos:notation "18";
  skos:prefLabel "Miscellaneous extractable elements" .

s:18A1 a skos:Concept, sosa:Procedure;
  dct:identifier "http://anzsoil.org/def/au/scma/18A1"^^xsd:anyURI;
  dct:source "URN:ISBN:978-0-643-10218-7";
  skos:definition <https://raw.githack.com/ANZSoilData/def-au-scma/master/html/18-miscellaneous-extractable-elements/18A1.html>;
  skos:inScheme s:scma-2011;
  skos:notation "18A1";
  skos:prefLabel "Bicarbonate-extractable K+";
  skos:topConceptOf s:scma-2011 .

s:18B1 a skos:Concept, sosa:Procedure;
  dct:identifier "http://anzsoil.org/def/au/scma/18B1"^^xsd:anyURI;
  dct:source "URN:ISBN:978-0-643-10218-7";
  skos:definition <https://raw.githack.com/ANZSoilData/def-au-scma/master/html/18-miscellaneous-extractable-elements/18B1.html>;
  skos:inScheme s:scma-2011;
  skos:notation "18B1";
  skos:prefLabel "Hydrochloric acid-extractable K+";
  skos:topConceptOf s:scma-2011 .

s:18C1 a skos:Concept, sosa:Procedure;
  dct:identifier "http://anzsoil.org/def/au/scma/18C1"^^xsd:anyURI;
  dct:source "URN:ISBN:978-0-643-10218-7";
  skos:definition <https://raw.githack.com/ANZSoilData/def-au-scma/master/html/18-miscellaneous-extractable-elements/18C1.html>;
  skos:inScheme s:scma-2011;
  skos:notation "18C1";
  skos:prefLabel "Boiling 0.1 nitric acid-extractable K+";
  skos:topConceptOf s:scma-2011 .

s:18D1 a skos:Concept, sosa:Procedure;
  dct:identifier "http://anzsoil.org/def/au/scma/18D1"^^xsd:anyURI;
  dct:source "URN:ISBN:978-0-643-10218-7";
  skos:definition <https://raw.githack.com/ANZSoilData/def-au-scma/master/html/18-miscellaneous-extractable-elements/18D1.html>;
  skos:inScheme s:scma-2011;
  skos:notation "18D1";
  skos:prefLabel "0.1 M calcium chloride-extractable Cd";
  skos:topConceptOf s:scma-2011 .

s:18E1 a skos:Concept, sosa:Procedure;
  dct:identifier "http://anzsoil.org/def/au/scma/18E1"^^xsd:anyURI;
  dct:source "URN:ISBN:978-0-643-10218-7";
  skos:definition <https://raw.githack.com/ANZSoilData/def-au-scma/master/html/18-miscellaneous-extractable-elements/18E1.html>;
  skos:inScheme s:scma-2011;
  skos:notation "18E1";
  skos:prefLabel "0.01 M calcium chloride-extractable Cd";
  skos:topConceptOf s:scma-2011 .

s:18F a skos:Concept, sosa:Procedure;
  dct:identifier "http://anzsoil.org/def/au/scma/18F"^^xsd:anyURI;
  dct:source "URN:ISBN:978-0-643-10218-7";
  skos:definition <https://raw.githack.com/ANZSoilData/def-au-scma/master/html/18-miscellaneous-extractable-elements/18F.html>;
  skos:inScheme s:scma-2011;
  skos:narrower s:18F1, s:18F2;
  skos:notation "18F";
  skos:prefLabel "Mehlich 3 multi-element tests";
  skos:topConceptOf s:scma-2011 .

s:18F1 a skos:Concept, sosa:Procedure;
  dct:identifier "http://anzsoil.org/def/au/scma/18F1"^^xsd:anyURI;
  dct:source "URN:ISBN:978-0-643-10218-7";
  skos:broader s:18F;
  skos:definition <https://raw.githack.com/ANZSoilData/def-au-scma/master/html/18-miscellaneous-extractable-elements/18F1.html>;
  skos:inScheme s:scma-2011;
  skos:notation "18F1";
  skos:prefLabel "Mehlich 3-extractable elements (P, Ca, Mg, Na, K, Fe, Cu, Mn, Zn, B, S, Al)" .

s:18F2 a skos:Concept, sosa:Procedure;
  dct:identifier "http://anzsoil.org/def/au/scma/18F2"^^xsd:anyURI;
  dct:source "URN:ISBN:978-0-643-10218-7";
  skos:broader s:18F;
  skos:definition <https://raw.githack.com/ANZSoilData/def-au-scma/master/html/18-miscellaneous-extractable-elements/18F2.html>;
  skos:inScheme s:scma-2011;
  skos:notation "18F2";
  skos:prefLabel "Mehlich 3 Extractable P - colour finish" .

s:18G1 a skos:Concept, sosa:Procedure;
  dct:identifier "http://anzsoil.org/def/au/scma/18G1"^^xsd:anyURI;
  dct:source "URN:ISBN:978-0-643-10218-7";
  skos:definition <https://raw.githack.com/ANZSoilData/def-au-scma/master/html/18-miscellaneous-extractable-elements/18G1.html>;
  skos:inScheme s:scma-2011;
  skos:notation "18G1";
  skos:prefLabel "Reverse soil K+ by copper-modified sodium tetraphenylboron extraction (TBK 4h)";
  skos:topConceptOf s:scma-2011 .

s:19 a skos:Collection;
  dct:identifier "http://anzsoil.org/def/au/scma/19"^^xsd:anyURI;
  dct:source "URN:ISBN:978-0-643-10218-7";
  skos:definition <https://raw.githack.com/ANZSoilData/def-au-scma/master/html/19-alkaline-earth-carbonates/19.html>;
  skos:inScheme s:scma-2011;
  skos:member s:19A1, s:19B, s:19B1, s:19B2, s:19C1, s:19D1;
  skos:notation "19";
  skos:prefLabel "Alkaline earth carbonates" .

s:19A1 a skos:Concept, sosa:Procedure;
  dct:identifier "http://anzsoil.org/def/au/scma/19A1"^^xsd:anyURI;
  dct:source "URN:ISBN:978-0-643-10218-7";
  skos:definition <https://raw.githack.com/ANZSoilData/def-au-scma/master/html/19-alkaline-earth-carbonates/19A1.html>;
  skos:inScheme s:scma-2011;
  skos:notation "19A1";
  skos:prefLabel "Carbonates -rapid titration";
  skos:topConceptOf s:scma-2011 .

s:19B a skos:Concept, sosa:Procedure;
  dct:identifier "http://anzsoil.org/def/au/scma/19B"^^xsd:anyURI;
  dct:source "URN:ISBN:978-0-643-10218-7";
  skos:definition <https://raw.githack.com/ANZSoilData/def-au-scma/master/html/19-alkaline-earth-carbonates/19B.html>;
  skos:inScheme s:scma-2011;
  skos:narrower s:19B1, s:19B2;
  skos:notation "19B";
  skos:prefLabel "Carbonates by pressure change";
  skos:topConceptOf s:scma-2011 .

s:19B1 a skos:Concept, sosa:Procedure;
  dct:identifier "http://anzsoil.org/def/au/scma/19B1"^^xsd:anyURI;
  dct:source "URN:ISBN:978-0-643-10218-7";
  skos:broader s:19B;
  skos:definition <https://raw.githack.com/ANZSoilData/def-au-scma/master/html/19-alkaline-earth-carbonates/19B1.html>;
  skos:inScheme s:scma-2011;
  skos:notation "19B1";
  skos:prefLabel "Carbonates by pressure change - manometric" .

s:19B2 a skos:Concept, sosa:Procedure;
  dct:identifier "http://anzsoil.org/def/au/scma/19B2"^^xsd:anyURI;
  dct:source "URN:ISBN:978-0-643-10218-7";
  skos:broader s:19B;
  skos:definition <https://raw.githack.com/ANZSoilData/def-au-scma/master/html/19-alkaline-earth-carbonates/19B2.html>;
  skos:inScheme s:scma-2011;
  skos:notation "19B2";
  skos:prefLabel "Carbonates by pressure change - transducer" .

s:19C1 a skos:Concept, sosa:Procedure;
  dct:identifier "http://anzsoil.org/def/au/scma/19C1"^^xsd:anyURI;
  dct:source "URN:ISBN:978-0-643-10218-7";
  skos:definition <https://raw.githack.com/ANZSoilData/def-au-scma/master/html/19-alkaline-earth-carbonates/19C1.html>;
  skos:inScheme s:scma-2011;
  skos:notation "19C1";
  skos:prefLabel "Spot field test for the presence of soil carbonates with dilute HCl";
  skos:topConceptOf s:scma-2011 .

s:19D1 a skos:Concept, sosa:Procedure;
  dct:identifier "http://anzsoil.org/def/au/scma/19D1"^^xsd:anyURI;
  dct:source "URN:ISBN:978-0-643-10218-7";
  skos:definition <https://raw.githack.com/ANZSoilData/def-au-scma/master/html/19-alkaline-earth-carbonates/19D1.html>;
  skos:inScheme s:scma-2011;
  skos:notation "19D1";
  skos:prefLabel "Field test for carbonates with dilute HCl and effervescence class assessment";
  skos:topConceptOf s:scma-2011 .

s:20 a skos:Collection;
  dct:identifier "http://anzsoil.org/def/au/scma/20"^^xsd:anyURI;
  dct:source "URN:ISBN:978-0-643-10218-7";
  skos:definition <https://raw.githack.com/ANZSoilData/def-au-scma/master/html/20-acid-sulfate-soils/20.html>;
  skos:inScheme s:scma-2011;
  skos:member s:20A1, s:20B1, s:20C1, s:20D1, s:20E1, s:20F1, s:20F2, s:20G1, s:20H1,
    s:20I1, s:20J1, s:20K1;
  skos:notation "20";
  skos:prefLabel "Acid sulfate soils" .

s:20A1 a skos:Concept, sosa:Procedure;
  dct:identifier "http://anzsoil.org/def/au/scma/20A1"^^xsd:anyURI;
  dct:source "URN:ISBN:978-0-643-10218-7";
  skos:definition <https://raw.githack.com/ANZSoilData/def-au-scma/master/html/20-acid-sulfate-soils/20A1.html>;
  skos:inScheme s:scma-2011;
  skos:notation "20A1";
  skos:prefLabel "Chromium reducible S (S CR)";
  skos:topConceptOf s:scma-2011 .

s:20B1 a skos:Concept, sosa:Procedure;
  dct:identifier "http://anzsoil.org/def/au/scma/20B1"^^xsd:anyURI;
  dct:source "URN:ISBN:978-0-643-10218-7";
  skos:definition <https://raw.githack.com/ANZSoilData/def-au-scma/master/html/20-acid-sulfate-soils/20B1.html>;
  skos:inScheme s:scma-2011;
  skos:notation "20B1";
  skos:prefLabel "SPOCAS acid trail - titratable actual acidity (TAA)";
  skos:topConceptOf s:scma-2011 .

s:20C1 a skos:Concept, sosa:Procedure;
  dct:identifier "http://anzsoil.org/def/au/scma/20C1"^^xsd:anyURI;
  dct:source "URN:ISBN:978-0-643-10218-7";
  skos:definition <https://raw.githack.com/ANZSoilData/def-au-scma/master/html/20-acid-sulfate-soils/20C1.html>;
  skos:inScheme s:scma-2011;
  skos:notation "20C1";
  skos:prefLabel "SPOCAS acid trail - titratable peroxide acidity (TPA) and Net (excess) Acid Neutralising Capacity (a-ANC E)";
  skos:topConceptOf s:scma-2011 .

s:20D1 a skos:Concept, sosa:Procedure;
  dct:identifier "http://anzsoil.org/def/au/scma/20D1"^^xsd:anyURI;
  dct:source "URN:ISBN:978-0-643-10218-7";
  skos:definition <https://raw.githack.com/ANZSoilData/def-au-scma/master/html/20-acid-sulfate-soils/20D1.html>;
  skos:inScheme s:scma-2011;
  skos:notation "20D1";
  skos:prefLabel "1 M KCl-extractable S, Ca and Mg";
  skos:topConceptOf s:scma-2011 .

s:20E1 a skos:Concept, sosa:Procedure;
  dct:identifier "http://anzsoil.org/def/au/scma/20E1"^^xsd:anyURI;
  dct:source "URN:ISBN:978-0-643-10218-7";
  skos:definition <https://raw.githack.com/ANZSoilData/def-au-scma/master/html/20-acid-sulfate-soils/20E1.html>;
  skos:inScheme s:scma-2011;
  skos:notation "20E1";
  skos:prefLabel "1 M KCl-extractable S, Ca and Mg after peroxide oxidation";
  skos:topConceptOf s:scma-2011 .

s:20F1 a skos:Concept, sosa:Procedure;
  dct:identifier "http://anzsoil.org/def/au/scma/20F1"^^xsd:anyURI;
  dct:source "URN:ISBN:978-0-643-10218-7";
  skos:definition <https://raw.githack.com/ANZSoilData/def-au-scma/master/html/20-acid-sulfate-soils/20F1.html>;
  skos:inScheme s:scma-2011;
  skos:notation "20F1";
  skos:prefLabel "Sulfur - 4 M HCl extraction (S HCl), ICPAES finish";
  skos:topConceptOf s:scma-2011 .

s:20F2 a skos:Concept, sosa:Procedure;
  dct:identifier "http://anzsoil.org/def/au/scma/20F2"^^xsd:anyURI;
  dct:source "URN:ISBN:978-0-643-10218-7";
  skos:definition <https://raw.githack.com/ANZSoilData/def-au-scma/master/html/20-acid-sulfate-soils/20F2.html>;
  skos:inScheme s:scma-2011;
  skos:notation "20F2";
  skos:prefLabel "Sulfur - 4 M HCl extraction (S HCl), ion chromatography finish";
  skos:topConceptOf s:scma-2011 .

s:20G1 a skos:Concept, sosa:Procedure;
  dct:identifier "http://anzsoil.org/def/au/scma/20G1"^^xsd:anyURI;
  dct:source "URN:ISBN:978-0-643-10218-7";
  skos:definition <https://raw.githack.com/ANZSoilData/def-au-scma/master/html/20-acid-sulfate-soils/20G1.html>;
  skos:inScheme s:scma-2011;
  skos:notation "20G1";
  skos:prefLabel "Peroxide residual acid soluble sulfur (S RAS)";
  skos:topConceptOf s:scma-2011 .

s:20H1 a skos:Concept, sosa:Procedure;
  dct:identifier "http://anzsoil.org/def/au/scma/20H1"^^xsd:anyURI;
  dct:source "URN:ISBN:978-0-643-10218-7";
  skos:definition <https://raw.githack.com/ANZSoilData/def-au-scma/master/html/20-acid-sulfate-soils/20H1.html>;
  skos:inScheme s:scma-2011;
  skos:notation "20H1";
  skos:prefLabel "Acid neutralising capacity - acid reacted and back titration (ANC BT)";
  skos:topConceptOf s:scma-2011 .

s:20I1 a skos:Concept, sosa:Procedure;
  dct:identifier "http://anzsoil.org/def/au/scma/20I1"^^xsd:anyURI;
  dct:source "URN:ISBN:978-0-643-10218-7";
  skos:definition <https://raw.githack.com/ANZSoilData/def-au-scma/master/html/20-acid-sulfate-soils/20I1.html>;
  skos:inScheme s:scma-2011;
  skos:notation "20I1";
  skos:prefLabel "Acid neutralising capacity - from SPOCAS";
  skos:topConceptOf s:scma-2011 .

s:20J1 a skos:Concept, sosa:Procedure;
  dct:identifier "http://anzsoil.org/def/au/scma/20J1"^^xsd:anyURI;
  dct:source "URN:ISBN:978-0-643-10218-7";
  skos:definition <https://raw.githack.com/ANZSoilData/def-au-scma/master/html/20-acid-sulfate-soils/20J1.html>;
  skos:inScheme s:scma-2011;
  skos:notation "20J1";
  skos:prefLabel "Field approximation of ASS hazard";
  skos:topConceptOf s:scma-2011 .

s:20K1 a skos:Concept, sosa:Procedure;
  dct:identifier "http://anzsoil.org/def/au/scma/20K1"^^xsd:anyURI;
  dct:source "URN:ISBN:978-0-643-10218-7";
  skos:definition <https://raw.githack.com/ANZSoilData/def-au-scma/master/html/20-acid-sulfate-soils/20K1.html>;
  skos:inScheme s:scma-2011;
  skos:notation "20K1";
  skos:prefLabel "Quick field approximations of ASS presence and associated lime requirement for drain-spoil";
  skos:topConceptOf s:scma-2011 .