# baseURI: http://anzsoil.org/def/au/scma/
# imports: http://purl.org/dc/elements/1.1/
# prefix: scma

@prefix dc: <http://purl.org/dc/elements/1.1/> .
@prefix dcat: <http://www.w3.org/ns/dcat#> .
@prefix dcterms: <http://purl.org/dc/terms/> .
@prefix owl: <http://www.w3.org/2002/07/owl#> .
@prefix rdf: <http://www.w3.org/1999/02/22-rdf-syntax-ns#> .
@prefix rdfs: <http://www.w3.org/2000/01/rdf-schema#> .
@prefix reg: <http://purl.org/linked-data/registry#> .
@prefix scma: <http://anzsoil.org/def/au/scma/> .
@prefix sdo: <https://schema.org/> .
@prefix skos: <http://www.w3.org/2004/02/skos/core#> .
@prefix sosa: <http://www.w3.org/ns/sosa/> .
@prefix ui: <http://purl.org/linked-data/registry-ui#> .
@prefix xsd: <http://www.w3.org/2001/XMLSchema#> .

scma:
  a owl:Ontology ;
  a skos:ConceptScheme ;
  dcterms:accrualPeriodicity <http://purl.org/cld/freq/completelyIrregular> ;
  dcterms:contributor <https://orcid.org/0000-0002-3884-3420> ;
  dcterms:created "2021-01-01"^^xsd:date ;
  dcterms:creator <https://orcid.org/0000-0002-2991-2308> ;
  dcterms:description "<p>This register contains a machine-readable representation of the classifiers described in <a href='https://www.publish.csiro.au/book/6418'>Soil Chemical Methods Australasia</a> 1. (2011), by George E Rayment and David J Lyons. These comprise the laboratory and field chemical tests relevant to Australasia and beyond. </p> <p>Supersedes Australian Laboratory Handbook of Soil and Water Chemical Methods (Rayment and Higginson 1992) while retaining method codes and other strengths of that Handbook. This register includes the method codes from Rayment and Higginson (1992) that were made redundant or superseded by new codes in George E Rayment and David J Lyons (2011).</p>"^^rdf:HTML ;
  dcterms:identifier "http://anzsoil.org/def/au/scma"^^xsd:anyURI ;
  dcterms:isFormatOf <https://discovery.csiro.au/view/delivery/61CSIRO_INST/1289969120001981> ;
  dcterms:isFormatOf <https://ebooks.publish.csiro.au/content/soil-chemical-methods-australasia> ;
  dcterms:license <https://creativecommons.org/publicdomain/zero/1.0/> ;
  dcterms:modified "2021-04-26"^^xsd:date ;
  dcterms:source "URN:ISBN:978-0-643-10218-7" ;
  dcterms:title "Soil chemical methods - Australasia" ;
  ui:hierarchyChildProperty skos:member ;
  ui:hierarchyRootProperty ui:topMemberOf ;
  owl:imports dc: ;
  owl:imports <http://www.w3.org/2004/02/skos/core> ;
  skos:definition """<h2 class=\"h2\"><a id=\"page_1\"></a><a id=\"chapter01\"></a>1</h2>
<h2 class=\"h2a\">Introduction</h2>
<p class=\"para\">A plethora of methods for the chemical analysis of soils exists for at least six main reasons: (a) there are many types of soils with widely differing physical and chemical characteristics and problems; (b) the total elemental composition of soils mostly has little consistent association with the ability of soils to provide necessary levels of nutrients for good plant growth; (c) tests that are quick and cheap to perform are often sought for operational and commercial reasons, even when superior procedures exist; (d) technological advances in instrumentation and computing open new analytical opportunities; (e) an ongoing quest by soil scientists and chemists to develop tests superior to those of times past, and (f) broadening demands to deal with emerging natural resource management, soil health and environmental issues. In practice, soil test methodology used by soil testing services varies within and across regions, across states and from one nation to another, making it difficult to exchange meaningful soil chemical information.</p>
<p class=\"indent-para\">Calls from 19th century agricultural chemists failed to &#8216;settle on a uniform method of soil analysis, so that results obtained by different analysts might be comparable&#8217;. A two-part response in harmony with this book provides a way forward. The first, the main focus of this book, is to explain and define the (mostly) empirical methods (see Note 1) of analysis now in use or suitable for use in at least parts of Australasia. The second, also supported by this book, is to periodically assess whether the selected method/s can produce consistent results when used by individual and multiple laboratories. The now superseded Australian Laboratory Handbook of Soil and Water Chemical Methods (<a href=\"#ch01ref03\">Rayment and Higginson 1992</a>) made an important contribution to both components. This book extends that two-part framework for soil chemical methods, with a focus on the Australasian region. For this book, the Australasian region is that accepted by ASPAC, i.e. it comprises Oceania (Australia, New Zealand, Papua New Guinea, other islands in the south Pacific Ocean) plus areas of south-east Asia.</p>
<h3 class=\"h3a\"><em>Organisation</em></h3>
<p class=\"para\">This book contains over 200 ready-to-use methods, each accompanied by contemporary background information. There is sufficient detail for the book to be used as an operational laboratory methods manual and as a comprehensive reference to guide educators, researchers and end-users on choice and performance of the various methodological options contained therein. Key references are included to facilitate follow-up by those who seek additional knowledge.</p>
<p class=\"indent-para\">Each method has a unique, three-character or four-character alpha-numeric code number. These codes harmonise with those for soils in <a href=\"#ch01ref03\">Rayment and Higginson (1992)</a>. That is, code numbers used for particular methods and analytical finishes in the Rayment and Higginson Handbook are reproduced and extended when necessary. Specifically, the code incorporates two numerals separated by an upper-case alpha-character. The left-hand-side numeral represents methods with related features or applications, such as carbon (C), nitrogen (N), ion-exchange properties and the like. The first alpha-character identifies a variant of the main test, <a id=\"page_2\"></a>such as a specific extraction for soil phosphorus (P). The next numeral is used to distinguish alternative ways of completing the analytical measurement, or adjusting for variables such as the treatment of soluble salts in ion-exchange determinations. Occasionally, there is a final lower-case, alpha-character to identify a different analytical finish for a specified method that is unlikely to significantly affect the result reported at the three-character code level.</p>
<p class=\"indent-para\">All soil chemical methods, including information on sampling and sample preparation, have been grouped into 20 chapters, mostly the same or similar to those in the Rayment and Higginson Handbook. These chapter numbers are replicated in the left-hand-side numeral of the unique method code. References for each chapter are arranged in alphabetic order. In addition, there is guidance on the preferred way to report results (including codes for preparative details when necessary), and suggestions on the number of significant figures for reporting each relevant test. Appendices cover summary details on the accuracy and precision of key methods. They also provide information on concentrated and dilute acids, year 2007 atomic weights, examples of SI units, etc.</p>
<h3 class=\"h3a\"><em>Methodology</em></h3>
<p class=\"para\">Soil chemical methods from the Rayment and Higginson Handbook have been retained to ensure they remain accessible for historical purposes and often for contemporary use. At least some of the technologies specified in that publication, however, have suffered with the passage of time, due to advances in instrumentation and automation. Micro-bore and flow-injection analysis are examples of incremental improvements in continuous-flow technology, while alternatives to conventional chemical testing are offered by NIR and MIR diffuse reflectance spectroscopy these days. In addition, the superseded Handbook did not include quantitative procedures for acid sulfate soils and many other popular tests such as Mehlich No. 3.</p>
<p class=\"indent-para\">For 21st century Australasia, the book needed to embrace both laboratory and field procedures in a comprehensive, informative and consistent style. Soil chemical testing experience regionally and internationally was used to finalise the selections, based broadly on the following criteria:</p>
<p class=\"hangindent-para1\">1&#160;&#160;&#160;method/s used by one or more of the major soil testing laboratories in Australasia for soil fertility assessments, for natural resource management, for environmental protection, and/or for the characterisation of modal profiles collected for land-use survey purposes;</p>
<p class=\"hangindent-para\">2&#160;&#160;&#160;inclusion in ASPAC inter-laboratory proficiency programs for soil chemical tests, and</p>
<p class=\"hangindent-para\">3&#160;&#160;&#160;publication in the scientific and/or methodological literature, particularly when relevant to the Australasian region.</p>
<p class=\"indent-para1\">All methods have been described in reasonable detail, including guidance on the elemental composition of reagents. To save space, reagent preparation and operational procedures, once described, are not usually repeated but are cross-referenced. In addition, the preferred form for expressing results is provided for each code number. <a href=\"backmatter01.html#backmatter01\">Appendix 1</a> should be consulted to obtain the recommended numbers of decimal places for the reporting of results. Factors to convert results from an element to a species or vice versa are provided when warranted.</p>
<p class=\"indent-para\">Given the empirical nature of many of the tests described, analytical conditions such as sample particle size, moisture status of the test sample, the extractant, the soil/extractant ratio, and temperature/s should not be changed, unless there are experimental data to show what tolerances are permitted on each of these parameters. Concentrations of primary and/or working standards, however, can be tailored to suit particular sample types and analytical instrumentation, despite the inclusion of suggestions. All calculations for primary standard solutions are based on 2007 standard atomic weights (<a href=\"#ch01ref02\">Standard atomic weights 2007</a>) and <a id=\"page_3\"></a>assume 100% purity of the proposed chemical/s; adjustments based on actual assays should be made. Likewise, adjustments to segmented flow and flow-injection analysis flow-sheets and operating conditions may be necessary to account for different types of equipment and/or reagent quality, although changes to the specified wave lengths for associated detectors are less likely. Such adjustments, if made, must not significantly change the sample/reagent combinations, as this could affect the resultant concentration of the element or species under test. Laboratory participation in inter-laboratory proficiency programs is recommended to help benchmark contemporary measurement performance against others who participate in the same programs.</p>
<p class=\"indent-para\">An assumption throughout, unless otherwise specified, is that all chemicals are dry and of analytical grade, and that all mineral acids are concentrated (typical molarities are given). What is referred to as reagent water or deionised water should be of high and consistent quality, although distilled water of similar quality is acceptable and in a few cases may be superior. One example is in the preparation of the molybdenum-blue reagent associated with colorimetric determinations of orthophosphate-P, which can be adversely affected by organic impurities in some deionised waters.</p>
<p class=\"indent-para\">To limit opportunities for in-house errors, weights and volumes are consistently provided to guide the preparation of reagents. No particular significance, however, should be placed on the weight/volumes specified. These can be varied proportionately (with care), depending upon the number of samples to be analysed, in conjunction with the expected shelf lives of the particular solutions. Analysts must ensure all such solutions, if subjected to periods of storage, are in good condition prior to use. If not, the old solutions should be disposed of in an environmentally sensitive manner and fresh solutions prepared. Shelf life guidance is often provided, but these times may not apply if storage conditions are unfavourable.</p>
<p class=\"indent-para\">All specified dilutions, solution transfers, and volumes should be made as accurately as warranted. Descriptions requiring the use of pipettes, burettes, and volumetric flasks imply that accurate volumes are required. Moreover, while preparation of working standard solutions from a single primary standard solution are commonly described, there is a lower risk of systematic error if three or more weighings are involved in preparing a range of primary reference solutions. The use of commercially available standard stock solutions is acceptable: preparation time can be reduced and errors minimised if the quality of the commercial product is assured and stated instructions for mixing and dilutions are followed carefully.</p>
<p class=\"indent-para\">Importantly, analysts using the methods described should be appropriately trained and practiced in the safe use and handling of laboratory chemicals and equipment, and should apply this training at all times. Moreover, risk assessment profiles should be developed for all methods involved with hazardous substances and temperatures outside of ambient conditions. It is further assumed that all laboratories are equipped with normal laboratory equipment, glassware, fume cabinets, well-calibrated balances, refrigeration, and at least one constant-temperature room at 25&#177;2&#176;C (or better) for the extraction of soils and equilibration of extracting solutions and reagents. If the constant-temperature room is not within the 25&#177;2&#176;C specification, the actual temperature used (e.g. 20&#177;2&#176;C) should be recorded, as temperature can affect apparent results.</p>
<p class=\"indent-para\">There should be facilities to receive soil samples from clients and to dry and grind/sieve soils to the moisture status and particle sizes specified (see <a href=\"#ch1fig1\">Figure 1.1</a>). These activities must not introduce chemical or physical changes to the samples or add measurable contamination via the materials used in construction of the equipment or from the air or surroundings. Airborne contaminants include particulates and chemical vapours, such as ammonia fumes. Subsequent storage of prepared samples in inert containers should be clean, cool and dry.</p>
<p class=\"image\"><a id=\"page_4\"></a><a id=\"ch1fig1\"></a><img src=\"../images/f0004-01.jpg\" alt=\"Image\"></img></p>
<p class=\"caption\"><strong>Figure 1.1.</strong> Examples of soil preparation and soil grinding equipment. The mills shown in the centre and right-hand side are located in a laminated enclosure with a stainless steel screen at the base to draw dust particles away from the sample and the operator. The left-hand side photograph shows simple equipment used for crushing soils (e.g. hard setting clays) if required before grinding.</p>
<p class=\"indent-para\">Where end-over-end extraction is specified, the equipment should ensure good, gentle and regular contact between all soil particles and extracting solutions. A drum diameter of around 560 mm revolving at about 15 rpm is most satisfactory. There should be a minimum of about 20% free airspace within each extraction bottle to facilitate good mixing, while moments of inertia for all extracting bottles in the one shaking machine should be as near as possible to equal (see <a href=\"#ch1fig2\">Figure 1.2</a> for an example).</p>
<p class=\"image\"><a id=\"ch1fig2\"></a><img src=\"../images/f0004-02.jpg\" alt=\"Image\"></img></p>
<p class=\"caption\"><strong>Figure 1.2.</strong> Part of an end-over-end soil shaking machine, showing the location of a rack of 10 soil extraction bottles prior to closure of the opening with a stainless steel lid. There is provision in the drum for 10 such racks, all with the same radius from the centre-point of rotation. The plastic-coated wire tray shown above the drum assists loading and unloading of the shaking machine.</p>
<p class=\"indent-para\">When a laboratory routinely performs tests for a particular element (e.g. potassium), and also uses soil extracting solutions containing the same element for other purposes, it is recommended <a id=\"page_5\"></a>that separate glassware and/or plasticware be used to minimise the opportunities for cross-contamination. All other apparatus, disposable equipment, filter papers, etc., should either be well cleaned before use or periodically tested for freedom from relevant contamination.</p>
<p class=\"indent-para\">Analysts should periodically seek independent verification of their analytical results. For example, certified and/or secondary reference materials should be used frequently. Acceptable values for empirical soil tests need to be established in collaboration with laboratories known to be proficient at performing such tests.</p>
<h3 class=\"h3a\"><em>Moisture status of test results</em></h3>
<p class=\"para\">As indicated, method codes identify often quite complex soil analytical procedures. The codes also cover the type of sample, method of extraction, the analytical &#8216;finish&#8217;, and what is reported. It follows that laboratories who report results against these codes infer full compliance, inclusive of the moisture status of reported results. Those in this book comply broadly with international best practice (e.g. <a href=\"#ch01ref04\">SSL 1996</a>).</p>
<p class=\"indent-para\">Specifically, characteristic soil properties generally are expressed on an oven-dry weight basis (oven drying to constant weight of 105&#8211;110&#176;C), where oven-dry refers to a soil without free water but inclusive of crystal water in the case of gypsiferous soils. Exceptions are results for electrical conductivity and pH, which cannot be readily adjusted to a moisture-free basis by simple calculations using the air-dry moisture to oven-dry moisture ratio. Other important exceptions are soil tests performed for &#8216;fertility&#8217; or &#8216;diagnostic&#8217; purposes. These are reported herein on an air-dry (&#8804; 40&#8211;45&#176;C) basis.</p>
<p class=\"indent-para\">As the great majority of laboratory soil tests described commence with air-dry samples, the tests to be reported on an oven-dry weight basis need to be adjusted, using the air-dry moisture to oven-dry moisture ratio. As an example of non-compliance, results for tests on the Vertosols of Australia, (these are widely distributed across the continent; see <a href=\"#ch1fig3\">Figure 1.3</a>) could be up to 12&#8211;14% lower if reported on an air-dry basis rather than on an oven-dry basis. Obviously, inter-laboratory proficiency programs for soils need to pay close attention to the moisture status of results they report on behalf of participating laboratories.</p>
<p class=\"image\"><a id=\"ch1fig3\"></a><img src=\"../images/f0005-01.jpg\" alt=\"Image\"></img></p>
<p class=\"caption\"><strong>Figure 1.3.</strong> Distribution of Australia&#8217;s Vertosols (from <a href=\"#ch01ref01\">Isbell <em>et al</em>. 1997</a>).</p>
<h3 class=\"h3a\"><a id=\"page_6\"></a><em>Note</em></h3>
<p class=\"hangindent-para\">1.&#160;&#160;Empirical methods generally arise via experience and speculation, combined with intuitive ability by the developer, rather than from theoretically based expectations. Typically, they follow the collection and interpretation of large amounts of experimental data and observations, combined with trial and error and meticulous analytical repeatability; i.e. the same soil particle size, a defined extractant and soil/extractant ratio, a set extraction time and temperature, and a robust analytical finish.</p>
<h3 class=\"h3\">References</h3>
<p class=\"ref\"><a id=\"ch01ref01\"></a>Isbell RF, McDonald WS and Ashton LJ (1997) <em>Concepts and Rationale of the Australian Soil Classification.</em> ACLEP, CSIRO, Australia.</p>
<p class=\"ref\"><a id=\"ch01ref02\"></a>Standard atomic weights (2007) of selected elements, updated from <em>Pure and Applied Chemistry</em> <strong>78</strong>, 2051&#8211;2066 (2006), with 2007 changes. IUPAC Commission on Atomic Weights and Isotopic Abundances. <a href=\"http://www.chem.qmul.ac.uk/iupac/AtWt/\">http://www.chem.qmul.ac.uk/iupac/AtWt/</a></p>
<p class=\"ref\"><a id=\"ch01ref03\"></a>Rayment GE and Higginson FR (1992) A<em>ustralian Laboratory Handbook of Soil and Water Chemical Methods.</em> Inkata Press, Port Melbourne.</p>
<p class=\"ref\"><a id=\"ch01ref04\"></a>SSL (1996) <em>Soil Survey Laboratory Methods Manual</em>. Soil Survey Investigations Report No. 42, Version 3.0. National Soil Survey Centre, Natural Resources Conservation Service, US Department of Agriculture, Washington DC.</p>"""^^rdf:HTML ;
  skos:hasTopConcept <http://anzsoil.org/def/au/scma/10A1> ;
  skos:hasTopConcept <http://anzsoil.org/def/au/scma/10A2> ;
  skos:hasTopConcept <http://anzsoil.org/def/au/scma/10B> ;
  skos:hasTopConcept <http://anzsoil.org/def/au/scma/10C1> ;
  skos:hasTopConcept <http://anzsoil.org/def/au/scma/10D1> ;
  skos:hasTopConcept <http://anzsoil.org/def/au/scma/11A1> ;
  skos:hasTopConcept <http://anzsoil.org/def/au/scma/11A2> ;
  skos:hasTopConcept <http://anzsoil.org/def/au/scma/12A1> ;
  skos:hasTopConcept <http://anzsoil.org/def/au/scma/12B1> ;
  skos:hasTopConcept <http://anzsoil.org/def/au/scma/12C1> ;
  skos:hasTopConcept <http://anzsoil.org/def/au/scma/12C2> ;
  skos:hasTopConcept <http://anzsoil.org/def/au/scma/12D1> ;
  skos:hasTopConcept <http://anzsoil.org/def/au/scma/12E1> ;
  skos:hasTopConcept <http://anzsoil.org/def/au/scma/13A1> ;
  skos:hasTopConcept <http://anzsoil.org/def/au/scma/13B1> ;
  skos:hasTopConcept <http://anzsoil.org/def/au/scma/13C1> ;
  skos:hasTopConcept <http://anzsoil.org/def/au/scma/13D> ;
  skos:hasTopConcept <http://anzsoil.org/def/au/scma/14A1> ;
  skos:hasTopConcept <http://anzsoil.org/def/au/scma/14A2> ;
  skos:hasTopConcept <http://anzsoil.org/def/au/scma/14A3> ;
  skos:hasTopConcept <http://anzsoil.org/def/au/scma/14A4> ;
  skos:hasTopConcept <http://anzsoil.org/def/au/scma/14B1> ;
  skos:hasTopConcept <http://anzsoil.org/def/au/scma/14C1> ;
  skos:hasTopConcept <http://anzsoil.org/def/au/scma/14D1> ;
  skos:hasTopConcept <http://anzsoil.org/def/au/scma/14D2> ;
  skos:hasTopConcept <http://anzsoil.org/def/au/scma/14E1> ;
  skos:hasTopConcept <http://anzsoil.org/def/au/scma/14E2> ;
  skos:hasTopConcept <http://anzsoil.org/def/au/scma/14E3> ;
  skos:hasTopConcept <http://anzsoil.org/def/au/scma/14F1> ;
  skos:hasTopConcept <http://anzsoil.org/def/au/scma/14F2> ;
  skos:hasTopConcept <http://anzsoil.org/def/au/scma/14F3> ;
  skos:hasTopConcept <http://anzsoil.org/def/au/scma/14F4> ;
  skos:hasTopConcept <http://anzsoil.org/def/au/scma/14F5> ;
  skos:hasTopConcept <http://anzsoil.org/def/au/scma/14G1> ;
  skos:hasTopConcept <http://anzsoil.org/def/au/scma/14G2> ;
  skos:hasTopConcept <http://anzsoil.org/def/au/scma/14H1> ;
  skos:hasTopConcept <http://anzsoil.org/def/au/scma/15A1> ;
  skos:hasTopConcept <http://anzsoil.org/def/au/scma/15A2> ;
  skos:hasTopConcept <http://anzsoil.org/def/au/scma/15A3> ;
  skos:hasTopConcept <http://anzsoil.org/def/au/scma/15B1> ;
  skos:hasTopConcept <http://anzsoil.org/def/au/scma/15B2> ;
  skos:hasTopConcept <http://anzsoil.org/def/au/scma/15B3> ;
  skos:hasTopConcept <http://anzsoil.org/def/au/scma/15C1> ;
  skos:hasTopConcept <http://anzsoil.org/def/au/scma/15C2> ;
  skos:hasTopConcept <http://anzsoil.org/def/au/scma/15D1> ;
  skos:hasTopConcept <http://anzsoil.org/def/au/scma/15D2> ;
  skos:hasTopConcept <http://anzsoil.org/def/au/scma/15D3> ;
  skos:hasTopConcept <http://anzsoil.org/def/au/scma/15E1> ;
  skos:hasTopConcept <http://anzsoil.org/def/au/scma/15E2> ;
  skos:hasTopConcept <http://anzsoil.org/def/au/scma/15E3> ;
  skos:hasTopConcept <http://anzsoil.org/def/au/scma/15F1> ;
  skos:hasTopConcept <http://anzsoil.org/def/au/scma/15F2> ;
  skos:hasTopConcept <http://anzsoil.org/def/au/scma/15F3> ;
  skos:hasTopConcept <http://anzsoil.org/def/au/scma/15G1> ;
  skos:hasTopConcept <http://anzsoil.org/def/au/scma/15H1> ;
  skos:hasTopConcept <http://anzsoil.org/def/au/scma/15I1> ;
  skos:hasTopConcept <http://anzsoil.org/def/au/scma/15I2> ;
  skos:hasTopConcept <http://anzsoil.org/def/au/scma/15I3> ;
  skos:hasTopConcept <http://anzsoil.org/def/au/scma/15I4> ;
  skos:hasTopConcept <http://anzsoil.org/def/au/scma/15J1> ;
  skos:hasTopConcept <http://anzsoil.org/def/au/scma/15K1> ;
  skos:hasTopConcept <http://anzsoil.org/def/au/scma/15L1> ;
  skos:hasTopConcept <http://anzsoil.org/def/au/scma/15M1> ;
  skos:hasTopConcept <http://anzsoil.org/def/au/scma/15N1> ;
  skos:hasTopConcept <http://anzsoil.org/def/au/scma/15O1> ;
  skos:hasTopConcept <http://anzsoil.org/def/au/scma/16A1> ;
  skos:hasTopConcept <http://anzsoil.org/def/au/scma/16B1> ;
  skos:hasTopConcept <http://anzsoil.org/def/au/scma/16C1> ;
  skos:hasTopConcept <http://anzsoil.org/def/au/scma/16D1> ;
  skos:hasTopConcept <http://anzsoil.org/def/au/scma/17A1> ;
  skos:hasTopConcept <http://anzsoil.org/def/au/scma/17A2> ;
  skos:hasTopConcept <http://anzsoil.org/def/au/scma/17B1> ;
  skos:hasTopConcept <http://anzsoil.org/def/au/scma/17B2> ;
  skos:hasTopConcept <http://anzsoil.org/def/au/scma/17C1> ;
  skos:hasTopConcept <http://anzsoil.org/def/au/scma/18A1> ;
  skos:hasTopConcept <http://anzsoil.org/def/au/scma/18B1> ;
  skos:hasTopConcept <http://anzsoil.org/def/au/scma/18C1> ;
  skos:hasTopConcept <http://anzsoil.org/def/au/scma/18D1> ;
  skos:hasTopConcept <http://anzsoil.org/def/au/scma/18E1> ;
  skos:hasTopConcept <http://anzsoil.org/def/au/scma/18F> ;
  skos:hasTopConcept <http://anzsoil.org/def/au/scma/18G1> ;
  skos:hasTopConcept <http://anzsoil.org/def/au/scma/19A1> ;
  skos:hasTopConcept <http://anzsoil.org/def/au/scma/19B> ;
  skos:hasTopConcept <http://anzsoil.org/def/au/scma/19C1> ;
  skos:hasTopConcept <http://anzsoil.org/def/au/scma/19D1> ;
  skos:hasTopConcept <http://anzsoil.org/def/au/scma/1A1> ;
  skos:hasTopConcept <http://anzsoil.org/def/au/scma/1A2> ;
  skos:hasTopConcept <http://anzsoil.org/def/au/scma/1B1> ;
  skos:hasTopConcept <http://anzsoil.org/def/au/scma/20A1> ;
  skos:hasTopConcept <http://anzsoil.org/def/au/scma/20B1> ;
  skos:hasTopConcept <http://anzsoil.org/def/au/scma/20C1> ;
  skos:hasTopConcept <http://anzsoil.org/def/au/scma/20D1> ;
  skos:hasTopConcept <http://anzsoil.org/def/au/scma/20E1> ;
  skos:hasTopConcept <http://anzsoil.org/def/au/scma/20F1> ;
  skos:hasTopConcept <http://anzsoil.org/def/au/scma/20F2> ;
  skos:hasTopConcept <http://anzsoil.org/def/au/scma/20G1> ;
  skos:hasTopConcept <http://anzsoil.org/def/au/scma/20H1> ;
  skos:hasTopConcept <http://anzsoil.org/def/au/scma/20I1> ;
  skos:hasTopConcept <http://anzsoil.org/def/au/scma/20J1> ;
  skos:hasTopConcept <http://anzsoil.org/def/au/scma/20K1> ;
  skos:hasTopConcept <http://anzsoil.org/def/au/scma/2A1> ;
  skos:hasTopConcept <http://anzsoil.org/def/au/scma/2B1> ;
  skos:hasTopConcept <http://anzsoil.org/def/au/scma/2C1> ;
  skos:hasTopConcept <http://anzsoil.org/def/au/scma/2D1> ;
  skos:hasTopConcept <http://anzsoil.org/def/au/scma/3A1> ;
  skos:hasTopConcept <http://anzsoil.org/def/au/scma/3B1> ;
  skos:hasTopConcept <http://anzsoil.org/def/au/scma/3C1> ;
  skos:hasTopConcept <http://anzsoil.org/def/au/scma/3D1> ;
  skos:hasTopConcept <http://anzsoil.org/def/au/scma/4A1> ;
  skos:hasTopConcept <http://anzsoil.org/def/au/scma/4A2> ;
  skos:hasTopConcept <http://anzsoil.org/def/au/scma/4A3> ;
  skos:hasTopConcept <http://anzsoil.org/def/au/scma/4B1> ;
  skos:hasTopConcept <http://anzsoil.org/def/au/scma/4B2> ;
  skos:hasTopConcept <http://anzsoil.org/def/au/scma/4B3> ;
  skos:hasTopConcept <http://anzsoil.org/def/au/scma/4B4> ;
  skos:hasTopConcept <http://anzsoil.org/def/au/scma/4B5> ;
  skos:hasTopConcept <http://anzsoil.org/def/au/scma/4C1> ;
  skos:hasTopConcept <http://anzsoil.org/def/au/scma/4C2> ;
  skos:hasTopConcept <http://anzsoil.org/def/au/scma/4C3> ;
  skos:hasTopConcept <http://anzsoil.org/def/au/scma/4C4> ;
  skos:hasTopConcept <http://anzsoil.org/def/au/scma/4D1> ;
  skos:hasTopConcept <http://anzsoil.org/def/au/scma/4E1> ;
  skos:hasTopConcept <http://anzsoil.org/def/au/scma/4F1> ;
  skos:hasTopConcept <http://anzsoil.org/def/au/scma/4G1> ;
  skos:hasTopConcept <http://anzsoil.org/def/au/scma/5A1> ;
  skos:hasTopConcept <http://anzsoil.org/def/au/scma/5A2> ;
  skos:hasTopConcept <http://anzsoil.org/def/au/scma/5A3a> ;
  skos:hasTopConcept <http://anzsoil.org/def/au/scma/5A3b> ;
  skos:hasTopConcept <http://anzsoil.org/def/au/scma/5A4> ;
  skos:hasTopConcept <http://anzsoil.org/def/au/scma/6A1> ;
  skos:hasTopConcept <http://anzsoil.org/def/au/scma/6B1> ;
  skos:hasTopConcept <http://anzsoil.org/def/au/scma/6B2> ;
  skos:hasTopConcept <http://anzsoil.org/def/au/scma/6B3> ;
  skos:hasTopConcept <http://anzsoil.org/def/au/scma/6B4> ;
  skos:hasTopConcept <http://anzsoil.org/def/au/scma/6C1> ;
  skos:hasTopConcept <http://anzsoil.org/def/au/scma/6D1> ;
  skos:hasTopConcept <http://anzsoil.org/def/au/scma/6E1> ;
  skos:hasTopConcept <http://anzsoil.org/def/au/scma/6F1> ;
  skos:hasTopConcept <http://anzsoil.org/def/au/scma/6G1> ;
  skos:hasTopConcept <http://anzsoil.org/def/au/scma/7A1> ;
  skos:hasTopConcept <http://anzsoil.org/def/au/scma/7A2> ;
  skos:hasTopConcept <http://anzsoil.org/def/au/scma/7A3> ;
  skos:hasTopConcept <http://anzsoil.org/def/au/scma/7A4> ;
  skos:hasTopConcept <http://anzsoil.org/def/au/scma/7A5> ;
  skos:hasTopConcept <http://anzsoil.org/def/au/scma/7A6> ;
  skos:hasTopConcept <http://anzsoil.org/def/au/scma/7B> ;
  skos:hasTopConcept <http://anzsoil.org/def/au/scma/7C1> ;
  skos:hasTopConcept <http://anzsoil.org/def/au/scma/7C2> ;
  skos:hasTopConcept <http://anzsoil.org/def/au/scma/7D> ;
  skos:hasTopConcept <http://anzsoil.org/def/au/scma/8A1> ;
  skos:hasTopConcept <http://anzsoil.org/def/au/scma/8B1> ;
  skos:hasTopConcept <http://anzsoil.org/def/au/scma/9A> ;
  skos:hasTopConcept <http://anzsoil.org/def/au/scma/9B> ;
  skos:hasTopConcept <http://anzsoil.org/def/au/scma/9C> ;
  skos:hasTopConcept <http://anzsoil.org/def/au/scma/9D1> ;
  skos:hasTopConcept <http://anzsoil.org/def/au/scma/9E> ;
  skos:hasTopConcept <http://anzsoil.org/def/au/scma/9F1> ;
  skos:hasTopConcept <http://anzsoil.org/def/au/scma/9F2> ;
  skos:hasTopConcept <http://anzsoil.org/def/au/scma/9G1> ;
  skos:hasTopConcept <http://anzsoil.org/def/au/scma/9G2> ;
  skos:hasTopConcept <http://anzsoil.org/def/au/scma/9H1> ;
  skos:hasTopConcept <http://anzsoil.org/def/au/scma/9I> ;
  skos:hasTopConcept <http://anzsoil.org/def/au/scma/9J> ;
  skos:hasTopConcept <http://anzsoil.org/def/au/scma/9K> ;
  sdo:codeRepository <https://github.com/ANZSoilData/aus-vocab> ;
.
<http://anzsoil.org/def/au/scma/1>
  a skos:Collection ;
  dcterms:description "Sampling and Sample Preparation" ;
  dcterms:identifier "http://anzsoil.org/def/au/scma/1"^^xsd:anyURI ;
  dcterms:isReplacedBy owl:Nothing ;
  dcterms:source "URN:ISBN:978-0-909605-68-1" ;
  ui:topMemberOf <http://anzsoil.org/def/au/scma> ;
  rdfs:label "Sampling and Sample Preparation" ;
  skos:inScheme <http://anzsoil.org/def/au/scma> ;
  skos:member <http://anzsoil.org/def/au/scma/1A1> ;
  skos:member <http://anzsoil.org/def/au/scma/1A2> ;
  skos:member <http://anzsoil.org/def/au/scma/1B1> ;
  skos:notation "1" ;
  skos:note "Retired in Soil Chemical Methods Australasia, Rayment G.E. and Lyons D.J. ISBN 9780643101364" ;
  skos:prefLabel "Sampling and Sample Preparation" ;
.
<http://anzsoil.org/def/au/scma/10>
  a skos:Collection ;
  dcterms:description "Sulfur" ;
  dcterms:identifier "http://anzsoil.org/def/au/scma/10"^^xsd:anyURI ;
  dcterms:source "URN:ISBN:978-0-643-10218-7" ;
  ui:topMemberOf <http://anzsoil.org/def/au/scma> ;
  rdfs:label "Sulfur" ;
  skos:definition "Sulfur" ;
  skos:inScheme <http://anzsoil.org/def/au/scma> ;
  skos:member <http://anzsoil.org/def/au/scma/10A1> ;
  skos:member <http://anzsoil.org/def/au/scma/10A2> ;
  skos:member <http://anzsoil.org/def/au/scma/10B> ;
  skos:member <http://anzsoil.org/def/au/scma/10B1> ;
  skos:member <http://anzsoil.org/def/au/scma/10B2> ;
  skos:member <http://anzsoil.org/def/au/scma/10B3> ;
  skos:member <http://anzsoil.org/def/au/scma/10B4> ;
  skos:member <http://anzsoil.org/def/au/scma/10C1> ;
  skos:member <http://anzsoil.org/def/au/scma/10D1> ;
  skos:notation "10" ;
  skos:prefLabel "Sulfur" ;
.
<http://anzsoil.org/def/au/scma/10A1>
  a skos:Concept ;
  a sosa:Procedure ;
  dcterms:description "Total S - X-ray fluorescence" ;
  dcterms:identifier "http://anzsoil.org/def/au/scma/10A1"^^xsd:anyURI ;
  dcterms:source "URN:ISBN:978-0-643-10218-7" ;
  rdfs:label "Total S - X-ray fluorescence" ;
  skos:definition "Total S - X-ray fluorescence" ;
  skos:inScheme <http://anzsoil.org/def/au/scma> ;
  skos:notation "10A1" ;
  skos:prefLabel "Total S - X-ray fluorescence" ;
  skos:topConceptOf <http://anzsoil.org/def/au/scma> ;
.
<http://anzsoil.org/def/au/scma/10A2>
  a skos:Concept ;
  a sosa:Procedure ;
  dcterms:description "Total soil S - high-temperature combustion" ;
  dcterms:identifier "http://anzsoil.org/def/au/scma/10A2"^^xsd:anyURI ;
  dcterms:source "URN:ISBN:978-0-643-10218-7" ;
  rdfs:label "Total soil S - high-temperature combustion" ;
  skos:definition "Total soil S - high-temperature combustion" ;
  skos:inScheme <http://anzsoil.org/def/au/scma> ;
  skos:notation "10A2" ;
  skos:prefLabel "Total soil S - high-temperature combustion" ;
  skos:topConceptOf <http://anzsoil.org/def/au/scma> ;
.
<http://anzsoil.org/def/au/scma/10B>
  a skos:Concept ;
  a sosa:Procedure ;
  dcterms:description "Calcium phosphate-extractable S" ;
  dcterms:identifier "http://anzsoil.org/def/au/scma/10B"^^xsd:anyURI ;
  dcterms:source "URN:ISBN:978-0-643-10218-7" ;
  rdfs:label "Calcium phosphate-extractable S" ;
  skos:definition "Calcium phosphate-extractable S" ;
  skos:inScheme <http://anzsoil.org/def/au/scma> ;
  skos:narrower <http://anzsoil.org/def/au/scma/10B1> ;
  skos:narrower <http://anzsoil.org/def/au/scma/10B2> ;
  skos:narrower <http://anzsoil.org/def/au/scma/10B3> ;
  skos:narrower <http://anzsoil.org/def/au/scma/10B4> ;
  skos:notation "10B" ;
  skos:prefLabel "Calcium phosphate-extractable S" ;
  skos:topConceptOf <http://anzsoil.org/def/au/scma> ;
.
<http://anzsoil.org/def/au/scma/10B1>
  a skos:Concept ;
  a sosa:Procedure ;
  dcterms:description "Calcium phosphate-extractable S - manual distillation" ;
  dcterms:identifier "http://anzsoil.org/def/au/scma/10B1"^^xsd:anyURI ;
  dcterms:source "URN:ISBN:978-0-643-10218-7" ;
  rdfs:label "Calcium phosphate-extractable S - manual distillation" ;
  skos:broader <http://anzsoil.org/def/au/scma/10B> ;
  skos:definition "Calcium phosphate-extractable S - manual distillation" ;
  skos:inScheme <http://anzsoil.org/def/au/scma> ;
  skos:notation "10B1" ;
  skos:prefLabel "Calcium phosphate-extractable S - manual distillation" ;
.
<http://anzsoil.org/def/au/scma/10B2>
  a skos:Concept ;
  a sosa:Procedure ;
  dcterms:description "Calcium phosphate-extractable S - automated distillation" ;
  dcterms:identifier "http://anzsoil.org/def/au/scma/10B2"^^xsd:anyURI ;
  dcterms:source "URN:ISBN:978-0-643-10218-7" ;
  rdfs:label "Calcium phosphate-extractable S - automated distillation" ;
  skos:broader <http://anzsoil.org/def/au/scma/10B> ;
  skos:definition "Calcium phosphate-extractable S - automated distillation" ;
  skos:inScheme <http://anzsoil.org/def/au/scma> ;
  skos:notation "10B2" ;
  skos:prefLabel "Calcium phosphate-extractable S - automated distillation" ;
.
<http://anzsoil.org/def/au/scma/10B3>
  a skos:Concept ;
  a sosa:Procedure ;
  dcterms:description "Calcium phosphate-extractable S - ICPAES" ;
  dcterms:identifier "http://anzsoil.org/def/au/scma/10B3"^^xsd:anyURI ;
  dcterms:source "URN:ISBN:978-0-643-10218-7" ;
  rdfs:label "Calcium phosphate-extractable S - ICPAES" ;
  skos:broader <http://anzsoil.org/def/au/scma/10B> ;
  skos:definition "Calcium phosphate-extractable S - ICPAES" ;
  skos:inScheme <http://anzsoil.org/def/au/scma> ;
  skos:notation "10B3" ;
  skos:prefLabel "Calcium phosphate-extractable S - ICPAES" ;
.
<http://anzsoil.org/def/au/scma/10B4>
  a skos:Concept ;
  a sosa:Procedure ;
  dcterms:description "Calcium phosphate-extractable S - ion chromatography" ;
  dcterms:identifier "http://anzsoil.org/def/au/scma/10B4"^^xsd:anyURI ;
  dcterms:source "URN:ISBN:978-0-643-10218-7" ;
  rdfs:label "Calcium phosphate-extractable S - ion chromatography" ;
  skos:broader <http://anzsoil.org/def/au/scma/10B> ;
  skos:definition "Calcium phosphate-extractable S - ion chromatography" ;
  skos:inScheme <http://anzsoil.org/def/au/scma> ;
  skos:notation "10B4" ;
  skos:prefLabel "Calcium phosphate-extractable S - ion chromatography" ;
.
<http://anzsoil.org/def/au/scma/10C1>
  a skos:Concept ;
  a sosa:Procedure ;
  dcterms:description "Calcium phosphate-extractable S - ICPAES, + charcoal (CPC-S)" ;
  dcterms:identifier "http://anzsoil.org/def/au/scma/10C1"^^xsd:anyURI ;
  dcterms:source "URN:ISBN:978-0-643-10218-7" ;
  rdfs:label "Calcium phosphate-extractable S - ICPAES, + charcoal (CPC-S)" ;
  skos:definition "Calcium phosphate-extractable S - ICPAES, + charcoal (CPC-S)" ;
  skos:inScheme <http://anzsoil.org/def/au/scma> ;
  skos:notation "10C1" ;
  skos:prefLabel "Calcium phosphate-extractable S - ICPAES, + charcoal (CPC-S)" ;
  skos:topConceptOf <http://anzsoil.org/def/au/scma> ;
.
<http://anzsoil.org/def/au/scma/10D1>
  a skos:Concept ;
  a sosa:Procedure ;
  dcterms:description "Potassium Chloride - 40 Sulfur (KCl-40)-S" ;
  dcterms:identifier "http://anzsoil.org/def/au/scma/10D1"^^xsd:anyURI ;
  dcterms:source "URN:ISBN:978-0-643-10218-7" ;
  rdfs:label "Potassium Chloride - 40 Sulfur (KCl-40)-S" ;
  skos:definition "Potassium Chloride - 40 Sulfur (KCl-40)-S" ;
  skos:inScheme <http://anzsoil.org/def/au/scma> ;
  skos:notation "10D1" ;
  skos:prefLabel "Potassium Chloride - 40 Sulfur (KCl-40)-S" ;
  skos:topConceptOf <http://anzsoil.org/def/au/scma> ;
.
<http://anzsoil.org/def/au/scma/11>
  a skos:Collection ;
  dcterms:description "Gypsum" ;
  dcterms:identifier "http://anzsoil.org/def/au/scma/11"^^xsd:anyURI ;
  dcterms:source "URN:ISBN:978-0-643-10218-7" ;
  ui:topMemberOf <http://anzsoil.org/def/au/scma> ;
  rdfs:label "Gypsum" ;
  skos:definition "Gypsum" ;
  skos:inScheme <http://anzsoil.org/def/au/scma> ;
  skos:member <http://anzsoil.org/def/au/scma/11A1> ;
  skos:member <http://anzsoil.org/def/au/scma/11A2> ;
  skos:notation "11" ;
  skos:prefLabel "Gypsum" ;
.
<http://anzsoil.org/def/au/scma/11A1>
  a skos:Concept ;
  a sosa:Procedure ;
  dcterms:description "Total gypsum" ;
  dcterms:identifier "http://anzsoil.org/def/au/scma/11A1"^^xsd:anyURI ;
  dcterms:source "URN:ISBN:978-0-643-10218-7" ;
  rdfs:label "Total gypsum" ;
  skos:definition "Total gypsum" ;
  skos:inScheme <http://anzsoil.org/def/au/scma> ;
  skos:notation "11A1" ;
  skos:prefLabel "Total gypsum" ;
  skos:topConceptOf <http://anzsoil.org/def/au/scma> ;
.
<http://anzsoil.org/def/au/scma/11A2>
  a skos:Concept ;
  a sosa:Procedure ;
  dcterms:description "Total gypsum by MIR reflectance spectroscopy" ;
  dcterms:identifier "http://anzsoil.org/def/au/scma/11A2"^^xsd:anyURI ;
  dcterms:source "URN:ISBN:978-0-643-10218-7" ;
  rdfs:label "Total gypsum by MIR reflectance spectroscopy" ;
  skos:definition "Total gypsum by MIR reflectance spectroscopy" ;
  skos:inScheme <http://anzsoil.org/def/au/scma> ;
  skos:notation "11A2" ;
  skos:prefLabel "Total gypsum by MIR reflectance spectroscopy" ;
  skos:topConceptOf <http://anzsoil.org/def/au/scma> ;
.
<http://anzsoil.org/def/au/scma/12>
  a skos:Collection ;
  dcterms:description "Micronutrients" ;
  dcterms:identifier "http://anzsoil.org/def/au/scma/12"^^xsd:anyURI ;
  dcterms:source "URN:ISBN:978-0-643-10218-7" ;
  ui:topMemberOf <http://anzsoil.org/def/au/scma> ;
  rdfs:label "Micronutrients" ;
  skos:definition "Micronutrients" ;
  skos:inScheme <http://anzsoil.org/def/au/scma> ;
  skos:member <http://anzsoil.org/def/au/scma/12A1> ;
  skos:member <http://anzsoil.org/def/au/scma/12B1> ;
  skos:member <http://anzsoil.org/def/au/scma/12C1> ;
  skos:member <http://anzsoil.org/def/au/scma/12C2> ;
  skos:member <http://anzsoil.org/def/au/scma/12D1> ;
  skos:member <http://anzsoil.org/def/au/scma/12E1> ;
  skos:notation "12" ;
  skos:prefLabel "Micronutrients" ;
.
<http://anzsoil.org/def/au/scma/12A1>
  a skos:Concept ;
  a sosa:Procedure ;
  dcterms:description "DTPA-extractable Cu, Zn, Mn and Fe" ;
  dcterms:identifier "http://anzsoil.org/def/au/scma/12A1"^^xsd:anyURI ;
  dcterms:source "URN:ISBN:978-0-643-10218-7" ;
  rdfs:label "DTPA-extractable Cu, Zn, Mn and Fe" ;
  skos:definition "DTPA-extractable Cu, Zn, Mn and Fe" ;
  skos:inScheme <http://anzsoil.org/def/au/scma> ;
  skos:notation "12A1" ;
  skos:prefLabel "DTPA-extractable Cu, Zn, Mn and Fe" ;
  skos:topConceptOf <http://anzsoil.org/def/au/scma> ;
.
<http://anzsoil.org/def/au/scma/12B1>
  a skos:Concept ;
  a sosa:Procedure ;
  dcterms:description "Ammonium bicarbonate/EDTA-extractable Cu and Zn" ;
  dcterms:identifier "http://anzsoil.org/def/au/scma/12B1"^^xsd:anyURI ;
  dcterms:source "URN:ISBN:978-0-643-10218-7" ;
  rdfs:label "Ammonium bicarbonate/EDTA-extractable Cu and Zn" ;
  skos:definition "Ammonium bicarbonate/EDTA-extractable Cu and Zn" ;
  skos:inScheme <http://anzsoil.org/def/au/scma> ;
  skos:notation "12B1" ;
  skos:prefLabel "Ammonium bicarbonate/EDTA-extractable Cu and Zn" ;
  skos:topConceptOf <http://anzsoil.org/def/au/scma> ;
.
<http://anzsoil.org/def/au/scma/12C1>
  a skos:Concept ;
  a sosa:Procedure ;
  dcterms:description "Calcium chloride-extractable B - manual colour" ;
  dcterms:identifier "http://anzsoil.org/def/au/scma/12C1"^^xsd:anyURI ;
  dcterms:source "URN:ISBN:978-0-643-10218-7" ;
  rdfs:label "Calcium chloride-extractable B - manual colour" ;
  skos:definition "Calcium chloride-extractable B - manual colour" ;
  skos:inScheme <http://anzsoil.org/def/au/scma> ;
  skos:notation "12C1" ;
  skos:prefLabel "Calcium chloride-extractable B - manual colour" ;
  skos:topConceptOf <http://anzsoil.org/def/au/scma> ;
.
<http://anzsoil.org/def/au/scma/12C2>
  a skos:Concept ;
  a sosa:Procedure ;
  dcterms:description "Calcium chloride-extractable B - ICPAES" ;
  dcterms:identifier "http://anzsoil.org/def/au/scma/12C2"^^xsd:anyURI ;
  dcterms:source "URN:ISBN:978-0-643-10218-7" ;
  rdfs:label "Calcium chloride-extractable B - ICPAES" ;
  skos:definition "Calcium chloride-extractable B - ICPAES" ;
  skos:inScheme <http://anzsoil.org/def/au/scma> ;
  skos:notation "12C2" ;
  skos:prefLabel "Calcium chloride-extractable B - ICPAES" ;
  skos:topConceptOf <http://anzsoil.org/def/au/scma> ;
.
<http://anzsoil.org/def/au/scma/12D1>
  a skos:Concept ;
  a sosa:Procedure ;
  dcterms:description "0.1 M HCl-extractable Cu, Zn, Mn and Fe" ;
  dcterms:identifier "http://anzsoil.org/def/au/scma/12D1"^^xsd:anyURI ;
  dcterms:source "URN:ISBN:978-0-643-10218-7" ;
  rdfs:label "0.1 M HCl-extractable Cu, Zn, Mn and Fe" ;
  skos:definition "0.1 M HCl-extractable Cu, Zn, Mn and Fe" ;
  skos:inScheme <http://anzsoil.org/def/au/scma> ;
  skos:notation "12D1" ;
  skos:prefLabel "0.1 M HCl-extractable Cu, Zn, Mn and Fe" ;
  skos:topConceptOf <http://anzsoil.org/def/au/scma> ;
.
<http://anzsoil.org/def/au/scma/12E1>
  a skos:Concept ;
  a sosa:Procedure ;
  dcterms:description "Calcium chloride-extractable Mo" ;
  dcterms:identifier "http://anzsoil.org/def/au/scma/12E1"^^xsd:anyURI ;
  dcterms:source "URN:ISBN:978-0-643-10218-7" ;
  rdfs:label "Calcium chloride-extractable Mo" ;
  skos:definition "Calcium chloride-extractable Mo" ;
  skos:inScheme <http://anzsoil.org/def/au/scma> ;
  skos:notation "12E1" ;
  skos:prefLabel "Calcium chloride-extractable Mo" ;
  skos:topConceptOf <http://anzsoil.org/def/au/scma> ;
.
<http://anzsoil.org/def/au/scma/13>
  a skos:Collection ;
  dcterms:description "Extractable iron, aluminium and silicon" ;
  dcterms:identifier "http://anzsoil.org/def/au/scma/13"^^xsd:anyURI ;
  dcterms:source "URN:ISBN:978-0-643-10218-7" ;
  ui:topMemberOf <http://anzsoil.org/def/au/scma> ;
  rdfs:label "Extractable iron, aluminium and silicon" ;
  skos:definition "Extractable iron, aluminium and silicon" ;
  skos:inScheme <http://anzsoil.org/def/au/scma> ;
  skos:member <http://anzsoil.org/def/au/scma/13A1> ;
  skos:member <http://anzsoil.org/def/au/scma/13B1> ;
  skos:member <http://anzsoil.org/def/au/scma/13C1> ;
  skos:member <http://anzsoil.org/def/au/scma/13D> ;
  skos:member <http://anzsoil.org/def/au/scma/13D1> ;
  skos:member <http://anzsoil.org/def/au/scma/13D2> ;
  skos:notation "13" ;
  skos:prefLabel "Extractable iron, aluminium and silicon" ;
.
<http://anzsoil.org/def/au/scma/13A1>
  a skos:Concept ;
  a sosa:Procedure ;
  dcterms:description "Oxalate-extractable iron, aluminium and silicon" ;
  dcterms:identifier "http://anzsoil.org/def/au/scma/13A1"^^xsd:anyURI ;
  dcterms:source "URN:ISBN:978-0-643-10218-7" ;
  rdfs:label "Oxalate-extractable iron, aluminium and silicon" ;
  skos:definition "Oxalate-extractable iron, aluminium and silicon" ;
  skos:inScheme <http://anzsoil.org/def/au/scma> ;
  skos:notation "13A1" ;
  skos:prefLabel "Oxalate-extractable iron, aluminium and silicon" ;
  skos:topConceptOf <http://anzsoil.org/def/au/scma> ;
.
<http://anzsoil.org/def/au/scma/13B1>
  a skos:Concept ;
  a sosa:Procedure ;
  dcterms:description "Pyrophosphate-extractable Fe and Al" ;
  dcterms:identifier "http://anzsoil.org/def/au/scma/13B1"^^xsd:anyURI ;
  dcterms:source "URN:ISBN:978-0-643-10218-7" ;
  rdfs:label "Pyrophosphate-extractable Fe and Al" ;
  skos:definition "Pyrophosphate-extractable Fe and Al" ;
  skos:inScheme <http://anzsoil.org/def/au/scma> ;
  skos:notation "13B1" ;
  skos:prefLabel "Pyrophosphate-extractable Fe and Al" ;
  skos:topConceptOf <http://anzsoil.org/def/au/scma> ;
.
<http://anzsoil.org/def/au/scma/13C1>
  a skos:Concept ;
  a sosa:Procedure ;
  dcterms:description "Citrate/dihionite-extractable iron and aluminium" ;
  dcterms:identifier "http://anzsoil.org/def/au/scma/13C1"^^xsd:anyURI ;
  dcterms:source "URN:ISBN:978-0-643-10218-7" ;
  rdfs:label "Citrate/dihionite-extractable iron and aluminium" ;
  skos:definition "Citrate/dihionite-extractable iron and aluminium" ;
  skos:inScheme <http://anzsoil.org/def/au/scma> ;
  skos:notation "13C1" ;
  skos:prefLabel "Citrate/dihionite-extractable iron and aluminium" ;
  skos:topConceptOf <http://anzsoil.org/def/au/scma> ;
.
<http://anzsoil.org/def/au/scma/13D>
  a skos:Concept ;
  a sosa:Procedure ;
  dcterms:description "Acid-extractable soil silicon" ;
  dcterms:identifier "http://anzsoil.org/def/au/scma/13D"^^xsd:anyURI ;
  dcterms:source "URN:ISBN:978-0-643-10218-7" ;
  rdfs:label "Acid-extractable soil silicon" ;
  skos:definition "Acid-extractable soil silicon" ;
  skos:inScheme <http://anzsoil.org/def/au/scma> ;
  skos:narrower <http://anzsoil.org/def/au/scma/13D1> ;
  skos:narrower <http://anzsoil.org/def/au/scma/13D2> ;
  skos:notation "13D" ;
  skos:prefLabel "Acid-extractable soil silicon" ;
  skos:topConceptOf <http://anzsoil.org/def/au/scma> ;
.
<http://anzsoil.org/def/au/scma/13D1>
  a skos:Concept ;
  a sosa:Procedure ;
  dcterms:description "Acid-extractable soil silicon - automated colour" ;
  dcterms:identifier "http://anzsoil.org/def/au/scma/13D1"^^xsd:anyURI ;
  dcterms:source "URN:ISBN:978-0-643-10218-7" ;
  rdfs:label "Acid-extractable soil silicon - automated colour" ;
  skos:broader <http://anzsoil.org/def/au/scma/13D> ;
  skos:definition "Acid-extractable soil silicon - automated colour" ;
  skos:inScheme <http://anzsoil.org/def/au/scma> ;
  skos:notation "13D1" ;
  skos:prefLabel "Acid-extractable soil silicon - automated colour" ;
.
<http://anzsoil.org/def/au/scma/13D2>
  a skos:Concept ;
  a sosa:Procedure ;
  dcterms:description "Acid-extractable soil silicon - ICPAES" ;
  dcterms:identifier "http://anzsoil.org/def/au/scma/13D2"^^xsd:anyURI ;
  dcterms:source "URN:ISBN:978-0-643-10218-7" ;
  rdfs:label "Acid-extractable soil silicon - ICPAES" ;
  skos:broader <http://anzsoil.org/def/au/scma/13D> ;
  skos:definition "Acid-extractable soil silicon - ICPAES" ;
  skos:inScheme <http://anzsoil.org/def/au/scma> ;
  skos:notation "13D2" ;
  skos:prefLabel "Acid-extractable soil silicon - ICPAES" ;
.
<http://anzsoil.org/def/au/scma/14>
  a skos:Collection ;
  dcterms:description "Saturation extracts" ;
  dcterms:identifier "http://anzsoil.org/def/au/scma/14"^^xsd:anyURI ;
  dcterms:source "URN:ISBN:978-0-643-10218-7" ;
  ui:topMemberOf <http://anzsoil.org/def/au/scma> ;
  rdfs:label "Saturation extracts" ;
  skos:definition "Saturation extracts" ;
  skos:inScheme <http://anzsoil.org/def/au/scma> ;
  skos:member <http://anzsoil.org/def/au/scma/14A1> ;
  skos:member <http://anzsoil.org/def/au/scma/14A2> ;
  skos:member <http://anzsoil.org/def/au/scma/14A3> ;
  skos:member <http://anzsoil.org/def/au/scma/14A4> ;
  skos:member <http://anzsoil.org/def/au/scma/14B1> ;
  skos:member <http://anzsoil.org/def/au/scma/14C1> ;
  skos:member <http://anzsoil.org/def/au/scma/14D1> ;
  skos:member <http://anzsoil.org/def/au/scma/14D2> ;
  skos:member <http://anzsoil.org/def/au/scma/14E1> ;
  skos:member <http://anzsoil.org/def/au/scma/14E2> ;
  skos:member <http://anzsoil.org/def/au/scma/14E2a> ;
  skos:member <http://anzsoil.org/def/au/scma/14E2b> ;
  skos:member <http://anzsoil.org/def/au/scma/14E3> ;
  skos:member <http://anzsoil.org/def/au/scma/14F1> ;
  skos:member <http://anzsoil.org/def/au/scma/14F2> ;
  skos:member <http://anzsoil.org/def/au/scma/14F3> ;
  skos:member <http://anzsoil.org/def/au/scma/14F4> ;
  skos:member <http://anzsoil.org/def/au/scma/14F5> ;
  skos:member <http://anzsoil.org/def/au/scma/14F5a> ;
  skos:member <http://anzsoil.org/def/au/scma/14F5b> ;
  skos:member <http://anzsoil.org/def/au/scma/14G1> ;
  skos:member <http://anzsoil.org/def/au/scma/14G2> ;
  skos:member <http://anzsoil.org/def/au/scma/14G2a> ;
  skos:member <http://anzsoil.org/def/au/scma/14G2b> ;
  skos:member <http://anzsoil.org/def/au/scma/14H1> ;
  skos:notation "14" ;
  skos:prefLabel "Saturation extracts" ;
.
<http://anzsoil.org/def/au/scma/14A1>
  a skos:Concept ;
  a sosa:Procedure ;
  dcterms:description "Saturation extract - filter suction" ;
  dcterms:identifier "http://anzsoil.org/def/au/scma/14A1"^^xsd:anyURI ;
  dcterms:source "URN:ISBN:978-0-643-10218-7" ;
  rdfs:label "Saturation extract - filter suction" ;
  skos:definition "Saturation extract - filter suction" ;
  skos:inScheme <http://anzsoil.org/def/au/scma> ;
  skos:notation "14A1" ;
  skos:prefLabel "Saturation extract - filter suction" ;
  skos:topConceptOf <http://anzsoil.org/def/au/scma> ;
.
<http://anzsoil.org/def/au/scma/14A2>
  a skos:Concept ;
  a sosa:Procedure ;
  dcterms:description "Saturation extract -automatic extractor" ;
  dcterms:identifier "http://anzsoil.org/def/au/scma/14A2"^^xsd:anyURI ;
  dcterms:source "URN:ISBN:978-0-643-10218-7" ;
  rdfs:label "Saturation extract -automatic extractor" ;
  skos:definition "Saturation extract -automatic extractor" ;
  skos:inScheme <http://anzsoil.org/def/au/scma> ;
  skos:notation "14A2" ;
  skos:prefLabel "Saturation extract -automatic extractor" ;
  skos:topConceptOf <http://anzsoil.org/def/au/scma> ;
.
<http://anzsoil.org/def/au/scma/14A3>
  a skos:Concept ;
  a sosa:Procedure ;
  dcterms:description "Saturation extract - centrifuge, closed system" ;
  dcterms:identifier "http://anzsoil.org/def/au/scma/14A3"^^xsd:anyURI ;
  dcterms:source "URN:ISBN:978-0-643-10218-7" ;
  rdfs:label "Saturation extract - centrifuge, closed system" ;
  skos:definition "Saturation extract - centrifuge, closed system" ;
  skos:inScheme <http://anzsoil.org/def/au/scma> ;
  skos:notation "14A3" ;
  skos:prefLabel "Saturation extract - centrifuge, closed system" ;
  skos:topConceptOf <http://anzsoil.org/def/au/scma> ;
.
<http://anzsoil.org/def/au/scma/14A4>
  a skos:Concept ;
  a sosa:Procedure ;
  dcterms:description "Saturation extract - centrifuge, Gillman" ;
  dcterms:identifier "http://anzsoil.org/def/au/scma/14A4"^^xsd:anyURI ;
  dcterms:source "URN:ISBN:978-0-643-10218-7" ;
  rdfs:label "Saturation extract - centrifuge, Gillman" ;
  skos:definition "Saturation extract - centrifuge, Gillman" ;
  skos:inScheme <http://anzsoil.org/def/au/scma> ;
  skos:notation "14A4" ;
  skos:prefLabel "Saturation extract - centrifuge, Gillman" ;
  skos:topConceptOf <http://anzsoil.org/def/au/scma> ;
.
<http://anzsoil.org/def/au/scma/14B1>
  a skos:Concept ;
  a sosa:Procedure ;
  dcterms:description "Electrical conductivity of SE (EC of SE)" ;
  dcterms:identifier "http://anzsoil.org/def/au/scma/14B1"^^xsd:anyURI ;
  dcterms:source "URN:ISBN:978-0-643-10218-7" ;
  rdfs:label "Electrical conductivity of SE (EC of SE)" ;
  skos:definition "Electrical conductivity of SE (EC of SE)" ;
  skos:inScheme <http://anzsoil.org/def/au/scma> ;
  skos:notation "14B1" ;
  skos:prefLabel "Electrical conductivity of SE (EC of SE)" ;
  skos:topConceptOf <http://anzsoil.org/def/au/scma> ;
.
<http://anzsoil.org/def/au/scma/14C1>
  a skos:Concept ;
  a sosa:Procedure ;
  dcterms:description "pH of SE" ;
  dcterms:identifier "http://anzsoil.org/def/au/scma/14C1"^^xsd:anyURI ;
  dcterms:source "URN:ISBN:978-0-643-10218-7" ;
  rdfs:label "pH of SE" ;
  skos:definition "pH of SE" ;
  skos:inScheme <http://anzsoil.org/def/au/scma> ;
  skos:notation "14C1" ;
  skos:prefLabel "pH of SE" ;
  skos:topConceptOf <http://anzsoil.org/def/au/scma> ;
.
<http://anzsoil.org/def/au/scma/14D1>
  a skos:Concept ;
  a sosa:Procedure ;
  dcterms:description "Bicarbonate of SE and carbonate of SE - potentiometric titration" ;
  dcterms:identifier "http://anzsoil.org/def/au/scma/14D1"^^xsd:anyURI ;
  dcterms:source "URN:ISBN:978-0-643-10218-7" ;
  rdfs:label "Bicarbonate of SE and carbonate of SE - potentiometric titration" ;
  skos:definition "Bicarbonate of SE and carbonate of SE - potentiometric titration" ;
  skos:inScheme <http://anzsoil.org/def/au/scma> ;
  skos:notation "14D1" ;
  skos:prefLabel "Bicarbonate of SE and carbonate of SE - potentiometric titration" ;
  skos:topConceptOf <http://anzsoil.org/def/au/scma> ;
.
<http://anzsoil.org/def/au/scma/14D2>
  a skos:Concept ;
  a sosa:Procedure ;
  dcterms:description "Bicarbonate of SE and carbonate of SE - indicator method" ;
  dcterms:identifier "http://anzsoil.org/def/au/scma/14D2"^^xsd:anyURI ;
  dcterms:source "URN:ISBN:978-0-643-10218-7" ;
  rdfs:label "Bicarbonate of SE and carbonate of SE - indicator method" ;
  skos:definition "Bicarbonate of SE and carbonate of SE - indicator method" ;
  skos:inScheme <http://anzsoil.org/def/au/scma> ;
  skos:notation "14D2" ;
  skos:prefLabel "Bicarbonate of SE and carbonate of SE - indicator method" ;
  skos:topConceptOf <http://anzsoil.org/def/au/scma> ;
.
<http://anzsoil.org/def/au/scma/14E1>
  a skos:Concept ;
  a sosa:Procedure ;
  dcterms:description "Chloride of SE - potentiometric titration" ;
  dcterms:identifier "http://anzsoil.org/def/au/scma/14E1"^^xsd:anyURI ;
  dcterms:source "URN:ISBN:978-0-643-10218-7" ;
  rdfs:label "Chloride of SE - potentiometric titration" ;
  skos:definition "Chloride of SE - potentiometric titration" ;
  skos:inScheme <http://anzsoil.org/def/au/scma> ;
  skos:notation "14E1" ;
  skos:prefLabel "Chloride of SE - potentiometric titration" ;
  skos:topConceptOf <http://anzsoil.org/def/au/scma> ;
.
<http://anzsoil.org/def/au/scma/14E2>
  a skos:Concept ;
  a sosa:Procedure ;
  dcterms:description "Chloride (saturation extract) - ion chromotography|Chloride of SE - IC" ;
  dcterms:identifier "http://anzsoil.org/def/au/scma/14E2"^^xsd:anyURI ;
  dcterms:isReplacedBy <http://anzsoil.org/def/au/scma/14E2a> ;
  dcterms:isReplacedBy <http://anzsoil.org/def/au/scma/14E2b> ;
  dcterms:source "URN:ISBN:978-0-909605-68-1" ;
  rdfs:label "Chloride (saturation extract) - ion chromotography|Chloride of SE - IC" ;
  skos:definition "Chloride (saturation extract) - ion chromotography|Chloride of SE - IC" ;
  skos:inScheme <http://anzsoil.org/def/au/scma> ;
  skos:narrower <http://anzsoil.org/def/au/scma/14E2a> ;
  skos:narrower <http://anzsoil.org/def/au/scma/14E2b> ;
  skos:notation "14E2" ;
  skos:note "14E2 has been superseded by 14E2a and 14E2b in Soil Chemical Methods Australasia, Rayment G.E. and Lyons D.J. ISBN 9780643101364" ;
  skos:prefLabel "Chloride (saturation extract) - ion chromotography|Chloride of SE - IC" ;
  skos:topConceptOf <http://anzsoil.org/def/au/scma> ;
.
<http://anzsoil.org/def/au/scma/14E2a>
  a skos:Concept ;
  a sosa:Procedure ;
  dcterms:description "Chloride of SE - IC (chemical suppression of eluent conductivity)" ;
  dcterms:identifier "http://anzsoil.org/def/au/scma/14E2a"^^xsd:anyURI ;
  dcterms:source "URN:ISBN:978-0-643-10218-7" ;
  rdfs:label "Chloride of SE - IC (chemical suppression of eluent conductivity)" ;
  skos:broader <http://anzsoil.org/def/au/scma/14E2> ;
  skos:definition "Chloride of SE - IC (chemical suppression of eluent conductivity)" ;
  skos:inScheme <http://anzsoil.org/def/au/scma> ;
  skos:notation "14E2a" ;
  skos:prefLabel "Chloride of SE - IC (chemical suppression of eluent conductivity)" ;
.
<http://anzsoil.org/def/au/scma/14E2b>
  a skos:Concept ;
  a sosa:Procedure ;
  dcterms:description "Chloride of SE - IC (single-column with electronic suppression of eluent conductivity)" ;
  dcterms:identifier "http://anzsoil.org/def/au/scma/14E2b"^^xsd:anyURI ;
  dcterms:source "URN:ISBN:978-0-643-10218-7" ;
  rdfs:label "Chloride of SE - IC (single-column with electronic suppression of eluent conductivity)" ;
  skos:broader <http://anzsoil.org/def/au/scma/14E2> ;
  skos:definition "Chloride of SE - IC (single-column with electronic suppression of eluent conductivity)" ;
  skos:inScheme <http://anzsoil.org/def/au/scma> ;
  skos:notation "14E2b" ;
  skos:prefLabel "Chloride of SE - IC (single-column with electronic suppression of eluent conductivity)" ;
.
<http://anzsoil.org/def/au/scma/14E3>
  a skos:Concept ;
  a sosa:Procedure ;
  dcterms:description "Chloride of SE - ICPAES" ;
  dcterms:identifier "http://anzsoil.org/def/au/scma/14E3"^^xsd:anyURI ;
  dcterms:source "URN:ISBN:978-0-643-10218-7" ;
  rdfs:label "Chloride of SE - ICPAES" ;
  skos:definition "Chloride of SE - ICPAES" ;
  skos:inScheme <http://anzsoil.org/def/au/scma> ;
  skos:notation "14E3" ;
  skos:prefLabel "Chloride of SE - ICPAES" ;
  skos:topConceptOf <http://anzsoil.org/def/au/scma> ;
.
<http://anzsoil.org/def/au/scma/14F1>
  a skos:Concept ;
  a sosa:Procedure ;
  dcterms:description "Sulfate-S of SE - ICPAES (plus P and soluble cations)" ;
  dcterms:identifier "http://anzsoil.org/def/au/scma/14F1"^^xsd:anyURI ;
  dcterms:source "URN:ISBN:978-0-643-10218-7" ;
  rdfs:label "Sulfate-S of SE - ICPAES (plus P and soluble cations)" ;
  skos:definition "Sulfate-S of SE - ICPAES (plus P and soluble cations)" ;
  skos:inScheme <http://anzsoil.org/def/au/scma> ;
  skos:notation "14F1" ;
  skos:prefLabel "Sulfate-S of SE - ICPAES (plus P and soluble cations)" ;
  skos:topConceptOf <http://anzsoil.org/def/au/scma> ;
.
<http://anzsoil.org/def/au/scma/14F2>
  a skos:Concept ;
  a sosa:Procedure ;
  dcterms:description "Sulfate-S of SE - turbidimetric" ;
  dcterms:identifier "http://anzsoil.org/def/au/scma/14F2"^^xsd:anyURI ;
  dcterms:source "URN:ISBN:978-0-643-10218-7" ;
  rdfs:label "Sulfate-S of SE - turbidimetric" ;
  skos:definition "Sulfate-S of SE - turbidimetric" ;
  skos:inScheme <http://anzsoil.org/def/au/scma> ;
  skos:notation "14F2" ;
  skos:prefLabel "Sulfate-S of SE - turbidimetric" ;
  skos:topConceptOf <http://anzsoil.org/def/au/scma> ;
.
<http://anzsoil.org/def/au/scma/14F3>
  a skos:Concept ;
  a sosa:Procedure ;
  dcterms:description "Sulfate-S of SE - gravimetric" ;
  dcterms:identifier "http://anzsoil.org/def/au/scma/14F3"^^xsd:anyURI ;
  dcterms:source "URN:ISBN:978-0-643-10218-7" ;
  rdfs:label "Sulfate-S of SE - gravimetric" ;
  skos:definition "Sulfate-S of SE - gravimetric" ;
  skos:inScheme <http://anzsoil.org/def/au/scma> ;
  skos:notation "14F3" ;
  skos:prefLabel "Sulfate-S of SE - gravimetric" ;
  skos:topConceptOf <http://anzsoil.org/def/au/scma> ;
.
<http://anzsoil.org/def/au/scma/14F4>
  a skos:Concept ;
  a sosa:Procedure ;
  dcterms:description "Sulfate-S of SE - automated colour" ;
  dcterms:identifier "http://anzsoil.org/def/au/scma/14F4"^^xsd:anyURI ;
  dcterms:source "URN:ISBN:978-0-643-10218-7" ;
  rdfs:label "Sulfate-S of SE - automated colour" ;
  skos:definition "Sulfate-S of SE - automated colour" ;
  skos:inScheme <http://anzsoil.org/def/au/scma> ;
  skos:notation "14F4" ;
  skos:prefLabel "Sulfate-S of SE - automated colour" ;
  skos:topConceptOf <http://anzsoil.org/def/au/scma> ;
.
<http://anzsoil.org/def/au/scma/14F5>
  a skos:Concept ;
  a sosa:Procedure ;
  dcterms:description "Sulfate-S (saturation extract) - ion chromotography|Sulfate-S of SE - IC" ;
  dcterms:identifier "http://anzsoil.org/def/au/scma/14F5"^^xsd:anyURI ;
  dcterms:isReplacedBy <http://anzsoil.org/def/au/scma/14F5a> ;
  dcterms:isReplacedBy <http://anzsoil.org/def/au/scma/14F5b> ;
  dcterms:source "URN:ISBN:978-0-909605-68-1" ;
  rdfs:label "Sulfate-S (saturation extract) - ion chromotography|Sulfate-S of SE - IC" ;
  skos:definition "Sulfate-S (saturation extract) - ion chromotography|Sulfate-S of SE - IC" ;
  skos:inScheme <http://anzsoil.org/def/au/scma> ;
  skos:narrower <http://anzsoil.org/def/au/scma/14F5a> ;
  skos:narrower <http://anzsoil.org/def/au/scma/14F5b> ;
  skos:notation "14F5" ;
  skos:note "14F5 has been superseded by 14F5a and 14F5b in Soil Chemical Methods Australasia, Rayment G.E. and Lyons D.J. ISBN 9780643101364" ;
  skos:prefLabel "Sulfate-S (saturation extract) - ion chromotography|Sulfate-S of SE - IC" ;
  skos:topConceptOf <http://anzsoil.org/def/au/scma> ;
.
<http://anzsoil.org/def/au/scma/14F5a>
  a skos:Concept ;
  a sosa:Procedure ;
  dcterms:description "Sulfate-S of SE - IC (chemical suppression of eluent conductivity)" ;
  dcterms:identifier "http://anzsoil.org/def/au/scma/14F5a"^^xsd:anyURI ;
  dcterms:source "URN:ISBN:978-0-643-10218-7" ;
  rdfs:label "Sulfate-S of SE - IC (chemical suppression of eluent conductivity)" ;
  skos:broader <http://anzsoil.org/def/au/scma/14F5> ;
  skos:definition "Sulfate-S of SE - IC (chemical suppression of eluent conductivity)" ;
  skos:inScheme <http://anzsoil.org/def/au/scma> ;
  skos:notation "14F5a" ;
  skos:prefLabel "Sulfate-S of SE - IC (chemical suppression of eluent conductivity)" ;
.
<http://anzsoil.org/def/au/scma/14F5b>
  a skos:Concept ;
  a sosa:Procedure ;
  dcterms:description "Sulfate-S of SE - IC (single-column with electronic suppression of eluent conductivity)" ;
  dcterms:identifier "http://anzsoil.org/def/au/scma/14F5b"^^xsd:anyURI ;
  dcterms:source "URN:ISBN:978-0-643-10218-7" ;
  rdfs:label "Sulfate-S of SE - IC (single-column with electronic suppression of eluent conductivity)" ;
  skos:broader <http://anzsoil.org/def/au/scma/14F5> ;
  skos:definition "Sulfate-S of SE - IC (single-column with electronic suppression of eluent conductivity)" ;
  skos:inScheme <http://anzsoil.org/def/au/scma> ;
  skos:notation "14F5b" ;
  skos:prefLabel "Sulfate-S of SE - IC (single-column with electronic suppression of eluent conductivity)" ;
.
<http://anzsoil.org/def/au/scma/14G1>
  a skos:Concept ;
  a sosa:Procedure ;
  dcterms:description "Fluoride of SE - specific ion electrode" ;
  dcterms:identifier "http://anzsoil.org/def/au/scma/14G1"^^xsd:anyURI ;
  dcterms:source "URN:ISBN:978-0-643-10218-7" ;
  rdfs:label "Fluoride of SE - specific ion electrode" ;
  skos:definition "Fluoride of SE - specific ion electrode" ;
  skos:inScheme <http://anzsoil.org/def/au/scma> ;
  skos:notation "14G1" ;
  skos:prefLabel "Fluoride of SE - specific ion electrode" ;
  skos:topConceptOf <http://anzsoil.org/def/au/scma> ;
.
<http://anzsoil.org/def/au/scma/14G2>
  a skos:Concept ;
  a sosa:Procedure ;
  dcterms:description "Fluoride (saturation extract) - ion chromotography|Fluoride of SE - IC" ;
  dcterms:identifier "http://anzsoil.org/def/au/scma/14G2"^^xsd:anyURI ;
  dcterms:isReplacedBy <http://anzsoil.org/def/au/scma/14G2a> ;
  dcterms:isReplacedBy <http://anzsoil.org/def/au/scma/14G2b> ;
  dcterms:source "URN:ISBN:978-0-909605-68-1" ;
  rdfs:label "Fluoride (saturation extract) - ion chromotography|Fluoride of SE - IC" ;
  skos:definition "Fluoride (saturation extract) - ion chromotography|Fluoride of SE - IC" ;
  skos:inScheme <http://anzsoil.org/def/au/scma> ;
  skos:narrower <http://anzsoil.org/def/au/scma/14G2a> ;
  skos:narrower <http://anzsoil.org/def/au/scma/14G2b> ;
  skos:notation "14G2" ;
  skos:note "14G2 has been superseded by 14G2a and 14G2b in Soil Chemical Methods Australasia, Rayment G.E. and Lyons D.J. ISBN 9780643101364" ;
  skos:prefLabel "Fluoride (saturation extract) - ion chromotography|Fluoride of SE - IC" ;
  skos:topConceptOf <http://anzsoil.org/def/au/scma> ;
.
<http://anzsoil.org/def/au/scma/14G2a>
  a skos:Concept ;
  a sosa:Procedure ;
  dcterms:description "Fluoride of SE - IC (chemical suppression of eluent conductivity)" ;
  dcterms:identifier "http://anzsoil.org/def/au/scma/14G2a"^^xsd:anyURI ;
  dcterms:source "URN:ISBN:978-0-643-10218-7" ;
  rdfs:label "Fluoride of SE - IC (chemical suppression of eluent conductivity)" ;
  skos:broader <http://anzsoil.org/def/au/scma/14G2> ;
  skos:definition "Fluoride of SE - IC (chemical suppression of eluent conductivity)" ;
  skos:inScheme <http://anzsoil.org/def/au/scma> ;
  skos:notation "14G2a" ;
  skos:prefLabel "Fluoride of SE - IC (chemical suppression of eluent conductivity)" ;
.
<http://anzsoil.org/def/au/scma/14G2b>
  a skos:Concept ;
  a sosa:Procedure ;
  dcterms:description "Fluoride of SE - IC (single-column with electronic suppression of eluent conductivity)" ;
  dcterms:identifier "http://anzsoil.org/def/au/scma/14G2b"^^xsd:anyURI ;
  dcterms:source "URN:ISBN:978-0-643-10218-7" ;
  rdfs:label "Fluoride of SE - IC (single-column with electronic suppression of eluent conductivity)" ;
  skos:broader <http://anzsoil.org/def/au/scma/14G2> ;
  skos:definition "Fluoride of SE - IC (single-column with electronic suppression of eluent conductivity)" ;
  skos:inScheme <http://anzsoil.org/def/au/scma> ;
  skos:notation "14G2b" ;
  skos:prefLabel "Fluoride of SE - IC (single-column with electronic suppression of eluent conductivity)" ;
.
<http://anzsoil.org/def/au/scma/14H1>
  a skos:Concept ;
  a sosa:Procedure ;
  dcterms:description "Soluble bases of SE (Ca, Mg, K, Na)" ;
  dcterms:identifier "http://anzsoil.org/def/au/scma/14H1"^^xsd:anyURI ;
  dcterms:source "URN:ISBN:978-0-643-10218-7" ;
  rdfs:label "Soluble bases of SE (Ca, Mg, K, Na)" ;
  skos:definition "Soluble bases of SE (Ca, Mg, K, Na)" ;
  skos:inScheme <http://anzsoil.org/def/au/scma> ;
  skos:notation "14H1" ;
  skos:prefLabel "Soluble bases of SE (Ca, Mg, K, Na)" ;
  skos:topConceptOf <http://anzsoil.org/def/au/scma> ;
.
<http://anzsoil.org/def/au/scma/15>
  a skos:Collection ;
  dcterms:description "Ion-exchange properties" ;
  dcterms:identifier "http://anzsoil.org/def/au/scma/15"^^xsd:anyURI ;
  dcterms:source "URN:ISBN:978-0-643-10218-7" ;
  ui:topMemberOf <http://anzsoil.org/def/au/scma> ;
  rdfs:label "Ion-exchange properties" ;
  skos:definition "Ion-exchange properties" ;
  skos:inScheme <http://anzsoil.org/def/au/scma> ;
  skos:member <http://anzsoil.org/def/au/scma/15A1> ;
  skos:member <http://anzsoil.org/def/au/scma/15A2> ;
  skos:member <http://anzsoil.org/def/au/scma/15A3> ;
  skos:member <http://anzsoil.org/def/au/scma/15B1> ;
  skos:member <http://anzsoil.org/def/au/scma/15B2> ;
  skos:member <http://anzsoil.org/def/au/scma/15B3> ;
  skos:member <http://anzsoil.org/def/au/scma/15C1> ;
  skos:member <http://anzsoil.org/def/au/scma/15C2> ;
  skos:member <http://anzsoil.org/def/au/scma/15D1> ;
  skos:member <http://anzsoil.org/def/au/scma/15D2> ;
  skos:member <http://anzsoil.org/def/au/scma/15D3> ;
  skos:member <http://anzsoil.org/def/au/scma/15E1> ;
  skos:member <http://anzsoil.org/def/au/scma/15E2> ;
  skos:member <http://anzsoil.org/def/au/scma/15E3> ;
  skos:member <http://anzsoil.org/def/au/scma/15F1> ;
  skos:member <http://anzsoil.org/def/au/scma/15F2> ;
  skos:member <http://anzsoil.org/def/au/scma/15F3> ;
  skos:member <http://anzsoil.org/def/au/scma/15G1> ;
  skos:member <http://anzsoil.org/def/au/scma/15H1> ;
  skos:member <http://anzsoil.org/def/au/scma/15I1> ;
  skos:member <http://anzsoil.org/def/au/scma/15I2> ;
  skos:member <http://anzsoil.org/def/au/scma/15I3> ;
  skos:member <http://anzsoil.org/def/au/scma/15I4> ;
  skos:member <http://anzsoil.org/def/au/scma/15J1> ;
  skos:member <http://anzsoil.org/def/au/scma/15K1> ;
  skos:member <http://anzsoil.org/def/au/scma/15L1> ;
  skos:member <http://anzsoil.org/def/au/scma/15M1> ;
  skos:member <http://anzsoil.org/def/au/scma/15N1> ;
  skos:member <http://anzsoil.org/def/au/scma/15O1> ;
  skos:notation "15" ;
  skos:prefLabel "Ion-exchange properties" ;
.
<http://anzsoil.org/def/au/scma/15A1>
  a skos:Concept ;
  a sosa:Procedure ;
  dcterms:description "Exchangeable bases (Ca2+, Mg2+, Na+, K+) - 1 M ammonium chloride at pH 7.0, no pre-treatment for soluble salts" ;
  dcterms:identifier "http://anzsoil.org/def/au/scma/15A1"^^xsd:anyURI ;
  dcterms:source "URN:ISBN:978-0-643-10218-7" ;
  rdfs:label "Exchangeable bases (Ca2+, Mg2+, Na+, K+) - 1 M ammonium chloride at pH 7.0, no pre-treatment for soluble salts" ;
  skos:definition "Exchangeable bases (Ca2+, Mg2+, Na+, K+) - 1 M ammonium chloride at pH 7.0, no pre-treatment for soluble salts" ;
  skos:inScheme <http://anzsoil.org/def/au/scma> ;
  skos:notation "15A1" ;
  skos:prefLabel "Exchangeable bases (Ca2+, Mg2+, Na+, K+) - 1 M ammonium chloride at pH 7.0, no pre-treatment for soluble salts" ;
  skos:topConceptOf <http://anzsoil.org/def/au/scma> ;
.
<http://anzsoil.org/def/au/scma/15A2>
  a skos:Concept ;
  a sosa:Procedure ;
  dcterms:description "Exchangeable bases by 1 M ammonium chloride at pH 7.0, pre-treatment for soluble salts" ;
  dcterms:identifier "http://anzsoil.org/def/au/scma/15A2"^^xsd:anyURI ;
  dcterms:source "URN:ISBN:978-0-643-10218-7" ;
  rdfs:label "Exchangeable bases by 1 M ammonium chloride at pH 7.0, pre-treatment for soluble salts" ;
  skos:definition "Exchangeable bases by 1 M ammonium chloride at pH 7.0, pre-treatment for soluble salts" ;
  skos:inScheme <http://anzsoil.org/def/au/scma> ;
  skos:notation "15A2" ;
  skos:prefLabel "Exchangeable bases by 1 M ammonium chloride at pH 7.0, pre-treatment for soluble salts" ;
  skos:topConceptOf <http://anzsoil.org/def/au/scma> ;
.
<http://anzsoil.org/def/au/scma/15A3>
  a skos:Concept ;
  a sosa:Procedure ;
  dcterms:description "Exchangeable bases - 1 M ammonium chloride at pH 7.0, adjusted for soluble Na+" ;
  dcterms:identifier "http://anzsoil.org/def/au/scma/15A3"^^xsd:anyURI ;
  dcterms:source "URN:ISBN:978-0-643-10218-7" ;
  rdfs:label "Exchangeable bases - 1 M ammonium chloride at pH 7.0, adjusted for soluble Na+" ;
  skos:definition "Exchangeable bases - 1 M ammonium chloride at pH 7.0, adjusted for soluble Na+" ;
  skos:inScheme <http://anzsoil.org/def/au/scma> ;
  skos:notation "15A3" ;
  skos:prefLabel "Exchangeable bases - 1 M ammonium chloride at pH 7.0, adjusted for soluble Na+" ;
  skos:topConceptOf <http://anzsoil.org/def/au/scma> ;
.
<http://anzsoil.org/def/au/scma/15B1>
  a skos:Concept ;
  a sosa:Procedure ;
  dcterms:description "Exchangeable bases and cation exchange capacity - 1 M ammonium chloride at pH 7.0, no pre-treatment for soluble salts" ;
  dcterms:identifier "http://anzsoil.org/def/au/scma/15B1"^^xsd:anyURI ;
  dcterms:source "URN:ISBN:978-0-643-10218-7" ;
  rdfs:label "Exchangeable bases and cation exchange capacity - 1 M ammonium chloride at pH 7.0, no pre-treatment for soluble salts" ;
  skos:definition "Exchangeable bases and cation exchange capacity - 1 M ammonium chloride at pH 7.0, no pre-treatment for soluble salts" ;
  skos:inScheme <http://anzsoil.org/def/au/scma> ;
  skos:notation "15B1" ;
  skos:prefLabel "Exchangeable bases and cation exchange capacity - 1 M ammonium chloride at pH 7.0, no pre-treatment for soluble salts" ;
  skos:topConceptOf <http://anzsoil.org/def/au/scma> ;
.
<http://anzsoil.org/def/au/scma/15B2>
  a skos:Concept ;
  a sosa:Procedure ;
  dcterms:description "Exchangeable bases and CEC - 1 M ammonium chloride at pH 7.0, pre-treatment for soluble salts" ;
  dcterms:identifier "http://anzsoil.org/def/au/scma/15B2"^^xsd:anyURI ;
  dcterms:source "URN:ISBN:978-0-643-10218-7" ;
  rdfs:label "Exchangeable bases and CEC - 1 M ammonium chloride at pH 7.0, pre-treatment for soluble salts" ;
  skos:definition "Exchangeable bases and CEC - 1 M ammonium chloride at pH 7.0, pre-treatment for soluble salts" ;
  skos:inScheme <http://anzsoil.org/def/au/scma> ;
  skos:notation "15B2" ;
  skos:prefLabel "Exchangeable bases and CEC - 1 M ammonium chloride at pH 7.0, pre-treatment for soluble salts" ;
  skos:topConceptOf <http://anzsoil.org/def/au/scma> ;
.
<http://anzsoil.org/def/au/scma/15B3>
  a skos:Concept ;
  a sosa:Procedure ;
  dcterms:description "Exchangeable bases and CEC - 1 M ammonium chloride at pH 7.0, adjusted for soluble Na+" ;
  dcterms:identifier "http://anzsoil.org/def/au/scma/15B3"^^xsd:anyURI ;
  dcterms:source "URN:ISBN:978-0-643-10218-7" ;
  rdfs:label "Exchangeable bases and CEC - 1 M ammonium chloride at pH 7.0, adjusted for soluble Na+" ;
  skos:definition "Exchangeable bases and CEC - 1 M ammonium chloride at pH 7.0, adjusted for soluble Na+" ;
  skos:inScheme <http://anzsoil.org/def/au/scma> ;
  skos:notation "15B3" ;
  skos:prefLabel "Exchangeable bases and CEC - 1 M ammonium chloride at pH 7.0, adjusted for soluble Na+" ;
  skos:topConceptOf <http://anzsoil.org/def/au/scma> ;
.
<http://anzsoil.org/def/au/scma/15C1>
  a skos:Concept ;
  a sosa:Procedure ;
  dcterms:description "Exchangeable bases and CEC - alcoholic 1 M ammonium chloride at pH 8.5, pre-treatment for soluble salts" ;
  dcterms:identifier "http://anzsoil.org/def/au/scma/15C1"^^xsd:anyURI ;
  dcterms:source "URN:ISBN:978-0-643-10218-7" ;
  rdfs:label "Exchangeable bases and CEC - alcoholic 1 M ammonium chloride at pH 8.5, pre-treatment for soluble salts" ;
  skos:definition "Exchangeable bases and CEC - alcoholic 1 M ammonium chloride at pH 8.5, pre-treatment for soluble salts" ;
  skos:inScheme <http://anzsoil.org/def/au/scma> ;
  skos:notation "15C1" ;
  skos:prefLabel "Exchangeable bases and CEC - alcoholic 1 M ammonium chloride at pH 8.5, pre-treatment for soluble salts" ;
  skos:topConceptOf <http://anzsoil.org/def/au/scma> ;
.
<http://anzsoil.org/def/au/scma/15C2>
  a skos:Concept ;
  a sosa:Procedure ;
  dcterms:description "Exchangeable divalent cations and CEC - by MIR diffuse reflectance spectroscopy" ;
  dcterms:identifier "http://anzsoil.org/def/au/scma/15C2"^^xsd:anyURI ;
  dcterms:source "URN:ISBN:978-0-643-10218-7" ;
  rdfs:label "Exchangeable divalent cations and CEC - by MIR diffuse reflectance spectroscopy" ;
  skos:definition "Exchangeable divalent cations and CEC - by MIR diffuse reflectance spectroscopy" ;
  skos:inScheme <http://anzsoil.org/def/au/scma> ;
  skos:notation "15C2" ;
  skos:prefLabel "Exchangeable divalent cations and CEC - by MIR diffuse reflectance spectroscopy" ;
  skos:topConceptOf <http://anzsoil.org/def/au/scma> ;
.
<http://anzsoil.org/def/au/scma/15D1>
  a skos:Concept ;
  a sosa:Procedure ;
  dcterms:description "Exchangeable bases and CEC - 1 M ammonium acetate at pH 7.0, pre-treatment for soluble salts, manual leach" ;
  dcterms:identifier "http://anzsoil.org/def/au/scma/15D1"^^xsd:anyURI ;
  dcterms:source "URN:ISBN:978-0-643-10218-7" ;
  rdfs:label "Exchangeable bases and CEC - 1 M ammonium acetate at pH 7.0, pre-treatment for soluble salts, manual leach" ;
  skos:definition "Exchangeable bases and CEC - 1 M ammonium acetate at pH 7.0, pre-treatment for soluble salts, manual leach" ;
  skos:inScheme <http://anzsoil.org/def/au/scma> ;
  skos:notation "15D1" ;
  skos:prefLabel "Exchangeable bases and CEC - 1 M ammonium acetate at pH 7.0, pre-treatment for soluble salts, manual leach" ;
  skos:topConceptOf <http://anzsoil.org/def/au/scma> ;
.
<http://anzsoil.org/def/au/scma/15D2>
  a skos:Concept ;
  a sosa:Procedure ;
  dcterms:description "Exchangeable bases and CEC - 1 M ammonium acetate at pH 7.0, pre-treatment for soluble salts, automatic extractor" ;
  dcterms:identifier "http://anzsoil.org/def/au/scma/15D2"^^xsd:anyURI ;
  dcterms:source "URN:ISBN:978-0-643-10218-7" ;
  rdfs:label "Exchangeable bases and CEC - 1 M ammonium acetate at pH 7.0, pre-treatment for soluble salts, automatic extractor" ;
  skos:definition "Exchangeable bases and CEC - 1 M ammonium acetate at pH 7.0, pre-treatment for soluble salts, automatic extractor" ;
  skos:inScheme <http://anzsoil.org/def/au/scma> ;
  skos:notation "15D2" ;
  skos:prefLabel "Exchangeable bases and CEC - 1 M ammonium acetate at pH 7.0, pre-treatment for soluble salts, automatic extractor" ;
  skos:topConceptOf <http://anzsoil.org/def/au/scma> ;
.
<http://anzsoil.org/def/au/scma/15D3>
  a skos:Concept ;
  a sosa:Procedure ;
  dcterms:description "Exchangeable bases and CEC - 1 M ammonium acetate at pH 7.0, rapid method with no pre-treatment for soluble salts" ;
  dcterms:identifier "http://anzsoil.org/def/au/scma/15D3"^^xsd:anyURI ;
  dcterms:source "URN:ISBN:978-0-643-10218-7" ;
  rdfs:label "Exchangeable bases and CEC - 1 M ammonium acetate at pH 7.0, rapid method with no pre-treatment for soluble salts" ;
  skos:definition "Exchangeable bases and CEC - 1 M ammonium acetate at pH 7.0, rapid method with no pre-treatment for soluble salts" ;
  skos:inScheme <http://anzsoil.org/def/au/scma> ;
  skos:notation "15D3" ;
  skos:prefLabel "Exchangeable bases and CEC - 1 M ammonium acetate at pH 7.0, rapid method with no pre-treatment for soluble salts" ;
  skos:topConceptOf <http://anzsoil.org/def/au/scma> ;
.
<http://anzsoil.org/def/au/scma/15E1>
  a skos:Concept ;
  a sosa:Procedure ;
  dcterms:description "Exchangeable bases, CEC and anion exchange capacity by compulsive exchange, no pre-treatment for soluble salts" ;
  dcterms:identifier "http://anzsoil.org/def/au/scma/15E1"^^xsd:anyURI ;
  dcterms:source "URN:ISBN:978-0-643-10218-7" ;
  rdfs:label "Exchangeable bases, CEC and anion exchange capacity by compulsive exchange, no pre-treatment for soluble salts" ;
  skos:definition "Exchangeable bases, CEC and anion exchange capacity by compulsive exchange, no pre-treatment for soluble salts" ;
  skos:inScheme <http://anzsoil.org/def/au/scma> ;
  skos:notation "15E1" ;
  skos:prefLabel "Exchangeable bases, CEC and anion exchange capacity by compulsive exchange, no pre-treatment for soluble salts" ;
  skos:topConceptOf <http://anzsoil.org/def/au/scma> ;
.
<http://anzsoil.org/def/au/scma/15E2>
  a skos:Concept ;
  a sosa:Procedure ;
  dcterms:description "Exchangeable bases, CEC and AEC by compulsive exchange, pre-treatment for soluble salts" ;
  dcterms:identifier "http://anzsoil.org/def/au/scma/15E2"^^xsd:anyURI ;
  dcterms:source "URN:ISBN:978-0-643-10218-7" ;
  rdfs:label "Exchangeable bases, CEC and AEC by compulsive exchange, pre-treatment for soluble salts" ;
  skos:definition "Exchangeable bases, CEC and AEC by compulsive exchange, pre-treatment for soluble salts" ;
  skos:inScheme <http://anzsoil.org/def/au/scma> ;
  skos:notation "15E2" ;
  skos:prefLabel "Exchangeable bases, CEC and AEC by compulsive exchange, pre-treatment for soluble salts" ;
  skos:topConceptOf <http://anzsoil.org/def/au/scma> ;
.
<http://anzsoil.org/def/au/scma/15E3>
  a skos:Concept ;
  a sosa:Procedure ;
  dcterms:description "Exchangeable bases, CEC and AEC by compulsive exchange, adjusted for soluble Na+" ;
  dcterms:identifier "http://anzsoil.org/def/au/scma/15E3"^^xsd:anyURI ;
  dcterms:source "URN:ISBN:978-0-643-10218-7" ;
  rdfs:label "Exchangeable bases, CEC and AEC by compulsive exchange, adjusted for soluble Na+" ;
  skos:definition "Exchangeable bases, CEC and AEC by compulsive exchange, adjusted for soluble Na+" ;
  skos:inScheme <http://anzsoil.org/def/au/scma> ;
  skos:notation "15E3" ;
  skos:prefLabel "Exchangeable bases, CEC and AEC by compulsive exchange, adjusted for soluble Na+" ;
  skos:topConceptOf <http://anzsoil.org/def/au/scma> ;
.
<http://anzsoil.org/def/au/scma/15F1>
  a skos:Concept ;
  a sosa:Procedure ;
  dcterms:description "Exchangeable bases by 0.01 M silver-thiourea (AgTU+) - no pre-treatment for soluble salts" ;
  dcterms:identifier "http://anzsoil.org/def/au/scma/15F1"^^xsd:anyURI ;
  dcterms:source "URN:ISBN:978-0-643-10218-7" ;
  rdfs:label "Exchangeable bases by 0.01 M silver-thiourea (AgTU+) - no pre-treatment for soluble salts" ;
  skos:definition "Exchangeable bases by 0.01 M silver-thiourea (AgTU+) - no pre-treatment for soluble salts" ;
  skos:inScheme <http://anzsoil.org/def/au/scma> ;
  skos:notation "15F1" ;
  skos:prefLabel "Exchangeable bases by 0.01 M silver-thiourea (AgTU+) - no pre-treatment for soluble salts" ;
  skos:topConceptOf <http://anzsoil.org/def/au/scma> ;
.
<http://anzsoil.org/def/au/scma/15F2>
  a skos:Concept ;
  a sosa:Procedure ;
  dcterms:description "Exchangeable aluminium by 0.01 M AgTU+" ;
  dcterms:identifier "http://anzsoil.org/def/au/scma/15F2"^^xsd:anyURI ;
  dcterms:source "URN:ISBN:978-0-643-10218-7" ;
  rdfs:label "Exchangeable aluminium by 0.01 M AgTU+" ;
  skos:definition "Exchangeable aluminium by 0.01 M AgTU+" ;
  skos:inScheme <http://anzsoil.org/def/au/scma> ;
  skos:notation "15F2" ;
  skos:prefLabel "Exchangeable aluminium by 0.01 M AgTU+" ;
  skos:topConceptOf <http://anzsoil.org/def/au/scma> ;
.
<http://anzsoil.org/def/au/scma/15F3>
  a skos:Concept ;
  a sosa:Procedure ;
  dcterms:description "Cation exchange capacity by 0.01 M AgTU+ [CEC AgTU]" ;
  dcterms:identifier "http://anzsoil.org/def/au/scma/15F3"^^xsd:anyURI ;
  dcterms:source "URN:ISBN:978-0-643-10218-7" ;
  rdfs:label "Cation exchange capacity by 0.01 M AgTU+ [CEC AgTU]" ;
  skos:definition "Cation exchange capacity by 0.01 M AgTU+ [CEC AgTU]" ;
  skos:inScheme <http://anzsoil.org/def/au/scma> ;
  skos:notation "15F3" ;
  skos:prefLabel "Cation exchange capacity by 0.01 M AgTU+ [CEC AgTU]" ;
  skos:topConceptOf <http://anzsoil.org/def/au/scma> ;
.
<http://anzsoil.org/def/au/scma/15G1>
  a skos:Concept ;
  a sosa:Procedure ;
  dcterms:description "Exchange acidity (H+ + Al3+) by 1 M potassium chloride" ;
  dcterms:identifier "http://anzsoil.org/def/au/scma/15G1"^^xsd:anyURI ;
  dcterms:source "URN:ISBN:978-0-643-10218-7" ;
  rdfs:label "Exchange acidity (H+ + Al3+) by 1 M potassium chloride" ;
  skos:definition "Exchange acidity (H+ + Al3+) by 1 M potassium chloride" ;
  skos:inScheme <http://anzsoil.org/def/au/scma> ;
  skos:notation "15G1" ;
  skos:prefLabel "Exchange acidity (H+ + Al3+) by 1 M potassium chloride" ;
  skos:topConceptOf <http://anzsoil.org/def/au/scma> ;
.
<http://anzsoil.org/def/au/scma/15H1>
  a skos:Concept ;
  a sosa:Procedure ;
  dcterms:description "Exchange acidity by triethanolamine (TEA)" ;
  dcterms:identifier "http://anzsoil.org/def/au/scma/15H1"^^xsd:anyURI ;
  dcterms:source "URN:ISBN:978-0-643-10218-7" ;
  rdfs:label "Exchange acidity by triethanolamine (TEA)" ;
  skos:definition "Exchange acidity by triethanolamine (TEA)" ;
  skos:inScheme <http://anzsoil.org/def/au/scma> ;
  skos:notation "15H1" ;
  skos:prefLabel "Exchange acidity by triethanolamine (TEA)" ;
  skos:topConceptOf <http://anzsoil.org/def/au/scma> ;
.
<http://anzsoil.org/def/au/scma/15I1>
  a skos:Concept ;
  a sosa:Procedure ;
  dcterms:description "Cation exchange capacity measurement - distillation of NH+4" ;
  dcterms:identifier "http://anzsoil.org/def/au/scma/15I1"^^xsd:anyURI ;
  dcterms:source "URN:ISBN:978-0-643-10218-7" ;
  rdfs:label "Cation exchange capacity measurement - distillation of NH+4" ;
  skos:definition "Cation exchange capacity measurement - distillation of NH+4" ;
  skos:inScheme <http://anzsoil.org/def/au/scma> ;
  skos:notation "15I1" ;
  skos:prefLabel "Cation exchange capacity measurement - distillation of NH+4" ;
  skos:topConceptOf <http://anzsoil.org/def/au/scma> ;
.
<http://anzsoil.org/def/au/scma/15I2>
  a skos:Concept ;
  a sosa:Procedure ;
  dcterms:description "Cation exchange capacity measurement - automated determination of NH+4" ;
  dcterms:identifier "http://anzsoil.org/def/au/scma/15I2"^^xsd:anyURI ;
  dcterms:source "URN:ISBN:978-0-643-10218-7" ;
  rdfs:label "Cation exchange capacity measurement - automated determination of NH+4" ;
  skos:definition "Cation exchange capacity measurement - automated determination of NH+4" ;
  skos:inScheme <http://anzsoil.org/def/au/scma> ;
  skos:notation "15I2" ;
  skos:prefLabel "Cation exchange capacity measurement - automated determination of NH+4" ;
  skos:topConceptOf <http://anzsoil.org/def/au/scma> ;
.
<http://anzsoil.org/def/au/scma/15I3>
  a skos:Concept ;
  a sosa:Procedure ;
  dcterms:description "Cation exchange capacity measurement - automated determination of NH+4 and Cl+" ;
  dcterms:identifier "http://anzsoil.org/def/au/scma/15I3"^^xsd:anyURI ;
  dcterms:source "URN:ISBN:978-0-643-10218-7" ;
  rdfs:label "Cation exchange capacity measurement - automated determination of NH+4 and Cl+" ;
  skos:definition "Cation exchange capacity measurement - automated determination of NH+4 and Cl+" ;
  skos:inScheme <http://anzsoil.org/def/au/scma> ;
  skos:notation "15I3" ;
  skos:prefLabel "Cation exchange capacity measurement - automated determination of NH+4 and Cl+" ;
  skos:topConceptOf <http://anzsoil.org/def/au/scma> ;
.
<http://anzsoil.org/def/au/scma/15I4>
  a skos:Concept ;
  a sosa:Procedure ;
  dcterms:description "Cation exchange capacity measurement - titration of NH+4 and Cl-" ;
  dcterms:identifier "http://anzsoil.org/def/au/scma/15I4"^^xsd:anyURI ;
  dcterms:source "URN:ISBN:978-0-643-10218-7" ;
  rdfs:label "Cation exchange capacity measurement - titration of NH+4 and Cl-" ;
  skos:definition "Cation exchange capacity measurement - titration of NH+4 and Cl-" ;
  skos:inScheme <http://anzsoil.org/def/au/scma> ;
  skos:notation "15I4" ;
  skos:prefLabel "Cation exchange capacity measurement - titration of NH+4 and Cl-" ;
  skos:topConceptOf <http://anzsoil.org/def/au/scma> ;
.
<http://anzsoil.org/def/au/scma/15J1>
  a skos:Concept ;
  a sosa:Procedure ;
  dcterms:description "Effective cation exchange capacity (ECEC)" ;
  dcterms:identifier "http://anzsoil.org/def/au/scma/15J1"^^xsd:anyURI ;
  dcterms:source "URN:ISBN:978-0-643-10218-7" ;
  rdfs:label "Effective cation exchange capacity (ECEC)" ;
  skos:definition "Effective cation exchange capacity (ECEC)" ;
  skos:inScheme <http://anzsoil.org/def/au/scma> ;
  skos:notation "15J1" ;
  skos:prefLabel "Effective cation exchange capacity (ECEC)" ;
  skos:topConceptOf <http://anzsoil.org/def/au/scma> ;
.
<http://anzsoil.org/def/au/scma/15K1>
  a skos:Concept ;
  a sosa:Procedure ;
  dcterms:description "Cation exchange capacity - pH 8.2 (CEC pH 8.2)" ;
  dcterms:identifier "http://anzsoil.org/def/au/scma/15K1"^^xsd:anyURI ;
  dcterms:source "URN:ISBN:978-0-643-10218-7" ;
  rdfs:label "Cation exchange capacity - pH 8.2 (CEC pH 8.2)" ;
  skos:definition "Cation exchange capacity - pH 8.2 (CEC pH 8.2)" ;
  skos:inScheme <http://anzsoil.org/def/au/scma> ;
  skos:notation "15K1" ;
  skos:prefLabel "Cation exchange capacity - pH 8.2 (CEC pH 8.2)" ;
  skos:topConceptOf <http://anzsoil.org/def/au/scma> ;
.
<http://anzsoil.org/def/au/scma/15L1>
  a skos:Concept ;
  a sosa:Procedure ;
  dcterms:description "Base saturation percentage (ESP)" ;
  dcterms:identifier "http://anzsoil.org/def/au/scma/15L1"^^xsd:anyURI ;
  dcterms:source "URN:ISBN:978-0-643-10218-7" ;
  rdfs:label "Base saturation percentage (ESP)" ;
  skos:definition "Base saturation percentage (ESP)" ;
  skos:inScheme <http://anzsoil.org/def/au/scma> ;
  skos:notation "15L1" ;
  skos:prefLabel "Base saturation percentage (ESP)" ;
  skos:topConceptOf <http://anzsoil.org/def/au/scma> ;
.
<http://anzsoil.org/def/au/scma/15M1>
  a skos:Concept ;
  a sosa:Procedure ;
  dcterms:description "Basic cation saturation ratios" ;
  dcterms:identifier "http://anzsoil.org/def/au/scma/15M1"^^xsd:anyURI ;
  dcterms:source "URN:ISBN:978-0-643-10218-7" ;
  rdfs:label "Basic cation saturation ratios" ;
  skos:definition "Basic cation saturation ratios" ;
  skos:inScheme <http://anzsoil.org/def/au/scma> ;
  skos:notation "15M1" ;
  skos:prefLabel "Basic cation saturation ratios" ;
  skos:topConceptOf <http://anzsoil.org/def/au/scma> ;
.
<http://anzsoil.org/def/au/scma/15N1>
  a skos:Concept ;
  a sosa:Procedure ;
  dcterms:description "Exchangeable Na+ percentage (ESP)" ;
  dcterms:identifier "http://anzsoil.org/def/au/scma/15N1"^^xsd:anyURI ;
  dcterms:source "URN:ISBN:978-0-643-10218-7" ;
  rdfs:label "Exchangeable Na+ percentage (ESP)" ;
  skos:definition "Exchangeable Na+ percentage (ESP)" ;
  skos:inScheme <http://anzsoil.org/def/au/scma> ;
  skos:notation "15N1" ;
  skos:prefLabel "Exchangeable Na+ percentage (ESP)" ;
  skos:topConceptOf <http://anzsoil.org/def/au/scma> ;
.
<http://anzsoil.org/def/au/scma/15O1>
  a skos:Concept ;
  a sosa:Procedure ;
  dcterms:description "Percent Al saturation" ;
  dcterms:identifier "http://anzsoil.org/def/au/scma/15O1"^^xsd:anyURI ;
  dcterms:source "URN:ISBN:978-0-643-10218-7" ;
  rdfs:label "Percent Al saturation" ;
  skos:definition "Percent Al saturation" ;
  skos:inScheme <http://anzsoil.org/def/au/scma> ;
  skos:notation "15O1" ;
  skos:prefLabel "Percent Al saturation" ;
  skos:topConceptOf <http://anzsoil.org/def/au/scma> ;
.
<http://anzsoil.org/def/au/scma/16>
  a skos:Collection ;
  dcterms:description "Lime requirement" ;
  dcterms:identifier "http://anzsoil.org/def/au/scma/16"^^xsd:anyURI ;
  dcterms:source "URN:ISBN:978-0-643-10218-7" ;
  ui:topMemberOf <http://anzsoil.org/def/au/scma> ;
  rdfs:label "Lime requirement" ;
  skos:definition "Lime requirement" ;
  skos:inScheme <http://anzsoil.org/def/au/scma> ;
  skos:member <http://anzsoil.org/def/au/scma/16A1> ;
  skos:member <http://anzsoil.org/def/au/scma/16B1> ;
  skos:member <http://anzsoil.org/def/au/scma/16C1> ;
  skos:member <http://anzsoil.org/def/au/scma/16D1> ;
  skos:notation "16" ;
  skos:prefLabel "Lime requirement" ;
.
<http://anzsoil.org/def/au/scma/16A1>
  a skos:Concept ;
  a sosa:Procedure ;
  dcterms:description "Calculated lime rate - from exchangeable Al3+" ;
  dcterms:identifier "http://anzsoil.org/def/au/scma/16A1"^^xsd:anyURI ;
  dcterms:source "URN:ISBN:978-0-643-10218-7" ;
  rdfs:label "Calculated lime rate - from exchangeable Al3+" ;
  skos:definition "Calculated lime rate - from exchangeable Al3+" ;
  skos:inScheme <http://anzsoil.org/def/au/scma> ;
  skos:notation "16A1" ;
  skos:prefLabel "Calculated lime rate - from exchangeable Al3+" ;
  skos:topConceptOf <http://anzsoil.org/def/au/scma> ;
.
<http://anzsoil.org/def/au/scma/16B1>
  a skos:Concept ;
  a sosa:Procedure ;
  dcterms:description "Calculated lime rate - Cregan" ;
  dcterms:identifier "http://anzsoil.org/def/au/scma/16B1"^^xsd:anyURI ;
  dcterms:source "URN:ISBN:978-0-643-10218-7" ;
  rdfs:label "Calculated lime rate - Cregan" ;
  skos:definition "Calculated lime rate - Cregan" ;
  skos:inScheme <http://anzsoil.org/def/au/scma> ;
  skos:notation "16B1" ;
  skos:prefLabel "Calculated lime rate - Cregan" ;
  skos:topConceptOf <http://anzsoil.org/def/au/scma> ;
.
<http://anzsoil.org/def/au/scma/16C1>
  a skos:Concept ;
  a sosa:Procedure ;
  dcterms:description "Lime requirement - Mehlich single buffer" ;
  dcterms:identifier "http://anzsoil.org/def/au/scma/16C1"^^xsd:anyURI ;
  dcterms:source "URN:ISBN:978-0-643-10218-7" ;
  rdfs:label "Lime requirement - Mehlich single buffer" ;
  skos:definition "Lime requirement - Mehlich single buffer" ;
  skos:inScheme <http://anzsoil.org/def/au/scma> ;
  skos:notation "16C1" ;
  skos:prefLabel "Lime requirement - Mehlich single buffer" ;
  skos:topConceptOf <http://anzsoil.org/def/au/scma> ;
.
<http://anzsoil.org/def/au/scma/16D1>
  a skos:Concept ;
  a sosa:Procedure ;
  dcterms:description "Lime requirement - Dunn titration curves" ;
  dcterms:identifier "http://anzsoil.org/def/au/scma/16D1"^^xsd:anyURI ;
  dcterms:source "URN:ISBN:978-0-643-10218-7" ;
  rdfs:label "Lime requirement - Dunn titration curves" ;
  skos:definition "Lime requirement - Dunn titration curves" ;
  skos:inScheme <http://anzsoil.org/def/au/scma> ;
  skos:notation "16D1" ;
  skos:prefLabel "Lime requirement - Dunn titration curves" ;
  skos:topConceptOf <http://anzsoil.org/def/au/scma> ;
.
<http://anzsoil.org/def/au/scma/17>
  a skos:Collection ;
  dcterms:description "Total miscellaneous elements" ;
  dcterms:identifier "http://anzsoil.org/def/au/scma/17"^^xsd:anyURI ;
  dcterms:source "URN:ISBN:978-0-643-10218-7" ;
  ui:topMemberOf <http://anzsoil.org/def/au/scma> ;
  rdfs:label "Total miscellaneous elements" ;
  skos:definition "Total miscellaneous elements" ;
  skos:inScheme <http://anzsoil.org/def/au/scma> ;
  skos:member <http://anzsoil.org/def/au/scma/17A1> ;
  skos:member <http://anzsoil.org/def/au/scma/17A2> ;
  skos:member <http://anzsoil.org/def/au/scma/17B1> ;
  skos:member <http://anzsoil.org/def/au/scma/17B2> ;
  skos:member <http://anzsoil.org/def/au/scma/17C1> ;
  skos:notation "17" ;
  skos:prefLabel "Total miscellaneous elements" ;
.
<http://anzsoil.org/def/au/scma/17A1>
  a skos:Concept ;
  a sosa:Procedure ;
  dcterms:description "Total elemental analysis of soils and sediments -X-ray fluorescence spectroscopy" ;
  dcterms:identifier "http://anzsoil.org/def/au/scma/17A1"^^xsd:anyURI ;
  dcterms:source "URN:ISBN:978-0-643-10218-7" ;
  rdfs:label "Total elemental analysis of soils and sediments -X-ray fluorescence spectroscopy" ;
  skos:definition "Total elemental analysis of soils and sediments -X-ray fluorescence spectroscopy" ;
  skos:inScheme <http://anzsoil.org/def/au/scma> ;
  skos:notation "17A1" ;
  skos:prefLabel "Total elemental analysis of soils and sediments -X-ray fluorescence spectroscopy" ;
  skos:topConceptOf <http://anzsoil.org/def/au/scma> ;
.
<http://anzsoil.org/def/au/scma/17A2>
  a skos:Concept ;
  a sosa:Procedure ;
  dcterms:description "Total elemental analysis of soils and sediments - microwave assisted digestion, with determination by atomic spectroscopy" ;
  dcterms:identifier "http://anzsoil.org/def/au/scma/17A2"^^xsd:anyURI ;
  dcterms:source "URN:ISBN:978-0-643-10218-7" ;
  rdfs:label "Total elemental analysis of soils and sediments - microwave assisted digestion, with determination by atomic spectroscopy" ;
  skos:definition "Total elemental analysis of soils and sediments - microwave assisted digestion, with determination by atomic spectroscopy" ;
  skos:inScheme <http://anzsoil.org/def/au/scma> ;
  skos:notation "17A2" ;
  skos:prefLabel "Total elemental analysis of soils and sediments - microwave assisted digestion, with determination by atomic spectroscopy" ;
  skos:topConceptOf <http://anzsoil.org/def/au/scma> ;
.
<http://anzsoil.org/def/au/scma/17B1>
  a skos:Concept ;
  a sosa:Procedure ;
  dcterms:description "Pseudo-total elemental analysis of soils and sediments - reverse aqua regia block digestion with determination by atomic spectroscopy" ;
  dcterms:identifier "http://anzsoil.org/def/au/scma/17B1"^^xsd:anyURI ;
  dcterms:source "URN:ISBN:978-0-643-10218-7" ;
  rdfs:label "Pseudo-total elemental analysis of soils and sediments - reverse aqua regia block digestion with determination by atomic spectroscopy" ;
  skos:definition "Pseudo-total elemental analysis of soils and sediments - reverse aqua regia block digestion with determination by atomic spectroscopy" ;
  skos:inScheme <http://anzsoil.org/def/au/scma> ;
  skos:notation "17B1" ;
  skos:prefLabel "Pseudo-total elemental analysis of soils and sediments - reverse aqua regia block digestion with determination by atomic spectroscopy" ;
  skos:topConceptOf <http://anzsoil.org/def/au/scma> ;
.
<http://anzsoil.org/def/au/scma/17B2>
  a skos:Concept ;
  a sosa:Procedure ;
  dcterms:description "Pseudo-total elements of soils and sediments - reverse aqua regia microwave assisted digestion of sludges, soils and sediments, with determination by atomic spectroscopy" ;
  dcterms:identifier "http://anzsoil.org/def/au/scma/17B2"^^xsd:anyURI ;
  dcterms:source "URN:ISBN:978-0-643-10218-7" ;
  rdfs:label "Pseudo-total elements of soils and sediments - reverse aqua regia microwave assisted digestion of sludges, soils and sediments, with determination by atomic spectroscopy" ;
  skos:definition "Pseudo-total elements of soils and sediments - reverse aqua regia microwave assisted digestion of sludges, soils and sediments, with determination by atomic spectroscopy" ;
  skos:inScheme <http://anzsoil.org/def/au/scma> ;
  skos:notation "17B2" ;
  skos:prefLabel "Pseudo-total elements of soils and sediments - reverse aqua regia microwave assisted digestion of sludges, soils and sediments, with determination by atomic spectroscopy" ;
  skos:topConceptOf <http://anzsoil.org/def/au/scma> ;
.
<http://anzsoil.org/def/au/scma/17C1>
  a skos:Concept ;
  a sosa:Procedure ;
  dcterms:description "Pseudo-total elements of soils and sediments - conventional aqua regia block digestion and determination by atomic spectroscopy" ;
  dcterms:identifier "http://anzsoil.org/def/au/scma/17C1"^^xsd:anyURI ;
  dcterms:source "URN:ISBN:978-0-643-10218-7" ;
  rdfs:label "Pseudo-total elements of soils and sediments - conventional aqua regia block digestion and determination by atomic spectroscopy" ;
  skos:definition "Pseudo-total elements of soils and sediments - conventional aqua regia block digestion and determination by atomic spectroscopy" ;
  skos:inScheme <http://anzsoil.org/def/au/scma> ;
  skos:notation "17C1" ;
  skos:prefLabel "Pseudo-total elements of soils and sediments - conventional aqua regia block digestion and determination by atomic spectroscopy" ;
  skos:topConceptOf <http://anzsoil.org/def/au/scma> ;
.
<http://anzsoil.org/def/au/scma/18>
  a skos:Collection ;
  dcterms:description "Miscellaneous extractable elements" ;
  dcterms:identifier "http://anzsoil.org/def/au/scma/18"^^xsd:anyURI ;
  dcterms:source "URN:ISBN:978-0-643-10218-7" ;
  ui:topMemberOf <http://anzsoil.org/def/au/scma> ;
  rdfs:label "Miscellaneous extractable elements" ;
  skos:definition "Miscellaneous extractable elements" ;
  skos:inScheme <http://anzsoil.org/def/au/scma> ;
  skos:member <http://anzsoil.org/def/au/scma/18A1> ;
  skos:member <http://anzsoil.org/def/au/scma/18B1> ;
  skos:member <http://anzsoil.org/def/au/scma/18C1> ;
  skos:member <http://anzsoil.org/def/au/scma/18D1> ;
  skos:member <http://anzsoil.org/def/au/scma/18E1> ;
  skos:member <http://anzsoil.org/def/au/scma/18F> ;
  skos:member <http://anzsoil.org/def/au/scma/18F1> ;
  skos:member <http://anzsoil.org/def/au/scma/18F2> ;
  skos:member <http://anzsoil.org/def/au/scma/18G1> ;
  skos:notation "18" ;
  skos:prefLabel "Miscellaneous extractable elements" ;
.
<http://anzsoil.org/def/au/scma/18A1>
  a skos:Concept ;
  a sosa:Procedure ;
  dcterms:description "Bicarbonate-extractable K+" ;
  dcterms:identifier "http://anzsoil.org/def/au/scma/18A1"^^xsd:anyURI ;
  dcterms:source "URN:ISBN:978-0-643-10218-7" ;
  rdfs:label "Bicarbonate-extractable K+" ;
  skos:definition "Bicarbonate-extractable K+" ;
  skos:inScheme <http://anzsoil.org/def/au/scma> ;
  skos:notation "18A1" ;
  skos:prefLabel "Bicarbonate-extractable K+" ;
  skos:topConceptOf <http://anzsoil.org/def/au/scma> ;
.
<http://anzsoil.org/def/au/scma/18B1>
  a skos:Concept ;
  a sosa:Procedure ;
  dcterms:description "Hydrochloric acid-extractable K+" ;
  dcterms:identifier "http://anzsoil.org/def/au/scma/18B1"^^xsd:anyURI ;
  dcterms:source "URN:ISBN:978-0-643-10218-7" ;
  rdfs:label "Hydrochloric acid-extractable K+" ;
  skos:definition "Hydrochloric acid-extractable K+" ;
  skos:inScheme <http://anzsoil.org/def/au/scma> ;
  skos:notation "18B1" ;
  skos:prefLabel "Hydrochloric acid-extractable K+" ;
  skos:topConceptOf <http://anzsoil.org/def/au/scma> ;
.
<http://anzsoil.org/def/au/scma/18C1>
  a skos:Concept ;
  a sosa:Procedure ;
  dcterms:description "Boiling 0.1 nitric acid-extractable K+" ;
  dcterms:identifier "http://anzsoil.org/def/au/scma/18C1"^^xsd:anyURI ;
  dcterms:source "URN:ISBN:978-0-643-10218-7" ;
  rdfs:label "Boiling 0.1 nitric acid-extractable K+" ;
  skos:definition "Boiling 0.1 nitric acid-extractable K+" ;
  skos:inScheme <http://anzsoil.org/def/au/scma> ;
  skos:notation "18C1" ;
  skos:prefLabel "Boiling 0.1 nitric acid-extractable K+" ;
  skos:topConceptOf <http://anzsoil.org/def/au/scma> ;
.
<http://anzsoil.org/def/au/scma/18D1>
  a skos:Concept ;
  a sosa:Procedure ;
  dcterms:description "0.1 M calcium chloride-extractable Cd" ;
  dcterms:identifier "http://anzsoil.org/def/au/scma/18D1"^^xsd:anyURI ;
  dcterms:source "URN:ISBN:978-0-643-10218-7" ;
  rdfs:label "0.1 M calcium chloride-extractable Cd" ;
  skos:definition "0.1 M calcium chloride-extractable Cd" ;
  skos:inScheme <http://anzsoil.org/def/au/scma> ;
  skos:notation "18D1" ;
  skos:prefLabel "0.1 M calcium chloride-extractable Cd" ;
  skos:topConceptOf <http://anzsoil.org/def/au/scma> ;
.
<http://anzsoil.org/def/au/scma/18E1>
  a skos:Concept ;
  a sosa:Procedure ;
  dcterms:description "0.01 M calcium chloride-extractable Cd" ;
  dcterms:identifier "http://anzsoil.org/def/au/scma/18E1"^^xsd:anyURI ;
  dcterms:source "URN:ISBN:978-0-643-10218-7" ;
  rdfs:label "0.01 M calcium chloride-extractable Cd" ;
  skos:definition "0.01 M calcium chloride-extractable Cd" ;
  skos:inScheme <http://anzsoil.org/def/au/scma> ;
  skos:notation "18E1" ;
  skos:prefLabel "0.01 M calcium chloride-extractable Cd" ;
  skos:topConceptOf <http://anzsoil.org/def/au/scma> ;
.
<http://anzsoil.org/def/au/scma/18F>
  a skos:Concept ;
  a sosa:Procedure ;
  dcterms:description "Mehlich 3 multi-element tests" ;
  dcterms:identifier "http://anzsoil.org/def/au/scma/18F"^^xsd:anyURI ;
  dcterms:source "URN:ISBN:978-0-643-10218-7" ;
  rdfs:label "Mehlich 3 multi-element tests" ;
  skos:definition "Mehlich 3 multi-element tests" ;
  skos:inScheme <http://anzsoil.org/def/au/scma> ;
  skos:narrower <http://anzsoil.org/def/au/scma/18F1> ;
  skos:narrower <http://anzsoil.org/def/au/scma/18F2> ;
  skos:notation "18F" ;
  skos:prefLabel "Mehlich 3 multi-element tests" ;
  skos:topConceptOf <http://anzsoil.org/def/au/scma> ;
.
<http://anzsoil.org/def/au/scma/18F1>
  a skos:Concept ;
  a sosa:Procedure ;
  dcterms:description "Mehlich 3-extractable elements (P, Ca, Mg, Na, K, Fe, Cu, Mn, Zn, B, S, Al)" ;
  dcterms:identifier "http://anzsoil.org/def/au/scma/18F1"^^xsd:anyURI ;
  dcterms:source "URN:ISBN:978-0-643-10218-7" ;
  rdfs:label "Mehlich 3-extractable elements (P, Ca, Mg, Na, K, Fe, Cu, Mn, Zn, B, S, Al)" ;
  skos:broader <http://anzsoil.org/def/au/scma/18F> ;
  skos:definition "Mehlich 3-extractable elements (P, Ca, Mg, Na, K, Fe, Cu, Mn, Zn, B, S, Al)" ;
  skos:inScheme <http://anzsoil.org/def/au/scma> ;
  skos:notation "18F1" ;
  skos:prefLabel "Mehlich 3-extractable elements (P, Ca, Mg, Na, K, Fe, Cu, Mn, Zn, B, S, Al)" ;
.
<http://anzsoil.org/def/au/scma/18F2>
  a skos:Concept ;
  a sosa:Procedure ;
  dcterms:description "Mehlich 3 Extractable P - colour finish" ;
  dcterms:identifier "http://anzsoil.org/def/au/scma/18F2"^^xsd:anyURI ;
  dcterms:source "URN:ISBN:978-0-643-10218-7" ;
  rdfs:label "Mehlich 3 Extractable P - colour finish" ;
  skos:broader <http://anzsoil.org/def/au/scma/18F> ;
  skos:definition "Mehlich 3 Extractable P - colour finish" ;
  skos:inScheme <http://anzsoil.org/def/au/scma> ;
  skos:notation "18F2" ;
  skos:prefLabel "Mehlich 3 Extractable P - colour finish" ;
.
<http://anzsoil.org/def/au/scma/18G1>
  a skos:Concept ;
  a sosa:Procedure ;
  dcterms:description "Reverse soil K+ by copper-modified sodium tetraphenylboron extraction (TBK 4h)" ;
  dcterms:identifier "http://anzsoil.org/def/au/scma/18G1"^^xsd:anyURI ;
  dcterms:source "URN:ISBN:978-0-643-10218-7" ;
  rdfs:label "Reverse soil K+ by copper-modified sodium tetraphenylboron extraction (TBK 4h)" ;
  skos:definition "Reverse soil K+ by copper-modified sodium tetraphenylboron extraction (TBK 4h)" ;
  skos:inScheme <http://anzsoil.org/def/au/scma> ;
  skos:notation "18G1" ;
  skos:prefLabel "Reverse soil K+ by copper-modified sodium tetraphenylboron extraction (TBK 4h)" ;
  skos:topConceptOf <http://anzsoil.org/def/au/scma> ;
.
<http://anzsoil.org/def/au/scma/19>
  a skos:Collection ;
  dcterms:description "Alkaline earth carbonates" ;
  dcterms:identifier "http://anzsoil.org/def/au/scma/19"^^xsd:anyURI ;
  dcterms:source "URN:ISBN:978-0-643-10218-7" ;
  ui:topMemberOf <http://anzsoil.org/def/au/scma> ;
  rdfs:label "Alkaline earth carbonates" ;
  skos:definition "Alkaline earth carbonates" ;
  skos:inScheme <http://anzsoil.org/def/au/scma> ;
  skos:member <http://anzsoil.org/def/au/scma/19A1> ;
  skos:member <http://anzsoil.org/def/au/scma/19B> ;
  skos:member <http://anzsoil.org/def/au/scma/19B1> ;
  skos:member <http://anzsoil.org/def/au/scma/19B2> ;
  skos:member <http://anzsoil.org/def/au/scma/19C1> ;
  skos:member <http://anzsoil.org/def/au/scma/19D1> ;
  skos:notation "19" ;
  skos:prefLabel "Alkaline earth carbonates" ;
.
<http://anzsoil.org/def/au/scma/19A1>
  a skos:Concept ;
  a sosa:Procedure ;
  dcterms:description "Carbonates -rapid titration" ;
  dcterms:identifier "http://anzsoil.org/def/au/scma/19A1"^^xsd:anyURI ;
  dcterms:source "URN:ISBN:978-0-643-10218-7" ;
  rdfs:label "Carbonates -rapid titration" ;
  skos:definition "Carbonates -rapid titration" ;
  skos:inScheme <http://anzsoil.org/def/au/scma> ;
  skos:notation "19A1" ;
  skos:prefLabel "Carbonates -rapid titration" ;
  skos:topConceptOf <http://anzsoil.org/def/au/scma> ;
.
<http://anzsoil.org/def/au/scma/19B>
  a skos:Concept ;
  a sosa:Procedure ;
  dcterms:description "Carbonates by pressure change" ;
  dcterms:identifier "http://anzsoil.org/def/au/scma/19B"^^xsd:anyURI ;
  dcterms:source "URN:ISBN:978-0-643-10218-7" ;
  rdfs:label "Carbonates by pressure change" ;
  skos:definition "Carbonates by pressure change" ;
  skos:inScheme <http://anzsoil.org/def/au/scma> ;
  skos:narrower <http://anzsoil.org/def/au/scma/19B1> ;
  skos:narrower <http://anzsoil.org/def/au/scma/19B2> ;
  skos:notation "19B" ;
  skos:prefLabel "Carbonates by pressure change" ;
  skos:topConceptOf <http://anzsoil.org/def/au/scma> ;
.
<http://anzsoil.org/def/au/scma/19B1>
  a skos:Concept ;
  a sosa:Procedure ;
  dcterms:description "Carbonates by pressure change - manometric" ;
  dcterms:identifier "http://anzsoil.org/def/au/scma/19B1"^^xsd:anyURI ;
  dcterms:source "URN:ISBN:978-0-643-10218-7" ;
  rdfs:label "Carbonates by pressure change - manometric" ;
  skos:broader <http://anzsoil.org/def/au/scma/19B> ;
  skos:definition "Carbonates by pressure change - manometric" ;
  skos:inScheme <http://anzsoil.org/def/au/scma> ;
  skos:notation "19B1" ;
  skos:prefLabel "Carbonates by pressure change - manometric" ;
.
<http://anzsoil.org/def/au/scma/19B2>
  a skos:Concept ;
  a sosa:Procedure ;
  dcterms:description "Carbonates by pressure change - transducer" ;
  dcterms:identifier "http://anzsoil.org/def/au/scma/19B2"^^xsd:anyURI ;
  dcterms:source "URN:ISBN:978-0-643-10218-7" ;
  rdfs:label "Carbonates by pressure change - transducer" ;
  skos:broader <http://anzsoil.org/def/au/scma/19B> ;
  skos:definition "Carbonates by pressure change - transducer" ;
  skos:inScheme <http://anzsoil.org/def/au/scma> ;
  skos:notation "19B2" ;
  skos:prefLabel "Carbonates by pressure change - transducer" ;
.
<http://anzsoil.org/def/au/scma/19C1>
  a skos:Concept ;
  a sosa:Procedure ;
  dcterms:description "Spot field test for the presence of soil carbonates with dilute HCl" ;
  dcterms:identifier "http://anzsoil.org/def/au/scma/19C1"^^xsd:anyURI ;
  dcterms:source "URN:ISBN:978-0-643-10218-7" ;
  rdfs:label "Spot field test for the presence of soil carbonates with dilute HCl" ;
  skos:definition "Spot field test for the presence of soil carbonates with dilute HCl" ;
  skos:inScheme <http://anzsoil.org/def/au/scma> ;
  skos:notation "19C1" ;
  skos:prefLabel "Spot field test for the presence of soil carbonates with dilute HCl" ;
  skos:topConceptOf <http://anzsoil.org/def/au/scma> ;
.
<http://anzsoil.org/def/au/scma/19D1>
  a skos:Concept ;
  a sosa:Procedure ;
  dcterms:description "Field test for carbonates with dilute HCl and effervescence class assessment" ;
  dcterms:identifier "http://anzsoil.org/def/au/scma/19D1"^^xsd:anyURI ;
  dcterms:source "URN:ISBN:978-0-643-10218-7" ;
  rdfs:label "Field test for carbonates with dilute HCl and effervescence class assessment" ;
  skos:definition "Field test for carbonates with dilute HCl and effervescence class assessment" ;
  skos:inScheme <http://anzsoil.org/def/au/scma> ;
  skos:notation "19D1" ;
  skos:prefLabel "Field test for carbonates with dilute HCl and effervescence class assessment" ;
  skos:topConceptOf <http://anzsoil.org/def/au/scma> ;
.
<http://anzsoil.org/def/au/scma/1A1>
  a skos:Concept ;
  a sosa:Procedure ;
  dcterms:description "Field sampling - soil and land use surveys" ;
  dcterms:identifier "http://anzsoil.org/def/au/scma/1A1"^^xsd:anyURI ;
  dcterms:source "URN:ISBN:978-0-643-10218-7" ;
  rdfs:label "Field sampling - soil and land use surveys" ;
  skos:definition "Field sampling - soil and land use surveys" ;
  skos:inScheme <http://anzsoil.org/def/au/scma> ;
  skos:notation "1A1" ;
  skos:prefLabel "Field sampling - soil and land use surveys" ;
  skos:topConceptOf <http://anzsoil.org/def/au/scma> ;
.
<http://anzsoil.org/def/au/scma/1A2>
  a skos:Concept ;
  a sosa:Procedure ;
  dcterms:description "Field sampling - diagnostic" ;
  dcterms:identifier "http://anzsoil.org/def/au/scma/1A2"^^xsd:anyURI ;
  dcterms:source "URN:ISBN:978-0-643-10218-7" ;
  rdfs:label "Field sampling - diagnostic" ;
  skos:definition "Field sampling - diagnostic" ;
  skos:inScheme <http://anzsoil.org/def/au/scma> ;
  skos:notation "1A2" ;
  skos:prefLabel "Field sampling - diagnostic" ;
  skos:topConceptOf <http://anzsoil.org/def/au/scma> ;
.
<http://anzsoil.org/def/au/scma/1B1>
  a skos:Concept ;
  a sosa:Procedure ;
  dcterms:description "Laboratory preparation" ;
  dcterms:identifier "http://anzsoil.org/def/au/scma/1B1"^^xsd:anyURI ;
  dcterms:source "URN:ISBN:978-0-643-10218-7" ;
  rdfs:label "Laboratory preparation" ;
  skos:definition "Laboratory preparation" ;
  skos:inScheme <http://anzsoil.org/def/au/scma> ;
  skos:notation "1B1" ;
  skos:prefLabel "Laboratory preparation" ;
  skos:topConceptOf <http://anzsoil.org/def/au/scma> ;
.
<http://anzsoil.org/def/au/scma/2>
  a skos:Collection ;
  dcterms:description "Sampling, preparation and moisture content" ;
  dcterms:identifier "http://anzsoil.org/def/au/scma/2"^^xsd:anyURI ;
  dcterms:source "URN:ISBN:978-0-909605-68-1" ;
  ui:topMemberOf <http://anzsoil.org/def/au/scma> ;
  rdfs:label "Sampling, preparation and moisture content" ;
  skos:definition "Sampling, preparation and moisture content" ;
  skos:inScheme <http://anzsoil.org/def/au/scma> ;
  skos:member <http://anzsoil.org/def/au/scma/2A1> ;
  skos:member <http://anzsoil.org/def/au/scma/2B1> ;
  skos:member <http://anzsoil.org/def/au/scma/2C1> ;
  skos:member <http://anzsoil.org/def/au/scma/2D1> ;
  skos:notation "2" ;
  skos:prefLabel "Sampling, preparation and moisture content" ;
.
<http://anzsoil.org/def/au/scma/20>
  a skos:Collection ;
  dcterms:description "Acid sulfate soils" ;
  dcterms:identifier "http://anzsoil.org/def/au/scma/20"^^xsd:anyURI ;
  dcterms:source "URN:ISBN:978-0-643-10218-7" ;
  ui:topMemberOf <http://anzsoil.org/def/au/scma> ;
  rdfs:label "Acid sulfate soils" ;
  skos:definition "Acid sulfate soils" ;
  skos:inScheme <http://anzsoil.org/def/au/scma> ;
  skos:member <http://anzsoil.org/def/au/scma/20A1> ;
  skos:member <http://anzsoil.org/def/au/scma/20B1> ;
  skos:member <http://anzsoil.org/def/au/scma/20C1> ;
  skos:member <http://anzsoil.org/def/au/scma/20D1> ;
  skos:member <http://anzsoil.org/def/au/scma/20E1> ;
  skos:member <http://anzsoil.org/def/au/scma/20F1> ;
  skos:member <http://anzsoil.org/def/au/scma/20F2> ;
  skos:member <http://anzsoil.org/def/au/scma/20G1> ;
  skos:member <http://anzsoil.org/def/au/scma/20H1> ;
  skos:member <http://anzsoil.org/def/au/scma/20I1> ;
  skos:member <http://anzsoil.org/def/au/scma/20J1> ;
  skos:member <http://anzsoil.org/def/au/scma/20K1> ;
  skos:notation "20" ;
  skos:prefLabel "Acid sulfate soils" ;
.
<http://anzsoil.org/def/au/scma/20A1>
  a skos:Concept ;
  a sosa:Procedure ;
  dcterms:description "Chromium reducible S (S CR)" ;
  dcterms:identifier "http://anzsoil.org/def/au/scma/20A1"^^xsd:anyURI ;
  dcterms:source "URN:ISBN:978-0-643-10218-7" ;
  rdfs:label "Chromium reducible S (S CR)" ;
  skos:definition "Chromium reducible S (S CR)" ;
  skos:inScheme <http://anzsoil.org/def/au/scma> ;
  skos:notation "20A1" ;
  skos:prefLabel "Chromium reducible S (S CR)" ;
  skos:topConceptOf <http://anzsoil.org/def/au/scma> ;
.
<http://anzsoil.org/def/au/scma/20B1>
  a skos:Concept ;
  a sosa:Procedure ;
  dcterms:description "SPOCAS acid trail - titratable actual acidity (TAA)" ;
  dcterms:identifier "http://anzsoil.org/def/au/scma/20B1"^^xsd:anyURI ;
  dcterms:source "URN:ISBN:978-0-643-10218-7" ;
  rdfs:label "SPOCAS acid trail - titratable actual acidity (TAA)" ;
  skos:definition "SPOCAS acid trail - titratable actual acidity (TAA)" ;
  skos:inScheme <http://anzsoil.org/def/au/scma> ;
  skos:notation "20B1" ;
  skos:prefLabel "SPOCAS acid trail - titratable actual acidity (TAA)" ;
  skos:topConceptOf <http://anzsoil.org/def/au/scma> ;
.
<http://anzsoil.org/def/au/scma/20C1>
  a skos:Concept ;
  a sosa:Procedure ;
  dcterms:description "SPOCAS acid trail - titratable peroxide acidity (TPA) and Net (excess) Acid Neutralising Capacity (a-ANC E)" ;
  dcterms:identifier "http://anzsoil.org/def/au/scma/20C1"^^xsd:anyURI ;
  dcterms:source "URN:ISBN:978-0-643-10218-7" ;
  rdfs:label "SPOCAS acid trail - titratable peroxide acidity (TPA) and Net (excess) Acid Neutralising Capacity (a-ANC E)" ;
  skos:definition "SPOCAS acid trail - titratable peroxide acidity (TPA) and Net (excess) Acid Neutralising Capacity (a-ANC E)" ;
  skos:inScheme <http://anzsoil.org/def/au/scma> ;
  skos:notation "20C1" ;
  skos:prefLabel "SPOCAS acid trail - titratable peroxide acidity (TPA) and Net (excess) Acid Neutralising Capacity (a-ANC E)" ;
  skos:topConceptOf <http://anzsoil.org/def/au/scma> ;
.
<http://anzsoil.org/def/au/scma/20D1>
  a skos:Concept ;
  a sosa:Procedure ;
  dcterms:description "1 M KCl-extractable S, Ca and Mg" ;
  dcterms:identifier "http://anzsoil.org/def/au/scma/20D1"^^xsd:anyURI ;
  dcterms:source "URN:ISBN:978-0-643-10218-7" ;
  rdfs:label "1 M KCl-extractable S, Ca and Mg" ;
  skos:definition "1 M KCl-extractable S, Ca and Mg" ;
  skos:inScheme <http://anzsoil.org/def/au/scma> ;
  skos:notation "20D1" ;
  skos:prefLabel "1 M KCl-extractable S, Ca and Mg" ;
  skos:topConceptOf <http://anzsoil.org/def/au/scma> ;
.
<http://anzsoil.org/def/au/scma/20E1>
  a skos:Concept ;
  a sosa:Procedure ;
  dcterms:description "1 M KCl-extractable S, Ca and Mg after peroxide oxidation" ;
  dcterms:identifier "http://anzsoil.org/def/au/scma/20E1"^^xsd:anyURI ;
  dcterms:source "URN:ISBN:978-0-643-10218-7" ;
  rdfs:label "1 M KCl-extractable S, Ca and Mg after peroxide oxidation" ;
  skos:definition "1 M KCl-extractable S, Ca and Mg after peroxide oxidation" ;
  skos:inScheme <http://anzsoil.org/def/au/scma> ;
  skos:notation "20E1" ;
  skos:prefLabel "1 M KCl-extractable S, Ca and Mg after peroxide oxidation" ;
  skos:topConceptOf <http://anzsoil.org/def/au/scma> ;
.
<http://anzsoil.org/def/au/scma/20F1>
  a skos:Concept ;
  a sosa:Procedure ;
  dcterms:description "Sulfur - 4 M HCl extraction (S HCl), ICPAES finish" ;
  dcterms:identifier "http://anzsoil.org/def/au/scma/20F1"^^xsd:anyURI ;
  dcterms:source "URN:ISBN:978-0-643-10218-7" ;
  rdfs:label "Sulfur - 4 M HCl extraction (S HCl), ICPAES finish" ;
  skos:definition "Sulfur - 4 M HCl extraction (S HCl), ICPAES finish" ;
  skos:inScheme <http://anzsoil.org/def/au/scma> ;
  skos:notation "20F1" ;
  skos:prefLabel "Sulfur - 4 M HCl extraction (S HCl), ICPAES finish" ;
  skos:topConceptOf <http://anzsoil.org/def/au/scma> ;
.
<http://anzsoil.org/def/au/scma/20F2>
  a skos:Concept ;
  a sosa:Procedure ;
  dcterms:description "Sulfur - 4 M HCl extraction (S HCl), ion chromatography finish" ;
  dcterms:identifier "http://anzsoil.org/def/au/scma/20F2"^^xsd:anyURI ;
  dcterms:source "URN:ISBN:978-0-643-10218-7" ;
  rdfs:label "Sulfur - 4 M HCl extraction (S HCl), ion chromatography finish" ;
  skos:definition "Sulfur - 4 M HCl extraction (S HCl), ion chromatography finish" ;
  skos:inScheme <http://anzsoil.org/def/au/scma> ;
  skos:notation "20F2" ;
  skos:prefLabel "Sulfur - 4 M HCl extraction (S HCl), ion chromatography finish" ;
  skos:topConceptOf <http://anzsoil.org/def/au/scma> ;
.
<http://anzsoil.org/def/au/scma/20G1>
  a skos:Concept ;
  a sosa:Procedure ;
  dcterms:description "Peroxide residual acid soluble sulfur (S RAS)" ;
  dcterms:identifier "http://anzsoil.org/def/au/scma/20G1"^^xsd:anyURI ;
  dcterms:source "URN:ISBN:978-0-643-10218-7" ;
  rdfs:label "Peroxide residual acid soluble sulfur (S RAS)" ;
  skos:definition "Peroxide residual acid soluble sulfur (S RAS)" ;
  skos:inScheme <http://anzsoil.org/def/au/scma> ;
  skos:notation "20G1" ;
  skos:prefLabel "Peroxide residual acid soluble sulfur (S RAS)" ;
  skos:topConceptOf <http://anzsoil.org/def/au/scma> ;
.
<http://anzsoil.org/def/au/scma/20H1>
  a skos:Concept ;
  a sosa:Procedure ;
  dcterms:description "Acid neutralising capacity - acid reacted and back titration (ANC BT)" ;
  dcterms:identifier "http://anzsoil.org/def/au/scma/20H1"^^xsd:anyURI ;
  dcterms:source "URN:ISBN:978-0-643-10218-7" ;
  rdfs:label "Acid neutralising capacity - acid reacted and back titration (ANC BT)" ;
  skos:definition "Acid neutralising capacity - acid reacted and back titration (ANC BT)" ;
  skos:inScheme <http://anzsoil.org/def/au/scma> ;
  skos:notation "20H1" ;
  skos:prefLabel "Acid neutralising capacity - acid reacted and back titration (ANC BT)" ;
  skos:topConceptOf <http://anzsoil.org/def/au/scma> ;
.
<http://anzsoil.org/def/au/scma/20I1>
  a skos:Concept ;
  a sosa:Procedure ;
  dcterms:description "Acid neutralising capacity - from SPOCAS" ;
  dcterms:identifier "http://anzsoil.org/def/au/scma/20I1"^^xsd:anyURI ;
  dcterms:source "URN:ISBN:978-0-643-10218-7" ;
  rdfs:label "Acid neutralising capacity - from SPOCAS" ;
  skos:definition "Acid neutralising capacity - from SPOCAS" ;
  skos:inScheme <http://anzsoil.org/def/au/scma> ;
  skos:notation "20I1" ;
  skos:prefLabel "Acid neutralising capacity - from SPOCAS" ;
  skos:topConceptOf <http://anzsoil.org/def/au/scma> ;
.
<http://anzsoil.org/def/au/scma/20J1>
  a skos:Concept ;
  a sosa:Procedure ;
  dcterms:description "Field approximation of ASS hazard" ;
  dcterms:identifier "http://anzsoil.org/def/au/scma/20J1"^^xsd:anyURI ;
  dcterms:source "URN:ISBN:978-0-643-10218-7" ;
  rdfs:label "Field approximation of ASS hazard" ;
  skos:definition "Field approximation of ASS hazard" ;
  skos:inScheme <http://anzsoil.org/def/au/scma> ;
  skos:notation "20J1" ;
  skos:prefLabel "Field approximation of ASS hazard" ;
  skos:topConceptOf <http://anzsoil.org/def/au/scma> ;
.
<http://anzsoil.org/def/au/scma/20K1>
  a skos:Concept ;
  a sosa:Procedure ;
  dcterms:description "Quick field approximations of ASS presence and associated lime requirement for drain-spoil" ;
  dcterms:identifier "http://anzsoil.org/def/au/scma/20K1"^^xsd:anyURI ;
  dcterms:source "URN:ISBN:978-0-643-10218-7" ;
  rdfs:label "Quick field approximations of ASS presence and associated lime requirement for drain-spoil" ;
  skos:definition "Quick field approximations of ASS presence and associated lime requirement for drain-spoil" ;
  skos:inScheme <http://anzsoil.org/def/au/scma> ;
  skos:notation "20K1" ;
  skos:prefLabel "Quick field approximations of ASS presence and associated lime requirement for drain-spoil" ;
  skos:topConceptOf <http://anzsoil.org/def/au/scma> ;
.
<http://anzsoil.org/def/au/scma/2A1>
  a skos:Concept ;
  a sosa:Procedure ;
  dcterms:description "Air-dry moisture content" ;
  dcterms:identifier "http://anzsoil.org/def/au/scma/2A1"^^xsd:anyURI ;
  dcterms:source "URN:ISBN:978-0-643-10218-7" ;
  rdfs:label "Air-dry moisture content" ;
  skos:definition "Air-dry moisture content" ;
  skos:inScheme <http://anzsoil.org/def/au/scma> ;
  skos:notation "2A1" ;
  skos:prefLabel "Air-dry moisture content" ;
  skos:topConceptOf <http://anzsoil.org/def/au/scma> ;
.
<http://anzsoil.org/def/au/scma/2B1>
  a skos:Concept ;
  a sosa:Procedure ;
  dcterms:description "As received moisture content" ;
  dcterms:identifier "http://anzsoil.org/def/au/scma/2B1"^^xsd:anyURI ;
  dcterms:source "URN:ISBN:978-0-643-10218-7" ;
  rdfs:label "As received moisture content" ;
  skos:definition "As received moisture content" ;
  skos:inScheme <http://anzsoil.org/def/au/scma> ;
  skos:notation "2B1" ;
  skos:prefLabel "As received moisture content" ;
  skos:topConceptOf <http://anzsoil.org/def/au/scma> ;
.
<http://anzsoil.org/def/au/scma/2C1>
  a skos:Concept ;
  a sosa:Procedure ;
  dcterms:description "Moisture content - 10 mm tension" ;
  dcterms:identifier "http://anzsoil.org/def/au/scma/2C1"^^xsd:anyURI ;
  dcterms:source "URN:ISBN:978-0-643-10218-7" ;
  rdfs:label "Moisture content - 10 mm tension" ;
  skos:definition "Moisture content - 10 mm tension" ;
  skos:inScheme <http://anzsoil.org/def/au/scma> ;
  skos:notation "2C1" ;
  skos:prefLabel "Moisture content - 10 mm tension" ;
  skos:topConceptOf <http://anzsoil.org/def/au/scma> ;
.
<http://anzsoil.org/def/au/scma/2D1>
  a skos:Concept ;
  a sosa:Procedure ;
  dcterms:description "Moisture content - approximate saturation paste" ;
  dcterms:identifier "http://anzsoil.org/def/au/scma/2D1"^^xsd:anyURI ;
  dcterms:source "URN:ISBN:978-0-643-10218-7" ;
  rdfs:label "Moisture content - approximate saturation paste" ;
  skos:definition "Moisture content - approximate saturation paste" ;
  skos:inScheme <http://anzsoil.org/def/au/scma> ;
  skos:notation "2D1" ;
  skos:prefLabel "Moisture content - approximate saturation paste" ;
  skos:topConceptOf <http://anzsoil.org/def/au/scma> ;
.
<http://anzsoil.org/def/au/scma/3>
  a skos:Collection ;
  dcterms:description "Electrical conductivity, related attributes and redox potential" ;
  dcterms:identifier "http://anzsoil.org/def/au/scma/3"^^xsd:anyURI ;
  dcterms:source "URN:ISBN:978-0-643-10218-7" ;
  ui:topMemberOf <http://anzsoil.org/def/au/scma> ;
  rdfs:label "Electrical conductivity, related attributes and redox potential" ;
  skos:definition "Electrical conductivity, related attributes and redox potential" ;
  skos:inScheme <http://anzsoil.org/def/au/scma> ;
  skos:member <http://anzsoil.org/def/au/scma/3A1> ;
  skos:member <http://anzsoil.org/def/au/scma/3B1> ;
  skos:member <http://anzsoil.org/def/au/scma/3C1> ;
  skos:member <http://anzsoil.org/def/au/scma/3D1> ;
  skos:notation "3" ;
  skos:prefLabel "Electrical conductivity, related attributes and redox potential" ;
.
<http://anzsoil.org/def/au/scma/3A1>
  a skos:Concept ;
  a sosa:Procedure ;
  dcterms:description "Electrical conductivity (EC) of 1:5 soil/water extract" ;
  dcterms:identifier "http://anzsoil.org/def/au/scma/3A1"^^xsd:anyURI ;
  dcterms:source "URN:ISBN:978-0-643-10218-7" ;
  rdfs:label "Electrical conductivity (EC) of 1:5 soil/water extract" ;
  skos:definition "Electrical conductivity (EC) of 1:5 soil/water extract" ;
  skos:inScheme <http://anzsoil.org/def/au/scma> ;
  skos:notation "3A1" ;
  skos:prefLabel "Electrical conductivity (EC) of 1:5 soil/water extract" ;
  skos:topConceptOf <http://anzsoil.org/def/au/scma> ;
.
<http://anzsoil.org/def/au/scma/3B1>
  a skos:Concept ;
  a sosa:Procedure ;
  dcterms:description "Estimated soluble salt concentration" ;
  dcterms:identifier "http://anzsoil.org/def/au/scma/3B1"^^xsd:anyURI ;
  dcterms:source "URN:ISBN:978-0-643-10218-7" ;
  rdfs:label "Estimated soluble salt concentration" ;
  skos:definition "Estimated soluble salt concentration" ;
  skos:inScheme <http://anzsoil.org/def/au/scma> ;
  skos:notation "3B1" ;
  skos:prefLabel "Estimated soluble salt concentration" ;
  skos:topConceptOf <http://anzsoil.org/def/au/scma> ;
.
<http://anzsoil.org/def/au/scma/3C1>
  a skos:Concept ;
  a sosa:Procedure ;
  dcterms:description "Estimated soil ionic strength" ;
  dcterms:identifier "http://anzsoil.org/def/au/scma/3C1"^^xsd:anyURI ;
  dcterms:source "URN:ISBN:978-0-643-10218-7" ;
  rdfs:label "Estimated soil ionic strength" ;
  skos:definition "Estimated soil ionic strength" ;
  skos:inScheme <http://anzsoil.org/def/au/scma> ;
  skos:notation "3C1" ;
  skos:prefLabel "Estimated soil ionic strength" ;
  skos:topConceptOf <http://anzsoil.org/def/au/scma> ;
.
<http://anzsoil.org/def/au/scma/3D1>
  a skos:Concept ;
  a sosa:Procedure ;
  dcterms:description "Redox potential (Eh; field)" ;
  dcterms:identifier "http://anzsoil.org/def/au/scma/3D1"^^xsd:anyURI ;
  dcterms:source "URN:ISBN:978-0-643-10218-7" ;
  rdfs:label "Redox potential (Eh; field)" ;
  skos:definition "Redox potential (Eh; field)" ;
  skos:inScheme <http://anzsoil.org/def/au/scma> ;
  skos:notation "3D1" ;
  skos:prefLabel "Redox potential (Eh; field)" ;
  skos:topConceptOf <http://anzsoil.org/def/au/scma> ;
.
<http://anzsoil.org/def/au/scma/4>
  a skos:Collection ;
  dcterms:description "Soil pH" ;
  dcterms:identifier "http://anzsoil.org/def/au/scma/4"^^xsd:anyURI ;
  dcterms:source "URN:ISBN:978-0-909605-68-1" ;
  ui:topMemberOf <http://anzsoil.org/def/au/scma> ;
  rdfs:label "Soil pH" ;
  skos:definition "Soil pH" ;
  skos:inScheme <http://anzsoil.org/def/au/scma> ;
  skos:member <http://anzsoil.org/def/au/scma/4A1> ;
  skos:member <http://anzsoil.org/def/au/scma/4A2> ;
  skos:member <http://anzsoil.org/def/au/scma/4A3> ;
  skos:member <http://anzsoil.org/def/au/scma/4B1> ;
  skos:member <http://anzsoil.org/def/au/scma/4B2> ;
  skos:member <http://anzsoil.org/def/au/scma/4B3> ;
  skos:member <http://anzsoil.org/def/au/scma/4B4> ;
  skos:member <http://anzsoil.org/def/au/scma/4B5> ;
  skos:member <http://anzsoil.org/def/au/scma/4C1> ;
  skos:member <http://anzsoil.org/def/au/scma/4C2> ;
  skos:member <http://anzsoil.org/def/au/scma/4C3> ;
  skos:member <http://anzsoil.org/def/au/scma/4C4> ;
  skos:member <http://anzsoil.org/def/au/scma/4D1> ;
  skos:member <http://anzsoil.org/def/au/scma/4E1> ;
  skos:member <http://anzsoil.org/def/au/scma/4F1> ;
  skos:member <http://anzsoil.org/def/au/scma/4G1> ;
  skos:notation "4" ;
  skos:prefLabel "Soil pH" ;
.
<http://anzsoil.org/def/au/scma/4A1>
  a skos:Concept ;
  a sosa:Procedure ;
  dcterms:description "pH of a 1:5 soil/water suspension" ;
  dcterms:identifier "http://anzsoil.org/def/au/scma/4A1"^^xsd:anyURI ;
  dcterms:source "URN:ISBN:978-0-909605-68-1" ;
  rdfs:label "pH of a 1:5 soil/water suspension" ;
  skos:definition "pH of a 1:5 soil/water suspension" ;
  skos:inScheme <http://anzsoil.org/def/au/scma> ;
  skos:notation "4A1" ;
  skos:prefLabel "pH of a 1:5 soil/water suspension" ;
  skos:topConceptOf <http://anzsoil.org/def/au/scma> ;
.
<http://anzsoil.org/def/au/scma/4A2>
  a skos:Concept ;
  a sosa:Procedure ;
  dcterms:description "pH of a 1:1 soil/water suspension" ;
  dcterms:identifier "http://anzsoil.org/def/au/scma/4A2"^^xsd:anyURI ;
  dcterms:source "URN:ISBN:978-0-643-10218-7" ;
  rdfs:label "pH of a 1:1 soil/water suspension" ;
  skos:definition "pH of a 1:1 soil/water suspension" ;
  skos:inScheme <http://anzsoil.org/def/au/scma> ;
  skos:notation "4A2" ;
  skos:prefLabel "pH of a 1:1 soil/water suspension" ;
  skos:topConceptOf <http://anzsoil.org/def/au/scma> ;
.
<http://anzsoil.org/def/au/scma/4A3>
  a skos:Concept ;
  a sosa:Procedure ;
  dcterms:description "pH of a 1:2.5 soil/water suspension" ;
  dcterms:identifier "http://anzsoil.org/def/au/scma/4A3"^^xsd:anyURI ;
  dcterms:source "URN:ISBN:978-0-643-10218-7" ;
  rdfs:label "pH of a 1:2.5 soil/water suspension" ;
  skos:definition "pH of a 1:2.5 soil/water suspension" ;
  skos:inScheme <http://anzsoil.org/def/au/scma> ;
  skos:notation "4A3" ;
  skos:prefLabel "pH of a 1:2.5 soil/water suspension" ;
  skos:topConceptOf <http://anzsoil.org/def/au/scma> ;
.
<http://anzsoil.org/def/au/scma/4B1>
  a skos:Concept ;
  a sosa:Procedure ;
  dcterms:description "pH of 1:5 soil/0.01 M calcium chloride extract - direct (without stirring during measurement)" ;
  dcterms:identifier "http://anzsoil.org/def/au/scma/4B1"^^xsd:anyURI ;
  dcterms:source "URN:ISBN:978-0-643-10218-7" ;
  rdfs:label "pH of 1:5 soil/0.01 M calcium chloride extract - direct (without stirring during measurement)" ;
  skos:definition "pH of 1:5 soil/0.01 M calcium chloride extract - direct (without stirring during measurement)" ;
  skos:inScheme <http://anzsoil.org/def/au/scma> ;
  skos:notation "4B1" ;
  skos:prefLabel "pH of 1:5 soil/0.01 M calcium chloride extract - direct (without stirring during measurement)" ;
  skos:topConceptOf <http://anzsoil.org/def/au/scma> ;
.
<http://anzsoil.org/def/au/scma/4B2>
  a skos:Concept ;
  a sosa:Procedure ;
  dcterms:description "pH of 1:5 soil/0.01 M calcium chloride extract - following method 4A1 (without stirring during measurement)" ;
  dcterms:identifier "http://anzsoil.org/def/au/scma/4B2"^^xsd:anyURI ;
  dcterms:source "URN:ISBN:978-0-643-10218-7" ;
  rdfs:label "pH of 1:5 soil/0.01 M calcium chloride extract - following method 4A1 (without stirring during measurement)" ;
  skos:definition "pH of 1:5 soil/0.01 M calcium chloride extract - following method 4A1 (without stirring during measurement)" ;
  skos:inScheme <http://anzsoil.org/def/au/scma> ;
  skos:notation "4B2" ;
  skos:prefLabel "pH of 1:5 soil/0.01 M calcium chloride extract - following method 4A1 (without stirring during measurement)" ;
  skos:topConceptOf <http://anzsoil.org/def/au/scma> ;
.
<http://anzsoil.org/def/au/scma/4B3>
  a skos:Concept ;
  a sosa:Procedure ;
  dcterms:description "pH of 1:5 soil/0.01 M calcium chloride extract -direct (without stirring during measurement)" ;
  dcterms:identifier "http://anzsoil.org/def/au/scma/4B3"^^xsd:anyURI ;
  dcterms:source "URN:ISBN:978-0-643-10218-7" ;
  rdfs:label "pH of 1:5 soil/0.01 M calcium chloride extract -direct (without stirring during measurement)" ;
  skos:definition "pH of 1:5 soil/0.01 M calcium chloride extract -direct (without stirring during measurement)" ;
  skos:inScheme <http://anzsoil.org/def/au/scma> ;
  skos:notation "4B3" ;
  skos:prefLabel "pH of 1:5 soil/0.01 M calcium chloride extract -direct (without stirring during measurement)" ;
  skos:topConceptOf <http://anzsoil.org/def/au/scma> ;
.
<http://anzsoil.org/def/au/scma/4B4>
  a skos:Concept ;
  a sosa:Procedure ;
  dcterms:description "pH of 1:5 soil/0.01 M calcium chloride extract - following method 4A1 (with stirring during measurement)" ;
  dcterms:identifier "http://anzsoil.org/def/au/scma/4B4"^^xsd:anyURI ;
  dcterms:source "URN:ISBN:978-0-643-10218-7" ;
  rdfs:label "pH of 1:5 soil/0.01 M calcium chloride extract - following method 4A1 (with stirring during measurement)" ;
  skos:definition "pH of 1:5 soil/0.01 M calcium chloride extract - following method 4A1 (with stirring during measurement)" ;
  skos:inScheme <http://anzsoil.org/def/au/scma> ;
  skos:notation "4B4" ;
  skos:prefLabel "pH of 1:5 soil/0.01 M calcium chloride extract - following method 4A1 (with stirring during measurement)" ;
  skos:topConceptOf <http://anzsoil.org/def/au/scma> ;
.
<http://anzsoil.org/def/au/scma/4B5>
  a skos:Concept ;
  a sosa:Procedure ;
  dcterms:description "pH of 1:5 soil/0.01 M calcium chloride extract equivalent, by MIR reflectance spectroscopy" ;
  dcterms:identifier "http://anzsoil.org/def/au/scma/4B5"^^xsd:anyURI ;
  dcterms:source "URN:ISBN:978-0-643-10218-7" ;
  rdfs:label "pH of 1:5 soil/0.01 M calcium chloride extract equivalent, by MIR reflectance spectroscopy" ;
  skos:definition "pH of 1:5 soil/0.01 M calcium chloride extract equivalent, by MIR reflectance spectroscopy" ;
  skos:inScheme <http://anzsoil.org/def/au/scma> ;
  skos:notation "4B5" ;
  skos:prefLabel "pH of 1:5 soil/0.01 M calcium chloride extract equivalent, by MIR reflectance spectroscopy" ;
  skos:topConceptOf <http://anzsoil.org/def/au/scma> ;
.
<http://anzsoil.org/def/au/scma/4C1>
  a skos:Concept ;
  a sosa:Procedure ;
  dcterms:description "pH of 1:5 soil/1M potassium chloride extract - direct (without stirring during measurement)" ;
  dcterms:identifier "http://anzsoil.org/def/au/scma/4C1"^^xsd:anyURI ;
  dcterms:source "URN:ISBN:978-0-643-10218-7" ;
  rdfs:label "pH of 1:5 soil/1M potassium chloride extract - direct (without stirring during measurement)" ;
  skos:definition "pH of 1:5 soil/1M potassium chloride extract - direct (without stirring during measurement)" ;
  skos:inScheme <http://anzsoil.org/def/au/scma> ;
  skos:notation "4C1" ;
  skos:prefLabel "pH of 1:5 soil/1M potassium chloride extract - direct (without stirring during measurement)" ;
  skos:topConceptOf <http://anzsoil.org/def/au/scma> ;
.
<http://anzsoil.org/def/au/scma/4C2>
  a skos:Concept ;
  a sosa:Procedure ;
  dcterms:description "pH of 1:5 soil/1M potassium chloride extract following method 4A1 (without stirring during measurement)" ;
  dcterms:identifier "http://anzsoil.org/def/au/scma/4C2"^^xsd:anyURI ;
  dcterms:source "URN:ISBN:978-0-643-10218-7" ;
  rdfs:label "pH of 1:5 soil/1M potassium chloride extract following method 4A1 (without stirring during measurement)" ;
  skos:definition "pH of 1:5 soil/1M potassium chloride extract following method 4A1 (without stirring during measurement)" ;
  skos:inScheme <http://anzsoil.org/def/au/scma> ;
  skos:notation "4C2" ;
  skos:prefLabel "pH of 1:5 soil/1M potassium chloride extract following method 4A1 (without stirring during measurement)" ;
  skos:topConceptOf <http://anzsoil.org/def/au/scma> ;
.
<http://anzsoil.org/def/au/scma/4C3>
  a skos:Concept ;
  a sosa:Procedure ;
  dcterms:description "pH of 1:5 soil/1M potassium chloride extract - direct (with stirring during measurement)" ;
  dcterms:identifier "http://anzsoil.org/def/au/scma/4C3"^^xsd:anyURI ;
  dcterms:source "URN:ISBN:978-0-643-10218-7" ;
  rdfs:label "pH of 1:5 soil/1M potassium chloride extract - direct (with stirring during measurement)" ;
  skos:definition "pH of 1:5 soil/1M potassium chloride extract - direct (with stirring during measurement)" ;
  skos:inScheme <http://anzsoil.org/def/au/scma> ;
  skos:notation "4C3" ;
  skos:prefLabel "pH of 1:5 soil/1M potassium chloride extract - direct (with stirring during measurement)" ;
  skos:topConceptOf <http://anzsoil.org/def/au/scma> ;
.
<http://anzsoil.org/def/au/scma/4C4>
  a skos:Concept ;
  a sosa:Procedure ;
  dcterms:description "pH of 1:5 soil 1M potassium chloride extract - following method 4A1 (with stirring during measurement)" ;
  dcterms:identifier "http://anzsoil.org/def/au/scma/4C4"^^xsd:anyURI ;
  dcterms:source "URN:ISBN:978-0-643-10218-7" ;
  rdfs:label "pH of 1:5 soil 1M potassium chloride extract - following method 4A1 (with stirring during measurement)" ;
  skos:definition "pH of 1:5 soil 1M potassium chloride extract - following method 4A1 (with stirring during measurement)" ;
  skos:inScheme <http://anzsoil.org/def/au/scma> ;
  skos:notation "4C4" ;
  skos:prefLabel "pH of 1:5 soil 1M potassium chloride extract - following method 4A1 (with stirring during measurement)" ;
  skos:topConceptOf <http://anzsoil.org/def/au/scma> ;
.
<http://anzsoil.org/def/au/scma/4D1>
  a skos:Concept ;
  a sosa:Procedure ;
  dcterms:description "pH of sodium fluoride potential suspension and \\'reactivity class\\'" ;
  dcterms:identifier "http://anzsoil.org/def/au/scma/4D1"^^xsd:anyURI ;
  dcterms:source "URN:ISBN:978-0-643-10218-7" ;
  rdfs:label "pH of sodium fluoride potential suspension and \\'reactivity class\\'" ;
  skos:definition "pH of sodium fluoride potential suspension and \\'reactivity class\\'" ;
  skos:inScheme <http://anzsoil.org/def/au/scma> ;
  skos:notation "4D1" ;
  skos:prefLabel "pH of sodium fluoride potential suspension and \\'reactivity class\\'" ;
  skos:topConceptOf <http://anzsoil.org/def/au/scma> ;
.
<http://anzsoil.org/def/au/scma/4E1>
  a skos:Concept ;
  a sosa:Procedure ;
  dcterms:description "pH of hydrogen peroxide extract" ;
  dcterms:identifier "http://anzsoil.org/def/au/scma/4E1"^^xsd:anyURI ;
  dcterms:source "URN:ISBN:978-0-643-10218-7" ;
  rdfs:label "pH of hydrogen peroxide extract" ;
  skos:definition "pH of hydrogen peroxide extract" ;
  skos:inScheme <http://anzsoil.org/def/au/scma> ;
  skos:notation "4E1" ;
  skos:prefLabel "pH of hydrogen peroxide extract" ;
  skos:topConceptOf <http://anzsoil.org/def/au/scma> ;
.
<http://anzsoil.org/def/au/scma/4F1>
  a skos:Concept ;
  a sosa:Procedure ;
  dcterms:description "pH change" ;
  dcterms:identifier "http://anzsoil.org/def/au/scma/4F1"^^xsd:anyURI ;
  dcterms:source "URN:ISBN:978-0-643-10218-7" ;
  rdfs:label "pH change" ;
  skos:definition "pH change" ;
  skos:inScheme <http://anzsoil.org/def/au/scma> ;
  skos:notation "4F1" ;
  skos:prefLabel "pH change" ;
  skos:topConceptOf <http://anzsoil.org/def/au/scma> ;
.
<http://anzsoil.org/def/au/scma/4G1>
  a skos:Concept ;
  a sosa:Procedure ;
  dcterms:description "Field determination of pH" ;
  dcterms:identifier "http://anzsoil.org/def/au/scma/4G1"^^xsd:anyURI ;
  dcterms:source "URN:ISBN:978-0-643-10218-7" ;
  rdfs:label "Field determination of pH" ;
  skos:definition "Field determination of pH" ;
  skos:inScheme <http://anzsoil.org/def/au/scma> ;
  skos:notation "4G1" ;
  skos:prefLabel "Field determination of pH" ;
  skos:topConceptOf <http://anzsoil.org/def/au/scma> ;
.
<http://anzsoil.org/def/au/scma/5>
  a skos:Collection ;
  dcterms:description "Soluble chloride" ;
  dcterms:identifier "http://anzsoil.org/def/au/scma/5"^^xsd:anyURI ;
  dcterms:source "URN:ISBN:978-0-643-10218-7" ;
  ui:topMemberOf <http://anzsoil.org/def/au/scma> ;
  rdfs:label "Soluble chloride" ;
  skos:definition "Soluble chloride" ;
  skos:inScheme <http://anzsoil.org/def/au/scma> ;
  skos:member <http://anzsoil.org/def/au/scma/5A1> ;
  skos:member <http://anzsoil.org/def/au/scma/5A2> ;
  skos:member <http://anzsoil.org/def/au/scma/5A2a> ;
  skos:member <http://anzsoil.org/def/au/scma/5A2b> ;
  skos:member <http://anzsoil.org/def/au/scma/5A3a> ;
  skos:member <http://anzsoil.org/def/au/scma/5A3b> ;
  skos:member <http://anzsoil.org/def/au/scma/5A4> ;
  skos:notation "5" ;
  skos:prefLabel "Soluble chloride" ;
.
<http://anzsoil.org/def/au/scma/5A1>
  a skos:Concept ;
  a sosa:Procedure ;
  dcterms:description "Chloride - 1:5 soil/water extract, potentiometric titration" ;
  dcterms:identifier "http://anzsoil.org/def/au/scma/5A1"^^xsd:anyURI ;
  dcterms:source "URN:ISBN:978-0-643-10218-7" ;
  rdfs:label "Chloride - 1:5 soil/water extract, potentiometric titration" ;
  skos:definition "Chloride - 1:5 soil/water extract, potentiometric titration" ;
  skos:inScheme <http://anzsoil.org/def/au/scma> ;
  skos:notation "5A1" ;
  skos:prefLabel "Chloride - 1:5 soil/water extract, potentiometric titration" ;
  skos:topConceptOf <http://anzsoil.org/def/au/scma> ;
.
<http://anzsoil.org/def/au/scma/5A2>
  a skos:Concept ;
  a sosa:Procedure ;
  dcterms:description "Chloride - 1:5 soil/water extract, automated colour" ;
  dcterms:identifier "http://anzsoil.org/def/au/scma/5A2"^^xsd:anyURI ;
  dcterms:isReplacedBy <http://anzsoil.org/def/au/scma/5A2a> ;
  dcterms:isReplacedBy <http://anzsoil.org/def/au/scma/5A2b> ;
  dcterms:source "URN:ISBN:978-0-909605-68-1" ;
  rdfs:label "Chloride - 1:5 soil/water extract, automated colour" ;
  skos:definition "Chloride - 1:5 soil/water extract, automated colour" ;
  skos:inScheme <http://anzsoil.org/def/au/scma> ;
  skos:narrower <http://anzsoil.org/def/au/scma/5A2a> ;
  skos:narrower <http://anzsoil.org/def/au/scma/5A2b> ;
  skos:notation "5A2" ;
  skos:note "5A2 has been superseded by 5A2a and 5A2b in Soil Chemical Methods Australasia, Rayment G.E. and Lyons D.J. ISBN 9780643101364" ;
  skos:prefLabel "Chloride - 1:5 soil/water extract, automated colour" ;
  skos:topConceptOf <http://anzsoil.org/def/au/scma> ;
.
<http://anzsoil.org/def/au/scma/5A2a>
  a skos:Concept ;
  a sosa:Procedure ;
  dcterms:description "Chloride - 1:5 soil/water extract, automated colour" ;
  dcterms:identifier "http://anzsoil.org/def/au/scma/5A2a"^^xsd:anyURI ;
  dcterms:source "URN:ISBN:978-0-643-10218-7" ;
  rdfs:label "Chloride - 1:5 soil/water extract, automated colour" ;
  skos:broader <http://anzsoil.org/def/au/scma/5A2> ;
  skos:definition "Chloride - 1:5 soil/water extract, automated colour" ;
  skos:inScheme <http://anzsoil.org/def/au/scma> ;
  skos:notation "5A2a" ;
  skos:prefLabel "Chloride - 1:5 soil/water extract, automated colour" ;
.
<http://anzsoil.org/def/au/scma/5A2b>
  a skos:Concept ;
  a sosa:Procedure ;
  dcterms:description "Chloride - 1:5 soil/water extract, FIA" ;
  dcterms:identifier "http://anzsoil.org/def/au/scma/5A2b"^^xsd:anyURI ;
  dcterms:source "URN:ISBN:978-0-643-10218-7" ;
  rdfs:label "Chloride - 1:5 soil/water extract, FIA" ;
  skos:broader <http://anzsoil.org/def/au/scma/5A2> ;
  skos:definition "Chloride - 1:5 soil/water extract, FIA" ;
  skos:inScheme <http://anzsoil.org/def/au/scma> ;
  skos:notation "5A2b" ;
  skos:prefLabel "Chloride - 1:5 soil/water extract, FIA" ;
.
<http://anzsoil.org/def/au/scma/5A3a>
  a skos:Concept ;
  a sosa:Procedure ;
  dcterms:description "Chloride - 1:5 soil/water extract, ion chromatography (chemical suppression of eluent conductivity)" ;
  dcterms:identifier "http://anzsoil.org/def/au/scma/5A3a"^^xsd:anyURI ;
  dcterms:source "URN:ISBN:978-0-643-10218-7" ;
  rdfs:label "Chloride - 1:5 soil/water extract, ion chromatography (chemical suppression of eluent conductivity)" ;
  skos:definition "Chloride - 1:5 soil/water extract, ion chromatography (chemical suppression of eluent conductivity)" ;
  skos:inScheme <http://anzsoil.org/def/au/scma> ;
  skos:notation "5A3a" ;
  skos:prefLabel "Chloride - 1:5 soil/water extract, ion chromatography (chemical suppression of eluent conductivity)" ;
  skos:topConceptOf <http://anzsoil.org/def/au/scma> ;
.
<http://anzsoil.org/def/au/scma/5A3b>
  a skos:Concept ;
  a sosa:Procedure ;
  dcterms:description "Chloride - 1:5 soil/water extract, ion chromatography (single-column with electronic suppression of eluent conductivity)" ;
  dcterms:identifier "http://anzsoil.org/def/au/scma/5A3b"^^xsd:anyURI ;
  dcterms:source "URN:ISBN:978-0-643-10218-7" ;
  rdfs:label "Chloride - 1:5 soil/water extract, ion chromatography (single-column with electronic suppression of eluent conductivity)" ;
  skos:definition "Chloride - 1:5 soil/water extract, ion chromatography (single-column with electronic suppression of eluent conductivity)" ;
  skos:inScheme <http://anzsoil.org/def/au/scma> ;
  skos:notation "5A3b" ;
  skos:prefLabel "Chloride - 1:5 soil/water extract, ion chromatography (single-column with electronic suppression of eluent conductivity)" ;
  skos:topConceptOf <http://anzsoil.org/def/au/scma> ;
.
<http://anzsoil.org/def/au/scma/5A4>
  a skos:Concept ;
  a sosa:Procedure ;
  dcterms:description "Chloride - 1:5 soil/water extract ICPAES" ;
  dcterms:identifier "http://anzsoil.org/def/au/scma/5A4"^^xsd:anyURI ;
  dcterms:source "URN:ISBN:978-0-643-10218-7" ;
  rdfs:label "Chloride - 1:5 soil/water extract ICPAES" ;
  skos:definition "Chloride - 1:5 soil/water extract ICPAES" ;
  skos:inScheme <http://anzsoil.org/def/au/scma> ;
  skos:notation "5A4" ;
  skos:prefLabel "Chloride - 1:5 soil/water extract ICPAES" ;
  skos:topConceptOf <http://anzsoil.org/def/au/scma> ;
.
<http://anzsoil.org/def/au/scma/6>
  a skos:Collection ;
  dcterms:description "Carbon" ;
  dcterms:identifier "http://anzsoil.org/def/au/scma/6"^^xsd:anyURI ;
  dcterms:source "URN:ISBN:978-0-643-10218-7" ;
  ui:topMemberOf <http://anzsoil.org/def/au/scma> ;
  rdfs:label "Carbon" ;
  skos:definition "Carbon" ;
  skos:inScheme <http://anzsoil.org/def/au/scma> ;
  skos:member <http://anzsoil.org/def/au/scma/6A1> ;
  skos:member <http://anzsoil.org/def/au/scma/6B1> ;
  skos:member <http://anzsoil.org/def/au/scma/6B2> ;
  skos:member <http://anzsoil.org/def/au/scma/6B2a> ;
  skos:member <http://anzsoil.org/def/au/scma/6B2b> ;
  skos:member <http://anzsoil.org/def/au/scma/6B3> ;
  skos:member <http://anzsoil.org/def/au/scma/6B4> ;
  skos:member <http://anzsoil.org/def/au/scma/6B4a> ;
  skos:member <http://anzsoil.org/def/au/scma/6B4b> ;
  skos:member <http://anzsoil.org/def/au/scma/6C1> ;
  skos:member <http://anzsoil.org/def/au/scma/6D1> ;
  skos:member <http://anzsoil.org/def/au/scma/6E1> ;
  skos:member <http://anzsoil.org/def/au/scma/6F1> ;
  skos:member <http://anzsoil.org/def/au/scma/6G1> ;
  skos:notation "6" ;
  skos:prefLabel "Carbon" ;
.
<http://anzsoil.org/def/au/scma/6A1>
  a skos:Concept ;
  a sosa:Procedure ;
  dcterms:description "Organic C - W&B" ;
  dcterms:identifier "http://anzsoil.org/def/au/scma/6A1"^^xsd:anyURI ;
  dcterms:source "URN:ISBN:978-0-643-10218-7" ;
  rdfs:label "Organic C - W&B" ;
  skos:definition "Organic C - W&B" ;
  skos:inScheme <http://anzsoil.org/def/au/scma> ;
  skos:notation "6A1" ;
  skos:prefLabel "Organic C - W&B" ;
  skos:topConceptOf <http://anzsoil.org/def/au/scma> ;
.
<http://anzsoil.org/def/au/scma/6B1>
  a skos:Concept ;
  a sosa:Procedure ;
  dcterms:description "Total organic C - Heanes wet oxidisation" ;
  dcterms:identifier "http://anzsoil.org/def/au/scma/6B1"^^xsd:anyURI ;
  dcterms:source "URN:ISBN:978-0-643-10218-7" ;
  rdfs:label "Total organic C - Heanes wet oxidisation" ;
  skos:definition "Total organic C - Heanes wet oxidisation" ;
  skos:inScheme <http://anzsoil.org/def/au/scma> ;
  skos:notation "6B1" ;
  skos:prefLabel "Total organic C - Heanes wet oxidisation" ;
  skos:topConceptOf <http://anzsoil.org/def/au/scma> ;
.
<http://anzsoil.org/def/au/scma/6B2>
  a skos:Concept ;
  a sosa:Procedure ;
  dcterms:description "Total organic C - Dumas high-temperature combustion" ;
  dcterms:identifier "http://anzsoil.org/def/au/scma/6B2"^^xsd:anyURI ;
  dcterms:source "URN:ISBN:978-0-643-10218-7" ;
  rdfs:label "Total organic C - Dumas high-temperature combustion" ;
  skos:definition "Total organic C - Dumas high-temperature combustion" ;
  skos:inScheme <http://anzsoil.org/def/au/scma> ;
  skos:narrower <http://anzsoil.org/def/au/scma/6B2a> ;
  skos:narrower <http://anzsoil.org/def/au/scma/6B2b> ;
  skos:notation "6B2" ;
  skos:prefLabel "Total organic C - Dumas high-temperature combustion" ;
  skos:topConceptOf <http://anzsoil.org/def/au/scma> ;
.
<http://anzsoil.org/def/au/scma/6B2a>
  a skos:Concept ;
  a sosa:Procedure ;
  dcterms:description "Total organic C - Dumas high-temperature combustion, volumetric (no soil pretreatment)" ;
  dcterms:identifier "http://anzsoil.org/def/au/scma/6B2a"^^xsd:anyURI ;
  dcterms:source "URN:ISBN:978-0-643-10218-7" ;
  rdfs:label "Total organic C - Dumas high-temperature combustion, volumetric (no soil pretreatment)" ;
  skos:broader <http://anzsoil.org/def/au/scma/6B2> ;
  skos:definition "Total organic C - Dumas high-temperature combustion, volumetric (no soil pretreatment)" ;
  skos:inScheme <http://anzsoil.org/def/au/scma> ;
  skos:notation "6B2a" ;
  skos:prefLabel "Total organic C - Dumas high-temperature combustion, volumetric (no soil pretreatment)" ;
.
<http://anzsoil.org/def/au/scma/6B2b>
  a skos:Concept ;
  a sosa:Procedure ;
  dcterms:description "Total organic C - Dumas high-temperature combustion, infrared/thermal conductivity detection (no soil pretreatment)" ;
  dcterms:identifier "http://anzsoil.org/def/au/scma/6B2b"^^xsd:anyURI ;
  dcterms:source "URN:ISBN:978-0-643-10218-7" ;
  rdfs:label "Total organic C - Dumas high-temperature combustion, infrared/thermal conductivity detection (no soil pretreatment)" ;
  skos:broader <http://anzsoil.org/def/au/scma/6B2> ;
  skos:definition "Total organic C - Dumas high-temperature combustion, infrared/thermal conductivity detection (no soil pretreatment)" ;
  skos:inScheme <http://anzsoil.org/def/au/scma> ;
  skos:notation "6B2b" ;
  skos:prefLabel "Total organic C - Dumas high-temperature combustion, infrared/thermal conductivity detection (no soil pretreatment)" ;
.
<http://anzsoil.org/def/au/scma/6B3>
  a skos:Concept ;
  a sosa:Procedure ;
  dcterms:description "Total organic C - Dumas high-temperature combustion, infrared/thermal conductivity detection (with prior physical removal of charcoal and chemical removal of carbonates)" ;
  dcterms:identifier "http://anzsoil.org/def/au/scma/6B3"^^xsd:anyURI ;
  dcterms:source "URN:ISBN:978-0-643-10218-7" ;
  rdfs:label "Total organic C - Dumas high-temperature combustion, infrared/thermal conductivity detection (with prior physical removal of charcoal and chemical removal of carbonates)" ;
  skos:definition "Total organic C - Dumas high-temperature combustion, infrared/thermal conductivity detection (with prior physical removal of charcoal and chemical removal of carbonates)" ;
  skos:inScheme <http://anzsoil.org/def/au/scma> ;
  skos:notation "6B3" ;
  skos:prefLabel "Total organic C - Dumas high-temperature combustion, infrared/thermal conductivity detection (with prior physical removal of charcoal and chemical removal of carbonates)" ;
  skos:topConceptOf <http://anzsoil.org/def/au/scma> ;
.
<http://anzsoil.org/def/au/scma/6B4>
  a skos:Concept ;
  a sosa:Procedure ;
  dcterms:description "Total organic C - infrared diffuse reflectance spectroscopy" ;
  dcterms:identifier "http://anzsoil.org/def/au/scma/6B4"^^xsd:anyURI ;
  dcterms:source "URN:ISBN:978-0-643-10218-7" ;
  rdfs:label "Total organic C - infrared diffuse reflectance spectroscopy" ;
  skos:definition "Total organic C - infrared diffuse reflectance spectroscopy" ;
  skos:inScheme <http://anzsoil.org/def/au/scma> ;
  skos:narrower <http://anzsoil.org/def/au/scma/6B4a> ;
  skos:narrower <http://anzsoil.org/def/au/scma/6B4b> ;
  skos:notation "6B4" ;
  skos:prefLabel "Total organic C - infrared diffuse reflectance spectroscopy" ;
  skos:topConceptOf <http://anzsoil.org/def/au/scma> ;
.
<http://anzsoil.org/def/au/scma/6B4a>
  a skos:Concept ;
  a sosa:Procedure ;
  dcterms:description "Total organic C - NIR reflectance spectroscopy" ;
  dcterms:identifier "http://anzsoil.org/def/au/scma/6B4a"^^xsd:anyURI ;
  dcterms:source "URN:ISBN:978-0-643-10218-7" ;
  rdfs:label "Total organic C - NIR reflectance spectroscopy" ;
  skos:broader <http://anzsoil.org/def/au/scma/6B4> ;
  skos:definition "Total organic C - NIR reflectance spectroscopy" ;
  skos:inScheme <http://anzsoil.org/def/au/scma> ;
  skos:notation "6B4a" ;
  skos:prefLabel "Total organic C - NIR reflectance spectroscopy" ;
.
<http://anzsoil.org/def/au/scma/6B4b>
  a skos:Concept ;
  a sosa:Procedure ;
  dcterms:description "Total organic C - MIR reflectance spectroscopy" ;
  dcterms:identifier "http://anzsoil.org/def/au/scma/6B4b"^^xsd:anyURI ;
  dcterms:source "URN:ISBN:978-0-643-10218-7" ;
  rdfs:label "Total organic C - MIR reflectance spectroscopy" ;
  skos:broader <http://anzsoil.org/def/au/scma/6B4> ;
  skos:definition "Total organic C - MIR reflectance spectroscopy" ;
  skos:inScheme <http://anzsoil.org/def/au/scma> ;
  skos:notation "6B4b" ;
  skos:prefLabel "Total organic C - MIR reflectance spectroscopy" ;
.
<http://anzsoil.org/def/au/scma/6C1>
  a skos:Concept ;
  a sosa:Procedure ;
  dcterms:description "Particulate organic C (POC)" ;
  dcterms:identifier "http://anzsoil.org/def/au/scma/6C1"^^xsd:anyURI ;
  dcterms:source "URN:ISBN:978-0-643-10218-7" ;
  rdfs:label "Particulate organic C (POC)" ;
  skos:definition "Particulate organic C (POC)" ;
  skos:inScheme <http://anzsoil.org/def/au/scma> ;
  skos:notation "6C1" ;
  skos:prefLabel "Particulate organic C (POC)" ;
  skos:topConceptOf <http://anzsoil.org/def/au/scma> ;
.
<http://anzsoil.org/def/au/scma/6D1>
  a skos:Concept ;
  a sosa:Procedure ;
  dcterms:description "Pyrophosphate-extractable C" ;
  dcterms:identifier "http://anzsoil.org/def/au/scma/6D1"^^xsd:anyURI ;
  dcterms:source "URN:ISBN:978-0-643-10218-7" ;
  rdfs:label "Pyrophosphate-extractable C" ;
  skos:definition "Pyrophosphate-extractable C" ;
  skos:inScheme <http://anzsoil.org/def/au/scma> ;
  skos:notation "6D1" ;
  skos:prefLabel "Pyrophosphate-extractable C" ;
  skos:topConceptOf <http://anzsoil.org/def/au/scma> ;
.
<http://anzsoil.org/def/au/scma/6E1>
  a skos:Concept ;
  a sosa:Procedure ;
  dcterms:description "Potassium permanganate oxidisable C (PPOC)" ;
  dcterms:identifier "http://anzsoil.org/def/au/scma/6E1"^^xsd:anyURI ;
  dcterms:source "URN:ISBN:978-0-643-10218-7" ;
  rdfs:label "Potassium permanganate oxidisable C (PPOC)" ;
  skos:definition "Potassium permanganate oxidisable C (PPOC)" ;
  skos:inScheme <http://anzsoil.org/def/au/scma> ;
  skos:notation "6E1" ;
  skos:prefLabel "Potassium permanganate oxidisable C (PPOC)" ;
  skos:topConceptOf <http://anzsoil.org/def/au/scma> ;
.
<http://anzsoil.org/def/au/scma/6F1>
  a skos:Concept ;
  a sosa:Procedure ;
  dcterms:description "Charcoal-C" ;
  dcterms:identifier "http://anzsoil.org/def/au/scma/6F1"^^xsd:anyURI ;
  dcterms:source "URN:ISBN:978-0-643-10218-7" ;
  rdfs:label "Charcoal-C" ;
  skos:definition "Charcoal-C" ;
  skos:inScheme <http://anzsoil.org/def/au/scma> ;
  skos:notation "6F1" ;
  skos:prefLabel "Charcoal-C" ;
  skos:topConceptOf <http://anzsoil.org/def/au/scma> ;
.
<http://anzsoil.org/def/au/scma/6G1>
  a skos:Concept ;
  a sosa:Procedure ;
  dcterms:description "Total organic matter, organic C, and carbonate by loss-on-ignition" ;
  dcterms:identifier "http://anzsoil.org/def/au/scma/6G1"^^xsd:anyURI ;
  dcterms:source "URN:ISBN:978-0-643-10218-7" ;
  rdfs:label "Total organic matter, organic C, and carbonate by loss-on-ignition" ;
  skos:definition "Total organic matter, organic C, and carbonate by loss-on-ignition" ;
  skos:inScheme <http://anzsoil.org/def/au/scma> ;
  skos:notation "6G1" ;
  skos:prefLabel "Total organic matter, organic C, and carbonate by loss-on-ignition" ;
  skos:topConceptOf <http://anzsoil.org/def/au/scma> ;
.
<http://anzsoil.org/def/au/scma/7>
  a skos:Collection ;
  dcterms:description "Nitrogen" ;
  dcterms:identifier "http://anzsoil.org/def/au/scma/7"^^xsd:anyURI ;
  dcterms:source "URN:ISBN:978-0-643-10218-7" ;
  ui:topMemberOf <http://anzsoil.org/def/au/scma> ;
  rdfs:label "Nitrogen" ;
  skos:definition "Nitrogen" ;
  skos:inScheme <http://anzsoil.org/def/au/scma> ;
  skos:member <http://anzsoil.org/def/au/scma/7A1> ;
  skos:member <http://anzsoil.org/def/au/scma/7A2> ;
  skos:member <http://anzsoil.org/def/au/scma/7A2a> ;
  skos:member <http://anzsoil.org/def/au/scma/7A2b> ;
  skos:member <http://anzsoil.org/def/au/scma/7A3> ;
  skos:member <http://anzsoil.org/def/au/scma/7A4> ;
  skos:member <http://anzsoil.org/def/au/scma/7A5> ;
  skos:member <http://anzsoil.org/def/au/scma/7A6> ;
  skos:member <http://anzsoil.org/def/au/scma/7A6a> ;
  skos:member <http://anzsoil.org/def/au/scma/7A6b> ;
  skos:member <http://anzsoil.org/def/au/scma/7B> ;
  skos:member <http://anzsoil.org/def/au/scma/7B1> ;
  skos:member <http://anzsoil.org/def/au/scma/7B1a> ;
  skos:member <http://anzsoil.org/def/au/scma/7B1b> ;
  skos:member <http://anzsoil.org/def/au/scma/7B2> ;
  skos:member <http://anzsoil.org/def/au/scma/7C1> ;
  skos:member <http://anzsoil.org/def/au/scma/7C1a> ;
  skos:member <http://anzsoil.org/def/au/scma/7C1b> ;
  skos:member <http://anzsoil.org/def/au/scma/7C1c> ;
  skos:member <http://anzsoil.org/def/au/scma/7C1d> ;
  skos:member <http://anzsoil.org/def/au/scma/7C1e> ;
  skos:member <http://anzsoil.org/def/au/scma/7C1f> ;
  skos:member <http://anzsoil.org/def/au/scma/7C1g> ;
  skos:member <http://anzsoil.org/def/au/scma/7C1h> ;
  skos:member <http://anzsoil.org/def/au/scma/7C2> ;
  skos:member <http://anzsoil.org/def/au/scma/7C2a> ;
  skos:member <http://anzsoil.org/def/au/scma/7C2b> ;
  skos:member <http://anzsoil.org/def/au/scma/7D> ;
  skos:member <http://anzsoil.org/def/au/scma/7D1a> ;
  skos:member <http://anzsoil.org/def/au/scma/7D1b> ;
  skos:member <http://anzsoil.org/def/au/scma/7D1c> ;
  skos:member <http://anzsoil.org/def/au/scma/7D2a> ;
  skos:member <http://anzsoil.org/def/au/scma/7D2b> ;
  skos:notation "7" ;
  skos:prefLabel "Nitrogen" ;
.
<http://anzsoil.org/def/au/scma/7A1>
  a skos:Concept ;
  a sosa:Procedure ;
  dcterms:description "Total soil-N, semi micro Kjeldahl - steam distillation" ;
  dcterms:identifier "http://anzsoil.org/def/au/scma/7A1"^^xsd:anyURI ;
  dcterms:source "URN:ISBN:978-0-643-10218-7" ;
  rdfs:label "Total soil-N, semi micro Kjeldahl - steam distillation" ;
  skos:definition "Total soil-N, semi micro Kjeldahl - steam distillation" ;
  skos:inScheme <http://anzsoil.org/def/au/scma> ;
  skos:notation "7A1" ;
  skos:prefLabel "Total soil-N, semi micro Kjeldahl - steam distillation" ;
  skos:topConceptOf <http://anzsoil.org/def/au/scma> ;
.
<http://anzsoil.org/def/au/scma/7A2>
  a skos:Concept ;
  a sosa:Procedure ;
  dcterms:description "Total soil-N, semi micro Kjeldahl - automated colour|Total nitrogen - semimicro Kjeldahl, automated colour" ;
  dcterms:identifier "http://anzsoil.org/def/au/scma/7A2"^^xsd:anyURI ;
  dcterms:isReplacedBy <http://anzsoil.org/def/au/scma/7A2a> ;
  dcterms:isReplacedBy <http://anzsoil.org/def/au/scma/7A2b> ;
  dcterms:source "URN:ISBN:978-0-909605-68-1" ;
  rdfs:label "Total soil-N, semi micro Kjeldahl - automated colour|Total nitrogen - semimicro Kjeldahl, automated colour" ;
  skos:definition "Total soil-N, semi micro Kjeldahl - automated colour|Total nitrogen - semimicro Kjeldahl, automated colour" ;
  skos:inScheme <http://anzsoil.org/def/au/scma> ;
  skos:narrower <http://anzsoil.org/def/au/scma/7A2a> ;
  skos:narrower <http://anzsoil.org/def/au/scma/7A2b> ;
  skos:notation "7A2" ;
  skos:note "7A2 has been superseded by 7A2a and 7A2b in Soil Chemical Methods Australasia, Rayment G.E. and Lyons D.J. ISBN 9780643101364" ;
  skos:prefLabel "Total soil-N, semi micro Kjeldahl - automated colour|Total nitrogen - semimicro Kjeldahl, automated colour" ;
  skos:topConceptOf <http://anzsoil.org/def/au/scma> ;
.
<http://anzsoil.org/def/au/scma/7A2a>
  a skos:Concept ;
  a sosa:Procedure ;
  dcterms:description "Total soil-N, semi micro Kjeldahl - automated colour, continuous segmented flow" ;
  dcterms:identifier "http://anzsoil.org/def/au/scma/7A2a"^^xsd:anyURI ;
  dcterms:source "URN:ISBN:978-0-643-10218-7" ;
  rdfs:label "Total soil-N, semi micro Kjeldahl - automated colour, continuous segmented flow" ;
  skos:broader <http://anzsoil.org/def/au/scma/7A2> ;
  skos:definition "Total soil-N, semi micro Kjeldahl - automated colour, continuous segmented flow" ;
  skos:inScheme <http://anzsoil.org/def/au/scma> ;
  skos:notation "7A2a" ;
  skos:prefLabel "Total soil-N, semi micro Kjeldahl - automated colour, continuous segmented flow" ;
.
<http://anzsoil.org/def/au/scma/7A2b>
  a skos:Concept ;
  a sosa:Procedure ;
  dcterms:description "Total soil-N, semi micro Kjeldahl - automated colour - FIA" ;
  dcterms:identifier "http://anzsoil.org/def/au/scma/7A2b"^^xsd:anyURI ;
  dcterms:source "URN:ISBN:978-0-643-10218-7" ;
  rdfs:label "Total soil-N, semi micro Kjeldahl - automated colour - FIA" ;
  skos:broader <http://anzsoil.org/def/au/scma/7A2> ;
  skos:definition "Total soil-N, semi micro Kjeldahl - automated colour - FIA" ;
  skos:inScheme <http://anzsoil.org/def/au/scma> ;
  skos:notation "7A2b" ;
  skos:prefLabel "Total soil-N, semi micro Kjeldahl - automated colour - FIA" ;
.
<http://anzsoil.org/def/au/scma/7A3>
  a skos:Concept ;
  a sosa:Procedure ;
  dcterms:description "Total soil-N (where nitrate >20 mg N/kg) - steam distillation" ;
  dcterms:identifier "http://anzsoil.org/def/au/scma/7A3"^^xsd:anyURI ;
  dcterms:source "URN:ISBN:978-0-643-10218-7" ;
  rdfs:label "Total soil-N (where nitrate >20 mg N/kg) - steam distillation" ;
  skos:definition "Total soil-N (where nitrate >20 mg N/kg) - steam distillation" ;
  skos:inScheme <http://anzsoil.org/def/au/scma> ;
  skos:notation "7A3" ;
  skos:prefLabel "Total soil-N (where nitrate >20 mg N/kg) - steam distillation" ;
  skos:topConceptOf <http://anzsoil.org/def/au/scma> ;
.
<http://anzsoil.org/def/au/scma/7A4>
  a skos:Concept ;
  a sosa:Procedure ;
  dcterms:description "Total-N (where nitrate >20 mg N/kg) - automated colour, continuous segmented flow/FIA" ;
  dcterms:identifier "http://anzsoil.org/def/au/scma/7A4"^^xsd:anyURI ;
  dcterms:source "URN:ISBN:978-0-643-10218-7" ;
  rdfs:label "Total-N (where nitrate >20 mg N/kg) - automated colour, continuous segmented flow/FIA" ;
  skos:definition "Total-N (where nitrate >20 mg N/kg) - automated colour, continuous segmented flow/FIA" ;
  skos:inScheme <http://anzsoil.org/def/au/scma> ;
  skos:notation "7A4" ;
  skos:prefLabel "Total-N (where nitrate >20 mg N/kg) - automated colour, continuous segmented flow/FIA" ;
  skos:topConceptOf <http://anzsoil.org/def/au/scma> ;
.
<http://anzsoil.org/def/au/scma/7A5>
  a skos:Concept ;
  a sosa:Procedure ;
  dcterms:description "Total soil-N - Dumas high-temperature combustion" ;
  dcterms:identifier "http://anzsoil.org/def/au/scma/7A5"^^xsd:anyURI ;
  dcterms:source "URN:ISBN:978-0-643-10218-7" ;
  rdfs:label "Total soil-N - Dumas high-temperature combustion" ;
  skos:definition "Total soil-N - Dumas high-temperature combustion" ;
  skos:inScheme <http://anzsoil.org/def/au/scma> ;
  skos:notation "7A5" ;
  skos:prefLabel "Total soil-N - Dumas high-temperature combustion" ;
  skos:topConceptOf <http://anzsoil.org/def/au/scma> ;
.
<http://anzsoil.org/def/au/scma/7A6>
  a skos:Concept ;
  a sosa:Procedure ;
  dcterms:description "Total soil-N - infrared diffuse reflectance spectroscopy" ;
  dcterms:identifier "http://anzsoil.org/def/au/scma/7A6"^^xsd:anyURI ;
  dcterms:source "URN:ISBN:978-0-643-10218-7" ;
  rdfs:label "Total soil-N - infrared diffuse reflectance spectroscopy" ;
  skos:definition "Total soil-N - infrared diffuse reflectance spectroscopy" ;
  skos:inScheme <http://anzsoil.org/def/au/scma> ;
  skos:narrower <http://anzsoil.org/def/au/scma/7A6a> ;
  skos:narrower <http://anzsoil.org/def/au/scma/7A6b> ;
  skos:notation "7A6" ;
  skos:prefLabel "Total soil-N - infrared diffuse reflectance spectroscopy" ;
  skos:topConceptOf <http://anzsoil.org/def/au/scma> ;
.
<http://anzsoil.org/def/au/scma/7A6a>
  a skos:Concept ;
  a sosa:Procedure ;
  dcterms:description "Total Soil-N - NIR diffuse reflectance spectroscopy" ;
  dcterms:identifier "http://anzsoil.org/def/au/scma/7A6a"^^xsd:anyURI ;
  dcterms:source "URN:ISBN:978-0-643-10218-7" ;
  rdfs:label "Total Soil-N - NIR diffuse reflectance spectroscopy" ;
  skos:broader <http://anzsoil.org/def/au/scma/7A6> ;
  skos:definition "Total Soil-N - NIR diffuse reflectance spectroscopy" ;
  skos:inScheme <http://anzsoil.org/def/au/scma> ;
  skos:notation "7A6a" ;
  skos:prefLabel "Total Soil-N - NIR diffuse reflectance spectroscopy" ;
.
<http://anzsoil.org/def/au/scma/7A6b>
  a skos:Concept ;
  a sosa:Procedure ;
  dcterms:description "Total soil-N - MIR diffuse reflectance spectroscopy" ;
  dcterms:identifier "http://anzsoil.org/def/au/scma/7A6b"^^xsd:anyURI ;
  dcterms:source "URN:ISBN:978-0-643-10218-7" ;
  rdfs:label "Total soil-N - MIR diffuse reflectance spectroscopy" ;
  skos:broader <http://anzsoil.org/def/au/scma/7A6> ;
  skos:definition "Total soil-N - MIR diffuse reflectance spectroscopy" ;
  skos:inScheme <http://anzsoil.org/def/au/scma> ;
  skos:notation "7A6b" ;
  skos:prefLabel "Total soil-N - MIR diffuse reflectance spectroscopy" ;
.
<http://anzsoil.org/def/au/scma/7B>
  a skos:Concept ;
  a sosa:Procedure ;
  dcterms:description "Water-soluble nitrate-N" ;
  dcterms:identifier "http://anzsoil.org/def/au/scma/7B"^^xsd:anyURI ;
  dcterms:source "URN:ISBN:978-0-643-10218-7" ;
  rdfs:label "Water-soluble nitrate-N" ;
  skos:definition "Water-soluble nitrate-N" ;
  skos:inScheme <http://anzsoil.org/def/au/scma> ;
  skos:narrower <http://anzsoil.org/def/au/scma/7B1> ;
  skos:narrower <http://anzsoil.org/def/au/scma/7B2> ;
  skos:notation "7B" ;
  skos:prefLabel "Water-soluble nitrate-N" ;
  skos:topConceptOf <http://anzsoil.org/def/au/scma> ;
.
<http://anzsoil.org/def/au/scma/7B1>
  a skos:Concept ;
  a sosa:Procedure ;
  dcterms:description "Water-soluble nitrate-N - automated colour|Water soluble nitrate - automated colour" ;
  dcterms:identifier "http://anzsoil.org/def/au/scma/7B1"^^xsd:anyURI ;
  dcterms:isReplacedBy <http://anzsoil.org/def/au/scma/7B1a> ;
  dcterms:isReplacedBy <http://anzsoil.org/def/au/scma/7B1b> ;
  dcterms:source "URN:ISBN:978-0-909605-68-1" ;
  rdfs:label "Water-soluble nitrate-N - automated colour|Water soluble nitrate - automated colour" ;
  skos:broader <http://anzsoil.org/def/au/scma/7B> ;
  skos:definition "Water-soluble nitrate-N - automated colour|Water soluble nitrate - automated colour" ;
  skos:inScheme <http://anzsoil.org/def/au/scma> ;
  skos:narrower <http://anzsoil.org/def/au/scma/7B1a> ;
  skos:narrower <http://anzsoil.org/def/au/scma/7B1b> ;
  skos:notation "7B1" ;
  skos:note "7B1 has been superseded by 7B1a and 7B1b in Soil Chemical Methods Australasia, Rayment G.E. and Lyons D.J. ISBN 9780643101364" ;
  skos:prefLabel "Water-soluble nitrate-N - automated colour|Water soluble nitrate - automated colour" ;
.
<http://anzsoil.org/def/au/scma/7B1a>
  a skos:Concept ;
  a sosa:Procedure ;
  dcterms:description "Water-soluble nitrate-N - automated colour, continuous segmented flow" ;
  dcterms:identifier "http://anzsoil.org/def/au/scma/7B1a"^^xsd:anyURI ;
  dcterms:source "URN:ISBN:978-0-643-10218-7" ;
  rdfs:label "Water-soluble nitrate-N - automated colour, continuous segmented flow" ;
  skos:broader <http://anzsoil.org/def/au/scma/7B1> ;
  skos:definition "Water-soluble nitrate-N - automated colour, continuous segmented flow" ;
  skos:inScheme <http://anzsoil.org/def/au/scma> ;
  skos:notation "7B1a" ;
  skos:prefLabel "Water-soluble nitrate-N - automated colour, continuous segmented flow" ;
.
<http://anzsoil.org/def/au/scma/7B1b>
  a skos:Concept ;
  a sosa:Procedure ;
  dcterms:description "Water-soluble nitrate-N - automated colour, FIA" ;
  dcterms:identifier "http://anzsoil.org/def/au/scma/7B1b"^^xsd:anyURI ;
  dcterms:source "URN:ISBN:978-0-643-10218-7" ;
  rdfs:label "Water-soluble nitrate-N - automated colour, FIA" ;
  skos:broader <http://anzsoil.org/def/au/scma/7B1> ;
  skos:definition "Water-soluble nitrate-N - automated colour, FIA" ;
  skos:inScheme <http://anzsoil.org/def/au/scma> ;
  skos:notation "7B1b" ;
  skos:prefLabel "Water-soluble nitrate-N - automated colour, FIA" ;
.
<http://anzsoil.org/def/au/scma/7B2>
  a skos:Concept ;
  a sosa:Procedure ;
  dcterms:description "Water-soluble nitrate-N - ion chromatography" ;
  dcterms:identifier "http://anzsoil.org/def/au/scma/7B2"^^xsd:anyURI ;
  dcterms:source "URN:ISBN:978-0-643-10218-7" ;
  rdfs:label "Water-soluble nitrate-N - ion chromatography" ;
  skos:broader <http://anzsoil.org/def/au/scma/7B> ;
  skos:definition "Water-soluble nitrate-N - ion chromatography" ;
  skos:inScheme <http://anzsoil.org/def/au/scma> ;
  skos:notation "7B2" ;
  skos:prefLabel "Water-soluble nitrate-N - ion chromatography" ;
.
<http://anzsoil.org/def/au/scma/7C1>
  a skos:Concept ;
  a sosa:Procedure ;
  dcterms:description "Mineral-N 2 M KCl, steam distillation" ;
  dcterms:identifier "http://anzsoil.org/def/au/scma/7C1"^^xsd:anyURI ;
  dcterms:source "URN:ISBN:978-0-643-10218-7" ;
  rdfs:label "Mineral-N 2 M KCl, steam distillation" ;
  skos:definition "Mineral-N 2 M KCl, steam distillation" ;
  skos:inScheme <http://anzsoil.org/def/au/scma> ;
  skos:narrower <http://anzsoil.org/def/au/scma/7C1a> ;
  skos:narrower <http://anzsoil.org/def/au/scma/7C1b> ;
  skos:narrower <http://anzsoil.org/def/au/scma/7C1c> ;
  skos:narrower <http://anzsoil.org/def/au/scma/7C1d> ;
  skos:narrower <http://anzsoil.org/def/au/scma/7C1e> ;
  skos:narrower <http://anzsoil.org/def/au/scma/7C1f> ;
  skos:narrower <http://anzsoil.org/def/au/scma/7C1g> ;
  skos:narrower <http://anzsoil.org/def/au/scma/7C1h> ;
  skos:notation "7C1" ;
  skos:prefLabel "Mineral-N 2 M KCl, steam distillation" ;
  skos:topConceptOf <http://anzsoil.org/def/au/scma> ;
.
<http://anzsoil.org/def/au/scma/7C1a>
  a skos:Concept ;
  a sosa:Procedure ;
  dcterms:description "Ammonium-N (in presence or absence of nitrite) - steam distillation" ;
  dcterms:identifier "http://anzsoil.org/def/au/scma/7C1a"^^xsd:anyURI ;
  dcterms:source "URN:ISBN:978-0-643-10218-7" ;
  rdfs:label "Ammonium-N (in presence or absence of nitrite) - steam distillation" ;
  skos:broader <http://anzsoil.org/def/au/scma/7C1> ;
  skos:definition "Ammonium-N (in presence or absence of nitrite) - steam distillation" ;
  skos:inScheme <http://anzsoil.org/def/au/scma> ;
  skos:notation "7C1a" ;
  skos:prefLabel "Ammonium-N (in presence or absence of nitrite) - steam distillation" ;
.
<http://anzsoil.org/def/au/scma/7C1b>
  a skos:Concept ;
  a sosa:Procedure ;
  dcterms:description "(Nitrate + Nitrite)-N - steam distillation" ;
  dcterms:identifier "http://anzsoil.org/def/au/scma/7C1b"^^xsd:anyURI ;
  dcterms:source "URN:ISBN:978-0-643-10218-7" ;
  rdfs:label "(Nitrate + Nitrite)-N - steam distillation" ;
  skos:broader <http://anzsoil.org/def/au/scma/7C1> ;
  skos:definition "(Nitrate + Nitrite)-N - steam distillation" ;
  skos:inScheme <http://anzsoil.org/def/au/scma> ;
  skos:notation "7C1b" ;
  skos:prefLabel "(Nitrate + Nitrite)-N - steam distillation" ;
.
<http://anzsoil.org/def/au/scma/7C1c>
  a skos:Concept ;
  a sosa:Procedure ;
  dcterms:description "(Ammonium + Nitrate + Nitrite)-N - steam distillation" ;
  dcterms:identifier "http://anzsoil.org/def/au/scma/7C1c"^^xsd:anyURI ;
  dcterms:source "URN:ISBN:978-0-643-10218-7" ;
  rdfs:label "(Ammonium + Nitrate + Nitrite)-N - steam distillation" ;
  skos:broader <http://anzsoil.org/def/au/scma/7C1> ;
  skos:definition "(Ammonium + Nitrate + Nitrite)-N - steam distillation" ;
  skos:inScheme <http://anzsoil.org/def/au/scma> ;
  skos:notation "7C1c" ;
  skos:prefLabel "(Ammonium + Nitrate + Nitrite)-N - steam distillation" ;
.
<http://anzsoil.org/def/au/scma/7C1d>
  a skos:Concept ;
  a sosa:Procedure ;
  dcterms:description "(Ammonium + Nitrate)-N, in presence of nitrite - steam distillation" ;
  dcterms:identifier "http://anzsoil.org/def/au/scma/7C1d"^^xsd:anyURI ;
  dcterms:source "URN:ISBN:978-0-643-10218-7" ;
  rdfs:label "(Ammonium + Nitrate)-N, in presence of nitrite - steam distillation" ;
  skos:broader <http://anzsoil.org/def/au/scma/7C1> ;
  skos:definition "(Ammonium + Nitrate)-N, in presence of nitrite - steam distillation" ;
  skos:inScheme <http://anzsoil.org/def/au/scma> ;
  skos:notation "7C1d" ;
  skos:prefLabel "(Ammonium + Nitrate)-N, in presence of nitrite - steam distillation" ;
.
<http://anzsoil.org/def/au/scma/7C1e>
  a skos:Concept ;
  a sosa:Procedure ;
  dcterms:description "Nitrate-N, in presence of nitrite - steam distillation" ;
  dcterms:identifier "http://anzsoil.org/def/au/scma/7C1e"^^xsd:anyURI ;
  dcterms:source "URN:ISBN:978-0-643-10218-7" ;
  rdfs:label "Nitrate-N, in presence of nitrite - steam distillation" ;
  skos:broader <http://anzsoil.org/def/au/scma/7C1> ;
  skos:definition "Nitrate-N, in presence of nitrite - steam distillation" ;
  skos:inScheme <http://anzsoil.org/def/au/scma> ;
  skos:notation "7C1e" ;
  skos:prefLabel "Nitrate-N, in presence of nitrite - steam distillation" ;
.
<http://anzsoil.org/def/au/scma/7C1f>
  a skos:Concept ;
  a sosa:Procedure ;
  dcterms:description "Nitrate-N, in absence of nitrite - steam distillation" ;
  dcterms:identifier "http://anzsoil.org/def/au/scma/7C1f"^^xsd:anyURI ;
  dcterms:source "URN:ISBN:978-0-643-10218-7" ;
  rdfs:label "Nitrate-N, in absence of nitrite - steam distillation" ;
  skos:broader <http://anzsoil.org/def/au/scma/7C1> ;
  skos:definition "Nitrate-N, in absence of nitrite - steam distillation" ;
  skos:inScheme <http://anzsoil.org/def/au/scma> ;
  skos:notation "7C1f" ;
  skos:prefLabel "Nitrate-N, in absence of nitrite - steam distillation" ;
.
<http://anzsoil.org/def/au/scma/7C1g>
  a skos:Concept ;
  a sosa:Procedure ;
  dcterms:description "(Ammonium + Nitrate)-N, in absence of nitrite - steam distillation" ;
  dcterms:identifier "http://anzsoil.org/def/au/scma/7C1g"^^xsd:anyURI ;
  dcterms:source "URN:ISBN:978-0-643-10218-7" ;
  rdfs:label "(Ammonium + Nitrate)-N, in absence of nitrite - steam distillation" ;
  skos:broader <http://anzsoil.org/def/au/scma/7C1> ;
  skos:definition "(Ammonium + Nitrate)-N, in absence of nitrite - steam distillation" ;
  skos:inScheme <http://anzsoil.org/def/au/scma> ;
  skos:notation "7C1g" ;
  skos:prefLabel "(Ammonium + Nitrate)-N, in absence of nitrite - steam distillation" ;
.
<http://anzsoil.org/def/au/scma/7C1h>
  a skos:Concept ;
  a sosa:Procedure ;
  dcterms:description "Nitrite-N - steam distillation" ;
  dcterms:identifier "http://anzsoil.org/def/au/scma/7C1h"^^xsd:anyURI ;
  dcterms:source "URN:ISBN:978-0-643-10218-7" ;
  rdfs:label "Nitrite-N - steam distillation" ;
  skos:broader <http://anzsoil.org/def/au/scma/7C1> ;
  skos:definition "Nitrite-N - steam distillation" ;
  skos:inScheme <http://anzsoil.org/def/au/scma> ;
  skos:notation "7C1h" ;
  skos:prefLabel "Nitrite-N - steam distillation" ;
.
<http://anzsoil.org/def/au/scma/7C2>
  a skos:Concept ;
  a sosa:Procedure ;
  dcterms:description "Mineral-N 2 M KCl, automated colour|mineral nitrogen with 2M KCl - automated colour" ;
  dcterms:identifier "http://anzsoil.org/def/au/scma/7C2"^^xsd:anyURI ;
  dcterms:isReplacedBy <http://anzsoil.org/def/au/scma/7C2a> ;
  dcterms:isReplacedBy <http://anzsoil.org/def/au/scma/7C2b> ;
  dcterms:source "URN:ISBN:978-0-909605-68-1" ;
  rdfs:label "Mineral-N 2 M KCl, automated colour|mineral nitrogen with 2M KCl - automated colour" ;
  skos:definition "Mineral-N 2 M KCl, automated colour|mineral nitrogen with 2M KCl - automated colour" ;
  skos:inScheme <http://anzsoil.org/def/au/scma> ;
  skos:narrower <http://anzsoil.org/def/au/scma/7C2a> ;
  skos:narrower <http://anzsoil.org/def/au/scma/7C2b> ;
  skos:notation "7C2" ;
  skos:note "7C2 has been superseded by 7C2a and 7C2b in Soil Chemical Methods Australasia, Rayment G.E. and Lyons D.J. ISBN 9780643101364" ;
  skos:prefLabel "Mineral-N 2 M KCl, automated colour|mineral nitrogen with 2M KCl - automated colour" ;
  skos:topConceptOf <http://anzsoil.org/def/au/scma> ;
.
<http://anzsoil.org/def/au/scma/7C2a>
  a skos:Concept ;
  a sosa:Procedure ;
  dcterms:description "Mineral-N 2 M KCl, automated colour, continuous segmented flow" ;
  dcterms:identifier "http://anzsoil.org/def/au/scma/7C2a"^^xsd:anyURI ;
  dcterms:source "URN:ISBN:978-0-643-10218-7" ;
  rdfs:label "Mineral-N 2 M KCl, automated colour, continuous segmented flow" ;
  skos:broader <http://anzsoil.org/def/au/scma/7C2> ;
  skos:definition "Mineral-N 2 M KCl, automated colour, continuous segmented flow" ;
  skos:inScheme <http://anzsoil.org/def/au/scma> ;
  skos:notation "7C2a" ;
  skos:prefLabel "Mineral-N 2 M KCl, automated colour, continuous segmented flow" ;
.
<http://anzsoil.org/def/au/scma/7C2b>
  a skos:Concept ;
  a sosa:Procedure ;
  dcterms:description "Mineral-N - 2 M KCl, automated colour, FIA" ;
  dcterms:identifier "http://anzsoil.org/def/au/scma/7C2b"^^xsd:anyURI ;
  dcterms:source "URN:ISBN:978-0-643-10218-7" ;
  rdfs:label "Mineral-N - 2 M KCl, automated colour, FIA" ;
  skos:broader <http://anzsoil.org/def/au/scma/7C2> ;
  skos:definition "Mineral-N - 2 M KCl, automated colour, FIA" ;
  skos:inScheme <http://anzsoil.org/def/au/scma> ;
  skos:notation "7C2b" ;
  skos:prefLabel "Mineral-N - 2 M KCl, automated colour, FIA" ;
.
<http://anzsoil.org/def/au/scma/7D>
  a skos:Concept ;
  a sosa:Procedure ;
  dcterms:description "Potentially mineralisable N (PMN)" ;
  dcterms:identifier "http://anzsoil.org/def/au/scma/7D"^^xsd:anyURI ;
  dcterms:source "URN:ISBN:978-0-643-10218-7" ;
  rdfs:label "Potentially mineralisable N (PMN)" ;
  skos:definition "Potentially mineralisable N (PMN)" ;
  skos:inScheme <http://anzsoil.org/def/au/scma> ;
  skos:narrower <http://anzsoil.org/def/au/scma/7D1a> ;
  skos:narrower <http://anzsoil.org/def/au/scma/7D1b> ;
  skos:narrower <http://anzsoil.org/def/au/scma/7D1c> ;
  skos:narrower <http://anzsoil.org/def/au/scma/7D2a> ;
  skos:narrower <http://anzsoil.org/def/au/scma/7D2b> ;
  skos:notation "7D" ;
  skos:prefLabel "Potentially mineralisable N (PMN)" ;
  skos:topConceptOf <http://anzsoil.org/def/au/scma> ;
.
<http://anzsoil.org/def/au/scma/7D1a>
  a skos:Concept ;
  a sosa:Procedure ;
  dcterms:description "Potentially mineralisable N, hot-KCl extraction (PMN KCl) - automated colour, continuous segmented flow" ;
  dcterms:identifier "http://anzsoil.org/def/au/scma/7D1a"^^xsd:anyURI ;
  dcterms:source "URN:ISBN:978-0-643-10218-7" ;
  rdfs:label "Potentially mineralisable N, hot-KCl extraction (PMN KCl) - automated colour, continuous segmented flow" ;
  skos:broader <http://anzsoil.org/def/au/scma/7D> ;
  skos:definition "Potentially mineralisable N, hot-KCl extraction (PMN KCl) - automated colour, continuous segmented flow" ;
  skos:inScheme <http://anzsoil.org/def/au/scma> ;
  skos:notation "7D1a" ;
  skos:prefLabel "Potentially mineralisable N, hot-KCl extraction (PMN KCl) - automated colour, continuous segmented flow" ;
.
<http://anzsoil.org/def/au/scma/7D1b>
  a skos:Concept ;
  a sosa:Procedure ;
  dcterms:description "Potentially mineralisable N, hot-KCl extraction (PMN KCl) - automated colour, FIA" ;
  dcterms:identifier "http://anzsoil.org/def/au/scma/7D1b"^^xsd:anyURI ;
  dcterms:source "URN:ISBN:978-0-643-10218-7" ;
  rdfs:label "Potentially mineralisable N, hot-KCl extraction (PMN KCl) - automated colour, FIA" ;
  skos:broader <http://anzsoil.org/def/au/scma/7D> ;
  skos:definition "Potentially mineralisable N, hot-KCl extraction (PMN KCl) - automated colour, FIA" ;
  skos:inScheme <http://anzsoil.org/def/au/scma> ;
  skos:notation "7D1b" ;
  skos:prefLabel "Potentially mineralisable N, hot-KCl extraction (PMN KCl) - automated colour, FIA" ;
.
<http://anzsoil.org/def/au/scma/7D1c>
  a skos:Concept ;
  a sosa:Procedure ;
  dcterms:description "Potentially mineralisable N, hot-KCl extraction (PMN KCl) - NIR diffuse reflectance spectroscopy" ;
  dcterms:identifier "http://anzsoil.org/def/au/scma/7D1c"^^xsd:anyURI ;
  dcterms:source "URN:ISBN:978-0-643-10218-7" ;
  rdfs:label "Potentially mineralisable N, hot-KCl extraction (PMN KCl) - NIR diffuse reflectance spectroscopy" ;
  skos:broader <http://anzsoil.org/def/au/scma/7D> ;
  skos:definition "Potentially mineralisable N, hot-KCl extraction (PMN KCl) - NIR diffuse reflectance spectroscopy" ;
  skos:inScheme <http://anzsoil.org/def/au/scma> ;
  skos:notation "7D1c" ;
  skos:prefLabel "Potentially mineralisable N, hot-KCl extraction (PMN KCl) - NIR diffuse reflectance spectroscopy" ;
.
<http://anzsoil.org/def/au/scma/7D2a>
  a skos:Concept ;
  a sosa:Procedure ;
  dcterms:description "Potentially mineralisable N, anaerobic incubation - automated colour, continuous segmented flow" ;
  dcterms:identifier "http://anzsoil.org/def/au/scma/7D2a"^^xsd:anyURI ;
  dcterms:source "URN:ISBN:978-0-643-10218-7" ;
  rdfs:label "Potentially mineralisable N, anaerobic incubation - automated colour, continuous segmented flow" ;
  skos:broader <http://anzsoil.org/def/au/scma/7D> ;
  skos:definition "Potentially mineralisable N, anaerobic incubation - automated colour, continuous segmented flow" ;
  skos:inScheme <http://anzsoil.org/def/au/scma> ;
  skos:notation "7D2a" ;
  skos:prefLabel "Potentially mineralisable N, anaerobic incubation - automated colour, continuous segmented flow" ;
.
<http://anzsoil.org/def/au/scma/7D2b>
  a skos:Concept ;
  a sosa:Procedure ;
  dcterms:description "Potentially mineralisable N, anaerobic incubation - automated colour, FIA" ;
  dcterms:identifier "http://anzsoil.org/def/au/scma/7D2b"^^xsd:anyURI ;
  dcterms:source "URN:ISBN:978-0-643-10218-7" ;
  rdfs:label "Potentially mineralisable N, anaerobic incubation - automated colour, FIA" ;
  skos:broader <http://anzsoil.org/def/au/scma/7D> ;
  skos:definition "Potentially mineralisable N, anaerobic incubation - automated colour, FIA" ;
  skos:inScheme <http://anzsoil.org/def/au/scma> ;
  skos:notation "7D2b" ;
  skos:prefLabel "Potentially mineralisable N, anaerobic incubation - automated colour, FIA" ;
.
<http://anzsoil.org/def/au/scma/8>
  a skos:Collection ;
  dcterms:description "Carbon/nitrogen ratio" ;
  dcterms:identifier "http://anzsoil.org/def/au/scma/8"^^xsd:anyURI ;
  dcterms:source "URN:ISBN:978-0-643-10218-7" ;
  ui:topMemberOf <http://anzsoil.org/def/au/scma> ;
  rdfs:label "Carbon/nitrogen ratio" ;
  skos:definition "Carbon/nitrogen ratio" ;
  skos:inScheme <http://anzsoil.org/def/au/scma> ;
  skos:member <http://anzsoil.org/def/au/scma/8A1> ;
  skos:member <http://anzsoil.org/def/au/scma/8B1> ;
  skos:notation "8" ;
  skos:prefLabel "Carbon/nitrogen ratio" ;
.
<http://anzsoil.org/def/au/scma/8A1>
  a skos:Concept ;
  a sosa:Procedure ;
  dcterms:description "Total organic carbon/total nitrogen ratio" ;
  dcterms:identifier "http://anzsoil.org/def/au/scma/8A1"^^xsd:anyURI ;
  dcterms:source "URN:ISBN:978-0-643-10218-7" ;
  rdfs:label "Total organic carbon/total nitrogen ratio" ;
  skos:definition "Total organic carbon/total nitrogen ratio" ;
  skos:inScheme <http://anzsoil.org/def/au/scma> ;
  skos:notation "8A1" ;
  skos:prefLabel "Total organic carbon/total nitrogen ratio" ;
  skos:topConceptOf <http://anzsoil.org/def/au/scma> ;
.
<http://anzsoil.org/def/au/scma/8B1>
  a skos:Concept ;
  a sosa:Procedure ;
  dcterms:description "Organic carbon - W&B/total nitrogen ratio" ;
  dcterms:identifier "http://anzsoil.org/def/au/scma/8B1"^^xsd:anyURI ;
  dcterms:source "URN:ISBN:978-0-643-10218-7" ;
  rdfs:label "Organic carbon - W&B/total nitrogen ratio" ;
  skos:definition "Organic carbon - W&B/total nitrogen ratio" ;
  skos:inScheme <http://anzsoil.org/def/au/scma> ;
  skos:notation "8B1" ;
  skos:prefLabel "Organic carbon - W&B/total nitrogen ratio" ;
  skos:topConceptOf <http://anzsoil.org/def/au/scma> ;
.
<http://anzsoil.org/def/au/scma/9>
  a skos:Collection ;
  dcterms:identifier "http://anzsoil.org/def/au/scma/9"^^xsd:anyURI ;
  dcterms:source "URN:ISBN:978-0-643-10218-7" ;
  ui:topMemberOf <http://anzsoil.org/def/au/scma> ;
  rdfs:label "Phosphorus" ;
  skos:definition <https://raw.githack.com/ANZSoilData/def-au-scma/master/html/9-P/9.html> ;
  skos:inScheme <http://anzsoil.org/def/au/scma> ;
  skos:member <http://anzsoil.org/def/au/scma/9A> ;
  skos:member <http://anzsoil.org/def/au/scma/9B> ;
  skos:member <http://anzsoil.org/def/au/scma/9C> ;
  skos:member <http://anzsoil.org/def/au/scma/9D1> ;
  skos:member <http://anzsoil.org/def/au/scma/9E> ;
  skos:member <http://anzsoil.org/def/au/scma/9F1> ;
  skos:member <http://anzsoil.org/def/au/scma/9F2> ;
  skos:member <http://anzsoil.org/def/au/scma/9G1> ;
  skos:member <http://anzsoil.org/def/au/scma/9G2> ;
  skos:member <http://anzsoil.org/def/au/scma/9H1> ;
  skos:member <http://anzsoil.org/def/au/scma/9I> ;
  skos:member <http://anzsoil.org/def/au/scma/9J> ;
  skos:member <http://anzsoil.org/def/au/scma/9K> ;
  skos:notation "9" ;
  skos:prefLabel "Phosphorus" ;
.
<http://anzsoil.org/def/au/scma/9A>
  a skos:Concept ;
  a sosa:Procedure ;
  dcterms:description "Total P" ;
  dcterms:identifier "http://anzsoil.org/def/au/scma/9A"^^xsd:anyURI ;
  dcterms:source "URN:ISBN:978-0-643-10218-7" ;
  rdfs:label "Total P" ;
  skos:definition <https://raw.githack.com/ANZSoilData/def-au-scma/master/html/9-P/9A.html> ;
  skos:inScheme <http://anzsoil.org/def/au/scma> ;
  skos:narrower <http://anzsoil.org/def/au/scma/9A1> ;
  skos:narrower <http://anzsoil.org/def/au/scma/9A2> ;
  skos:narrower <http://anzsoil.org/def/au/scma/9A3a> ;
  skos:narrower <http://anzsoil.org/def/au/scma/9A3b> ;
  skos:notation "9A" ;
  skos:prefLabel "Total P" ;
  skos:topConceptOf <http://anzsoil.org/def/au/scma> ;
.
<http://anzsoil.org/def/au/scma/9A1>
  a skos:Concept ;
  a sosa:Procedure ;
  dcterms:description "Total P - X-ray fluorescence" ;
  dcterms:identifier "http://anzsoil.org/def/au/scma/9A1"^^xsd:anyURI ;
  dcterms:source "URN:ISBN:978-0-643-10218-7" ;
  rdfs:label "Total P - X-ray fluorescence" ;
  skos:broader <http://anzsoil.org/def/au/scma/9A> ;
  skos:definition <https://raw.githack.com/ANZSoilData/def-au-scma/master/html/9-P/9A1.html> ;
  skos:inScheme <http://anzsoil.org/def/au/scma> ;
  skos:notation "9A1" ;
  skos:prefLabel "Total P - X-ray fluorescence" ;
.
<http://anzsoil.org/def/au/scma/9A2>
  a skos:Concept ;
  a sosa:Procedure ;
  dcterms:description "Total P - sodium carbonate fusion" ;
  dcterms:identifier "http://anzsoil.org/def/au/scma/9A2"^^xsd:anyURI ;
  dcterms:source "URN:ISBN:978-0-643-10218-7" ;
  rdfs:label "Total P - sodium carbonate fusion" ;
  skos:broader <http://anzsoil.org/def/au/scma/9A> ;
  skos:definition <https://raw.githack.com/ANZSoilData/def-au-scma/master/html/9-P/9A2.html> ;
  skos:inScheme <http://anzsoil.org/def/au/scma> ;
  skos:notation "9A2" ;
  skos:prefLabel "Total P - sodium carbonate fusion" ;
.
<http://anzsoil.org/def/au/scma/9A3a>
  a skos:Concept ;
  a sosa:Procedure ;
  dcterms:description "Kjeldahl P (KP) - automated colour, FIA/continuous segmented flow" ;
  dcterms:identifier "http://anzsoil.org/def/au/scma/9A3a"^^xsd:anyURI ;
  dcterms:source "URN:ISBN:978-0-643-10218-7" ;
  rdfs:label "Kjeldahl P (KP) - automated colour, FIA/continuous segmented flow" ;
  skos:broader <http://anzsoil.org/def/au/scma/9A> ;
  skos:definition <https://raw.githack.com/ANZSoilData/def-au-scma/master/html/9-P/9A3a.html> ;
  skos:inScheme <http://anzsoil.org/def/au/scma> ;
  skos:notation "9A3a" ;
  skos:prefLabel "Kjeldahl P (KP) - automated colour, FIA/continuous segmented flow" ;
.
<http://anzsoil.org/def/au/scma/9A3b>
  a skos:Concept ;
  a sosa:Procedure ;
  dcterms:description "Kjeldahl P (KP) - ICPAES" ;
  dcterms:identifier "http://anzsoil.org/def/au/scma/9A3b"^^xsd:anyURI ;
  dcterms:source "URN:ISBN:978-0-643-10218-7" ;
  rdfs:label "Kjeldahl P (KP) - ICPAES" ;
  skos:broader <http://anzsoil.org/def/au/scma/9A> ;
  skos:definition <https://raw.githack.com/ANZSoilData/def-au-scma/master/html/9-P/9A3b.html> ;
  skos:inScheme <http://anzsoil.org/def/au/scma> ;
  skos:notation "9A3b" ;
  skos:prefLabel "Kjeldahl P (KP) - ICPAES" ;
.
<http://anzsoil.org/def/au/scma/9B>
  a skos:Concept ;
  a sosa:Procedure ;
  dcterms:description "Bicarbonate-extractable P (Colwell-P)" ;
  dcterms:identifier "http://anzsoil.org/def/au/scma/9B"^^xsd:anyURI ;
  dcterms:source "URN:ISBN:978-0-643-10218-7" ;
  rdfs:label "Bicarbonate-extractable P (Colwell-P)" ;
  skos:definition <https://raw.githack.com/ANZSoilData/def-au-scma/master/html/9-P/9B.html> ;
  skos:inScheme <http://anzsoil.org/def/au/scma> ;
  skos:narrower <http://anzsoil.org/def/au/scma/9B1> ;
  skos:narrower <http://anzsoil.org/def/au/scma/9B2> ;
  skos:notation "9B" ;
  skos:prefLabel "Bicarbonate-extractable P (Colwell-P)" ;
  skos:topConceptOf <http://anzsoil.org/def/au/scma> ;
.
<http://anzsoil.org/def/au/scma/9B1>
  a skos:Concept ;
  a sosa:Procedure ;
  dcterms:description "Bicarbonate-extractable P (Colwell-P) - manual colour" ;
  dcterms:identifier "http://anzsoil.org/def/au/scma/9B1"^^xsd:anyURI ;
  dcterms:source "URN:ISBN:978-0-643-10218-7" ;
  rdfs:label "Bicarbonate-extractable P (Colwell-P) - manual colour" ;
  skos:broader <http://anzsoil.org/def/au/scma/9B> ;
  skos:definition <https://raw.githack.com/ANZSoilData/def-au-scma/master/html/9-P/9B1.html> ;
  skos:inScheme <http://anzsoil.org/def/au/scma> ;
  skos:notation "9B1" ;
  skos:prefLabel "Bicarbonate-extractable P (Colwell-P) - manual colour" ;
.
<http://anzsoil.org/def/au/scma/9B2>
  a skos:Concept ;
  a sosa:Procedure ;
  dcterms:description "Bicarbonate-extractable P (Colwell-P) - automated colour, continuous segmented flow/FIA" ;
  dcterms:identifier "http://anzsoil.org/def/au/scma/9B2"^^xsd:anyURI ;
  dcterms:source "URN:ISBN:978-0-643-10218-7" ;
  rdfs:label "Bicarbonate-extractable P (Colwell-P) - automated colour, continuous segmented flow/FIA" ;
  skos:broader <http://anzsoil.org/def/au/scma/9B> ;
  skos:definition <https://raw.githack.com/ANZSoilData/def-au-scma/master/html/9-P/9B2.html> ;
  skos:inScheme <http://anzsoil.org/def/au/scma> ;
  skos:notation "9B2" ;
  skos:prefLabel "Bicarbonate-extractable P (Colwell-P) - automated colour, continuous segmented flow/FIA" ;
.
<http://anzsoil.org/def/au/scma/9C>
  a skos:Concept ;
  a sosa:Procedure ;
  dcterms:description "Olsen-extractable P (Olsen-P)" ;
  dcterms:identifier "http://anzsoil.org/def/au/scma/9C"^^xsd:anyURI ;
  dcterms:source "URN:ISBN:978-0-643-10218-7" ;
  rdfs:label "Olsen-extractable P (Olsen-P)" ;
  skos:definition <https://raw.githack.com/ANZSoilData/def-au-scma/master/html/9-P/9C.html> ;
  skos:inScheme <http://anzsoil.org/def/au/scma> ;
  skos:narrower <http://anzsoil.org/def/au/scma/9C1> ;
  skos:narrower <http://anzsoil.org/def/au/scma/9C2> ;
  skos:notation "9C" ;
  skos:prefLabel "Olsen-extractable P (Olsen-P)" ;
  skos:topConceptOf <http://anzsoil.org/def/au/scma> ;
.
<http://anzsoil.org/def/au/scma/9C1>
  a skos:Concept ;
  a sosa:Procedure ;
  dcterms:description "Olsen-extractable P (Olsen-P) - manual colour" ;
  dcterms:identifier "http://anzsoil.org/def/au/scma/9C1"^^xsd:anyURI ;
  dcterms:source "URN:ISBN:978-0-643-10218-7" ;
  rdfs:label "Olsen-extractable P (Olsen-P) - manual colour" ;
  skos:broader <http://anzsoil.org/def/au/scma/9C> ;
  skos:definition <https://raw.githack.com/ANZSoilData/def-au-scma/master/html/9-P/9C1.html> ;
  skos:inScheme <http://anzsoil.org/def/au/scma> ;
  skos:notation "9C1" ;
  skos:prefLabel "Olsen-extractable P (Olsen-P) - manual colour" ;
.
<http://anzsoil.org/def/au/scma/9C2>
  a skos:Concept ;
  a sosa:Procedure ;
  dcterms:description "Olsen-extractable phosphorus - automated colour|Olsen-extractable P (Olsen-P) - automated colour" ;
  dcterms:identifier "http://anzsoil.org/def/au/scma/9C2"^^xsd:anyURI ;
  dcterms:isReplacedBy <http://anzsoil.org/def/au/scma/9C2a> ;
  dcterms:isReplacedBy <http://anzsoil.org/def/au/scma/9C2b> ;
  dcterms:source "URN:ISBN:978-0-909605-68-1" ;
  rdfs:label "Olsen-extractable phosphorus - automated colour|Olsen-extractable P (Olsen-P) - automated colour" ;
  skos:broader <http://anzsoil.org/def/au/scma/9C> ;
  skos:definition <https://raw.githack.com/ANZSoilData/def-au-scma/master/html/9-P/9C2.html> ;
  skos:inScheme <http://anzsoil.org/def/au/scma> ;
  skos:narrower <http://anzsoil.org/def/au/scma/9C2a> ;
  skos:narrower <http://anzsoil.org/def/au/scma/9C2b> ;
  skos:notation "9C2" ;
  skos:note "9C2 has been superseded by 9C2a and 9C2b in Soil Chemical Methods Australasia, Rayment G.E. and Lyons D.J. ISBN 9780643101364" ;
  skos:prefLabel "Olsen-extractable phosphorus - automated colour|Olsen-extractable P (Olsen-P) - automated colour" ;
.
<http://anzsoil.org/def/au/scma/9C2a>
  a skos:Concept ;
  a sosa:Procedure ;
  dcterms:description "Olsen-extractable P (Olsen-P) - automated colour, continuous segmented flow" ;
  dcterms:identifier "http://anzsoil.org/def/au/scma/9C2a"^^xsd:anyURI ;
  dcterms:source "URN:ISBN:978-0-643-10218-7" ;
  rdfs:label "Olsen-extractable P (Olsen-P) - automated colour, continuous segmented flow" ;
  skos:broader <http://anzsoil.org/def/au/scma/9C2> ;
  skos:definition <https://raw.githack.com/ANZSoilData/def-au-scma/master/html/9-P/9C2a.html> ;
  skos:inScheme <http://anzsoil.org/def/au/scma> ;
  skos:notation "9C2a" ;
  skos:prefLabel "Olsen-extractable P (Olsen-P) - automated colour, continuous segmented flow" ;
.
<http://anzsoil.org/def/au/scma/9C2b>
  a skos:Concept ;
  a sosa:Procedure ;
  dcterms:description "Olsen-extractable P (Olsen-P) - automated colour/FIA" ;
  dcterms:identifier "http://anzsoil.org/def/au/scma/9C2b"^^xsd:anyURI ;
  dcterms:source "URN:ISBN:978-0-643-10218-7" ;
  rdfs:label "Olsen-extractable P (Olsen-P) - automated colour/FIA" ;
  skos:broader <http://anzsoil.org/def/au/scma/9C2> ;
  skos:definition <https://raw.githack.com/ANZSoilData/def-au-scma/master/html/9-P/9C2b.html> ;
  skos:inScheme <http://anzsoil.org/def/au/scma> ;
  skos:notation "9C2b" ;
  skos:prefLabel "Olsen-extractable P (Olsen-P) - automated colour/FIA" ;
.
<http://anzsoil.org/def/au/scma/9D1>
  a skos:Concept ;
  a sosa:Procedure ;
  dcterms:description "Lactate-extractable P (Lactate-P) - manual colour" ;
  dcterms:identifier "http://anzsoil.org/def/au/scma/9D1"^^xsd:anyURI ;
  dcterms:source "URN:ISBN:978-0-643-10218-7" ;
  rdfs:label "Lactate-extractable P (Lactate-P) - manual colour" ;
  skos:definition <https://raw.githack.com/ANZSoilData/def-au-scma/master/html/9-P/9D1.html> ;
  skos:inScheme <http://anzsoil.org/def/au/scma> ;
  skos:notation "9D1" ;
  skos:prefLabel "Lactate-extractable P (Lactate-P) - manual colour" ;
  skos:topConceptOf <http://anzsoil.org/def/au/scma> ;
.
<http://anzsoil.org/def/au/scma/9E>
  a skos:Concept ;
  a sosa:Procedure ;
  dcterms:description "Fluoride-extractable P (Bray-1 P)" ;
  dcterms:identifier "http://anzsoil.org/def/au/scma/9E"^^xsd:anyURI ;
  dcterms:source "URN:ISBN:978-0-643-10218-7" ;
  rdfs:label "Fluoride-extractable P (Bray-1 P)" ;
  skos:definition <https://raw.githack.com/ANZSoilData/def-au-scma/master/html/9-P/9E.html> ;
  skos:inScheme <http://anzsoil.org/def/au/scma> ;
  skos:narrower <http://anzsoil.org/def/au/scma/9E1> ;
  skos:narrower <http://anzsoil.org/def/au/scma/9E2> ;
  skos:notation "9E" ;
  skos:prefLabel "Fluoride-extractable P (Bray-1 P)" ;
  skos:topConceptOf <http://anzsoil.org/def/au/scma> ;
.
<http://anzsoil.org/def/au/scma/9E1>
  a skos:Concept ;
  a sosa:Procedure ;
  dcterms:description "Fluoride-extractable P (Bray-1 P) - manual colour" ;
  dcterms:identifier "http://anzsoil.org/def/au/scma/9E1"^^xsd:anyURI ;
  dcterms:source "URN:ISBN:978-0-643-10218-7" ;
  rdfs:label "Fluoride-extractable P (Bray-1 P) - manual colour" ;
  skos:broader <http://anzsoil.org/def/au/scma/9E> ;
  skos:definition <https://raw.githack.com/ANZSoilData/def-au-scma/master/html/9-P/9E1.html> ;
  skos:inScheme <http://anzsoil.org/def/au/scma> ;
  skos:notation "9E1" ;
  skos:prefLabel "Fluoride-extractable P (Bray-1 P) - manual colour" ;
.
<http://anzsoil.org/def/au/scma/9E2>
  a skos:Concept ;
  a sosa:Procedure ;
  dcterms:description "Fluoride-extractable P (Bray-1 P) - continuous segmented flow/FIA automated colour" ;
  dcterms:identifier "http://anzsoil.org/def/au/scma/9E2"^^xsd:anyURI ;
  dcterms:source "URN:ISBN:978-0-643-10218-7" ;
  rdfs:label "Fluoride-extractable P (Bray-1 P) - continuous segmented flow/FIA automated colour" ;
  skos:broader <http://anzsoil.org/def/au/scma/9E> ;
  skos:definition <https://raw.githack.com/ANZSoilData/def-au-scma/master/html/9-P/9E2.html> ;
  skos:inScheme <http://anzsoil.org/def/au/scma> ;
  skos:notation "9E2" ;
  skos:prefLabel "Fluoride-extractable P (Bray-1 P) - continuous segmented flow/FIA automated colour" ;
.
<http://anzsoil.org/def/au/scma/9F1>
  a skos:Concept ;
  a sosa:Procedure ;
  dcterms:description "Calcium chloride-extractable P - manual colour" ;
  dcterms:identifier "http://anzsoil.org/def/au/scma/9F1"^^xsd:anyURI ;
  dcterms:source "URN:ISBN:978-0-643-10218-7" ;
  rdfs:label "Calcium chloride-extractable P - manual colour" ;
  skos:definition <https://raw.githack.com/ANZSoilData/def-au-scma/master/html/9-P/9F1.html> ;
  skos:inScheme <http://anzsoil.org/def/au/scma> ;
  skos:notation "9F1" ;
  skos:prefLabel "Calcium chloride-extractable P - manual colour" ;
  skos:topConceptOf <http://anzsoil.org/def/au/scma> ;
.
<http://anzsoil.org/def/au/scma/9F2>
  a skos:Concept ;
  a sosa:Procedure ;
  dcterms:description "Calcium chloride-extractable P - continuous segmented flow/FIA automated colour" ;
  dcterms:identifier "http://anzsoil.org/def/au/scma/9F2"^^xsd:anyURI ;
  dcterms:source "URN:ISBN:978-0-643-10218-7" ;
  rdfs:label "Calcium chloride-extractable P - continuous segmented flow/FIA automated colour" ;
  skos:definition <https://raw.githack.com/ANZSoilData/def-au-scma/master/html/9-P/9F2.html> ;
  skos:inScheme <http://anzsoil.org/def/au/scma> ;
  skos:notation "9F2" ;
  skos:prefLabel "Calcium chloride-extractable P - continuous segmented flow/FIA automated colour" ;
  skos:topConceptOf <http://anzsoil.org/def/au/scma> ;
.
<http://anzsoil.org/def/au/scma/9G1>
  a skos:Concept ;
  a sosa:Procedure ;
  dcterms:description "Acid-extractable P (BSES-P) - manual colour" ;
  dcterms:identifier "http://anzsoil.org/def/au/scma/9G1"^^xsd:anyURI ;
  dcterms:source "URN:ISBN:978-0-643-10218-7" ;
  rdfs:label "Acid-extractable P (BSES-P) - manual colour" ;
  skos:definition <https://raw.githack.com/ANZSoilData/def-au-scma/master/html/9-P/9G1.html> ;
  skos:inScheme <http://anzsoil.org/def/au/scma> ;
  skos:notation "9G1" ;
  skos:prefLabel "Acid-extractable P (BSES-P) - manual colour" ;
  skos:topConceptOf <http://anzsoil.org/def/au/scma> ;
.
<http://anzsoil.org/def/au/scma/9G2>
  a skos:Concept ;
  a sosa:Procedure ;
  dcterms:description "Acid-extractable P (BSES-P) - continuous segmented flow/FIA automated colour" ;
  dcterms:identifier "http://anzsoil.org/def/au/scma/9G2"^^xsd:anyURI ;
  dcterms:source "URN:ISBN:978-0-643-10218-7" ;
  rdfs:label "Acid-extractable P (BSES-P) - continuous segmented flow/FIA automated colour" ;
  skos:definition <https://raw.githack.com/ANZSoilData/def-au-scma/master/html/9-P/9G2.html> ;
  skos:inScheme <http://anzsoil.org/def/au/scma> ;
  skos:notation "9G2" ;
  skos:prefLabel "Acid-extractable P (BSES-P) - continuous segmented flow/FIA automated colour" ;
  skos:topConceptOf <http://anzsoil.org/def/au/scma> ;
.
<http://anzsoil.org/def/au/scma/9H1>
  a skos:Concept ;
  a sosa:Procedure ;
  dcterms:description "Anion Storage Capacity (previously P Retention)" ;
  dcterms:identifier "http://anzsoil.org/def/au/scma/9H1"^^xsd:anyURI ;
  dcterms:source "URN:ISBN:978-0-643-10218-7" ;
  rdfs:label "Anion Storage Capacity (previously P Retention)" ;
  skos:definition <https://raw.githack.com/ANZSoilData/def-au-scma/master/html/9-P/9H1.html> ;
  skos:inScheme <http://anzsoil.org/def/au/scma> ;
  skos:notation "9H1" ;
  skos:prefLabel "Anion Storage Capacity (previously P Retention)" ;
  skos:topConceptOf <http://anzsoil.org/def/au/scma> ;
.
<http://anzsoil.org/def/au/scma/9I>
  a skos:Concept ;
  a sosa:Procedure ;
  dcterms:description "Phosphate Indices" ;
  dcterms:identifier "http://anzsoil.org/def/au/scma/9I"^^xsd:anyURI ;
  dcterms:source "URN:ISBN:978-0-643-10218-7" ;
  rdfs:label "Phosphate Indices" ;
  skos:definition <https://raw.githack.com/ANZSoilData/def-au-scma/master/html/9-P/9I.html> ;
  skos:inScheme <http://anzsoil.org/def/au/scma> ;
  skos:narrower <http://anzsoil.org/def/au/scma/9I1> ;
  skos:narrower <http://anzsoil.org/def/au/scma/9I2a> ;
  skos:narrower <http://anzsoil.org/def/au/scma/9I2b> ;
  skos:narrower <http://anzsoil.org/def/au/scma/9I2c> ;
  skos:narrower <http://anzsoil.org/def/au/scma/9I3a> ;
  skos:narrower <http://anzsoil.org/def/au/scma/9I3b> ;
  skos:narrower <http://anzsoil.org/def/au/scma/9I3c> ;
  skos:narrower <http://anzsoil.org/def/au/scma/9I4a> ;
  skos:narrower <http://anzsoil.org/def/au/scma/9I4b> ;
  skos:narrower <http://anzsoil.org/def/au/scma/9I4c> ;
  skos:notation "9I" ;
  skos:prefLabel "Phosphate Indices" ;
  skos:topConceptOf <http://anzsoil.org/def/au/scma> ;
.
<http://anzsoil.org/def/au/scma/9I1>
  a skos:Concept ;
  a sosa:Procedure ;
  dcterms:description "Phosphate Sorption Index" ;
  dcterms:identifier "http://anzsoil.org/def/au/scma/9I1"^^xsd:anyURI ;
  dcterms:source "URN:ISBN:978-0-643-10218-7" ;
  rdfs:label "Phosphate Sorption Index" ;
  skos:broader <http://anzsoil.org/def/au/scma/9I> ;
  skos:definition <https://raw.githack.com/ANZSoilData/def-au-scma/master/html/9-P/9I1.html> ;
  skos:inScheme <http://anzsoil.org/def/au/scma> ;
  skos:notation "9I1" ;
  skos:prefLabel "Phosphate Sorption Index" ;
.
<http://anzsoil.org/def/au/scma/9I2a>
  a skos:Concept ;
  a sosa:Procedure ;
  dcterms:description "P buffer index - PBI (ColP) - Murphy and Riley|P buffer index - PBI (ColP)" ;
  dcterms:identifier "http://anzsoil.org/def/au/scma/9I2a"^^xsd:anyURI ;
  dcterms:source "URN:ISBN:978-0-643-10218-7" ;
  rdfs:label "P buffer index - PBI (ColP) - Murphy and Riley|P buffer index - PBI (ColP)" ;
  skos:broader <http://anzsoil.org/def/au/scma/9I> ;
  skos:definition <https://raw.githack.com/ANZSoilData/def-au-scma/master/html/9-P/9I2a.html> ;
  skos:inScheme <http://anzsoil.org/def/au/scma> ;
  skos:notation "9I2a" ;
  skos:prefLabel "P buffer index - PBI (ColP) - Murphy and Riley|P buffer index - PBI (ColP)" ;
.
<http://anzsoil.org/def/au/scma/9I2b>
  a skos:Concept ;
  a sosa:Procedure ;
  dcterms:description "P buffer index - PBI (ColP)|P buffer index - PBI (ColP) - ICPAES" ;
  dcterms:identifier "http://anzsoil.org/def/au/scma/9I2b"^^xsd:anyURI ;
  dcterms:source "URN:ISBN:978-0-643-10218-7" ;
  rdfs:label "P buffer index - PBI (ColP)|P buffer index - PBI (ColP) - ICPAES" ;
  skos:broader <http://anzsoil.org/def/au/scma/9I> ;
  skos:definition <https://raw.githack.com/ANZSoilData/def-au-scma/master/html/9-P/9I2b.html> ;
  skos:inScheme <http://anzsoil.org/def/au/scma> ;
  skos:notation "9I2b" ;
  skos:prefLabel "P buffer index - PBI (ColP)|P buffer index - PBI (ColP) - ICPAES" ;
.
<http://anzsoil.org/def/au/scma/9I2c>
  a skos:Concept ;
  a sosa:Procedure ;
  dcterms:description "P buffer index - PBI (ColP)|P buffer index - PBI (ColP) - Vanadate" ;
  dcterms:identifier "http://anzsoil.org/def/au/scma/9I2c"^^xsd:anyURI ;
  dcterms:source "URN:ISBN:978-0-643-10218-7" ;
  rdfs:label "P buffer index - PBI (ColP)|P buffer index - PBI (ColP) - Vanadate" ;
  skos:broader <http://anzsoil.org/def/au/scma/9I> ;
  skos:definition <https://raw.githack.com/ANZSoilData/def-au-scma/master/html/9-P/9I2c.html> ;
  skos:inScheme <http://anzsoil.org/def/au/scma> ;
  skos:notation "9I2c" ;
  skos:prefLabel "P buffer index - PBI (ColP)|P buffer index - PBI (ColP) - Vanadate" ;
.
<http://anzsoil.org/def/au/scma/9I3a>
  a skos:Concept ;
  a sosa:Procedure ;
  dcterms:description "P buffer index - PBI (OlsenP)|P buffer index - PBI (OlsenP) - Murphy and Riley" ;
  dcterms:identifier "http://anzsoil.org/def/au/scma/9I3a"^^xsd:anyURI ;
  dcterms:source "URN:ISBN:978-0-643-10218-7" ;
  rdfs:label "P buffer index - PBI (OlsenP)|P buffer index - PBI (OlsenP) - Murphy and Riley" ;
  skos:broader <http://anzsoil.org/def/au/scma/9I> ;
  skos:definition <https://raw.githack.com/ANZSoilData/def-au-scma/master/html/9-P/9I3a.html> ;
  skos:inScheme <http://anzsoil.org/def/au/scma> ;
  skos:notation "9I3a" ;
  skos:prefLabel "P buffer index - PBI (OlsenP)|P buffer index - PBI (OlsenP) - Murphy and Riley" ;
.
<http://anzsoil.org/def/au/scma/9I3b>
  a skos:Concept ;
  a sosa:Procedure ;
  dcterms:description "P buffer index - PBI (OlsenP)|P buffer index - PBI (OlsenP) - ICPAES" ;
  dcterms:identifier "http://anzsoil.org/def/au/scma/9I3b"^^xsd:anyURI ;
  dcterms:source "URN:ISBN:978-0-643-10218-7" ;
  rdfs:label "P buffer index - PBI (OlsenP)|P buffer index - PBI (OlsenP) - ICPAES" ;
  skos:broader <http://anzsoil.org/def/au/scma/9I> ;
  skos:definition <https://raw.githack.com/ANZSoilData/def-au-scma/master/html/9-P/9I3b.html> ;
  skos:inScheme <http://anzsoil.org/def/au/scma> ;
  skos:notation "9I3b" ;
  skos:prefLabel "P buffer index - PBI (OlsenP)|P buffer index - PBI (OlsenP) - ICPAES" ;
.
<http://anzsoil.org/def/au/scma/9I3c>
  a skos:Concept ;
  a sosa:Procedure ;
  dcterms:description "P buffer index - PBI (OlsenP)|P buffer index - PBI (OlsenP) - Vanadate" ;
  dcterms:identifier "http://anzsoil.org/def/au/scma/9I3c"^^xsd:anyURI ;
  dcterms:source "URN:ISBN:978-0-643-10218-7" ;
  rdfs:label "P buffer index - PBI (OlsenP)|P buffer index - PBI (OlsenP) - Vanadate" ;
  skos:broader <http://anzsoil.org/def/au/scma/9I> ;
  skos:definition <https://raw.githack.com/ANZSoilData/def-au-scma/master/html/9-P/9I3c.html> ;
  skos:inScheme <http://anzsoil.org/def/au/scma> ;
  skos:notation "9I3c" ;
  skos:prefLabel "P buffer index - PBI (OlsenP)|P buffer index - PBI (OlsenP) - Vanadate" ;
.
<http://anzsoil.org/def/au/scma/9I4a>
  a skos:Concept ;
  a sosa:Procedure ;
  dcterms:description "P buffer index - PBI (unadj) - Murphy and Riley|P buffer index - PBI (unadj)" ;
  dcterms:identifier "http://anzsoil.org/def/au/scma/9I4a"^^xsd:anyURI ;
  dcterms:source "URN:ISBN:978-0-643-10218-7" ;
  rdfs:label "P buffer index - PBI (unadj) - Murphy and Riley|P buffer index - PBI (unadj)" ;
  skos:broader <http://anzsoil.org/def/au/scma/9I> ;
  skos:definition <https://raw.githack.com/ANZSoilData/def-au-scma/master/html/9-P/9I4a.html> ;
  skos:inScheme <http://anzsoil.org/def/au/scma> ;
  skos:notation "9I4a" ;
  skos:prefLabel "P buffer index - PBI (unadj) - Murphy and Riley|P buffer index - PBI (unadj)" ;
.
<http://anzsoil.org/def/au/scma/9I4b>
  a skos:Concept ;
  a sosa:Procedure ;
  dcterms:description "P buffer index - PBI (unadj) - ICPAES|P buffer index - PBI (unadj)" ;
  dcterms:identifier "http://anzsoil.org/def/au/scma/9I4b"^^xsd:anyURI ;
  dcterms:source "URN:ISBN:978-0-643-10218-7" ;
  rdfs:label "P buffer index - PBI (unadj) - ICPAES|P buffer index - PBI (unadj)" ;
  skos:broader <http://anzsoil.org/def/au/scma/9I> ;
  skos:definition <https://raw.githack.com/ANZSoilData/def-au-scma/master/html/9-P/9I4b.html> ;
  skos:inScheme <http://anzsoil.org/def/au/scma> ;
  skos:notation "9I4b" ;
  skos:prefLabel "P buffer index - PBI (unadj) - ICPAES|P buffer index - PBI (unadj)" ;
.
<http://anzsoil.org/def/au/scma/9I4c>
  a skos:Concept ;
  a sosa:Procedure ;
  dcterms:description "P buffer index - PBI (unadj)|P buffer index - PBI (unadj) - Vanadate" ;
  dcterms:identifier "http://anzsoil.org/def/au/scma/9I4c"^^xsd:anyURI ;
  dcterms:source "URN:ISBN:978-0-643-10218-7" ;
  rdfs:label "P buffer index - PBI (unadj)|P buffer index - PBI (unadj) - Vanadate" ;
  skos:broader <http://anzsoil.org/def/au/scma/9I> ;
  skos:definition <https://raw.githack.com/ANZSoilData/def-au-scma/master/html/9-P/9I4c.html> ;
  skos:inScheme <http://anzsoil.org/def/au/scma> ;
  skos:notation "9I4c" ;
  skos:prefLabel "P buffer index - PBI (unadj)|P buffer index - PBI (unadj) - Vanadate" ;
.
<http://anzsoil.org/def/au/scma/9J>
  a skos:Concept ;
  a sosa:Procedure ;
  dcterms:description "Phosphate sorption curve" ;
  dcterms:identifier "http://anzsoil.org/def/au/scma/9J"^^xsd:anyURI ;
  dcterms:source "URN:ISBN:978-0-643-10218-7" ;
  rdfs:label "Phosphate sorption curve" ;
  skos:definition <https://raw.githack.com/ANZSoilData/def-au-scma/master/html/9-P/9J.html> ;
  skos:inScheme <http://anzsoil.org/def/au/scma> ;
  skos:narrower <http://anzsoil.org/def/au/scma/9J1> ;
  skos:narrower <http://anzsoil.org/def/au/scma/9J2> ;
  skos:notation "9J" ;
  skos:prefLabel "Phosphate sorption curve" ;
  skos:topConceptOf <http://anzsoil.org/def/au/scma> ;
.
<http://anzsoil.org/def/au/scma/9J1>
  a skos:Concept ;
  a sosa:Procedure ;
  dcterms:description "Phosphate sorption curve - manual colour" ;
  dcterms:identifier "http://anzsoil.org/def/au/scma/9J1"^^xsd:anyURI ;
  dcterms:source "URN:ISBN:978-0-643-10218-7" ;
  rdfs:label "Phosphate sorption curve - manual colour" ;
  skos:broader <http://anzsoil.org/def/au/scma/9J> ;
  skos:definition <https://raw.githack.com/ANZSoilData/def-au-scma/master/html/9-P/9J1.html> ;
  skos:inScheme <http://anzsoil.org/def/au/scma> ;
  skos:notation "9J1" ;
  skos:prefLabel "Phosphate sorption curve - manual colour" ;
.
<http://anzsoil.org/def/au/scma/9J2>
  a skos:Concept ;
  a sosa:Procedure ;
  dcterms:description "Phosphate sorption curve - continuous segmented flow/FIA automated colour" ;
  dcterms:identifier "http://anzsoil.org/def/au/scma/9J2"^^xsd:anyURI ;
  dcterms:source "URN:ISBN:978-0-643-10218-7" ;
  rdfs:label "Phosphate sorption curve - continuous segmented flow/FIA automated colour" ;
  skos:broader <http://anzsoil.org/def/au/scma/9J> ;
  skos:definition <https://raw.githack.com/ANZSoilData/def-au-scma/master/html/9-P/9J2.html> ;
  skos:inScheme <http://anzsoil.org/def/au/scma> ;
  skos:notation "9J2" ;
  skos:prefLabel "Phosphate sorption curve - continuous segmented flow/FIA automated colour" ;
.
<http://anzsoil.org/def/au/scma/9K>
  a skos:Concept ;
  a sosa:Procedure ;
  dcterms:description "Environmental soil P tests" ;
  dcterms:identifier "http://anzsoil.org/def/au/scma/9K"^^xsd:anyURI ;
  dcterms:source "URN:ISBN:978-0-643-10218-7" ;
  rdfs:label "Environmental soil P tests" ;
  skos:definition <https://raw.githack.com/ANZSoilData/def-au-scma/master/html/9-P/9K.html> ;
  skos:inScheme <http://anzsoil.org/def/au/scma> ;
  skos:narrower <http://anzsoil.org/def/au/scma/9K1a> ;
  skos:narrower <http://anzsoil.org/def/au/scma/9K1b> ;
  skos:narrower <http://anzsoil.org/def/au/scma/9K2> ;
  skos:notation "9K" ;
  skos:prefLabel "Environmental soil P tests" ;
  skos:topConceptOf <http://anzsoil.org/def/au/scma> ;
.
<http://anzsoil.org/def/au/scma/9K1a>
  a skos:Concept ;
  a sosa:Procedure ;
  dcterms:description "Mehlich 3-P saturation ratio (M3PSR colour) [colormetric estimate of P]" ;
  dcterms:identifier "http://anzsoil.org/def/au/scma/9K1a"^^xsd:anyURI ;
  dcterms:source "URN:ISBN:978-0-643-10218-7" ;
  rdfs:label "Mehlich 3-P saturation ratio (M3PSR colour) [colormetric estimate of P]" ;
  skos:broader <http://anzsoil.org/def/au/scma/9K> ;
  skos:definition <https://raw.githack.com/ANZSoilData/def-au-scma/master/html/9-P/9K1a.html> ;
  skos:inScheme <http://anzsoil.org/def/au/scma> ;
  skos:notation "9K1a" ;
  skos:prefLabel "Mehlich 3-P saturation ratio (M3PSR colour) [colormetric estimate of P]" ;
.
<http://anzsoil.org/def/au/scma/9K1b>
  a skos:Concept ;
  a sosa:Procedure ;
  dcterms:description "Mehlich 3-P saturation ratio (M3PSR ICPAES) [ICPAES estimate of P]" ;
  dcterms:identifier "http://anzsoil.org/def/au/scma/9K1b"^^xsd:anyURI ;
  dcterms:source "URN:ISBN:978-0-643-10218-7" ;
  rdfs:label "Mehlich 3-P saturation ratio (M3PSR ICPAES) [ICPAES estimate of P]" ;
  skos:broader <http://anzsoil.org/def/au/scma/9K> ;
  skos:definition <https://raw.githack.com/ANZSoilData/def-au-scma/master/html/9-P/9K1b.html> ;
  skos:inScheme <http://anzsoil.org/def/au/scma> ;
  skos:notation "9K1b" ;
  skos:prefLabel "Mehlich 3-P saturation ratio (M3PSR ICPAES) [ICPAES estimate of P]" ;
.
<http://anzsoil.org/def/au/scma/9K2>
  a skos:Concept ;
  a sosa:Procedure ;
  dcterms:description "Colwell-P/PBI (ColP) ratio" ;
  dcterms:identifier "http://anzsoil.org/def/au/scma/9K2"^^xsd:anyURI ;
  dcterms:source "URN:ISBN:978-0-643-10218-7" ;
  rdfs:label "Colwell-P/PBI (ColP) ratio" ;
  skos:broader <http://anzsoil.org/def/au/scma/9K> ;
  skos:definition <https://raw.githack.com/ANZSoilData/def-au-scma/master/html/9-P/9K2.html> ;
  skos:inScheme <http://anzsoil.org/def/au/scma> ;
  skos:notation "9K2" ;
  skos:prefLabel "Colwell-P/PBI (ColP) ratio" ;
.
