# baseURI: http://anzsoil.org/def/au/scma/
# imports: http://purl.org/dc/elements/1.1/
# prefix: s

@prefix dc: <http://purl.org/dc/elements/1.1/> .
@prefix dcat: <http://www.w3.org/ns/dcat#> .
@prefix dct: <http://purl.org/dc/terms/> .
@prefix euvoc: <http://publications.europa.eu/ontology/euvoc#> .
@prefix foaf: <http://xmlns.com/foaf/0.1/> .
@prefix org: <http://www.w3.org/ns/org#> .
@prefix owl: <http://www.w3.org/2002/07/owl#> .
@prefix prov: <http://www.w3.org/ns/prov#> .
@prefix qb: <http://purl.org/linked-data/cube#> .
@prefix rdf: <http://www.w3.org/1999/02/22-rdf-syntax-ns#> .
@prefix rdfs: <http://www.w3.org/2000/01/rdf-schema#> .
@prefix s: <http://anzsoil.org/def/au/scma/> .
@prefix schema: <http://schema.org/> .
@prefix sdo: <https://schema.org/> .
@prefix sh: <http://www.w3.org/ns/shacl#> .
@prefix skos: <http://www.w3.org/2004/02/skos/core#> .
@prefix skosthes: <http://purl.org/iso25964/skos-thes#> .
@prefix skosxl: <http://www.w3.org/2008/05/skos-xl#> .
@prefix sosa: <http://www.w3.org/ns/sosa/> .
@prefix xsd: <http://www.w3.org/2001/XMLSchema#> .

s:
  a owl:Ontology ;
  owl:imports dc: ;
.
<http://anzsoil.org/def/au/scma/01>
  a skos:Collection ;
  dct:identifier "http://anzsoil.org/def/au/scma/01"^^xsd:anyURI ;
  dct:source "URN:ISBN:978-0-909605-68-1" ;
  skos:member <http://anzsoil.org/def/au/scma/01A1> ;
  skos:member <http://anzsoil.org/def/au/scma/01A2> ;
  skos:member <http://anzsoil.org/def/au/scma/01B1> ;
  skos:notation "01" ;
  skos:note "Retired in Soil Chemical Methods Australasia, Rayment G.E. and Lyons D.J. ISBN 9780643101364" ;
  skos:prefLabel "Sampling and Sample Preparation" ;
.
<http://anzsoil.org/def/au/scma/01A1>
  a skos:Concept ;
  a sosa:Procedure ;
  dct:identifier "http://anzsoil.org/def/au/scma/01A1"^^xsd:anyURI ;
  dct:source "URN:ISBN:978-0-909605-68-1" ;
  skos:inScheme s:swcm-1992 ;
  skos:notation "01A1" ;
  skos:prefLabel "Field sampling - soil and land use surveys" ;
  skos:topConceptOf s:swcm-1992 ;
.
<http://anzsoil.org/def/au/scma/01A2>
  a skos:Concept ;
  a sosa:Procedure ;
  dct:identifier "http://anzsoil.org/def/au/scma/01A2"^^xsd:anyURI ;
  dct:source "URN:ISBN:978-0-909605-68-1" ;
  skos:inScheme s:swcm-1992 ;
  skos:notation "01A2" ;
  skos:prefLabel "Field sampling - diagnostic" ;
  skos:topConceptOf s:swcm-1992 ;
.
<http://anzsoil.org/def/au/scma/01B1>
  a skos:Concept ;
  a sosa:Procedure ;
  dct:identifier "http://anzsoil.org/def/au/scma/01B1"^^xsd:anyURI ;
  dct:source "URN:ISBN:978-0-909605-68-1" ;
  skos:inScheme s:swcm-1992 ;
  skos:notation "01B1" ;
  skos:prefLabel "Laboratory preparation" ;
  skos:topConceptOf s:swcm-1992 ;
.
<http://anzsoil.org/def/au/scma/02>
  a skos:Collection ;
  dct:identifier "http://anzsoil.org/def/au/scma/02"^^xsd:anyURI ;
  dct:source "URN:ISBN:978-0-643-10218-7" ;
  skos:definition <https://raw.githack.com/ANZSoilData/def-au-scma/master/html/02/02.html> ;
  skos:member <http://anzsoil.org/def/au/scma/02A1> ;
  skos:member <http://anzsoil.org/def/au/scma/02B1> ;
  skos:member <http://anzsoil.org/def/au/scma/02C1> ;
  skos:member <http://anzsoil.org/def/au/scma/02D1> ;
  skos:notation "02" ;
  skos:prefLabel "Sampling, preparation and moisture content" ;
.
<http://anzsoil.org/def/au/scma/02A1>
  a skos:Concept ;
  a sosa:Procedure ;
  dct:identifier "http://anzsoil.org/def/au/scma/02A1"^^xsd:anyURI ;
  dct:source "URN:ISBN:978-0-643-10218-7" ;
  skos:definition <https://raw.githack.com/ANZSoilData/def-au-scma/master/html/02/02A1.html> ;
  skos:inScheme s:scma-2011 ;
  skos:inScheme s:swcm-1992 ;
  skos:notation "02A1" ;
  skos:prefLabel "Air-dry moisture content" ;
  skos:topConceptOf s:scma-2011 ;
  skos:topConceptOf s:swcm-1992 ;
.
<http://anzsoil.org/def/au/scma/02B1>
  a skos:Concept ;
  a sosa:Procedure ;
  dct:identifier "http://anzsoil.org/def/au/scma/02B1"^^xsd:anyURI ;
  dct:source "URN:ISBN:978-0-643-10218-7" ;
  skos:definition <https://raw.githack.com/ANZSoilData/def-au-scma/master/html/02/02B1.html> ;
  skos:inScheme s:scma-2011 ;
  skos:inScheme s:swcm-1992 ;
  skos:notation "02B1" ;
  skos:prefLabel "As received moisture content" ;
  skos:topConceptOf s:scma-2011 ;
  skos:topConceptOf s:swcm-1992 ;
.
<http://anzsoil.org/def/au/scma/02C1>
  a skos:Concept ;
  a sosa:Procedure ;
  dct:identifier "http://anzsoil.org/def/au/scma/02C1"^^xsd:anyURI ;
  dct:source "URN:ISBN:978-0-643-10218-7" ;
  skos:definition <https://raw.githack.com/ANZSoilData/def-au-scma/master/html/02/02C1.html> ;
  skos:inScheme s:scma-2011 ;
  skos:inScheme s:swcm-1992 ;
  skos:notation "02C1" ;
  skos:prefLabel "Moisture content - 10 mm tension" ;
  skos:topConceptOf s:scma-2011 ;
  skos:topConceptOf s:swcm-1992 ;
.
<http://anzsoil.org/def/au/scma/02D1>
  a skos:Concept ;
  a sosa:Procedure ;
  dct:identifier "http://anzsoil.org/def/au/scma/02D1"^^xsd:anyURI ;
  dct:source "URN:ISBN:978-0-643-10218-7" ;
  skos:definition <https://raw.githack.com/ANZSoilData/def-au-scma/master/html/02/02D1.html> ;
  skos:inScheme s:scma-2011 ;
  skos:inScheme s:swcm-1992 ;
  skos:notation "02D1" ;
  skos:prefLabel "Moisture content - approximate saturation paste" ;
  skos:topConceptOf s:scma-2011 ;
  skos:topConceptOf s:swcm-1992 ;
.
<http://anzsoil.org/def/au/scma/03>
  a skos:Collection ;
  dct:identifier "http://anzsoil.org/def/au/scma/03"^^xsd:anyURI ;
  dct:source "URN:ISBN:978-0-643-10218-7" ;
  skos:definition <https://raw.githack.com/ANZSoilData/def-au-scma/master/html/03/03.html> ;
  skos:member <http://anzsoil.org/def/au/scma/03A1> ;
  skos:member <http://anzsoil.org/def/au/scma/03B1> ;
  skos:member <http://anzsoil.org/def/au/scma/03C1> ;
  skos:member <http://anzsoil.org/def/au/scma/03D1> ;
  skos:notation "03" ;
  skos:prefLabel "Electrical conductivity, related attributes and redox potential" ;
.
<http://anzsoil.org/def/au/scma/03A1>
  a skos:Concept ;
  a sosa:Procedure ;
  dct:identifier "http://anzsoil.org/def/au/scma/03A1"^^xsd:anyURI ;
  dct:source "URN:ISBN:978-0-643-10218-7" ;
  skos:definition <https://raw.githack.com/ANZSoilData/def-au-scma/master/html/03/03A1.html> ;
  skos:inScheme s:scma-2011 ;
  skos:inScheme s:swcm-1992 ;
  skos:notation "03A1" ;
  skos:prefLabel "Electrical conductivity (EC) of 1:5 soil/water extract" ;
  skos:topConceptOf s:scma-2011 ;
  skos:topConceptOf s:swcm-1992 ;
.
<http://anzsoil.org/def/au/scma/03B1>
  a skos:Concept ;
  a sosa:Procedure ;
  dct:identifier "http://anzsoil.org/def/au/scma/03B1"^^xsd:anyURI ;
  dct:source "URN:ISBN:978-0-643-10218-7" ;
  skos:definition <https://raw.githack.com/ANZSoilData/def-au-scma/master/html/03/03B1.html> ;
  skos:inScheme s:scma-2011 ;
  skos:inScheme s:swcm-1992 ;
  skos:notation "03B1" ;
  skos:prefLabel "Estimated soluble salt concentration" ;
  skos:topConceptOf s:scma-2011 ;
  skos:topConceptOf s:swcm-1992 ;
.
<http://anzsoil.org/def/au/scma/03C1>
  a skos:Concept ;
  a sosa:Procedure ;
  dct:identifier "http://anzsoil.org/def/au/scma/03C1"^^xsd:anyURI ;
  dct:source "URN:ISBN:978-0-643-10218-7" ;
  skos:definition <https://raw.githack.com/ANZSoilData/def-au-scma/master/html/03/03C1.html> ;
  skos:inScheme s:scma-2011 ;
  skos:inScheme s:swcm-1992 ;
  skos:notation "03C1" ;
  skos:prefLabel "Estimated soil ionic strength" ;
  skos:topConceptOf s:scma-2011 ;
  skos:topConceptOf s:swcm-1992 ;
.
<http://anzsoil.org/def/au/scma/03D1>
  a skos:Concept ;
  a sosa:Procedure ;
  dct:identifier "http://anzsoil.org/def/au/scma/03D1"^^xsd:anyURI ;
  dct:source "URN:ISBN:978-0-643-10218-7" ;
  skos:definition <https://raw.githack.com/ANZSoilData/def-au-scma/master/html/03/03D1.html> ;
  skos:inScheme s:scma-2011 ;
  skos:inScheme s:swcm-1992 ;
  skos:notation "03D1" ;
  skos:prefLabel "Redox potential (Eh; field)" ;
  skos:topConceptOf s:scma-2011 ;
  skos:topConceptOf s:swcm-1992 ;
.
<http://anzsoil.org/def/au/scma/04>
  a skos:Collection ;
  dct:identifier "http://anzsoil.org/def/au/scma/04"^^xsd:anyURI ;
  dct:source "URN:ISBN:978-0-643-10218-7" ;
  skos:definition <https://raw.githack.com/ANZSoilData/def-au-scma/master/html/04-pH/04.html> ;
  skos:member <http://anzsoil.org/def/au/scma/04A1> ;
  skos:member <http://anzsoil.org/def/au/scma/04A2> ;
  skos:member <http://anzsoil.org/def/au/scma/04A3> ;
  skos:member <http://anzsoil.org/def/au/scma/04B1> ;
  skos:member <http://anzsoil.org/def/au/scma/04B2> ;
  skos:member <http://anzsoil.org/def/au/scma/04B3> ;
  skos:member <http://anzsoil.org/def/au/scma/04B4> ;
  skos:member <http://anzsoil.org/def/au/scma/04B5> ;
  skos:member <http://anzsoil.org/def/au/scma/04C1> ;
  skos:member <http://anzsoil.org/def/au/scma/04C2> ;
  skos:member <http://anzsoil.org/def/au/scma/04C3> ;
  skos:member <http://anzsoil.org/def/au/scma/04C4> ;
  skos:member <http://anzsoil.org/def/au/scma/04D1> ;
  skos:member <http://anzsoil.org/def/au/scma/04E1> ;
  skos:member <http://anzsoil.org/def/au/scma/04F1> ;
  skos:member <http://anzsoil.org/def/au/scma/04G1> ;
  skos:notation "04" ;
  skos:prefLabel "Soil pH" ;
.
<http://anzsoil.org/def/au/scma/04A1>
  a skos:Concept ;
  a sosa:Procedure ;
  dct:identifier "http://anzsoil.org/def/au/scma/04A1"^^xsd:anyURI ;
  dct:source "URN:ISBN:978-0-643-10218-7" ;
  skos:definition <https://raw.githack.com/ANZSoilData/def-au-scma/master/html/04-pH/04A1.html> ;
  skos:inScheme s:scma-2011 ;
  skos:inScheme s:swcm-1992 ;
  skos:notation "04A1" ;
  skos:prefLabel "pH of a 1:5 soil/water suspension" ;
  skos:topConceptOf s:scma-2011 ;
  skos:topConceptOf s:swcm-1992 ;
.
<http://anzsoil.org/def/au/scma/04A2>
  a skos:Concept ;
  a sosa:Procedure ;
  dct:identifier "http://anzsoil.org/def/au/scma/04A2"^^xsd:anyURI ;
  dct:source "URN:ISBN:978-0-643-10218-7" ;
  skos:definition <https://raw.githack.com/ANZSoilData/def-au-scma/master/html/04-pH/04A2.html> ;
  skos:inScheme s:scma-2011 ;
  skos:inScheme s:swcm-1992 ;
  skos:notation "04A2" ;
  skos:prefLabel "pH of a 1:1 soil/water suspension" ;
  skos:topConceptOf s:scma-2011 ;
  skos:topConceptOf s:swcm-1992 ;
.
<http://anzsoil.org/def/au/scma/04A3>
  a skos:Concept ;
  a sosa:Procedure ;
  dct:identifier "http://anzsoil.org/def/au/scma/04A3"^^xsd:anyURI ;
  dct:source "URN:ISBN:978-0-643-10218-7" ;
  skos:definition <https://raw.githack.com/ANZSoilData/def-au-scma/master/html/04-pH/04A3.html> ;
  skos:inScheme s:scma-2011 ;
  skos:inScheme s:swcm-1992 ;
  skos:notation "04A3" ;
  skos:prefLabel "pH of a 1:2.5 soil/water suspension" ;
  skos:topConceptOf s:scma-2011 ;
  skos:topConceptOf s:swcm-1992 ;
.
<http://anzsoil.org/def/au/scma/04B1>
  a skos:Concept ;
  a sosa:Procedure ;
  dct:identifier "http://anzsoil.org/def/au/scma/04B1"^^xsd:anyURI ;
  dct:source "URN:ISBN:978-0-643-10218-7" ;
  skos:definition <https://raw.githack.com/ANZSoilData/def-au-scma/master/html/04-pH/04B1.html> ;
  skos:inScheme s:scma-2011 ;
  skos:inScheme s:swcm-1992 ;
  skos:notation "04B1" ;
  skos:prefLabel "pH of 1:5 soil/0.01 M calcium chloride extract - direct (without stirring during measurement)" ;
  skos:topConceptOf s:scma-2011 ;
  skos:topConceptOf s:swcm-1992 ;
.
<http://anzsoil.org/def/au/scma/04B2>
  a skos:Concept ;
  a sosa:Procedure ;
  dct:identifier "http://anzsoil.org/def/au/scma/04B2"^^xsd:anyURI ;
  dct:source "URN:ISBN:978-0-643-10218-7" ;
  skos:definition <https://raw.githack.com/ANZSoilData/def-au-scma/master/html/04-pH/04B2.html> ;
  skos:inScheme s:scma-2011 ;
  skos:inScheme s:swcm-1992 ;
  skos:notation "04B2" ;
  skos:prefLabel "pH of 1:5 soil/0.01 M calcium chloride extract - following method 4A1 (without stirring during measurement)" ;
  skos:topConceptOf s:scma-2011 ;
  skos:topConceptOf s:swcm-1992 ;
.
<http://anzsoil.org/def/au/scma/04B3>
  a skos:Concept ;
  a sosa:Procedure ;
  dct:identifier "http://anzsoil.org/def/au/scma/04B3"^^xsd:anyURI ;
  dct:source "URN:ISBN:978-0-643-10218-7" ;
  skos:definition <https://raw.githack.com/ANZSoilData/def-au-scma/master/html/04-pH/04B3.html> ;
  skos:inScheme s:scma-2011 ;
  skos:inScheme s:swcm-1992 ;
  skos:notation "04B3" ;
  skos:prefLabel "pH of 1:5 soil/0.01 M calcium chloride extract -direct (without stirring during measurement)" ;
  skos:topConceptOf s:scma-2011 ;
  skos:topConceptOf s:swcm-1992 ;
.
<http://anzsoil.org/def/au/scma/04B4>
  a skos:Concept ;
  a sosa:Procedure ;
  dct:identifier "http://anzsoil.org/def/au/scma/04B4"^^xsd:anyURI ;
  dct:source "URN:ISBN:978-0-643-10218-7" ;
  skos:definition <https://raw.githack.com/ANZSoilData/def-au-scma/master/html/04-pH/04B4.html> ;
  skos:inScheme s:scma-2011 ;
  skos:inScheme s:swcm-1992 ;
  skos:notation "04B4" ;
  skos:prefLabel "pH of 1:5 soil/0.01 M calcium chloride extract - following method 4A1 (with stirring during measurement)" ;
  skos:topConceptOf s:scma-2011 ;
  skos:topConceptOf s:swcm-1992 ;
.
<http://anzsoil.org/def/au/scma/04B5>
  a skos:Concept ;
  a sosa:Procedure ;
  dct:identifier "http://anzsoil.org/def/au/scma/04B5"^^xsd:anyURI ;
  dct:source "URN:ISBN:978-0-643-10218-7" ;
  skos:definition <https://raw.githack.com/ANZSoilData/def-au-scma/master/html/04-pH/04B5.html> ;
  skos:inScheme s:scma-2011 ;
  skos:inScheme s:swcm-1992 ;
  skos:notation "04B5" ;
  skos:prefLabel "pH of 1:5 soil/0.01 M calcium chloride extract equivalent, by MIR reflectance spectroscopy" ;
  skos:topConceptOf s:scma-2011 ;
  skos:topConceptOf s:swcm-1992 ;
.
<http://anzsoil.org/def/au/scma/04C1>
  a skos:Concept ;
  a sosa:Procedure ;
  dct:identifier "http://anzsoil.org/def/au/scma/04C1"^^xsd:anyURI ;
  dct:source "URN:ISBN:978-0-643-10218-7" ;
  skos:definition <https://raw.githack.com/ANZSoilData/def-au-scma/master/html/04-pH/04C1.html> ;
  skos:inScheme s:scma-2011 ;
  skos:inScheme s:swcm-1992 ;
  skos:notation "04C1" ;
  skos:prefLabel "pH of 1:5 soil/1M potassium chloride extract - direct (without stirring during measurement)" ;
  skos:topConceptOf s:scma-2011 ;
  skos:topConceptOf s:swcm-1992 ;
.
<http://anzsoil.org/def/au/scma/04C2>
  a skos:Concept ;
  a sosa:Procedure ;
  dct:identifier "http://anzsoil.org/def/au/scma/04C2"^^xsd:anyURI ;
  dct:source "URN:ISBN:978-0-643-10218-7" ;
  skos:definition <https://raw.githack.com/ANZSoilData/def-au-scma/master/html/04-pH/04C2.html> ;
  skos:inScheme s:scma-2011 ;
  skos:inScheme s:swcm-1992 ;
  skos:notation "04C2" ;
  skos:prefLabel "pH of 1:5 soil/1M potassium chloride extract following method 4A1 (without stirring during measurement)" ;
  skos:topConceptOf s:scma-2011 ;
  skos:topConceptOf s:swcm-1992 ;
.
<http://anzsoil.org/def/au/scma/04C3>
  a skos:Concept ;
  a sosa:Procedure ;
  dct:identifier "http://anzsoil.org/def/au/scma/04C3"^^xsd:anyURI ;
  dct:source "URN:ISBN:978-0-643-10218-7" ;
  skos:definition <https://raw.githack.com/ANZSoilData/def-au-scma/master/html/04-pH/04C3.html> ;
  skos:inScheme s:scma-2011 ;
  skos:inScheme s:swcm-1992 ;
  skos:notation "04C3" ;
  skos:prefLabel "pH of 1:5 soil/1M potassium chloride extract - direct (with stirring during measurement)" ;
  skos:topConceptOf s:scma-2011 ;
  skos:topConceptOf s:swcm-1992 ;
.
<http://anzsoil.org/def/au/scma/04C4>
  a skos:Concept ;
  a sosa:Procedure ;
  dct:identifier "http://anzsoil.org/def/au/scma/04C4"^^xsd:anyURI ;
  dct:source "URN:ISBN:978-0-643-10218-7" ;
  skos:definition <https://raw.githack.com/ANZSoilData/def-au-scma/master/html/04-pH/04C4.html> ;
  skos:inScheme s:scma-2011 ;
  skos:inScheme s:swcm-1992 ;
  skos:notation "04C4" ;
  skos:prefLabel "pH of 1:5 soil 1M potassium chloride extract - following method 4A1 (with stirring during measurement)" ;
  skos:topConceptOf s:scma-2011 ;
  skos:topConceptOf s:swcm-1992 ;
.
<http://anzsoil.org/def/au/scma/04D1>
  a skos:Concept ;
  a sosa:Procedure ;
  dct:identifier "http://anzsoil.org/def/au/scma/04D1"^^xsd:anyURI ;
  dct:source "URN:ISBN:978-0-643-10218-7" ;
  skos:definition <https://raw.githack.com/ANZSoilData/def-au-scma/master/html/04-pH/04D1.html> ;
  skos:inScheme s:scma-2011 ;
  skos:inScheme s:swcm-1992 ;
  skos:notation "04D1" ;
  skos:prefLabel "pH of sodium fluoride potential suspension and \\'reactivity class\\'" ;
  skos:topConceptOf s:scma-2011 ;
  skos:topConceptOf s:swcm-1992 ;
.
<http://anzsoil.org/def/au/scma/04E1>
  a skos:Concept ;
  a sosa:Procedure ;
  dct:identifier "http://anzsoil.org/def/au/scma/04E1"^^xsd:anyURI ;
  dct:source "URN:ISBN:978-0-643-10218-7" ;
  skos:definition <https://raw.githack.com/ANZSoilData/def-au-scma/master/html/04-pH/04E1.html> ;
  skos:inScheme s:scma-2011 ;
  skos:inScheme s:swcm-1992 ;
  skos:notation "04E1" ;
  skos:prefLabel "pH of hydrogen peroxide extract" ;
  skos:topConceptOf s:scma-2011 ;
  skos:topConceptOf s:swcm-1992 ;
.
<http://anzsoil.org/def/au/scma/04F1>
  a skos:Concept ;
  a sosa:Procedure ;
  dct:identifier "http://anzsoil.org/def/au/scma/04F1"^^xsd:anyURI ;
  dct:source "URN:ISBN:978-0-643-10218-7" ;
  skos:definition <https://raw.githack.com/ANZSoilData/def-au-scma/master/html/04-pH/04F1.html> ;
  skos:inScheme s:scma-2011 ;
  skos:inScheme s:swcm-1992 ;
  skos:notation "04F1" ;
  skos:prefLabel "pH change" ;
  skos:topConceptOf s:scma-2011 ;
  skos:topConceptOf s:swcm-1992 ;
.
<http://anzsoil.org/def/au/scma/04G1>
  a skos:Concept ;
  a sosa:Procedure ;
  dct:identifier "http://anzsoil.org/def/au/scma/04G1"^^xsd:anyURI ;
  dct:source "URN:ISBN:978-0-643-10218-7" ;
  skos:definition <https://raw.githack.com/ANZSoilData/def-au-scma/master/html/04-pH/04G1.html> ;
  skos:inScheme s:scma-2011 ;
  skos:inScheme s:swcm-1992 ;
  skos:notation "04G1" ;
  skos:prefLabel "Field determination of pH" ;
  skos:topConceptOf s:scma-2011 ;
  skos:topConceptOf s:swcm-1992 ;
.
<http://anzsoil.org/def/au/scma/05>
  a skos:Collection ;
  dct:identifier "http://anzsoil.org/def/au/scma/05"^^xsd:anyURI ;
  dct:source "URN:ISBN:978-0-643-10218-7" ;
  skos:definition <https://raw.githack.com/ANZSoilData/def-au-scma/master/html/05-soluble-Cl/05.html> ;
  skos:member <http://anzsoil.org/def/au/scma/05A1> ;
  skos:member <http://anzsoil.org/def/au/scma/05A2> ;
  skos:member <http://anzsoil.org/def/au/scma/05A2a> ;
  skos:member <http://anzsoil.org/def/au/scma/05A2b> ;
  skos:member <http://anzsoil.org/def/au/scma/05A3a> ;
  skos:member <http://anzsoil.org/def/au/scma/05A3b> ;
  skos:member <http://anzsoil.org/def/au/scma/05A4> ;
  skos:notation "05" ;
  skos:prefLabel "Soluble chloride" ;
.
<http://anzsoil.org/def/au/scma/05A1>
  a skos:Concept ;
  a sosa:Procedure ;
  dct:identifier "http://anzsoil.org/def/au/scma/05A1"^^xsd:anyURI ;
  dct:source "URN:ISBN:978-0-643-10218-7" ;
  skos:definition <https://raw.githack.com/ANZSoilData/def-au-scma/master/html/05-soluble-Cl/05A1.html> ;
  skos:inScheme s:scma-2011 ;
  skos:inScheme s:swcm-1992 ;
  skos:notation "05A1" ;
  skos:prefLabel "Chloride - 1:5 soil/water extract, potentiometric titration" ;
  skos:topConceptOf s:scma-2011 ;
  skos:topConceptOf s:swcm-1992 ;
.
<http://anzsoil.org/def/au/scma/05A2>
  a skos:Concept ;
  a sosa:Procedure ;
  dct:identifier "http://anzsoil.org/def/au/scma/05A2"^^xsd:anyURI ;
  dct:isReplacedBy <http://anzsoil.org/def/au/scma/05A2a> ;
  dct:isReplacedBy <http://anzsoil.org/def/au/scma/05A2b> ;
  dct:source "URN:ISBN:978-0-909605-68-1" ;
  skos:inScheme s:scma-2011 ;
  skos:inScheme s:swcm-1992 ;
  skos:narrower <http://anzsoil.org/def/au/scma/05A2a> ;
  skos:narrower <http://anzsoil.org/def/au/scma/05A2b> ;
  skos:notation "05A2" ;
  skos:prefLabel "Chloride - 1:5 soil/water extract, automated colour" ;
  skos:topConceptOf s:scma-2011 ;
  skos:topConceptOf s:swcm-1992 ;
.
<http://anzsoil.org/def/au/scma/05A2a>
  a skos:Concept ;
  a sosa:Procedure ;
  dct:identifier "http://anzsoil.org/def/au/scma/05A2a"^^xsd:anyURI ;
  dct:source "URN:ISBN:978-0-643-10218-7" ;
  skos:broader <http://anzsoil.org/def/au/scma/05A2> ;
  skos:definition <https://raw.githack.com/ANZSoilData/def-au-scma/master/html/05-soluble-Cl/05A2a.html> ;
  skos:inScheme s:scma-2011 ;
  skos:inScheme s:swcm-1992 ;
  skos:notation "05A2a" ;
  skos:prefLabel "Chloride - 1:5 soil/water extract, automated colour" ;
.
<http://anzsoil.org/def/au/scma/05A2b>
  a skos:Concept ;
  a sosa:Procedure ;
  dct:identifier "http://anzsoil.org/def/au/scma/05A2b"^^xsd:anyURI ;
  dct:source "URN:ISBN:978-0-643-10218-7" ;
  skos:broader <http://anzsoil.org/def/au/scma/05A2> ;
  skos:definition <https://raw.githack.com/ANZSoilData/def-au-scma/master/html/05-soluble-Cl/05A2b.html> ;
  skos:inScheme s:scma-2011 ;
  skos:inScheme s:swcm-1992 ;
  skos:notation "05A2b" ;
  skos:prefLabel "Chloride - 1:5 soil/water extract, FIA" ;
.
<http://anzsoil.org/def/au/scma/05A3a>
  a skos:Concept ;
  a sosa:Procedure ;
  dct:identifier "http://anzsoil.org/def/au/scma/05A3a"^^xsd:anyURI ;
  dct:source "URN:ISBN:978-0-643-10218-7" ;
  skos:definition <https://raw.githack.com/ANZSoilData/def-au-scma/master/html/05-soluble-Cl/05A3a.html> ;
  skos:inScheme s:scma-2011 ;
  skos:inScheme s:swcm-1992 ;
  skos:notation "05A3a" ;
  skos:prefLabel "Chloride - 1:5 soil/water extract, ion chromatography (chemical suppression of eluent conductivity)" ;
  skos:topConceptOf s:scma-2011 ;
  skos:topConceptOf s:swcm-1992 ;
.
<http://anzsoil.org/def/au/scma/05A3b>
  a skos:Concept ;
  a sosa:Procedure ;
  dct:identifier "http://anzsoil.org/def/au/scma/05A3b"^^xsd:anyURI ;
  dct:source "URN:ISBN:978-0-643-10218-7" ;
  skos:definition <https://raw.githack.com/ANZSoilData/def-au-scma/master/html/05-soluble-Cl/05A3b.html> ;
  skos:inScheme s:scma-2011 ;
  skos:inScheme s:swcm-1992 ;
  skos:notation "05A3b" ;
  skos:prefLabel "Chloride - 1:5 soil/water extract, ion chromatography (single-column with electronic suppression of eluent conductivity)" ;
  skos:topConceptOf s:scma-2011 ;
  skos:topConceptOf s:swcm-1992 ;
.
<http://anzsoil.org/def/au/scma/05A4>
  a skos:Concept ;
  a sosa:Procedure ;
  dct:identifier "http://anzsoil.org/def/au/scma/05A4"^^xsd:anyURI ;
  dct:source "URN:ISBN:978-0-643-10218-7" ;
  skos:definition <https://raw.githack.com/ANZSoilData/def-au-scma/master/html/05-soluble-Cl/05A4.html> ;
  skos:inScheme s:scma-2011 ;
  skos:inScheme s:swcm-1992 ;
  skos:notation "05A4" ;
  skos:prefLabel "Chloride - 1:5 soil/water extract ICPAES" ;
  skos:topConceptOf s:scma-2011 ;
  skos:topConceptOf s:swcm-1992 ;
.
<http://anzsoil.org/def/au/scma/06>
  a skos:Collection ;
  dct:identifier "http://anzsoil.org/def/au/scma/06"^^xsd:anyURI ;
  dct:source "URN:ISBN:978-0-643-10218-7" ;
  skos:definition <https://raw.githack.com/ANZSoilData/def-au-scma/master/html/06-C/06.html> ;
  skos:member <http://anzsoil.org/def/au/scma/06A1> ;
  skos:member <http://anzsoil.org/def/au/scma/06B1> ;
  skos:member <http://anzsoil.org/def/au/scma/06B2> ;
  skos:member <http://anzsoil.org/def/au/scma/06B2a> ;
  skos:member <http://anzsoil.org/def/au/scma/06B2b> ;
  skos:member <http://anzsoil.org/def/au/scma/06B3> ;
  skos:member <http://anzsoil.org/def/au/scma/06B4> ;
  skos:member <http://anzsoil.org/def/au/scma/06B4a> ;
  skos:member <http://anzsoil.org/def/au/scma/06B4b> ;
  skos:member <http://anzsoil.org/def/au/scma/06C1> ;
  skos:member <http://anzsoil.org/def/au/scma/06D1> ;
  skos:member <http://anzsoil.org/def/au/scma/06E1> ;
  skos:member <http://anzsoil.org/def/au/scma/06F1> ;
  skos:member <http://anzsoil.org/def/au/scma/06G1> ;
  skos:notation "06" ;
  skos:prefLabel "Carbon" ;
.
<http://anzsoil.org/def/au/scma/06A1>
  a skos:Concept ;
  a sosa:Procedure ;
  dct:identifier "http://anzsoil.org/def/au/scma/06A1"^^xsd:anyURI ;
  dct:source "URN:ISBN:978-0-643-10218-7" ;
  skos:definition <https://raw.githack.com/ANZSoilData/def-au-scma/master/html/06-C/06A1.html> ;
  skos:inScheme s:scma-2011 ;
  skos:inScheme s:swcm-1992 ;
  skos:notation "06A1" ;
  skos:prefLabel "Organic C - W&B" ;
  skos:topConceptOf s:scma-2011 ;
  skos:topConceptOf s:swcm-1992 ;
.
<http://anzsoil.org/def/au/scma/06B1>
  a skos:Concept ;
  a sosa:Procedure ;
  dct:identifier "http://anzsoil.org/def/au/scma/06B1"^^xsd:anyURI ;
  dct:source "URN:ISBN:978-0-643-10218-7" ;
  skos:definition <https://raw.githack.com/ANZSoilData/def-au-scma/master/html/06-C/06B1.html> ;
  skos:inScheme s:scma-2011 ;
  skos:inScheme s:swcm-1992 ;
  skos:notation "06B1" ;
  skos:prefLabel "Total organic C - Heanes wet oxidisation" ;
  skos:topConceptOf s:scma-2011 ;
  skos:topConceptOf s:swcm-1992 ;
.
<http://anzsoil.org/def/au/scma/06B2>
  a skos:Concept ;
  a sosa:Procedure ;
  dct:identifier "http://anzsoil.org/def/au/scma/06B2"^^xsd:anyURI ;
  dct:source "URN:ISBN:978-0-643-10218-7" ;
  skos:definition <https://raw.githack.com/ANZSoilData/def-au-scma/master/html/06-C/06B2.html> ;
  skos:inScheme s:scma-2011 ;
  skos:inScheme s:swcm-1992 ;
  skos:narrower <http://anzsoil.org/def/au/scma/06B2a> ;
  skos:narrower <http://anzsoil.org/def/au/scma/06B2b> ;
  skos:notation "06B2" ;
  skos:prefLabel "Total organic C - Dumas high-temperature combustion" ;
  skos:topConceptOf s:scma-2011 ;
  skos:topConceptOf s:swcm-1992 ;
.
<http://anzsoil.org/def/au/scma/06B2a>
  a skos:Concept ;
  a sosa:Procedure ;
  dct:identifier "http://anzsoil.org/def/au/scma/06B2a"^^xsd:anyURI ;
  dct:source "URN:ISBN:978-0-643-10218-7" ;
  skos:broader <http://anzsoil.org/def/au/scma/06B2> ;
  skos:definition <https://raw.githack.com/ANZSoilData/def-au-scma/master/html/06-C/06B2a.html> ;
  skos:inScheme s:scma-2011 ;
  skos:inScheme s:swcm-1992 ;
  skos:notation "06B2a" ;
  skos:prefLabel "Total organic C - Dumas high-temperature combustion, volumetric (no soil pretreatment)" ;
.
<http://anzsoil.org/def/au/scma/06B2b>
  a skos:Concept ;
  a sosa:Procedure ;
  dct:identifier "http://anzsoil.org/def/au/scma/06B2b"^^xsd:anyURI ;
  dct:source "URN:ISBN:978-0-643-10218-7" ;
  skos:broader <http://anzsoil.org/def/au/scma/06B2> ;
  skos:definition <https://raw.githack.com/ANZSoilData/def-au-scma/master/html/06-C/06B2b.html> ;
  skos:inScheme s:scma-2011 ;
  skos:inScheme s:swcm-1992 ;
  skos:notation "06B2b" ;
  skos:prefLabel "Total organic C - Dumas high-temperature combustion, infrared/thermal conductivity detection (no soil pretreatment)" ;
.
<http://anzsoil.org/def/au/scma/06B3>
  a skos:Concept ;
  a sosa:Procedure ;
  dct:identifier "http://anzsoil.org/def/au/scma/06B3"^^xsd:anyURI ;
  dct:source "URN:ISBN:978-0-643-10218-7" ;
  skos:definition <https://raw.githack.com/ANZSoilData/def-au-scma/master/html/06-C/06B3.html> ;
  skos:inScheme s:scma-2011 ;
  skos:inScheme s:swcm-1992 ;
  skos:notation "06B3" ;
  skos:prefLabel "Total organic C - Dumas high-temperature combustion, infrared/thermal conductivity detection (with prior physical removal of charcoal and chemical removal of carbonates)" ;
  skos:topConceptOf s:scma-2011 ;
  skos:topConceptOf s:swcm-1992 ;
.
<http://anzsoil.org/def/au/scma/06B4>
  a skos:Concept ;
  a sosa:Procedure ;
  dct:identifier "http://anzsoil.org/def/au/scma/06B4"^^xsd:anyURI ;
  dct:source "URN:ISBN:978-0-643-10218-7" ;
  skos:definition <https://raw.githack.com/ANZSoilData/def-au-scma/master/html/06-C/06B4.html> ;
  skos:inScheme s:scma-2011 ;
  skos:inScheme s:swcm-1992 ;
  skos:narrower <http://anzsoil.org/def/au/scma/06B4a> ;
  skos:narrower <http://anzsoil.org/def/au/scma/06B4b> ;
  skos:notation "06B4" ;
  skos:prefLabel "Total organic C - infrared diffuse reflectance spectroscopy" ;
  skos:topConceptOf s:scma-2011 ;
  skos:topConceptOf s:swcm-1992 ;
.
<http://anzsoil.org/def/au/scma/06B4a>
  a skos:Concept ;
  a sosa:Procedure ;
  dct:identifier "http://anzsoil.org/def/au/scma/06B4a"^^xsd:anyURI ;
  dct:source "URN:ISBN:978-0-643-10218-7" ;
  skos:broader <http://anzsoil.org/def/au/scma/06B4> ;
  skos:definition <https://raw.githack.com/ANZSoilData/def-au-scma/master/html/06-C/06B4a.html> ;
  skos:inScheme s:scma-2011 ;
  skos:inScheme s:swcm-1992 ;
  skos:notation "06B4a" ;
  skos:prefLabel "Total organic C - NIR reflectance spectroscopy" ;
.
<http://anzsoil.org/def/au/scma/06B4b>
  a skos:Concept ;
  a sosa:Procedure ;
  dct:identifier "http://anzsoil.org/def/au/scma/06B4b"^^xsd:anyURI ;
  dct:source "URN:ISBN:978-0-643-10218-7" ;
  skos:broader <http://anzsoil.org/def/au/scma/06B4> ;
  skos:definition <https://raw.githack.com/ANZSoilData/def-au-scma/master/html/06-C/06B4b.html> ;
  skos:inScheme s:scma-2011 ;
  skos:inScheme s:swcm-1992 ;
  skos:notation "06B4b" ;
  skos:prefLabel "Total organic C - MIR reflectance spectroscopy" ;
.
<http://anzsoil.org/def/au/scma/06C1>
  a skos:Concept ;
  a sosa:Procedure ;
  dct:identifier "http://anzsoil.org/def/au/scma/06C1"^^xsd:anyURI ;
  dct:source "URN:ISBN:978-0-643-10218-7" ;
  skos:definition <https://raw.githack.com/ANZSoilData/def-au-scma/master/html/06-C/06C1.html> ;
  skos:inScheme s:scma-2011 ;
  skos:inScheme s:swcm-1992 ;
  skos:notation "06C1" ;
  skos:prefLabel "Particulate organic C (POC)" ;
  skos:topConceptOf s:scma-2011 ;
  skos:topConceptOf s:swcm-1992 ;
.
<http://anzsoil.org/def/au/scma/06D1>
  a skos:Concept ;
  a sosa:Procedure ;
  dct:identifier "http://anzsoil.org/def/au/scma/06D1"^^xsd:anyURI ;
  dct:source "URN:ISBN:978-0-643-10218-7" ;
  skos:definition <https://raw.githack.com/ANZSoilData/def-au-scma/master/html/06-C/06D1.html> ;
  skos:inScheme s:scma-2011 ;
  skos:inScheme s:swcm-1992 ;
  skos:notation "06D1" ;
  skos:prefLabel "Pyrophosphate-extractable C" ;
  skos:topConceptOf s:scma-2011 ;
  skos:topConceptOf s:swcm-1992 ;
.
<http://anzsoil.org/def/au/scma/06E1>
  a skos:Concept ;
  a sosa:Procedure ;
  dct:identifier "http://anzsoil.org/def/au/scma/06E1"^^xsd:anyURI ;
  dct:source "URN:ISBN:978-0-643-10218-7" ;
  skos:definition <https://raw.githack.com/ANZSoilData/def-au-scma/master/html/06-C/06E1.html> ;
  skos:inScheme s:scma-2011 ;
  skos:inScheme s:swcm-1992 ;
  skos:notation "06E1" ;
  skos:prefLabel "Potassium permanganate oxidisable C (PPOC)" ;
  skos:topConceptOf s:scma-2011 ;
  skos:topConceptOf s:swcm-1992 ;
.
<http://anzsoil.org/def/au/scma/06F1>
  a skos:Concept ;
  a sosa:Procedure ;
  dct:identifier "http://anzsoil.org/def/au/scma/06F1"^^xsd:anyURI ;
  dct:source "URN:ISBN:978-0-643-10218-7" ;
  skos:definition <https://raw.githack.com/ANZSoilData/def-au-scma/master/html/06-C/06F1.html> ;
  skos:inScheme s:scma-2011 ;
  skos:inScheme s:swcm-1992 ;
  skos:notation "06F1" ;
  skos:prefLabel "Charcoal-C" ;
  skos:topConceptOf s:scma-2011 ;
  skos:topConceptOf s:swcm-1992 ;
.
<http://anzsoil.org/def/au/scma/06G1>
  a skos:Concept ;
  a sosa:Procedure ;
  dct:identifier "http://anzsoil.org/def/au/scma/06G1"^^xsd:anyURI ;
  dct:source "URN:ISBN:978-0-643-10218-7" ;
  skos:definition <https://raw.githack.com/ANZSoilData/def-au-scma/master/html/06-C/06G1.html> ;
  skos:inScheme s:scma-2011 ;
  skos:inScheme s:swcm-1992 ;
  skos:notation "06G1" ;
  skos:prefLabel "Total organic matter, organic C, and carbonate by loss-on-ignition" ;
  skos:topConceptOf s:scma-2011 ;
  skos:topConceptOf s:swcm-1992 ;
.
<http://anzsoil.org/def/au/scma/07>
  a skos:Collection ;
  dct:identifier "http://anzsoil.org/def/au/scma/07"^^xsd:anyURI ;
  dct:source "URN:ISBN:978-0-643-10218-7" ;
  skos:definition <https://raw.githack.com/ANZSoilData/def-au-scma/master/html/07-N/07.html> ;
  skos:member <http://anzsoil.org/def/au/scma/07A1> ;
  skos:member <http://anzsoil.org/def/au/scma/07A2> ;
  skos:member <http://anzsoil.org/def/au/scma/07A2a> ;
  skos:member <http://anzsoil.org/def/au/scma/07A2b> ;
  skos:member <http://anzsoil.org/def/au/scma/07A3> ;
  skos:member <http://anzsoil.org/def/au/scma/07A4> ;
  skos:member <http://anzsoil.org/def/au/scma/07A5> ;
  skos:member <http://anzsoil.org/def/au/scma/07A6> ;
  skos:member <http://anzsoil.org/def/au/scma/07A6a> ;
  skos:member <http://anzsoil.org/def/au/scma/07A6b> ;
  skos:member <http://anzsoil.org/def/au/scma/07B> ;
  skos:member <http://anzsoil.org/def/au/scma/07B1> ;
  skos:member <http://anzsoil.org/def/au/scma/07B1a> ;
  skos:member <http://anzsoil.org/def/au/scma/07B1b> ;
  skos:member <http://anzsoil.org/def/au/scma/07B2> ;
  skos:member <http://anzsoil.org/def/au/scma/07C1> ;
  skos:member <http://anzsoil.org/def/au/scma/07C1a> ;
  skos:member <http://anzsoil.org/def/au/scma/07C1b> ;
  skos:member <http://anzsoil.org/def/au/scma/07C1c> ;
  skos:member <http://anzsoil.org/def/au/scma/07C1d> ;
  skos:member <http://anzsoil.org/def/au/scma/07C1e> ;
  skos:member <http://anzsoil.org/def/au/scma/07C1f> ;
  skos:member <http://anzsoil.org/def/au/scma/07C1g> ;
  skos:member <http://anzsoil.org/def/au/scma/07C1h> ;
  skos:member <http://anzsoil.org/def/au/scma/07C2> ;
  skos:member <http://anzsoil.org/def/au/scma/07C2a> ;
  skos:member <http://anzsoil.org/def/au/scma/07C2b> ;
  skos:member <http://anzsoil.org/def/au/scma/07D> ;
  skos:member <http://anzsoil.org/def/au/scma/07D1a> ;
  skos:member <http://anzsoil.org/def/au/scma/07D1b> ;
  skos:member <http://anzsoil.org/def/au/scma/07D1c> ;
  skos:member <http://anzsoil.org/def/au/scma/07D2a> ;
  skos:member <http://anzsoil.org/def/au/scma/07D2b> ;
  skos:notation "07" ;
  skos:prefLabel "Nitrogen" ;
.
<http://anzsoil.org/def/au/scma/07A1>
  a skos:Concept ;
  a sosa:Procedure ;
  dct:identifier "http://anzsoil.org/def/au/scma/07A1"^^xsd:anyURI ;
  dct:source "URN:ISBN:978-0-643-10218-7" ;
  skos:definition <https://raw.githack.com/ANZSoilData/def-au-scma/master/html/07-N/07A1.html> ;
  skos:inScheme s:scma-2011 ;
  skos:inScheme s:swcm-1992 ;
  skos:notation "07A1" ;
  skos:prefLabel "Total soil-N, semi micro Kjeldahl - steam distillation" ;
  skos:topConceptOf s:scma-2011 ;
  skos:topConceptOf s:swcm-1992 ;
.
<http://anzsoil.org/def/au/scma/07A2>
  a skos:Concept ;
  a sosa:Procedure ;
  dct:identifier "http://anzsoil.org/def/au/scma/07A2"^^xsd:anyURI ;
  dct:isReplacedBy <http://anzsoil.org/def/au/scma/07A2a> ;
  dct:isReplacedBy <http://anzsoil.org/def/au/scma/07A2b> ;
  dct:source "URN:ISBN:978-0-909605-68-1" ;
  skos:inScheme s:scma-2011 ;
  skos:inScheme s:swcm-1992 ;
  skos:narrower <http://anzsoil.org/def/au/scma/07A2a> ;
  skos:narrower <http://anzsoil.org/def/au/scma/07A2b> ;
  skos:notation "07A2" ;
  skos:prefLabel "Total soil-N, semi micro Kjeldahl - automated colour|Total nitrogen - semimicro Kjeldahl, automated colour" ;
  skos:topConceptOf s:scma-2011 ;
  skos:topConceptOf s:swcm-1992 ;
.
<http://anzsoil.org/def/au/scma/07A2a>
  a skos:Concept ;
  a sosa:Procedure ;
  dct:identifier "http://anzsoil.org/def/au/scma/07A2a"^^xsd:anyURI ;
  dct:source "URN:ISBN:978-0-643-10218-7" ;
  skos:broader <http://anzsoil.org/def/au/scma/07A2> ;
  skos:definition <https://raw.githack.com/ANZSoilData/def-au-scma/master/html/07-N/07A2a.html> ;
  skos:inScheme s:scma-2011 ;
  skos:inScheme s:swcm-1992 ;
  skos:notation "07A2a" ;
  skos:prefLabel "Total soil-N, semi micro Kjeldahl - automated colour, continuous segmented flow" ;
.
<http://anzsoil.org/def/au/scma/07A2b>
  a skos:Concept ;
  a sosa:Procedure ;
  dct:identifier "http://anzsoil.org/def/au/scma/07A2b"^^xsd:anyURI ;
  dct:source "URN:ISBN:978-0-643-10218-7" ;
  skos:broader <http://anzsoil.org/def/au/scma/07A2> ;
  skos:definition <https://raw.githack.com/ANZSoilData/def-au-scma/master/html/07-N/07A2b.html> ;
  skos:inScheme s:scma-2011 ;
  skos:inScheme s:swcm-1992 ;
  skos:notation "07A2b" ;
  skos:prefLabel "Total soil-N, semi micro Kjeldahl - automated colour - FIA" ;
.
<http://anzsoil.org/def/au/scma/07A3>
  a skos:Concept ;
  a sosa:Procedure ;
  dct:identifier "http://anzsoil.org/def/au/scma/07A3"^^xsd:anyURI ;
  dct:source "URN:ISBN:978-0-643-10218-7" ;
  skos:definition <https://raw.githack.com/ANZSoilData/def-au-scma/master/html/07-N/07A3.html> ;
  skos:inScheme s:scma-2011 ;
  skos:inScheme s:swcm-1992 ;
  skos:notation "07A3" ;
  skos:prefLabel "Total soil-N (where nitrate >20 mg N/kg) - steam distillation" ;
  skos:topConceptOf s:scma-2011 ;
  skos:topConceptOf s:swcm-1992 ;
.
<http://anzsoil.org/def/au/scma/07A4>
  a skos:Concept ;
  a sosa:Procedure ;
  dct:identifier "http://anzsoil.org/def/au/scma/07A4"^^xsd:anyURI ;
  dct:source "URN:ISBN:978-0-643-10218-7" ;
  skos:definition <https://raw.githack.com/ANZSoilData/def-au-scma/master/html/07-N/07A4.html> ;
  skos:inScheme s:scma-2011 ;
  skos:inScheme s:swcm-1992 ;
  skos:notation "07A4" ;
  skos:prefLabel "Total-N (where nitrate >20 mg N/kg) - automated colour, continuous segmented flow/FIA" ;
  skos:topConceptOf s:scma-2011 ;
  skos:topConceptOf s:swcm-1992 ;
.
<http://anzsoil.org/def/au/scma/07A5>
  a skos:Concept ;
  a sosa:Procedure ;
  dct:identifier "http://anzsoil.org/def/au/scma/07A5"^^xsd:anyURI ;
  dct:source "URN:ISBN:978-0-643-10218-7" ;
  skos:definition <https://raw.githack.com/ANZSoilData/def-au-scma/master/html/07-N/07A5.html> ;
  skos:inScheme s:scma-2011 ;
  skos:inScheme s:swcm-1992 ;
  skos:notation "07A5" ;
  skos:prefLabel "Total soil-N - Dumas high-temperature combustion" ;
  skos:topConceptOf s:scma-2011 ;
  skos:topConceptOf s:swcm-1992 ;
.
<http://anzsoil.org/def/au/scma/07A6>
  a skos:Concept ;
  a sosa:Procedure ;
  dct:identifier "http://anzsoil.org/def/au/scma/07A6"^^xsd:anyURI ;
  dct:source "URN:ISBN:978-0-643-10218-7" ;
  skos:definition <https://raw.githack.com/ANZSoilData/def-au-scma/master/html/07-N/07A6.html> ;
  skos:inScheme s:scma-2011 ;
  skos:inScheme s:swcm-1992 ;
  skos:narrower <http://anzsoil.org/def/au/scma/07A6a> ;
  skos:narrower <http://anzsoil.org/def/au/scma/07A6b> ;
  skos:notation "07A6" ;
  skos:prefLabel "Total soil-N - infrared diffuse reflectance spectroscopy" ;
  skos:topConceptOf s:scma-2011 ;
  skos:topConceptOf s:swcm-1992 ;
.
<http://anzsoil.org/def/au/scma/07A6a>
  a skos:Concept ;
  a sosa:Procedure ;
  dct:identifier "http://anzsoil.org/def/au/scma/07A6a"^^xsd:anyURI ;
  dct:source "URN:ISBN:978-0-643-10218-7" ;
  skos:broader <http://anzsoil.org/def/au/scma/07A6> ;
  skos:definition <https://raw.githack.com/ANZSoilData/def-au-scma/master/html/07-N/07A6a.html> ;
  skos:inScheme s:scma-2011 ;
  skos:inScheme s:swcm-1992 ;
  skos:notation "07A6a" ;
  skos:prefLabel "Total Soil-N - NIR diffuse reflectance spectroscopy" ;
.
<http://anzsoil.org/def/au/scma/07A6b>
  a skos:Concept ;
  a sosa:Procedure ;
  dct:identifier "http://anzsoil.org/def/au/scma/07A6b"^^xsd:anyURI ;
  dct:source "URN:ISBN:978-0-643-10218-7" ;
  skos:broader <http://anzsoil.org/def/au/scma/07A6> ;
  skos:definition <https://raw.githack.com/ANZSoilData/def-au-scma/master/html/07-N/07A6b.html> ;
  skos:inScheme s:scma-2011 ;
  skos:inScheme s:swcm-1992 ;
  skos:notation "07A6b" ;
  skos:prefLabel "Total soil-N - MIR diffuse reflectance spectroscopy" ;
.
<http://anzsoil.org/def/au/scma/07B>
  a skos:Concept ;
  a sosa:Procedure ;
  dct:identifier "http://anzsoil.org/def/au/scma/07B"^^xsd:anyURI ;
  dct:source "URN:ISBN:978-0-643-10218-7" ;
  skos:definition <https://raw.githack.com/ANZSoilData/def-au-scma/master/html/07-N/07B.html> ;
  skos:inScheme s:scma-2011 ;
  skos:inScheme s:swcm-1992 ;
  skos:narrower <http://anzsoil.org/def/au/scma/07B1> ;
  skos:narrower <http://anzsoil.org/def/au/scma/07B2> ;
  skos:notation "07B" ;
  skos:prefLabel "Water-soluble nitrate-N" ;
  skos:topConceptOf s:scma-2011 ;
  skos:topConceptOf s:swcm-1992 ;
.
<http://anzsoil.org/def/au/scma/07B1>
  a skos:Concept ;
  a sosa:Procedure ;
  dct:identifier "http://anzsoil.org/def/au/scma/07B1"^^xsd:anyURI ;
  dct:isReplacedBy <http://anzsoil.org/def/au/scma/07B1a> ;
  dct:isReplacedBy <http://anzsoil.org/def/au/scma/07B1b> ;
  dct:source "URN:ISBN:978-0-909605-68-1" ;
  skos:broader <http://anzsoil.org/def/au/scma/07B> ;
  skos:inScheme s:scma-2011 ;
  skos:inScheme s:swcm-1992 ;
  skos:narrower <http://anzsoil.org/def/au/scma/07B1a> ;
  skos:narrower <http://anzsoil.org/def/au/scma/07B1b> ;
  skos:notation "07B1" ;
  skos:prefLabel "Water-soluble nitrate-N - automated colour|Water soluble nitrate - automated colour" ;
.
<http://anzsoil.org/def/au/scma/07B1a>
  a skos:Concept ;
  a sosa:Procedure ;
  dct:identifier "http://anzsoil.org/def/au/scma/07B1a"^^xsd:anyURI ;
  dct:source "URN:ISBN:978-0-643-10218-7" ;
  skos:broader <http://anzsoil.org/def/au/scma/07B1> ;
  skos:definition <https://raw.githack.com/ANZSoilData/def-au-scma/master/html/07-N/07B1a.html> ;
  skos:inScheme s:scma-2011 ;
  skos:inScheme s:swcm-1992 ;
  skos:notation "07B1a" ;
  skos:prefLabel "Water-soluble nitrate-N - automated colour, continuous segmented flow" ;
.
<http://anzsoil.org/def/au/scma/07B1b>
  a skos:Concept ;
  a sosa:Procedure ;
  dct:identifier "http://anzsoil.org/def/au/scma/07B1b"^^xsd:anyURI ;
  dct:source "URN:ISBN:978-0-643-10218-7" ;
  skos:broader <http://anzsoil.org/def/au/scma/07B1> ;
  skos:definition <https://raw.githack.com/ANZSoilData/def-au-scma/master/html/07-N/07B1b.html> ;
  skos:inScheme s:scma-2011 ;
  skos:inScheme s:swcm-1992 ;
  skos:notation "07B1b" ;
  skos:prefLabel "Water-soluble nitrate-N - automated colour, FIA" ;
.
<http://anzsoil.org/def/au/scma/07B2>
  a skos:Concept ;
  a sosa:Procedure ;
  dct:identifier "http://anzsoil.org/def/au/scma/07B2"^^xsd:anyURI ;
  dct:source "URN:ISBN:978-0-643-10218-7" ;
  skos:broader <http://anzsoil.org/def/au/scma/07B> ;
  skos:definition <https://raw.githack.com/ANZSoilData/def-au-scma/master/html/07-N/07B2.html> ;
  skos:inScheme s:scma-2011 ;
  skos:inScheme s:swcm-1992 ;
  skos:notation "07B2" ;
  skos:prefLabel "Water-soluble nitrate-N - ion chromatography" ;
.
<http://anzsoil.org/def/au/scma/07C1>
  a skos:Concept ;
  a sosa:Procedure ;
  dct:identifier "http://anzsoil.org/def/au/scma/07C1"^^xsd:anyURI ;
  dct:source "URN:ISBN:978-0-643-10218-7" ;
  skos:definition <https://raw.githack.com/ANZSoilData/def-au-scma/master/html/07-N/07C1.html> ;
  skos:inScheme s:scma-2011 ;
  skos:inScheme s:swcm-1992 ;
  skos:narrower <http://anzsoil.org/def/au/scma/07C1a> ;
  skos:narrower <http://anzsoil.org/def/au/scma/07C1b> ;
  skos:narrower <http://anzsoil.org/def/au/scma/07C1c> ;
  skos:narrower <http://anzsoil.org/def/au/scma/07C1d> ;
  skos:narrower <http://anzsoil.org/def/au/scma/07C1e> ;
  skos:narrower <http://anzsoil.org/def/au/scma/07C1f> ;
  skos:narrower <http://anzsoil.org/def/au/scma/07C1g> ;
  skos:narrower <http://anzsoil.org/def/au/scma/07C1h> ;
  skos:notation "07C1" ;
  skos:prefLabel "Mineral-N 2 M KCl, steam distillation" ;
  skos:topConceptOf s:scma-2011 ;
  skos:topConceptOf s:swcm-1992 ;
.
<http://anzsoil.org/def/au/scma/07C1a>
  a skos:Concept ;
  a sosa:Procedure ;
  dct:identifier "http://anzsoil.org/def/au/scma/07C1a"^^xsd:anyURI ;
  dct:source "URN:ISBN:978-0-643-10218-7" ;
  skos:broader <http://anzsoil.org/def/au/scma/07C1> ;
  skos:definition <https://raw.githack.com/ANZSoilData/def-au-scma/master/html/07-N/07C1a.html> ;
  skos:inScheme s:scma-2011 ;
  skos:inScheme s:swcm-1992 ;
  skos:notation "07C1a" ;
  skos:prefLabel "Ammonium-N (in presence or absence of nitrite) - steam distillation" ;
.
<http://anzsoil.org/def/au/scma/07C1b>
  a skos:Concept ;
  a sosa:Procedure ;
  dct:identifier "http://anzsoil.org/def/au/scma/07C1b"^^xsd:anyURI ;
  dct:source "URN:ISBN:978-0-643-10218-7" ;
  skos:broader <http://anzsoil.org/def/au/scma/07C1> ;
  skos:definition <https://raw.githack.com/ANZSoilData/def-au-scma/master/html/07-N/07C1b.html> ;
  skos:inScheme s:scma-2011 ;
  skos:inScheme s:swcm-1992 ;
  skos:notation "07C1b" ;
  skos:prefLabel "(Nitrate + Nitrite)-N - steam distillation" ;
.
<http://anzsoil.org/def/au/scma/07C1c>
  a skos:Concept ;
  a sosa:Procedure ;
  dct:identifier "http://anzsoil.org/def/au/scma/07C1c"^^xsd:anyURI ;
  dct:source "URN:ISBN:978-0-643-10218-7" ;
  skos:broader <http://anzsoil.org/def/au/scma/07C1> ;
  skos:definition <https://raw.githack.com/ANZSoilData/def-au-scma/master/html/07-N/07C1c.html> ;
  skos:inScheme s:scma-2011 ;
  skos:inScheme s:swcm-1992 ;
  skos:notation "07C1c" ;
  skos:prefLabel "(Ammonium + Nitrate + Nitrite)-N - steam distillation" ;
.
<http://anzsoil.org/def/au/scma/07C1d>
  a skos:Concept ;
  a sosa:Procedure ;
  dct:identifier "http://anzsoil.org/def/au/scma/07C1d"^^xsd:anyURI ;
  dct:source "URN:ISBN:978-0-643-10218-7" ;
  skos:broader <http://anzsoil.org/def/au/scma/07C1> ;
  skos:definition <https://raw.githack.com/ANZSoilData/def-au-scma/master/html/07-N/07C1d.html> ;
  skos:inScheme s:scma-2011 ;
  skos:inScheme s:swcm-1992 ;
  skos:notation "07C1d" ;
  skos:prefLabel "(Ammonium + Nitrate)-N, in presence of nitrite - steam distillation" ;
.
<http://anzsoil.org/def/au/scma/07C1e>
  a skos:Concept ;
  a sosa:Procedure ;
  dct:identifier "http://anzsoil.org/def/au/scma/07C1e"^^xsd:anyURI ;
  dct:source "URN:ISBN:978-0-643-10218-7" ;
  skos:broader <http://anzsoil.org/def/au/scma/07C1> ;
  skos:definition <https://raw.githack.com/ANZSoilData/def-au-scma/master/html/07-N/07C1e.html> ;
  skos:inScheme s:scma-2011 ;
  skos:inScheme s:swcm-1992 ;
  skos:notation "07C1e" ;
  skos:prefLabel "Nitrate-N, in presence of nitrite - steam distillation" ;
.
<http://anzsoil.org/def/au/scma/07C1f>
  a skos:Concept ;
  a sosa:Procedure ;
  dct:identifier "http://anzsoil.org/def/au/scma/07C1f"^^xsd:anyURI ;
  dct:source "URN:ISBN:978-0-643-10218-7" ;
  skos:broader <http://anzsoil.org/def/au/scma/07C1> ;
  skos:definition <https://raw.githack.com/ANZSoilData/def-au-scma/master/html/07-N/07C1f.html> ;
  skos:inScheme s:scma-2011 ;
  skos:inScheme s:swcm-1992 ;
  skos:notation "07C1f" ;
  skos:prefLabel "Nitrate-N, in absence of nitrite - steam distillation" ;
.
<http://anzsoil.org/def/au/scma/07C1g>
  a skos:Concept ;
  a sosa:Procedure ;
  dct:identifier "http://anzsoil.org/def/au/scma/07C1g"^^xsd:anyURI ;
  dct:source "URN:ISBN:978-0-643-10218-7" ;
  skos:broader <http://anzsoil.org/def/au/scma/07C1> ;
  skos:definition <https://raw.githack.com/ANZSoilData/def-au-scma/master/html/07-N/07C1g.html> ;
  skos:inScheme s:scma-2011 ;
  skos:inScheme s:swcm-1992 ;
  skos:notation "07C1g" ;
  skos:prefLabel "(Ammonium + Nitrate)-N, in absence of nitrite - steam distillation" ;
.
<http://anzsoil.org/def/au/scma/07C1h>
  a skos:Concept ;
  a sosa:Procedure ;
  dct:identifier "http://anzsoil.org/def/au/scma/07C1h"^^xsd:anyURI ;
  dct:source "URN:ISBN:978-0-643-10218-7" ;
  skos:broader <http://anzsoil.org/def/au/scma/07C1> ;
  skos:definition <https://raw.githack.com/ANZSoilData/def-au-scma/master/html/07-N/07C1h.html> ;
  skos:inScheme s:scma-2011 ;
  skos:inScheme s:swcm-1992 ;
  skos:notation "07C1h" ;
  skos:prefLabel "Nitrite-N - steam distillation" ;
.
<http://anzsoil.org/def/au/scma/07C2>
  a skos:Concept ;
  a sosa:Procedure ;
  dct:identifier "http://anzsoil.org/def/au/scma/07C2"^^xsd:anyURI ;
  dct:isReplacedBy <http://anzsoil.org/def/au/scma/07C2a> ;
  dct:isReplacedBy <http://anzsoil.org/def/au/scma/07C2b> ;
  dct:source "URN:ISBN:978-0-909605-68-1" ;
  skos:inScheme s:scma-2011 ;
  skos:inScheme s:swcm-1992 ;
  skos:narrower <http://anzsoil.org/def/au/scma/07C2a> ;
  skos:narrower <http://anzsoil.org/def/au/scma/07C2b> ;
  skos:notation "07C2" ;
  skos:prefLabel "Mineral-N 2 M KCl, automated colour|mineral nitrogen with 2M KCl - automated colour" ;
  skos:topConceptOf s:scma-2011 ;
  skos:topConceptOf s:swcm-1992 ;
.
<http://anzsoil.org/def/au/scma/07C2a>
  a skos:Concept ;
  a sosa:Procedure ;
  dct:identifier "http://anzsoil.org/def/au/scma/07C2a"^^xsd:anyURI ;
  dct:source "URN:ISBN:978-0-643-10218-7" ;
  skos:broader <http://anzsoil.org/def/au/scma/07C2> ;
  skos:definition <https://raw.githack.com/ANZSoilData/def-au-scma/master/html/07-N/07C2a.html> ;
  skos:inScheme s:scma-2011 ;
  skos:inScheme s:swcm-1992 ;
  skos:notation "07C2a" ;
  skos:prefLabel "Mineral-N 2 M KCl, automated colour, continuous segmented flow" ;
.
<http://anzsoil.org/def/au/scma/07C2b>
  a skos:Concept ;
  a sosa:Procedure ;
  dct:identifier "http://anzsoil.org/def/au/scma/07C2b"^^xsd:anyURI ;
  dct:source "URN:ISBN:978-0-643-10218-7" ;
  skos:broader <http://anzsoil.org/def/au/scma/07C2> ;
  skos:definition <https://raw.githack.com/ANZSoilData/def-au-scma/master/html/07-N/07C2b.html> ;
  skos:inScheme s:scma-2011 ;
  skos:inScheme s:swcm-1992 ;
  skos:notation "07C2b" ;
  skos:prefLabel "Mineral-N - 2 M KCl, automated colour, FIA" ;
.
<http://anzsoil.org/def/au/scma/07D>
  a skos:Concept ;
  a sosa:Procedure ;
  dct:identifier "http://anzsoil.org/def/au/scma/07D"^^xsd:anyURI ;
  dct:source "URN:ISBN:978-0-643-10218-7" ;
  skos:definition <https://raw.githack.com/ANZSoilData/def-au-scma/master/html/07-N/07D.html> ;
  skos:inScheme s:scma-2011 ;
  skos:inScheme s:swcm-1992 ;
  skos:narrower <http://anzsoil.org/def/au/scma/07D1a> ;
  skos:narrower <http://anzsoil.org/def/au/scma/07D1b> ;
  skos:narrower <http://anzsoil.org/def/au/scma/07D1c> ;
  skos:narrower <http://anzsoil.org/def/au/scma/07D2a> ;
  skos:narrower <http://anzsoil.org/def/au/scma/07D2b> ;
  skos:notation "07D" ;
  skos:prefLabel "Potentially mineralisable N (PMN)" ;
  skos:topConceptOf s:scma-2011 ;
  skos:topConceptOf s:swcm-1992 ;
.
<http://anzsoil.org/def/au/scma/07D1a>
  a skos:Concept ;
  a sosa:Procedure ;
  dct:identifier "http://anzsoil.org/def/au/scma/07D1a"^^xsd:anyURI ;
  dct:source "URN:ISBN:978-0-643-10218-7" ;
  skos:broader <http://anzsoil.org/def/au/scma/07D> ;
  skos:definition <https://raw.githack.com/ANZSoilData/def-au-scma/master/html/07-N/07D1a.html> ;
  skos:inScheme s:scma-2011 ;
  skos:inScheme s:swcm-1992 ;
  skos:notation "07D1a" ;
  skos:prefLabel "Potentially mineralisable N, hot-KCl extraction (PMN KCl) - automated colour, continuous segmented flow" ;
.
<http://anzsoil.org/def/au/scma/07D1b>
  a skos:Concept ;
  a sosa:Procedure ;
  dct:identifier "http://anzsoil.org/def/au/scma/07D1b"^^xsd:anyURI ;
  dct:source "URN:ISBN:978-0-643-10218-7" ;
  skos:broader <http://anzsoil.org/def/au/scma/07D> ;
  skos:definition <https://raw.githack.com/ANZSoilData/def-au-scma/master/html/07-N/07D1b.html> ;
  skos:inScheme s:scma-2011 ;
  skos:inScheme s:swcm-1992 ;
  skos:notation "07D1b" ;
  skos:prefLabel "Potentially mineralisable N, hot-KCl extraction (PMN KCl) - automated colour, FIA" ;
.
<http://anzsoil.org/def/au/scma/07D1c>
  a skos:Concept ;
  a sosa:Procedure ;
  dct:identifier "http://anzsoil.org/def/au/scma/07D1c"^^xsd:anyURI ;
  dct:source "URN:ISBN:978-0-643-10218-7" ;
  skos:broader <http://anzsoil.org/def/au/scma/07D> ;
  skos:definition <https://raw.githack.com/ANZSoilData/def-au-scma/master/html/07-N/07D1c.html> ;
  skos:inScheme s:scma-2011 ;
  skos:inScheme s:swcm-1992 ;
  skos:notation "07D1c" ;
  skos:prefLabel "Potentially mineralisable N, hot-KCl extraction (PMN KCl) - NIR diffuse reflectance spectroscopy" ;
.
<http://anzsoil.org/def/au/scma/07D2a>
  a skos:Concept ;
  a sosa:Procedure ;
  dct:identifier "http://anzsoil.org/def/au/scma/07D2a"^^xsd:anyURI ;
  dct:source "URN:ISBN:978-0-643-10218-7" ;
  skos:broader <http://anzsoil.org/def/au/scma/07D> ;
  skos:definition <https://raw.githack.com/ANZSoilData/def-au-scma/master/html/07-N/07D2a.html> ;
  skos:inScheme s:scma-2011 ;
  skos:inScheme s:swcm-1992 ;
  skos:notation "07D2a" ;
  skos:prefLabel "Potentially mineralisable N, anaerobic incubation - automated colour, continuous segmented flow" ;
.
<http://anzsoil.org/def/au/scma/07D2b>
  a skos:Concept ;
  a sosa:Procedure ;
  dct:identifier "http://anzsoil.org/def/au/scma/07D2b"^^xsd:anyURI ;
  dct:source "URN:ISBN:978-0-643-10218-7" ;
  skos:broader <http://anzsoil.org/def/au/scma/07D> ;
  skos:definition <https://raw.githack.com/ANZSoilData/def-au-scma/master/html/07-N/07D2b.html> ;
  skos:inScheme s:scma-2011 ;
  skos:inScheme s:swcm-1992 ;
  skos:notation "07D2b" ;
  skos:prefLabel "Potentially mineralisable N, anaerobic incubation - automated colour, FIA" ;
.
<http://anzsoil.org/def/au/scma/08>
  a skos:Collection ;
  dct:identifier "http://anzsoil.org/def/au/scma/08"^^xsd:anyURI ;
  dct:source "URN:ISBN:978-0-643-10218-7" ;
  skos:definition <https://raw.githack.com/ANZSoilData/def-au-scma/master/html/08-CN-ratio/08.html> ;
  skos:member <http://anzsoil.org/def/au/scma/08A1> ;
  skos:member <http://anzsoil.org/def/au/scma/08B1> ;
  skos:notation "08" ;
  skos:prefLabel "Carbon/nitrogen ratio" ;
.
<http://anzsoil.org/def/au/scma/08A1>
  a skos:Concept ;
  a sosa:Procedure ;
  dct:identifier "http://anzsoil.org/def/au/scma/08A1"^^xsd:anyURI ;
  dct:source "URN:ISBN:978-0-643-10218-7" ;
  skos:definition <https://raw.githack.com/ANZSoilData/def-au-scma/master/html/08-CN-ratio/08A1.html> ;
  skos:inScheme s:scma-2011 ;
  skos:inScheme s:swcm-1992 ;
  skos:notation "08A1" ;
  skos:prefLabel "Total organic carbon/total nitrogen ratio" ;
  skos:topConceptOf s:scma-2011 ;
  skos:topConceptOf s:swcm-1992 ;
.
<http://anzsoil.org/def/au/scma/08B1>
  a skos:Concept ;
  a sosa:Procedure ;
  dct:identifier "http://anzsoil.org/def/au/scma/08B1"^^xsd:anyURI ;
  dct:source "URN:ISBN:978-0-643-10218-7" ;
  skos:definition <https://raw.githack.com/ANZSoilData/def-au-scma/master/html/08-CN-ratio/08B1.html> ;
  skos:inScheme s:scma-2011 ;
  skos:inScheme s:swcm-1992 ;
  skos:notation "08B1" ;
  skos:prefLabel "Organic carbon - W&B/total nitrogen ratio" ;
  skos:topConceptOf s:scma-2011 ;
  skos:topConceptOf s:swcm-1992 ;
.
<http://anzsoil.org/def/au/scma/09>
  a skos:Collection ;
  dct:identifier "http://anzsoil.org/def/au/scma/09"^^xsd:anyURI ;
  dct:source "URN:ISBN:978-0-643-10218-7" ;
  skos:definition <https://raw.githack.com/ANZSoilData/def-au-scma/master/html/09-P/09.html> ;
  skos:member <http://anzsoil.org/def/au/scma/09A> ;
  skos:member <http://anzsoil.org/def/au/scma/09A1> ;
  skos:member <http://anzsoil.org/def/au/scma/09A2> ;
  skos:member <http://anzsoil.org/def/au/scma/09A3a> ;
  skos:member <http://anzsoil.org/def/au/scma/09A3b> ;
  skos:member <http://anzsoil.org/def/au/scma/09B> ;
  skos:member <http://anzsoil.org/def/au/scma/09B1> ;
  skos:member <http://anzsoil.org/def/au/scma/09B2> ;
  skos:member <http://anzsoil.org/def/au/scma/09C> ;
  skos:member <http://anzsoil.org/def/au/scma/09C1> ;
  skos:member <http://anzsoil.org/def/au/scma/09C2> ;
  skos:member <http://anzsoil.org/def/au/scma/09C2a> ;
  skos:member <http://anzsoil.org/def/au/scma/09C2b> ;
  skos:member <http://anzsoil.org/def/au/scma/09D1> ;
  skos:member <http://anzsoil.org/def/au/scma/09E> ;
  skos:member <http://anzsoil.org/def/au/scma/09E1> ;
  skos:member <http://anzsoil.org/def/au/scma/09E2> ;
  skos:member <http://anzsoil.org/def/au/scma/09F1> ;
  skos:member <http://anzsoil.org/def/au/scma/09F2> ;
  skos:member <http://anzsoil.org/def/au/scma/09G1> ;
  skos:member <http://anzsoil.org/def/au/scma/09G2> ;
  skos:member <http://anzsoil.org/def/au/scma/09H1> ;
  skos:member <http://anzsoil.org/def/au/scma/09I> ;
  skos:member <http://anzsoil.org/def/au/scma/09I1> ;
  skos:member <http://anzsoil.org/def/au/scma/09I2a> ;
  skos:member <http://anzsoil.org/def/au/scma/09I2b> ;
  skos:member <http://anzsoil.org/def/au/scma/09I2c> ;
  skos:member <http://anzsoil.org/def/au/scma/09I3a> ;
  skos:member <http://anzsoil.org/def/au/scma/09I3b> ;
  skos:member <http://anzsoil.org/def/au/scma/09I3c> ;
  skos:member <http://anzsoil.org/def/au/scma/09I4a> ;
  skos:member <http://anzsoil.org/def/au/scma/09I4b> ;
  skos:member <http://anzsoil.org/def/au/scma/09I4c> ;
  skos:member <http://anzsoil.org/def/au/scma/09J> ;
  skos:member <http://anzsoil.org/def/au/scma/09J1> ;
  skos:member <http://anzsoil.org/def/au/scma/09J2> ;
  skos:member <http://anzsoil.org/def/au/scma/09K> ;
  skos:member <http://anzsoil.org/def/au/scma/09K1a> ;
  skos:member <http://anzsoil.org/def/au/scma/09K1b> ;
  skos:member <http://anzsoil.org/def/au/scma/09K2> ;
  skos:notation "09" ;
  skos:prefLabel "Phosphorus" ;
.
<http://anzsoil.org/def/au/scma/09A>
  a skos:Concept ;
  a sosa:Procedure ;
  dct:identifier "http://anzsoil.org/def/au/scma/09A"^^xsd:anyURI ;
  dct:source "URN:ISBN:978-0-643-10218-7" ;
  skos:definition <https://raw.githack.com/ANZSoilData/def-au-scma/master/html/09-P/09A.html> ;
  skos:inScheme s:scma-2011 ;
  skos:inScheme s:swcm-1992 ;
  skos:narrower <http://anzsoil.org/def/au/scma/09A1> ;
  skos:narrower <http://anzsoil.org/def/au/scma/09A2> ;
  skos:narrower <http://anzsoil.org/def/au/scma/09A3a> ;
  skos:narrower <http://anzsoil.org/def/au/scma/09A3b> ;
  skos:notation "09A" ;
  skos:prefLabel "Total P" ;
  skos:topConceptOf s:scma-2011 ;
  skos:topConceptOf s:swcm-1992 ;
.
<http://anzsoil.org/def/au/scma/09A1>
  a skos:Concept ;
  a sosa:Procedure ;
  dct:identifier "http://anzsoil.org/def/au/scma/09A1"^^xsd:anyURI ;
  dct:source "URN:ISBN:978-0-643-10218-7" ;
  skos:broader <http://anzsoil.org/def/au/scma/09A> ;
  skos:definition <https://raw.githack.com/ANZSoilData/def-au-scma/master/html/09-P/09A1.html> ;
  skos:inScheme s:scma-2011 ;
  skos:inScheme s:swcm-1992 ;
  skos:notation "09A1" ;
  skos:prefLabel "Total P - X-ray fluorescence" ;
.
<http://anzsoil.org/def/au/scma/09A2>
  a skos:Concept ;
  a sosa:Procedure ;
  dct:identifier "http://anzsoil.org/def/au/scma/09A2"^^xsd:anyURI ;
  dct:source "URN:ISBN:978-0-643-10218-7" ;
  skos:broader <http://anzsoil.org/def/au/scma/09A> ;
  skos:definition <https://raw.githack.com/ANZSoilData/def-au-scma/master/html/09-P/09A2.html> ;
  skos:inScheme s:scma-2011 ;
  skos:inScheme s:swcm-1992 ;
  skos:notation "09A2" ;
  skos:prefLabel "Total P - sodium carbonate fusion" ;
.
<http://anzsoil.org/def/au/scma/09A3a>
  a skos:Concept ;
  a sosa:Procedure ;
  dct:identifier "http://anzsoil.org/def/au/scma/09A3a"^^xsd:anyURI ;
  dct:source "URN:ISBN:978-0-643-10218-7" ;
  skos:broader <http://anzsoil.org/def/au/scma/09A> ;
  skos:definition <https://raw.githack.com/ANZSoilData/def-au-scma/master/html/09-P/09A3a.html> ;
  skos:inScheme s:scma-2011 ;
  skos:inScheme s:swcm-1992 ;
  skos:notation "09A3a" ;
  skos:prefLabel "Kjeldahl P (KP) - automated colour, FIA/continuous segmented flow" ;
.
<http://anzsoil.org/def/au/scma/09A3b>
  a skos:Concept ;
  a sosa:Procedure ;
  dct:identifier "http://anzsoil.org/def/au/scma/09A3b"^^xsd:anyURI ;
  dct:source "URN:ISBN:978-0-643-10218-7" ;
  skos:broader <http://anzsoil.org/def/au/scma/09A> ;
  skos:definition <https://raw.githack.com/ANZSoilData/def-au-scma/master/html/09-P/09A3b.html> ;
  skos:inScheme s:scma-2011 ;
  skos:inScheme s:swcm-1992 ;
  skos:notation "09A3b" ;
  skos:prefLabel "Kjeldahl P (KP) - ICPAES" ;
.
<http://anzsoil.org/def/au/scma/09B>
  a skos:Concept ;
  a sosa:Procedure ;
  dct:identifier "http://anzsoil.org/def/au/scma/09B"^^xsd:anyURI ;
  dct:source "URN:ISBN:978-0-643-10218-7" ;
  skos:definition <https://raw.githack.com/ANZSoilData/def-au-scma/master/html/09-P/09B.html> ;
  skos:inScheme s:scma-2011 ;
  skos:inScheme s:swcm-1992 ;
  skos:narrower <http://anzsoil.org/def/au/scma/09B1> ;
  skos:narrower <http://anzsoil.org/def/au/scma/09B2> ;
  skos:notation "09B" ;
  skos:prefLabel "Bicarbonate-extractable P (Colwell-P)" ;
  skos:topConceptOf s:scma-2011 ;
  skos:topConceptOf s:swcm-1992 ;
.
<http://anzsoil.org/def/au/scma/09B1>
  a skos:Concept ;
  a sosa:Procedure ;
  dct:identifier "http://anzsoil.org/def/au/scma/09B1"^^xsd:anyURI ;
  dct:source "URN:ISBN:978-0-643-10218-7" ;
  skos:broader <http://anzsoil.org/def/au/scma/09B> ;
  skos:definition <https://raw.githack.com/ANZSoilData/def-au-scma/master/html/09-P/09B1.html> ;
  skos:inScheme s:scma-2011 ;
  skos:inScheme s:swcm-1992 ;
  skos:notation "09B1" ;
  skos:prefLabel "Bicarbonate-extractable P (Colwell-P) - manual colour" ;
.
<http://anzsoil.org/def/au/scma/09B2>
  a skos:Concept ;
  a sosa:Procedure ;
  dct:identifier "http://anzsoil.org/def/au/scma/09B2"^^xsd:anyURI ;
  dct:source "URN:ISBN:978-0-643-10218-7" ;
  skos:broader <http://anzsoil.org/def/au/scma/09B> ;
  skos:definition <https://raw.githack.com/ANZSoilData/def-au-scma/master/html/09-P/09B2.html> ;
  skos:inScheme s:scma-2011 ;
  skos:inScheme s:swcm-1992 ;
  skos:notation "09B2" ;
  skos:prefLabel "Bicarbonate-extractable P (Colwell-P) - automated colour, continuous segmented flow/FIA" ;
.
<http://anzsoil.org/def/au/scma/09C>
  a skos:Concept ;
  a sosa:Procedure ;
  dct:identifier "http://anzsoil.org/def/au/scma/09C"^^xsd:anyURI ;
  dct:source "URN:ISBN:978-0-643-10218-7" ;
  skos:definition <https://raw.githack.com/ANZSoilData/def-au-scma/master/html/09-P/09C.html> ;
  skos:inScheme s:scma-2011 ;
  skos:inScheme s:swcm-1992 ;
  skos:narrower <http://anzsoil.org/def/au/scma/09C1> ;
  skos:narrower <http://anzsoil.org/def/au/scma/09C2> ;
  skos:notation "09C" ;
  skos:prefLabel "Olsen-extractable P (Olsen-P)" ;
  skos:topConceptOf s:scma-2011 ;
  skos:topConceptOf s:swcm-1992 ;
.
<http://anzsoil.org/def/au/scma/09C1>
  a skos:Concept ;
  a sosa:Procedure ;
  dct:identifier "http://anzsoil.org/def/au/scma/09C1"^^xsd:anyURI ;
  dct:source "URN:ISBN:978-0-643-10218-7" ;
  skos:broader <http://anzsoil.org/def/au/scma/09C> ;
  skos:definition <https://raw.githack.com/ANZSoilData/def-au-scma/master/html/09-P/09C1.html> ;
  skos:inScheme s:scma-2011 ;
  skos:inScheme s:swcm-1992 ;
  skos:notation "09C1" ;
  skos:prefLabel "Olsen-extractable P (Olsen-P) - manual colour" ;
.
<http://anzsoil.org/def/au/scma/09C2>
  a skos:Concept ;
  a sosa:Procedure ;
  dct:identifier "http://anzsoil.org/def/au/scma/09C2"^^xsd:anyURI ;
  dct:isReplacedBy <http://anzsoil.org/def/au/scma/09C2a> ;
  dct:isReplacedBy <http://anzsoil.org/def/au/scma/09C2b> ;
  dct:source "URN:ISBN:978-0-909605-68-1" ;
  skos:broader <http://anzsoil.org/def/au/scma/09C> ;
  skos:inScheme s:scma-2011 ;
  skos:inScheme s:swcm-1992 ;
  skos:narrower <http://anzsoil.org/def/au/scma/09C2a> ;
  skos:narrower <http://anzsoil.org/def/au/scma/09C2b> ;
  skos:notation "09C2" ;
  skos:prefLabel "Olsen-extractable phosphorus - automated colour|Olsen-extractable P (Olsen-P) - automated colour" ;
.
<http://anzsoil.org/def/au/scma/09C2a>
  a skos:Concept ;
  a sosa:Procedure ;
  dct:identifier "http://anzsoil.org/def/au/scma/09C2a"^^xsd:anyURI ;
  dct:source "URN:ISBN:978-0-643-10218-7" ;
  skos:broader <http://anzsoil.org/def/au/scma/09C2> ;
  skos:definition <https://raw.githack.com/ANZSoilData/def-au-scma/master/html/09-P/09C2a.html> ;
  skos:inScheme s:scma-2011 ;
  skos:inScheme s:swcm-1992 ;
  skos:notation "09C2a" ;
  skos:prefLabel "Olsen-extractable P (Olsen-P) - automated colour, continuous segmented flow" ;
.
<http://anzsoil.org/def/au/scma/09C2b>
  a skos:Concept ;
  a sosa:Procedure ;
  dct:identifier "http://anzsoil.org/def/au/scma/09C2b"^^xsd:anyURI ;
  dct:source "URN:ISBN:978-0-643-10218-7" ;
  skos:broader <http://anzsoil.org/def/au/scma/09C2> ;
  skos:definition <https://raw.githack.com/ANZSoilData/def-au-scma/master/html/09-P/09C2b.html> ;
  skos:inScheme s:scma-2011 ;
  skos:inScheme s:swcm-1992 ;
  skos:notation "09C2b" ;
  skos:prefLabel "Olsen-extractable P (Olsen-P) - automated colour/FIA" ;
.
<http://anzsoil.org/def/au/scma/09D1>
  a skos:Concept ;
  a sosa:Procedure ;
  dct:identifier "http://anzsoil.org/def/au/scma/09D1"^^xsd:anyURI ;
  dct:source "URN:ISBN:978-0-643-10218-7" ;
  skos:definition <https://raw.githack.com/ANZSoilData/def-au-scma/master/html/09-P/09D1.html> ;
  skos:inScheme s:scma-2011 ;
  skos:inScheme s:swcm-1992 ;
  skos:notation "09D1" ;
  skos:prefLabel "Lactate-extractable P (Lactate-P) - manual colour" ;
  skos:topConceptOf s:scma-2011 ;
  skos:topConceptOf s:swcm-1992 ;
.
<http://anzsoil.org/def/au/scma/09E>
  a skos:Concept ;
  a sosa:Procedure ;
  dct:identifier "http://anzsoil.org/def/au/scma/09E"^^xsd:anyURI ;
  dct:source "URN:ISBN:978-0-643-10218-7" ;
  skos:definition <https://raw.githack.com/ANZSoilData/def-au-scma/master/html/09-P/09E.html> ;
  skos:inScheme s:scma-2011 ;
  skos:inScheme s:swcm-1992 ;
  skos:narrower <http://anzsoil.org/def/au/scma/09E1> ;
  skos:narrower <http://anzsoil.org/def/au/scma/09E2> ;
  skos:notation "09E" ;
  skos:prefLabel "Fluoride-extractable P (Bray-1 P)" ;
  skos:topConceptOf s:scma-2011 ;
  skos:topConceptOf s:swcm-1992 ;
.
<http://anzsoil.org/def/au/scma/09E1>
  a skos:Concept ;
  a sosa:Procedure ;
  dct:identifier "http://anzsoil.org/def/au/scma/09E1"^^xsd:anyURI ;
  dct:source "URN:ISBN:978-0-643-10218-7" ;
  skos:broader <http://anzsoil.org/def/au/scma/09E> ;
  skos:definition <https://raw.githack.com/ANZSoilData/def-au-scma/master/html/09-P/09E1.html> ;
  skos:inScheme s:scma-2011 ;
  skos:inScheme s:swcm-1992 ;
  skos:notation "09E1" ;
  skos:prefLabel "Fluoride-extractable P (Bray-1 P) - manual colour" ;
.
<http://anzsoil.org/def/au/scma/09E2>
  a skos:Concept ;
  a sosa:Procedure ;
  dct:identifier "http://anzsoil.org/def/au/scma/09E2"^^xsd:anyURI ;
  dct:source "URN:ISBN:978-0-643-10218-7" ;
  skos:broader <http://anzsoil.org/def/au/scma/09E> ;
  skos:definition <https://raw.githack.com/ANZSoilData/def-au-scma/master/html/09-P/09E2.html> ;
  skos:inScheme s:scma-2011 ;
  skos:inScheme s:swcm-1992 ;
  skos:notation "09E2" ;
  skos:prefLabel "Fluoride-extractable P (Bray-1 P) - continuous segmented flow/FIA automated colour" ;
.
<http://anzsoil.org/def/au/scma/09F1>
  a skos:Concept ;
  a sosa:Procedure ;
  dct:identifier "http://anzsoil.org/def/au/scma/09F1"^^xsd:anyURI ;
  dct:source "URN:ISBN:978-0-643-10218-7" ;
  skos:definition <https://raw.githack.com/ANZSoilData/def-au-scma/master/html/09-P/09F1.html> ;
  skos:inScheme s:scma-2011 ;
  skos:inScheme s:swcm-1992 ;
  skos:notation "09F1" ;
  skos:prefLabel "Calcium chloride-extractable P - manual colour" ;
  skos:topConceptOf s:scma-2011 ;
  skos:topConceptOf s:swcm-1992 ;
.
<http://anzsoil.org/def/au/scma/09F2>
  a skos:Concept ;
  a sosa:Procedure ;
  dct:identifier "http://anzsoil.org/def/au/scma/09F2"^^xsd:anyURI ;
  dct:source "URN:ISBN:978-0-643-10218-7" ;
  skos:definition <https://raw.githack.com/ANZSoilData/def-au-scma/master/html/09-P/09F2.html> ;
  skos:inScheme s:scma-2011 ;
  skos:inScheme s:swcm-1992 ;
  skos:notation "09F2" ;
  skos:prefLabel "Calcium chloride-extractable P - continuous segmented flow/FIA automated colour" ;
  skos:topConceptOf s:scma-2011 ;
  skos:topConceptOf s:swcm-1992 ;
.
<http://anzsoil.org/def/au/scma/09G1>
  a skos:Concept ;
  a sosa:Procedure ;
  dct:identifier "http://anzsoil.org/def/au/scma/09G1"^^xsd:anyURI ;
  dct:source "URN:ISBN:978-0-643-10218-7" ;
  skos:definition <https://raw.githack.com/ANZSoilData/def-au-scma/master/html/09-P/09G1.html> ;
  skos:inScheme s:scma-2011 ;
  skos:inScheme s:swcm-1992 ;
  skos:notation "09G1" ;
  skos:prefLabel "Acid-extractable P (BSES-P) - manual colour" ;
  skos:topConceptOf s:scma-2011 ;
  skos:topConceptOf s:swcm-1992 ;
.
<http://anzsoil.org/def/au/scma/09G2>
  a skos:Concept ;
  a sosa:Procedure ;
  dct:identifier "http://anzsoil.org/def/au/scma/09G2"^^xsd:anyURI ;
  dct:source "URN:ISBN:978-0-643-10218-7" ;
  skos:definition <https://raw.githack.com/ANZSoilData/def-au-scma/master/html/09-P/09G2.html> ;
  skos:inScheme s:scma-2011 ;
  skos:inScheme s:swcm-1992 ;
  skos:notation "09G2" ;
  skos:prefLabel "Acid-extractable P (BSES-P) - continuous segmented flow/FIA automated colour" ;
  skos:topConceptOf s:scma-2011 ;
  skos:topConceptOf s:swcm-1992 ;
.
<http://anzsoil.org/def/au/scma/09H1>
  a skos:Concept ;
  a sosa:Procedure ;
  dct:identifier "http://anzsoil.org/def/au/scma/09H1"^^xsd:anyURI ;
  dct:source "URN:ISBN:978-0-643-10218-7" ;
  skos:definition <https://raw.githack.com/ANZSoilData/def-au-scma/master/html/09-P/09H1.html> ;
  skos:inScheme s:scma-2011 ;
  skos:inScheme s:swcm-1992 ;
  skos:notation "09H1" ;
  skos:prefLabel "Anion Storage Capacity (previously P Retention)" ;
  skos:topConceptOf s:scma-2011 ;
  skos:topConceptOf s:swcm-1992 ;
.
<http://anzsoil.org/def/au/scma/09I>
  a skos:Concept ;
  a sosa:Procedure ;
  dct:identifier "http://anzsoil.org/def/au/scma/09I"^^xsd:anyURI ;
  dct:source "URN:ISBN:978-0-643-10218-7" ;
  skos:definition <https://raw.githack.com/ANZSoilData/def-au-scma/master/html/09-P/09I.html> ;
  skos:inScheme s:scma-2011 ;
  skos:inScheme s:swcm-1992 ;
  skos:narrower <http://anzsoil.org/def/au/scma/09I1> ;
  skos:narrower <http://anzsoil.org/def/au/scma/09I2a> ;
  skos:narrower <http://anzsoil.org/def/au/scma/09I2b> ;
  skos:narrower <http://anzsoil.org/def/au/scma/09I2c> ;
  skos:narrower <http://anzsoil.org/def/au/scma/09I3a> ;
  skos:narrower <http://anzsoil.org/def/au/scma/09I3b> ;
  skos:narrower <http://anzsoil.org/def/au/scma/09I3c> ;
  skos:narrower <http://anzsoil.org/def/au/scma/09I4a> ;
  skos:narrower <http://anzsoil.org/def/au/scma/09I4b> ;
  skos:narrower <http://anzsoil.org/def/au/scma/09I4c> ;
  skos:notation "09I" ;
  skos:prefLabel "Phosphate Indices" ;
  skos:topConceptOf s:scma-2011 ;
  skos:topConceptOf s:swcm-1992 ;
.
<http://anzsoil.org/def/au/scma/09I1>
  a skos:Concept ;
  a sosa:Procedure ;
  dct:identifier "http://anzsoil.org/def/au/scma/09I1"^^xsd:anyURI ;
  dct:source "URN:ISBN:978-0-643-10218-7" ;
  skos:broader <http://anzsoil.org/def/au/scma/09I> ;
  skos:definition <https://raw.githack.com/ANZSoilData/def-au-scma/master/html/09-P/09I1.html> ;
  skos:inScheme s:scma-2011 ;
  skos:inScheme s:swcm-1992 ;
  skos:notation "09I1" ;
  skos:prefLabel "Phosphate Sorption Index" ;
.
<http://anzsoil.org/def/au/scma/09I2a>
  a skos:Concept ;
  a sosa:Procedure ;
  dct:identifier "http://anzsoil.org/def/au/scma/09I2a"^^xsd:anyURI ;
  dct:source "URN:ISBN:978-0-643-10218-7" ;
  skos:broader <http://anzsoil.org/def/au/scma/09I> ;
  skos:definition <https://raw.githack.com/ANZSoilData/def-au-scma/master/html/09-P/09I2a.html> ;
  skos:inScheme s:scma-2011 ;
  skos:inScheme s:swcm-1992 ;
  skos:notation "09I2a" ;
  skos:prefLabel "P buffer index - PBI (ColP) - Murphy and Riley|P buffer index - PBI (ColP)" ;
.
<http://anzsoil.org/def/au/scma/09I2b>
  a skos:Concept ;
  a sosa:Procedure ;
  dct:identifier "http://anzsoil.org/def/au/scma/09I2b"^^xsd:anyURI ;
  dct:source "URN:ISBN:978-0-643-10218-7" ;
  skos:broader <http://anzsoil.org/def/au/scma/09I> ;
  skos:definition <https://raw.githack.com/ANZSoilData/def-au-scma/master/html/09-P/09I2b.html> ;
  skos:inScheme s:scma-2011 ;
  skos:inScheme s:swcm-1992 ;
  skos:notation "09I2b" ;
  skos:prefLabel "P buffer index - PBI (ColP)|P buffer index - PBI (ColP) - ICPAES" ;
.
<http://anzsoil.org/def/au/scma/09I2c>
  a skos:Concept ;
  a sosa:Procedure ;
  dct:identifier "http://anzsoil.org/def/au/scma/09I2c"^^xsd:anyURI ;
  dct:source "URN:ISBN:978-0-643-10218-7" ;
  skos:broader <http://anzsoil.org/def/au/scma/09I> ;
  skos:definition <https://raw.githack.com/ANZSoilData/def-au-scma/master/html/09-P/09I2c.html> ;
  skos:inScheme s:scma-2011 ;
  skos:inScheme s:swcm-1992 ;
  skos:notation "09I2c" ;
  skos:prefLabel "P buffer index - PBI (ColP)|P buffer index - PBI (ColP) - Vanadate" ;
.
<http://anzsoil.org/def/au/scma/09I3a>
  a skos:Concept ;
  a sosa:Procedure ;
  dct:identifier "http://anzsoil.org/def/au/scma/09I3a"^^xsd:anyURI ;
  dct:source "URN:ISBN:978-0-643-10218-7" ;
  skos:broader <http://anzsoil.org/def/au/scma/09I> ;
  skos:definition <https://raw.githack.com/ANZSoilData/def-au-scma/master/html/09-P/09I3a.html> ;
  skos:inScheme s:scma-2011 ;
  skos:inScheme s:swcm-1992 ;
  skos:notation "09I3a" ;
  skos:prefLabel "P buffer index - PBI (OlsenP)|P buffer index - PBI (OlsenP) - Murphy and Riley" ;
.
<http://anzsoil.org/def/au/scma/09I3b>
  a skos:Concept ;
  a sosa:Procedure ;
  dct:identifier "http://anzsoil.org/def/au/scma/09I3b"^^xsd:anyURI ;
  dct:source "URN:ISBN:978-0-643-10218-7" ;
  skos:broader <http://anzsoil.org/def/au/scma/09I> ;
  skos:definition <https://raw.githack.com/ANZSoilData/def-au-scma/master/html/09-P/09I3b.html> ;
  skos:inScheme s:scma-2011 ;
  skos:inScheme s:swcm-1992 ;
  skos:notation "09I3b" ;
  skos:prefLabel "P buffer index - PBI (OlsenP)|P buffer index - PBI (OlsenP) - ICPAES" ;
.
<http://anzsoil.org/def/au/scma/09I3c>
  a skos:Concept ;
  a sosa:Procedure ;
  dct:identifier "http://anzsoil.org/def/au/scma/09I3c"^^xsd:anyURI ;
  dct:source "URN:ISBN:978-0-643-10218-7" ;
  skos:broader <http://anzsoil.org/def/au/scma/09I> ;
  skos:definition <https://raw.githack.com/ANZSoilData/def-au-scma/master/html/09-P/09I3c.html> ;
  skos:inScheme s:scma-2011 ;
  skos:inScheme s:swcm-1992 ;
  skos:notation "09I3c" ;
  skos:prefLabel "P buffer index - PBI (OlsenP)|P buffer index - PBI (OlsenP) - Vanadate" ;
.
<http://anzsoil.org/def/au/scma/09I4a>
  a skos:Concept ;
  a sosa:Procedure ;
  dct:identifier "http://anzsoil.org/def/au/scma/09I4a"^^xsd:anyURI ;
  dct:source "URN:ISBN:978-0-643-10218-7" ;
  skos:broader <http://anzsoil.org/def/au/scma/09I> ;
  skos:definition <https://raw.githack.com/ANZSoilData/def-au-scma/master/html/09-P/09I4a.html> ;
  skos:inScheme s:scma-2011 ;
  skos:inScheme s:swcm-1992 ;
  skos:notation "09I4a" ;
  skos:prefLabel "P buffer index - PBI (unadj) - Murphy and Riley|P buffer index - PBI (unadj)" ;
.
<http://anzsoil.org/def/au/scma/09I4b>
  a skos:Concept ;
  a sosa:Procedure ;
  dct:identifier "http://anzsoil.org/def/au/scma/09I4b"^^xsd:anyURI ;
  dct:source "URN:ISBN:978-0-643-10218-7" ;
  skos:broader <http://anzsoil.org/def/au/scma/09I> ;
  skos:definition <https://raw.githack.com/ANZSoilData/def-au-scma/master/html/09-P/09I4b.html> ;
  skos:inScheme s:scma-2011 ;
  skos:inScheme s:swcm-1992 ;
  skos:notation "09I4b" ;
  skos:prefLabel "P buffer index - PBI (unadj) - ICPAES|P buffer index - PBI (unadj)" ;
.
<http://anzsoil.org/def/au/scma/09I4c>
  a skos:Concept ;
  a sosa:Procedure ;
  dct:identifier "http://anzsoil.org/def/au/scma/09I4c"^^xsd:anyURI ;
  dct:source "URN:ISBN:978-0-643-10218-7" ;
  skos:broader <http://anzsoil.org/def/au/scma/09I> ;
  skos:definition <https://raw.githack.com/ANZSoilData/def-au-scma/master/html/09-P/09I4c.html> ;
  skos:inScheme s:scma-2011 ;
  skos:inScheme s:swcm-1992 ;
  skos:notation "09I4c" ;
  skos:prefLabel "P buffer index - PBI (unadj)|P buffer index - PBI (unadj) - Vanadate" ;
.
<http://anzsoil.org/def/au/scma/09J>
  a skos:Concept ;
  a sosa:Procedure ;
  dct:identifier "http://anzsoil.org/def/au/scma/09J"^^xsd:anyURI ;
  dct:source "URN:ISBN:978-0-643-10218-7" ;
  skos:definition <https://raw.githack.com/ANZSoilData/def-au-scma/master/html/09-P/09J.html> ;
  skos:inScheme s:scma-2011 ;
  skos:inScheme s:swcm-1992 ;
  skos:narrower <http://anzsoil.org/def/au/scma/09J1> ;
  skos:narrower <http://anzsoil.org/def/au/scma/09J2> ;
  skos:notation "09J" ;
  skos:prefLabel "Phosphate sorption curve" ;
  skos:topConceptOf s:scma-2011 ;
  skos:topConceptOf s:swcm-1992 ;
.
<http://anzsoil.org/def/au/scma/09J1>
  a skos:Concept ;
  a sosa:Procedure ;
  dct:identifier "http://anzsoil.org/def/au/scma/09J1"^^xsd:anyURI ;
  dct:source "URN:ISBN:978-0-643-10218-7" ;
  skos:broader <http://anzsoil.org/def/au/scma/09J> ;
  skos:definition <https://raw.githack.com/ANZSoilData/def-au-scma/master/html/09-P/09J1.html> ;
  skos:inScheme s:scma-2011 ;
  skos:inScheme s:swcm-1992 ;
  skos:notation "09J1" ;
  skos:prefLabel "Phosphate sorption curve - manual colour" ;
.
<http://anzsoil.org/def/au/scma/09J2>
  a skos:Concept ;
  a sosa:Procedure ;
  dct:identifier "http://anzsoil.org/def/au/scma/09J2"^^xsd:anyURI ;
  dct:source "URN:ISBN:978-0-643-10218-7" ;
  skos:broader <http://anzsoil.org/def/au/scma/09J> ;
  skos:definition <https://raw.githack.com/ANZSoilData/def-au-scma/master/html/09-P/09J2.html> ;
  skos:inScheme s:scma-2011 ;
  skos:inScheme s:swcm-1992 ;
  skos:notation "09J2" ;
  skos:prefLabel "Phosphate sorption curve - continuous segmented flow/FIA automated colour" ;
.
<http://anzsoil.org/def/au/scma/09K>
  a skos:Concept ;
  a sosa:Procedure ;
  dct:identifier "http://anzsoil.org/def/au/scma/09K"^^xsd:anyURI ;
  dct:source "URN:ISBN:978-0-643-10218-7" ;
  skos:definition <https://raw.githack.com/ANZSoilData/def-au-scma/master/html/09-P/09K.html> ;
  skos:inScheme s:scma-2011 ;
  skos:inScheme s:swcm-1992 ;
  skos:narrower <http://anzsoil.org/def/au/scma/09K1a> ;
  skos:narrower <http://anzsoil.org/def/au/scma/09K1b> ;
  skos:narrower <http://anzsoil.org/def/au/scma/09K2> ;
  skos:notation "09K" ;
  skos:prefLabel "Environmental soil P tests" ;
  skos:topConceptOf s:scma-2011 ;
  skos:topConceptOf s:swcm-1992 ;
.
<http://anzsoil.org/def/au/scma/09K1a>
  a skos:Concept ;
  a sosa:Procedure ;
  dct:identifier "http://anzsoil.org/def/au/scma/09K1a"^^xsd:anyURI ;
  dct:source "URN:ISBN:978-0-643-10218-7" ;
  skos:broader <http://anzsoil.org/def/au/scma/09K> ;
  skos:definition <https://raw.githack.com/ANZSoilData/def-au-scma/master/html/09-P/09K1a.html> ;
  skos:inScheme s:scma-2011 ;
  skos:inScheme s:swcm-1992 ;
  skos:notation "09K1a" ;
  skos:prefLabel "Mehlich 3-P saturation ratio (M3PSR colour) [colormetric estimate of P]" ;
.
<http://anzsoil.org/def/au/scma/09K1b>
  a skos:Concept ;
  a sosa:Procedure ;
  dct:identifier "http://anzsoil.org/def/au/scma/09K1b"^^xsd:anyURI ;
  dct:source "URN:ISBN:978-0-643-10218-7" ;
  skos:broader <http://anzsoil.org/def/au/scma/09K> ;
  skos:definition <https://raw.githack.com/ANZSoilData/def-au-scma/master/html/09-P/09K1b.html> ;
  skos:inScheme s:scma-2011 ;
  skos:inScheme s:swcm-1992 ;
  skos:notation "09K1b" ;
  skos:prefLabel "Mehlich 3-P saturation ratio (M3PSR ICPAES) [ICPAES estimate of P]" ;
.
<http://anzsoil.org/def/au/scma/09K2>
  a skos:Concept ;
  a sosa:Procedure ;
  dct:identifier "http://anzsoil.org/def/au/scma/09K2"^^xsd:anyURI ;
  dct:source "URN:ISBN:978-0-643-10218-7" ;
  skos:broader <http://anzsoil.org/def/au/scma/09K> ;
  skos:definition <https://raw.githack.com/ANZSoilData/def-au-scma/master/html/09-P/09K2.html> ;
  skos:inScheme s:scma-2011 ;
  skos:inScheme s:swcm-1992 ;
  skos:notation "09K2" ;
  skos:prefLabel "Colwell-P/PBI (ColP) ratio" ;
.
<http://anzsoil.org/def/au/scma/10>
  a skos:Collection ;
  dct:identifier "http://anzsoil.org/def/au/scma/10"^^xsd:anyURI ;
  dct:source "URN:ISBN:978-0-643-10218-7" ;
  skos:definition <https://raw.githack.com/ANZSoilData/def-au-scma/master/html/10-S/10.html> ;
  skos:member <http://anzsoil.org/def/au/scma/10A1> ;
  skos:member <http://anzsoil.org/def/au/scma/10A2> ;
  skos:member <http://anzsoil.org/def/au/scma/10B> ;
  skos:member <http://anzsoil.org/def/au/scma/10B1> ;
  skos:member <http://anzsoil.org/def/au/scma/10B2> ;
  skos:member <http://anzsoil.org/def/au/scma/10B3> ;
  skos:member <http://anzsoil.org/def/au/scma/10B4> ;
  skos:member <http://anzsoil.org/def/au/scma/10C1> ;
  skos:member <http://anzsoil.org/def/au/scma/10D1> ;
  skos:notation "10" ;
  skos:prefLabel "Sulfur" ;
.
<http://anzsoil.org/def/au/scma/10A1>
  a skos:Concept ;
  a sosa:Procedure ;
  dct:identifier "http://anzsoil.org/def/au/scma/10A1"^^xsd:anyURI ;
  dct:source "URN:ISBN:978-0-643-10218-7" ;
  skos:definition <https://raw.githack.com/ANZSoilData/def-au-scma/master/html/10-S/10A1.html> ;
  skos:inScheme s:scma-2011 ;
  skos:inScheme s:swcm-1992 ;
  skos:notation "10A1" ;
  skos:prefLabel "Total S - X-ray fluorescence" ;
  skos:topConceptOf s:scma-2011 ;
  skos:topConceptOf s:swcm-1992 ;
.
<http://anzsoil.org/def/au/scma/10A2>
  a skos:Concept ;
  a sosa:Procedure ;
  dct:identifier "http://anzsoil.org/def/au/scma/10A2"^^xsd:anyURI ;
  dct:source "URN:ISBN:978-0-643-10218-7" ;
  skos:definition <https://raw.githack.com/ANZSoilData/def-au-scma/master/html/10-S/10A2.html> ;
  skos:inScheme s:scma-2011 ;
  skos:inScheme s:swcm-1992 ;
  skos:notation "10A2" ;
  skos:prefLabel "Total soil S - high-temperature combustion" ;
  skos:topConceptOf s:scma-2011 ;
  skos:topConceptOf s:swcm-1992 ;
.
<http://anzsoil.org/def/au/scma/10B>
  a skos:Concept ;
  a sosa:Procedure ;
  dct:identifier "http://anzsoil.org/def/au/scma/10B"^^xsd:anyURI ;
  dct:source "URN:ISBN:978-0-643-10218-7" ;
  skos:definition <https://raw.githack.com/ANZSoilData/def-au-scma/master/html/10-S/10B.html> ;
  skos:inScheme s:scma-2011 ;
  skos:inScheme s:swcm-1992 ;
  skos:narrower <http://anzsoil.org/def/au/scma/10B1> ;
  skos:narrower <http://anzsoil.org/def/au/scma/10B2> ;
  skos:narrower <http://anzsoil.org/def/au/scma/10B3> ;
  skos:narrower <http://anzsoil.org/def/au/scma/10B4> ;
  skos:notation "10B" ;
  skos:prefLabel "Calcium phosphate-extractable S" ;
  skos:topConceptOf s:scma-2011 ;
  skos:topConceptOf s:swcm-1992 ;
.
<http://anzsoil.org/def/au/scma/10B1>
  a skos:Concept ;
  a sosa:Procedure ;
  dct:identifier "http://anzsoil.org/def/au/scma/10B1"^^xsd:anyURI ;
  dct:source "URN:ISBN:978-0-643-10218-7" ;
  skos:broader <http://anzsoil.org/def/au/scma/10B> ;
  skos:definition <https://raw.githack.com/ANZSoilData/def-au-scma/master/html/10-S/10B1.html> ;
  skos:inScheme s:scma-2011 ;
  skos:inScheme s:swcm-1992 ;
  skos:notation "10B1" ;
  skos:prefLabel "Calcium phosphate-extractable S - manual distillation" ;
.
<http://anzsoil.org/def/au/scma/10B2>
  a skos:Concept ;
  a sosa:Procedure ;
  dct:identifier "http://anzsoil.org/def/au/scma/10B2"^^xsd:anyURI ;
  dct:source "URN:ISBN:978-0-643-10218-7" ;
  skos:broader <http://anzsoil.org/def/au/scma/10B> ;
  skos:definition <https://raw.githack.com/ANZSoilData/def-au-scma/master/html/10-S/10B2.html> ;
  skos:inScheme s:scma-2011 ;
  skos:inScheme s:swcm-1992 ;
  skos:notation "10B2" ;
  skos:prefLabel "Calcium phosphate-extractable S - automated distillation" ;
.
<http://anzsoil.org/def/au/scma/10B3>
  a skos:Concept ;
  a sosa:Procedure ;
  dct:identifier "http://anzsoil.org/def/au/scma/10B3"^^xsd:anyURI ;
  dct:source "URN:ISBN:978-0-643-10218-7" ;
  skos:broader <http://anzsoil.org/def/au/scma/10B> ;
  skos:definition <https://raw.githack.com/ANZSoilData/def-au-scma/master/html/10-S/10B3.html> ;
  skos:inScheme s:scma-2011 ;
  skos:inScheme s:swcm-1992 ;
  skos:notation "10B3" ;
  skos:prefLabel "Calcium phosphate-extractable S - ICPAES" ;
.
<http://anzsoil.org/def/au/scma/10B4>
  a skos:Concept ;
  a sosa:Procedure ;
  dct:identifier "http://anzsoil.org/def/au/scma/10B4"^^xsd:anyURI ;
  dct:source "URN:ISBN:978-0-643-10218-7" ;
  skos:broader <http://anzsoil.org/def/au/scma/10B> ;
  skos:definition <https://raw.githack.com/ANZSoilData/def-au-scma/master/html/10-S/10B4.html> ;
  skos:inScheme s:scma-2011 ;
  skos:inScheme s:swcm-1992 ;
  skos:notation "10B4" ;
  skos:prefLabel "Calcium phosphate-extractable S - ion chromatography" ;
.
<http://anzsoil.org/def/au/scma/10C1>
  a skos:Concept ;
  a sosa:Procedure ;
  dct:identifier "http://anzsoil.org/def/au/scma/10C1"^^xsd:anyURI ;
  dct:source "URN:ISBN:978-0-643-10218-7" ;
  skos:definition <https://raw.githack.com/ANZSoilData/def-au-scma/master/html/10-S/10C1.html> ;
  skos:inScheme s:scma-2011 ;
  skos:inScheme s:swcm-1992 ;
  skos:notation "10C1" ;
  skos:prefLabel "Calcium phosphate-extractable S - ICPAES, + charcoal (CPC-S)" ;
  skos:topConceptOf s:scma-2011 ;
  skos:topConceptOf s:swcm-1992 ;
.
<http://anzsoil.org/def/au/scma/10D1>
  a skos:Concept ;
  a sosa:Procedure ;
  dct:identifier "http://anzsoil.org/def/au/scma/10D1"^^xsd:anyURI ;
  dct:source "URN:ISBN:978-0-643-10218-7" ;
  skos:definition <https://raw.githack.com/ANZSoilData/def-au-scma/master/html/10-S/10D1.html> ;
  skos:inScheme s:scma-2011 ;
  skos:inScheme s:swcm-1992 ;
  skos:notation "10D1" ;
  skos:prefLabel "Potassium Chloride - 40 Sulfur (KCl-40)-S" ;
  skos:topConceptOf s:scma-2011 ;
  skos:topConceptOf s:swcm-1992 ;
.
<http://anzsoil.org/def/au/scma/11>
  a skos:Collection ;
  dct:identifier "http://anzsoil.org/def/au/scma/11"^^xsd:anyURI ;
  dct:source "URN:ISBN:978-0-643-10218-7" ;
  skos:definition <https://raw.githack.com/ANZSoilData/def-au-scma/master/html/11-gypsum/11.html> ;
  skos:member <http://anzsoil.org/def/au/scma/11A1> ;
  skos:member <http://anzsoil.org/def/au/scma/11A2> ;
  skos:notation "11" ;
  skos:prefLabel "Gypsum" ;
.
<http://anzsoil.org/def/au/scma/11A1>
  a skos:Concept ;
  a sosa:Procedure ;
  dct:identifier "http://anzsoil.org/def/au/scma/11A1"^^xsd:anyURI ;
  dct:source "URN:ISBN:978-0-643-10218-7" ;
  skos:definition <https://raw.githack.com/ANZSoilData/def-au-scma/master/html/11-gypsum/11A1.html> ;
  skos:inScheme s:scma-2011 ;
  skos:inScheme s:swcm-1992 ;
  skos:notation "11A1" ;
  skos:prefLabel "Total gypsum" ;
  skos:topConceptOf s:scma-2011 ;
  skos:topConceptOf s:swcm-1992 ;
.
<http://anzsoil.org/def/au/scma/11A2>
  a skos:Concept ;
  a sosa:Procedure ;
  dct:identifier "http://anzsoil.org/def/au/scma/11A2"^^xsd:anyURI ;
  dct:source "URN:ISBN:978-0-643-10218-7" ;
  skos:definition <https://raw.githack.com/ANZSoilData/def-au-scma/master/html/11-gypsum/11A2.html> ;
  skos:inScheme s:scma-2011 ;
  skos:inScheme s:swcm-1992 ;
  skos:notation "11A2" ;
  skos:prefLabel "Total gypsum by MIR reflectance spectroscopy" ;
  skos:topConceptOf s:scma-2011 ;
  skos:topConceptOf s:swcm-1992 ;
.
<http://anzsoil.org/def/au/scma/12>
  a skos:Collection ;
  dct:identifier "http://anzsoil.org/def/au/scma/12"^^xsd:anyURI ;
  dct:source "URN:ISBN:978-0-643-10218-7" ;
  skos:definition <https://raw.githack.com/ANZSoilData/def-au-scma/master/html/12-micronutrients/12.html> ;
  skos:member <http://anzsoil.org/def/au/scma/12A1> ;
  skos:member <http://anzsoil.org/def/au/scma/12B1> ;
  skos:member <http://anzsoil.org/def/au/scma/12C1> ;
  skos:member <http://anzsoil.org/def/au/scma/12C2> ;
  skos:member <http://anzsoil.org/def/au/scma/12D1> ;
  skos:member <http://anzsoil.org/def/au/scma/12E1> ;
  skos:notation "12" ;
  skos:prefLabel "Micronutrients" ;
.
<http://anzsoil.org/def/au/scma/12A1>
  a skos:Concept ;
  a sosa:Procedure ;
  dct:identifier "http://anzsoil.org/def/au/scma/12A1"^^xsd:anyURI ;
  dct:source "URN:ISBN:978-0-643-10218-7" ;
  skos:definition <https://raw.githack.com/ANZSoilData/def-au-scma/master/html/12-micronutrients/12A1.html> ;
  skos:inScheme s:scma-2011 ;
  skos:inScheme s:swcm-1992 ;
  skos:notation "12A1" ;
  skos:prefLabel "DTPA-extractable Cu, Zn, Mn and Fe" ;
  skos:topConceptOf s:scma-2011 ;
  skos:topConceptOf s:swcm-1992 ;
.
<http://anzsoil.org/def/au/scma/12B1>
  a skos:Concept ;
  a sosa:Procedure ;
  dct:identifier "http://anzsoil.org/def/au/scma/12B1"^^xsd:anyURI ;
  dct:source "URN:ISBN:978-0-643-10218-7" ;
  skos:definition <https://raw.githack.com/ANZSoilData/def-au-scma/master/html/12-micronutrients/12B1.html> ;
  skos:inScheme s:scma-2011 ;
  skos:inScheme s:swcm-1992 ;
  skos:notation "12B1" ;
  skos:prefLabel "Ammonium bicarbonate/EDTA-extractable Cu and Zn" ;
  skos:topConceptOf s:scma-2011 ;
  skos:topConceptOf s:swcm-1992 ;
.
<http://anzsoil.org/def/au/scma/12C1>
  a skos:Concept ;
  a sosa:Procedure ;
  dct:identifier "http://anzsoil.org/def/au/scma/12C1"^^xsd:anyURI ;
  dct:source "URN:ISBN:978-0-643-10218-7" ;
  skos:definition <https://raw.githack.com/ANZSoilData/def-au-scma/master/html/12-micronutrients/12C1.html> ;
  skos:inScheme s:scma-2011 ;
  skos:inScheme s:swcm-1992 ;
  skos:notation "12C1" ;
  skos:prefLabel "Calcium chloride-extractable B - manual colour" ;
  skos:topConceptOf s:scma-2011 ;
  skos:topConceptOf s:swcm-1992 ;
.
<http://anzsoil.org/def/au/scma/12C2>
  a skos:Concept ;
  a sosa:Procedure ;
  dct:identifier "http://anzsoil.org/def/au/scma/12C2"^^xsd:anyURI ;
  dct:source "URN:ISBN:978-0-643-10218-7" ;
  skos:definition <https://raw.githack.com/ANZSoilData/def-au-scma/master/html/12-micronutrients/12C2.html> ;
  skos:inScheme s:scma-2011 ;
  skos:inScheme s:swcm-1992 ;
  skos:notation "12C2" ;
  skos:prefLabel "Calcium chloride-extractable B - ICPAES" ;
  skos:topConceptOf s:scma-2011 ;
  skos:topConceptOf s:swcm-1992 ;
.
<http://anzsoil.org/def/au/scma/12D1>
  a skos:Concept ;
  a sosa:Procedure ;
  dct:identifier "http://anzsoil.org/def/au/scma/12D1"^^xsd:anyURI ;
  dct:source "URN:ISBN:978-0-643-10218-7" ;
  skos:definition <https://raw.githack.com/ANZSoilData/def-au-scma/master/html/12-micronutrients/12D1.html> ;
  skos:inScheme s:scma-2011 ;
  skos:inScheme s:swcm-1992 ;
  skos:notation "12D1" ;
  skos:prefLabel "0.1 M HCl-extractable Cu, Zn, Mn and Fe" ;
  skos:topConceptOf s:scma-2011 ;
  skos:topConceptOf s:swcm-1992 ;
.
<http://anzsoil.org/def/au/scma/12E1>
  a skos:Concept ;
  a sosa:Procedure ;
  dct:identifier "http://anzsoil.org/def/au/scma/12E1"^^xsd:anyURI ;
  dct:source "URN:ISBN:978-0-643-10218-7" ;
  skos:definition <https://raw.githack.com/ANZSoilData/def-au-scma/master/html/12-micronutrients/12E1.html> ;
  skos:inScheme s:scma-2011 ;
  skos:inScheme s:swcm-1992 ;
  skos:notation "12E1" ;
  skos:prefLabel "Calcium chloride-extractable Mo" ;
  skos:topConceptOf s:scma-2011 ;
  skos:topConceptOf s:swcm-1992 ;
.
<http://anzsoil.org/def/au/scma/13>
  a skos:Collection ;
  dct:identifier "http://anzsoil.org/def/au/scma/13"^^xsd:anyURI ;
  dct:source "URN:ISBN:978-0-643-10218-7" ;
  skos:definition <https://raw.githack.com/ANZSoilData/def-au-scma/master/html/13-extractable-Fe-Al-Si/13.html> ;
  skos:member <http://anzsoil.org/def/au/scma/13A1> ;
  skos:member <http://anzsoil.org/def/au/scma/13B1> ;
  skos:member <http://anzsoil.org/def/au/scma/13C1> ;
  skos:member <http://anzsoil.org/def/au/scma/13D> ;
  skos:member <http://anzsoil.org/def/au/scma/13D1> ;
  skos:member <http://anzsoil.org/def/au/scma/13D2> ;
  skos:notation "13" ;
  skos:prefLabel "Extractable iron, aluminium and silicon" ;
.
<http://anzsoil.org/def/au/scma/13A1>
  a skos:Concept ;
  a sosa:Procedure ;
  dct:identifier "http://anzsoil.org/def/au/scma/13A1"^^xsd:anyURI ;
  dct:source "URN:ISBN:978-0-643-10218-7" ;
  skos:definition <https://raw.githack.com/ANZSoilData/def-au-scma/master/html/13-extractable-Fe-Al-Si/13A1.html> ;
  skos:inScheme s:scma-2011 ;
  skos:inScheme s:swcm-1992 ;
  skos:notation "13A1" ;
  skos:prefLabel "Oxalate-extractable iron, aluminium and silicon" ;
  skos:topConceptOf s:scma-2011 ;
  skos:topConceptOf s:swcm-1992 ;
.
<http://anzsoil.org/def/au/scma/13B1>
  a skos:Concept ;
  a sosa:Procedure ;
  dct:identifier "http://anzsoil.org/def/au/scma/13B1"^^xsd:anyURI ;
  dct:source "URN:ISBN:978-0-643-10218-7" ;
  skos:definition <https://raw.githack.com/ANZSoilData/def-au-scma/master/html/13-extractable-Fe-Al-Si/13B1.html> ;
  skos:inScheme s:scma-2011 ;
  skos:inScheme s:swcm-1992 ;
  skos:notation "13B1" ;
  skos:prefLabel "Pyrophosphate-extractable Fe and Al" ;
  skos:topConceptOf s:scma-2011 ;
  skos:topConceptOf s:swcm-1992 ;
.
<http://anzsoil.org/def/au/scma/13C1>
  a skos:Concept ;
  a sosa:Procedure ;
  dct:identifier "http://anzsoil.org/def/au/scma/13C1"^^xsd:anyURI ;
  dct:source "URN:ISBN:978-0-643-10218-7" ;
  skos:definition <https://raw.githack.com/ANZSoilData/def-au-scma/master/html/13-extractable-Fe-Al-Si/13C1.html> ;
  skos:inScheme s:scma-2011 ;
  skos:inScheme s:swcm-1992 ;
  skos:notation "13C1" ;
  skos:prefLabel "Citrate/dihionite-extractable iron and aluminium" ;
  skos:topConceptOf s:scma-2011 ;
  skos:topConceptOf s:swcm-1992 ;
.
<http://anzsoil.org/def/au/scma/13D>
  a skos:Concept ;
  a sosa:Procedure ;
  dct:identifier "http://anzsoil.org/def/au/scma/13D"^^xsd:anyURI ;
  dct:source "URN:ISBN:978-0-643-10218-7" ;
  skos:definition <https://raw.githack.com/ANZSoilData/def-au-scma/master/html/13-extractable-Fe-Al-Si/13D.html> ;
  skos:inScheme s:scma-2011 ;
  skos:inScheme s:swcm-1992 ;
  skos:narrower <http://anzsoil.org/def/au/scma/13D1> ;
  skos:narrower <http://anzsoil.org/def/au/scma/13D2> ;
  skos:notation "13D" ;
  skos:prefLabel "Acid-extractable soil silicon" ;
  skos:topConceptOf s:scma-2011 ;
  skos:topConceptOf s:swcm-1992 ;
.
<http://anzsoil.org/def/au/scma/13D1>
  a skos:Concept ;
  a sosa:Procedure ;
  dct:identifier "http://anzsoil.org/def/au/scma/13D1"^^xsd:anyURI ;
  dct:source "URN:ISBN:978-0-643-10218-7" ;
  skos:broader <http://anzsoil.org/def/au/scma/13D> ;
  skos:definition <https://raw.githack.com/ANZSoilData/def-au-scma/master/html/13-extractable-Fe-Al-Si/13D1.html> ;
  skos:inScheme s:scma-2011 ;
  skos:inScheme s:swcm-1992 ;
  skos:notation "13D1" ;
  skos:prefLabel "Acid-extractable soil silicon - automated colour" ;
.
<http://anzsoil.org/def/au/scma/13D2>
  a skos:Concept ;
  a sosa:Procedure ;
  dct:identifier "http://anzsoil.org/def/au/scma/13D2"^^xsd:anyURI ;
  dct:source "URN:ISBN:978-0-643-10218-7" ;
  skos:broader <http://anzsoil.org/def/au/scma/13D> ;
  skos:definition <https://raw.githack.com/ANZSoilData/def-au-scma/master/html/13-extractable-Fe-Al-Si/13D2.html> ;
  skos:inScheme s:scma-2011 ;
  skos:inScheme s:swcm-1992 ;
  skos:notation "13D2" ;
  skos:prefLabel "Acid-extractable soil silicon - ICPAES" ;
.
<http://anzsoil.org/def/au/scma/14>
  a skos:Collection ;
  dct:identifier "http://anzsoil.org/def/au/scma/14"^^xsd:anyURI ;
  dct:source "URN:ISBN:978-0-643-10218-7" ;
  skos:definition <https://raw.githack.com/ANZSoilData/def-au-scma/master/html/14-saturation-extracts/14.html> ;
  skos:member <http://anzsoil.org/def/au/scma/14A1> ;
  skos:member <http://anzsoil.org/def/au/scma/14A2> ;
  skos:member <http://anzsoil.org/def/au/scma/14A3> ;
  skos:member <http://anzsoil.org/def/au/scma/14A4> ;
  skos:member <http://anzsoil.org/def/au/scma/14B1> ;
  skos:member <http://anzsoil.org/def/au/scma/14C1> ;
  skos:member <http://anzsoil.org/def/au/scma/14D1> ;
  skos:member <http://anzsoil.org/def/au/scma/14D2> ;
  skos:member <http://anzsoil.org/def/au/scma/14E1> ;
  skos:member <http://anzsoil.org/def/au/scma/14E2> ;
  skos:member <http://anzsoil.org/def/au/scma/14E2a> ;
  skos:member <http://anzsoil.org/def/au/scma/14E2b> ;
  skos:member <http://anzsoil.org/def/au/scma/14E3> ;
  skos:member <http://anzsoil.org/def/au/scma/14F1> ;
  skos:member <http://anzsoil.org/def/au/scma/14F2> ;
  skos:member <http://anzsoil.org/def/au/scma/14F3> ;
  skos:member <http://anzsoil.org/def/au/scma/14F4> ;
  skos:member <http://anzsoil.org/def/au/scma/14F5> ;
  skos:member <http://anzsoil.org/def/au/scma/14F5a> ;
  skos:member <http://anzsoil.org/def/au/scma/14F5b> ;
  skos:member <http://anzsoil.org/def/au/scma/14G1> ;
  skos:member <http://anzsoil.org/def/au/scma/14G2> ;
  skos:member <http://anzsoil.org/def/au/scma/14G2a> ;
  skos:member <http://anzsoil.org/def/au/scma/14G2b> ;
  skos:member <http://anzsoil.org/def/au/scma/14H1> ;
  skos:notation "14" ;
  skos:prefLabel "Saturation extracts" ;
.
<http://anzsoil.org/def/au/scma/14A1>
  a skos:Concept ;
  a sosa:Procedure ;
  dct:identifier "http://anzsoil.org/def/au/scma/14A1"^^xsd:anyURI ;
  dct:source "URN:ISBN:978-0-643-10218-7" ;
  skos:definition <https://raw.githack.com/ANZSoilData/def-au-scma/master/html/14-saturation-extracts/14A1.html> ;
  skos:inScheme s:scma-2011 ;
  skos:inScheme s:swcm-1992 ;
  skos:notation "14A1" ;
  skos:prefLabel "Saturation extract - filter suction" ;
  skos:topConceptOf s:scma-2011 ;
  skos:topConceptOf s:swcm-1992 ;
.
<http://anzsoil.org/def/au/scma/14A2>
  a skos:Concept ;
  a sosa:Procedure ;
  dct:identifier "http://anzsoil.org/def/au/scma/14A2"^^xsd:anyURI ;
  dct:source "URN:ISBN:978-0-643-10218-7" ;
  skos:definition <https://raw.githack.com/ANZSoilData/def-au-scma/master/html/14-saturation-extracts/14A2.html> ;
  skos:inScheme s:scma-2011 ;
  skos:inScheme s:swcm-1992 ;
  skos:notation "14A2" ;
  skos:prefLabel "Saturation extract -automatic extractor" ;
  skos:topConceptOf s:scma-2011 ;
  skos:topConceptOf s:swcm-1992 ;
.
<http://anzsoil.org/def/au/scma/14A3>
  a skos:Concept ;
  a sosa:Procedure ;
  dct:identifier "http://anzsoil.org/def/au/scma/14A3"^^xsd:anyURI ;
  dct:source "URN:ISBN:978-0-643-10218-7" ;
  skos:definition <https://raw.githack.com/ANZSoilData/def-au-scma/master/html/14-saturation-extracts/14A3.html> ;
  skos:inScheme s:scma-2011 ;
  skos:inScheme s:swcm-1992 ;
  skos:notation "14A3" ;
  skos:prefLabel "Saturation extract - centrifuge, closed system" ;
  skos:topConceptOf s:scma-2011 ;
  skos:topConceptOf s:swcm-1992 ;
.
<http://anzsoil.org/def/au/scma/14A4>
  a skos:Concept ;
  a sosa:Procedure ;
  dct:identifier "http://anzsoil.org/def/au/scma/14A4"^^xsd:anyURI ;
  dct:source "URN:ISBN:978-0-643-10218-7" ;
  skos:definition <https://raw.githack.com/ANZSoilData/def-au-scma/master/html/14-saturation-extracts/14A4.html> ;
  skos:inScheme s:scma-2011 ;
  skos:inScheme s:swcm-1992 ;
  skos:notation "14A4" ;
  skos:prefLabel "Saturation extract - centrifuge, Gillman" ;
  skos:topConceptOf s:scma-2011 ;
  skos:topConceptOf s:swcm-1992 ;
.
<http://anzsoil.org/def/au/scma/14B1>
  a skos:Concept ;
  a sosa:Procedure ;
  dct:identifier "http://anzsoil.org/def/au/scma/14B1"^^xsd:anyURI ;
  dct:source "URN:ISBN:978-0-643-10218-7" ;
  skos:definition <https://raw.githack.com/ANZSoilData/def-au-scma/master/html/14-saturation-extracts/14B1.html> ;
  skos:inScheme s:scma-2011 ;
  skos:inScheme s:swcm-1992 ;
  skos:notation "14B1" ;
  skos:prefLabel "Electrical conductivity of SE (EC of SE)" ;
  skos:topConceptOf s:scma-2011 ;
  skos:topConceptOf s:swcm-1992 ;
.
<http://anzsoil.org/def/au/scma/14C1>
  a skos:Concept ;
  a sosa:Procedure ;
  dct:identifier "http://anzsoil.org/def/au/scma/14C1"^^xsd:anyURI ;
  dct:source "URN:ISBN:978-0-643-10218-7" ;
  skos:definition <https://raw.githack.com/ANZSoilData/def-au-scma/master/html/14-saturation-extracts/14C1.html> ;
  skos:inScheme s:scma-2011 ;
  skos:inScheme s:swcm-1992 ;
  skos:notation "14C1" ;
  skos:prefLabel "pH of SE" ;
  skos:topConceptOf s:scma-2011 ;
  skos:topConceptOf s:swcm-1992 ;
.
<http://anzsoil.org/def/au/scma/14D1>
  a skos:Concept ;
  a sosa:Procedure ;
  dct:identifier "http://anzsoil.org/def/au/scma/14D1"^^xsd:anyURI ;
  dct:source "URN:ISBN:978-0-643-10218-7" ;
  skos:definition <https://raw.githack.com/ANZSoilData/def-au-scma/master/html/14-saturation-extracts/14D1.html> ;
  skos:inScheme s:scma-2011 ;
  skos:inScheme s:swcm-1992 ;
  skos:notation "14D1" ;
  skos:prefLabel "Bicarbonate of SE and carbonate of SE - potentiometric titration" ;
  skos:topConceptOf s:scma-2011 ;
  skos:topConceptOf s:swcm-1992 ;
.
<http://anzsoil.org/def/au/scma/14D2>
  a skos:Concept ;
  a sosa:Procedure ;
  dct:identifier "http://anzsoil.org/def/au/scma/14D2"^^xsd:anyURI ;
  dct:source "URN:ISBN:978-0-643-10218-7" ;
  skos:definition <https://raw.githack.com/ANZSoilData/def-au-scma/master/html/14-saturation-extracts/14D2.html> ;
  skos:inScheme s:scma-2011 ;
  skos:inScheme s:swcm-1992 ;
  skos:notation "14D2" ;
  skos:prefLabel "Bicarbonate of SE and carbonate of SE - indicator method" ;
  skos:topConceptOf s:scma-2011 ;
  skos:topConceptOf s:swcm-1992 ;
.
<http://anzsoil.org/def/au/scma/14E1>
  a skos:Concept ;
  a sosa:Procedure ;
  dct:identifier "http://anzsoil.org/def/au/scma/14E1"^^xsd:anyURI ;
  dct:source "URN:ISBN:978-0-643-10218-7" ;
  skos:definition <https://raw.githack.com/ANZSoilData/def-au-scma/master/html/14-saturation-extracts/14E1.html> ;
  skos:inScheme s:scma-2011 ;
  skos:inScheme s:swcm-1992 ;
  skos:notation "14E1" ;
  skos:prefLabel "Chloride of SE - potentiometric titration" ;
  skos:topConceptOf s:scma-2011 ;
  skos:topConceptOf s:swcm-1992 ;
.
<http://anzsoil.org/def/au/scma/14E2>
  a skos:Concept ;
  a sosa:Procedure ;
  dct:identifier "http://anzsoil.org/def/au/scma/14E2"^^xsd:anyURI ;
  dct:isReplacedBy <http://anzsoil.org/def/au/scma/14E2a> ;
  dct:isReplacedBy <http://anzsoil.org/def/au/scma/14E2b> ;
  dct:source "URN:ISBN:978-0-909605-68-1" ;
  skos:inScheme s:scma-2011 ;
  skos:inScheme s:swcm-1992 ;
  skos:narrower <http://anzsoil.org/def/au/scma/14E2a> ;
  skos:narrower <http://anzsoil.org/def/au/scma/14E2b> ;
  skos:notation "14E2" ;
  skos:prefLabel "Chloride (saturation extract) - ion chromotography|Chloride of SE - IC" ;
  skos:topConceptOf s:scma-2011 ;
  skos:topConceptOf s:swcm-1992 ;
.
<http://anzsoil.org/def/au/scma/14E2a>
  a skos:Concept ;
  a sosa:Procedure ;
  dct:identifier "http://anzsoil.org/def/au/scma/14E2a"^^xsd:anyURI ;
  dct:source "URN:ISBN:978-0-643-10218-7" ;
  skos:broader <http://anzsoil.org/def/au/scma/14E2> ;
  skos:definition <https://raw.githack.com/ANZSoilData/def-au-scma/master/html/14-saturation-extracts/14E2a.html> ;
  skos:inScheme s:scma-2011 ;
  skos:inScheme s:swcm-1992 ;
  skos:notation "14E2a" ;
  skos:prefLabel "Chloride of SE - IC (chemical suppression of eluent conductivity)" ;
.
<http://anzsoil.org/def/au/scma/14E2b>
  a skos:Concept ;
  a sosa:Procedure ;
  dct:identifier "http://anzsoil.org/def/au/scma/14E2b"^^xsd:anyURI ;
  dct:source "URN:ISBN:978-0-643-10218-7" ;
  skos:broader <http://anzsoil.org/def/au/scma/14E2> ;
  skos:definition <https://raw.githack.com/ANZSoilData/def-au-scma/master/html/14-saturation-extracts/14E2b.html> ;
  skos:inScheme s:scma-2011 ;
  skos:inScheme s:swcm-1992 ;
  skos:notation "14E2b" ;
  skos:prefLabel "Chloride of SE - IC (single-column with electronic suppression of eluent conductivity)" ;
.
<http://anzsoil.org/def/au/scma/14E3>
  a skos:Concept ;
  a sosa:Procedure ;
  dct:identifier "http://anzsoil.org/def/au/scma/14E3"^^xsd:anyURI ;
  dct:source "URN:ISBN:978-0-643-10218-7" ;
  skos:definition <https://raw.githack.com/ANZSoilData/def-au-scma/master/html/14-saturation-extracts/14E3.html> ;
  skos:inScheme s:scma-2011 ;
  skos:inScheme s:swcm-1992 ;
  skos:notation "14E3" ;
  skos:prefLabel "Chloride of SE - ICPAES" ;
  skos:topConceptOf s:scma-2011 ;
  skos:topConceptOf s:swcm-1992 ;
.
<http://anzsoil.org/def/au/scma/14F1>
  a skos:Concept ;
  a sosa:Procedure ;
  dct:identifier "http://anzsoil.org/def/au/scma/14F1"^^xsd:anyURI ;
  dct:source "URN:ISBN:978-0-643-10218-7" ;
  skos:definition <https://raw.githack.com/ANZSoilData/def-au-scma/master/html/14-saturation-extracts/14F1.html> ;
  skos:inScheme s:scma-2011 ;
  skos:inScheme s:swcm-1992 ;
  skos:notation "14F1" ;
  skos:prefLabel "Sulfate-S of SE - ICPAES (plus P and soluble cations)" ;
  skos:topConceptOf s:scma-2011 ;
  skos:topConceptOf s:swcm-1992 ;
.
<http://anzsoil.org/def/au/scma/14F2>
  a skos:Concept ;
  a sosa:Procedure ;
  dct:identifier "http://anzsoil.org/def/au/scma/14F2"^^xsd:anyURI ;
  dct:source "URN:ISBN:978-0-643-10218-7" ;
  skos:definition <https://raw.githack.com/ANZSoilData/def-au-scma/master/html/14-saturation-extracts/14F2.html> ;
  skos:inScheme s:scma-2011 ;
  skos:inScheme s:swcm-1992 ;
  skos:notation "14F2" ;
  skos:prefLabel "Sulfate-S of SE - turbidimetric" ;
  skos:topConceptOf s:scma-2011 ;
  skos:topConceptOf s:swcm-1992 ;
.
<http://anzsoil.org/def/au/scma/14F3>
  a skos:Concept ;
  a sosa:Procedure ;
  dct:identifier "http://anzsoil.org/def/au/scma/14F3"^^xsd:anyURI ;
  dct:source "URN:ISBN:978-0-643-10218-7" ;
  skos:definition <https://raw.githack.com/ANZSoilData/def-au-scma/master/html/14-saturation-extracts/14F3.html> ;
  skos:inScheme s:scma-2011 ;
  skos:inScheme s:swcm-1992 ;
  skos:notation "14F3" ;
  skos:prefLabel "Sulfate-S of SE - gravimetric" ;
  skos:topConceptOf s:scma-2011 ;
  skos:topConceptOf s:swcm-1992 ;
.
<http://anzsoil.org/def/au/scma/14F4>
  a skos:Concept ;
  a sosa:Procedure ;
  dct:identifier "http://anzsoil.org/def/au/scma/14F4"^^xsd:anyURI ;
  dct:source "URN:ISBN:978-0-643-10218-7" ;
  skos:definition <https://raw.githack.com/ANZSoilData/def-au-scma/master/html/14-saturation-extracts/14F4.html> ;
  skos:inScheme s:scma-2011 ;
  skos:inScheme s:swcm-1992 ;
  skos:notation "14F4" ;
  skos:prefLabel "Sulfate-S of SE - automated colour" ;
  skos:topConceptOf s:scma-2011 ;
  skos:topConceptOf s:swcm-1992 ;
.
<http://anzsoil.org/def/au/scma/14F5>
  a skos:Concept ;
  a sosa:Procedure ;
  dct:identifier "http://anzsoil.org/def/au/scma/14F5"^^xsd:anyURI ;
  dct:isReplacedBy <http://anzsoil.org/def/au/scma/14F5a> ;
  dct:isReplacedBy <http://anzsoil.org/def/au/scma/14F5b> ;
  dct:source "URN:ISBN:978-0-909605-68-1" ;
  skos:inScheme s:scma-2011 ;
  skos:inScheme s:swcm-1992 ;
  skos:narrower <http://anzsoil.org/def/au/scma/14F5a> ;
  skos:narrower <http://anzsoil.org/def/au/scma/14F5b> ;
  skos:notation "14F5" ;
  skos:prefLabel "Sulfate-S (saturation extract) - ion chromotography|Sulfate-S of SE - IC" ;
  skos:topConceptOf s:scma-2011 ;
  skos:topConceptOf s:swcm-1992 ;
.
<http://anzsoil.org/def/au/scma/14F5a>
  a skos:Concept ;
  a sosa:Procedure ;
  dct:identifier "http://anzsoil.org/def/au/scma/14F5a"^^xsd:anyURI ;
  dct:source "URN:ISBN:978-0-643-10218-7" ;
  skos:broader <http://anzsoil.org/def/au/scma/14F5> ;
  skos:definition <https://raw.githack.com/ANZSoilData/def-au-scma/master/html/14-saturation-extracts/14F5a.html> ;
  skos:inScheme s:scma-2011 ;
  skos:inScheme s:swcm-1992 ;
  skos:notation "14F5a" ;
  skos:prefLabel "Sulfate-S of SE - IC (chemical suppression of eluent conductivity)" ;
.
<http://anzsoil.org/def/au/scma/14F5b>
  a skos:Concept ;
  a sosa:Procedure ;
  dct:identifier "http://anzsoil.org/def/au/scma/14F5b"^^xsd:anyURI ;
  dct:source "URN:ISBN:978-0-643-10218-7" ;
  skos:broader <http://anzsoil.org/def/au/scma/14F5> ;
  skos:definition <https://raw.githack.com/ANZSoilData/def-au-scma/master/html/14-saturation-extracts/14F5b.html> ;
  skos:inScheme s:scma-2011 ;
  skos:inScheme s:swcm-1992 ;
  skos:notation "14F5b" ;
  skos:prefLabel "Sulfate-S of SE - IC (single-column with electronic suppression of eluent conductivity)" ;
.
<http://anzsoil.org/def/au/scma/14G1>
  a skos:Concept ;
  a sosa:Procedure ;
  dct:identifier "http://anzsoil.org/def/au/scma/14G1"^^xsd:anyURI ;
  dct:source "URN:ISBN:978-0-643-10218-7" ;
  skos:definition <https://raw.githack.com/ANZSoilData/def-au-scma/master/html/14-saturation-extracts/14G1.html> ;
  skos:inScheme s:scma-2011 ;
  skos:inScheme s:swcm-1992 ;
  skos:notation "14G1" ;
  skos:prefLabel "Fluoride of SE - specific ion electrode" ;
  skos:topConceptOf s:scma-2011 ;
  skos:topConceptOf s:swcm-1992 ;
.
<http://anzsoil.org/def/au/scma/14G2>
  a skos:Concept ;
  a sosa:Procedure ;
  dct:identifier "http://anzsoil.org/def/au/scma/14G2"^^xsd:anyURI ;
  dct:isReplacedBy <http://anzsoil.org/def/au/scma/14G2a> ;
  dct:isReplacedBy <http://anzsoil.org/def/au/scma/14G2b> ;
  dct:source "URN:ISBN:978-0-909605-68-1" ;
  skos:inScheme s:scma-2011 ;
  skos:inScheme s:swcm-1992 ;
  skos:narrower <http://anzsoil.org/def/au/scma/14G2a> ;
  skos:narrower <http://anzsoil.org/def/au/scma/14G2b> ;
  skos:notation "14G2" ;
  skos:prefLabel "Fluoride (saturation extract) - ion chromotography|Fluoride of SE - IC" ;
  skos:topConceptOf s:scma-2011 ;
  skos:topConceptOf s:swcm-1992 ;
.
<http://anzsoil.org/def/au/scma/14G2a>
  a skos:Concept ;
  a sosa:Procedure ;
  dct:identifier "http://anzsoil.org/def/au/scma/14G2a"^^xsd:anyURI ;
  dct:source "URN:ISBN:978-0-643-10218-7" ;
  skos:broader <http://anzsoil.org/def/au/scma/14G2> ;
  skos:definition <https://raw.githack.com/ANZSoilData/def-au-scma/master/html/14-saturation-extracts/14G2a.html> ;
  skos:inScheme s:scma-2011 ;
  skos:inScheme s:swcm-1992 ;
  skos:notation "14G2a" ;
  skos:prefLabel "Fluoride of SE - IC (chemical suppression of eluent conductivity)" ;
.
<http://anzsoil.org/def/au/scma/14G2b>
  a skos:Concept ;
  a sosa:Procedure ;
  dct:identifier "http://anzsoil.org/def/au/scma/14G2b"^^xsd:anyURI ;
  dct:source "URN:ISBN:978-0-643-10218-7" ;
  skos:broader <http://anzsoil.org/def/au/scma/14G2> ;
  skos:definition <https://raw.githack.com/ANZSoilData/def-au-scma/master/html/14-saturation-extracts/14G2b.html> ;
  skos:inScheme s:scma-2011 ;
  skos:inScheme s:swcm-1992 ;
  skos:notation "14G2b" ;
  skos:prefLabel "Fluoride of SE - IC (single-column with electronic suppression of eluent conductivity)" ;
.
<http://anzsoil.org/def/au/scma/14H1>
  a skos:Concept ;
  a sosa:Procedure ;
  dct:identifier "http://anzsoil.org/def/au/scma/14H1"^^xsd:anyURI ;
  dct:source "URN:ISBN:978-0-643-10218-7" ;
  skos:definition <https://raw.githack.com/ANZSoilData/def-au-scma/master/html/14-saturation-extracts/14H1.html> ;
  skos:inScheme s:scma-2011 ;
  skos:inScheme s:swcm-1992 ;
  skos:notation "14H1" ;
  skos:prefLabel "Soluble bases of SE (Ca, Mg, K, Na)" ;
  skos:topConceptOf s:scma-2011 ;
  skos:topConceptOf s:swcm-1992 ;
.
<http://anzsoil.org/def/au/scma/15>
  a skos:Collection ;
  dct:identifier "http://anzsoil.org/def/au/scma/15"^^xsd:anyURI ;
  dct:source "URN:ISBN:978-0-643-10218-7" ;
  skos:definition <https://raw.githack.com/ANZSoilData/def-au-scma/master/html/15-ion-exchange-properties/15.html> ;
  skos:member <http://anzsoil.org/def/au/scma/15A1> ;
  skos:member <http://anzsoil.org/def/au/scma/15A2> ;
  skos:member <http://anzsoil.org/def/au/scma/15A3> ;
  skos:member <http://anzsoil.org/def/au/scma/15B1> ;
  skos:member <http://anzsoil.org/def/au/scma/15B2> ;
  skos:member <http://anzsoil.org/def/au/scma/15B3> ;
  skos:member <http://anzsoil.org/def/au/scma/15C1> ;
  skos:member <http://anzsoil.org/def/au/scma/15C2> ;
  skos:member <http://anzsoil.org/def/au/scma/15D1> ;
  skos:member <http://anzsoil.org/def/au/scma/15D2> ;
  skos:member <http://anzsoil.org/def/au/scma/15D3> ;
  skos:member <http://anzsoil.org/def/au/scma/15E1> ;
  skos:member <http://anzsoil.org/def/au/scma/15E2> ;
  skos:member <http://anzsoil.org/def/au/scma/15E3> ;
  skos:member <http://anzsoil.org/def/au/scma/15F1> ;
  skos:member <http://anzsoil.org/def/au/scma/15F2> ;
  skos:member <http://anzsoil.org/def/au/scma/15F3> ;
  skos:member <http://anzsoil.org/def/au/scma/15G1> ;
  skos:member <http://anzsoil.org/def/au/scma/15H1> ;
  skos:member <http://anzsoil.org/def/au/scma/15I1> ;
  skos:member <http://anzsoil.org/def/au/scma/15I2> ;
  skos:member <http://anzsoil.org/def/au/scma/15I3> ;
  skos:member <http://anzsoil.org/def/au/scma/15I4> ;
  skos:member <http://anzsoil.org/def/au/scma/15J1> ;
  skos:member <http://anzsoil.org/def/au/scma/15K1> ;
  skos:member <http://anzsoil.org/def/au/scma/15L1> ;
  skos:member <http://anzsoil.org/def/au/scma/15M1> ;
  skos:member <http://anzsoil.org/def/au/scma/15N1> ;
  skos:member <http://anzsoil.org/def/au/scma/15O1> ;
  skos:notation "15" ;
  skos:prefLabel "Ion-exchange properties" ;
.
<http://anzsoil.org/def/au/scma/15A1>
  a skos:Concept ;
  a sosa:Procedure ;
  dct:identifier "http://anzsoil.org/def/au/scma/15A1"^^xsd:anyURI ;
  dct:source "URN:ISBN:978-0-643-10218-7" ;
  skos:definition <https://raw.githack.com/ANZSoilData/def-au-scma/master/html/15-ion-exchange-properties/15A1.html> ;
  skos:inScheme s:scma-2011 ;
  skos:inScheme s:swcm-1992 ;
  skos:notation "15A1" ;
  skos:prefLabel "Exchangeable bases (Ca2+, Mg2+, Na+, K+) - 1 M ammonium chloride at pH 7.0, no pre-treatment for soluble salts" ;
  skos:topConceptOf s:scma-2011 ;
  skos:topConceptOf s:swcm-1992 ;
.
<http://anzsoil.org/def/au/scma/15A2>
  a skos:Concept ;
  a sosa:Procedure ;
  dct:identifier "http://anzsoil.org/def/au/scma/15A2"^^xsd:anyURI ;
  dct:source "URN:ISBN:978-0-643-10218-7" ;
  skos:definition <https://raw.githack.com/ANZSoilData/def-au-scma/master/html/15-ion-exchange-properties/15A2.html> ;
  skos:inScheme s:scma-2011 ;
  skos:inScheme s:swcm-1992 ;
  skos:notation "15A2" ;
  skos:prefLabel "Exchangeable bases by 1 M ammonium chloride at pH 7.0, pre-treatment for soluble salts" ;
  skos:topConceptOf s:scma-2011 ;
  skos:topConceptOf s:swcm-1992 ;
.
<http://anzsoil.org/def/au/scma/15A3>
  a skos:Concept ;
  a sosa:Procedure ;
  dct:identifier "http://anzsoil.org/def/au/scma/15A3"^^xsd:anyURI ;
  dct:source "URN:ISBN:978-0-643-10218-7" ;
  skos:definition <https://raw.githack.com/ANZSoilData/def-au-scma/master/html/15-ion-exchange-properties/15A3.html> ;
  skos:inScheme s:scma-2011 ;
  skos:inScheme s:swcm-1992 ;
  skos:notation "15A3" ;
  skos:prefLabel "Exchangeable bases - 1 M ammonium chloride at pH 7.0, adjusted for soluble Na+" ;
  skos:topConceptOf s:scma-2011 ;
  skos:topConceptOf s:swcm-1992 ;
.
<http://anzsoil.org/def/au/scma/15B1>
  a skos:Concept ;
  a sosa:Procedure ;
  dct:identifier "http://anzsoil.org/def/au/scma/15B1"^^xsd:anyURI ;
  dct:source "URN:ISBN:978-0-643-10218-7" ;
  skos:definition <https://raw.githack.com/ANZSoilData/def-au-scma/master/html/15-ion-exchange-properties/15B1.html> ;
  skos:inScheme s:scma-2011 ;
  skos:inScheme s:swcm-1992 ;
  skos:notation "15B1" ;
  skos:prefLabel "Exchangeable bases and cation exchange capacity - 1 M ammonium chloride at pH 7.0, no pre-treatment for soluble salts" ;
  skos:topConceptOf s:scma-2011 ;
  skos:topConceptOf s:swcm-1992 ;
.
<http://anzsoil.org/def/au/scma/15B2>
  a skos:Concept ;
  a sosa:Procedure ;
  dct:identifier "http://anzsoil.org/def/au/scma/15B2"^^xsd:anyURI ;
  dct:source "URN:ISBN:978-0-643-10218-7" ;
  skos:definition <https://raw.githack.com/ANZSoilData/def-au-scma/master/html/15-ion-exchange-properties/15B2.html> ;
  skos:inScheme s:scma-2011 ;
  skos:inScheme s:swcm-1992 ;
  skos:notation "15B2" ;
  skos:prefLabel "Exchangeable bases and CEC - 1 M ammonium chloride at pH 7.0, pre-treatment for soluble salts" ;
  skos:topConceptOf s:scma-2011 ;
  skos:topConceptOf s:swcm-1992 ;
.
<http://anzsoil.org/def/au/scma/15B3>
  a skos:Concept ;
  a sosa:Procedure ;
  dct:identifier "http://anzsoil.org/def/au/scma/15B3"^^xsd:anyURI ;
  dct:source "URN:ISBN:978-0-643-10218-7" ;
  skos:definition <https://raw.githack.com/ANZSoilData/def-au-scma/master/html/15-ion-exchange-properties/15B3.html> ;
  skos:inScheme s:scma-2011 ;
  skos:inScheme s:swcm-1992 ;
  skos:notation "15B3" ;
  skos:prefLabel "Exchangeable bases and CEC - 1 M ammonium chloride at pH 7.0, adjusted for soluble Na+" ;
  skos:topConceptOf s:scma-2011 ;
  skos:topConceptOf s:swcm-1992 ;
.
<http://anzsoil.org/def/au/scma/15C1>
  a skos:Concept ;
  a sosa:Procedure ;
  dct:identifier "http://anzsoil.org/def/au/scma/15C1"^^xsd:anyURI ;
  dct:source "URN:ISBN:978-0-643-10218-7" ;
  skos:definition <https://raw.githack.com/ANZSoilData/def-au-scma/master/html/15-ion-exchange-properties/15C1.html> ;
  skos:inScheme s:scma-2011 ;
  skos:inScheme s:swcm-1992 ;
  skos:notation "15C1" ;
  skos:prefLabel "Exchangeable bases and CEC - alcoholic 1 M ammonium chloride at pH 8.5, pre-treatment for soluble salts" ;
  skos:topConceptOf s:scma-2011 ;
  skos:topConceptOf s:swcm-1992 ;
.
<http://anzsoil.org/def/au/scma/15C2>
  a skos:Concept ;
  a sosa:Procedure ;
  dct:identifier "http://anzsoil.org/def/au/scma/15C2"^^xsd:anyURI ;
  dct:source "URN:ISBN:978-0-643-10218-7" ;
  skos:definition <https://raw.githack.com/ANZSoilData/def-au-scma/master/html/15-ion-exchange-properties/15C2.html> ;
  skos:inScheme s:scma-2011 ;
  skos:inScheme s:swcm-1992 ;
  skos:notation "15C2" ;
  skos:prefLabel "Exchangeable divalent cations and CEC - by MIR diffuse reflectance spectroscopy" ;
  skos:topConceptOf s:scma-2011 ;
  skos:topConceptOf s:swcm-1992 ;
.
<http://anzsoil.org/def/au/scma/15D1>
  a skos:Concept ;
  a sosa:Procedure ;
  dct:identifier "http://anzsoil.org/def/au/scma/15D1"^^xsd:anyURI ;
  dct:source "URN:ISBN:978-0-643-10218-7" ;
  skos:definition <https://raw.githack.com/ANZSoilData/def-au-scma/master/html/15-ion-exchange-properties/15D1.html> ;
  skos:inScheme s:scma-2011 ;
  skos:inScheme s:swcm-1992 ;
  skos:notation "15D1" ;
  skos:prefLabel "Exchangeable bases and CEC - 1 M ammonium acetate at pH 7.0, pre-treatment for soluble salts, manual leach" ;
  skos:topConceptOf s:scma-2011 ;
  skos:topConceptOf s:swcm-1992 ;
.
<http://anzsoil.org/def/au/scma/15D2>
  a skos:Concept ;
  a sosa:Procedure ;
  dct:identifier "http://anzsoil.org/def/au/scma/15D2"^^xsd:anyURI ;
  dct:source "URN:ISBN:978-0-643-10218-7" ;
  skos:definition <https://raw.githack.com/ANZSoilData/def-au-scma/master/html/15-ion-exchange-properties/15D2.html> ;
  skos:inScheme s:scma-2011 ;
  skos:inScheme s:swcm-1992 ;
  skos:notation "15D2" ;
  skos:prefLabel "Exchangeable bases and CEC - 1 M ammonium acetate at pH 7.0, pre-treatment for soluble salts, automatic extractor" ;
  skos:topConceptOf s:scma-2011 ;
  skos:topConceptOf s:swcm-1992 ;
.
<http://anzsoil.org/def/au/scma/15D3>
  a skos:Concept ;
  a sosa:Procedure ;
  dct:identifier "http://anzsoil.org/def/au/scma/15D3"^^xsd:anyURI ;
  dct:source "URN:ISBN:978-0-643-10218-7" ;
  skos:definition <https://raw.githack.com/ANZSoilData/def-au-scma/master/html/15-ion-exchange-properties/15D3.html> ;
  skos:inScheme s:scma-2011 ;
  skos:inScheme s:swcm-1992 ;
  skos:notation "15D3" ;
  skos:prefLabel "Exchangeable bases and CEC - 1 M ammonium acetate at pH 7.0, rapid method with no pre-treatment for soluble salts" ;
  skos:topConceptOf s:scma-2011 ;
  skos:topConceptOf s:swcm-1992 ;
.
<http://anzsoil.org/def/au/scma/15E1>
  a skos:Concept ;
  a sosa:Procedure ;
  dct:identifier "http://anzsoil.org/def/au/scma/15E1"^^xsd:anyURI ;
  dct:source "URN:ISBN:978-0-643-10218-7" ;
  skos:definition <https://raw.githack.com/ANZSoilData/def-au-scma/master/html/15-ion-exchange-properties/15E1.html> ;
  skos:inScheme s:scma-2011 ;
  skos:inScheme s:swcm-1992 ;
  skos:notation "15E1" ;
  skos:prefLabel "Exchangeable bases, CEC and anion exchange capacity by compulsive exchange, no pre-treatment for soluble salts" ;
  skos:topConceptOf s:scma-2011 ;
  skos:topConceptOf s:swcm-1992 ;
.
<http://anzsoil.org/def/au/scma/15E2>
  a skos:Concept ;
  a sosa:Procedure ;
  dct:identifier "http://anzsoil.org/def/au/scma/15E2"^^xsd:anyURI ;
  dct:source "URN:ISBN:978-0-643-10218-7" ;
  skos:definition <https://raw.githack.com/ANZSoilData/def-au-scma/master/html/15-ion-exchange-properties/15E2.html> ;
  skos:inScheme s:scma-2011 ;
  skos:inScheme s:swcm-1992 ;
  skos:notation "15E2" ;
  skos:prefLabel "Exchangeable bases, CEC and AEC by compulsive exchange, pre-treatment for soluble salts" ;
  skos:topConceptOf s:scma-2011 ;
  skos:topConceptOf s:swcm-1992 ;
.
<http://anzsoil.org/def/au/scma/15E3>
  a skos:Concept ;
  a sosa:Procedure ;
  dct:identifier "http://anzsoil.org/def/au/scma/15E3"^^xsd:anyURI ;
  dct:source "URN:ISBN:978-0-643-10218-7" ;
  skos:definition <https://raw.githack.com/ANZSoilData/def-au-scma/master/html/15-ion-exchange-properties/15E3.html> ;
  skos:inScheme s:scma-2011 ;
  skos:inScheme s:swcm-1992 ;
  skos:notation "15E3" ;
  skos:prefLabel "Exchangeable bases, CEC and AEC by compulsive exchange, adjusted for soluble Na+" ;
  skos:topConceptOf s:scma-2011 ;
  skos:topConceptOf s:swcm-1992 ;
.
<http://anzsoil.org/def/au/scma/15F1>
  a skos:Concept ;
  a sosa:Procedure ;
  dct:identifier "http://anzsoil.org/def/au/scma/15F1"^^xsd:anyURI ;
  dct:source "URN:ISBN:978-0-643-10218-7" ;
  skos:definition <https://raw.githack.com/ANZSoilData/def-au-scma/master/html/15-ion-exchange-properties/15F1.html> ;
  skos:inScheme s:scma-2011 ;
  skos:inScheme s:swcm-1992 ;
  skos:notation "15F1" ;
  skos:prefLabel "Exchangeable bases by 0.01 M silver-thiourea (AgTU+) - no pre-treatment for soluble salts" ;
  skos:topConceptOf s:scma-2011 ;
  skos:topConceptOf s:swcm-1992 ;
.
<http://anzsoil.org/def/au/scma/15F2>
  a skos:Concept ;
  a sosa:Procedure ;
  dct:identifier "http://anzsoil.org/def/au/scma/15F2"^^xsd:anyURI ;
  dct:source "URN:ISBN:978-0-643-10218-7" ;
  skos:definition <https://raw.githack.com/ANZSoilData/def-au-scma/master/html/15-ion-exchange-properties/15F2.html> ;
  skos:inScheme s:scma-2011 ;
  skos:inScheme s:swcm-1992 ;
  skos:notation "15F2" ;
  skos:prefLabel "Exchangeable aluminium by 0.01 M AgTU+" ;
  skos:topConceptOf s:scma-2011 ;
  skos:topConceptOf s:swcm-1992 ;
.
<http://anzsoil.org/def/au/scma/15F3>
  a skos:Concept ;
  a sosa:Procedure ;
  dct:identifier "http://anzsoil.org/def/au/scma/15F3"^^xsd:anyURI ;
  dct:source "URN:ISBN:978-0-643-10218-7" ;
  skos:definition <https://raw.githack.com/ANZSoilData/def-au-scma/master/html/15-ion-exchange-properties/15F3.html> ;
  skos:inScheme s:scma-2011 ;
  skos:inScheme s:swcm-1992 ;
  skos:notation "15F3" ;
  skos:prefLabel "Cation exchange capacity by 0.01 M AgTU+ [CEC AgTU]" ;
  skos:topConceptOf s:scma-2011 ;
  skos:topConceptOf s:swcm-1992 ;
.
<http://anzsoil.org/def/au/scma/15G1>
  a skos:Concept ;
  a sosa:Procedure ;
  dct:identifier "http://anzsoil.org/def/au/scma/15G1"^^xsd:anyURI ;
  dct:source "URN:ISBN:978-0-643-10218-7" ;
  skos:definition <https://raw.githack.com/ANZSoilData/def-au-scma/master/html/15-ion-exchange-properties/15G1.html> ;
  skos:inScheme s:scma-2011 ;
  skos:inScheme s:swcm-1992 ;
  skos:notation "15G1" ;
  skos:prefLabel "Exchange acidity (H+ + Al3+) by 1 M potassium chloride" ;
  skos:topConceptOf s:scma-2011 ;
  skos:topConceptOf s:swcm-1992 ;
.
<http://anzsoil.org/def/au/scma/15H1>
  a skos:Concept ;
  a sosa:Procedure ;
  dct:identifier "http://anzsoil.org/def/au/scma/15H1"^^xsd:anyURI ;
  dct:source "URN:ISBN:978-0-643-10218-7" ;
  skos:definition <https://raw.githack.com/ANZSoilData/def-au-scma/master/html/15-ion-exchange-properties/15H1.html> ;
  skos:inScheme s:scma-2011 ;
  skos:inScheme s:swcm-1992 ;
  skos:notation "15H1" ;
  skos:prefLabel "Exchange acidity by triethanolamine (TEA)" ;
  skos:topConceptOf s:scma-2011 ;
  skos:topConceptOf s:swcm-1992 ;
.
<http://anzsoil.org/def/au/scma/15I1>
  a skos:Concept ;
  a sosa:Procedure ;
  dct:identifier "http://anzsoil.org/def/au/scma/15I1"^^xsd:anyURI ;
  dct:source "URN:ISBN:978-0-643-10218-7" ;
  skos:definition <https://raw.githack.com/ANZSoilData/def-au-scma/master/html/15-ion-exchange-properties/15I1.html> ;
  skos:inScheme s:scma-2011 ;
  skos:inScheme s:swcm-1992 ;
  skos:notation "15I1" ;
  skos:prefLabel "Cation exchange capacity measurement - distillation of NH+4" ;
  skos:topConceptOf s:scma-2011 ;
  skos:topConceptOf s:swcm-1992 ;
.
<http://anzsoil.org/def/au/scma/15I2>
  a skos:Concept ;
  a sosa:Procedure ;
  dct:identifier "http://anzsoil.org/def/au/scma/15I2"^^xsd:anyURI ;
  dct:source "URN:ISBN:978-0-643-10218-7" ;
  skos:definition <https://raw.githack.com/ANZSoilData/def-au-scma/master/html/15-ion-exchange-properties/15I2.html> ;
  skos:inScheme s:scma-2011 ;
  skos:inScheme s:swcm-1992 ;
  skos:notation "15I2" ;
  skos:prefLabel "Cation exchange capacity measurement - automated determination of NH+4" ;
  skos:topConceptOf s:scma-2011 ;
  skos:topConceptOf s:swcm-1992 ;
.
<http://anzsoil.org/def/au/scma/15I3>
  a skos:Concept ;
  a sosa:Procedure ;
  dct:identifier "http://anzsoil.org/def/au/scma/15I3"^^xsd:anyURI ;
  dct:source "URN:ISBN:978-0-643-10218-7" ;
  skos:definition <https://raw.githack.com/ANZSoilData/def-au-scma/master/html/15-ion-exchange-properties/15I3.html> ;
  skos:inScheme s:scma-2011 ;
  skos:inScheme s:swcm-1992 ;
  skos:notation "15I3" ;
  skos:prefLabel "Cation exchange capacity measurement - automated determination of NH+4 and Cl+" ;
  skos:topConceptOf s:scma-2011 ;
  skos:topConceptOf s:swcm-1992 ;
.
<http://anzsoil.org/def/au/scma/15I4>
  a skos:Concept ;
  a sosa:Procedure ;
  dct:identifier "http://anzsoil.org/def/au/scma/15I4"^^xsd:anyURI ;
  dct:source "URN:ISBN:978-0-643-10218-7" ;
  skos:definition <https://raw.githack.com/ANZSoilData/def-au-scma/master/html/15-ion-exchange-properties/15I4.html> ;
  skos:inScheme s:scma-2011 ;
  skos:inScheme s:swcm-1992 ;
  skos:notation "15I4" ;
  skos:prefLabel "Cation exchange capacity measurement - titration of NH+4 and Cl-" ;
  skos:topConceptOf s:scma-2011 ;
  skos:topConceptOf s:swcm-1992 ;
.
<http://anzsoil.org/def/au/scma/15J1>
  a skos:Concept ;
  a sosa:Procedure ;
  dct:identifier "http://anzsoil.org/def/au/scma/15J1"^^xsd:anyURI ;
  dct:source "URN:ISBN:978-0-643-10218-7" ;
  skos:definition <https://raw.githack.com/ANZSoilData/def-au-scma/master/html/15-ion-exchange-properties/15J1.html> ;
  skos:inScheme s:scma-2011 ;
  skos:inScheme s:swcm-1992 ;
  skos:notation "15J1" ;
  skos:prefLabel "Effective cation exchange capacity (ECEC)" ;
  skos:topConceptOf s:scma-2011 ;
  skos:topConceptOf s:swcm-1992 ;
.
<http://anzsoil.org/def/au/scma/15K1>
  a skos:Concept ;
  a sosa:Procedure ;
  dct:identifier "http://anzsoil.org/def/au/scma/15K1"^^xsd:anyURI ;
  dct:source "URN:ISBN:978-0-643-10218-7" ;
  skos:definition <https://raw.githack.com/ANZSoilData/def-au-scma/master/html/15-ion-exchange-properties/15K1.html> ;
  skos:inScheme s:scma-2011 ;
  skos:inScheme s:swcm-1992 ;
  skos:notation "15K1" ;
  skos:prefLabel "Cation exchange capacity - pH 8.2 (CEC pH 8.2)" ;
  skos:topConceptOf s:scma-2011 ;
  skos:topConceptOf s:swcm-1992 ;
.
<http://anzsoil.org/def/au/scma/15L1>
  a skos:Concept ;
  a sosa:Procedure ;
  dct:identifier "http://anzsoil.org/def/au/scma/15L1"^^xsd:anyURI ;
  dct:source "URN:ISBN:978-0-643-10218-7" ;
  skos:definition <https://raw.githack.com/ANZSoilData/def-au-scma/master/html/15-ion-exchange-properties/15L1.html> ;
  skos:inScheme s:scma-2011 ;
  skos:inScheme s:swcm-1992 ;
  skos:notation "15L1" ;
  skos:prefLabel "Base saturation percentage (ESP)" ;
  skos:topConceptOf s:scma-2011 ;
  skos:topConceptOf s:swcm-1992 ;
.
<http://anzsoil.org/def/au/scma/15M1>
  a skos:Concept ;
  a sosa:Procedure ;
  dct:identifier "http://anzsoil.org/def/au/scma/15M1"^^xsd:anyURI ;
  dct:source "URN:ISBN:978-0-643-10218-7" ;
  skos:definition <https://raw.githack.com/ANZSoilData/def-au-scma/master/html/15-ion-exchange-properties/15M1.html> ;
  skos:inScheme s:scma-2011 ;
  skos:inScheme s:swcm-1992 ;
  skos:notation "15M1" ;
  skos:prefLabel "Basic cation saturation ratios" ;
  skos:topConceptOf s:scma-2011 ;
  skos:topConceptOf s:swcm-1992 ;
.
<http://anzsoil.org/def/au/scma/15N1>
  a skos:Concept ;
  a sosa:Procedure ;
  dct:identifier "http://anzsoil.org/def/au/scma/15N1"^^xsd:anyURI ;
  dct:source "URN:ISBN:978-0-643-10218-7" ;
  skos:definition <https://raw.githack.com/ANZSoilData/def-au-scma/master/html/15-ion-exchange-properties/15N1.html> ;
  skos:inScheme s:scma-2011 ;
  skos:inScheme s:swcm-1992 ;
  skos:notation "15N1" ;
  skos:prefLabel "Exchangeable Na+ percentage (ESP)" ;
  skos:topConceptOf s:scma-2011 ;
  skos:topConceptOf s:swcm-1992 ;
.
<http://anzsoil.org/def/au/scma/15O1>
  a skos:Concept ;
  a sosa:Procedure ;
  dct:identifier "http://anzsoil.org/def/au/scma/15O1"^^xsd:anyURI ;
  dct:source "URN:ISBN:978-0-643-10218-7" ;
  skos:definition <https://raw.githack.com/ANZSoilData/def-au-scma/master/html/15-ion-exchange-properties/15O1.html> ;
  skos:inScheme s:scma-2011 ;
  skos:inScheme s:swcm-1992 ;
  skos:notation "15O1" ;
  skos:prefLabel "Percent Al saturation" ;
  skos:topConceptOf s:scma-2011 ;
  skos:topConceptOf s:swcm-1992 ;
.
<http://anzsoil.org/def/au/scma/16>
  a skos:Collection ;
  dct:identifier "http://anzsoil.org/def/au/scma/16"^^xsd:anyURI ;
  dct:source "URN:ISBN:978-0-643-10218-7" ;
  skos:definition <https://raw.githack.com/ANZSoilData/def-au-scma/master/html/16-lime-requirement/16.html> ;
  skos:member <http://anzsoil.org/def/au/scma/16A1> ;
  skos:member <http://anzsoil.org/def/au/scma/16B1> ;
  skos:member <http://anzsoil.org/def/au/scma/16C1> ;
  skos:member <http://anzsoil.org/def/au/scma/16D1> ;
  skos:notation "16" ;
  skos:prefLabel "Lime requirement" ;
.
<http://anzsoil.org/def/au/scma/16A1>
  a skos:Concept ;
  a sosa:Procedure ;
  dct:identifier "http://anzsoil.org/def/au/scma/16A1"^^xsd:anyURI ;
  dct:source "URN:ISBN:978-0-643-10218-7" ;
  skos:definition <https://raw.githack.com/ANZSoilData/def-au-scma/master/html/16-lime-requirement/16A.html> ;
  skos:inScheme s:scma-2011 ;
  skos:inScheme s:swcm-1992 ;
  skos:notation "16A1" ;
  skos:prefLabel "Calculated lime rate - from exchangeable Al3+" ;
  skos:topConceptOf s:scma-2011 ;
  skos:topConceptOf s:swcm-1992 ;
.
<http://anzsoil.org/def/au/scma/16B1>
  a skos:Concept ;
  a sosa:Procedure ;
  dct:identifier "http://anzsoil.org/def/au/scma/16B1"^^xsd:anyURI ;
  dct:source "URN:ISBN:978-0-643-10218-7" ;
  skos:definition <https://raw.githack.com/ANZSoilData/def-au-scma/master/html/16-lime-requirement/16B1.html> ;
  skos:inScheme s:scma-2011 ;
  skos:inScheme s:swcm-1992 ;
  skos:notation "16B1" ;
  skos:prefLabel "Calculated lime rate - Cregan" ;
  skos:topConceptOf s:scma-2011 ;
  skos:topConceptOf s:swcm-1992 ;
.
<http://anzsoil.org/def/au/scma/16C1>
  a skos:Concept ;
  a sosa:Procedure ;
  dct:identifier "http://anzsoil.org/def/au/scma/16C1"^^xsd:anyURI ;
  dct:source "URN:ISBN:978-0-643-10218-7" ;
  skos:definition <https://raw.githack.com/ANZSoilData/def-au-scma/master/html/16-lime-requirement/16C1.html> ;
  skos:inScheme s:scma-2011 ;
  skos:inScheme s:swcm-1992 ;
  skos:notation "16C1" ;
  skos:prefLabel "Lime requirement - Mehlich single buffer" ;
  skos:topConceptOf s:scma-2011 ;
  skos:topConceptOf s:swcm-1992 ;
.
<http://anzsoil.org/def/au/scma/16D1>
  a skos:Concept ;
  a sosa:Procedure ;
  dct:identifier "http://anzsoil.org/def/au/scma/16D1"^^xsd:anyURI ;
  dct:source "URN:ISBN:978-0-643-10218-7" ;
  skos:definition <https://raw.githack.com/ANZSoilData/def-au-scma/master/html/16-lime-requirement/16D1.html> ;
  skos:inScheme s:scma-2011 ;
  skos:inScheme s:swcm-1992 ;
  skos:notation "16D1" ;
  skos:prefLabel "Lime requirement - Dunn titration curves" ;
  skos:topConceptOf s:scma-2011 ;
  skos:topConceptOf s:swcm-1992 ;
.
<http://anzsoil.org/def/au/scma/17>
  a skos:Collection ;
  dct:identifier "http://anzsoil.org/def/au/scma/17"^^xsd:anyURI ;
  dct:source "URN:ISBN:978-0-643-10218-7" ;
  skos:definition <https://raw.githack.com/ANZSoilData/def-au-scma/master/html/17-total-miscellaneous-elements/17.html> ;
  skos:member <http://anzsoil.org/def/au/scma/17A1> ;
  skos:member <http://anzsoil.org/def/au/scma/17A2> ;
  skos:member <http://anzsoil.org/def/au/scma/17B1> ;
  skos:member <http://anzsoil.org/def/au/scma/17B2> ;
  skos:member <http://anzsoil.org/def/au/scma/17C1> ;
  skos:notation "17" ;
  skos:prefLabel "Total miscellaneous elements" ;
.
<http://anzsoil.org/def/au/scma/17A1>
  a skos:Concept ;
  a sosa:Procedure ;
  dct:identifier "http://anzsoil.org/def/au/scma/17A1"^^xsd:anyURI ;
  dct:source "URN:ISBN:978-0-643-10218-7" ;
  skos:definition <https://raw.githack.com/ANZSoilData/def-au-scma/master/html/17-total-miscellaneous-elements/17A1.html> ;
  skos:inScheme s:scma-2011 ;
  skos:inScheme s:swcm-1992 ;
  skos:notation "17A1" ;
  skos:prefLabel "Total elemental analysis of soils and sediments -X-ray fluorescence spectroscopy" ;
  skos:topConceptOf s:scma-2011 ;
  skos:topConceptOf s:swcm-1992 ;
.
<http://anzsoil.org/def/au/scma/17A2>
  a skos:Concept ;
  a sosa:Procedure ;
  dct:identifier "http://anzsoil.org/def/au/scma/17A2"^^xsd:anyURI ;
  dct:source "URN:ISBN:978-0-643-10218-7" ;
  skos:definition <https://raw.githack.com/ANZSoilData/def-au-scma/master/html/17-total-miscellaneous-elements/17A2.html> ;
  skos:inScheme s:scma-2011 ;
  skos:inScheme s:swcm-1992 ;
  skos:notation "17A2" ;
  skos:prefLabel "Total elemental analysis of soils and sediments - microwave assisted digestion, with determination by atomic spectroscopy" ;
  skos:topConceptOf s:scma-2011 ;
  skos:topConceptOf s:swcm-1992 ;
.
<http://anzsoil.org/def/au/scma/17B1>
  a skos:Concept ;
  a sosa:Procedure ;
  dct:identifier "http://anzsoil.org/def/au/scma/17B1"^^xsd:anyURI ;
  dct:source "URN:ISBN:978-0-643-10218-7" ;
  skos:definition <https://raw.githack.com/ANZSoilData/def-au-scma/master/html/17-total-miscellaneous-elements/17B1.html> ;
  skos:inScheme s:scma-2011 ;
  skos:inScheme s:swcm-1992 ;
  skos:notation "17B1" ;
  skos:prefLabel "Pseudo-total elemental analysis of soils and sediments - reverse aqua regia block digestion with determination by atomic spectroscopy" ;
  skos:topConceptOf s:scma-2011 ;
  skos:topConceptOf s:swcm-1992 ;
.
<http://anzsoil.org/def/au/scma/17B2>
  a skos:Concept ;
  a sosa:Procedure ;
  dct:identifier "http://anzsoil.org/def/au/scma/17B2"^^xsd:anyURI ;
  dct:source "URN:ISBN:978-0-643-10218-7" ;
  skos:definition <https://raw.githack.com/ANZSoilData/def-au-scma/master/html/17-total-miscellaneous-elements/17B2.html> ;
  skos:inScheme s:scma-2011 ;
  skos:inScheme s:swcm-1992 ;
  skos:notation "17B2" ;
  skos:prefLabel "Pseudo-total elements of soils and sediments - reverse aqua regia microwave assisted digestion of sludges, soils and sediments, with determination by atomic spectroscopy" ;
  skos:topConceptOf s:scma-2011 ;
  skos:topConceptOf s:swcm-1992 ;
.
<http://anzsoil.org/def/au/scma/17C1>
  a skos:Concept ;
  a sosa:Procedure ;
  dct:identifier "http://anzsoil.org/def/au/scma/17C1"^^xsd:anyURI ;
  dct:source "URN:ISBN:978-0-643-10218-7" ;
  skos:definition <https://raw.githack.com/ANZSoilData/def-au-scma/master/html/17-total-miscellaneous-elements/17C1.html> ;
  skos:inScheme s:scma-2011 ;
  skos:inScheme s:swcm-1992 ;
  skos:notation "17C1" ;
  skos:prefLabel "Pseudo-total elements of soils and sediments - conventional aqua regia block digestion and determination by atomic spectroscopy" ;
  skos:topConceptOf s:scma-2011 ;
  skos:topConceptOf s:swcm-1992 ;
.
<http://anzsoil.org/def/au/scma/18>
  a skos:Collection ;
  dct:identifier "http://anzsoil.org/def/au/scma/18"^^xsd:anyURI ;
  dct:source "URN:ISBN:978-0-643-10218-7" ;
  skos:definition <https://raw.githack.com/ANZSoilData/def-au-scma/master/html/18-miscellaneous-extractable-elements/18.html> ;
  skos:member <http://anzsoil.org/def/au/scma/18A1> ;
  skos:member <http://anzsoil.org/def/au/scma/18B1> ;
  skos:member <http://anzsoil.org/def/au/scma/18C1> ;
  skos:member <http://anzsoil.org/def/au/scma/18D1> ;
  skos:member <http://anzsoil.org/def/au/scma/18E1> ;
  skos:member <http://anzsoil.org/def/au/scma/18F> ;
  skos:member <http://anzsoil.org/def/au/scma/18F1> ;
  skos:member <http://anzsoil.org/def/au/scma/18F2> ;
  skos:member <http://anzsoil.org/def/au/scma/18G1> ;
  skos:notation "18" ;
  skos:prefLabel "Miscellaneous extractable elements" ;
.
<http://anzsoil.org/def/au/scma/18A1>
  a skos:Concept ;
  a sosa:Procedure ;
  dct:identifier "http://anzsoil.org/def/au/scma/18A1"^^xsd:anyURI ;
  dct:source "URN:ISBN:978-0-643-10218-7" ;
  skos:definition <https://raw.githack.com/ANZSoilData/def-au-scma/master/html/18-miscellaneous-extractable-elements/18A1.html> ;
  skos:inScheme s:scma-2011 ;
  skos:inScheme s:swcm-1992 ;
  skos:notation "18A1" ;
  skos:prefLabel "Bicarbonate-extractable K+" ;
  skos:topConceptOf s:scma-2011 ;
  skos:topConceptOf s:swcm-1992 ;
.
<http://anzsoil.org/def/au/scma/18B1>
  a skos:Concept ;
  a sosa:Procedure ;
  dct:identifier "http://anzsoil.org/def/au/scma/18B1"^^xsd:anyURI ;
  dct:source "URN:ISBN:978-0-643-10218-7" ;
  skos:definition <https://raw.githack.com/ANZSoilData/def-au-scma/master/html/18-miscellaneous-extractable-elements/18B1.html> ;
  skos:inScheme s:scma-2011 ;
  skos:inScheme s:swcm-1992 ;
  skos:notation "18B1" ;
  skos:prefLabel "Hydrochloric acid-extractable K+" ;
  skos:topConceptOf s:scma-2011 ;
  skos:topConceptOf s:swcm-1992 ;
.
<http://anzsoil.org/def/au/scma/18C1>
  a skos:Concept ;
  a sosa:Procedure ;
  dct:identifier "http://anzsoil.org/def/au/scma/18C1"^^xsd:anyURI ;
  dct:source "URN:ISBN:978-0-643-10218-7" ;
  skos:definition <https://raw.githack.com/ANZSoilData/def-au-scma/master/html/18-miscellaneous-extractable-elements/18C1.html> ;
  skos:inScheme s:scma-2011 ;
  skos:inScheme s:swcm-1992 ;
  skos:notation "18C1" ;
  skos:prefLabel "Boiling 0.1 nitric acid-extractable K+" ;
  skos:topConceptOf s:scma-2011 ;
  skos:topConceptOf s:swcm-1992 ;
.
<http://anzsoil.org/def/au/scma/18D1>
  a skos:Concept ;
  a sosa:Procedure ;
  dct:identifier "http://anzsoil.org/def/au/scma/18D1"^^xsd:anyURI ;
  dct:source "URN:ISBN:978-0-643-10218-7" ;
  skos:definition <https://raw.githack.com/ANZSoilData/def-au-scma/master/html/18-miscellaneous-extractable-elements/18D1.html> ;
  skos:inScheme s:scma-2011 ;
  skos:inScheme s:swcm-1992 ;
  skos:notation "18D1" ;
  skos:prefLabel "0.1 M calcium chloride-extractable Cd" ;
  skos:topConceptOf s:scma-2011 ;
  skos:topConceptOf s:swcm-1992 ;
.
<http://anzsoil.org/def/au/scma/18E1>
  a skos:Concept ;
  a sosa:Procedure ;
  dct:identifier "http://anzsoil.org/def/au/scma/18E1"^^xsd:anyURI ;
  dct:source "URN:ISBN:978-0-643-10218-7" ;
  skos:definition <https://raw.githack.com/ANZSoilData/def-au-scma/master/html/18-miscellaneous-extractable-elements/18E1.html> ;
  skos:inScheme s:scma-2011 ;
  skos:inScheme s:swcm-1992 ;
  skos:notation "18E1" ;
  skos:prefLabel "0.01 M calcium chloride-extractable Cd" ;
  skos:topConceptOf s:scma-2011 ;
  skos:topConceptOf s:swcm-1992 ;
.
<http://anzsoil.org/def/au/scma/18F>
  a skos:Concept ;
  a sosa:Procedure ;
  dct:identifier "http://anzsoil.org/def/au/scma/18F"^^xsd:anyURI ;
  dct:source "URN:ISBN:978-0-643-10218-7" ;
  skos:definition <https://raw.githack.com/ANZSoilData/def-au-scma/master/html/18-miscellaneous-extractable-elements/18F.html> ;
  skos:inScheme s:scma-2011 ;
  skos:inScheme s:swcm-1992 ;
  skos:narrower <http://anzsoil.org/def/au/scma/18F1> ;
  skos:narrower <http://anzsoil.org/def/au/scma/18F2> ;
  skos:notation "18F" ;
  skos:prefLabel "Mehlich 3 multi-element tests" ;
  skos:topConceptOf s:scma-2011 ;
  skos:topConceptOf s:swcm-1992 ;
.
<http://anzsoil.org/def/au/scma/18F1>
  a skos:Concept ;
  a sosa:Procedure ;
  dct:identifier "http://anzsoil.org/def/au/scma/18F1"^^xsd:anyURI ;
  dct:source "URN:ISBN:978-0-643-10218-7" ;
  skos:broader <http://anzsoil.org/def/au/scma/18F> ;
  skos:definition <https://raw.githack.com/ANZSoilData/def-au-scma/master/html/18-miscellaneous-extractable-elements/18F1.html> ;
  skos:inScheme s:scma-2011 ;
  skos:inScheme s:swcm-1992 ;
  skos:notation "18F1" ;
  skos:prefLabel "Mehlich 3-extractable elements (P, Ca, Mg, Na, K, Fe, Cu, Mn, Zn, B, S, Al)" ;
.
<http://anzsoil.org/def/au/scma/18F2>
  a skos:Concept ;
  a sosa:Procedure ;
  dct:identifier "http://anzsoil.org/def/au/scma/18F2"^^xsd:anyURI ;
  dct:source "URN:ISBN:978-0-643-10218-7" ;
  skos:broader <http://anzsoil.org/def/au/scma/18F> ;
  skos:definition <https://raw.githack.com/ANZSoilData/def-au-scma/master/html/18-miscellaneous-extractable-elements/18F2.html> ;
  skos:inScheme s:scma-2011 ;
  skos:inScheme s:swcm-1992 ;
  skos:notation "18F2" ;
  skos:prefLabel "Mehlich 3 Extractable P - colour finish" ;
.
<http://anzsoil.org/def/au/scma/18G1>
  a skos:Concept ;
  a sosa:Procedure ;
  dct:identifier "http://anzsoil.org/def/au/scma/18G1"^^xsd:anyURI ;
  dct:source "URN:ISBN:978-0-643-10218-7" ;
  skos:definition <https://raw.githack.com/ANZSoilData/def-au-scma/master/html/18-miscellaneous-extractable-elements/18G1.html> ;
  skos:inScheme s:scma-2011 ;
  skos:inScheme s:swcm-1992 ;
  skos:notation "18G1" ;
  skos:prefLabel "Reverse soil K+ by copper-modified sodium tetraphenylboron extraction (TBK 4h)" ;
  skos:topConceptOf s:scma-2011 ;
  skos:topConceptOf s:swcm-1992 ;
.
<http://anzsoil.org/def/au/scma/19>
  a skos:Collection ;
  dct:identifier "http://anzsoil.org/def/au/scma/19"^^xsd:anyURI ;
  dct:source "URN:ISBN:978-0-643-10218-7" ;
  skos:definition <https://raw.githack.com/ANZSoilData/def-au-scma/master/html/19-alkaline-earth-carbonates/19.html> ;
  skos:member <http://anzsoil.org/def/au/scma/19A1> ;
  skos:member <http://anzsoil.org/def/au/scma/19B> ;
  skos:member <http://anzsoil.org/def/au/scma/19B1> ;
  skos:member <http://anzsoil.org/def/au/scma/19B2> ;
  skos:member <http://anzsoil.org/def/au/scma/19C1> ;
  skos:member <http://anzsoil.org/def/au/scma/19D1> ;
  skos:notation "19" ;
  skos:prefLabel "Alkaline earth carbonates" ;
.
<http://anzsoil.org/def/au/scma/19A1>
  a skos:Concept ;
  a sosa:Procedure ;
  dct:identifier "http://anzsoil.org/def/au/scma/19A1"^^xsd:anyURI ;
  dct:source "URN:ISBN:978-0-643-10218-7" ;
  skos:definition <https://raw.githack.com/ANZSoilData/def-au-scma/master/html/19-alkaline-earth-carbonates/19A1.html> ;
  skos:inScheme s:scma-2011 ;
  skos:inScheme s:swcm-1992 ;
  skos:notation "19A1" ;
  skos:prefLabel "Carbonates -rapid titration" ;
  skos:topConceptOf s:scma-2011 ;
  skos:topConceptOf s:swcm-1992 ;
.
<http://anzsoil.org/def/au/scma/19B>
  a skos:Concept ;
  a sosa:Procedure ;
  dct:identifier "http://anzsoil.org/def/au/scma/19B"^^xsd:anyURI ;
  dct:source "URN:ISBN:978-0-643-10218-7" ;
  skos:definition <https://raw.githack.com/ANZSoilData/def-au-scma/master/html/19-alkaline-earth-carbonates/19B.html> ;
  skos:inScheme s:scma-2011 ;
  skos:inScheme s:swcm-1992 ;
  skos:narrower <http://anzsoil.org/def/au/scma/19B1> ;
  skos:narrower <http://anzsoil.org/def/au/scma/19B2> ;
  skos:notation "19B" ;
  skos:prefLabel "Carbonates by pressure change" ;
  skos:topConceptOf s:scma-2011 ;
  skos:topConceptOf s:swcm-1992 ;
.
<http://anzsoil.org/def/au/scma/19B1>
  a skos:Concept ;
  a sosa:Procedure ;
  dct:identifier "http://anzsoil.org/def/au/scma/19B1"^^xsd:anyURI ;
  dct:source "URN:ISBN:978-0-643-10218-7" ;
  skos:broader <http://anzsoil.org/def/au/scma/19B> ;
  skos:definition <https://raw.githack.com/ANZSoilData/def-au-scma/master/html/19-alkaline-earth-carbonates/19B1.html> ;
  skos:inScheme s:scma-2011 ;
  skos:inScheme s:swcm-1992 ;
  skos:notation "19B1" ;
  skos:prefLabel "Carbonates by pressure change - manometric" ;
.
<http://anzsoil.org/def/au/scma/19B2>
  a skos:Concept ;
  a sosa:Procedure ;
  dct:identifier "http://anzsoil.org/def/au/scma/19B2"^^xsd:anyURI ;
  dct:source "URN:ISBN:978-0-643-10218-7" ;
  skos:broader <http://anzsoil.org/def/au/scma/19B> ;
  skos:definition <https://raw.githack.com/ANZSoilData/def-au-scma/master/html/19-alkaline-earth-carbonates/19B2.html> ;
  skos:inScheme s:scma-2011 ;
  skos:inScheme s:swcm-1992 ;
  skos:notation "19B2" ;
  skos:prefLabel "Carbonates by pressure change - transducer" ;
.
<http://anzsoil.org/def/au/scma/19C1>
  a skos:Concept ;
  a sosa:Procedure ;
  dct:identifier "http://anzsoil.org/def/au/scma/19C1"^^xsd:anyURI ;
  dct:source "URN:ISBN:978-0-643-10218-7" ;
  skos:definition <https://raw.githack.com/ANZSoilData/def-au-scma/master/html/19-alkaline-earth-carbonates/19C1.html> ;
  skos:inScheme s:scma-2011 ;
  skos:inScheme s:swcm-1992 ;
  skos:notation "19C1" ;
  skos:prefLabel "Spot field test for the presence of soil carbonates with dilute HCl" ;
  skos:topConceptOf s:scma-2011 ;
  skos:topConceptOf s:swcm-1992 ;
.
<http://anzsoil.org/def/au/scma/19D1>
  a skos:Concept ;
  a sosa:Procedure ;
  dct:identifier "http://anzsoil.org/def/au/scma/19D1"^^xsd:anyURI ;
  dct:source "URN:ISBN:978-0-643-10218-7" ;
  skos:definition <https://raw.githack.com/ANZSoilData/def-au-scma/master/html/19-alkaline-earth-carbonates/19D1.html> ;
  skos:inScheme s:scma-2011 ;
  skos:inScheme s:swcm-1992 ;
  skos:notation "19D1" ;
  skos:prefLabel "Field test for carbonates with dilute HCl and effervescence class assessment" ;
  skos:topConceptOf s:scma-2011 ;
  skos:topConceptOf s:swcm-1992 ;
.
<http://anzsoil.org/def/au/scma/20>
  a skos:Collection ;
  dct:identifier "http://anzsoil.org/def/au/scma/20"^^xsd:anyURI ;
  dct:source "URN:ISBN:978-0-643-10218-7" ;
  skos:definition <https://raw.githack.com/ANZSoilData/def-au-scma/master/html/20-acid-sulfate-soils/20.html> ;
  skos:member <http://anzsoil.org/def/au/scma/20A1> ;
  skos:member <http://anzsoil.org/def/au/scma/20B1> ;
  skos:member <http://anzsoil.org/def/au/scma/20C1> ;
  skos:member <http://anzsoil.org/def/au/scma/20D1> ;
  skos:member <http://anzsoil.org/def/au/scma/20E1> ;
  skos:member <http://anzsoil.org/def/au/scma/20F1> ;
  skos:member <http://anzsoil.org/def/au/scma/20F2> ;
  skos:member <http://anzsoil.org/def/au/scma/20G1> ;
  skos:member <http://anzsoil.org/def/au/scma/20H1> ;
  skos:member <http://anzsoil.org/def/au/scma/20I1> ;
  skos:member <http://anzsoil.org/def/au/scma/20J1> ;
  skos:member <http://anzsoil.org/def/au/scma/20K1> ;
  skos:notation "20" ;
  skos:prefLabel "Acid sulfate soils" ;
.
<http://anzsoil.org/def/au/scma/20A1>
  a skos:Concept ;
  a sosa:Procedure ;
  dct:identifier "http://anzsoil.org/def/au/scma/20A1"^^xsd:anyURI ;
  dct:source "URN:ISBN:978-0-643-10218-7" ;
  skos:definition <https://raw.githack.com/ANZSoilData/def-au-scma/master/html/20-acid-sulfate-soils/20A1.html> ;
  skos:inScheme s:scma-2011 ;
  skos:inScheme s:swcm-1992 ;
  skos:notation "20A1" ;
  skos:prefLabel "Chromium reducible S (S CR)" ;
  skos:topConceptOf s:scma-2011 ;
  skos:topConceptOf s:swcm-1992 ;
.
<http://anzsoil.org/def/au/scma/20B1>
  a skos:Concept ;
  a sosa:Procedure ;
  dct:identifier "http://anzsoil.org/def/au/scma/20B1"^^xsd:anyURI ;
  dct:source "URN:ISBN:978-0-643-10218-7" ;
  skos:definition <https://raw.githack.com/ANZSoilData/def-au-scma/master/html/20-acid-sulfate-soils/20B1.html> ;
  skos:inScheme s:scma-2011 ;
  skos:inScheme s:swcm-1992 ;
  skos:notation "20B1" ;
  skos:prefLabel "SPOCAS acid trail - titratable actual acidity (TAA)" ;
  skos:topConceptOf s:scma-2011 ;
  skos:topConceptOf s:swcm-1992 ;
.
<http://anzsoil.org/def/au/scma/20C1>
  a skos:Concept ;
  a sosa:Procedure ;
  dct:identifier "http://anzsoil.org/def/au/scma/20C1"^^xsd:anyURI ;
  dct:source "URN:ISBN:978-0-643-10218-7" ;
  skos:definition <https://raw.githack.com/ANZSoilData/def-au-scma/master/html/20-acid-sulfate-soils/20C1.html> ;
  skos:inScheme s:scma-2011 ;
  skos:inScheme s:swcm-1992 ;
  skos:notation "20C1" ;
  skos:prefLabel "SPOCAS acid trail - titratable peroxide acidity (TPA) and Net (excess) Acid Neutralising Capacity (a-ANC E)" ;
  skos:topConceptOf s:scma-2011 ;
  skos:topConceptOf s:swcm-1992 ;
.
<http://anzsoil.org/def/au/scma/20D1>
  a skos:Concept ;
  a sosa:Procedure ;
  dct:identifier "http://anzsoil.org/def/au/scma/20D1"^^xsd:anyURI ;
  dct:source "URN:ISBN:978-0-643-10218-7" ;
  skos:definition <https://raw.githack.com/ANZSoilData/def-au-scma/master/html/20-acid-sulfate-soils/20D1.html> ;
  skos:inScheme s:scma-2011 ;
  skos:inScheme s:swcm-1992 ;
  skos:notation "20D1" ;
  skos:prefLabel "1 M KCl-extractable S, Ca and Mg" ;
  skos:topConceptOf s:scma-2011 ;
  skos:topConceptOf s:swcm-1992 ;
.
<http://anzsoil.org/def/au/scma/20E1>
  a skos:Concept ;
  a sosa:Procedure ;
  dct:identifier "http://anzsoil.org/def/au/scma/20E1"^^xsd:anyURI ;
  dct:source "URN:ISBN:978-0-643-10218-7" ;
  skos:definition <https://raw.githack.com/ANZSoilData/def-au-scma/master/html/20-acid-sulfate-soils/20E1.html> ;
  skos:inScheme s:scma-2011 ;
  skos:inScheme s:swcm-1992 ;
  skos:notation "20E1" ;
  skos:prefLabel "1 M KCl-extractable S, Ca and Mg after peroxide oxidation" ;
  skos:topConceptOf s:scma-2011 ;
  skos:topConceptOf s:swcm-1992 ;
.
<http://anzsoil.org/def/au/scma/20F1>
  a skos:Concept ;
  a sosa:Procedure ;
  dct:identifier "http://anzsoil.org/def/au/scma/20F1"^^xsd:anyURI ;
  dct:source "URN:ISBN:978-0-643-10218-7" ;
  skos:definition <https://raw.githack.com/ANZSoilData/def-au-scma/master/html/20-acid-sulfate-soils/20F1.html> ;
  skos:inScheme s:scma-2011 ;
  skos:inScheme s:swcm-1992 ;
  skos:notation "20F1" ;
  skos:prefLabel "Sulfur - 4 M HCl extraction (S HCl), ICPAES finish" ;
  skos:topConceptOf s:scma-2011 ;
  skos:topConceptOf s:swcm-1992 ;
.
<http://anzsoil.org/def/au/scma/20F2>
  a skos:Concept ;
  a sosa:Procedure ;
  dct:identifier "http://anzsoil.org/def/au/scma/20F2"^^xsd:anyURI ;
  dct:source "URN:ISBN:978-0-643-10218-7" ;
  skos:definition <https://raw.githack.com/ANZSoilData/def-au-scma/master/html/20-acid-sulfate-soils/20F2.html> ;
  skos:inScheme s:scma-2011 ;
  skos:inScheme s:swcm-1992 ;
  skos:notation "20F2" ;
  skos:prefLabel "Sulfur - 4 M HCl extraction (S HCl), ion chromatography finish" ;
  skos:topConceptOf s:scma-2011 ;
  skos:topConceptOf s:swcm-1992 ;
.
<http://anzsoil.org/def/au/scma/20G1>
  a skos:Concept ;
  a sosa:Procedure ;
  dct:identifier "http://anzsoil.org/def/au/scma/20G1"^^xsd:anyURI ;
  dct:source "URN:ISBN:978-0-643-10218-7" ;
  skos:definition <https://raw.githack.com/ANZSoilData/def-au-scma/master/html/20-acid-sulfate-soils/20G1.html> ;
  skos:inScheme s:scma-2011 ;
  skos:inScheme s:swcm-1992 ;
  skos:notation "20G1" ;
  skos:prefLabel "Peroxide residual acid soluble sulfur (S RAS)" ;
  skos:topConceptOf s:scma-2011 ;
  skos:topConceptOf s:swcm-1992 ;
.
<http://anzsoil.org/def/au/scma/20H1>
  a skos:Concept ;
  a sosa:Procedure ;
  dct:identifier "http://anzsoil.org/def/au/scma/20H1"^^xsd:anyURI ;
  dct:source "URN:ISBN:978-0-643-10218-7" ;
  skos:definition <https://raw.githack.com/ANZSoilData/def-au-scma/master/html/20-acid-sulfate-soils/20H1.html> ;
  skos:inScheme s:scma-2011 ;
  skos:inScheme s:swcm-1992 ;
  skos:notation "20H1" ;
  skos:prefLabel "Acid neutralising capacity - acid reacted and back titration (ANC BT)" ;
  skos:topConceptOf s:scma-2011 ;
  skos:topConceptOf s:swcm-1992 ;
.
<http://anzsoil.org/def/au/scma/20I1>
  a skos:Concept ;
  a sosa:Procedure ;
  dct:identifier "http://anzsoil.org/def/au/scma/20I1"^^xsd:anyURI ;
  dct:source "URN:ISBN:978-0-643-10218-7" ;
  skos:definition <https://raw.githack.com/ANZSoilData/def-au-scma/master/html/20-acid-sulfate-soils/20I1.html> ;
  skos:inScheme s:scma-2011 ;
  skos:inScheme s:swcm-1992 ;
  skos:notation "20I1" ;
  skos:prefLabel "Acid neutralising capacity - from SPOCAS" ;
  skos:topConceptOf s:scma-2011 ;
  skos:topConceptOf s:swcm-1992 ;
.
<http://anzsoil.org/def/au/scma/20J1>
  a skos:Concept ;
  a sosa:Procedure ;
  dct:identifier "http://anzsoil.org/def/au/scma/20J1"^^xsd:anyURI ;
  dct:source "URN:ISBN:978-0-643-10218-7" ;
  skos:definition <https://raw.githack.com/ANZSoilData/def-au-scma/master/html/20-acid-sulfate-soils/20J1.html> ;
  skos:inScheme s:scma-2011 ;
  skos:inScheme s:swcm-1992 ;
  skos:notation "20J1" ;
  skos:prefLabel "Field approximation of ASS hazard" ;
  skos:topConceptOf s:scma-2011 ;
  skos:topConceptOf s:swcm-1992 ;
.
<http://anzsoil.org/def/au/scma/20K1>
  a skos:Concept ;
  a sosa:Procedure ;
  dct:identifier "http://anzsoil.org/def/au/scma/20K1"^^xsd:anyURI ;
  dct:source "URN:ISBN:978-0-643-10218-7" ;
  skos:definition <https://raw.githack.com/ANZSoilData/def-au-scma/master/html/20-acid-sulfate-soils/20K1.html> ;
  skos:inScheme s:scma-2011 ;
  skos:inScheme s:swcm-1992 ;
  skos:notation "20K1" ;
  skos:prefLabel "Quick field approximations of ASS presence and associated lime requirement for drain-spoil" ;
  skos:topConceptOf s:scma-2011 ;
  skos:topConceptOf s:swcm-1992 ;
.
s:scma-2011
  a skos:ConceptScheme ;
  dct:accrualPeriodicity <http://purl.org/cld/freq/irregular> ;
  dct:contributor <https://orcid.org/0000-0002-2991-2308> ;
  dct:contributor <https://orcid.org/0000-0002-3884-3420> ;
  dct:created "2021-01-01"^^xsd:date ;
  dct:description "<p>This Concept Scheme is a machine-readable representation of the classifiers described in <a href='https://catalogue.nla.gov.au/Record/4854518'>Soil Chemical Methods Australasia</a> 1. (2011), by George E Rayment and David J Lyons. These comprise the laboratory and field chemical tests relevant to Australasia and beyond. </p> <p>Supersedes <a href='https://catalogue.nla.gov.au/Record/685915'>Australian Laboratory Handbook of Soil and Water Chemical Methods</a> (Rayment and Higginson 1992) while retaining method codes and other strengths of that Handbook. This register includes the method codes from Rayment and Higginson (1992) that were made redundant or superseded by new codes in George E Rayment and David J Lyons (2011).</p>"^^rdf:HTML ;
  dct:identifier "http://anzsoil.org/def/au/scma/scma-2011"^^xsd:anyURI ;
  dct:license <https://creativecommons.org/publicdomain/zero/1.0/> ;
  dct:modified "2022-03-04"^^xsd:date ;
  dct:replaces s:swcm-1992 ;
  dct:source <https://catalogue.nla.gov.au/Record/4854518> ;
  dct:title "Soil chemical methods - Australasia" ;
  skos:hasTopConcept <http://anzsoil.org/def/au/scma/02A1> ;
  skos:hasTopConcept <http://anzsoil.org/def/au/scma/02B1> ;
  skos:hasTopConcept <http://anzsoil.org/def/au/scma/02C1> ;
  skos:hasTopConcept <http://anzsoil.org/def/au/scma/02D1> ;
  skos:hasTopConcept <http://anzsoil.org/def/au/scma/03A1> ;
  skos:hasTopConcept <http://anzsoil.org/def/au/scma/03B1> ;
  skos:hasTopConcept <http://anzsoil.org/def/au/scma/03C1> ;
  skos:hasTopConcept <http://anzsoil.org/def/au/scma/03D1> ;
  skos:hasTopConcept <http://anzsoil.org/def/au/scma/04A1> ;
  skos:hasTopConcept <http://anzsoil.org/def/au/scma/04A2> ;
  skos:hasTopConcept <http://anzsoil.org/def/au/scma/04A3> ;
  skos:hasTopConcept <http://anzsoil.org/def/au/scma/04B1> ;
  skos:hasTopConcept <http://anzsoil.org/def/au/scma/04B2> ;
  skos:hasTopConcept <http://anzsoil.org/def/au/scma/04B3> ;
  skos:hasTopConcept <http://anzsoil.org/def/au/scma/04B4> ;
  skos:hasTopConcept <http://anzsoil.org/def/au/scma/04B5> ;
  skos:hasTopConcept <http://anzsoil.org/def/au/scma/04C1> ;
  skos:hasTopConcept <http://anzsoil.org/def/au/scma/04C2> ;
  skos:hasTopConcept <http://anzsoil.org/def/au/scma/04C3> ;
  skos:hasTopConcept <http://anzsoil.org/def/au/scma/04C4> ;
  skos:hasTopConcept <http://anzsoil.org/def/au/scma/04D1> ;
  skos:hasTopConcept <http://anzsoil.org/def/au/scma/04E1> ;
  skos:hasTopConcept <http://anzsoil.org/def/au/scma/04F1> ;
  skos:hasTopConcept <http://anzsoil.org/def/au/scma/04G1> ;
  skos:hasTopConcept <http://anzsoil.org/def/au/scma/05A1> ;
  skos:hasTopConcept <http://anzsoil.org/def/au/scma/05A2> ;
  skos:hasTopConcept <http://anzsoil.org/def/au/scma/05A3a> ;
  skos:hasTopConcept <http://anzsoil.org/def/au/scma/05A3b> ;
  skos:hasTopConcept <http://anzsoil.org/def/au/scma/05A4> ;
  skos:hasTopConcept <http://anzsoil.org/def/au/scma/06A1> ;
  skos:hasTopConcept <http://anzsoil.org/def/au/scma/06B1> ;
  skos:hasTopConcept <http://anzsoil.org/def/au/scma/06B2> ;
  skos:hasTopConcept <http://anzsoil.org/def/au/scma/06B3> ;
  skos:hasTopConcept <http://anzsoil.org/def/au/scma/06B4> ;
  skos:hasTopConcept <http://anzsoil.org/def/au/scma/06C1> ;
  skos:hasTopConcept <http://anzsoil.org/def/au/scma/06D1> ;
  skos:hasTopConcept <http://anzsoil.org/def/au/scma/06E1> ;
  skos:hasTopConcept <http://anzsoil.org/def/au/scma/06F1> ;
  skos:hasTopConcept <http://anzsoil.org/def/au/scma/06G1> ;
  skos:hasTopConcept <http://anzsoil.org/def/au/scma/07A1> ;
  skos:hasTopConcept <http://anzsoil.org/def/au/scma/07A2> ;
  skos:hasTopConcept <http://anzsoil.org/def/au/scma/07A3> ;
  skos:hasTopConcept <http://anzsoil.org/def/au/scma/07A4> ;
  skos:hasTopConcept <http://anzsoil.org/def/au/scma/07A5> ;
  skos:hasTopConcept <http://anzsoil.org/def/au/scma/07A6> ;
  skos:hasTopConcept <http://anzsoil.org/def/au/scma/07B> ;
  skos:hasTopConcept <http://anzsoil.org/def/au/scma/07C1> ;
  skos:hasTopConcept <http://anzsoil.org/def/au/scma/07C2> ;
  skos:hasTopConcept <http://anzsoil.org/def/au/scma/07D> ;
  skos:hasTopConcept <http://anzsoil.org/def/au/scma/08A1> ;
  skos:hasTopConcept <http://anzsoil.org/def/au/scma/08B1> ;
  skos:hasTopConcept <http://anzsoil.org/def/au/scma/09A> ;
  skos:hasTopConcept <http://anzsoil.org/def/au/scma/09B> ;
  skos:hasTopConcept <http://anzsoil.org/def/au/scma/09C> ;
  skos:hasTopConcept <http://anzsoil.org/def/au/scma/09D1> ;
  skos:hasTopConcept <http://anzsoil.org/def/au/scma/09E> ;
  skos:hasTopConcept <http://anzsoil.org/def/au/scma/09F1> ;
  skos:hasTopConcept <http://anzsoil.org/def/au/scma/09F2> ;
  skos:hasTopConcept <http://anzsoil.org/def/au/scma/09G1> ;
  skos:hasTopConcept <http://anzsoil.org/def/au/scma/09G2> ;
  skos:hasTopConcept <http://anzsoil.org/def/au/scma/09H1> ;
  skos:hasTopConcept <http://anzsoil.org/def/au/scma/09I> ;
  skos:hasTopConcept <http://anzsoil.org/def/au/scma/09J> ;
  skos:hasTopConcept <http://anzsoil.org/def/au/scma/09K> ;
  skos:hasTopConcept <http://anzsoil.org/def/au/scma/10A1> ;
  skos:hasTopConcept <http://anzsoil.org/def/au/scma/10A2> ;
  skos:hasTopConcept <http://anzsoil.org/def/au/scma/10B> ;
  skos:hasTopConcept <http://anzsoil.org/def/au/scma/10C1> ;
  skos:hasTopConcept <http://anzsoil.org/def/au/scma/10D1> ;
  skos:hasTopConcept <http://anzsoil.org/def/au/scma/11A1> ;
  skos:hasTopConcept <http://anzsoil.org/def/au/scma/11A2> ;
  skos:hasTopConcept <http://anzsoil.org/def/au/scma/12A1> ;
  skos:hasTopConcept <http://anzsoil.org/def/au/scma/12B1> ;
  skos:hasTopConcept <http://anzsoil.org/def/au/scma/12C1> ;
  skos:hasTopConcept <http://anzsoil.org/def/au/scma/12C2> ;
  skos:hasTopConcept <http://anzsoil.org/def/au/scma/12D1> ;
  skos:hasTopConcept <http://anzsoil.org/def/au/scma/12E1> ;
  skos:hasTopConcept <http://anzsoil.org/def/au/scma/13A1> ;
  skos:hasTopConcept <http://anzsoil.org/def/au/scma/13B1> ;
  skos:hasTopConcept <http://anzsoil.org/def/au/scma/13C1> ;
  skos:hasTopConcept <http://anzsoil.org/def/au/scma/13D> ;
  skos:hasTopConcept <http://anzsoil.org/def/au/scma/14A1> ;
  skos:hasTopConcept <http://anzsoil.org/def/au/scma/14A2> ;
  skos:hasTopConcept <http://anzsoil.org/def/au/scma/14A3> ;
  skos:hasTopConcept <http://anzsoil.org/def/au/scma/14A4> ;
  skos:hasTopConcept <http://anzsoil.org/def/au/scma/14B1> ;
  skos:hasTopConcept <http://anzsoil.org/def/au/scma/14C1> ;
  skos:hasTopConcept <http://anzsoil.org/def/au/scma/14D1> ;
  skos:hasTopConcept <http://anzsoil.org/def/au/scma/14D2> ;
  skos:hasTopConcept <http://anzsoil.org/def/au/scma/14E1> ;
  skos:hasTopConcept <http://anzsoil.org/def/au/scma/14E2> ;
  skos:hasTopConcept <http://anzsoil.org/def/au/scma/14E3> ;
  skos:hasTopConcept <http://anzsoil.org/def/au/scma/14F1> ;
  skos:hasTopConcept <http://anzsoil.org/def/au/scma/14F2> ;
  skos:hasTopConcept <http://anzsoil.org/def/au/scma/14F3> ;
  skos:hasTopConcept <http://anzsoil.org/def/au/scma/14F4> ;
  skos:hasTopConcept <http://anzsoil.org/def/au/scma/14F5> ;
  skos:hasTopConcept <http://anzsoil.org/def/au/scma/14G1> ;
  skos:hasTopConcept <http://anzsoil.org/def/au/scma/14G2> ;
  skos:hasTopConcept <http://anzsoil.org/def/au/scma/14H1> ;
  skos:hasTopConcept <http://anzsoil.org/def/au/scma/15A1> ;
  skos:hasTopConcept <http://anzsoil.org/def/au/scma/15A2> ;
  skos:hasTopConcept <http://anzsoil.org/def/au/scma/15A3> ;
  skos:hasTopConcept <http://anzsoil.org/def/au/scma/15B1> ;
  skos:hasTopConcept <http://anzsoil.org/def/au/scma/15B2> ;
  skos:hasTopConcept <http://anzsoil.org/def/au/scma/15B3> ;
  skos:hasTopConcept <http://anzsoil.org/def/au/scma/15C1> ;
  skos:hasTopConcept <http://anzsoil.org/def/au/scma/15C2> ;
  skos:hasTopConcept <http://anzsoil.org/def/au/scma/15D1> ;
  skos:hasTopConcept <http://anzsoil.org/def/au/scma/15D2> ;
  skos:hasTopConcept <http://anzsoil.org/def/au/scma/15D3> ;
  skos:hasTopConcept <http://anzsoil.org/def/au/scma/15E1> ;
  skos:hasTopConcept <http://anzsoil.org/def/au/scma/15E2> ;
  skos:hasTopConcept <http://anzsoil.org/def/au/scma/15E3> ;
  skos:hasTopConcept <http://anzsoil.org/def/au/scma/15F1> ;
  skos:hasTopConcept <http://anzsoil.org/def/au/scma/15F2> ;
  skos:hasTopConcept <http://anzsoil.org/def/au/scma/15F3> ;
  skos:hasTopConcept <http://anzsoil.org/def/au/scma/15G1> ;
  skos:hasTopConcept <http://anzsoil.org/def/au/scma/15H1> ;
  skos:hasTopConcept <http://anzsoil.org/def/au/scma/15I1> ;
  skos:hasTopConcept <http://anzsoil.org/def/au/scma/15I2> ;
  skos:hasTopConcept <http://anzsoil.org/def/au/scma/15I3> ;
  skos:hasTopConcept <http://anzsoil.org/def/au/scma/15I4> ;
  skos:hasTopConcept <http://anzsoil.org/def/au/scma/15J1> ;
  skos:hasTopConcept <http://anzsoil.org/def/au/scma/15K1> ;
  skos:hasTopConcept <http://anzsoil.org/def/au/scma/15L1> ;
  skos:hasTopConcept <http://anzsoil.org/def/au/scma/15M1> ;
  skos:hasTopConcept <http://anzsoil.org/def/au/scma/15N1> ;
  skos:hasTopConcept <http://anzsoil.org/def/au/scma/15O1> ;
  skos:hasTopConcept <http://anzsoil.org/def/au/scma/16A1> ;
  skos:hasTopConcept <http://anzsoil.org/def/au/scma/16B1> ;
  skos:hasTopConcept <http://anzsoil.org/def/au/scma/16C1> ;
  skos:hasTopConcept <http://anzsoil.org/def/au/scma/16D1> ;
  skos:hasTopConcept <http://anzsoil.org/def/au/scma/17A1> ;
  skos:hasTopConcept <http://anzsoil.org/def/au/scma/17A2> ;
  skos:hasTopConcept <http://anzsoil.org/def/au/scma/17B1> ;
  skos:hasTopConcept <http://anzsoil.org/def/au/scma/17B2> ;
  skos:hasTopConcept <http://anzsoil.org/def/au/scma/17C1> ;
  skos:hasTopConcept <http://anzsoil.org/def/au/scma/18A1> ;
  skos:hasTopConcept <http://anzsoil.org/def/au/scma/18B1> ;
  skos:hasTopConcept <http://anzsoil.org/def/au/scma/18C1> ;
  skos:hasTopConcept <http://anzsoil.org/def/au/scma/18D1> ;
  skos:hasTopConcept <http://anzsoil.org/def/au/scma/18E1> ;
  skos:hasTopConcept <http://anzsoil.org/def/au/scma/18F> ;
  skos:hasTopConcept <http://anzsoil.org/def/au/scma/18G1> ;
  skos:hasTopConcept <http://anzsoil.org/def/au/scma/19A1> ;
  skos:hasTopConcept <http://anzsoil.org/def/au/scma/19B> ;
  skos:hasTopConcept <http://anzsoil.org/def/au/scma/19C1> ;
  skos:hasTopConcept <http://anzsoil.org/def/au/scma/19D1> ;
  skos:hasTopConcept <http://anzsoil.org/def/au/scma/20A1> ;
  skos:hasTopConcept <http://anzsoil.org/def/au/scma/20B1> ;
  skos:hasTopConcept <http://anzsoil.org/def/au/scma/20C1> ;
  skos:hasTopConcept <http://anzsoil.org/def/au/scma/20D1> ;
  skos:hasTopConcept <http://anzsoil.org/def/au/scma/20E1> ;
  skos:hasTopConcept <http://anzsoil.org/def/au/scma/20F1> ;
  skos:hasTopConcept <http://anzsoil.org/def/au/scma/20F2> ;
  skos:hasTopConcept <http://anzsoil.org/def/au/scma/20G1> ;
  skos:hasTopConcept <http://anzsoil.org/def/au/scma/20H1> ;
  skos:hasTopConcept <http://anzsoil.org/def/au/scma/20I1> ;
  skos:hasTopConcept <http://anzsoil.org/def/au/scma/20J1> ;
  skos:hasTopConcept <http://anzsoil.org/def/au/scma/20K1> ;
  sdo:codeRepository <https://github.com/ANZSoilData/def-au-scma> ;
.
s:swcm-1992
  a skos:ConceptScheme ;
  dct:contributor <https://orcid.org/0000-0002-2991-2308> ;
  dct:contributor <https://orcid.org/0000-0002-3884-3420> ;
  dct:created "2022-03-04"^^xsd:date ;
  dct:description "<p>This Concept Scheme is a machine-readable representation of the classifiers described in <a href='https://catalogue.nla.gov.au/Record/685915'>Australian Laboratory Handbook of Soil and Water Chemical Methods</a> (Rayment and Higginson 1992).</p>"^^rdf:HTML ;
  dct:identifier "http://anzsoil.org/def/au/scma/swcm-1992"^^xsd:anyURI ;
  dct:isReplacedBy s:scma-2011 ;
  dct:license <https://creativecommons.org/publicdomain/zero/1.0/> ;
  dct:modified "2022-03-04"^^xsd:date ;
  dct:source <https://catalogue.nla.gov.au/Record/685915> ;
  dct:title "Australian laboratory handbook of soil and water chemical methods" ;
  skos:hasTopConcept <http://anzsoil.org/def/au/scma/01A1> ;
  skos:hasTopConcept <http://anzsoil.org/def/au/scma/01A2> ;
  skos:hasTopConcept <http://anzsoil.org/def/au/scma/01B1> ;
  skos:hasTopConcept <http://anzsoil.org/def/au/scma/02A1> ;
  skos:hasTopConcept <http://anzsoil.org/def/au/scma/02B1> ;
  skos:hasTopConcept <http://anzsoil.org/def/au/scma/02C1> ;
  skos:hasTopConcept <http://anzsoil.org/def/au/scma/02D1> ;
  skos:hasTopConcept <http://anzsoil.org/def/au/scma/03A1> ;
  skos:hasTopConcept <http://anzsoil.org/def/au/scma/03B1> ;
  skos:hasTopConcept <http://anzsoil.org/def/au/scma/03C1> ;
  skos:hasTopConcept <http://anzsoil.org/def/au/scma/03D1> ;
  skos:hasTopConcept <http://anzsoil.org/def/au/scma/04A1> ;
  skos:hasTopConcept <http://anzsoil.org/def/au/scma/04A2> ;
  skos:hasTopConcept <http://anzsoil.org/def/au/scma/04A3> ;
  skos:hasTopConcept <http://anzsoil.org/def/au/scma/04B1> ;
  skos:hasTopConcept <http://anzsoil.org/def/au/scma/04B2> ;
  skos:hasTopConcept <http://anzsoil.org/def/au/scma/04B3> ;
  skos:hasTopConcept <http://anzsoil.org/def/au/scma/04B4> ;
  skos:hasTopConcept <http://anzsoil.org/def/au/scma/04B5> ;
  skos:hasTopConcept <http://anzsoil.org/def/au/scma/04C1> ;
  skos:hasTopConcept <http://anzsoil.org/def/au/scma/04C2> ;
  skos:hasTopConcept <http://anzsoil.org/def/au/scma/04C3> ;
  skos:hasTopConcept <http://anzsoil.org/def/au/scma/04C4> ;
  skos:hasTopConcept <http://anzsoil.org/def/au/scma/04D1> ;
  skos:hasTopConcept <http://anzsoil.org/def/au/scma/04E1> ;
  skos:hasTopConcept <http://anzsoil.org/def/au/scma/04F1> ;
  skos:hasTopConcept <http://anzsoil.org/def/au/scma/04G1> ;
  skos:hasTopConcept <http://anzsoil.org/def/au/scma/05A1> ;
  skos:hasTopConcept <http://anzsoil.org/def/au/scma/05A2> ;
  skos:hasTopConcept <http://anzsoil.org/def/au/scma/05A3a> ;
  skos:hasTopConcept <http://anzsoil.org/def/au/scma/05A3b> ;
  skos:hasTopConcept <http://anzsoil.org/def/au/scma/05A4> ;
  skos:hasTopConcept <http://anzsoil.org/def/au/scma/06A1> ;
  skos:hasTopConcept <http://anzsoil.org/def/au/scma/06B1> ;
  skos:hasTopConcept <http://anzsoil.org/def/au/scma/06B2> ;
  skos:hasTopConcept <http://anzsoil.org/def/au/scma/06B3> ;
  skos:hasTopConcept <http://anzsoil.org/def/au/scma/06B4> ;
  skos:hasTopConcept <http://anzsoil.org/def/au/scma/06C1> ;
  skos:hasTopConcept <http://anzsoil.org/def/au/scma/06D1> ;
  skos:hasTopConcept <http://anzsoil.org/def/au/scma/06E1> ;
  skos:hasTopConcept <http://anzsoil.org/def/au/scma/06F1> ;
  skos:hasTopConcept <http://anzsoil.org/def/au/scma/06G1> ;
  skos:hasTopConcept <http://anzsoil.org/def/au/scma/07A1> ;
  skos:hasTopConcept <http://anzsoil.org/def/au/scma/07A2> ;
  skos:hasTopConcept <http://anzsoil.org/def/au/scma/07A3> ;
  skos:hasTopConcept <http://anzsoil.org/def/au/scma/07A4> ;
  skos:hasTopConcept <http://anzsoil.org/def/au/scma/07A5> ;
  skos:hasTopConcept <http://anzsoil.org/def/au/scma/07A6> ;
  skos:hasTopConcept <http://anzsoil.org/def/au/scma/07B> ;
  skos:hasTopConcept <http://anzsoil.org/def/au/scma/07C1> ;
  skos:hasTopConcept <http://anzsoil.org/def/au/scma/07C2> ;
  skos:hasTopConcept <http://anzsoil.org/def/au/scma/07D> ;
  skos:hasTopConcept <http://anzsoil.org/def/au/scma/08A1> ;
  skos:hasTopConcept <http://anzsoil.org/def/au/scma/08B1> ;
  skos:hasTopConcept <http://anzsoil.org/def/au/scma/09A> ;
  skos:hasTopConcept <http://anzsoil.org/def/au/scma/09B> ;
  skos:hasTopConcept <http://anzsoil.org/def/au/scma/09C> ;
  skos:hasTopConcept <http://anzsoil.org/def/au/scma/09D1> ;
  skos:hasTopConcept <http://anzsoil.org/def/au/scma/09E> ;
  skos:hasTopConcept <http://anzsoil.org/def/au/scma/09F1> ;
  skos:hasTopConcept <http://anzsoil.org/def/au/scma/09F2> ;
  skos:hasTopConcept <http://anzsoil.org/def/au/scma/09G1> ;
  skos:hasTopConcept <http://anzsoil.org/def/au/scma/09G2> ;
  skos:hasTopConcept <http://anzsoil.org/def/au/scma/09H1> ;
  skos:hasTopConcept <http://anzsoil.org/def/au/scma/09I> ;
  skos:hasTopConcept <http://anzsoil.org/def/au/scma/09J> ;
  skos:hasTopConcept <http://anzsoil.org/def/au/scma/09K> ;
  skos:hasTopConcept <http://anzsoil.org/def/au/scma/10A1> ;
  skos:hasTopConcept <http://anzsoil.org/def/au/scma/10A2> ;
  skos:hasTopConcept <http://anzsoil.org/def/au/scma/10B> ;
  skos:hasTopConcept <http://anzsoil.org/def/au/scma/10C1> ;
  skos:hasTopConcept <http://anzsoil.org/def/au/scma/10D1> ;
  skos:hasTopConcept <http://anzsoil.org/def/au/scma/11A1> ;
  skos:hasTopConcept <http://anzsoil.org/def/au/scma/11A2> ;
  skos:hasTopConcept <http://anzsoil.org/def/au/scma/12A1> ;
  skos:hasTopConcept <http://anzsoil.org/def/au/scma/12B1> ;
  skos:hasTopConcept <http://anzsoil.org/def/au/scma/12C1> ;
  skos:hasTopConcept <http://anzsoil.org/def/au/scma/12C2> ;
  skos:hasTopConcept <http://anzsoil.org/def/au/scma/12D1> ;
  skos:hasTopConcept <http://anzsoil.org/def/au/scma/12E1> ;
  skos:hasTopConcept <http://anzsoil.org/def/au/scma/13A1> ;
  skos:hasTopConcept <http://anzsoil.org/def/au/scma/13B1> ;
  skos:hasTopConcept <http://anzsoil.org/def/au/scma/13C1> ;
  skos:hasTopConcept <http://anzsoil.org/def/au/scma/13D> ;
  skos:hasTopConcept <http://anzsoil.org/def/au/scma/14A1> ;
  skos:hasTopConcept <http://anzsoil.org/def/au/scma/14A2> ;
  skos:hasTopConcept <http://anzsoil.org/def/au/scma/14A3> ;
  skos:hasTopConcept <http://anzsoil.org/def/au/scma/14A4> ;
  skos:hasTopConcept <http://anzsoil.org/def/au/scma/14B1> ;
  skos:hasTopConcept <http://anzsoil.org/def/au/scma/14C1> ;
  skos:hasTopConcept <http://anzsoil.org/def/au/scma/14D1> ;
  skos:hasTopConcept <http://anzsoil.org/def/au/scma/14D2> ;
  skos:hasTopConcept <http://anzsoil.org/def/au/scma/14E1> ;
  skos:hasTopConcept <http://anzsoil.org/def/au/scma/14E2> ;
  skos:hasTopConcept <http://anzsoil.org/def/au/scma/14E3> ;
  skos:hasTopConcept <http://anzsoil.org/def/au/scma/14F1> ;
  skos:hasTopConcept <http://anzsoil.org/def/au/scma/14F2> ;
  skos:hasTopConcept <http://anzsoil.org/def/au/scma/14F3> ;
  skos:hasTopConcept <http://anzsoil.org/def/au/scma/14F4> ;
  skos:hasTopConcept <http://anzsoil.org/def/au/scma/14F5> ;
  skos:hasTopConcept <http://anzsoil.org/def/au/scma/14G1> ;
  skos:hasTopConcept <http://anzsoil.org/def/au/scma/14G2> ;
  skos:hasTopConcept <http://anzsoil.org/def/au/scma/14H1> ;
  skos:hasTopConcept <http://anzsoil.org/def/au/scma/15A1> ;
  skos:hasTopConcept <http://anzsoil.org/def/au/scma/15A2> ;
  skos:hasTopConcept <http://anzsoil.org/def/au/scma/15A3> ;
  skos:hasTopConcept <http://anzsoil.org/def/au/scma/15B1> ;
  skos:hasTopConcept <http://anzsoil.org/def/au/scma/15B2> ;
  skos:hasTopConcept <http://anzsoil.org/def/au/scma/15B3> ;
  skos:hasTopConcept <http://anzsoil.org/def/au/scma/15C1> ;
  skos:hasTopConcept <http://anzsoil.org/def/au/scma/15C2> ;
  skos:hasTopConcept <http://anzsoil.org/def/au/scma/15D1> ;
  skos:hasTopConcept <http://anzsoil.org/def/au/scma/15D2> ;
  skos:hasTopConcept <http://anzsoil.org/def/au/scma/15D3> ;
  skos:hasTopConcept <http://anzsoil.org/def/au/scma/15E1> ;
  skos:hasTopConcept <http://anzsoil.org/def/au/scma/15E2> ;
  skos:hasTopConcept <http://anzsoil.org/def/au/scma/15E3> ;
  skos:hasTopConcept <http://anzsoil.org/def/au/scma/15F1> ;
  skos:hasTopConcept <http://anzsoil.org/def/au/scma/15F2> ;
  skos:hasTopConcept <http://anzsoil.org/def/au/scma/15F3> ;
  skos:hasTopConcept <http://anzsoil.org/def/au/scma/15G1> ;
  skos:hasTopConcept <http://anzsoil.org/def/au/scma/15H1> ;
  skos:hasTopConcept <http://anzsoil.org/def/au/scma/15I1> ;
  skos:hasTopConcept <http://anzsoil.org/def/au/scma/15I2> ;
  skos:hasTopConcept <http://anzsoil.org/def/au/scma/15I3> ;
  skos:hasTopConcept <http://anzsoil.org/def/au/scma/15I4> ;
  skos:hasTopConcept <http://anzsoil.org/def/au/scma/15J1> ;
  skos:hasTopConcept <http://anzsoil.org/def/au/scma/15K1> ;
  skos:hasTopConcept <http://anzsoil.org/def/au/scma/15L1> ;
  skos:hasTopConcept <http://anzsoil.org/def/au/scma/15M1> ;
  skos:hasTopConcept <http://anzsoil.org/def/au/scma/15N1> ;
  skos:hasTopConcept <http://anzsoil.org/def/au/scma/15O1> ;
  skos:hasTopConcept <http://anzsoil.org/def/au/scma/16A1> ;
  skos:hasTopConcept <http://anzsoil.org/def/au/scma/16B1> ;
  skos:hasTopConcept <http://anzsoil.org/def/au/scma/16C1> ;
  skos:hasTopConcept <http://anzsoil.org/def/au/scma/16D1> ;
  skos:hasTopConcept <http://anzsoil.org/def/au/scma/17A1> ;
  skos:hasTopConcept <http://anzsoil.org/def/au/scma/17A2> ;
  skos:hasTopConcept <http://anzsoil.org/def/au/scma/17B1> ;
  skos:hasTopConcept <http://anzsoil.org/def/au/scma/17B2> ;
  skos:hasTopConcept <http://anzsoil.org/def/au/scma/17C1> ;
  skos:hasTopConcept <http://anzsoil.org/def/au/scma/18A1> ;
  skos:hasTopConcept <http://anzsoil.org/def/au/scma/18B1> ;
  skos:hasTopConcept <http://anzsoil.org/def/au/scma/18C1> ;
  skos:hasTopConcept <http://anzsoil.org/def/au/scma/18D1> ;
  skos:hasTopConcept <http://anzsoil.org/def/au/scma/18E1> ;
  skos:hasTopConcept <http://anzsoil.org/def/au/scma/18F> ;
  skos:hasTopConcept <http://anzsoil.org/def/au/scma/18G1> ;
  skos:hasTopConcept <http://anzsoil.org/def/au/scma/19A1> ;
  skos:hasTopConcept <http://anzsoil.org/def/au/scma/19B> ;
  skos:hasTopConcept <http://anzsoil.org/def/au/scma/19C1> ;
  skos:hasTopConcept <http://anzsoil.org/def/au/scma/19D1> ;
  skos:hasTopConcept <http://anzsoil.org/def/au/scma/20A1> ;
  skos:hasTopConcept <http://anzsoil.org/def/au/scma/20B1> ;
  skos:hasTopConcept <http://anzsoil.org/def/au/scma/20C1> ;
  skos:hasTopConcept <http://anzsoil.org/def/au/scma/20D1> ;
  skos:hasTopConcept <http://anzsoil.org/def/au/scma/20E1> ;
  skos:hasTopConcept <http://anzsoil.org/def/au/scma/20F1> ;
  skos:hasTopConcept <http://anzsoil.org/def/au/scma/20F2> ;
  skos:hasTopConcept <http://anzsoil.org/def/au/scma/20G1> ;
  skos:hasTopConcept <http://anzsoil.org/def/au/scma/20H1> ;
  skos:hasTopConcept <http://anzsoil.org/def/au/scma/20I1> ;
  skos:hasTopConcept <http://anzsoil.org/def/au/scma/20J1> ;
  skos:hasTopConcept <http://anzsoil.org/def/au/scma/20K1> ;
  sdo:codeRepository <https://github.com/ANZSoilData/def-au-scma> ;
.
