@prefix dc: <http://purl.org/dc/elements/1.1/> .
@prefix dcat: <http://www.w3.org/ns/dcat#> .
@prefix dct: <http://purl.org/dc/terms/> .
@prefix euvoc: <http://publications.europa.eu/ontology/euvoc#> .
@prefix foaf: <http://xmlns.com/foaf/0.1/> .
@prefix org: <http://www.w3.org/ns/org#> .
@prefix owl: <http://www.w3.org/2002/07/owl#> .
@prefix prov: <http://www.w3.org/ns/prov#> .
@prefix qb: <http://purl.org/linked-data/cube#> .
@prefix rdf: <http://www.w3.org/1999/02/22-rdf-syntax-ns#> .
@prefix rdfs: <http://www.w3.org/2000/01/rdf-schema#> .
@prefix s: <http://registry.it.csiro.au/sandbox/soil/scma/> .
@prefix schema: <http://schema.org/> .
@prefix sh: <http://www.w3.org/ns/shacl#> .
@prefix skos: <http://www.w3.org/2004/02/skos/core#> .
@prefix skosthes: <http://purl.org/iso25964/skos-thes#> .
@prefix skosxl: <http://www.w3.org/2008/05/skos-xl#> .
@prefix sosa: <http://www.w3.org/ns/sosa/> .
@prefix ui: <http://purl.org/linked-data/registry-ui#> .
@prefix xsd: <http://www.w3.org/2001/XMLSchema#> .

<http://registry.it.csiro.au/sandbox/soil/scma/> a skos:ConceptScheme;
  dct:description "<p>This register contains a machine-readable representation of the classifiers described in <a href='https://www.publish.csiro.au/book/6418'>Soil Chemical Methods  Australasia</a> 1. (2011), by George E Rayment and David J Lyons. These comprise the laboratory and field chemical tests relevant to Australasia and beyond. </p> <p>Supersedes Australian Laboratory Handbook of Soil and Water Chemical Methods (Rayment and Higginson 1992) while retaining method codes and other strengths of that Handbook. This register includes the method codes from Rayment and Higginson (1992) that were made redundant or superseded by new codes in George E Rayment and David J Lyons (2011).</p>"^^rdf:HTML;
  dct:title "Soil chemical methods - Australasia"@en;
  skos:hasTopConcept s:10A1, s:10A2, s:10B, s:10C1, s:10D1, s:11A1, s:11A2, s:12A1,
    s:12B1, s:12C1, s:12C2, s:12D1, s:12E1, s:13A1, s:13B1, s:13C1, s:13D, s:14A1, s:14A2,
    s:14A3, s:14A4, s:14B1, s:14C1, s:14D1, s:14D2, s:14E1, s:14E2, s:14E3, s:14F1, s:14F2,
    s:14F3, s:14F4, s:14F5, s:14G1, s:14G2, s:14H1, s:15A1, s:15A2, s:15A3, s:15B1, s:15B2,
    s:15B3, s:15C1, s:15C2, s:15D1, s:15D2, s:15D3, s:15E1, s:15E2, s:15E3, s:15F1, s:15F2,
    s:15F3, s:15G1, s:15H1, s:15I1, s:15I2, s:15I3, s:15I4, s:15J1, s:15K1, s:15L1, s:15M1,
    s:15N1, s:15O1, s:16A1, s:16B1, s:16C1, s:16D1, s:17A1, s:17A2, s:17B1, s:17B2, s:17C1,
    s:18A1, s:18B1, s:18C1, s:18D1, s:18E1, s:18F, s:18G1, s:19A1, s:19B, s:19C1, s:19D1,
    s:1A1, s:1A2, s:1B1, s:20A1, s:20B1, s:20C1, s:20D1, s:20E1, s:20F1, s:20F2, s:20G1,
    s:20H1, s:20I1, s:20J1, s:20K1, s:2A1, s:2B1, s:2C1, s:2D1, s:3A1, s:3B1, s:3C1, s:3D1,
    s:4A1, s:4A2, s:4A3, s:4B1, s:4B2, s:4B3, s:4B4, s:4B5, s:4C1, s:4C2, s:4C3, s:4C4,
    s:4D1, s:4E1, s:4F1, s:4G1, s:5A1, s:5A2, s:5A3a, s:5A3b, s:5A4, s:6A1, s:6B1, s:6B2,
    s:6B3, s:6B4, s:6C1, s:6D1, s:6E1, s:6F1, s:6G1, s:7A1, s:7A2, s:7A3, s:7A4, s:7A5,
    s:7A6, s:7B, s:7C1, s:7C2, s:7D, s:8A1, s:8B1, s:9A, s:9B, s:9C, s:9D1, s:9E, s:9F1,
    s:9F2, s:9G1, s:9G2, s:9H1, s:9I, s:9J, s:9K .

s:1 a skos:Collection;
  dct:description "Sampling and Sample Preparation"@en;
  dct:identifier "http://registry.it.csiro.au/sandbox/soil/scma/1"^^xsd:anyURI;
  dct:source "ISBN 0909605688"@en;
  ui:topMemberOf <http://registry.it.csiro.au/sandbox/soil/scma>;
  rdfs:label "Sampling and Sample Preparation"@en;
  skos:definition "Sampling and Sample Preparation"@en;
  skos:inScheme <http://registry.it.csiro.au/sandbox/soil/scma/>;
  skos:notation "1";
  skos:note "Retired in Soil Chemical Methods Australasia, Rayment G.E. and Lyons D.J. ISBN 9780643101364"@en;
  skos:prefLabel "Sampling and Sample Preparation"@en .

s:1A2 a skos:Concept, sosa:Procedure;
  dct:description "Field sampling - diagnostic"@en;
  dct:identifier "http://registry.it.csiro.au/sandbox/soil/scma/1A2"^^xsd:anyURI;
  dct:source "ISBN 9780643101364"@en;
  rdfs:label "Field sampling - diagnostic"@en;
  skos:definition "Field sampling - diagnostic"@en;
  skos:inScheme <http://registry.it.csiro.au/sandbox/soil/scma/>;
  skos:member s:1;
  skos:notation "1A2";
  skos:prefLabel "Field sampling - diagnostic"@en;
  skos:topConceptOf <http://registry.it.csiro.au/sandbox/soil/scma/> .

s:1A1 a skos:Concept, sosa:Procedure;
  dct:description "Field sampling - soil and land use surveys"@en;
  dct:identifier "http://registry.it.csiro.au/sandbox/soil/scma/1A1"^^xsd:anyURI;
  dct:source "ISBN 9780643101364"@en;
  rdfs:label "Field sampling - soil and land use surveys"@en;
  skos:definition "Field sampling - soil and land use surveys"@en;
  skos:inScheme <http://registry.it.csiro.au/sandbox/soil/scma/>;
  skos:member s:1;
  skos:notation "1A1";
  skos:prefLabel "Field sampling - soil and land use surveys"@en;
  skos:topConceptOf <http://registry.it.csiro.au/sandbox/soil/scma/> .

s:1B1 a skos:Concept, sosa:Procedure;
  dct:description "Laboratory preparation"@en;
  dct:identifier "http://registry.it.csiro.au/sandbox/soil/scma/1B1"^^xsd:anyURI;
  dct:source "ISBN 9780643101364"@en;
  rdfs:label "Laboratory preparation"@en;
  skos:definition "Laboratory preparation"@en;
  skos:inScheme <http://registry.it.csiro.au/sandbox/soil/scma/>;
  skos:member s:1;
  skos:notation "1B1";
  skos:prefLabel "Laboratory preparation"@en;
  skos:topConceptOf <http://registry.it.csiro.au/sandbox/soil/scma/> .

s:10 a skos:Collection;
  dct:description "Sulfur"@en;
  dct:identifier "http://registry.it.csiro.au/sandbox/soil/scma/10"^^xsd:anyURI;
  dct:source "ISBN 9780643101364"@en;
  ui:topMemberOf <http://registry.it.csiro.au/sandbox/soil/scma>;
  rdfs:label "Sulfur"@en;
  skos:definition "Sulfur"@en;
  skos:inScheme <http://registry.it.csiro.au/sandbox/soil/scma/>;
  skos:notation "10";
  skos:prefLabel "Sulfur"@en .

s:10A2 a skos:Concept, sosa:Procedure;
  dct:description "Total soil S - high-temperature combustion"@en;
  dct:identifier "http://registry.it.csiro.au/sandbox/soil/scma/10A2"^^xsd:anyURI;
  dct:source "ISBN 9780643101364"@en;
  rdfs:label "Total soil S - high-temperature combustion"@en;
  skos:definition "Total soil S - high-temperature combustion"@en;
  skos:inScheme <http://registry.it.csiro.au/sandbox/soil/scma/>;
  skos:member s:10;
  skos:notation "10A2";
  skos:prefLabel "Total soil S - high-temperature combustion"@en;
  skos:topConceptOf <http://registry.it.csiro.au/sandbox/soil/scma/> .

s:10A1 a skos:Concept, sosa:Procedure;
  dct:description "Total S - X-ray fluorescence"@en;
  dct:identifier "http://registry.it.csiro.au/sandbox/soil/scma/10A1"^^xsd:anyURI;
  dct:source "ISBN 9780643101364"@en;
  rdfs:label "Total S - X-ray fluorescence"@en;
  skos:definition "Total S - X-ray fluorescence"@en;
  skos:inScheme <http://registry.it.csiro.au/sandbox/soil/scma/>;
  skos:member s:10;
  skos:notation "10A1";
  skos:prefLabel "Total S - X-ray fluorescence"@en;
  skos:topConceptOf <http://registry.it.csiro.au/sandbox/soil/scma/> .

s:10B a skos:Concept, sosa:Procedure;
  dct:description "Calcium phosphate-extractable S"@en;
  dct:identifier "http://registry.it.csiro.au/sandbox/soil/scma/10B"^^xsd:anyURI;
  dct:source "ISBN 9780643101364"@en;
  rdfs:label "Calcium phosphate-extractable S"@en;
  skos:definition "Calcium phosphate-extractable S"@en;
  skos:inScheme <http://registry.it.csiro.au/sandbox/soil/scma/>;
  skos:member s:10;
  skos:narrower s:10B1, s:10B2, s:10B3, s:10B4;
  skos:notation "10B";
  skos:prefLabel "Calcium phosphate-extractable S"@en;
  skos:topConceptOf <http://registry.it.csiro.au/sandbox/soil/scma/> .

s:10C1 a skos:Concept, sosa:Procedure;
  dct:description "Calcium phosphate-extractable S - ICPAES, + charcoal (CPC-S)"@en;
  dct:identifier "http://registry.it.csiro.au/sandbox/soil/scma/10C1"^^xsd:anyURI;
  dct:source "ISBN 9780643101364"@en;
  rdfs:label "Calcium phosphate-extractable S - ICPAES, + charcoal (CPC-S)"@en;
  skos:definition "Calcium phosphate-extractable S - ICPAES, + charcoal (CPC-S)"@en;
  skos:inScheme <http://registry.it.csiro.au/sandbox/soil/scma/>;
  skos:member s:10;
  skos:notation "10C1";
  skos:prefLabel "Calcium phosphate-extractable S - ICPAES, + charcoal (CPC-S)"@en;
  skos:topConceptOf <http://registry.it.csiro.au/sandbox/soil/scma/> .

s:10D1 a skos:Concept, sosa:Procedure;
  dct:description "Potassium Chloride - 40 Sulfur (KCl-40)-S"@en;
  dct:identifier "http://registry.it.csiro.au/sandbox/soil/scma/10D1"^^xsd:anyURI;
  dct:source "ISBN 9780643101364"@en;
  rdfs:label "Potassium Chloride - 40 Sulfur (KCl-40)-S"@en;
  skos:definition "Potassium Chloride - 40 Sulfur (KCl-40)-S"@en;
  skos:inScheme <http://registry.it.csiro.au/sandbox/soil/scma/>;
  skos:member s:10;
  skos:notation "10D1";
  skos:prefLabel "Potassium Chloride - 40 Sulfur (KCl-40)-S"@en;
  skos:topConceptOf <http://registry.it.csiro.au/sandbox/soil/scma/> .

s:10B1 a skos:Concept, sosa:Procedure;
  dct:description "Calcium phosphate-extractable S - manual distillation"@en;
  dct:identifier "http://registry.it.csiro.au/sandbox/soil/scma/10B1"^^xsd:anyURI;
  dct:source "ISBN 9780643101364"@en;
  rdfs:label "Calcium phosphate-extractable S - manual distillation"@en;
  skos:broader s:10B;
  skos:definition "Calcium phosphate-extractable S - manual distillation"@en;
  skos:inScheme <http://registry.it.csiro.au/sandbox/soil/scma/>;
  skos:notation "10B1";
  skos:prefLabel "Calcium phosphate-extractable S - manual distillation"@en .

s:10B2 a skos:Concept, sosa:Procedure;
  dct:description "Calcium phosphate-extractable S - automated distillation"@en;
  dct:identifier "http://registry.it.csiro.au/sandbox/soil/scma/10B2"^^xsd:anyURI;
  dct:source "ISBN 9780643101364"@en;
  rdfs:label "Calcium phosphate-extractable S - automated distillation"@en;
  skos:broader s:10B;
  skos:definition "Calcium phosphate-extractable S - automated distillation"@en;
  skos:inScheme <http://registry.it.csiro.au/sandbox/soil/scma/>;
  skos:notation "10B2";
  skos:prefLabel "Calcium phosphate-extractable S - automated distillation"@en .

s:10B3 a skos:Concept, sosa:Procedure;
  dct:description "Calcium phosphate-extractable S - ICPAES"@en;
  dct:identifier "http://registry.it.csiro.au/sandbox/soil/scma/10B3"^^xsd:anyURI;
  dct:source "ISBN 9780643101364"@en;
  rdfs:label "Calcium phosphate-extractable S - ICPAES"@en;
  skos:broader s:10B;
  skos:definition "Calcium phosphate-extractable S - ICPAES"@en;
  skos:inScheme <http://registry.it.csiro.au/sandbox/soil/scma/>;
  skos:notation "10B3";
  skos:prefLabel "Calcium phosphate-extractable S - ICPAES"@en .

s:10B4 a skos:Concept, sosa:Procedure;
  dct:description "Calcium phosphate-extractable S - ion chromatography"@en;
  dct:identifier "http://registry.it.csiro.au/sandbox/soil/scma/10B4"^^xsd:anyURI;
  dct:source "ISBN 9780643101364"@en;
  rdfs:label "Calcium phosphate-extractable S - ion chromatography"@en;
  skos:broader s:10B;
  skos:definition "Calcium phosphate-extractable S - ion chromatography"@en;
  skos:inScheme <http://registry.it.csiro.au/sandbox/soil/scma/>;
  skos:notation "10B4";
  skos:prefLabel "Calcium phosphate-extractable S - ion chromatography"@en .

s:11 a skos:Collection;
  dct:description "Gypsum"@en;
  dct:identifier "http://registry.it.csiro.au/sandbox/soil/scma/11"^^xsd:anyURI;
  dct:source "ISBN 9780643101364"@en;
  ui:topMemberOf <http://registry.it.csiro.au/sandbox/soil/scma>;
  rdfs:label "Gypsum"@en;
  skos:definition "Gypsum"@en;
  skos:inScheme <http://registry.it.csiro.au/sandbox/soil/scma/>;
  skos:notation "11";
  skos:prefLabel "Gypsum"@en .

s:11A2 a skos:Concept, sosa:Procedure;
  dct:description "Total gypsum by MIR reflectance spectroscopy"@en;
  dct:identifier "http://registry.it.csiro.au/sandbox/soil/scma/11A2"^^xsd:anyURI;
  dct:source "ISBN 9780643101364"@en;
  rdfs:label "Total gypsum by MIR reflectance spectroscopy"@en;
  skos:definition "Total gypsum by MIR reflectance spectroscopy"@en;
  skos:inScheme <http://registry.it.csiro.au/sandbox/soil/scma/>;
  skos:member s:11;
  skos:notation "11A2";
  skos:prefLabel "Total gypsum by MIR reflectance spectroscopy"@en;
  skos:topConceptOf <http://registry.it.csiro.au/sandbox/soil/scma/> .

s:11A1 a skos:Concept, sosa:Procedure;
  dct:description "Total gypsum"@en;
  dct:identifier "http://registry.it.csiro.au/sandbox/soil/scma/11A1"^^xsd:anyURI;
  dct:source "ISBN 9780643101364"@en;
  rdfs:label "Total gypsum"@en;
  skos:definition "Total gypsum"@en;
  skos:inScheme <http://registry.it.csiro.au/sandbox/soil/scma/>;
  skos:member s:11;
  skos:notation "11A1";
  skos:prefLabel "Total gypsum"@en;
  skos:topConceptOf <http://registry.it.csiro.au/sandbox/soil/scma/> .

s:12 a skos:Collection;
  dct:description "Micronutrients"@en;
  dct:identifier "http://registry.it.csiro.au/sandbox/soil/scma/12"^^xsd:anyURI;
  dct:source "ISBN 9780643101364"@en;
  ui:topMemberOf <http://registry.it.csiro.au/sandbox/soil/scma>;
  rdfs:label "Micronutrients"@en;
  skos:definition "Micronutrients"@en;
  skos:inScheme <http://registry.it.csiro.au/sandbox/soil/scma/>;
  skos:notation "12";
  skos:prefLabel "Micronutrients"@en .

s:12E1 a skos:Concept, sosa:Procedure;
  dct:description "Calcium chloride-extractable Mo"@en;
  dct:identifier "http://registry.it.csiro.au/sandbox/soil/scma/12E1"^^xsd:anyURI;
  dct:source "ISBN 9780643101364"@en;
  rdfs:label "Calcium chloride-extractable Mo"@en;
  skos:definition "Calcium chloride-extractable Mo"@en;
  skos:inScheme <http://registry.it.csiro.au/sandbox/soil/scma/>;
  skos:member s:12;
  skos:notation "12E1";
  skos:prefLabel "Calcium chloride-extractable Mo"@en;
  skos:topConceptOf <http://registry.it.csiro.au/sandbox/soil/scma/> .

s:12C2 a skos:Concept, sosa:Procedure;
  dct:description "Calcium chloride-extractable B - ICPAES"@en;
  dct:identifier "http://registry.it.csiro.au/sandbox/soil/scma/12C2"^^xsd:anyURI;
  dct:source "ISBN 9780643101364"@en;
  rdfs:label "Calcium chloride-extractable B - ICPAES"@en;
  skos:definition "Calcium chloride-extractable B - ICPAES"@en;
  skos:inScheme <http://registry.it.csiro.au/sandbox/soil/scma/>;
  skos:member s:12;
  skos:notation "12C2";
  skos:prefLabel "Calcium chloride-extractable B - ICPAES"@en;
  skos:topConceptOf <http://registry.it.csiro.au/sandbox/soil/scma/> .

s:12C1 a skos:Concept, sosa:Procedure;
  dct:description "Calcium chloride-extractable B - manual colour"@en;
  dct:identifier "http://registry.it.csiro.au/sandbox/soil/scma/12C1"^^xsd:anyURI;
  dct:source "ISBN 9780643101364"@en;
  rdfs:label "Calcium chloride-extractable B - manual colour"@en;
  skos:definition "Calcium chloride-extractable B - manual colour"@en;
  skos:inScheme <http://registry.it.csiro.au/sandbox/soil/scma/>;
  skos:member s:12;
  skos:notation "12C1";
  skos:prefLabel "Calcium chloride-extractable B - manual colour"@en;
  skos:topConceptOf <http://registry.it.csiro.au/sandbox/soil/scma/> .

s:12A1 a skos:Concept, sosa:Procedure;
  dct:description "DTPA-extractable Cu, Zn, Mn and Fe"@en;
  dct:identifier "http://registry.it.csiro.au/sandbox/soil/scma/12A1"^^xsd:anyURI;
  dct:source "ISBN 9780643101364"@en;
  rdfs:label "DTPA-extractable Cu, Zn, Mn and Fe"@en;
  skos:definition "DTPA-extractable Cu, Zn, Mn and Fe"@en;
  skos:inScheme <http://registry.it.csiro.au/sandbox/soil/scma/>;
  skos:member s:12;
  skos:notation "12A1";
  skos:prefLabel "DTPA-extractable Cu, Zn, Mn and Fe"@en;
  skos:topConceptOf <http://registry.it.csiro.au/sandbox/soil/scma/> .

s:12D1 a skos:Concept, sosa:Procedure;
  dct:description "0.1 M HCl-extractable Cu, Zn, Mn and Fe"@en;
  dct:identifier "http://registry.it.csiro.au/sandbox/soil/scma/12D1"^^xsd:anyURI;
  dct:source "ISBN 9780643101364"@en;
  rdfs:label "0.1 M HCl-extractable Cu, Zn, Mn and Fe"@en;
  skos:definition "0.1 M HCl-extractable Cu, Zn, Mn and Fe"@en;
  skos:inScheme <http://registry.it.csiro.au/sandbox/soil/scma/>;
  skos:member s:12;
  skos:notation "12D1";
  skos:prefLabel "0.1 M HCl-extractable Cu, Zn, Mn and Fe"@en;
  skos:topConceptOf <http://registry.it.csiro.au/sandbox/soil/scma/> .

s:12B1 a skos:Concept, sosa:Procedure;
  dct:description "Ammonium bicarbonate/EDTA-extractable Cu and Zn"@en;
  dct:identifier "http://registry.it.csiro.au/sandbox/soil/scma/12B1"^^xsd:anyURI;
  dct:source "ISBN 9780643101364"@en;
  rdfs:label "Ammonium bicarbonate/EDTA-extractable Cu and Zn"@en;
  skos:definition "Ammonium bicarbonate/EDTA-extractable Cu and Zn"@en;
  skos:inScheme <http://registry.it.csiro.au/sandbox/soil/scma/>;
  skos:member s:12;
  skos:notation "12B1";
  skos:prefLabel "Ammonium bicarbonate/EDTA-extractable Cu and Zn"@en;
  skos:topConceptOf <http://registry.it.csiro.au/sandbox/soil/scma/> .

s:13 a skos:Collection;
  dct:description "Extractable iron, aluminium and silicon"@en;
  dct:identifier "http://registry.it.csiro.au/sandbox/soil/scma/13"^^xsd:anyURI;
  dct:source "ISBN 9780643101364"@en;
  ui:topMemberOf <http://registry.it.csiro.au/sandbox/soil/scma>;
  rdfs:label "Extractable iron, aluminium and silicon"@en;
  skos:definition "Extractable iron, aluminium and silicon"@en;
  skos:inScheme <http://registry.it.csiro.au/sandbox/soil/scma/>;
  skos:notation "13";
  skos:prefLabel "Extractable iron, aluminium and silicon"@en .

s:13D a skos:Concept, sosa:Procedure;
  dct:description "Acid-extractable soil silicon"@en;
  dct:identifier "http://registry.it.csiro.au/sandbox/soil/scma/13D"^^xsd:anyURI;
  dct:source "ISBN 9780643101364"@en;
  rdfs:label "Acid-extractable soil silicon"@en;
  skos:definition "Acid-extractable soil silicon"@en;
  skos:inScheme <http://registry.it.csiro.au/sandbox/soil/scma/>;
  skos:member s:13;
  skos:narrower s:13D1, s:13D2;
  skos:notation "13D";
  skos:prefLabel "Acid-extractable soil silicon"@en;
  skos:topConceptOf <http://registry.it.csiro.au/sandbox/soil/scma/> .

s:13C1 a skos:Concept, sosa:Procedure;
  dct:description "Citrate/dihionite-extractable iron and aluminium"@en;
  dct:identifier "http://registry.it.csiro.au/sandbox/soil/scma/13C1"^^xsd:anyURI;
  dct:source "ISBN 9780643101364"@en;
  rdfs:label "Citrate/dihionite-extractable iron and aluminium"@en;
  skos:definition "Citrate/dihionite-extractable iron and aluminium"@en;
  skos:inScheme <http://registry.it.csiro.au/sandbox/soil/scma/>;
  skos:member s:13;
  skos:notation "13C1";
  skos:prefLabel "Citrate/dihionite-extractable iron and aluminium"@en;
  skos:topConceptOf <http://registry.it.csiro.au/sandbox/soil/scma/> .

s:13B1 a skos:Concept, sosa:Procedure;
  dct:description "Pyrophosphate-extractable Fe and Al"@en;
  dct:identifier "http://registry.it.csiro.au/sandbox/soil/scma/13B1"^^xsd:anyURI;
  dct:source "ISBN 9780643101364"@en;
  rdfs:label "Pyrophosphate-extractable Fe and Al"@en;
  skos:definition "Pyrophosphate-extractable Fe and Al"@en;
  skos:inScheme <http://registry.it.csiro.au/sandbox/soil/scma/>;
  skos:member s:13;
  skos:notation "13B1";
  skos:prefLabel "Pyrophosphate-extractable Fe and Al"@en;
  skos:topConceptOf <http://registry.it.csiro.au/sandbox/soil/scma/> .

s:13A1 a skos:Concept, sosa:Procedure;
  dct:description "Oxalate-extractable iron, aluminium and silicon"@en;
  dct:identifier "http://registry.it.csiro.au/sandbox/soil/scma/13A1"^^xsd:anyURI;
  dct:source "ISBN 9780643101364"@en;
  rdfs:label "Oxalate-extractable iron, aluminium and silicon"@en;
  skos:definition "Oxalate-extractable iron, aluminium and silicon"@en;
  skos:inScheme <http://registry.it.csiro.au/sandbox/soil/scma/>;
  skos:member s:13;
  skos:notation "13A1";
  skos:prefLabel "Oxalate-extractable iron, aluminium and silicon"@en;
  skos:topConceptOf <http://registry.it.csiro.au/sandbox/soil/scma/> .

s:13D1 a skos:Concept, sosa:Procedure;
  dct:description "Acid-extractable soil silicon - automated colour"@en;
  dct:identifier "http://registry.it.csiro.au/sandbox/soil/scma/13D1"^^xsd:anyURI;
  dct:source "ISBN 9780643101364"@en;
  rdfs:label "Acid-extractable soil silicon - automated colour"@en;
  skos:broader s:13D;
  skos:definition "Acid-extractable soil silicon - automated colour"@en;
  skos:inScheme <http://registry.it.csiro.au/sandbox/soil/scma/>;
  skos:notation "13D1";
  skos:prefLabel "Acid-extractable soil silicon - automated colour"@en .

s:13D2 a skos:Concept, sosa:Procedure;
  dct:description "Acid-extractable soil silicon - ICPAES"@en;
  dct:identifier "http://registry.it.csiro.au/sandbox/soil/scma/13D2"^^xsd:anyURI;
  dct:source "ISBN 9780643101364"@en;
  rdfs:label "Acid-extractable soil silicon - ICPAES"@en;
  skos:broader s:13D;
  skos:definition "Acid-extractable soil silicon - ICPAES"@en;
  skos:inScheme <http://registry.it.csiro.au/sandbox/soil/scma/>;
  skos:notation "13D2";
  skos:prefLabel "Acid-extractable soil silicon - ICPAES"@en .

s:14 a skos:Collection;
  dct:description "Saturation extracts"@en;
  dct:identifier "http://registry.it.csiro.au/sandbox/soil/scma/14"^^xsd:anyURI;
  dct:source "ISBN 9780643101364"@en;
  ui:topMemberOf <http://registry.it.csiro.au/sandbox/soil/scma>;
  rdfs:label "Saturation extracts"@en;
  skos:definition "Saturation extracts"@en;
  skos:inScheme <http://registry.it.csiro.au/sandbox/soil/scma/>;
  skos:notation "14";
  skos:prefLabel "Saturation extracts"@en .

s:14G2 a skos:Concept, sosa:Procedure;
  dct:description "Fluoride (saturation extract) - ion chromotography|Fluoride of SE - IC"@en;
  dct:identifier "http://registry.it.csiro.au/sandbox/soil/scma/14G2"^^xsd:anyURI;
  dct:source "ISBN 0909605688"@en;
  rdfs:label "Fluoride (saturation extract) - ion chromotography|Fluoride of SE - IC"@en;
  skos:definition "Fluoride (saturation extract) - ion chromotography|Fluoride of SE - IC"@en;
  skos:inScheme <http://registry.it.csiro.au/sandbox/soil/scma/>;
  skos:member s:14;
  skos:narrower s:14G2a, s:14G2b;
  skos:notation "14G2";
  skos:note "14G2 has been superseded by 14G2a and 14G2b in Soil Chemical Methods Australasia, Rayment G.E. and Lyons D.J. ISBN 9780643101364"@en;
  skos:prefLabel "Fluoride (saturation extract) - ion chromotography|Fluoride of SE - IC"@en;
  skos:topConceptOf <http://registry.it.csiro.au/sandbox/soil/scma/> .

s:14F3 a skos:Concept, sosa:Procedure;
  dct:description "Sulfate-S of SE - gravimetric"@en;
  dct:identifier "http://registry.it.csiro.au/sandbox/soil/scma/14F3"^^xsd:anyURI;
  dct:source "ISBN 9780643101364"@en;
  rdfs:label "Sulfate-S of SE - gravimetric"@en;
  skos:definition "Sulfate-S of SE - gravimetric"@en;
  skos:inScheme <http://registry.it.csiro.au/sandbox/soil/scma/>;
  skos:member s:14;
  skos:notation "14F3";
  skos:prefLabel "Sulfate-S of SE - gravimetric"@en;
  skos:topConceptOf <http://registry.it.csiro.au/sandbox/soil/scma/> .

s:14E2 a skos:Concept, sosa:Procedure;
  dct:description "Chloride (saturation extract) - ion chromotography|Chloride of SE - IC"@en;
  dct:identifier "http://registry.it.csiro.au/sandbox/soil/scma/14E2"^^xsd:anyURI;
  dct:source "ISBN 0909605688"@en;
  rdfs:label "Chloride (saturation extract) - ion chromotography|Chloride of SE - IC"@en;
  skos:definition "Chloride (saturation extract) - ion chromotography|Chloride of SE - IC"@en;
  skos:inScheme <http://registry.it.csiro.au/sandbox/soil/scma/>;
  skos:member s:14;
  skos:narrower s:14E2a, s:14E2b;
  skos:notation "14E2";
  skos:note "14E2 has been superseded by 14E2a and 14E2b in Soil Chemical Methods Australasia, Rayment G.E. and Lyons D.J. ISBN 9780643101364"@en;
  skos:prefLabel "Chloride (saturation extract) - ion chromotography|Chloride of SE - IC"@en;
  skos:topConceptOf <http://registry.it.csiro.au/sandbox/soil/scma/> .

s:14F1 a skos:Concept, sosa:Procedure;
  dct:description "Sulfate-S of SE - ICPAES (plus P and soluble cations)"@en;
  dct:identifier "http://registry.it.csiro.au/sandbox/soil/scma/14F1"^^xsd:anyURI;
  dct:source "ISBN 9780643101364"@en;
  rdfs:label "Sulfate-S of SE - ICPAES (plus P and soluble cations)"@en;
  skos:definition "Sulfate-S of SE - ICPAES (plus P and soluble cations)"@en;
  skos:inScheme <http://registry.it.csiro.au/sandbox/soil/scma/>;
  skos:member s:14;
  skos:notation "14F1";
  skos:prefLabel "Sulfate-S of SE - ICPAES (plus P and soluble cations)"@en;
  skos:topConceptOf <http://registry.it.csiro.au/sandbox/soil/scma/> .

s:14E3 a skos:Concept, sosa:Procedure;
  dct:description "Chloride of SE - ICPAES"@en;
  dct:identifier "http://registry.it.csiro.au/sandbox/soil/scma/14E3"^^xsd:anyURI;
  dct:source "ISBN 9780643101364"@en;
  rdfs:label "Chloride of SE - ICPAES"@en;
  skos:definition "Chloride of SE - ICPAES"@en;
  skos:inScheme <http://registry.it.csiro.au/sandbox/soil/scma/>;
  skos:member s:14;
  skos:notation "14E3";
  skos:prefLabel "Chloride of SE - ICPAES"@en;
  skos:topConceptOf <http://registry.it.csiro.au/sandbox/soil/scma/> .

s:14A1 a skos:Concept, sosa:Procedure;
  dct:description "Saturation extract - filter suction"@en;
  dct:identifier "http://registry.it.csiro.au/sandbox/soil/scma/14A1"^^xsd:anyURI;
  dct:source "ISBN 9780643101364"@en;
  rdfs:label "Saturation extract - filter suction"@en;
  skos:definition "Saturation extract - filter suction"@en;
  skos:inScheme <http://registry.it.csiro.au/sandbox/soil/scma/>;
  skos:member s:14;
  skos:notation "14A1";
  skos:prefLabel "Saturation extract - filter suction"@en;
  skos:topConceptOf <http://registry.it.csiro.au/sandbox/soil/scma/> .

s:14G1 a skos:Concept, sosa:Procedure;
  dct:description "Fluoride of SE - specific ion electrode"@en;
  dct:identifier "http://registry.it.csiro.au/sandbox/soil/scma/14G1"^^xsd:anyURI;
  dct:source "ISBN 9780643101364"@en;
  rdfs:label "Fluoride of SE - specific ion electrode"@en;
  skos:definition "Fluoride of SE - specific ion electrode"@en;
  skos:inScheme <http://registry.it.csiro.au/sandbox/soil/scma/>;
  skos:member s:14;
  skos:notation "14G1";
  skos:prefLabel "Fluoride of SE - specific ion electrode"@en;
  skos:topConceptOf <http://registry.it.csiro.au/sandbox/soil/scma/> .

s:14D1 a skos:Concept, sosa:Procedure;
  dct:description "Bicarbonate of SE and carbonate of SE - potentiometric titration"@en;
  dct:identifier "http://registry.it.csiro.au/sandbox/soil/scma/14D1"^^xsd:anyURI;
  dct:source "ISBN 9780643101364"@en;
  rdfs:label "Bicarbonate of SE and carbonate of SE - potentiometric titration"@en;
  skos:definition "Bicarbonate of SE and carbonate of SE - potentiometric titration"@en;
  skos:inScheme <http://registry.it.csiro.au/sandbox/soil/scma/>;
  skos:member s:14;
  skos:notation "14D1";
  skos:prefLabel "Bicarbonate of SE and carbonate of SE - potentiometric titration"@en;
  skos:topConceptOf <http://registry.it.csiro.au/sandbox/soil/scma/> .

s:14E1 a skos:Concept, sosa:Procedure;
  dct:description "Chloride of SE - potentiometric titration"@en;
  dct:identifier "http://registry.it.csiro.au/sandbox/soil/scma/14E1"^^xsd:anyURI;
  dct:source "ISBN 9780643101364"@en;
  rdfs:label "Chloride of SE - potentiometric titration"@en;
  skos:definition "Chloride of SE - potentiometric titration"@en;
  skos:inScheme <http://registry.it.csiro.au/sandbox/soil/scma/>;
  skos:member s:14;
  skos:notation "14E1";
  skos:prefLabel "Chloride of SE - potentiometric titration"@en;
  skos:topConceptOf <http://registry.it.csiro.au/sandbox/soil/scma/> .

s:14F4 a skos:Concept, sosa:Procedure;
  dct:description "Sulfate-S of SE - automated colour"@en;
  dct:identifier "http://registry.it.csiro.au/sandbox/soil/scma/14F4"^^xsd:anyURI;
  dct:source "ISBN 9780643101364"@en;
  rdfs:label "Sulfate-S of SE - automated colour"@en;
  skos:definition "Sulfate-S of SE - automated colour"@en;
  skos:inScheme <http://registry.it.csiro.au/sandbox/soil/scma/>;
  skos:member s:14;
  skos:notation "14F4";
  skos:prefLabel "Sulfate-S of SE - automated colour"@en;
  skos:topConceptOf <http://registry.it.csiro.au/sandbox/soil/scma/> .

s:14A4 a skos:Concept, sosa:Procedure;
  dct:description "Saturation extract - centrifuge, Gillman"@en;
  dct:identifier "http://registry.it.csiro.au/sandbox/soil/scma/14A4"^^xsd:anyURI;
  dct:source "ISBN 9780643101364"@en;
  rdfs:label "Saturation extract - centrifuge, Gillman"@en;
  skos:definition "Saturation extract - centrifuge, Gillman"@en;
  skos:inScheme <http://registry.it.csiro.au/sandbox/soil/scma/>;
  skos:member s:14;
  skos:notation "14A4";
  skos:prefLabel "Saturation extract - centrifuge, Gillman"@en;
  skos:topConceptOf <http://registry.it.csiro.au/sandbox/soil/scma/> .

s:14B1 a skos:Concept, sosa:Procedure;
  dct:description "Electrical conductivity of SE (EC of SE)"@en;
  dct:identifier "http://registry.it.csiro.au/sandbox/soil/scma/14B1"^^xsd:anyURI;
  dct:source "ISBN 9780643101364"@en;
  rdfs:label "Electrical conductivity of SE (EC of SE)"@en;
  skos:definition "Electrical conductivity of SE (EC of SE)"@en;
  skos:inScheme <http://registry.it.csiro.au/sandbox/soil/scma/>;
  skos:member s:14;
  skos:notation "14B1";
  skos:prefLabel "Electrical conductivity of SE (EC of SE)"@en;
  skos:topConceptOf <http://registry.it.csiro.au/sandbox/soil/scma/> .

s:14C1 a skos:Concept, sosa:Procedure;
  dct:description "pH of SE"@en;
  dct:identifier "http://registry.it.csiro.au/sandbox/soil/scma/14C1"^^xsd:anyURI;
  dct:source "ISBN 9780643101364"@en;
  rdfs:label "pH of SE"@en;
  skos:definition "pH of SE"@en;
  skos:inScheme <http://registry.it.csiro.au/sandbox/soil/scma/>;
  skos:member s:14;
  skos:notation "14C1";
  skos:prefLabel "pH of SE"@en;
  skos:topConceptOf <http://registry.it.csiro.au/sandbox/soil/scma/> .

s:14F2 a skos:Concept, sosa:Procedure;
  dct:description "Sulfate-S of SE - turbidimetric"@en;
  dct:identifier "http://registry.it.csiro.au/sandbox/soil/scma/14F2"^^xsd:anyURI;
  dct:source "ISBN 9780643101364"@en;
  rdfs:label "Sulfate-S of SE - turbidimetric"@en;
  skos:definition "Sulfate-S of SE - turbidimetric"@en;
  skos:inScheme <http://registry.it.csiro.au/sandbox/soil/scma/>;
  skos:member s:14;
  skos:notation "14F2";
  skos:prefLabel "Sulfate-S of SE - turbidimetric"@en;
  skos:topConceptOf <http://registry.it.csiro.au/sandbox/soil/scma/> .

s:14F5 a skos:Concept, sosa:Procedure;
  dct:description "Sulfate-S (saturation extract) - ion chromotography|Sulfate-S of SE - IC"@en;
  dct:identifier "http://registry.it.csiro.au/sandbox/soil/scma/14F5"^^xsd:anyURI;
  dct:source "ISBN 0909605688"@en;
  rdfs:label "Sulfate-S (saturation extract) - ion chromotography|Sulfate-S of SE - IC"@en;
  skos:definition "Sulfate-S (saturation extract) - ion chromotography|Sulfate-S of SE - IC"@en;
  skos:inScheme <http://registry.it.csiro.au/sandbox/soil/scma/>;
  skos:member s:14;
  skos:narrower s:14F5a, s:14F5b;
  skos:notation "14F5";
  skos:note "14F5 has been superseded by 14F5a and 14F5b in Soil Chemical Methods Australasia, Rayment G.E. and Lyons D.J. ISBN 9780643101364"@en;
  skos:prefLabel "Sulfate-S (saturation extract) - ion chromotography|Sulfate-S of SE - IC"@en;
  skos:topConceptOf <http://registry.it.csiro.au/sandbox/soil/scma/> .

s:14A2 a skos:Concept, sosa:Procedure;
  dct:description "Saturation extract -automatic extractor"@en;
  dct:identifier "http://registry.it.csiro.au/sandbox/soil/scma/14A2"^^xsd:anyURI;
  dct:source "ISBN 9780643101364"@en;
  rdfs:label "Saturation extract -automatic extractor"@en;
  skos:definition "Saturation extract -automatic extractor"@en;
  skos:inScheme <http://registry.it.csiro.au/sandbox/soil/scma/>;
  skos:member s:14;
  skos:notation "14A2";
  skos:prefLabel "Saturation extract -automatic extractor"@en;
  skos:topConceptOf <http://registry.it.csiro.au/sandbox/soil/scma/> .

s:14H1 a skos:Concept, sosa:Procedure;
  dct:description "Soluble bases of SE (Ca, Mg, K, Na)"@en;
  dct:identifier "http://registry.it.csiro.au/sandbox/soil/scma/14H1"^^xsd:anyURI;
  dct:source "ISBN 9780643101364"@en;
  rdfs:label "Soluble bases of SE (Ca, Mg, K, Na)"@en;
  skos:definition "Soluble bases of SE (Ca, Mg, K, Na)"@en;
  skos:inScheme <http://registry.it.csiro.au/sandbox/soil/scma/>;
  skos:member s:14;
  skos:notation "14H1";
  skos:prefLabel "Soluble bases of SE (Ca, Mg, K, Na)"@en;
  skos:topConceptOf <http://registry.it.csiro.au/sandbox/soil/scma/> .

s:14D2 a skos:Concept, sosa:Procedure;
  dct:description "Bicarbonate of SE and carbonate of SE - indicator method"@en;
  dct:identifier "http://registry.it.csiro.au/sandbox/soil/scma/14D2"^^xsd:anyURI;
  dct:source "ISBN 9780643101364"@en;
  rdfs:label "Bicarbonate of SE and carbonate of SE - indicator method"@en;
  skos:definition "Bicarbonate of SE and carbonate of SE - indicator method"@en;
  skos:inScheme <http://registry.it.csiro.au/sandbox/soil/scma/>;
  skos:member s:14;
  skos:notation "14D2";
  skos:prefLabel "Bicarbonate of SE and carbonate of SE - indicator method"@en;
  skos:topConceptOf <http://registry.it.csiro.au/sandbox/soil/scma/> .

s:14A3 a skos:Concept, sosa:Procedure;
  dct:description "Saturation extract - centrifuge, closed system"@en;
  dct:identifier "http://registry.it.csiro.au/sandbox/soil/scma/14A3"^^xsd:anyURI;
  dct:source "ISBN 9780643101364"@en;
  rdfs:label "Saturation extract - centrifuge, closed system"@en;
  skos:definition "Saturation extract - centrifuge, closed system"@en;
  skos:inScheme <http://registry.it.csiro.au/sandbox/soil/scma/>;
  skos:member s:14;
  skos:notation "14A3";
  skos:prefLabel "Saturation extract - centrifuge, closed system"@en;
  skos:topConceptOf <http://registry.it.csiro.au/sandbox/soil/scma/> .

s:14E2a a skos:Concept, sosa:Procedure;
  dct:description "Chloride of SE - IC (chemical suppression of eluent conductivity)"@en;
  dct:identifier "http://registry.it.csiro.au/sandbox/soil/scma/14E2a"^^xsd:anyURI;
  dct:source "ISBN 9780643101364"@en;
  rdfs:label "Chloride of SE - IC (chemical suppression of eluent conductivity)"@en;
  skos:broader s:14E2;
  skos:definition "Chloride of SE - IC (chemical suppression of eluent conductivity)"@en;
  skos:inScheme <http://registry.it.csiro.au/sandbox/soil/scma/>;
  skos:notation "14E2a";
  skos:prefLabel "Chloride of SE - IC (chemical suppression of eluent conductivity)"@en .

s:14E2b a skos:Concept, sosa:Procedure;
  dct:description "Chloride of SE - IC (single-column with electronic suppression of eluent conductivity)"@en;
  dct:identifier "http://registry.it.csiro.au/sandbox/soil/scma/14E2b"^^xsd:anyURI;
  dct:source "ISBN 9780643101364"@en;
  rdfs:label "Chloride of SE - IC (single-column with electronic suppression of eluent conductivity)"@en;
  skos:broader s:14E2;
  skos:definition "Chloride of SE - IC (single-column with electronic suppression of eluent conductivity)"@en;
  skos:inScheme <http://registry.it.csiro.au/sandbox/soil/scma/>;
  skos:notation "14E2b";
  skos:prefLabel "Chloride of SE - IC (single-column with electronic suppression of eluent conductivity)"@en .

s:14F5a a skos:Concept, sosa:Procedure;
  dct:description "Sulfate-S of SE - IC (chemical suppression of eluent conductivity)"@en;
  dct:identifier "http://registry.it.csiro.au/sandbox/soil/scma/14F5a"^^xsd:anyURI;
  dct:source "ISBN 9780643101364"@en;
  rdfs:label "Sulfate-S of SE - IC (chemical suppression of eluent conductivity)"@en;
  skos:broader s:14F5;
  skos:definition "Sulfate-S of SE - IC (chemical suppression of eluent conductivity)"@en;
  skos:inScheme <http://registry.it.csiro.au/sandbox/soil/scma/>;
  skos:notation "14F5a";
  skos:prefLabel "Sulfate-S of SE - IC (chemical suppression of eluent conductivity)"@en .

s:14F5b a skos:Concept, sosa:Procedure;
  dct:description "Sulfate-S of SE - IC (single-column with electronic suppression of eluent conductivity)"@en;
  dct:identifier "http://registry.it.csiro.au/sandbox/soil/scma/14F5b"^^xsd:anyURI;
  dct:source "ISBN 9780643101364"@en;
  rdfs:label "Sulfate-S of SE - IC (single-column with electronic suppression of eluent conductivity)"@en;
  skos:broader s:14F5;
  skos:definition "Sulfate-S of SE - IC (single-column with electronic suppression of eluent conductivity)"@en;
  skos:inScheme <http://registry.it.csiro.au/sandbox/soil/scma/>;
  skos:notation "14F5b";
  skos:prefLabel "Sulfate-S of SE - IC (single-column with electronic suppression of eluent conductivity)"@en .

s:14G2a a skos:Concept, sosa:Procedure;
  dct:description "Fluoride of SE - IC (chemical suppression of eluent conductivity)"@en;
  dct:identifier "http://registry.it.csiro.au/sandbox/soil/scma/14G2a"^^xsd:anyURI;
  dct:source "ISBN 9780643101364"@en;
  rdfs:label "Fluoride of SE - IC (chemical suppression of eluent conductivity)"@en;
  skos:broader s:14G2;
  skos:definition "Fluoride of SE - IC (chemical suppression of eluent conductivity)"@en;
  skos:inScheme <http://registry.it.csiro.au/sandbox/soil/scma/>;
  skos:notation "14G2a";
  skos:prefLabel "Fluoride of SE - IC (chemical suppression of eluent conductivity)"@en .

s:14G2b a skos:Concept, sosa:Procedure;
  dct:description "Fluoride of SE - IC (single-column with electronic suppression of eluent conductivity)"@en;
  dct:identifier "http://registry.it.csiro.au/sandbox/soil/scma/14G2b"^^xsd:anyURI;
  dct:source "ISBN 9780643101364"@en;
  rdfs:label "Fluoride of SE - IC (single-column with electronic suppression of eluent conductivity)"@en;
  skos:broader s:14G2;
  skos:definition "Fluoride of SE - IC (single-column with electronic suppression of eluent conductivity)"@en;
  skos:inScheme <http://registry.it.csiro.au/sandbox/soil/scma/>;
  skos:notation "14G2b";
  skos:prefLabel "Fluoride of SE - IC (single-column with electronic suppression of eluent conductivity)"@en .

s:15 a skos:Collection;
  dct:description "Ion-exchange properties"@en;
  dct:identifier "http://registry.it.csiro.au/sandbox/soil/scma/15"^^xsd:anyURI;
  dct:source "ISBN 9780643101364"@en;
  ui:topMemberOf <http://registry.it.csiro.au/sandbox/soil/scma>;
  rdfs:label "Ion-exchange properties"@en;
  skos:definition "Ion-exchange properties"@en;
  skos:inScheme <http://registry.it.csiro.au/sandbox/soil/scma/>;
  skos:notation "15";
  skos:prefLabel "Ion-exchange properties"@en .

s:15I4 a skos:Concept, sosa:Procedure;
  dct:description "Cation exchange capacity measurement - titration of NH+4 and Cl-"@en;
  dct:identifier "http://registry.it.csiro.au/sandbox/soil/scma/15I4"^^xsd:anyURI;
  dct:source "ISBN 9780643101364"@en;
  rdfs:label "Cation exchange capacity measurement - titration of NH+4 and Cl-"@en;
  skos:definition "Cation exchange capacity measurement - titration of NH+4 and Cl-"@en;
  skos:inScheme <http://registry.it.csiro.au/sandbox/soil/scma/>;
  skos:member s:15;
  skos:notation "15I4";
  skos:prefLabel "Cation exchange capacity measurement - titration of NH+4 and Cl-"@en;
  skos:topConceptOf <http://registry.it.csiro.au/sandbox/soil/scma/> .

s:15I1 a skos:Concept, sosa:Procedure;
  dct:description "Cation exchange capacity measurement - distillation of NH+4"@en;
  dct:identifier "http://registry.it.csiro.au/sandbox/soil/scma/15I1"^^xsd:anyURI;
  dct:source "ISBN 9780643101364"@en;
  rdfs:label "Cation exchange capacity measurement - distillation of NH+4"@en;
  skos:definition "Cation exchange capacity measurement - distillation of NH+4"@en;
  skos:inScheme <http://registry.it.csiro.au/sandbox/soil/scma/>;
  skos:member s:15;
  skos:notation "15I1";
  skos:prefLabel "Cation exchange capacity measurement - distillation of NH+4"@en;
  skos:topConceptOf <http://registry.it.csiro.au/sandbox/soil/scma/> .

s:15D1 a skos:Concept, sosa:Procedure;
  dct:description "Exchangeable bases and CEC - 1 M ammonium acetate at pH 7.0, pre-treatment for soluble salts, manual leach"@en;
  dct:identifier "http://registry.it.csiro.au/sandbox/soil/scma/15D1"^^xsd:anyURI;
  dct:source "ISBN 9780643101364"@en;
  rdfs:label "Exchangeable bases and CEC - 1 M ammonium acetate at pH 7.0, pre-treatment for soluble salts, manual leach"@en;
  skos:definition "Exchangeable bases and CEC - 1 M ammonium acetate at pH 7.0, pre-treatment for soluble salts, manual leach"@en;
  skos:inScheme <http://registry.it.csiro.au/sandbox/soil/scma/>;
  skos:member s:15;
  skos:notation "15D1";
  skos:prefLabel "Exchangeable bases and CEC - 1 M ammonium acetate at pH 7.0, pre-treatment for soluble salts, manual leach"@en;
  skos:topConceptOf <http://registry.it.csiro.au/sandbox/soil/scma/> .

s:15J1 a skos:Concept, sosa:Procedure;
  dct:description "Effective cation exchange capacity (ECEC)"@en;
  dct:identifier "http://registry.it.csiro.au/sandbox/soil/scma/15J1"^^xsd:anyURI;
  dct:source "ISBN 9780643101364"@en;
  rdfs:label "Effective cation exchange capacity (ECEC)"@en;
  skos:definition "Effective cation exchange capacity (ECEC)"@en;
  skos:inScheme <http://registry.it.csiro.au/sandbox/soil/scma/>;
  skos:member s:15;
  skos:notation "15J1";
  skos:prefLabel "Effective cation exchange capacity (ECEC)"@en;
  skos:topConceptOf <http://registry.it.csiro.au/sandbox/soil/scma/> .

s:15B2 a skos:Concept, sosa:Procedure;
  dct:description "Exchangeable bases and CEC - 1 M ammonium chloride at pH 7.0, pre-treatment for soluble salts"@en;
  dct:identifier "http://registry.it.csiro.au/sandbox/soil/scma/15B2"^^xsd:anyURI;
  dct:source "ISBN 9780643101364"@en;
  rdfs:label "Exchangeable bases and CEC - 1 M ammonium chloride at pH 7.0, pre-treatment for soluble salts"@en;
  skos:definition "Exchangeable bases and CEC - 1 M ammonium chloride at pH 7.0, pre-treatment for soluble salts"@en;
  skos:inScheme <http://registry.it.csiro.au/sandbox/soil/scma/>;
  skos:member s:15;
  skos:notation "15B2";
  skos:prefLabel "Exchangeable bases and CEC - 1 M ammonium chloride at pH 7.0, pre-treatment for soluble salts"@en;
  skos:topConceptOf <http://registry.it.csiro.au/sandbox/soil/scma/> .

s:15I2 a skos:Concept, sosa:Procedure;
  dct:description "Cation exchange capacity measurement - automated determination of NH+4"@en;
  dct:identifier "http://registry.it.csiro.au/sandbox/soil/scma/15I2"^^xsd:anyURI;
  dct:source "ISBN 9780643101364"@en;
  rdfs:label "Cation exchange capacity measurement - automated determination of NH+4"@en;
  skos:definition "Cation exchange capacity measurement - automated determination of NH+4"@en;
  skos:inScheme <http://registry.it.csiro.au/sandbox/soil/scma/>;
  skos:member s:15;
  skos:notation "15I2";
  skos:prefLabel "Cation exchange capacity measurement - automated determination of NH+4"@en;
  skos:topConceptOf <http://registry.it.csiro.au/sandbox/soil/scma/> .

s:15G1 a skos:Concept, sosa:Procedure;
  dct:description "Exchange acidity (H+ + Al3+) by 1 M potassium chloride"@en;
  dct:identifier "http://registry.it.csiro.au/sandbox/soil/scma/15G1"^^xsd:anyURI;
  dct:source "ISBN 9780643101364"@en;
  rdfs:label "Exchange acidity (H+ + Al3+) by 1 M potassium chloride"@en;
  skos:definition "Exchange acidity (H+ + Al3+) by 1 M potassium chloride"@en;
  skos:inScheme <http://registry.it.csiro.au/sandbox/soil/scma/>;
  skos:member s:15;
  skos:notation "15G1";
  skos:prefLabel "Exchange acidity (H+ + Al3+) by 1 M potassium chloride"@en;
  skos:topConceptOf <http://registry.it.csiro.au/sandbox/soil/scma/> .

s:15A3 a skos:Concept, sosa:Procedure;
  dct:description "Exchangeable bases - 1 M ammonium chloride at pH 7.0, adjusted for soluble Na+"@en;
  dct:identifier "http://registry.it.csiro.au/sandbox/soil/scma/15A3"^^xsd:anyURI;
  dct:source "ISBN 9780643101364"@en;
  rdfs:label "Exchangeable bases - 1 M ammonium chloride at pH 7.0, adjusted for soluble Na+"@en;
  skos:definition "Exchangeable bases - 1 M ammonium chloride at pH 7.0, adjusted for soluble Na+"@en;
  skos:inScheme <http://registry.it.csiro.au/sandbox/soil/scma/>;
  skos:member s:15;
  skos:notation "15A3";
  skos:prefLabel "Exchangeable bases - 1 M ammonium chloride at pH 7.0, adjusted for soluble Na+"@en;
  skos:topConceptOf <http://registry.it.csiro.au/sandbox/soil/scma/> .

s:15O1 a skos:Concept, sosa:Procedure;
  dct:description "Percent Al saturation"@en;
  dct:identifier "http://registry.it.csiro.au/sandbox/soil/scma/15O1"^^xsd:anyURI;
  dct:source "ISBN 9780643101364"@en;
  rdfs:label "Percent Al saturation"@en;
  skos:definition "Percent Al saturation"@en;
  skos:inScheme <http://registry.it.csiro.au/sandbox/soil/scma/>;
  skos:member s:15;
  skos:notation "15O1";
  skos:prefLabel "Percent Al saturation"@en;
  skos:topConceptOf <http://registry.it.csiro.au/sandbox/soil/scma/> .

s:15H1 a skos:Concept, sosa:Procedure;
  dct:description "Exchange acidity by triethanolamine (TEA)"@en;
  dct:identifier "http://registry.it.csiro.au/sandbox/soil/scma/15H1"^^xsd:anyURI;
  dct:source "ISBN 9780643101364"@en;
  rdfs:label "Exchange acidity by triethanolamine (TEA)"@en;
  skos:definition "Exchange acidity by triethanolamine (TEA)"@en;
  skos:inScheme <http://registry.it.csiro.au/sandbox/soil/scma/>;
  skos:member s:15;
  skos:notation "15H1";
  skos:prefLabel "Exchange acidity by triethanolamine (TEA)"@en;
  skos:topConceptOf <http://registry.it.csiro.au/sandbox/soil/scma/> .

s:15D3 a skos:Concept, sosa:Procedure;
  dct:description "Exchangeable bases and CEC - 1 M ammonium acetate at pH 7.0, rapid method with no pre-treatment for soluble salts"@en;
  dct:identifier "http://registry.it.csiro.au/sandbox/soil/scma/15D3"^^xsd:anyURI;
  dct:source "ISBN 9780643101364"@en;
  rdfs:label "Exchangeable bases and CEC - 1 M ammonium acetate at pH 7.0, rapid method with no pre-treatment for soluble salts"@en;
  skos:definition "Exchangeable bases and CEC - 1 M ammonium acetate at pH 7.0, rapid method with no pre-treatment for soluble salts"@en;
  skos:inScheme <http://registry.it.csiro.au/sandbox/soil/scma/>;
  skos:member s:15;
  skos:notation "15D3";
  skos:prefLabel "Exchangeable bases and CEC - 1 M ammonium acetate at pH 7.0, rapid method with no pre-treatment for soluble salts"@en;
  skos:topConceptOf <http://registry.it.csiro.au/sandbox/soil/scma/> .

s:15F3 a skos:Concept, sosa:Procedure;
  dct:description "Cation exchange capacity by 0.01 M AgTU+ [CEC AgTU]"@en;
  dct:identifier "http://registry.it.csiro.au/sandbox/soil/scma/15F3"^^xsd:anyURI;
  dct:source "ISBN 9780643101364"@en;
  rdfs:label "Cation exchange capacity by 0.01 M AgTU+ [CEC AgTU]"@en;
  skos:definition "Cation exchange capacity by 0.01 M AgTU+ [CEC AgTU]"@en;
  skos:inScheme <http://registry.it.csiro.au/sandbox/soil/scma/>;
  skos:member s:15;
  skos:notation "15F3";
  skos:prefLabel "Cation exchange capacity by 0.01 M AgTU+ [CEC AgTU]"@en;
  skos:topConceptOf <http://registry.it.csiro.au/sandbox/soil/scma/> .

s:15K1 a skos:Concept, sosa:Procedure;
  dct:description "Cation exchange capacity - pH 8.2 (CEC pH 8.2)"@en;
  dct:identifier "http://registry.it.csiro.au/sandbox/soil/scma/15K1"^^xsd:anyURI;
  dct:source "ISBN 9780643101364"@en;
  rdfs:label "Cation exchange capacity - pH 8.2 (CEC pH 8.2)"@en;
  skos:definition "Cation exchange capacity - pH 8.2 (CEC pH 8.2)"@en;
  skos:inScheme <http://registry.it.csiro.au/sandbox/soil/scma/>;
  skos:member s:15;
  skos:notation "15K1";
  skos:prefLabel "Cation exchange capacity - pH 8.2 (CEC pH 8.2)"@en;
  skos:topConceptOf <http://registry.it.csiro.au/sandbox/soil/scma/> .

s:15A1 a skos:Concept, sosa:Procedure;
  dct:description "Exchangeable bases (Ca2+, Mg2+, Na+, K+) - 1 M ammonium chloride at pH 7.0, no pre-treatment for soluble salts"@en;
  dct:identifier "http://registry.it.csiro.au/sandbox/soil/scma/15A1"^^xsd:anyURI;
  dct:source "ISBN 9780643101364"@en;
  rdfs:label "Exchangeable bases (Ca2+, Mg2+, Na+, K+) - 1 M ammonium chloride at pH 7.0, no pre-treatment for soluble salts"@en;
  skos:definition "Exchangeable bases (Ca2+, Mg2+, Na+, K+) - 1 M ammonium chloride at pH 7.0, no pre-treatment for soluble salts"@en;
  skos:inScheme <http://registry.it.csiro.au/sandbox/soil/scma/>;
  skos:member s:15;
  skos:notation "15A1";
  skos:prefLabel "Exchangeable bases (Ca2+, Mg2+, Na+, K+) - 1 M ammonium chloride at pH 7.0, no pre-treatment for soluble salts"@en;
  skos:topConceptOf <http://registry.it.csiro.au/sandbox/soil/scma/> .

s:15C1 a skos:Concept, sosa:Procedure;
  dct:description "Exchangeable bases and CEC - alcoholic 1 M ammonium chloride at pH 8.5, pre-treatment for soluble salts"@en;
  dct:identifier "http://registry.it.csiro.au/sandbox/soil/scma/15C1"^^xsd:anyURI;
  dct:source "ISBN 9780643101364"@en;
  rdfs:label "Exchangeable bases and CEC - alcoholic 1 M ammonium chloride at pH 8.5, pre-treatment for soluble salts"@en;
  skos:definition "Exchangeable bases and CEC - alcoholic 1 M ammonium chloride at pH 8.5, pre-treatment for soluble salts"@en;
  skos:inScheme <http://registry.it.csiro.au/sandbox/soil/scma/>;
  skos:member s:15;
  skos:notation "15C1";
  skos:prefLabel "Exchangeable bases and CEC - alcoholic 1 M ammonium chloride at pH 8.5, pre-treatment for soluble salts"@en;
  skos:topConceptOf <http://registry.it.csiro.au/sandbox/soil/scma/> .

s:15E1 a skos:Concept, sosa:Procedure;
  dct:description "Exchangeable bases, CEC and anion exchange capacity by compulsive exchange, no pre-treatment for soluble salts"@en;
  dct:identifier "http://registry.it.csiro.au/sandbox/soil/scma/15E1"^^xsd:anyURI;
  dct:source "ISBN 9780643101364"@en;
  rdfs:label "Exchangeable bases, CEC and anion exchange capacity by compulsive exchange, no pre-treatment for soluble salts"@en;
  skos:definition "Exchangeable bases, CEC and anion exchange capacity by compulsive exchange, no pre-treatment for soluble salts"@en;
  skos:inScheme <http://registry.it.csiro.au/sandbox/soil/scma/>;
  skos:member s:15;
  skos:notation "15E1";
  skos:prefLabel "Exchangeable bases, CEC and anion exchange capacity by compulsive exchange, no pre-treatment for soluble salts"@en;
  skos:topConceptOf <http://registry.it.csiro.au/sandbox/soil/scma/> .

s:15A2 a skos:Concept, sosa:Procedure;
  dct:description "Exchangeable bases by 1 M ammonium chloride at pH 7.0, pre-treatment for soluble salts"@en;
  dct:identifier "http://registry.it.csiro.au/sandbox/soil/scma/15A2"^^xsd:anyURI;
  dct:source "ISBN 9780643101364"@en;
  rdfs:label "Exchangeable bases by 1 M ammonium chloride at pH 7.0, pre-treatment for soluble salts"@en;
  skos:definition "Exchangeable bases by 1 M ammonium chloride at pH 7.0, pre-treatment for soluble salts"@en;
  skos:inScheme <http://registry.it.csiro.au/sandbox/soil/scma/>;
  skos:member s:15;
  skos:notation "15A2";
  skos:prefLabel "Exchangeable bases by 1 M ammonium chloride at pH 7.0, pre-treatment for soluble salts"@en;
  skos:topConceptOf <http://registry.it.csiro.au/sandbox/soil/scma/> .

s:15M1 a skos:Concept, sosa:Procedure;
  dct:description "Basic cation saturation ratios"@en;
  dct:identifier "http://registry.it.csiro.au/sandbox/soil/scma/15M1"^^xsd:anyURI;
  dct:source "ISBN 9780643101364"@en;
  rdfs:label "Basic cation saturation ratios"@en;
  skos:definition "Basic cation saturation ratios"@en;
  skos:inScheme <http://registry.it.csiro.au/sandbox/soil/scma/>;
  skos:member s:15;
  skos:notation "15M1";
  skos:prefLabel "Basic cation saturation ratios"@en;
  skos:topConceptOf <http://registry.it.csiro.au/sandbox/soil/scma/> .

s:15C2 a skos:Concept, sosa:Procedure;
  dct:description "Exchangeable divalent cations and CEC - by MIR diffuse reflectance spectroscopy"@en;
  dct:identifier "http://registry.it.csiro.au/sandbox/soil/scma/15C2"^^xsd:anyURI;
  dct:source "ISBN 9780643101364"@en;
  rdfs:label "Exchangeable divalent cations and CEC - by MIR diffuse reflectance spectroscopy"@en;
  skos:definition "Exchangeable divalent cations and CEC - by MIR diffuse reflectance spectroscopy"@en;
  skos:inScheme <http://registry.it.csiro.au/sandbox/soil/scma/>;
  skos:member s:15;
  skos:notation "15C2";
  skos:prefLabel "Exchangeable divalent cations and CEC - by MIR diffuse reflectance spectroscopy"@en;
  skos:topConceptOf <http://registry.it.csiro.au/sandbox/soil/scma/> .

s:15F1 a skos:Concept, sosa:Procedure;
  dct:description "Exchangeable bases by 0.01 M silver-thiourea (AgTU+) - no pre-treatment for soluble salts"@en;
  dct:identifier "http://registry.it.csiro.au/sandbox/soil/scma/15F1"^^xsd:anyURI;
  dct:source "ISBN 9780643101364"@en;
  rdfs:label "Exchangeable bases by 0.01 M silver-thiourea (AgTU+) - no pre-treatment for soluble salts"@en;
  skos:definition "Exchangeable bases by 0.01 M silver-thiourea (AgTU+) - no pre-treatment for soluble salts"@en;
  skos:inScheme <http://registry.it.csiro.au/sandbox/soil/scma/>;
  skos:member s:15;
  skos:notation "15F1";
  skos:prefLabel "Exchangeable bases by 0.01 M silver-thiourea (AgTU+) - no pre-treatment for soluble salts"@en;
  skos:topConceptOf <http://registry.it.csiro.au/sandbox/soil/scma/> .

s:15N1 a skos:Concept, sosa:Procedure;
  dct:description "Exchangeable Na+ percentage (ESP)"@en;
  dct:identifier "http://registry.it.csiro.au/sandbox/soil/scma/15N1"^^xsd:anyURI;
  dct:source "ISBN 9780643101364"@en;
  rdfs:label "Exchangeable Na+ percentage (ESP)"@en;
  skos:definition "Exchangeable Na+ percentage (ESP)"@en;
  skos:inScheme <http://registry.it.csiro.au/sandbox/soil/scma/>;
  skos:member s:15;
  skos:notation "15N1";
  skos:prefLabel "Exchangeable Na+ percentage (ESP)"@en;
  skos:topConceptOf <http://registry.it.csiro.au/sandbox/soil/scma/> .

s:15E2 a skos:Concept, sosa:Procedure;
  dct:description "Exchangeable bases, CEC and AEC by compulsive exchange, pre-treatment for soluble salts"@en;
  dct:identifier "http://registry.it.csiro.au/sandbox/soil/scma/15E2"^^xsd:anyURI;
  dct:source "ISBN 9780643101364"@en;
  rdfs:label "Exchangeable bases, CEC and AEC by compulsive exchange, pre-treatment for soluble salts"@en;
  skos:definition "Exchangeable bases, CEC and AEC by compulsive exchange, pre-treatment for soluble salts"@en;
  skos:inScheme <http://registry.it.csiro.au/sandbox/soil/scma/>;
  skos:member s:15;
  skos:notation "15E2";
  skos:prefLabel "Exchangeable bases, CEC and AEC by compulsive exchange, pre-treatment for soluble salts"@en;
  skos:topConceptOf <http://registry.it.csiro.au/sandbox/soil/scma/> .

s:15B3 a skos:Concept, sosa:Procedure;
  dct:description "Exchangeable bases and CEC - 1 M ammonium chloride at pH 7.0, adjusted for soluble Na+"@en;
  dct:identifier "http://registry.it.csiro.au/sandbox/soil/scma/15B3"^^xsd:anyURI;
  dct:source "ISBN 9780643101364"@en;
  rdfs:label "Exchangeable bases and CEC - 1 M ammonium chloride at pH 7.0, adjusted for soluble Na+"@en;
  skos:definition "Exchangeable bases and CEC - 1 M ammonium chloride at pH 7.0, adjusted for soluble Na+"@en;
  skos:inScheme <http://registry.it.csiro.au/sandbox/soil/scma/>;
  skos:member s:15;
  skos:notation "15B3";
  skos:prefLabel "Exchangeable bases and CEC - 1 M ammonium chloride at pH 7.0, adjusted for soluble Na+"@en;
  skos:topConceptOf <http://registry.it.csiro.au/sandbox/soil/scma/> .

s:15E3 a skos:Concept, sosa:Procedure;
  dct:description "Exchangeable bases, CEC and AEC by compulsive exchange, adjusted for soluble Na+"@en;
  dct:identifier "http://registry.it.csiro.au/sandbox/soil/scma/15E3"^^xsd:anyURI;
  dct:source "ISBN 9780643101364"@en;
  rdfs:label "Exchangeable bases, CEC and AEC by compulsive exchange, adjusted for soluble Na+"@en;
  skos:definition "Exchangeable bases, CEC and AEC by compulsive exchange, adjusted for soluble Na+"@en;
  skos:inScheme <http://registry.it.csiro.au/sandbox/soil/scma/>;
  skos:member s:15;
  skos:notation "15E3";
  skos:prefLabel "Exchangeable bases, CEC and AEC by compulsive exchange, adjusted for soluble Na+"@en;
  skos:topConceptOf <http://registry.it.csiro.au/sandbox/soil/scma/> .

s:15D2 a skos:Concept, sosa:Procedure;
  dct:description "Exchangeable bases and CEC - 1 M ammonium acetate at pH 7.0, pre-treatment for soluble salts, automatic extractor"@en;
  dct:identifier "http://registry.it.csiro.au/sandbox/soil/scma/15D2"^^xsd:anyURI;
  dct:source "ISBN 9780643101364"@en;
  rdfs:label "Exchangeable bases and CEC - 1 M ammonium acetate at pH 7.0, pre-treatment for soluble salts, automatic extractor"@en;
  skos:definition "Exchangeable bases and CEC - 1 M ammonium acetate at pH 7.0, pre-treatment for soluble salts, automatic extractor"@en;
  skos:inScheme <http://registry.it.csiro.au/sandbox/soil/scma/>;
  skos:member s:15;
  skos:notation "15D2";
  skos:prefLabel "Exchangeable bases and CEC - 1 M ammonium acetate at pH 7.0, pre-treatment for soluble salts, automatic extractor"@en;
  skos:topConceptOf <http://registry.it.csiro.au/sandbox/soil/scma/> .

s:15L1 a skos:Concept, sosa:Procedure;
  dct:description "Base saturation percentage (ESP)"@en;
  dct:identifier "http://registry.it.csiro.au/sandbox/soil/scma/15L1"^^xsd:anyURI;
  dct:source "ISBN 9780643101364"@en;
  rdfs:label "Base saturation percentage (ESP)"@en;
  skos:definition "Base saturation percentage (ESP)"@en;
  skos:inScheme <http://registry.it.csiro.au/sandbox/soil/scma/>;
  skos:member s:15;
  skos:notation "15L1";
  skos:prefLabel "Base saturation percentage (ESP)"@en;
  skos:topConceptOf <http://registry.it.csiro.au/sandbox/soil/scma/> .

s:15F2 a skos:Concept, sosa:Procedure;
  dct:description "Exchangeable aluminium by 0.01 M AgTU+"@en;
  dct:identifier "http://registry.it.csiro.au/sandbox/soil/scma/15F2"^^xsd:anyURI;
  dct:source "ISBN 9780643101364"@en;
  rdfs:label "Exchangeable aluminium by 0.01 M AgTU+"@en;
  skos:definition "Exchangeable aluminium by 0.01 M AgTU+"@en;
  skos:inScheme <http://registry.it.csiro.au/sandbox/soil/scma/>;
  skos:member s:15;
  skos:notation "15F2";
  skos:prefLabel "Exchangeable aluminium by 0.01 M AgTU+"@en;
  skos:topConceptOf <http://registry.it.csiro.au/sandbox/soil/scma/> .

s:15I3 a skos:Concept, sosa:Procedure;
  dct:description "Cation exchange capacity measurement - automated determination of NH+4 and Cl+"@en;
  dct:identifier "http://registry.it.csiro.au/sandbox/soil/scma/15I3"^^xsd:anyURI;
  dct:source "ISBN 9780643101364"@en;
  rdfs:label "Cation exchange capacity measurement - automated determination of NH+4 and Cl+"@en;
  skos:definition "Cation exchange capacity measurement - automated determination of NH+4 and Cl+"@en;
  skos:inScheme <http://registry.it.csiro.au/sandbox/soil/scma/>;
  skos:member s:15;
  skos:notation "15I3";
  skos:prefLabel "Cation exchange capacity measurement - automated determination of NH+4 and Cl+"@en;
  skos:topConceptOf <http://registry.it.csiro.au/sandbox/soil/scma/> .

s:15B1 a skos:Concept, sosa:Procedure;
  dct:description "Exchangeable bases and cation exchange capacity - 1 M ammonium chloride at pH 7.0, no pre-treatment for soluble salts"@en;
  dct:identifier "http://registry.it.csiro.au/sandbox/soil/scma/15B1"^^xsd:anyURI;
  dct:source "ISBN 9780643101364"@en;
  rdfs:label "Exchangeable bases and cation exchange capacity - 1 M ammonium chloride at pH 7.0, no pre-treatment for soluble salts"@en;
  skos:definition "Exchangeable bases and cation exchange capacity - 1 M ammonium chloride at pH 7.0, no pre-treatment for soluble salts"@en;
  skos:inScheme <http://registry.it.csiro.au/sandbox/soil/scma/>;
  skos:member s:15;
  skos:notation "15B1";
  skos:prefLabel "Exchangeable bases and cation exchange capacity - 1 M ammonium chloride at pH 7.0, no pre-treatment for soluble salts"@en;
  skos:topConceptOf <http://registry.it.csiro.au/sandbox/soil/scma/> .

s:16 a skos:Collection;
  dct:description "Lime requirement"@en;
  dct:identifier "http://registry.it.csiro.au/sandbox/soil/scma/16"^^xsd:anyURI;
  dct:source "ISBN 9780643101364"@en;
  ui:topMemberOf <http://registry.it.csiro.au/sandbox/soil/scma>;
  rdfs:label "Lime requirement"@en;
  skos:definition "Lime requirement"@en;
  skos:inScheme <http://registry.it.csiro.au/sandbox/soil/scma/>;
  skos:notation "16";
  skos:prefLabel "Lime requirement"@en .

s:16D1 a skos:Concept, sosa:Procedure;
  dct:description "Lime requirement - Dunn titration curves"@en;
  dct:identifier "http://registry.it.csiro.au/sandbox/soil/scma/16D1"^^xsd:anyURI;
  dct:source "ISBN 9780643101364"@en;
  rdfs:label "Lime requirement - Dunn titration curves"@en;
  skos:definition "Lime requirement - Dunn titration curves"@en;
  skos:inScheme <http://registry.it.csiro.au/sandbox/soil/scma/>;
  skos:member s:16;
  skos:notation "16D1";
  skos:prefLabel "Lime requirement - Dunn titration curves"@en;
  skos:topConceptOf <http://registry.it.csiro.au/sandbox/soil/scma/> .

s:16C1 a skos:Concept, sosa:Procedure;
  dct:description "Lime requirement - Mehlich single buffer"@en;
  dct:identifier "http://registry.it.csiro.au/sandbox/soil/scma/16C1"^^xsd:anyURI;
  dct:source "ISBN 9780643101364"@en;
  rdfs:label "Lime requirement - Mehlich single buffer"@en;
  skos:definition "Lime requirement - Mehlich single buffer"@en;
  skos:inScheme <http://registry.it.csiro.au/sandbox/soil/scma/>;
  skos:member s:16;
  skos:notation "16C1";
  skos:prefLabel "Lime requirement - Mehlich single buffer"@en;
  skos:topConceptOf <http://registry.it.csiro.au/sandbox/soil/scma/> .

s:16A1 a skos:Concept, sosa:Procedure;
  dct:description "Calculated lime rate - from exchangeable Al3+"@en;
  dct:identifier "http://registry.it.csiro.au/sandbox/soil/scma/16A1"^^xsd:anyURI;
  dct:source "ISBN 9780643101364"@en;
  rdfs:label "Calculated lime rate - from exchangeable Al3+"@en;
  skos:definition "Calculated lime rate - from exchangeable Al3+"@en;
  skos:inScheme <http://registry.it.csiro.au/sandbox/soil/scma/>;
  skos:member s:16;
  skos:notation "16A1";
  skos:prefLabel "Calculated lime rate - from exchangeable Al3+"@en;
  skos:topConceptOf <http://registry.it.csiro.au/sandbox/soil/scma/> .

s:16B1 a skos:Concept, sosa:Procedure;
  dct:description "Calculated lime rate - Cregan"@en;
  dct:identifier "http://registry.it.csiro.au/sandbox/soil/scma/16B1"^^xsd:anyURI;
  dct:source "ISBN 9780643101364"@en;
  rdfs:label "Calculated lime rate - Cregan"@en;
  skos:definition "Calculated lime rate - Cregan"@en;
  skos:inScheme <http://registry.it.csiro.au/sandbox/soil/scma/>;
  skos:member s:16;
  skos:notation "16B1";
  skos:prefLabel "Calculated lime rate - Cregan"@en;
  skos:topConceptOf <http://registry.it.csiro.au/sandbox/soil/scma/> .

s:17 a skos:Collection;
  dct:description "Total miscellaneous elements"@en;
  dct:identifier "http://registry.it.csiro.au/sandbox/soil/scma/17"^^xsd:anyURI;
  dct:source "ISBN 9780643101364"@en;
  ui:topMemberOf <http://registry.it.csiro.au/sandbox/soil/scma>;
  rdfs:label "Total miscellaneous elements"@en;
  skos:definition "Total miscellaneous elements"@en;
  skos:inScheme <http://registry.it.csiro.au/sandbox/soil/scma/>;
  skos:notation "17";
  skos:prefLabel "Total miscellaneous elements"@en .

s:17A2 a skos:Concept, sosa:Procedure;
  dct:description "Total elemental analysis of soils and sediments - microwave assisted digestion, with determination by atomic spectroscopy"@en;
  dct:identifier "http://registry.it.csiro.au/sandbox/soil/scma/17A2"^^xsd:anyURI;
  dct:source "ISBN 9780643101364"@en;
  rdfs:label "Total elemental analysis of soils and sediments - microwave assisted digestion, with determination by atomic spectroscopy"@en;
  skos:definition "Total elemental analysis of soils and sediments - microwave assisted digestion, with determination by atomic spectroscopy"@en;
  skos:inScheme <http://registry.it.csiro.au/sandbox/soil/scma/>;
  skos:member s:17;
  skos:notation "17A2";
  skos:prefLabel "Total elemental analysis of soils and sediments - microwave assisted digestion, with determination by atomic spectroscopy"@en;
  skos:topConceptOf <http://registry.it.csiro.au/sandbox/soil/scma/> .

s:17C1 a skos:Concept, sosa:Procedure;
  dct:description "Pseudo-total elements of soils and sediments - conventional aqua regia block digestion and determination by atomic spectroscopy"@en;
  dct:identifier "http://registry.it.csiro.au/sandbox/soil/scma/17C1"^^xsd:anyURI;
  dct:source "ISBN 9780643101364"@en;
  rdfs:label "Pseudo-total elements of soils and sediments - conventional aqua regia block digestion and determination by atomic spectroscopy"@en;
  skos:definition "Pseudo-total elements of soils and sediments - conventional aqua regia block digestion and determination by atomic spectroscopy"@en;
  skos:inScheme <http://registry.it.csiro.au/sandbox/soil/scma/>;
  skos:member s:17;
  skos:notation "17C1";
  skos:prefLabel "Pseudo-total elements of soils and sediments - conventional aqua regia block digestion and determination by atomic spectroscopy"@en;
  skos:topConceptOf <http://registry.it.csiro.au/sandbox/soil/scma/> .

s:17B2 a skos:Concept, sosa:Procedure;
  dct:description "Pseudo-total elements of soils and sediments - reverse aqua regia microwave assisted digestion of sludges, soils and sediments, with determination by atomic spectroscopy"@en;
  dct:identifier "http://registry.it.csiro.au/sandbox/soil/scma/17B2"^^xsd:anyURI;
  dct:source "ISBN 9780643101364"@en;
  rdfs:label "Pseudo-total elements of soils and sediments - reverse aqua regia microwave assisted digestion of sludges, soils and sediments, with determination by atomic spectroscopy"@en;
  skos:definition "Pseudo-total elements of soils and sediments - reverse aqua regia microwave assisted digestion of sludges, soils and sediments, with determination by atomic spectroscopy"@en;
  skos:inScheme <http://registry.it.csiro.au/sandbox/soil/scma/>;
  skos:member s:17;
  skos:notation "17B2";
  skos:prefLabel "Pseudo-total elements of soils and sediments - reverse aqua regia microwave assisted digestion of sludges, soils and sediments, with determination by atomic spectroscopy"@en;
  skos:topConceptOf <http://registry.it.csiro.au/sandbox/soil/scma/> .

s:17A1 a skos:Concept, sosa:Procedure;
  dct:description "Total elemental analysis of soils and sediments -X-ray fluorescence spectroscopy"@en;
  dct:identifier "http://registry.it.csiro.au/sandbox/soil/scma/17A1"^^xsd:anyURI;
  dct:source "ISBN 9780643101364"@en;
  rdfs:label "Total elemental analysis of soils and sediments -X-ray fluorescence spectroscopy"@en;
  skos:definition "Total elemental analysis of soils and sediments -X-ray fluorescence spectroscopy"@en;
  skos:inScheme <http://registry.it.csiro.au/sandbox/soil/scma/>;
  skos:member s:17;
  skos:notation "17A1";
  skos:prefLabel "Total elemental analysis of soils and sediments -X-ray fluorescence spectroscopy"@en;
  skos:topConceptOf <http://registry.it.csiro.au/sandbox/soil/scma/> .

s:17B1 a skos:Concept, sosa:Procedure;
  dct:description "Pseudo-total elemental analysis of soils and sediments - reverse aqua regia block digestion with determination by atomic spectroscopy"@en;
  dct:identifier "http://registry.it.csiro.au/sandbox/soil/scma/17B1"^^xsd:anyURI;
  dct:source "ISBN 9780643101364"@en;
  rdfs:label "Pseudo-total elemental analysis of soils and sediments - reverse aqua regia block digestion with determination by atomic spectroscopy"@en;
  skos:definition "Pseudo-total elemental analysis of soils and sediments - reverse aqua regia block digestion with determination by atomic spectroscopy"@en;
  skos:inScheme <http://registry.it.csiro.au/sandbox/soil/scma/>;
  skos:member s:17;
  skos:notation "17B1";
  skos:prefLabel "Pseudo-total elemental analysis of soils and sediments - reverse aqua regia block digestion with determination by atomic spectroscopy"@en;
  skos:topConceptOf <http://registry.it.csiro.au/sandbox/soil/scma/> .

s:18 a skos:Collection;
  dct:description "Miscellaneous extractable elements"@en;
  dct:identifier "http://registry.it.csiro.au/sandbox/soil/scma/18"^^xsd:anyURI;
  dct:source "ISBN 9780643101364"@en;
  ui:topMemberOf <http://registry.it.csiro.au/sandbox/soil/scma>;
  rdfs:label "Miscellaneous extractable elements"@en;
  skos:definition "Miscellaneous extractable elements"@en;
  skos:inScheme <http://registry.it.csiro.au/sandbox/soil/scma/>;
  skos:notation "18";
  skos:prefLabel "Miscellaneous extractable elements"@en .

s:18F a skos:Concept, sosa:Procedure;
  dct:description "Mehlich 3 multi-element tests"@en;
  dct:identifier "http://registry.it.csiro.au/sandbox/soil/scma/18F"^^xsd:anyURI;
  dct:source "ISBN 9780643101364"@en;
  rdfs:label "Mehlich 3 multi-element tests"@en;
  skos:definition "Mehlich 3 multi-element tests"@en;
  skos:inScheme <http://registry.it.csiro.au/sandbox/soil/scma/>;
  skos:member s:18;
  skos:narrower s:18F1, s:18F2;
  skos:notation "18F";
  skos:prefLabel "Mehlich 3 multi-element tests"@en;
  skos:topConceptOf <http://registry.it.csiro.au/sandbox/soil/scma/> .

s:18E1 a skos:Concept, sosa:Procedure;
  dct:description "0.01 M calcium chloride-extractable Cd"@en;
  dct:identifier "http://registry.it.csiro.au/sandbox/soil/scma/18E1"^^xsd:anyURI;
  dct:source "ISBN 9780643101364"@en;
  rdfs:label "0.01 M calcium chloride-extractable Cd"@en;
  skos:definition "0.01 M calcium chloride-extractable Cd"@en;
  skos:inScheme <http://registry.it.csiro.au/sandbox/soil/scma/>;
  skos:member s:18;
  skos:notation "18E1";
  skos:prefLabel "0.01 M calcium chloride-extractable Cd"@en;
  skos:topConceptOf <http://registry.it.csiro.au/sandbox/soil/scma/> .

s:18D1 a skos:Concept, sosa:Procedure;
  dct:description "0.1 M calcium chloride-extractable Cd"@en;
  dct:identifier "http://registry.it.csiro.au/sandbox/soil/scma/18D1"^^xsd:anyURI;
  dct:source "ISBN 9780643101364"@en;
  rdfs:label "0.1 M calcium chloride-extractable Cd"@en;
  skos:definition "0.1 M calcium chloride-extractable Cd"@en;
  skos:inScheme <http://registry.it.csiro.au/sandbox/soil/scma/>;
  skos:member s:18;
  skos:notation "18D1";
  skos:prefLabel "0.1 M calcium chloride-extractable Cd"@en;
  skos:topConceptOf <http://registry.it.csiro.au/sandbox/soil/scma/> .

s:18C1 a skos:Concept, sosa:Procedure;
  dct:description "Boiling 0.1 nitric acid-extractable K+"@en;
  dct:identifier "http://registry.it.csiro.au/sandbox/soil/scma/18C1"^^xsd:anyURI;
  dct:source "ISBN 9780643101364"@en;
  rdfs:label "Boiling 0.1 nitric acid-extractable K+"@en;
  skos:definition "Boiling 0.1 nitric acid-extractable K+"@en;
  skos:inScheme <http://registry.it.csiro.au/sandbox/soil/scma/>;
  skos:member s:18;
  skos:notation "18C1";
  skos:prefLabel "Boiling 0.1 nitric acid-extractable K+"@en;
  skos:topConceptOf <http://registry.it.csiro.au/sandbox/soil/scma/> .

s:18G1 a skos:Concept, sosa:Procedure;
  dct:description "Reverse soil K+ by copper-modified sodium tetraphenylboron extraction (TBK 4h)"@en;
  dct:identifier "http://registry.it.csiro.au/sandbox/soil/scma/18G1"^^xsd:anyURI;
  dct:source "ISBN 9780643101364"@en;
  rdfs:label "Reverse soil K+ by copper-modified sodium tetraphenylboron extraction (TBK 4h)"@en;
  skos:definition "Reverse soil K+ by copper-modified sodium tetraphenylboron extraction (TBK 4h)"@en;
  skos:inScheme <http://registry.it.csiro.au/sandbox/soil/scma/>;
  skos:member s:18;
  skos:notation "18G1";
  skos:prefLabel "Reverse soil K+ by copper-modified sodium tetraphenylboron extraction (TBK 4h)"@en;
  skos:topConceptOf <http://registry.it.csiro.au/sandbox/soil/scma/> .

s:18B1 a skos:Concept, sosa:Procedure;
  dct:description "Hydrochloric acid-extractable K+"@en;
  dct:identifier "http://registry.it.csiro.au/sandbox/soil/scma/18B1"^^xsd:anyURI;
  dct:source "ISBN 9780643101364"@en;
  rdfs:label "Hydrochloric acid-extractable K+"@en;
  skos:definition "Hydrochloric acid-extractable K+"@en;
  skos:inScheme <http://registry.it.csiro.au/sandbox/soil/scma/>;
  skos:member s:18;
  skos:notation "18B1";
  skos:prefLabel "Hydrochloric acid-extractable K+"@en;
  skos:topConceptOf <http://registry.it.csiro.au/sandbox/soil/scma/> .

s:18A1 a skos:Concept, sosa:Procedure;
  dct:description "Bicarbonate-extractable K+"@en;
  dct:identifier "http://registry.it.csiro.au/sandbox/soil/scma/18A1"^^xsd:anyURI;
  dct:source "ISBN 9780643101364"@en;
  rdfs:label "Bicarbonate-extractable K+"@en;
  skos:definition "Bicarbonate-extractable K+"@en;
  skos:inScheme <http://registry.it.csiro.au/sandbox/soil/scma/>;
  skos:member s:18;
  skos:notation "18A1";
  skos:prefLabel "Bicarbonate-extractable K+"@en;
  skos:topConceptOf <http://registry.it.csiro.au/sandbox/soil/scma/> .

s:18F1 a skos:Concept, sosa:Procedure;
  dct:description "Mehlich 3-extractable elements (P, Ca, Mg, Na, K, Fe, Cu, Mn, Zn, B, S, Al)"@en;
  dct:identifier "http://registry.it.csiro.au/sandbox/soil/scma/18F1"^^xsd:anyURI;
  dct:source "ISBN 9780643101364"@en;
  rdfs:label "Mehlich 3-extractable elements (P, Ca, Mg, Na, K, Fe, Cu, Mn, Zn, B, S, Al)"@en;
  skos:broader s:18F;
  skos:definition "Mehlich 3-extractable elements (P, Ca, Mg, Na, K, Fe, Cu, Mn, Zn, B, S, Al)"@en;
  skos:inScheme <http://registry.it.csiro.au/sandbox/soil/scma/>;
  skos:notation "18F1";
  skos:prefLabel "Mehlich 3-extractable elements (P, Ca, Mg, Na, K, Fe, Cu, Mn, Zn, B, S, Al)"@en .

s:18F2 a skos:Concept, sosa:Procedure;
  dct:description "Mehlich 3 Extractable P - colour finish"@en;
  dct:identifier "http://registry.it.csiro.au/sandbox/soil/scma/18F2"^^xsd:anyURI;
  dct:source "ISBN 9780643101364"@en;
  rdfs:label "Mehlich 3 Extractable P - colour finish"@en;
  skos:broader s:18F;
  skos:definition "Mehlich 3 Extractable P - colour finish"@en;
  skos:inScheme <http://registry.it.csiro.au/sandbox/soil/scma/>;
  skos:notation "18F2";
  skos:prefLabel "Mehlich 3 Extractable P - colour finish"@en .

s:19 a skos:Collection;
  dct:description "Alkaline earth carbonates"@en;
  dct:identifier "http://registry.it.csiro.au/sandbox/soil/scma/19"^^xsd:anyURI;
  dct:source "ISBN 9780643101364"@en;
  ui:topMemberOf <http://registry.it.csiro.au/sandbox/soil/scma>;
  rdfs:label "Alkaline earth carbonates"@en;
  skos:definition "Alkaline earth carbonates"@en;
  skos:inScheme <http://registry.it.csiro.au/sandbox/soil/scma/>;
  skos:notation "19";
  skos:prefLabel "Alkaline earth carbonates"@en .

s:19D1 a skos:Concept, sosa:Procedure;
  dct:description "Field test for carbonates with dilute HCl and effervescence class assessment"@en;
  dct:identifier "http://registry.it.csiro.au/sandbox/soil/scma/19D1"^^xsd:anyURI;
  dct:source "ISBN 9780643101364"@en;
  rdfs:label "Field test for carbonates with dilute HCl and effervescence class assessment"@en;
  skos:definition "Field test for carbonates with dilute HCl and effervescence class assessment"@en;
  skos:inScheme <http://registry.it.csiro.au/sandbox/soil/scma/>;
  skos:member s:19;
  skos:notation "19D1";
  skos:prefLabel "Field test for carbonates with dilute HCl and effervescence class assessment"@en;
  skos:topConceptOf <http://registry.it.csiro.au/sandbox/soil/scma/> .

s:19C1 a skos:Concept, sosa:Procedure;
  dct:description "Spot field test for the presence of soil carbonates with dilute HCl"@en;
  dct:identifier "http://registry.it.csiro.au/sandbox/soil/scma/19C1"^^xsd:anyURI;
  dct:source "ISBN 9780643101364"@en;
  rdfs:label "Spot field test for the presence of soil carbonates with dilute HCl"@en;
  skos:definition "Spot field test for the presence of soil carbonates with dilute HCl"@en;
  skos:inScheme <http://registry.it.csiro.au/sandbox/soil/scma/>;
  skos:member s:19;
  skos:notation "19C1";
  skos:prefLabel "Spot field test for the presence of soil carbonates with dilute HCl"@en;
  skos:topConceptOf <http://registry.it.csiro.au/sandbox/soil/scma/> .

s:19B a skos:Concept, sosa:Procedure;
  dct:description "Carbonates by pressure change"@en;
  dct:identifier "http://registry.it.csiro.au/sandbox/soil/scma/19B"^^xsd:anyURI;
  dct:source "ISBN 9780643101364"@en;
  rdfs:label "Carbonates by pressure change"@en;
  skos:definition "Carbonates by pressure change"@en;
  skos:inScheme <http://registry.it.csiro.au/sandbox/soil/scma/>;
  skos:member s:19;
  skos:narrower s:19B1, s:19B2;
  skos:notation "19B";
  skos:prefLabel "Carbonates by pressure change"@en;
  skos:topConceptOf <http://registry.it.csiro.au/sandbox/soil/scma/> .

s:19A1 a skos:Concept, sosa:Procedure;
  dct:description "Carbonates -rapid titration"@en;
  dct:identifier "http://registry.it.csiro.au/sandbox/soil/scma/19A1"^^xsd:anyURI;
  dct:source "ISBN 9780643101364"@en;
  rdfs:label "Carbonates -rapid titration"@en;
  skos:definition "Carbonates -rapid titration"@en;
  skos:inScheme <http://registry.it.csiro.au/sandbox/soil/scma/>;
  skos:member s:19;
  skos:notation "19A1";
  skos:prefLabel "Carbonates -rapid titration"@en;
  skos:topConceptOf <http://registry.it.csiro.au/sandbox/soil/scma/> .

s:19B1 a skos:Concept, sosa:Procedure;
  dct:description "Carbonates by pressure change - manometric"@en;
  dct:identifier "http://registry.it.csiro.au/sandbox/soil/scma/19B1"^^xsd:anyURI;
  dct:source "ISBN 9780643101364"@en;
  rdfs:label "Carbonates by pressure change - manometric"@en;
  skos:broader s:19B;
  skos:definition "Carbonates by pressure change - manometric"@en;
  skos:inScheme <http://registry.it.csiro.au/sandbox/soil/scma/>;
  skos:notation "19B1";
  skos:prefLabel "Carbonates by pressure change - manometric"@en .

s:19B2 a skos:Concept, sosa:Procedure;
  dct:description "Carbonates by pressure change - transducer"@en;
  dct:identifier "http://registry.it.csiro.au/sandbox/soil/scma/19B2"^^xsd:anyURI;
  dct:source "ISBN 9780643101364"@en;
  rdfs:label "Carbonates by pressure change - transducer"@en;
  skos:broader s:19B;
  skos:definition "Carbonates by pressure change - transducer"@en;
  skos:inScheme <http://registry.it.csiro.au/sandbox/soil/scma/>;
  skos:notation "19B2";
  skos:prefLabel "Carbonates by pressure change - transducer"@en .

s:2 a skos:Collection;
  dct:description "Sampling, preparation and moisture content"@en;
  dct:identifier "http://registry.it.csiro.au/sandbox/soil/scma/2"^^xsd:anyURI;
  dct:source "ISBN 0909605688"@en;
  ui:topMemberOf <http://registry.it.csiro.au/sandbox/soil/scma>;
  rdfs:label "Sampling, preparation and moisture content"@en;
  skos:definition "Sampling, preparation and moisture content"@en;
  skos:inScheme <http://registry.it.csiro.au/sandbox/soil/scma/>;
  skos:notation "2";
  skos:prefLabel "Sampling, preparation and moisture content"@en .

s:2D1 a skos:Concept, sosa:Procedure;
  dct:description "Moisture content - approximate saturation paste"@en;
  dct:identifier "http://registry.it.csiro.au/sandbox/soil/scma/2D1"^^xsd:anyURI;
  dct:source "ISBN 9780643101364"@en;
  rdfs:label "Moisture content - approximate saturation paste"@en;
  skos:definition "Moisture content - approximate saturation paste"@en;
  skos:inScheme <http://registry.it.csiro.au/sandbox/soil/scma/>;
  skos:member s:2;
  skos:notation "2D1";
  skos:prefLabel "Moisture content - approximate saturation paste"@en;
  skos:topConceptOf <http://registry.it.csiro.au/sandbox/soil/scma/> .

s:2B1 a skos:Concept, sosa:Procedure;
  dct:description "As received moisture content"@en;
  dct:identifier "http://registry.it.csiro.au/sandbox/soil/scma/2B1"^^xsd:anyURI;
  dct:source "ISBN 9780643101364"@en;
  rdfs:label "As received moisture content"@en;
  skos:definition "As received moisture content"@en;
  skos:inScheme <http://registry.it.csiro.au/sandbox/soil/scma/>;
  skos:member s:2;
  skos:notation "2B1";
  skos:prefLabel "As received moisture content"@en;
  skos:topConceptOf <http://registry.it.csiro.au/sandbox/soil/scma/> .

s:2A1 a skos:Concept, sosa:Procedure;
  dct:description "Air-dry moisture content"@en;
  dct:identifier "http://registry.it.csiro.au/sandbox/soil/scma/2A1"^^xsd:anyURI;
  dct:source "ISBN 9780643101364"@en;
  rdfs:label "Air-dry moisture content"@en;
  skos:definition "Air-dry moisture content"@en;
  skos:inScheme <http://registry.it.csiro.au/sandbox/soil/scma/>;
  skos:member s:2;
  skos:notation "2A1";
  skos:prefLabel "Air-dry moisture content"@en;
  skos:topConceptOf <http://registry.it.csiro.au/sandbox/soil/scma/> .

s:2C1 a skos:Concept, sosa:Procedure;
  dct:description "Moisture content - 10 mm tension"@en;
  dct:identifier "http://registry.it.csiro.au/sandbox/soil/scma/2C1"^^xsd:anyURI;
  dct:source "ISBN 9780643101364"@en;
  rdfs:label "Moisture content - 10 mm tension"@en;
  skos:definition "Moisture content - 10 mm tension"@en;
  skos:inScheme <http://registry.it.csiro.au/sandbox/soil/scma/>;
  skos:member s:2;
  skos:notation "2C1";
  skos:prefLabel "Moisture content - 10 mm tension"@en;
  skos:topConceptOf <http://registry.it.csiro.au/sandbox/soil/scma/> .

s:20 a skos:Collection;
  dct:description "Acid sulfate soils"@en;
  dct:identifier "http://registry.it.csiro.au/sandbox/soil/scma/20"^^xsd:anyURI;
  dct:source "ISBN 9780643101364"@en;
  ui:topMemberOf <http://registry.it.csiro.au/sandbox/soil/scma>;
  rdfs:label "Acid sulfate soils"@en;
  skos:definition "Acid sulfate soils"@en;
  skos:inScheme <http://registry.it.csiro.au/sandbox/soil/scma/>;
  skos:notation "20";
  skos:prefLabel "Acid sulfate soils"@en .

s:20E1 a skos:Concept, sosa:Procedure;
  dct:description "1 M KCl-extractable S, Ca and Mg after peroxide oxidation"@en;
  dct:identifier "http://registry.it.csiro.au/sandbox/soil/scma/20E1"^^xsd:anyURI;
  dct:source "ISBN 9780643101364"@en;
  rdfs:label "1 M KCl-extractable S, Ca and Mg after peroxide oxidation"@en;
  skos:definition "1 M KCl-extractable S, Ca and Mg after peroxide oxidation"@en;
  skos:inScheme <http://registry.it.csiro.au/sandbox/soil/scma/>;
  skos:member s:20;
  skos:notation "20E1";
  skos:prefLabel "1 M KCl-extractable S, Ca and Mg after peroxide oxidation"@en;
  skos:topConceptOf <http://registry.it.csiro.au/sandbox/soil/scma/> .

s:20C1 a skos:Concept, sosa:Procedure;
  dct:description "SPOCAS acid trail - titratable peroxide acidity (TPA) and Net (excess) Acid Neutralising Capacity (a-ANC E)"@en;
  dct:identifier "http://registry.it.csiro.au/sandbox/soil/scma/20C1"^^xsd:anyURI;
  dct:source "ISBN 9780643101364"@en;
  rdfs:label "SPOCAS acid trail - titratable peroxide acidity (TPA) and Net (excess) Acid Neutralising Capacity (a-ANC E)"@en;
  skos:definition "SPOCAS acid trail - titratable peroxide acidity (TPA) and Net (excess) Acid Neutralising Capacity (a-ANC E)"@en;
  skos:inScheme <http://registry.it.csiro.au/sandbox/soil/scma/>;
  skos:member s:20;
  skos:notation "20C1";
  skos:prefLabel "SPOCAS acid trail - titratable peroxide acidity (TPA) and Net (excess) Acid Neutralising Capacity (a-ANC E)"@en;
  skos:topConceptOf <http://registry.it.csiro.au/sandbox/soil/scma/> .

s:20D1 a skos:Concept, sosa:Procedure;
  dct:description "1 M KCl-extractable S, Ca and Mg"@en;
  dct:identifier "http://registry.it.csiro.au/sandbox/soil/scma/20D1"^^xsd:anyURI;
  dct:source "ISBN 9780643101364"@en;
  rdfs:label "1 M KCl-extractable S, Ca and Mg"@en;
  skos:definition "1 M KCl-extractable S, Ca and Mg"@en;
  skos:inScheme <http://registry.it.csiro.au/sandbox/soil/scma/>;
  skos:member s:20;
  skos:notation "20D1";
  skos:prefLabel "1 M KCl-extractable S, Ca and Mg"@en;
  skos:topConceptOf <http://registry.it.csiro.au/sandbox/soil/scma/> .

s:20B1 a skos:Concept, sosa:Procedure;
  dct:description "SPOCAS acid trail - titratable actual acidity (TAA)"@en;
  dct:identifier "http://registry.it.csiro.au/sandbox/soil/scma/20B1"^^xsd:anyURI;
  dct:source "ISBN 9780643101364"@en;
  rdfs:label "SPOCAS acid trail - titratable actual acidity (TAA)"@en;
  skos:definition "SPOCAS acid trail - titratable actual acidity (TAA)"@en;
  skos:inScheme <http://registry.it.csiro.au/sandbox/soil/scma/>;
  skos:member s:20;
  skos:notation "20B1";
  skos:prefLabel "SPOCAS acid trail - titratable actual acidity (TAA)"@en;
  skos:topConceptOf <http://registry.it.csiro.au/sandbox/soil/scma/> .

s:20K1 a skos:Concept, sosa:Procedure;
  dct:description "Quick field approximations of ASS presence and associated lime requirement for drain-spoil"@en;
  dct:identifier "http://registry.it.csiro.au/sandbox/soil/scma/20K1"^^xsd:anyURI;
  dct:source "ISBN 9780643101364"@en;
  rdfs:label "Quick field approximations of ASS presence and associated lime requirement for drain-spoil"@en;
  skos:definition "Quick field approximations of ASS presence and associated lime requirement for drain-spoil"@en;
  skos:inScheme <http://registry.it.csiro.au/sandbox/soil/scma/>;
  skos:member s:20;
  skos:notation "20K1";
  skos:prefLabel "Quick field approximations of ASS presence and associated lime requirement for drain-spoil"@en;
  skos:topConceptOf <http://registry.it.csiro.au/sandbox/soil/scma/> .

s:20I1 a skos:Concept, sosa:Procedure;
  dct:description "Acid neutralising capacity - from SPOCAS"@en;
  dct:identifier "http://registry.it.csiro.au/sandbox/soil/scma/20I1"^^xsd:anyURI;
  dct:source "ISBN 9780643101364"@en;
  rdfs:label "Acid neutralising capacity - from SPOCAS"@en;
  skos:definition "Acid neutralising capacity - from SPOCAS"@en;
  skos:inScheme <http://registry.it.csiro.au/sandbox/soil/scma/>;
  skos:member s:20;
  skos:notation "20I1";
  skos:prefLabel "Acid neutralising capacity - from SPOCAS"@en;
  skos:topConceptOf <http://registry.it.csiro.au/sandbox/soil/scma/> .

s:20G1 a skos:Concept, sosa:Procedure;
  dct:description "Peroxide residual acid soluble sulfur (S RAS)"@en;
  dct:identifier "http://registry.it.csiro.au/sandbox/soil/scma/20G1"^^xsd:anyURI;
  dct:source "ISBN 9780643101364"@en;
  rdfs:label "Peroxide residual acid soluble sulfur (S RAS)"@en;
  skos:definition "Peroxide residual acid soluble sulfur (S RAS)"@en;
  skos:inScheme <http://registry.it.csiro.au/sandbox/soil/scma/>;
  skos:member s:20;
  skos:notation "20G1";
  skos:prefLabel "Peroxide residual acid soluble sulfur (S RAS)"@en;
  skos:topConceptOf <http://registry.it.csiro.au/sandbox/soil/scma/> .

s:20F2 a skos:Concept, sosa:Procedure;
  dct:description "Sulfur - 4 M HCl extraction (S HCl), ion chromatography finish"@en;
  dct:identifier "http://registry.it.csiro.au/sandbox/soil/scma/20F2"^^xsd:anyURI;
  dct:source "ISBN 9780643101364"@en;
  rdfs:label "Sulfur - 4 M HCl extraction (S HCl), ion chromatography finish"@en;
  skos:definition "Sulfur - 4 M HCl extraction (S HCl), ion chromatography finish"@en;
  skos:inScheme <http://registry.it.csiro.au/sandbox/soil/scma/>;
  skos:member s:20;
  skos:notation "20F2";
  skos:prefLabel "Sulfur - 4 M HCl extraction (S HCl), ion chromatography finish"@en;
  skos:topConceptOf <http://registry.it.csiro.au/sandbox/soil/scma/> .

s:20J1 a skos:Concept, sosa:Procedure;
  dct:description "Field approximation of ASS hazard"@en;
  dct:identifier "http://registry.it.csiro.au/sandbox/soil/scma/20J1"^^xsd:anyURI;
  dct:source "ISBN 9780643101364"@en;
  rdfs:label "Field approximation of ASS hazard"@en;
  skos:definition "Field approximation of ASS hazard"@en;
  skos:inScheme <http://registry.it.csiro.au/sandbox/soil/scma/>;
  skos:member s:20;
  skos:notation "20J1";
  skos:prefLabel "Field approximation of ASS hazard"@en;
  skos:topConceptOf <http://registry.it.csiro.au/sandbox/soil/scma/> .

s:20A1 a skos:Concept, sosa:Procedure;
  dct:description "Chromium reducible S (S CR)"@en;
  dct:identifier "http://registry.it.csiro.au/sandbox/soil/scma/20A1"^^xsd:anyURI;
  dct:source "ISBN 9780643101364"@en;
  rdfs:label "Chromium reducible S (S CR)"@en;
  skos:definition "Chromium reducible S (S CR)"@en;
  skos:inScheme <http://registry.it.csiro.au/sandbox/soil/scma/>;
  skos:member s:20;
  skos:notation "20A1";
  skos:prefLabel "Chromium reducible S (S CR)"@en;
  skos:topConceptOf <http://registry.it.csiro.au/sandbox/soil/scma/> .

s:20H1 a skos:Concept, sosa:Procedure;
  dct:description "Acid neutralising capacity - acid reacted and back titration (ANC BT)"@en;
  dct:identifier "http://registry.it.csiro.au/sandbox/soil/scma/20H1"^^xsd:anyURI;
  dct:source "ISBN 9780643101364"@en;
  rdfs:label "Acid neutralising capacity - acid reacted and back titration (ANC BT)"@en;
  skos:definition "Acid neutralising capacity - acid reacted and back titration (ANC BT)"@en;
  skos:inScheme <http://registry.it.csiro.au/sandbox/soil/scma/>;
  skos:member s:20;
  skos:notation "20H1";
  skos:prefLabel "Acid neutralising capacity - acid reacted and back titration (ANC BT)"@en;
  skos:topConceptOf <http://registry.it.csiro.au/sandbox/soil/scma/> .

s:20F1 a skos:Concept, sosa:Procedure;
  dct:description "Sulfur - 4 M HCl extraction (S HCl), ICPAES finish"@en;
  dct:identifier "http://registry.it.csiro.au/sandbox/soil/scma/20F1"^^xsd:anyURI;
  dct:source "ISBN 9780643101364"@en;
  rdfs:label "Sulfur - 4 M HCl extraction (S HCl), ICPAES finish"@en;
  skos:definition "Sulfur - 4 M HCl extraction (S HCl), ICPAES finish"@en;
  skos:inScheme <http://registry.it.csiro.au/sandbox/soil/scma/>;
  skos:member s:20;
  skos:notation "20F1";
  skos:prefLabel "Sulfur - 4 M HCl extraction (S HCl), ICPAES finish"@en;
  skos:topConceptOf <http://registry.it.csiro.au/sandbox/soil/scma/> .

s:3 a skos:Collection;
  dct:description "Electrical conductivity, related attributes and redox potential"@en;
  dct:identifier "http://registry.it.csiro.au/sandbox/soil/scma/3"^^xsd:anyURI;
  dct:source "ISBN 9780643101364"@en;
  ui:topMemberOf <http://registry.it.csiro.au/sandbox/soil/scma>;
  rdfs:label "Electrical conductivity, related attributes and redox potential"@en;
  skos:definition "Electrical conductivity, related attributes and redox potential"@en;
  skos:inScheme <http://registry.it.csiro.au/sandbox/soil/scma/>;
  skos:notation "3";
  skos:prefLabel "Electrical conductivity, related attributes and redox potential"@en .

s:3A1 a skos:Concept, sosa:Procedure;
  dct:description "Electrical conductivity (EC) of 1:5 soil/water extract"@en;
  dct:identifier "http://registry.it.csiro.au/sandbox/soil/scma/3A1"^^xsd:anyURI;
  dct:source "ISBN 9780643101364"@en;
  rdfs:label "Electrical conductivity (EC) of 1:5 soil/water extract"@en;
  skos:definition "Electrical conductivity (EC) of 1:5 soil/water extract"@en;
  skos:inScheme <http://registry.it.csiro.au/sandbox/soil/scma/>;
  skos:member s:3;
  skos:notation "3A1";
  skos:prefLabel "Electrical conductivity (EC) of 1:5 soil/water extract"@en;
  skos:topConceptOf <http://registry.it.csiro.au/sandbox/soil/scma/> .

s:3B1 a skos:Concept, sosa:Procedure;
  dct:description "Estimated soluble salt concentration"@en;
  dct:identifier "http://registry.it.csiro.au/sandbox/soil/scma/3B1"^^xsd:anyURI;
  dct:source "ISBN 9780643101364"@en;
  rdfs:label "Estimated soluble salt concentration"@en;
  skos:definition "Estimated soluble salt concentration"@en;
  skos:inScheme <http://registry.it.csiro.au/sandbox/soil/scma/>;
  skos:member s:3;
  skos:notation "3B1";
  skos:prefLabel "Estimated soluble salt concentration"@en;
  skos:topConceptOf <http://registry.it.csiro.au/sandbox/soil/scma/> .

s:3C1 a skos:Concept, sosa:Procedure;
  dct:description "Estimated soil ionic strength"@en;
  dct:identifier "http://registry.it.csiro.au/sandbox/soil/scma/3C1"^^xsd:anyURI;
  dct:source "ISBN 9780643101364"@en;
  rdfs:label "Estimated soil ionic strength"@en;
  skos:definition "Estimated soil ionic strength"@en;
  skos:inScheme <http://registry.it.csiro.au/sandbox/soil/scma/>;
  skos:member s:3;
  skos:notation "3C1";
  skos:prefLabel "Estimated soil ionic strength"@en;
  skos:topConceptOf <http://registry.it.csiro.au/sandbox/soil/scma/> .

s:3D1 a skos:Concept, sosa:Procedure;
  dct:description "Redox potential (Eh; field)"@en;
  dct:identifier "http://registry.it.csiro.au/sandbox/soil/scma/3D1"^^xsd:anyURI;
  dct:source "ISBN 9780643101364"@en;
  rdfs:label "Redox potential (Eh; field)"@en;
  skos:definition "Redox potential (Eh; field)"@en;
  skos:inScheme <http://registry.it.csiro.au/sandbox/soil/scma/>;
  skos:member s:3;
  skos:notation "3D1";
  skos:prefLabel "Redox potential (Eh; field)"@en;
  skos:topConceptOf <http://registry.it.csiro.au/sandbox/soil/scma/> .

s:4 a skos:Collection;
  dct:description "Soil pH"@en;
  dct:identifier "http://registry.it.csiro.au/sandbox/soil/scma/4"^^xsd:anyURI;
  dct:source "ISBN 0909605688"@en;
  ui:topMemberOf <http://registry.it.csiro.au/sandbox/soil/scma>;
  rdfs:label "Soil pH"@en;
  skos:definition "Soil pH"@en;
  skos:inScheme <http://registry.it.csiro.au/sandbox/soil/scma/>;
  skos:notation "4";
  skos:prefLabel "Soil pH"@en .

s:4F1 a skos:Concept, sosa:Procedure;
  dct:description "pH change"@en;
  dct:identifier "http://registry.it.csiro.au/sandbox/soil/scma/4F1"^^xsd:anyURI;
  dct:source "ISBN 9780643101364"@en;
  rdfs:label "pH change"@en;
  skos:definition "pH change"@en;
  skos:inScheme <http://registry.it.csiro.au/sandbox/soil/scma/>;
  skos:member s:4;
  skos:notation "4F1";
  skos:prefLabel "pH change"@en;
  skos:topConceptOf <http://registry.it.csiro.au/sandbox/soil/scma/> .

s:4B1 a skos:Concept, sosa:Procedure;
  dct:description "pH of 1:5 soil/0.01 M calcium chloride extract - direct (without stirring during measurement)"@en;
  dct:identifier "http://registry.it.csiro.au/sandbox/soil/scma/4B1"^^xsd:anyURI;
  dct:source "ISBN 9780643101364"@en;
  rdfs:label "pH of 1:5 soil/0.01 M calcium chloride extract - direct (without stirring during measurement)"@en;
  skos:definition "pH of 1:5 soil/0.01 M calcium chloride extract - direct (without stirring during measurement)"@en;
  skos:inScheme <http://registry.it.csiro.au/sandbox/soil/scma/>;
  skos:member s:4;
  skos:notation "4B1";
  skos:prefLabel "pH of 1:5 soil/0.01 M calcium chloride extract - direct (without stirring during measurement)"@en;
  skos:topConceptOf <http://registry.it.csiro.au/sandbox/soil/scma/> .

s:4A2 a skos:Concept, sosa:Procedure;
  dct:description "pH of a 1:1 soil/water suspension"@en;
  dct:identifier "http://registry.it.csiro.au/sandbox/soil/scma/4A2"^^xsd:anyURI;
  dct:source "ISBN 9780643101364"@en;
  rdfs:label "pH of a 1:1 soil/water suspension"@en;
  skos:definition "pH of a 1:1 soil/water suspension"@en;
  skos:inScheme <http://registry.it.csiro.au/sandbox/soil/scma/>;
  skos:member s:4;
  skos:notation "4A2";
  skos:prefLabel "pH of a 1:1 soil/water suspension"@en;
  skos:topConceptOf <http://registry.it.csiro.au/sandbox/soil/scma/> .

s:4C4 a skos:Concept, sosa:Procedure;
  dct:description "pH of 1:5 soil 1M potassium chloride extract - following method 4A1 (with stirring during measurement)"@en;
  dct:identifier "http://registry.it.csiro.au/sandbox/soil/scma/4C4"^^xsd:anyURI;
  dct:source "ISBN 9780643101364"@en;
  rdfs:label "pH of 1:5 soil 1M potassium chloride extract - following method 4A1 (with stirring during measurement)"@en;
  skos:definition "pH of 1:5 soil 1M potassium chloride extract - following method 4A1 (with stirring during measurement)"@en;
  skos:inScheme <http://registry.it.csiro.au/sandbox/soil/scma/>;
  skos:member s:4;
  skos:notation "4C4";
  skos:prefLabel "pH of 1:5 soil 1M potassium chloride extract - following method 4A1 (with stirring during measurement)"@en;
  skos:topConceptOf <http://registry.it.csiro.au/sandbox/soil/scma/> .

s:4D1 a skos:Concept, sosa:Procedure;
  dct:description "pH of sodium fluoride potential suspension and \\'reactivity class\\'"@en;
  dct:identifier "http://registry.it.csiro.au/sandbox/soil/scma/4D1"^^xsd:anyURI;
  dct:source "ISBN 9780643101364"@en;
  rdfs:label "pH of sodium fluoride potential suspension and \\'reactivity class\\'"@en;
  skos:definition "pH of sodium fluoride potential suspension and \\'reactivity class\\'"@en;
  skos:inScheme <http://registry.it.csiro.au/sandbox/soil/scma/>;
  skos:member s:4;
  skos:notation "4D1";
  skos:prefLabel "pH of sodium fluoride potential suspension and \\'reactivity class\\'"@en;
  skos:topConceptOf <http://registry.it.csiro.au/sandbox/soil/scma/> .

s:4A3 a skos:Concept, sosa:Procedure;
  dct:description "pH of a 1:2.5 soil/water suspension"@en;
  dct:identifier "http://registry.it.csiro.au/sandbox/soil/scma/4A3"^^xsd:anyURI;
  dct:source "ISBN 9780643101364"@en;
  rdfs:label "pH of a 1:2.5 soil/water suspension"@en;
  skos:definition "pH of a 1:2.5 soil/water suspension"@en;
  skos:inScheme <http://registry.it.csiro.au/sandbox/soil/scma/>;
  skos:member s:4;
  skos:notation "4A3";
  skos:prefLabel "pH of a 1:2.5 soil/water suspension"@en;
  skos:topConceptOf <http://registry.it.csiro.au/sandbox/soil/scma/> .

s:4C2 a skos:Concept, sosa:Procedure;
  dct:description "pH of 1:5 soil/1M potassium chloride extract following method 4A1 (without stirring during measurement)"@en;
  dct:identifier "http://registry.it.csiro.au/sandbox/soil/scma/4C2"^^xsd:anyURI;
  dct:source "ISBN 9780643101364"@en;
  rdfs:label "pH of 1:5 soil/1M potassium chloride extract following method 4A1 (without stirring during measurement)"@en;
  skos:definition "pH of 1:5 soil/1M potassium chloride extract following method 4A1 (without stirring during measurement)"@en;
  skos:inScheme <http://registry.it.csiro.au/sandbox/soil/scma/>;
  skos:member s:4;
  skos:notation "4C2";
  skos:prefLabel "pH of 1:5 soil/1M potassium chloride extract following method 4A1 (without stirring during measurement)"@en;
  skos:topConceptOf <http://registry.it.csiro.au/sandbox/soil/scma/> .

s:4A1 a skos:Concept, sosa:Procedure;
  dct:description "pH of a 1:5 soil/water suspension"@en;
  dct:identifier "http://registry.it.csiro.au/sandbox/soil/scma/4A1"^^xsd:anyURI;
  dct:source "ISBN 0909605688"@en;
  rdfs:label "pH of a 1:5 soil/water suspension"@en;
  skos:definition "pH of a 1:5 soil/water suspension"@en;
  skos:inScheme <http://registry.it.csiro.au/sandbox/soil/scma/>;
  skos:member s:4;
  skos:notation "4A1";
  skos:prefLabel "pH of a 1:5 soil/water suspension"@en;
  skos:topConceptOf <http://registry.it.csiro.au/sandbox/soil/scma/> .

s:4C3 a skos:Concept, sosa:Procedure;
  dct:description "pH of 1:5 soil/1M potassium chloride extract - direct (with stirring during measurement)"@en;
  dct:identifier "http://registry.it.csiro.au/sandbox/soil/scma/4C3"^^xsd:anyURI;
  dct:source "ISBN 9780643101364"@en;
  rdfs:label "pH of 1:5 soil/1M potassium chloride extract - direct (with stirring during measurement)"@en;
  skos:definition "pH of 1:5 soil/1M potassium chloride extract - direct (with stirring during measurement)"@en;
  skos:inScheme <http://registry.it.csiro.au/sandbox/soil/scma/>;
  skos:member s:4;
  skos:notation "4C3";
  skos:prefLabel "pH of 1:5 soil/1M potassium chloride extract - direct (with stirring during measurement)"@en;
  skos:topConceptOf <http://registry.it.csiro.au/sandbox/soil/scma/> .

s:4B4 a skos:Concept, sosa:Procedure;
  dct:description "pH of 1:5 soil/0.01 M calcium chloride extract - following method 4A1 (with stirring during measurement)"@en;
  dct:identifier "http://registry.it.csiro.au/sandbox/soil/scma/4B4"^^xsd:anyURI;
  dct:source "ISBN 9780643101364"@en;
  rdfs:label "pH of 1:5 soil/0.01 M calcium chloride extract - following method 4A1 (with stirring during measurement)"@en;
  skos:definition "pH of 1:5 soil/0.01 M calcium chloride extract - following method 4A1 (with stirring during measurement)"@en;
  skos:inScheme <http://registry.it.csiro.au/sandbox/soil/scma/>;
  skos:member s:4;
  skos:notation "4B4";
  skos:prefLabel "pH of 1:5 soil/0.01 M calcium chloride extract - following method 4A1 (with stirring during measurement)"@en;
  skos:topConceptOf <http://registry.it.csiro.au/sandbox/soil/scma/> .

s:4G1 a skos:Concept, sosa:Procedure;
  dct:description "Field determination of pH"@en;
  dct:identifier "http://registry.it.csiro.au/sandbox/soil/scma/4G1"^^xsd:anyURI;
  dct:source "ISBN 9780643101364"@en;
  rdfs:label "Field determination of pH"@en;
  skos:definition "Field determination of pH"@en;
  skos:inScheme <http://registry.it.csiro.au/sandbox/soil/scma/>;
  skos:member s:4;
  skos:notation "4G1";
  skos:prefLabel "Field determination of pH"@en;
  skos:topConceptOf <http://registry.it.csiro.au/sandbox/soil/scma/> .

s:4B5 a skos:Concept, sosa:Procedure;
  dct:description "pH of 1:5 soil/0.01 M calcium chloride extract equivalent, by MIR reflectance spectroscopy"@en;
  dct:identifier "http://registry.it.csiro.au/sandbox/soil/scma/4B5"^^xsd:anyURI;
  dct:source "ISBN 9780643101364"@en;
  rdfs:label "pH of 1:5 soil/0.01 M calcium chloride extract equivalent, by MIR reflectance spectroscopy"@en;
  skos:definition "pH of 1:5 soil/0.01 M calcium chloride extract equivalent, by MIR reflectance spectroscopy"@en;
  skos:inScheme <http://registry.it.csiro.au/sandbox/soil/scma/>;
  skos:member s:4;
  skos:notation "4B5";
  skos:prefLabel "pH of 1:5 soil/0.01 M calcium chloride extract equivalent, by MIR reflectance spectroscopy"@en;
  skos:topConceptOf <http://registry.it.csiro.au/sandbox/soil/scma/> .

s:4C1 a skos:Concept, sosa:Procedure;
  dct:description "pH of 1:5 soil/1M potassium chloride extract - direct (without stirring during measurement)"@en;
  dct:identifier "http://registry.it.csiro.au/sandbox/soil/scma/4C1"^^xsd:anyURI;
  dct:source "ISBN 9780643101364"@en;
  rdfs:label "pH of 1:5 soil/1M potassium chloride extract - direct (without stirring during measurement)"@en;
  skos:definition "pH of 1:5 soil/1M potassium chloride extract - direct (without stirring during measurement)"@en;
  skos:inScheme <http://registry.it.csiro.au/sandbox/soil/scma/>;
  skos:member s:4;
  skos:notation "4C1";
  skos:prefLabel "pH of 1:5 soil/1M potassium chloride extract - direct (without stirring during measurement)"@en;
  skos:topConceptOf <http://registry.it.csiro.au/sandbox/soil/scma/> .

s:4B2 a skos:Concept, sosa:Procedure;
  dct:description "pH of 1:5 soil/0.01 M calcium chloride extract - following method 4A1 (without stirring during measurement)"@en;
  dct:identifier "http://registry.it.csiro.au/sandbox/soil/scma/4B2"^^xsd:anyURI;
  dct:source "ISBN 9780643101364"@en;
  rdfs:label "pH of 1:5 soil/0.01 M calcium chloride extract - following method 4A1 (without stirring during measurement)"@en;
  skos:definition "pH of 1:5 soil/0.01 M calcium chloride extract - following method 4A1 (without stirring during measurement)"@en;
  skos:inScheme <http://registry.it.csiro.au/sandbox/soil/scma/>;
  skos:member s:4;
  skos:notation "4B2";
  skos:prefLabel "pH of 1:5 soil/0.01 M calcium chloride extract - following method 4A1 (without stirring during measurement)"@en;
  skos:topConceptOf <http://registry.it.csiro.au/sandbox/soil/scma/> .

s:4E1 a skos:Concept, sosa:Procedure;
  dct:description "pH of hydrogen peroxide extract"@en;
  dct:identifier "http://registry.it.csiro.au/sandbox/soil/scma/4E1"^^xsd:anyURI;
  dct:source "ISBN 9780643101364"@en;
  rdfs:label "pH of hydrogen peroxide extract"@en;
  skos:definition "pH of hydrogen peroxide extract"@en;
  skos:inScheme <http://registry.it.csiro.au/sandbox/soil/scma/>;
  skos:member s:4;
  skos:notation "4E1";
  skos:prefLabel "pH of hydrogen peroxide extract"@en;
  skos:topConceptOf <http://registry.it.csiro.au/sandbox/soil/scma/> .

s:4B3 a skos:Concept, sosa:Procedure;
  dct:description "pH of 1:5 soil/0.01 M calcium chloride extract -direct (without stirring during measurement)"@en;
  dct:identifier "http://registry.it.csiro.au/sandbox/soil/scma/4B3"^^xsd:anyURI;
  dct:source "ISBN 9780643101364"@en;
  rdfs:label "pH of 1:5 soil/0.01 M calcium chloride extract -direct (without stirring during measurement)"@en;
  skos:definition "pH of 1:5 soil/0.01 M calcium chloride extract -direct (without stirring during measurement)"@en;
  skos:inScheme <http://registry.it.csiro.au/sandbox/soil/scma/>;
  skos:member s:4;
  skos:notation "4B3";
  skos:prefLabel "pH of 1:5 soil/0.01 M calcium chloride extract -direct (without stirring during measurement)"@en;
  skos:topConceptOf <http://registry.it.csiro.au/sandbox/soil/scma/> .

s:5 a skos:Collection;
  dct:description "Soluble chloride"@en;
  dct:identifier "http://registry.it.csiro.au/sandbox/soil/scma/5"^^xsd:anyURI;
  dct:source "ISBN 9780643101364"@en;
  ui:topMemberOf <http://registry.it.csiro.au/sandbox/soil/scma>;
  rdfs:label "Soluble chloride"@en;
  skos:definition "Soluble chloride"@en;
  skos:inScheme <http://registry.it.csiro.au/sandbox/soil/scma/>;
  skos:notation "5";
  skos:prefLabel "Soluble chloride"@en .

s:5A1 a skos:Concept, sosa:Procedure;
  dct:description "Chloride - 1:5 soil/water extract, potentiometric titration"@en;
  dct:identifier "http://registry.it.csiro.au/sandbox/soil/scma/5A1"^^xsd:anyURI;
  dct:source "ISBN 9780643101364"@en;
  rdfs:label "Chloride - 1:5 soil/water extract, potentiometric titration"@en;
  skos:definition "Chloride - 1:5 soil/water extract, potentiometric titration"@en;
  skos:inScheme <http://registry.it.csiro.au/sandbox/soil/scma/>;
  skos:member s:5;
  skos:notation "5A1";
  skos:prefLabel "Chloride - 1:5 soil/water extract, potentiometric titration"@en;
  skos:topConceptOf <http://registry.it.csiro.au/sandbox/soil/scma/> .

s:5A2 a skos:Concept, sosa:Procedure;
  dct:description "Chloride - 1:5 soil/water extract, automated colour"@en;
  dct:identifier "http://registry.it.csiro.au/sandbox/soil/scma/5A2"^^xsd:anyURI;
  dct:source "ISBN 0909605688"@en;
  rdfs:label "Chloride - 1:5 soil/water extract, automated colour"@en;
  skos:definition "Chloride - 1:5 soil/water extract, automated colour"@en;
  skos:inScheme <http://registry.it.csiro.au/sandbox/soil/scma/>;
  skos:member s:5;
  skos:narrower s:5A2a, s:5A2b;
  skos:notation "5A2";
  skos:note "5A2 has been superseded by 5A2a and 5A2b in Soil Chemical Methods Australasia, Rayment G.E. and Lyons D.J. ISBN 9780643101364"@en;
  skos:prefLabel "Chloride - 1:5 soil/water extract, automated colour"@en;
  skos:topConceptOf <http://registry.it.csiro.au/sandbox/soil/scma/> .

s:5A4 a skos:Concept, sosa:Procedure;
  dct:description "Chloride - 1:5 soil/water extract ICPAES"@en;
  dct:identifier "http://registry.it.csiro.au/sandbox/soil/scma/5A4"^^xsd:anyURI;
  dct:source "ISBN 9780643101364"@en;
  rdfs:label "Chloride - 1:5 soil/water extract ICPAES"@en;
  skos:definition "Chloride - 1:5 soil/water extract ICPAES"@en;
  skos:inScheme <http://registry.it.csiro.au/sandbox/soil/scma/>;
  skos:member s:5;
  skos:notation "5A4";
  skos:prefLabel "Chloride - 1:5 soil/water extract ICPAES"@en;
  skos:topConceptOf <http://registry.it.csiro.au/sandbox/soil/scma/> .

s:5A3b a skos:Concept, sosa:Procedure;
  dct:description "Chloride - 1:5 soil/water extract, ion chromatography (single-column with electronic suppression of eluent conductivity)"@en;
  dct:identifier "http://registry.it.csiro.au/sandbox/soil/scma/5A3b"^^xsd:anyURI;
  dct:source "ISBN 9780643101364"@en;
  rdfs:label "Chloride - 1:5 soil/water extract, ion chromatography (single-column with electronic suppression of eluent conductivity)"@en;
  skos:definition "Chloride - 1:5 soil/water extract, ion chromatography (single-column with electronic suppression of eluent conductivity)"@en;
  skos:inScheme <http://registry.it.csiro.au/sandbox/soil/scma/>;
  skos:member s:5;
  skos:notation "5A3b";
  skos:prefLabel "Chloride - 1:5 soil/water extract, ion chromatography (single-column with electronic suppression of eluent conductivity)"@en;
  skos:topConceptOf <http://registry.it.csiro.au/sandbox/soil/scma/> .

s:5A3a a skos:Concept, sosa:Procedure;
  dct:description "Chloride - 1:5 soil/water extract, ion chromatography (chemical suppression of eluent conductivity)"@en;
  dct:identifier "http://registry.it.csiro.au/sandbox/soil/scma/5A3a"^^xsd:anyURI;
  dct:source "ISBN 9780643101364"@en;
  rdfs:label "Chloride - 1:5 soil/water extract, ion chromatography (chemical suppression of eluent conductivity)"@en;
  skos:definition "Chloride - 1:5 soil/water extract, ion chromatography (chemical suppression of eluent conductivity)"@en;
  skos:inScheme <http://registry.it.csiro.au/sandbox/soil/scma/>;
  skos:member s:5;
  skos:notation "5A3a";
  skos:prefLabel "Chloride - 1:5 soil/water extract, ion chromatography (chemical suppression of eluent conductivity)"@en;
  skos:topConceptOf <http://registry.it.csiro.au/sandbox/soil/scma/> .

s:5A2a a skos:Concept, sosa:Procedure;
  dct:description "Chloride - 1:5 soil/water extract, automated colour"@en;
  dct:identifier "http://registry.it.csiro.au/sandbox/soil/scma/5A2a"^^xsd:anyURI;
  dct:source "ISBN 9780643101364"@en;
  rdfs:label "Chloride - 1:5 soil/water extract, automated colour"@en;
  skos:broader s:5A2;
  skos:definition "Chloride - 1:5 soil/water extract, automated colour"@en;
  skos:inScheme <http://registry.it.csiro.au/sandbox/soil/scma/>;
  skos:notation "5A2a";
  skos:prefLabel "Chloride - 1:5 soil/water extract, automated colour"@en .

s:5A2b a skos:Concept, sosa:Procedure;
  dct:description "Chloride - 1:5 soil/water extract, FIA"@en;
  dct:identifier "http://registry.it.csiro.au/sandbox/soil/scma/5A2b"^^xsd:anyURI;
  dct:source "ISBN 9780643101364"@en;
  rdfs:label "Chloride - 1:5 soil/water extract, FIA"@en;
  skos:broader s:5A2;
  skos:definition "Chloride - 1:5 soil/water extract, FIA"@en;
  skos:inScheme <http://registry.it.csiro.au/sandbox/soil/scma/>;
  skos:notation "5A2b";
  skos:prefLabel "Chloride - 1:5 soil/water extract, FIA"@en .

s:6 a skos:Collection;
  dct:description "Carbon"@en;
  dct:identifier "http://registry.it.csiro.au/sandbox/soil/scma/6"^^xsd:anyURI;
  dct:source "ISBN 9780643101364"@en;
  ui:topMemberOf <http://registry.it.csiro.au/sandbox/soil/scma>;
  rdfs:label "Carbon"@en;
  skos:definition "Carbon"@en;
  skos:inScheme <http://registry.it.csiro.au/sandbox/soil/scma/>;
  skos:notation "6";
  skos:prefLabel "Carbon"@en .

s:6G1 a skos:Concept, sosa:Procedure;
  dct:description "Total organic matter, organic C, and carbonate by loss-on-ignition"@en;
  dct:identifier "http://registry.it.csiro.au/sandbox/soil/scma/6G1"^^xsd:anyURI;
  dct:source "ISBN 9780643101364"@en;
  rdfs:label "Total organic matter, organic C, and carbonate by loss-on-ignition"@en;
  skos:definition "Total organic matter, organic C, and carbonate by loss-on-ignition"@en;
  skos:inScheme <http://registry.it.csiro.au/sandbox/soil/scma/>;
  skos:member s:6;
  skos:notation "6G1";
  skos:prefLabel "Total organic matter, organic C, and carbonate by loss-on-ignition"@en;
  skos:topConceptOf <http://registry.it.csiro.au/sandbox/soil/scma/> .

s:6B3 a skos:Concept, sosa:Procedure;
  dct:description "Total organic C - Dumas high-temperature combustion, infrared/thermal conductivity detection (with prior physical removal of charcoal and chemical removal of carbonates)"@en;
  dct:identifier "http://registry.it.csiro.au/sandbox/soil/scma/6B3"^^xsd:anyURI;
  dct:source "ISBN 9780643101364"@en;
  rdfs:label "Total organic C - Dumas high-temperature combustion, infrared/thermal conductivity detection (with prior physical removal of charcoal and chemical removal of carbonates)"@en;
  skos:definition "Total organic C - Dumas high-temperature combustion, infrared/thermal conductivity detection (with prior physical removal of charcoal and chemical removal of carbonates)"@en;
  skos:inScheme <http://registry.it.csiro.au/sandbox/soil/scma/>;
  skos:member s:6;
  skos:notation "6B3";
  skos:prefLabel "Total organic C - Dumas high-temperature combustion, infrared/thermal conductivity detection (with prior physical removal of charcoal and chemical removal of carbonates)"@en;
  skos:topConceptOf <http://registry.it.csiro.au/sandbox/soil/scma/> .

s:6B4 a skos:Concept, sosa:Procedure;
  dct:description "Total organic C - infrared diffuse reflectance spectroscopy"@en;
  dct:identifier "http://registry.it.csiro.au/sandbox/soil/scma/6B4"^^xsd:anyURI;
  dct:source "ISBN 9780643101364"@en;
  rdfs:label "Total organic C - infrared diffuse reflectance spectroscopy"@en;
  skos:definition "Total organic C - infrared diffuse reflectance spectroscopy"@en;
  skos:inScheme <http://registry.it.csiro.au/sandbox/soil/scma/>;
  skos:member s:6;
  skos:narrower s:6B4a, s:6B4b;
  skos:notation "6B4";
  skos:prefLabel "Total organic C - infrared diffuse reflectance spectroscopy"@en;
  skos:topConceptOf <http://registry.it.csiro.au/sandbox/soil/scma/> .

s:6B2 a skos:Concept, sosa:Procedure;
  dct:description "Total organic C - Dumas high-temperature combustion"@en;
  dct:identifier "http://registry.it.csiro.au/sandbox/soil/scma/6B2"^^xsd:anyURI;
  dct:source "ISBN 9780643101364"@en;
  rdfs:label "Total organic C - Dumas high-temperature combustion"@en;
  skos:definition "Total organic C - Dumas high-temperature combustion"@en;
  skos:inScheme <http://registry.it.csiro.au/sandbox/soil/scma/>;
  skos:member s:6;
  skos:narrower s:6B2a, s:6B2b;
  skos:notation "6B2";
  skos:prefLabel "Total organic C - Dumas high-temperature combustion"@en;
  skos:topConceptOf <http://registry.it.csiro.au/sandbox/soil/scma/> .

s:6B1 a skos:Concept, sosa:Procedure;
  dct:description "Total organic C - Heanes wet oxidisation"@en;
  dct:identifier "http://registry.it.csiro.au/sandbox/soil/scma/6B1"^^xsd:anyURI;
  dct:source "ISBN 9780643101364"@en;
  rdfs:label "Total organic C - Heanes wet oxidisation"@en;
  skos:definition "Total organic C - Heanes wet oxidisation"@en;
  skos:inScheme <http://registry.it.csiro.au/sandbox/soil/scma/>;
  skos:member s:6;
  skos:notation "6B1";
  skos:prefLabel "Total organic C - Heanes wet oxidisation"@en;
  skos:topConceptOf <http://registry.it.csiro.au/sandbox/soil/scma/> .

s:6A1 a skos:Concept, sosa:Procedure;
  dct:description "Organic C - W&B"@en;
  dct:identifier "http://registry.it.csiro.au/sandbox/soil/scma/6A1"^^xsd:anyURI;
  dct:source "ISBN 9780643101364"@en;
  rdfs:label "Organic C - W&B"@en;
  skos:definition "Organic C - W&B"@en;
  skos:inScheme <http://registry.it.csiro.au/sandbox/soil/scma/>;
  skos:member s:6;
  skos:notation "6A1";
  skos:prefLabel "Organic C - W&B"@en;
  skos:topConceptOf <http://registry.it.csiro.au/sandbox/soil/scma/> .

s:6C1 a skos:Concept, sosa:Procedure;
  dct:description "Particulate organic C (POC)"@en;
  dct:identifier "http://registry.it.csiro.au/sandbox/soil/scma/6C1"^^xsd:anyURI;
  dct:source "ISBN 9780643101364"@en;
  rdfs:label "Particulate organic C (POC)"@en;
  skos:definition "Particulate organic C (POC)"@en;
  skos:inScheme <http://registry.it.csiro.au/sandbox/soil/scma/>;
  skos:member s:6;
  skos:notation "6C1";
  skos:prefLabel "Particulate organic C (POC)"@en;
  skos:topConceptOf <http://registry.it.csiro.au/sandbox/soil/scma/> .

s:6D1 a skos:Concept, sosa:Procedure;
  dct:description "Pyrophosphate-extractable C"@en;
  dct:identifier "http://registry.it.csiro.au/sandbox/soil/scma/6D1"^^xsd:anyURI;
  dct:source "ISBN 9780643101364"@en;
  rdfs:label "Pyrophosphate-extractable C"@en;
  skos:definition "Pyrophosphate-extractable C"@en;
  skos:inScheme <http://registry.it.csiro.au/sandbox/soil/scma/>;
  skos:member s:6;
  skos:notation "6D1";
  skos:prefLabel "Pyrophosphate-extractable C"@en;
  skos:topConceptOf <http://registry.it.csiro.au/sandbox/soil/scma/> .

s:6F1 a skos:Concept, sosa:Procedure;
  dct:description "Charcoal-C"@en;
  dct:identifier "http://registry.it.csiro.au/sandbox/soil/scma/6F1"^^xsd:anyURI;
  dct:source "ISBN 9780643101364"@en;
  rdfs:label "Charcoal-C"@en;
  skos:definition "Charcoal-C"@en;
  skos:inScheme <http://registry.it.csiro.au/sandbox/soil/scma/>;
  skos:member s:6;
  skos:notation "6F1";
  skos:prefLabel "Charcoal-C"@en;
  skos:topConceptOf <http://registry.it.csiro.au/sandbox/soil/scma/> .

s:6E1 a skos:Concept, sosa:Procedure;
  dct:description "Potassium permanganate oxidisable C (PPOC)"@en;
  dct:identifier "http://registry.it.csiro.au/sandbox/soil/scma/6E1"^^xsd:anyURI;
  dct:source "ISBN 9780643101364"@en;
  rdfs:label "Potassium permanganate oxidisable C (PPOC)"@en;
  skos:definition "Potassium permanganate oxidisable C (PPOC)"@en;
  skos:inScheme <http://registry.it.csiro.au/sandbox/soil/scma/>;
  skos:member s:6;
  skos:notation "6E1";
  skos:prefLabel "Potassium permanganate oxidisable C (PPOC)"@en;
  skos:topConceptOf <http://registry.it.csiro.au/sandbox/soil/scma/> .

s:6B2a a skos:Concept, sosa:Procedure;
  dct:description "Total organic C - Dumas high-temperature combustion, volumetric (no soil pretreatment)"@en;
  dct:identifier "http://registry.it.csiro.au/sandbox/soil/scma/6B2a"^^xsd:anyURI;
  dct:source "ISBN 9780643101364"@en;
  rdfs:label "Total organic C - Dumas high-temperature combustion, volumetric (no soil pretreatment)"@en;
  skos:broader s:6B2;
  skos:definition "Total organic C - Dumas high-temperature combustion, volumetric (no soil pretreatment)"@en;
  skos:inScheme <http://registry.it.csiro.au/sandbox/soil/scma/>;
  skos:notation "6B2a";
  skos:prefLabel "Total organic C - Dumas high-temperature combustion, volumetric (no soil pretreatment)"@en .

s:6B2b a skos:Concept, sosa:Procedure;
  dct:description "Total organic C - Dumas high-temperature combustion, infrared/thermal conductivity detection (no soil pretreatment)"@en;
  dct:identifier "http://registry.it.csiro.au/sandbox/soil/scma/6B2b"^^xsd:anyURI;
  dct:source "ISBN 9780643101364"@en;
  rdfs:label "Total organic C - Dumas high-temperature combustion, infrared/thermal conductivity detection (no soil pretreatment)"@en;
  skos:broader s:6B2;
  skos:definition "Total organic C - Dumas high-temperature combustion, infrared/thermal conductivity detection (no soil pretreatment)"@en;
  skos:inScheme <http://registry.it.csiro.au/sandbox/soil/scma/>;
  skos:notation "6B2b";
  skos:prefLabel "Total organic C - Dumas high-temperature combustion, infrared/thermal conductivity detection (no soil pretreatment)"@en .

s:6B4a a skos:Concept, sosa:Procedure;
  dct:description "Total organic C - NIR reflectance spectroscopy"@en;
  dct:identifier "http://registry.it.csiro.au/sandbox/soil/scma/6B4a"^^xsd:anyURI;
  dct:source "ISBN 9780643101364"@en;
  rdfs:label "Total organic C - NIR reflectance spectroscopy"@en;
  skos:broader s:6B4;
  skos:definition "Total organic C - NIR reflectance spectroscopy"@en;
  skos:inScheme <http://registry.it.csiro.au/sandbox/soil/scma/>;
  skos:notation "6B4a";
  skos:prefLabel "Total organic C - NIR reflectance spectroscopy"@en .

s:6B4b a skos:Concept, sosa:Procedure;
  dct:description "Total organic C - MIR reflectance spectroscopy"@en;
  dct:identifier "http://registry.it.csiro.au/sandbox/soil/scma/6B4b"^^xsd:anyURI;
  dct:source "ISBN 9780643101364"@en;
  rdfs:label "Total organic C - MIR reflectance spectroscopy"@en;
  skos:broader s:6B4;
  skos:definition "Total organic C - MIR reflectance spectroscopy"@en;
  skos:inScheme <http://registry.it.csiro.au/sandbox/soil/scma/>;
  skos:notation "6B4b";
  skos:prefLabel "Total organic C - MIR reflectance spectroscopy"@en .

s:7 a skos:Collection;
  dct:description "Nitrogen"@en;
  dct:identifier "http://registry.it.csiro.au/sandbox/soil/scma/7"^^xsd:anyURI;
  dct:source "ISBN 9780643101364"@en;
  ui:topMemberOf <http://registry.it.csiro.au/sandbox/soil/scma>;
  rdfs:label "Nitrogen"@en;
  skos:definition "Nitrogen"@en;
  skos:inScheme <http://registry.it.csiro.au/sandbox/soil/scma/>;
  skos:notation "7";
  skos:prefLabel "Nitrogen"@en .

s:7A2 a skos:Concept, sosa:Procedure;
  dct:description "Total soil-N, semi micro Kjeldahl - automated colour|Total nitrogen - semimicro Kjeldahl, automated colour"@en;
  dct:identifier "http://registry.it.csiro.au/sandbox/soil/scma/7A2"^^xsd:anyURI;
  dct:source "ISBN 0909605688"@en;
  rdfs:label "Total soil-N, semi micro Kjeldahl - automated colour|Total nitrogen - semimicro Kjeldahl, automated colour"@en;
  skos:definition "Total soil-N, semi micro Kjeldahl - automated colour|Total nitrogen - semimicro Kjeldahl, automated colour"@en;
  skos:inScheme <http://registry.it.csiro.au/sandbox/soil/scma/>;
  skos:member s:7;
  skos:narrower s:7A2a, s:7A2b;
  skos:notation "7A2";
  skos:note "7A2 has been superseded by 7A2a and 7A2b in Soil Chemical Methods Australasia, Rayment G.E. and Lyons D.J. ISBN 9780643101364"@en;
  skos:prefLabel "Total soil-N, semi micro Kjeldahl - automated colour|Total nitrogen - semimicro Kjeldahl, automated colour"@en;
  skos:topConceptOf <http://registry.it.csiro.au/sandbox/soil/scma/> .

s:7C2 a skos:Concept, sosa:Procedure;
  dct:description "Mineral-N 2 M KCl, automated colour|mineral nitrogen with 2M KCl - automated colour"@en;
  dct:identifier "http://registry.it.csiro.au/sandbox/soil/scma/7C2"^^xsd:anyURI;
  dct:source "ISBN 0909605688"@en;
  rdfs:label "Mineral-N 2 M KCl, automated colour|mineral nitrogen with 2M KCl - automated colour"@en;
  skos:definition "Mineral-N 2 M KCl, automated colour|mineral nitrogen with 2M KCl - automated colour"@en;
  skos:inScheme <http://registry.it.csiro.au/sandbox/soil/scma/>;
  skos:member s:7;
  skos:narrower s:7C2a, s:7C2b;
  skos:notation "7C2";
  skos:note "7C2 has been superseded by 7C2a and 7C2b in Soil Chemical Methods Australasia, Rayment G.E. and Lyons D.J. ISBN 9780643101364"@en;
  skos:prefLabel "Mineral-N 2 M KCl, automated colour|mineral nitrogen with 2M KCl - automated colour"@en;
  skos:topConceptOf <http://registry.it.csiro.au/sandbox/soil/scma/> .

s:7A5 a skos:Concept, sosa:Procedure;
  dct:description "Total soil-N - Dumas high-temperature combustion"@en;
  dct:identifier "http://registry.it.csiro.au/sandbox/soil/scma/7A5"^^xsd:anyURI;
  dct:source "ISBN 9780643101364"@en;
  rdfs:label "Total soil-N - Dumas high-temperature combustion"@en;
  skos:definition "Total soil-N - Dumas high-temperature combustion"@en;
  skos:inScheme <http://registry.it.csiro.au/sandbox/soil/scma/>;
  skos:member s:7;
  skos:notation "7A5";
  skos:prefLabel "Total soil-N - Dumas high-temperature combustion"@en;
  skos:topConceptOf <http://registry.it.csiro.au/sandbox/soil/scma/> .

s:7B a skos:Concept, sosa:Procedure;
  dct:description "Water-soluble nitrate-N"@en;
  dct:identifier "http://registry.it.csiro.au/sandbox/soil/scma/7B"^^xsd:anyURI;
  dct:source "ISBN 9780643101364"@en;
  rdfs:label "Water-soluble nitrate-N"@en;
  skos:definition "Water-soluble nitrate-N"@en;
  skos:inScheme <http://registry.it.csiro.au/sandbox/soil/scma/>;
  skos:member s:7;
  skos:narrower s:7B1, s:7B1a, s:7B1b, s:7B2;
  skos:notation "7B";
  skos:prefLabel "Water-soluble nitrate-N"@en;
  skos:topConceptOf <http://registry.it.csiro.au/sandbox/soil/scma/> .

s:7A4 a skos:Concept, sosa:Procedure;
  dct:description "Total-N (where nitrate >20 mg N/kg) - automated colour, continuous segmented flow/FIA"@en;
  dct:identifier "http://registry.it.csiro.au/sandbox/soil/scma/7A4"^^xsd:anyURI;
  dct:source "ISBN 9780643101364"@en;
  rdfs:label "Total-N (where nitrate >20 mg N/kg) - automated colour, continuous segmented flow/FIA"@en;
  skos:definition "Total-N (where nitrate >20 mg N/kg) - automated colour, continuous segmented flow/FIA"@en;
  skos:inScheme <http://registry.it.csiro.au/sandbox/soil/scma/>;
  skos:member s:7;
  skos:notation "7A4";
  skos:prefLabel "Total-N (where nitrate >20 mg N/kg) - automated colour, continuous segmented flow/FIA"@en;
  skos:topConceptOf <http://registry.it.csiro.au/sandbox/soil/scma/> .

s:7A1 a skos:Concept, sosa:Procedure;
  dct:description "Total soil-N, semi micro Kjeldahl - steam distillation"@en;
  dct:identifier "http://registry.it.csiro.au/sandbox/soil/scma/7A1"^^xsd:anyURI;
  dct:source "ISBN 9780643101364"@en;
  rdfs:label "Total soil-N, semi micro Kjeldahl - steam distillation"@en;
  skos:definition "Total soil-N, semi micro Kjeldahl - steam distillation"@en;
  skos:inScheme <http://registry.it.csiro.au/sandbox/soil/scma/>;
  skos:member s:7;
  skos:notation "7A1";
  skos:prefLabel "Total soil-N, semi micro Kjeldahl - steam distillation"@en;
  skos:topConceptOf <http://registry.it.csiro.au/sandbox/soil/scma/> .

s:7D a skos:Concept, sosa:Procedure;
  dct:description "Potentially mineralisable N (PMN)"@en;
  dct:identifier "http://registry.it.csiro.au/sandbox/soil/scma/7D"^^xsd:anyURI;
  dct:source "ISBN 9780643101364"@en;
  rdfs:label "Potentially mineralisable N (PMN)"@en;
  skos:definition "Potentially mineralisable N (PMN)"@en;
  skos:inScheme <http://registry.it.csiro.au/sandbox/soil/scma/>;
  skos:member s:7;
  skos:narrower s:7D1a, s:7D1b, s:7D1c, s:7D2a, s:7D2b;
  skos:notation "7D";
  skos:prefLabel "Potentially mineralisable N (PMN)"@en;
  skos:topConceptOf <http://registry.it.csiro.au/sandbox/soil/scma/> .

s:7A6 a skos:Concept, sosa:Procedure;
  dct:description "Total soil-N - infrared diffuse reflectance spectroscopy"@en;
  dct:identifier "http://registry.it.csiro.au/sandbox/soil/scma/7A6"^^xsd:anyURI;
  dct:source "ISBN 9780643101364"@en;
  rdfs:label "Total soil-N - infrared diffuse reflectance spectroscopy"@en;
  skos:definition "Total soil-N - infrared diffuse reflectance spectroscopy"@en;
  skos:inScheme <http://registry.it.csiro.au/sandbox/soil/scma/>;
  skos:member s:7;
  skos:narrower s:7A6a, s:7A6b;
  skos:notation "7A6";
  skos:prefLabel "Total soil-N - infrared diffuse reflectance spectroscopy"@en;
  skos:topConceptOf <http://registry.it.csiro.au/sandbox/soil/scma/> .

s:7C1 a skos:Concept, sosa:Procedure;
  dct:description "Mineral-N 2 M KCl, steam distillation"@en;
  dct:identifier "http://registry.it.csiro.au/sandbox/soil/scma/7C1"^^xsd:anyURI;
  dct:source "ISBN 9780643101364"@en;
  rdfs:label "Mineral-N 2 M KCl, steam distillation"@en;
  skos:definition "Mineral-N 2 M KCl, steam distillation"@en;
  skos:inScheme <http://registry.it.csiro.au/sandbox/soil/scma/>;
  skos:member s:7;
  skos:narrower s:7C1a, s:7C1b, s:7C1c, s:7C1d, s:7C1e, s:7C1f, s:7C1g, s:7C1h;
  skos:notation "7C1";
  skos:prefLabel "Mineral-N 2 M KCl, steam distillation"@en;
  skos:topConceptOf <http://registry.it.csiro.au/sandbox/soil/scma/> .

s:7A3 a skos:Concept, sosa:Procedure;
  dct:description "Total soil-N (where nitrate >20 mg N/kg) - steam distillation"@en;
  dct:identifier "http://registry.it.csiro.au/sandbox/soil/scma/7A3"^^xsd:anyURI;
  dct:source "ISBN 9780643101364"@en;
  rdfs:label "Total soil-N (where nitrate >20 mg N/kg) - steam distillation"@en;
  skos:definition "Total soil-N (where nitrate >20 mg N/kg) - steam distillation"@en;
  skos:inScheme <http://registry.it.csiro.au/sandbox/soil/scma/>;
  skos:member s:7;
  skos:notation "7A3";
  skos:prefLabel "Total soil-N (where nitrate >20 mg N/kg) - steam distillation"@en;
  skos:topConceptOf <http://registry.it.csiro.au/sandbox/soil/scma/> .

s:7A2a a skos:Concept, sosa:Procedure;
  dct:description "Total soil-N, semi micro Kjeldahl - automated colour, continuous segmented flow"@en;
  dct:identifier "http://registry.it.csiro.au/sandbox/soil/scma/7A2a"^^xsd:anyURI;
  dct:source "ISBN 9780643101364"@en;
  rdfs:label "Total soil-N, semi micro Kjeldahl - automated colour, continuous segmented flow"@en;
  skos:broader s:7A2;
  skos:definition "Total soil-N, semi micro Kjeldahl - automated colour, continuous segmented flow"@en;
  skos:inScheme <http://registry.it.csiro.au/sandbox/soil/scma/>;
  skos:notation "7A2a";
  skos:prefLabel "Total soil-N, semi micro Kjeldahl - automated colour, continuous segmented flow"@en .

s:7A2b a skos:Concept, sosa:Procedure;
  dct:description "Total soil-N, semi micro Kjeldahl - automated colour - FIA"@en;
  dct:identifier "http://registry.it.csiro.au/sandbox/soil/scma/7A2b"^^xsd:anyURI;
  dct:source "ISBN 9780643101364"@en;
  rdfs:label "Total soil-N, semi micro Kjeldahl - automated colour - FIA"@en;
  skos:broader s:7A2;
  skos:definition "Total soil-N, semi micro Kjeldahl - automated colour - FIA"@en;
  skos:inScheme <http://registry.it.csiro.au/sandbox/soil/scma/>;
  skos:notation "7A2b";
  skos:prefLabel "Total soil-N, semi micro Kjeldahl - automated colour - FIA"@en .

s:7A6a a skos:Concept, sosa:Procedure;
  dct:description "Total Soil-N - NIR diffuse reflectance spectroscopy"@en;
  dct:identifier "http://registry.it.csiro.au/sandbox/soil/scma/7A6a"^^xsd:anyURI;
  dct:source "ISBN 9780643101364"@en;
  rdfs:label "Total Soil-N - NIR diffuse reflectance spectroscopy"@en;
  skos:broader s:7A6;
  skos:definition "Total Soil-N - NIR diffuse reflectance spectroscopy"@en;
  skos:inScheme <http://registry.it.csiro.au/sandbox/soil/scma/>;
  skos:notation "7A6a";
  skos:prefLabel "Total Soil-N - NIR diffuse reflectance spectroscopy"@en .

s:7A6b a skos:Concept, sosa:Procedure;
  dct:description "Total soil-N - MIR diffuse reflectance spectroscopy"@en;
  dct:identifier "http://registry.it.csiro.au/sandbox/soil/scma/7A6b"^^xsd:anyURI;
  dct:source "ISBN 9780643101364"@en;
  rdfs:label "Total soil-N - MIR diffuse reflectance spectroscopy"@en;
  skos:broader s:7A6;
  skos:definition "Total soil-N - MIR diffuse reflectance spectroscopy"@en;
  skos:inScheme <http://registry.it.csiro.au/sandbox/soil/scma/>;
  skos:notation "7A6b";
  skos:prefLabel "Total soil-N - MIR diffuse reflectance spectroscopy"@en .

s:7B1 a skos:Concept, sosa:Procedure;
  dct:description "Water-soluble nitrate-N - automated colour|Water soluble nitrate - automated colour"@en;
  dct:identifier "http://registry.it.csiro.au/sandbox/soil/scma/7B1"^^xsd:anyURI;
  dct:source "ISBN 0909605688"@en;
  rdfs:label "Water-soluble nitrate-N - automated colour|Water soluble nitrate - automated colour"@en;
  skos:broader s:7B;
  skos:definition "Water-soluble nitrate-N - automated colour|Water soluble nitrate - automated colour"@en;
  skos:inScheme <http://registry.it.csiro.au/sandbox/soil/scma/>;
  skos:narrower s:7B1a, s:7B1b;
  skos:notation "7B1";
  skos:note "7B1 has been superseded by 7B1a and 7B1b in Soil Chemical Methods Australasia, Rayment G.E. and Lyons D.J. ISBN 9780643101364"@en;
  skos:prefLabel "Water-soluble nitrate-N - automated colour|Water soluble nitrate - automated colour"@en .

s:7B1a a skos:Concept, sosa:Procedure;
  dct:description "Water-soluble nitrate-N - automated colour, continuous segmented flow"@en;
  dct:identifier "http://registry.it.csiro.au/sandbox/soil/scma/7B1a"^^xsd:anyURI;
  dct:source "ISBN 9780643101364"@en;
  rdfs:label "Water-soluble nitrate-N - automated colour, continuous segmented flow"@en;
  skos:broader s:7B, s:7B1;
  skos:definition "Water-soluble nitrate-N - automated colour, continuous segmented flow"@en;
  skos:inScheme <http://registry.it.csiro.au/sandbox/soil/scma/>;
  skos:notation "7B1a";
  skos:prefLabel "Water-soluble nitrate-N - automated colour, continuous segmented flow"@en .

s:7B1b a skos:Concept, sosa:Procedure;
  dct:description "Water-soluble nitrate-N - automated colour, FIA"@en;
  dct:identifier "http://registry.it.csiro.au/sandbox/soil/scma/7B1b"^^xsd:anyURI;
  dct:source "ISBN 9780643101364"@en;
  rdfs:label "Water-soluble nitrate-N - automated colour, FIA"@en;
  skos:broader s:7B, s:7B1;
  skos:definition "Water-soluble nitrate-N - automated colour, FIA"@en;
  skos:inScheme <http://registry.it.csiro.au/sandbox/soil/scma/>;
  skos:notation "7B1b";
  skos:prefLabel "Water-soluble nitrate-N - automated colour, FIA"@en .

s:7B2 a skos:Concept, sosa:Procedure;
  dct:description "Water-soluble nitrate-N - ion chromatography"@en;
  dct:identifier "http://registry.it.csiro.au/sandbox/soil/scma/7B2"^^xsd:anyURI;
  dct:source "ISBN 9780643101364"@en;
  rdfs:label "Water-soluble nitrate-N - ion chromatography"@en;
  skos:broader s:7B;
  skos:definition "Water-soluble nitrate-N - ion chromatography"@en;
  skos:inScheme <http://registry.it.csiro.au/sandbox/soil/scma/>;
  skos:notation "7B2";
  skos:prefLabel "Water-soluble nitrate-N - ion chromatography"@en .

s:7C1a a skos:Concept, sosa:Procedure;
  dct:description "Ammonium-N (in presence or absence of nitrite) - steam distillation"@en;
  dct:identifier "http://registry.it.csiro.au/sandbox/soil/scma/7C1a"^^xsd:anyURI;
  dct:source "ISBN 9780643101364"@en;
  rdfs:label "Ammonium-N (in presence or absence of nitrite) - steam distillation"@en;
  skos:broader s:7C1;
  skos:definition "Ammonium-N (in presence or absence of nitrite) - steam distillation"@en;
  skos:inScheme <http://registry.it.csiro.au/sandbox/soil/scma/>;
  skos:notation "7C1a";
  skos:prefLabel "Ammonium-N (in presence or absence of nitrite) - steam distillation"@en .

s:7C1b a skos:Concept, sosa:Procedure;
  dct:description "(Nitrate + Nitrite)-N - steam distillation"@en;
  dct:identifier "http://registry.it.csiro.au/sandbox/soil/scma/7C1b"^^xsd:anyURI;
  dct:source "ISBN 9780643101364"@en;
  rdfs:label "(Nitrate + Nitrite)-N - steam distillation"@en;
  skos:broader s:7C1;
  skos:definition "(Nitrate + Nitrite)-N - steam distillation"@en;
  skos:inScheme <http://registry.it.csiro.au/sandbox/soil/scma/>;
  skos:notation "7C1b";
  skos:prefLabel "(Nitrate + Nitrite)-N - steam distillation"@en .

s:7C1c a skos:Concept, sosa:Procedure;
  dct:description "(Ammonium + Nitrate + Nitrite)-N - steam distillation"@en;
  dct:identifier "http://registry.it.csiro.au/sandbox/soil/scma/7C1c"^^xsd:anyURI;
  dct:source "ISBN 9780643101364"@en;
  rdfs:label "(Ammonium + Nitrate + Nitrite)-N - steam distillation"@en;
  skos:broader s:7C1;
  skos:definition "(Ammonium + Nitrate + Nitrite)-N - steam distillation"@en;
  skos:inScheme <http://registry.it.csiro.au/sandbox/soil/scma/>;
  skos:notation "7C1c";
  skos:prefLabel "(Ammonium + Nitrate + Nitrite)-N - steam distillation"@en .

s:7C1d a skos:Concept, sosa:Procedure;
  dct:description "(Ammonium + Nitrate)-N, in presence of nitrite - steam distillation"@en;
  dct:identifier "http://registry.it.csiro.au/sandbox/soil/scma/7C1d"^^xsd:anyURI;
  dct:source "ISBN 9780643101364"@en;
  rdfs:label "(Ammonium + Nitrate)-N, in presence of nitrite - steam distillation"@en;
  skos:broader s:7C1;
  skos:definition "(Ammonium + Nitrate)-N, in presence of nitrite - steam distillation"@en;
  skos:inScheme <http://registry.it.csiro.au/sandbox/soil/scma/>;
  skos:notation "7C1d";
  skos:prefLabel "(Ammonium + Nitrate)-N, in presence of nitrite - steam distillation"@en .

s:7C1e a skos:Concept, sosa:Procedure;
  dct:description "Nitrate-N, in presence of nitrite - steam distillation"@en;
  dct:identifier "http://registry.it.csiro.au/sandbox/soil/scma/7C1e"^^xsd:anyURI;
  dct:source "ISBN 9780643101364"@en;
  rdfs:label "Nitrate-N, in presence of nitrite - steam distillation"@en;
  skos:broader s:7C1;
  skos:definition "Nitrate-N, in presence of nitrite - steam distillation"@en;
  skos:inScheme <http://registry.it.csiro.au/sandbox/soil/scma/>;
  skos:notation "7C1e";
  skos:prefLabel "Nitrate-N, in presence of nitrite - steam distillation"@en .

s:7C1f a skos:Concept, sosa:Procedure;
  dct:description "Nitrate-N, in absence of nitrite - steam distillation"@en;
  dct:identifier "http://registry.it.csiro.au/sandbox/soil/scma/7C1f"^^xsd:anyURI;
  dct:source "ISBN 9780643101364"@en;
  rdfs:label "Nitrate-N, in absence of nitrite - steam distillation"@en;
  skos:broader s:7C1;
  skos:definition "Nitrate-N, in absence of nitrite - steam distillation"@en;
  skos:inScheme <http://registry.it.csiro.au/sandbox/soil/scma/>;
  skos:notation "7C1f";
  skos:prefLabel "Nitrate-N, in absence of nitrite - steam distillation"@en .

s:7C1g a skos:Concept, sosa:Procedure;
  dct:description "(Ammonium + Nitrate)-N, in absence of nitrite - steam distillation"@en;
  dct:identifier "http://registry.it.csiro.au/sandbox/soil/scma/7C1g"^^xsd:anyURI;
  dct:source "ISBN 9780643101364"@en;
  rdfs:label "(Ammonium + Nitrate)-N, in absence of nitrite - steam distillation"@en;
  skos:broader s:7C1;
  skos:definition "(Ammonium + Nitrate)-N, in absence of nitrite - steam distillation"@en;
  skos:inScheme <http://registry.it.csiro.au/sandbox/soil/scma/>;
  skos:notation "7C1g";
  skos:prefLabel "(Ammonium + Nitrate)-N, in absence of nitrite - steam distillation"@en .

s:7C1h a skos:Concept, sosa:Procedure;
  dct:description "Nitrite-N - steam distillation"@en;
  dct:identifier "http://registry.it.csiro.au/sandbox/soil/scma/7C1h"^^xsd:anyURI;
  dct:source "ISBN 9780643101364"@en;
  rdfs:label "Nitrite-N - steam distillation"@en;
  skos:broader s:7C1;
  skos:definition "Nitrite-N - steam distillation"@en;
  skos:inScheme <http://registry.it.csiro.au/sandbox/soil/scma/>;
  skos:notation "7C1h";
  skos:prefLabel "Nitrite-N - steam distillation"@en .

s:7C2a a skos:Concept, sosa:Procedure;
  dct:description "Mineral-N 2 M KCl, automated colour, continuous segmented flow"@en;
  dct:identifier "http://registry.it.csiro.au/sandbox/soil/scma/7C2a"^^xsd:anyURI;
  dct:source "ISBN 9780643101364"@en;
  rdfs:label "Mineral-N 2 M KCl, automated colour, continuous segmented flow"@en;
  skos:broader s:7C2;
  skos:definition "Mineral-N 2 M KCl, automated colour, continuous segmented flow"@en;
  skos:inScheme <http://registry.it.csiro.au/sandbox/soil/scma/>;
  skos:notation "7C2a";
  skos:prefLabel "Mineral-N 2 M KCl, automated colour, continuous segmented flow"@en .

s:7C2b a skos:Concept, sosa:Procedure;
  dct:description "Mineral-N - 2 M KCl, automated colour, FIA"@en;
  dct:identifier "http://registry.it.csiro.au/sandbox/soil/scma/7C2b"^^xsd:anyURI;
  dct:source "ISBN 9780643101364"@en;
  rdfs:label "Mineral-N - 2 M KCl, automated colour, FIA"@en;
  skos:broader s:7C2;
  skos:definition "Mineral-N - 2 M KCl, automated colour, FIA"@en;
  skos:inScheme <http://registry.it.csiro.au/sandbox/soil/scma/>;
  skos:notation "7C2b";
  skos:prefLabel "Mineral-N - 2 M KCl, automated colour, FIA"@en .

s:7D1a a skos:Concept, sosa:Procedure;
  dct:description "Potentially mineralisable N, hot-KCl extraction (PMN KCl) - automated colour, continuous segmented flow"@en;
  dct:identifier "http://registry.it.csiro.au/sandbox/soil/scma/7D1a"^^xsd:anyURI;
  dct:source "ISBN 9780643101364"@en;
  rdfs:label "Potentially mineralisable N, hot-KCl extraction (PMN KCl) - automated colour, continuous segmented flow"@en;
  skos:broader s:7D;
  skos:definition "Potentially mineralisable N, hot-KCl extraction (PMN KCl) - automated colour, continuous segmented flow"@en;
  skos:inScheme <http://registry.it.csiro.au/sandbox/soil/scma/>;
  skos:notation "7D1a";
  skos:prefLabel "Potentially mineralisable N, hot-KCl extraction (PMN KCl) - automated colour, continuous segmented flow"@en .

s:7D1b a skos:Concept, sosa:Procedure;
  dct:description "Potentially mineralisable N, hot-KCl extraction (PMN KCl) - automated colour, FIA"@en;
  dct:identifier "http://registry.it.csiro.au/sandbox/soil/scma/7D1b"^^xsd:anyURI;
  dct:source "ISBN 9780643101364"@en;
  rdfs:label "Potentially mineralisable N, hot-KCl extraction (PMN KCl) - automated colour, FIA"@en;
  skos:broader s:7D;
  skos:definition "Potentially mineralisable N, hot-KCl extraction (PMN KCl) - automated colour, FIA"@en;
  skos:inScheme <http://registry.it.csiro.au/sandbox/soil/scma/>;
  skos:notation "7D1b";
  skos:prefLabel "Potentially mineralisable N, hot-KCl extraction (PMN KCl) - automated colour, FIA"@en .

s:7D1c a skos:Concept, sosa:Procedure;
  dct:description "Potentially mineralisable N, hot-KCl extraction (PMN KCl) - NIR diffuse reflectance spectroscopy"@en;
  dct:identifier "http://registry.it.csiro.au/sandbox/soil/scma/7D1c"^^xsd:anyURI;
  dct:source "ISBN 9780643101364"@en;
  rdfs:label "Potentially mineralisable N, hot-KCl extraction (PMN KCl) - NIR diffuse reflectance spectroscopy"@en;
  skos:broader s:7D;
  skos:definition "Potentially mineralisable N, hot-KCl extraction (PMN KCl) - NIR diffuse reflectance spectroscopy"@en;
  skos:inScheme <http://registry.it.csiro.au/sandbox/soil/scma/>;
  skos:notation "7D1c";
  skos:prefLabel "Potentially mineralisable N, hot-KCl extraction (PMN KCl) - NIR diffuse reflectance spectroscopy"@en .

s:7D2a a skos:Concept, sosa:Procedure;
  dct:description "Potentially mineralisable N, anaerobic incubation - automated colour, continuous segmented flow"@en;
  dct:identifier "http://registry.it.csiro.au/sandbox/soil/scma/7D2a"^^xsd:anyURI;
  dct:source "ISBN 9780643101364"@en;
  rdfs:label "Potentially mineralisable N, anaerobic incubation - automated colour, continuous segmented flow"@en;
  skos:broader s:7D;
  skos:definition "Potentially mineralisable N, anaerobic incubation - automated colour, continuous segmented flow"@en;
  skos:inScheme <http://registry.it.csiro.au/sandbox/soil/scma/>;
  skos:notation "7D2a";
  skos:prefLabel "Potentially mineralisable N, anaerobic incubation - automated colour, continuous segmented flow"@en .

s:7D2b a skos:Concept, sosa:Procedure;
  dct:description "Potentially mineralisable N, anaerobic incubation - automated colour, FIA"@en;
  dct:identifier "http://registry.it.csiro.au/sandbox/soil/scma/7D2b"^^xsd:anyURI;
  dct:source "ISBN 9780643101364"@en;
  rdfs:label "Potentially mineralisable N, anaerobic incubation - automated colour, FIA"@en;
  skos:broader s:7D;
  skos:definition "Potentially mineralisable N, anaerobic incubation - automated colour, FIA"@en;
  skos:inScheme <http://registry.it.csiro.au/sandbox/soil/scma/>;
  skos:notation "7D2b";
  skos:prefLabel "Potentially mineralisable N, anaerobic incubation - automated colour, FIA"@en .

s:8 a skos:Collection;
  dct:description "Carbon/nitrogen ratio"@en;
  dct:identifier "http://registry.it.csiro.au/sandbox/soil/scma/8"^^xsd:anyURI;
  dct:source "ISBN 9780643101364"@en;
  ui:topMemberOf <http://registry.it.csiro.au/sandbox/soil/scma>;
  rdfs:label "Carbon/nitrogen ratio"@en;
  skos:definition "Carbon/nitrogen ratio"@en;
  skos:inScheme <http://registry.it.csiro.au/sandbox/soil/scma/>;
  skos:notation "8";
  skos:prefLabel "Carbon/nitrogen ratio"@en .

s:8A1 a skos:Concept, sosa:Procedure;
  dct:description "Total organic carbon/total nitrogen ratio"@en;
  dct:identifier "http://registry.it.csiro.au/sandbox/soil/scma/8A1"^^xsd:anyURI;
  dct:source "ISBN 9780643101364"@en;
  rdfs:label "Total organic carbon/total nitrogen ratio"@en;
  skos:definition "Total organic carbon/total nitrogen ratio"@en;
  skos:inScheme <http://registry.it.csiro.au/sandbox/soil/scma/>;
  skos:member s:8;
  skos:notation "8A1";
  skos:prefLabel "Total organic carbon/total nitrogen ratio"@en;
  skos:topConceptOf <http://registry.it.csiro.au/sandbox/soil/scma/> .

s:8B1 a skos:Concept, sosa:Procedure;
  dct:description "Organic carbon - W&B/total nitrogen ratio"@en;
  dct:identifier "http://registry.it.csiro.au/sandbox/soil/scma/8B1"^^xsd:anyURI;
  dct:source "ISBN 9780643101364"@en;
  rdfs:label "Organic carbon - W&B/total nitrogen ratio"@en;
  skos:definition "Organic carbon - W&B/total nitrogen ratio"@en;
  skos:inScheme <http://registry.it.csiro.au/sandbox/soil/scma/>;
  skos:member s:8;
  skos:notation "8B1";
  skos:prefLabel "Organic carbon - W&B/total nitrogen ratio"@en;
  skos:topConceptOf <http://registry.it.csiro.au/sandbox/soil/scma/> .

s:9 a skos:Collection;
  dct:description "Phosphorus"@en;
  dct:identifier "http://registry.it.csiro.au/sandbox/soil/scma/9"^^xsd:anyURI;
  dct:source "ISBN 9780643101364"@en;
  ui:topMemberOf <http://registry.it.csiro.au/sandbox/soil/scma>;
  rdfs:label "Phosphorus"@en;
  skos:definition "Phosphorus"@en;
  skos:inScheme <http://registry.it.csiro.au/sandbox/soil/scma/>;
  skos:notation "9";
  skos:prefLabel "Phosphorus"@en .

s:9G2 a skos:Concept, sosa:Procedure;
  dct:description "Acid-extractable P (BSES-P) - continuous segmented flow/FIA automated colour"@en;
  dct:identifier "http://registry.it.csiro.au/sandbox/soil/scma/9G2"^^xsd:anyURI;
  dct:source "ISBN 9780643101364"@en;
  rdfs:label "Acid-extractable P (BSES-P) - continuous segmented flow/FIA automated colour"@en;
  skos:definition "Acid-extractable P (BSES-P) - continuous segmented flow/FIA automated colour"@en;
  skos:inScheme <http://registry.it.csiro.au/sandbox/soil/scma/>;
  skos:member s:9;
  skos:notation "9G2";
  skos:prefLabel "Acid-extractable P (BSES-P) - continuous segmented flow/FIA automated colour"@en;
  skos:topConceptOf <http://registry.it.csiro.au/sandbox/soil/scma/> .

s:9A a skos:Concept, sosa:Procedure;
  dct:description "Total P"@en;
  dct:identifier "http://registry.it.csiro.au/sandbox/soil/scma/9A"^^xsd:anyURI;
  dct:source "ISBN 9780643101364"@en;
  rdfs:label "Total P"@en;
  skos:definition "Total P"@en;
  skos:inScheme <http://registry.it.csiro.au/sandbox/soil/scma/>;
  skos:member s:9;
  skos:narrower s:9A1, s:9A2, s:9A3a, s:9A3b;
  skos:notation "9A";
  skos:prefLabel "Total P"@en;
  skos:topConceptOf <http://registry.it.csiro.au/sandbox/soil/scma/> .

s:9K a skos:Concept, sosa:Procedure;
  dct:description "Environmental soil P tests"@en;
  dct:identifier "http://registry.it.csiro.au/sandbox/soil/scma/9K"^^xsd:anyURI;
  dct:source "ISBN 9780643101364"@en;
  rdfs:label "Environmental soil P tests"@en;
  skos:definition "Environmental soil P tests"@en;
  skos:inScheme <http://registry.it.csiro.au/sandbox/soil/scma/>;
  skos:member s:9;
  skos:narrower s:9K1a, s:9K1b, s:9K2;
  skos:notation "9K";
  skos:prefLabel "Environmental soil P tests"@en;
  skos:topConceptOf <http://registry.it.csiro.au/sandbox/soil/scma/> .

s:9C a skos:Concept, sosa:Procedure;
  dct:description "Olsen-extractable P (Olsen-P)"@en;
  dct:identifier "http://registry.it.csiro.au/sandbox/soil/scma/9C"^^xsd:anyURI;
  dct:source "ISBN 9780643101364"@en;
  rdfs:label "Olsen-extractable P (Olsen-P)"@en;
  skos:definition "Olsen-extractable P (Olsen-P)"@en;
  skos:inScheme <http://registry.it.csiro.au/sandbox/soil/scma/>;
  skos:member s:9;
  skos:narrower s:9C1, s:9C2;
  skos:notation "9C";
  skos:prefLabel "Olsen-extractable P (Olsen-P)"@en;
  skos:topConceptOf <http://registry.it.csiro.au/sandbox/soil/scma/> .

s:9G1 a skos:Concept, sosa:Procedure;
  dct:description "Acid-extractable P (BSES-P) - manual colour"@en;
  dct:identifier "http://registry.it.csiro.au/sandbox/soil/scma/9G1"^^xsd:anyURI;
  dct:source "ISBN 9780643101364"@en;
  rdfs:label "Acid-extractable P (BSES-P) - manual colour"@en;
  skos:definition "Acid-extractable P (BSES-P) - manual colour"@en;
  skos:inScheme <http://registry.it.csiro.au/sandbox/soil/scma/>;
  skos:member s:9;
  skos:notation "9G1";
  skos:prefLabel "Acid-extractable P (BSES-P) - manual colour"@en;
  skos:topConceptOf <http://registry.it.csiro.au/sandbox/soil/scma/> .

s:9J a skos:Concept, sosa:Procedure;
  dct:description "Phosphate sorption curve"@en;
  dct:identifier "http://registry.it.csiro.au/sandbox/soil/scma/9J"^^xsd:anyURI;
  dct:source "ISBN 9780643101364"@en;
  rdfs:label "Phosphate sorption curve"@en;
  skos:definition "Phosphate sorption curve"@en;
  skos:inScheme <http://registry.it.csiro.au/sandbox/soil/scma/>;
  skos:member s:9;
  skos:narrower s:9J1, s:9J2;
  skos:notation "9J";
  skos:prefLabel "Phosphate sorption curve"@en;
  skos:topConceptOf <http://registry.it.csiro.au/sandbox/soil/scma/> .

s:9E a skos:Concept, sosa:Procedure;
  dct:description "Fluoride-extractable P (Bray-1 P)"@en;
  dct:identifier "http://registry.it.csiro.au/sandbox/soil/scma/9E"^^xsd:anyURI;
  dct:source "ISBN 9780643101364"@en;
  rdfs:label "Fluoride-extractable P (Bray-1 P)"@en;
  skos:definition "Fluoride-extractable P (Bray-1 P)"@en;
  skos:inScheme <http://registry.it.csiro.au/sandbox/soil/scma/>;
  skos:member s:9;
  skos:narrower s:9E1, s:9E2;
  skos:notation "9E";
  skos:prefLabel "Fluoride-extractable P (Bray-1 P)"@en;
  skos:topConceptOf <http://registry.it.csiro.au/sandbox/soil/scma/> .

s:9D1 a skos:Concept, sosa:Procedure;
  dct:description "Lactate-extractable P (Lactate-P) - manual colour"@en;
  dct:identifier "http://registry.it.csiro.au/sandbox/soil/scma/9D1"^^xsd:anyURI;
  dct:source "ISBN 9780643101364"@en;
  rdfs:label "Lactate-extractable P (Lactate-P) - manual colour"@en;
  skos:definition "Lactate-extractable P (Lactate-P) - manual colour"@en;
  skos:inScheme <http://registry.it.csiro.au/sandbox/soil/scma/>;
  skos:member s:9;
  skos:notation "9D1";
  skos:prefLabel "Lactate-extractable P (Lactate-P) - manual colour"@en;
  skos:topConceptOf <http://registry.it.csiro.au/sandbox/soil/scma/> .

s:9F2 a skos:Concept, sosa:Procedure;
  dct:description "Calcium chloride-extractable P - continuous segmented flow/FIA automated colour"@en;
  dct:identifier "http://registry.it.csiro.au/sandbox/soil/scma/9F2"^^xsd:anyURI;
  dct:source "ISBN 9780643101364"@en;
  rdfs:label "Calcium chloride-extractable P - continuous segmented flow/FIA automated colour"@en;
  skos:definition "Calcium chloride-extractable P - continuous segmented flow/FIA automated colour"@en;
  skos:inScheme <http://registry.it.csiro.au/sandbox/soil/scma/>;
  skos:member s:9;
  skos:notation "9F2";
  skos:prefLabel "Calcium chloride-extractable P - continuous segmented flow/FIA automated colour"@en;
  skos:topConceptOf <http://registry.it.csiro.au/sandbox/soil/scma/> .

s:9F1 a skos:Concept, sosa:Procedure;
  dct:description "Calcium chloride-extractable P - manual colour"@en;
  dct:identifier "http://registry.it.csiro.au/sandbox/soil/scma/9F1"^^xsd:anyURI;
  dct:source "ISBN 9780643101364"@en;
  rdfs:label "Calcium chloride-extractable P - manual colour"@en;
  skos:definition "Calcium chloride-extractable P - manual colour"@en;
  skos:inScheme <http://registry.it.csiro.au/sandbox/soil/scma/>;
  skos:member s:9;
  skos:notation "9F1";
  skos:prefLabel "Calcium chloride-extractable P - manual colour"@en;
  skos:topConceptOf <http://registry.it.csiro.au/sandbox/soil/scma/> .

s:9H1 a skos:Concept, sosa:Procedure;
  dct:description "Anion Storage Capacity (previously P Retention)"@en;
  dct:identifier "http://registry.it.csiro.au/sandbox/soil/scma/9H1"^^xsd:anyURI;
  dct:source "ISBN 9780643101364"@en;
  rdfs:label "Anion Storage Capacity (previously P Retention)"@en;
  skos:definition "Anion Storage Capacity (previously P Retention)"@en;
  skos:inScheme <http://registry.it.csiro.au/sandbox/soil/scma/>;
  skos:member s:9;
  skos:notation "9H1";
  skos:prefLabel "Anion Storage Capacity (previously P Retention)"@en;
  skos:topConceptOf <http://registry.it.csiro.au/sandbox/soil/scma/> .

s:9I a skos:Concept, sosa:Procedure;
  dct:description "Phosphate Indices"@en;
  dct:identifier "http://registry.it.csiro.au/sandbox/soil/scma/9I"^^xsd:anyURI;
  dct:source "ISBN 9780643101364"@en;
  rdfs:label "Phosphate Indices"@en;
  skos:definition "Phosphate Indices"@en;
  skos:inScheme <http://registry.it.csiro.au/sandbox/soil/scma/>;
  skos:member s:9;
  skos:narrower s:9I1, s:9I2a, s:9I2b, s:9I2c, s:9I3a, s:9I3b, s:9I3c, s:9I4a, s:9I4b,
    s:9I4c;
  skos:notation "9I";
  skos:prefLabel "Phosphate Indices"@en;
  skos:topConceptOf <http://registry.it.csiro.au/sandbox/soil/scma/> .

s:9B a skos:Concept, sosa:Procedure;
  dct:description "Bicarbonate-extractable P (Colwell-P)"@en;
  dct:identifier "http://registry.it.csiro.au/sandbox/soil/scma/9B"^^xsd:anyURI;
  dct:source "ISBN 9780643101364"@en;
  rdfs:label "Bicarbonate-extractable P (Colwell-P)"@en;
  skos:definition "Bicarbonate-extractable P (Colwell-P)"@en;
  skos:inScheme <http://registry.it.csiro.au/sandbox/soil/scma/>;
  skos:member s:9;
  skos:narrower s:9B1, s:9B2;
  skos:notation "9B";
  skos:prefLabel "Bicarbonate-extractable P (Colwell-P)"@en;
  skos:topConceptOf <http://registry.it.csiro.au/sandbox/soil/scma/> .

s:9A1 a skos:Concept, sosa:Procedure;
  dct:description "Total P - X-ray fluorescence"@en;
  dct:identifier "http://registry.it.csiro.au/sandbox/soil/scma/9A1"^^xsd:anyURI;
  dct:source "ISBN 9780643101364"@en;
  rdfs:label "Total P - X-ray fluorescence"@en;
  skos:broader s:9A;
  skos:definition "Total P - X-ray fluorescence"@en;
  skos:inScheme <http://registry.it.csiro.au/sandbox/soil/scma/>;
  skos:notation "9A1";
  skos:prefLabel "Total P - X-ray fluorescence"@en .

s:9A2 a skos:Concept, sosa:Procedure;
  dct:description "Total P - sodium carbonate fusion"@en;
  dct:identifier "http://registry.it.csiro.au/sandbox/soil/scma/9A2"^^xsd:anyURI;
  dct:source "ISBN 9780643101364"@en;
  rdfs:label "Total P - sodium carbonate fusion"@en;
  skos:broader s:9A;
  skos:definition "Total P - sodium carbonate fusion"@en;
  skos:inScheme <http://registry.it.csiro.au/sandbox/soil/scma/>;
  skos:notation "9A2";
  skos:prefLabel "Total P - sodium carbonate fusion"@en .

s:9A3a a skos:Concept, sosa:Procedure;
  dct:description "Kjeldahl P (KP) - automated colour, FIA/continuous segmented flow"@en;
  dct:identifier "http://registry.it.csiro.au/sandbox/soil/scma/9A3a"^^xsd:anyURI;
  dct:source "ISBN 9780643101364"@en;
  rdfs:label "Kjeldahl P (KP) - automated colour, FIA/continuous segmented flow"@en;
  skos:broader s:9A;
  skos:definition "Kjeldahl P (KP) - automated colour, FIA/continuous segmented flow"@en;
  skos:inScheme <http://registry.it.csiro.au/sandbox/soil/scma/>;
  skos:notation "9A3a";
  skos:prefLabel "Kjeldahl P (KP) - automated colour, FIA/continuous segmented flow"@en .

s:9A3b a skos:Concept, sosa:Procedure;
  dct:description "Kjeldahl P (KP) - ICPAES"@en;
  dct:identifier "http://registry.it.csiro.au/sandbox/soil/scma/9A3b"^^xsd:anyURI;
  dct:source "ISBN 9780643101364"@en;
  rdfs:label "Kjeldahl P (KP) - ICPAES"@en;
  skos:broader s:9A;
  skos:definition "Kjeldahl P (KP) - ICPAES"@en;
  skos:inScheme <http://registry.it.csiro.au/sandbox/soil/scma/>;
  skos:notation "9A3b";
  skos:prefLabel "Kjeldahl P (KP) - ICPAES"@en .

s:9B1 a skos:Concept, sosa:Procedure;
  dct:description "Bicarbonate-extractable P (Colwell-P) - manual colour"@en;
  dct:identifier "http://registry.it.csiro.au/sandbox/soil/scma/9B1"^^xsd:anyURI;
  dct:source "ISBN 9780643101364"@en;
  rdfs:label "Bicarbonate-extractable P (Colwell-P) - manual colour"@en;
  skos:broader s:9B;
  skos:definition "Bicarbonate-extractable P (Colwell-P) - manual colour"@en;
  skos:inScheme <http://registry.it.csiro.au/sandbox/soil/scma/>;
  skos:notation "9B1";
  skos:prefLabel "Bicarbonate-extractable P (Colwell-P) - manual colour"@en .

s:9B2 a skos:Concept, sosa:Procedure;
  dct:description "Bicarbonate-extractable P (Colwell-P) - automated colour, continuous segmented flow/FIA"@en;
  dct:identifier "http://registry.it.csiro.au/sandbox/soil/scma/9B2"^^xsd:anyURI;
  dct:source "ISBN 9780643101364"@en;
  rdfs:label "Bicarbonate-extractable P (Colwell-P) - automated colour, continuous segmented flow/FIA"@en;
  skos:broader s:9B;
  skos:definition "Bicarbonate-extractable P (Colwell-P) - automated colour, continuous segmented flow/FIA"@en;
  skos:inScheme <http://registry.it.csiro.au/sandbox/soil/scma/>;
  skos:notation "9B2";
  skos:prefLabel "Bicarbonate-extractable P (Colwell-P) - automated colour, continuous segmented flow/FIA"@en .

s:9C1 a skos:Concept, sosa:Procedure;
  dct:description "Olsen-extractable P (Olsen-P) - manual colour"@en;
  dct:identifier "http://registry.it.csiro.au/sandbox/soil/scma/9C1"^^xsd:anyURI;
  dct:source "ISBN 9780643101364"@en;
  rdfs:label "Olsen-extractable P (Olsen-P) - manual colour"@en;
  skos:broader s:9C;
  skos:definition "Olsen-extractable P (Olsen-P) - manual colour"@en;
  skos:inScheme <http://registry.it.csiro.au/sandbox/soil/scma/>;
  skos:notation "9C1";
  skos:prefLabel "Olsen-extractable P (Olsen-P) - manual colour"@en .

s:9C2 a skos:Concept, sosa:Procedure;
  dct:description "Olsen-extractable phosphorus - automated colour|Olsen-extractable P (Olsen-P) - automated colour"@en;
  dct:identifier "http://registry.it.csiro.au/sandbox/soil/scma/9C2"^^xsd:anyURI;
  dct:source "ISBN 0909605688"@en;
  rdfs:label "Olsen-extractable phosphorus - automated colour|Olsen-extractable P (Olsen-P) - automated colour"@en;
  skos:broader s:9C;
  skos:definition "Olsen-extractable phosphorus - automated colour|Olsen-extractable P (Olsen-P) - automated colour"@en;
  skos:inScheme <http://registry.it.csiro.au/sandbox/soil/scma/>;
  skos:narrower s:9C2a, s:9C2b;
  skos:notation "9C2";
  skos:note "9C2 has been superseded by 9C2a and 9C2b in Soil Chemical Methods Australasia, Rayment G.E. and Lyons D.J. ISBN 9780643101364"@en;
  skos:prefLabel "Olsen-extractable phosphorus - automated colour|Olsen-extractable P (Olsen-P) - automated colour"@en .

s:9C2a a skos:Concept, sosa:Procedure;
  dct:description "Olsen-extractable P (Olsen-P) - automated colour, continuous segmented flow"@en;
  dct:identifier "http://registry.it.csiro.au/sandbox/soil/scma/9C2a"^^xsd:anyURI;
  dct:source "ISBN 9780643101364"@en;
  rdfs:label "Olsen-extractable P (Olsen-P) - automated colour, continuous segmented flow"@en;
  skos:broader s:9C2;
  skos:definition "Olsen-extractable P (Olsen-P) - automated colour, continuous segmented flow"@en;
  skos:inScheme <http://registry.it.csiro.au/sandbox/soil/scma/>;
  skos:notation "9C2a";
  skos:prefLabel "Olsen-extractable P (Olsen-P) - automated colour, continuous segmented flow"@en .

s:9C2b a skos:Concept, sosa:Procedure;
  dct:description "Olsen-extractable P (Olsen-P) - automated colour/FIA"@en;
  dct:identifier "http://registry.it.csiro.au/sandbox/soil/scma/9C2b"^^xsd:anyURI;
  dct:source "ISBN 9780643101364"@en;
  rdfs:label "Olsen-extractable P (Olsen-P) - automated colour/FIA"@en;
  skos:broader s:9C2;
  skos:definition "Olsen-extractable P (Olsen-P) - automated colour/FIA"@en;
  skos:inScheme <http://registry.it.csiro.au/sandbox/soil/scma/>;
  skos:notation "9C2b";
  skos:prefLabel "Olsen-extractable P (Olsen-P) - automated colour/FIA"@en .

s:9E1 a skos:Concept, sosa:Procedure;
  dct:description "Fluoride-extractable P (Bray-1 P) - manual colour"@en;
  dct:identifier "http://registry.it.csiro.au/sandbox/soil/scma/9E1"^^xsd:anyURI;
  dct:source "ISBN 9780643101364"@en;
  rdfs:label "Fluoride-extractable P (Bray-1 P) - manual colour"@en;
  skos:broader s:9E;
  skos:definition "Fluoride-extractable P (Bray-1 P) - manual colour"@en;
  skos:inScheme <http://registry.it.csiro.au/sandbox/soil/scma/>;
  skos:notation "9E1";
  skos:prefLabel "Fluoride-extractable P (Bray-1 P) - manual colour"@en .

s:9E2 a skos:Concept, sosa:Procedure;
  dct:description "Fluoride-extractable P (Bray-1 P) - continuous segmented flow/FIA automated colour"@en;
  dct:identifier "http://registry.it.csiro.au/sandbox/soil/scma/9E2"^^xsd:anyURI;
  dct:source "ISBN 9780643101364"@en;
  rdfs:label "Fluoride-extractable P (Bray-1 P) - continuous segmented flow/FIA automated colour"@en;
  skos:broader s:9E;
  skos:definition "Fluoride-extractable P (Bray-1 P) - continuous segmented flow/FIA automated colour"@en;
  skos:inScheme <http://registry.it.csiro.au/sandbox/soil/scma/>;
  skos:notation "9E2";
  skos:prefLabel "Fluoride-extractable P (Bray-1 P) - continuous segmented flow/FIA automated colour"@en .

s:9I1 a skos:Concept, sosa:Procedure;
  dct:description "Phosphate Sorption Index"@en;
  dct:identifier "http://registry.it.csiro.au/sandbox/soil/scma/9I1"^^xsd:anyURI;
  dct:source "ISBN 9780643101364"@en;
  rdfs:label "Phosphate Sorption Index"@en;
  skos:broader s:9I;
  skos:definition "Phosphate Sorption Index"@en;
  skos:inScheme <http://registry.it.csiro.au/sandbox/soil/scma/>;
  skos:notation "9I1";
  skos:prefLabel "Phosphate Sorption Index"@en .

s:9I2a a skos:Concept, sosa:Procedure;
  dct:description "P buffer index - PBI (ColP) - Murphy and Riley|P buffer index - PBI (ColP)"@en;
  dct:identifier "http://registry.it.csiro.au/sandbox/soil/scma/9I2a"^^xsd:anyURI;
  dct:source "ISBN 9780643101364"@en;
  rdfs:label "P buffer index - PBI (ColP) - Murphy and Riley|P buffer index - PBI (ColP)"@en;
  skos:broader s:9I;
  skos:definition "P buffer index - PBI (ColP) - Murphy and Riley|P buffer index - PBI (ColP)"@en;
  skos:inScheme <http://registry.it.csiro.au/sandbox/soil/scma/>;
  skos:notation "9I2a";
  skos:prefLabel "P buffer index - PBI (ColP) - Murphy and Riley|P buffer index - PBI (ColP)"@en .

s:9I2b a skos:Concept, sosa:Procedure;
  dct:description "P buffer index - PBI (ColP)|P buffer index - PBI (ColP) - ICPAES"@en;
  dct:identifier "http://registry.it.csiro.au/sandbox/soil/scma/9I2b"^^xsd:anyURI;
  dct:source "ISBN 9780643101364"@en;
  rdfs:label "P buffer index - PBI (ColP)|P buffer index - PBI (ColP) - ICPAES"@en;
  skos:broader s:9I;
  skos:definition "P buffer index - PBI (ColP)|P buffer index - PBI (ColP) - ICPAES"@en;
  skos:inScheme <http://registry.it.csiro.au/sandbox/soil/scma/>;
  skos:notation "9I2b";
  skos:prefLabel "P buffer index - PBI (ColP)|P buffer index - PBI (ColP) - ICPAES"@en .

s:9I2c a skos:Concept, sosa:Procedure;
  dct:description "P buffer index - PBI (ColP)|P buffer index - PBI (ColP) - Vanadate"@en;
  dct:identifier "http://registry.it.csiro.au/sandbox/soil/scma/9I2c"^^xsd:anyURI;
  dct:source "ISBN 9780643101364"@en;
  rdfs:label "P buffer index - PBI (ColP)|P buffer index - PBI (ColP) - Vanadate"@en;
  skos:broader s:9I;
  skos:definition "P buffer index - PBI (ColP)|P buffer index - PBI (ColP) - Vanadate"@en;
  skos:inScheme <http://registry.it.csiro.au/sandbox/soil/scma/>;
  skos:notation "9I2c";
  skos:prefLabel "P buffer index - PBI (ColP)|P buffer index - PBI (ColP) - Vanadate"@en .

s:9I3a a skos:Concept, sosa:Procedure;
  dct:description "P buffer index - PBI (OlsenP)|P buffer index - PBI (OlsenP) - Murphy and Riley"@en;
  dct:identifier "http://registry.it.csiro.au/sandbox/soil/scma/9I3a"^^xsd:anyURI;
  dct:source "ISBN 9780643101364"@en;
  rdfs:label "P buffer index - PBI (OlsenP)|P buffer index - PBI (OlsenP) - Murphy and Riley"@en;
  skos:broader s:9I;
  skos:definition "P buffer index - PBI (OlsenP)|P buffer index - PBI (OlsenP) - Murphy and Riley"@en;
  skos:inScheme <http://registry.it.csiro.au/sandbox/soil/scma/>;
  skos:notation "9I3a";
  skos:prefLabel "P buffer index - PBI (OlsenP)|P buffer index - PBI (OlsenP) - Murphy and Riley"@en .

s:9I3b a skos:Concept, sosa:Procedure;
  dct:description "P buffer index - PBI (OlsenP)|P buffer index - PBI (OlsenP) - ICPAES"@en;
  dct:identifier "http://registry.it.csiro.au/sandbox/soil/scma/9I3b"^^xsd:anyURI;
  dct:source "ISBN 9780643101364"@en;
  rdfs:label "P buffer index - PBI (OlsenP)|P buffer index - PBI (OlsenP) - ICPAES"@en;
  skos:broader s:9I;
  skos:definition "P buffer index - PBI (OlsenP)|P buffer index - PBI (OlsenP) - ICPAES"@en;
  skos:inScheme <http://registry.it.csiro.au/sandbox/soil/scma/>;
  skos:notation "9I3b";
  skos:prefLabel "P buffer index - PBI (OlsenP)|P buffer index - PBI (OlsenP) - ICPAES"@en .

s:9I3c a skos:Concept, sosa:Procedure;
  dct:description "P buffer index - PBI (OlsenP)|P buffer index - PBI (OlsenP) - Vanadate"@en;
  dct:identifier "http://registry.it.csiro.au/sandbox/soil/scma/9I3c"^^xsd:anyURI;
  dct:source "ISBN 9780643101364"@en;
  rdfs:label "P buffer index - PBI (OlsenP)|P buffer index - PBI (OlsenP) - Vanadate"@en;
  skos:broader s:9I;
  skos:definition "P buffer index - PBI (OlsenP)|P buffer index - PBI (OlsenP) - Vanadate"@en;
  skos:inScheme <http://registry.it.csiro.au/sandbox/soil/scma/>;
  skos:notation "9I3c";
  skos:prefLabel "P buffer index - PBI (OlsenP)|P buffer index - PBI (OlsenP) - Vanadate"@en .

s:9I4a a skos:Concept, sosa:Procedure;
  dct:description "P buffer index - PBI (unadj) - Murphy and Riley|P buffer index - PBI (unadj)"@en;
  dct:identifier "http://registry.it.csiro.au/sandbox/soil/scma/9I4a"^^xsd:anyURI;
  dct:source "ISBN 9780643101364"@en;
  rdfs:label "P buffer index - PBI (unadj) - Murphy and Riley|P buffer index - PBI (unadj)"@en;
  skos:broader s:9I;
  skos:definition "P buffer index - PBI (unadj) - Murphy and Riley|P buffer index - PBI (unadj)"@en;
  skos:inScheme <http://registry.it.csiro.au/sandbox/soil/scma/>;
  skos:notation "9I4a";
  skos:prefLabel "P buffer index - PBI (unadj) - Murphy and Riley|P buffer index - PBI (unadj)"@en .

s:9I4b a skos:Concept, sosa:Procedure;
  dct:description "P buffer index - PBI (unadj) - ICPAES|P buffer index - PBI (unadj)"@en;
  dct:identifier "http://registry.it.csiro.au/sandbox/soil/scma/9I4b"^^xsd:anyURI;
  dct:source "ISBN 9780643101364"@en;
  rdfs:label "P buffer index - PBI (unadj) - ICPAES|P buffer index - PBI (unadj)"@en;
  skos:broader s:9I;
  skos:definition "P buffer index - PBI (unadj) - ICPAES|P buffer index - PBI (unadj)"@en;
  skos:inScheme <http://registry.it.csiro.au/sandbox/soil/scma/>;
  skos:notation "9I4b";
  skos:prefLabel "P buffer index - PBI (unadj) - ICPAES|P buffer index - PBI (unadj)"@en .

s:9I4c a skos:Concept, sosa:Procedure;
  dct:description "P buffer index - PBI (unadj)|P buffer index - PBI (unadj) - Vanadate"@en;
  dct:identifier "http://registry.it.csiro.au/sandbox/soil/scma/9I4c"^^xsd:anyURI;
  dct:source "ISBN 9780643101364"@en;
  rdfs:label "P buffer index - PBI (unadj)|P buffer index - PBI (unadj) - Vanadate"@en;
  skos:broader s:9I;
  skos:definition "P buffer index - PBI (unadj)|P buffer index - PBI (unadj) - Vanadate"@en;
  skos:inScheme <http://registry.it.csiro.au/sandbox/soil/scma/>;
  skos:notation "9I4c";
  skos:prefLabel "P buffer index - PBI (unadj)|P buffer index - PBI (unadj) - Vanadate"@en .

s:9J1 a skos:Concept, sosa:Procedure;
  dct:description "Phosphate sorption curve - manual colour"@en;
  dct:identifier "http://registry.it.csiro.au/sandbox/soil/scma/9J1"^^xsd:anyURI;
  dct:source "ISBN 9780643101364"@en;
  rdfs:label "Phosphate sorption curve - manual colour"@en;
  skos:broader s:9J;
  skos:definition "Phosphate sorption curve - manual colour"@en;
  skos:inScheme <http://registry.it.csiro.au/sandbox/soil/scma/>;
  skos:notation "9J1";
  skos:prefLabel "Phosphate sorption curve - manual colour"@en .

s:9J2 a skos:Concept, sosa:Procedure;
  dct:description "Phosphate sorption curve - continuous segmented flow/FIA automated colour"@en;
  dct:identifier "http://registry.it.csiro.au/sandbox/soil/scma/9J2"^^xsd:anyURI;
  dct:source "ISBN 9780643101364"@en;
  rdfs:label "Phosphate sorption curve - continuous segmented flow/FIA automated colour"@en;
  skos:broader s:9J;
  skos:definition "Phosphate sorption curve - continuous segmented flow/FIA automated colour"@en;
  skos:inScheme <http://registry.it.csiro.au/sandbox/soil/scma/>;
  skos:notation "9J2";
  skos:prefLabel "Phosphate sorption curve - continuous segmented flow/FIA automated colour"@en .

s:9K1a a skos:Concept, sosa:Procedure;
  dct:description "Mehlich 3-P saturation ratio (M3PSR colour) [colormetric estimate of P]"@en;
  dct:identifier "http://registry.it.csiro.au/sandbox/soil/scma/9K1a"^^xsd:anyURI;
  dct:source "ISBN 9780643101364"@en;
  rdfs:label "Mehlich 3-P saturation ratio (M3PSR colour) [colormetric estimate of P]"@en;
  skos:broader s:9K;
  skos:definition "Mehlich 3-P saturation ratio (M3PSR colour) [colormetric estimate of P]"@en;
  skos:inScheme <http://registry.it.csiro.au/sandbox/soil/scma/>;
  skos:notation "9K1a";
  skos:prefLabel "Mehlich 3-P saturation ratio (M3PSR colour) [colormetric estimate of P]"@en .

s:9K1b a skos:Concept, sosa:Procedure;
  dct:description "Mehlich 3-P saturation ratio (M3PSR ICPAES) [ICPAES estimate of P]"@en;
  dct:identifier "http://registry.it.csiro.au/sandbox/soil/scma/9K1b"^^xsd:anyURI;
  dct:source "ISBN 9780643101364"@en;
  rdfs:label "Mehlich 3-P saturation ratio (M3PSR ICPAES) [ICPAES estimate of P]"@en;
  skos:broader s:9K;
  skos:definition "Mehlich 3-P saturation ratio (M3PSR ICPAES) [ICPAES estimate of P]"@en;
  skos:inScheme <http://registry.it.csiro.au/sandbox/soil/scma/>;
  skos:notation "9K1b";
  skos:prefLabel "Mehlich 3-P saturation ratio (M3PSR ICPAES) [ICPAES estimate of P]"@en .

s:9K2 a skos:Concept, sosa:Procedure;
  dct:description "Colwell-P/PBI (ColP) ratio"@en;
  dct:identifier "http://registry.it.csiro.au/sandbox/soil/scma/9K2"^^xsd:anyURI;
  dct:source "ISBN 9780643101364"@en;
  rdfs:label "Colwell-P/PBI (ColP) ratio"@en;
  skos:broader s:9K;
  skos:definition "Colwell-P/PBI (ColP) ratio"@en;
  skos:inScheme <http://registry.it.csiro.au/sandbox/soil/scma/>;
  skos:notation "9K2";
  skos:prefLabel "Colwell-P/PBI (ColP) ratio"@en .
